@prefix rdf: <http://www.w3.org/1999/02/22-rdf-syntax-ns#> .
@prefix owl: <http://www.w3.org/2002/07/owl#> .
@prefix xsd: <http://www.w3.org/2001/XMLSchema#> .
@prefix skos: <http://www.w3.org/2004/02/skos/core#> .
@prefix rdfs: <http://www.w3.org/2000/01/rdf-schema#> .
@prefix foaf: <http://xmlns.com/foaf/0.1/> .
@prefix dc: <http://purl.org/dc/elements/1.1/> .


<https://acdh.oeaw.ac.at/vocabs/defcthesaurus/FindsSchema> a skos:ConceptScheme ;
	rdfs:comment "A schema of concepts related to class Finds and their relationships in database." .

<https://acdh.oeaw.ac.at/vocabs/defcthesaurus/NotInDatabase> a skos:ConceptScheme ;
	rdfs:comment "A concept schema related to the particular finds properties." .

<https://acdh.oeaw.ac.at/vocabs/defcthesaurus/finds_material/1.01> a skos:Concept ;
	skos:prefLabel "finds material"@en , "Fundmaterial"@de ;
	skos:definition "A material from which an archaeological artefact (small finds, lithics) were made of." ;
	skos:inScheme <https://acdh.oeaw.ac.at/vocabs/defcthesaurus/FindsSchema> , <https://acdh.oeaw.ac.at/vocabs/defcthesaurus/NotInDatabase> ;
	skos:editorialNote "dc_not_in_database;01" .

<https://acdh.oeaw.ac.at/vocabs/defcthesaurus/FindsMaterial> a skos:ConceptScheme ;
	rdfs:comment "A concept schema related to the particular finds properties." .

<https://acdh.oeaw.ac.at/vocabs/defcthesaurus/stone/2.1> a skos:Concept ;
	skos:prefLabel "stone"@en , "Stein"@de , "Stein"@la ;
	skos:altLabel "rock"@en ;
	skos:definition "Different kinds of stone used to produce small finds and lithics." ;
	skos:inScheme <https://acdh.oeaw.ac.at/vocabs/defcthesaurus/FindsSchema> , <https://acdh.oeaw.ac.at/vocabs/defcthesaurus/FindsMaterial> ;
	skos:editorialNote "dc_finds_material;1" ;
	skos:broader <https://acdh.oeaw.ac.at/vocabs/defcthesaurus/finds_material/1.01> .

<https://acdh.oeaw.ac.at/vocabs/defcthesaurus/finds_material/1.01> skos:narrower <https://acdh.oeaw.ac.at/vocabs/defcthesaurus/stone/2.1> .

<https://acdh.oeaw.ac.at/vocabs/defcthesaurus/obsidian/3.2> a skos:Concept ;
	skos:prefLabel "obsidian"@en , "Obsidian"@de ;
	skos:definition "Obsidian, natural glass of volcanic origin that is formed by the rapid cooling of viscous lava. Obsidian is extremely rich in silica, low in water, and has a chemical composition similar to rhyolite." ;
	skos:inScheme <https://acdh.oeaw.ac.at/vocabs/defcthesaurus/FindsSchema> , <https://acdh.oeaw.ac.at/vocabs/defcthesaurus/FindsMaterial> ;
	skos:editorialNote "dc_finds_material;2" ;
	skos:broader <https://acdh.oeaw.ac.at/vocabs/defcthesaurus/stone/2.1> .

<https://acdh.oeaw.ac.at/vocabs/defcthesaurus/stone/2.1> skos:narrower <https://acdh.oeaw.ac.at/vocabs/defcthesaurus/obsidian/3.2> .

<https://acdh.oeaw.ac.at/vocabs/defcthesaurus/chert/3.12> a skos:Concept ;
	skos:prefLabel "chert"@en , "Kieselschiefer"@de ;
	skos:altLabel "Gestein"@de ;
	skos:definition "Chert is a very fine-grained quarz and a silica mineral. Several varieties are included under the general term: jasper, chalcedony, agate, flint, porcelanite, and novaculite. In Neolithic it was used for tools and weapon." ;
	skos:inScheme <https://acdh.oeaw.ac.at/vocabs/defcthesaurus/FindsSchema> , <https://acdh.oeaw.ac.at/vocabs/defcthesaurus/FindsMaterial> ;
	skos:editorialNote "dc_finds_material;12" ;
	skos:broader <https://acdh.oeaw.ac.at/vocabs/defcthesaurus/stone/2.1> .

<https://acdh.oeaw.ac.at/vocabs/defcthesaurus/stone/2.1> skos:narrower <https://acdh.oeaw.ac.at/vocabs/defcthesaurus/chert/3.12> ;
	dc:source "Encyclopaedia Britannica - https://www.britannica.com/science/chert#ref272901" .

<https://acdh.oeaw.ac.at/vocabs/defcthesaurus/flint/4.11> a skos:Concept ;
	skos:prefLabel "flint"@en , "Flint"@de ;
	skos:definition "Flint os a fine-grained quarz and a silica mineral included under the general term chert. In Neolithic it was used as material source for tools and weapons." ;
	skos:inScheme <https://acdh.oeaw.ac.at/vocabs/defcthesaurus/FindsSchema> , <https://acdh.oeaw.ac.at/vocabs/defcthesaurus/FindsMaterial> ;
	skos:editorialNote "dc_finds_material;11" ;
	skos:broader <https://acdh.oeaw.ac.at/vocabs/defcthesaurus/chert/3.12> .

<https://acdh.oeaw.ac.at/vocabs/defcthesaurus/chert/3.12> skos:narrower <https://acdh.oeaw.ac.at/vocabs/defcthesaurus/flint/4.11> .

<https://acdh.oeaw.ac.at/vocabs/defcthesaurus/stone/2.1> dc:source "https://en.wikipedia.org/wiki/Radiolarite" .

<https://acdh.oeaw.ac.at/vocabs/defcthesaurus/radiolarite/4.18> a skos:Concept ;
	skos:prefLabel "radiolarite"@en , "Radiolarit"@de ;
	skos:definition "Radiolarite is a siliceous, comparatively hard, fine-grained, chert-like, and homogeneous sedimentary rock that is composed predominantly of the microscopic remains of radiolarians used to make stone tools and weapons." ;
	skos:inScheme <https://acdh.oeaw.ac.at/vocabs/defcthesaurus/FindsSchema> , <https://acdh.oeaw.ac.at/vocabs/defcthesaurus/FindsMaterial> ;
	skos:editorialNote "dc_finds_material;18" ;
	skos:broader <https://acdh.oeaw.ac.at/vocabs/defcthesaurus/chert/3.12> .

<https://acdh.oeaw.ac.at/vocabs/defcthesaurus/chert/3.12> skos:narrower <https://acdh.oeaw.ac.at/vocabs/defcthesaurus/radiolarite/4.18> .

<https://acdh.oeaw.ac.at/vocabs/defcthesaurus/chalcedony/3.13> a skos:Concept ;
	skos:prefLabel "chalcedony"@en , "Chalzedon"@de ;
	skos:definition "A very fine-grained (cryptocrystalline) variety of the silica mineral quartz. A form of chert, it occurs in concretionary, mammillated, or stalactitic forms of waxy lustre and has a compact fibrous structure, a fine splintery fracture." ;
	skos:inScheme <https://acdh.oeaw.ac.at/vocabs/defcthesaurus/FindsSchema> , <https://acdh.oeaw.ac.at/vocabs/defcthesaurus/FindsMaterial> ;
	skos:editorialNote "dc_finds_material;13" ;
	skos:broader <https://acdh.oeaw.ac.at/vocabs/defcthesaurus/stone/2.1> .

<https://acdh.oeaw.ac.at/vocabs/defcthesaurus/stone/2.1> skos:narrower <https://acdh.oeaw.ac.at/vocabs/defcthesaurus/chalcedony/3.13> .

<https://acdh.oeaw.ac.at/vocabs/defcthesaurus/jasper/3.14> a skos:Concept ;
	skos:prefLabel "jasper"@en , "Jaspis"@de ;
	skos:definition "An opaque, fine-grained or dense variety of the silica mineral chert that exhibits various colours. Chiefly brick red to brownish red, it owes its colour to admixed hematite; but when it occurs with clay admixed, the colour is a yellowish white or gray, o" ;
	skos:inScheme <https://acdh.oeaw.ac.at/vocabs/defcthesaurus/FindsSchema> , <https://acdh.oeaw.ac.at/vocabs/defcthesaurus/FindsMaterial> ;
	skos:editorialNote "dc_finds_material;14" ;
	skos:broader <https://acdh.oeaw.ac.at/vocabs/defcthesaurus/stone/2.1> .

<https://acdh.oeaw.ac.at/vocabs/defcthesaurus/stone/2.1> skos:narrower <https://acdh.oeaw.ac.at/vocabs/defcthesaurus/jasper/3.14> .

<https://acdh.oeaw.ac.at/vocabs/defcthesaurus/quartz/3.15> a skos:Concept ;
	skos:prefLabel "quartz"@en ;
	skos:definition "Widely distributed mineral of many varieties that consists primarily of silica, or silicon dioxide (SiO2)." ;
	skos:inScheme <https://acdh.oeaw.ac.at/vocabs/defcthesaurus/FindsSchema> , <https://acdh.oeaw.ac.at/vocabs/defcthesaurus/FindsMaterial> ;
	skos:editorialNote "dc_finds_material;15" ;
	skos:broader <https://acdh.oeaw.ac.at/vocabs/defcthesaurus/stone/2.1> .

<https://acdh.oeaw.ac.at/vocabs/defcthesaurus/stone/2.1> skos:narrower <https://acdh.oeaw.ac.at/vocabs/defcthesaurus/quartz/3.15> .

<https://acdh.oeaw.ac.at/vocabs/defcthesaurus/quarzite/3.17> a skos:Concept ;
	skos:prefLabel "quarzite"@en , "Quarzit"@de ;
	skos:definition "A sandstone that has been converted into a solid quartz rock. Unlike sandstones, quartzites are free from pores and have a smooth fracture;" ;
	skos:inScheme <https://acdh.oeaw.ac.at/vocabs/defcthesaurus/FindsSchema> , <https://acdh.oeaw.ac.at/vocabs/defcthesaurus/FindsMaterial> ;
	skos:editorialNote "dc_finds_material;17" ;
	skos:broader <https://acdh.oeaw.ac.at/vocabs/defcthesaurus/stone/2.1> .

<https://acdh.oeaw.ac.at/vocabs/defcthesaurus/stone/2.1> skos:narrower <https://acdh.oeaw.ac.at/vocabs/defcthesaurus/quarzite/3.17> .

<https://acdh.oeaw.ac.at/vocabs/defcthesaurus/marble/3.10> a skos:Concept ;
	skos:prefLabel "marble"@en , "Marmor"@de ;
	skos:definition "Marble is a non-foliated metamorphic rock composed of recrystallized carbonate minerals, most commonly calcite or dolomite." ;
	skos:inScheme <https://acdh.oeaw.ac.at/vocabs/defcthesaurus/FindsSchema> , <https://acdh.oeaw.ac.at/vocabs/defcthesaurus/FindsMaterial> ;
	skos:editorialNote "dc_finds_material;10" ;
	skos:broader <https://acdh.oeaw.ac.at/vocabs/defcthesaurus/stone/2.1> .

<https://acdh.oeaw.ac.at/vocabs/defcthesaurus/stone/2.1> skos:narrower <https://acdh.oeaw.ac.at/vocabs/defcthesaurus/marble/3.10> .

<https://acdh.oeaw.ac.at/vocabs/defcthesaurus/basalt/3.20> a skos:Concept ;
	skos:prefLabel "basalt"@en , "Basalt"@de ;
	skos:definition "A common extrusive igneous (volcanic) rock formed from the rapid cooling of basaltic lava exposed at or very near the surface." ;
	skos:inScheme <https://acdh.oeaw.ac.at/vocabs/defcthesaurus/FindsSchema> , <https://acdh.oeaw.ac.at/vocabs/defcthesaurus/FindsMaterial> ;
	skos:editorialNote "dc_finds_material;20" ;
	skos:broader <https://acdh.oeaw.ac.at/vocabs/defcthesaurus/stone/2.1> .

<https://acdh.oeaw.ac.at/vocabs/defcthesaurus/stone/2.1> skos:narrower <https://acdh.oeaw.ac.at/vocabs/defcthesaurus/basalt/3.20> .

<https://acdh.oeaw.ac.at/vocabs/defcthesaurus/limestone/3.22> a skos:Concept ;
	skos:prefLabel "limestone"@en , "Kalkstein"@de ;
	skos:definition "Limestone is a sedimentary rock composed largely of the minerals calcite and aragonite, which are different crystal forms of calcium carbonate (CaCO3).  Used as a building material or production of smaller objects." ;
	skos:inScheme <https://acdh.oeaw.ac.at/vocabs/defcthesaurus/FindsSchema> , <https://acdh.oeaw.ac.at/vocabs/defcthesaurus/FindsMaterial> ;
	skos:editorialNote "dc_finds_material;22" ;
	skos:broader <https://acdh.oeaw.ac.at/vocabs/defcthesaurus/stone/2.1> .

<https://acdh.oeaw.ac.at/vocabs/defcthesaurus/stone/2.1> skos:narrower <https://acdh.oeaw.ac.at/vocabs/defcthesaurus/limestone/3.22> .

<https://acdh.oeaw.ac.at/vocabs/defcthesaurus/granite/3.24> a skos:Concept ;
	skos:prefLabel "granite"@en , "Granit"@de ;
	skos:definition "A common type of felsic intrusive igneous rock that is granular and phaneritic in texture. Granites can be predominantly white, pink, or gray in color, depending on their mineralogy." ;
	skos:inScheme <https://acdh.oeaw.ac.at/vocabs/defcthesaurus/FindsSchema> , <https://acdh.oeaw.ac.at/vocabs/defcthesaurus/FindsMaterial> ;
	skos:editorialNote "dc_finds_material;24" ;
	skos:broader <https://acdh.oeaw.ac.at/vocabs/defcthesaurus/stone/2.1> .

<https://acdh.oeaw.ac.at/vocabs/defcthesaurus/stone/2.1> skos:narrower <https://acdh.oeaw.ac.at/vocabs/defcthesaurus/granite/3.24> .

<https://acdh.oeaw.ac.at/vocabs/defcthesaurus/sandstone/3.25> a skos:Concept ;
	skos:prefLabel "sandstone"@en , "Sandstein"@de ;
	skos:definition "Sandstone (sometimes known as arenite) is a clastic sedimentary rock composed mainly of sand-sized minerals or rock grains." ;
	skos:inScheme <https://acdh.oeaw.ac.at/vocabs/defcthesaurus/FindsSchema> , <https://acdh.oeaw.ac.at/vocabs/defcthesaurus/FindsMaterial> ;
	skos:editorialNote "dc_finds_material;25" ;
	skos:broader <https://acdh.oeaw.ac.at/vocabs/defcthesaurus/stone/2.1> .

<https://acdh.oeaw.ac.at/vocabs/defcthesaurus/stone/2.1> skos:narrower <https://acdh.oeaw.ac.at/vocabs/defcthesaurus/sandstone/3.25> .

<https://acdh.oeaw.ac.at/vocabs/defcthesaurus/schist/3.26> a skos:Concept ;
	skos:prefLabel "schist"@en , "Glimmerschiefer"@de ;
	skos:definition "A medium-grade metamorphic rock with medium to large, flat, sheet-like grains in a preferred orientation (nearby grains are roughly parallel). It is defined by having more than 50% platy and elongated minerals, often finely interleaved with quartz and fel" ;
	skos:inScheme <https://acdh.oeaw.ac.at/vocabs/defcthesaurus/FindsSchema> , <https://acdh.oeaw.ac.at/vocabs/defcthesaurus/FindsMaterial> ;
	skos:editorialNote "dc_finds_material;26" ;
	skos:broader <https://acdh.oeaw.ac.at/vocabs/defcthesaurus/stone/2.1> .

<https://acdh.oeaw.ac.at/vocabs/defcthesaurus/stone/2.1> skos:narrower <https://acdh.oeaw.ac.at/vocabs/defcthesaurus/schist/3.26> .

<https://acdh.oeaw.ac.at/vocabs/defcthesaurus/agate/3.27> a skos:Concept ;
	skos:prefLabel "agate"@en , "Achat"@de ;
	skos:definition "Cryptocrystalline variety of silica, chiefly chalcedony, characterised by its fineness of grain and brightness of color." ;
	skos:inScheme <https://acdh.oeaw.ac.at/vocabs/defcthesaurus/FindsSchema> , <https://acdh.oeaw.ac.at/vocabs/defcthesaurus/FindsMaterial> ;
	skos:editorialNote "dc_finds_material;27" ;
	skos:broader <https://acdh.oeaw.ac.at/vocabs/defcthesaurus/stone/2.1> .

<https://acdh.oeaw.ac.at/vocabs/defcthesaurus/stone/2.1> skos:narrower <https://acdh.oeaw.ac.at/vocabs/defcthesaurus/agate/3.27> .

<https://acdh.oeaw.ac.at/vocabs/defcthesaurus/andesit/3.29> a skos:Concept ;
	skos:prefLabel "andesit"@en , "Andesit"@de ;
	skos:definition "An extrusive igneous, volcanic rock, of intermediate composition, with aphanitic to porphyritic texture." ;
	skos:inScheme <https://acdh.oeaw.ac.at/vocabs/defcthesaurus/FindsSchema> , <https://acdh.oeaw.ac.at/vocabs/defcthesaurus/FindsMaterial> ;
	skos:editorialNote "dc_finds_material;29" ;
	skos:broader <https://acdh.oeaw.ac.at/vocabs/defcthesaurus/stone/2.1> .

<https://acdh.oeaw.ac.at/vocabs/defcthesaurus/stone/2.1> skos:narrower <https://acdh.oeaw.ac.at/vocabs/defcthesaurus/andesit/3.29> .

<https://acdh.oeaw.ac.at/vocabs/defcthesaurus/porphyry/3.30> a skos:Concept ;
	skos:prefLabel "porphyry"@en , "Porphyr"@de ;
	skos:definition "Porphyry is a textural term for an igneous rock consisting of large-grained crystals such as feldspar or quartz dispersed in a fine-grained feldspathic matrix or groundmass." ;
	skos:inScheme <https://acdh.oeaw.ac.at/vocabs/defcthesaurus/FindsSchema> , <https://acdh.oeaw.ac.at/vocabs/defcthesaurus/FindsMaterial> ;
	skos:editorialNote "dc_finds_material;30" ;
	skos:broader <https://acdh.oeaw.ac.at/vocabs/defcthesaurus/stone/2.1> .

<https://acdh.oeaw.ac.at/vocabs/defcthesaurus/stone/2.1> skos:narrower <https://acdh.oeaw.ac.at/vocabs/defcthesaurus/porphyry/3.30> .

<https://acdh.oeaw.ac.at/vocabs/defcthesaurus/green_stone/3.33> a skos:Concept ;
	skos:prefLabel "green stone"@en , "Gr체nstein"@de ;
	skos:altLabel "jade"@en , "Jade"@de ;
	skos:inScheme <https://acdh.oeaw.ac.at/vocabs/defcthesaurus/FindsSchema> , <https://acdh.oeaw.ac.at/vocabs/defcthesaurus/FindsMaterial> ;
	skos:editorialNote "dc_finds_material;33" ;
	skos:broader <https://acdh.oeaw.ac.at/vocabs/defcthesaurus/stone/2.1> .

<https://acdh.oeaw.ac.at/vocabs/defcthesaurus/stone/2.1> skos:narrower <https://acdh.oeaw.ac.at/vocabs/defcthesaurus/green_stone/3.33> .

<https://acdh.oeaw.ac.at/vocabs/defcthesaurus/metal/2.9> a skos:Concept ;
	skos:prefLabel "metal"@en , "Metall"@de , "Metall"@la ;
	skos:definition "A solid material which is typically hard, shiny, malleable, fusible, and ductile, with good thermal conductivity (e.g. iron, gold, silver, steel)." ;
	skos:inScheme <https://acdh.oeaw.ac.at/vocabs/defcthesaurus/FindsSchema> , <https://acdh.oeaw.ac.at/vocabs/defcthesaurus/FindsMaterial> ;
	skos:editorialNote "dc_finds_material;9" ;
	skos:broader <https://acdh.oeaw.ac.at/vocabs/defcthesaurus/finds_material/1.01> .

<https://acdh.oeaw.ac.at/vocabs/defcthesaurus/finds_material/1.01> skos:narrower <https://acdh.oeaw.ac.at/vocabs/defcthesaurus/metal/2.9> .

<https://acdh.oeaw.ac.at/vocabs/defcthesaurus/copper/3.31> a skos:Concept ;
	skos:prefLabel "copper"@en , "Kupfer"@de ;
	skos:definition "Copper (Cu) is a reddish, extremely ductile metal that can be found in the free metallic state in nature." ;
	skos:inScheme <https://acdh.oeaw.ac.at/vocabs/defcthesaurus/FindsSchema> , <https://acdh.oeaw.ac.at/vocabs/defcthesaurus/FindsMaterial> ;
	skos:editorialNote "dc_finds_material;31" ;
	skos:broader <https://acdh.oeaw.ac.at/vocabs/defcthesaurus/metal/2.9> .

<https://acdh.oeaw.ac.at/vocabs/defcthesaurus/metal/2.9> skos:narrower <https://acdh.oeaw.ac.at/vocabs/defcthesaurus/copper/3.31> .

<https://acdh.oeaw.ac.at/vocabs/defcthesaurus/gold/3.34> a skos:Concept ;
	skos:prefLabel "gold"@en , "Gold"@de ;
	skos:definition "Gold is a chemical element with symbol Au (from Latin: aurum) and atomic number 79. In its purest form, it is a bright, slightly reddish yellow, dense, soft, malleable and ductile metal." ;
	skos:inScheme <https://acdh.oeaw.ac.at/vocabs/defcthesaurus/FindsSchema> , <https://acdh.oeaw.ac.at/vocabs/defcthesaurus/FindsMaterial> ;
	skos:editorialNote "dc_finds_material;34" ;
	skos:broader <https://acdh.oeaw.ac.at/vocabs/defcthesaurus/metal/2.9> .

<https://acdh.oeaw.ac.at/vocabs/defcthesaurus/metal/2.9> skos:narrower <https://acdh.oeaw.ac.at/vocabs/defcthesaurus/gold/3.34> .

<https://acdh.oeaw.ac.at/vocabs/defcthesaurus/mineral/2.03> a skos:Concept ;
	skos:prefLabel "mineral"@en , "Mineral"@de , "Mineral"@la ;
	skos:definition "Different kinds of minerals used to produce small finds and lithics." ;
	skos:inScheme <https://acdh.oeaw.ac.at/vocabs/defcthesaurus/FindsSchema> , <https://acdh.oeaw.ac.at/vocabs/defcthesaurus/NotInDatabase> ;
	skos:editorialNote "dc_not_in_database;03" ;
	skos:broader <https://acdh.oeaw.ac.at/vocabs/defcthesaurus/finds_material/1.01> .

<https://acdh.oeaw.ac.at/vocabs/defcthesaurus/finds_material/1.01> skos:narrower <https://acdh.oeaw.ac.at/vocabs/defcthesaurus/mineral/2.03> .

<https://acdh.oeaw.ac.at/vocabs/defcthesaurus/rock_crystal/3.16> a skos:Concept ;
	skos:prefLabel "rock crystal"@en , "Bergkristall"@de ;
	skos:definition "Rock crystal, transparent variety of the silica mineral quartz that is valued for its clarity and total lack of colour or flaws. Used for carving and as an ornamental mineral." ;
	skos:inScheme <https://acdh.oeaw.ac.at/vocabs/defcthesaurus/FindsSchema> , <https://acdh.oeaw.ac.at/vocabs/defcthesaurus/FindsMaterial> ;
	skos:editorialNote "dc_finds_material;16" ;
	skos:broader <https://acdh.oeaw.ac.at/vocabs/defcthesaurus/mineral/2.03> .

<https://acdh.oeaw.ac.at/vocabs/defcthesaurus/mineral/2.03> skos:narrower <https://acdh.oeaw.ac.at/vocabs/defcthesaurus/rock_crystal/3.16> .

<https://acdh.oeaw.ac.at/vocabs/defcthesaurus/chlorite/3.21> a skos:Concept ;
	skos:prefLabel "chlorite"@en , "Chlorite"@de ;
	skos:definition "A chlorite (compound) is a compound that contains this group,with chlorine in oxidation state +3. Chlorites are also known as salts of chlorous acid." ;
	skos:inScheme <https://acdh.oeaw.ac.at/vocabs/defcthesaurus/FindsSchema> , <https://acdh.oeaw.ac.at/vocabs/defcthesaurus/FindsMaterial> ;
	skos:editorialNote "dc_finds_material;21" ;
	skos:broader <https://acdh.oeaw.ac.at/vocabs/defcthesaurus/mineral/2.03> .

<https://acdh.oeaw.ac.at/vocabs/defcthesaurus/mineral/2.03> skos:narrower <https://acdh.oeaw.ac.at/vocabs/defcthesaurus/chlorite/3.21> .

<https://acdh.oeaw.ac.at/vocabs/defcthesaurus/serpentine/3.23> a skos:Concept ;
	skos:prefLabel "serpentine"@en , "Serpentin"@de ;
	skos:definition "The serpentine subgroup (part of the kaolinite-serpentine group) are greenish, brownish, or spotted minerals commonly found in serpentinite rocks." ;
	skos:inScheme <https://acdh.oeaw.ac.at/vocabs/defcthesaurus/FindsSchema> , <https://acdh.oeaw.ac.at/vocabs/defcthesaurus/FindsMaterial> ;
	skos:editorialNote "dc_finds_material;23" ;
	skos:broader <https://acdh.oeaw.ac.at/vocabs/defcthesaurus/mineral/2.03> .

<https://acdh.oeaw.ac.at/vocabs/defcthesaurus/mineral/2.03> skos:narrower <https://acdh.oeaw.ac.at/vocabs/defcthesaurus/serpentine/3.23> .

<https://acdh.oeaw.ac.at/vocabs/defcthesaurus/malachite/3.35> a skos:Concept ;
	skos:prefLabel "malachite"@en , "Malachit"@de ;
	skos:definition "Malachite is a copper carbonate hydroxide mineral, with the formula Cu2CO3(OH)2." ;
	skos:inScheme <https://acdh.oeaw.ac.at/vocabs/defcthesaurus/FindsSchema> , <https://acdh.oeaw.ac.at/vocabs/defcthesaurus/FindsMaterial> ;
	skos:editorialNote "dc_finds_material;35" ;
	skos:broader <https://acdh.oeaw.ac.at/vocabs/defcthesaurus/mineral/2.03> .

<https://acdh.oeaw.ac.at/vocabs/defcthesaurus/mineral/2.03> skos:narrower <https://acdh.oeaw.ac.at/vocabs/defcthesaurus/malachite/3.35> .

<https://acdh.oeaw.ac.at/vocabs/defcthesaurus/calcite/3.37> a skos:Concept ;
	skos:prefLabel "calcite"@en , "Calcit"@de ;
	skos:altLabel "Kalkspat"@de , "Kalzit"@de ;
	skos:definition "Calcite is a carbonate mineral and the most stable polymorph of calcium carbonate (CaCO3)." ;
	skos:inScheme <https://acdh.oeaw.ac.at/vocabs/defcthesaurus/FindsSchema> , <https://acdh.oeaw.ac.at/vocabs/defcthesaurus/FindsMaterial> ;
	skos:editorialNote "dc_finds_material;37" ;
	skos:broader <https://acdh.oeaw.ac.at/vocabs/defcthesaurus/mineral/2.03> .

<https://acdh.oeaw.ac.at/vocabs/defcthesaurus/mineral/2.03> skos:narrower <https://acdh.oeaw.ac.at/vocabs/defcthesaurus/calcite/3.37> .

<https://acdh.oeaw.ac.at/vocabs/defcthesaurus/organic/2.04> a skos:Concept ;
	skos:prefLabel "organic"@en , "Organisches Material"@de , "Organisches Material"@la ;
	skos:altLabel "organisch"@de ;
	skos:definition "Organic material that was used to create objects." ;
	skos:inScheme <https://acdh.oeaw.ac.at/vocabs/defcthesaurus/FindsSchema> , <https://acdh.oeaw.ac.at/vocabs/defcthesaurus/NotInDatabase> ;
	skos:editorialNote "dc_not_in_database;04" ;
	skos:broader <https://acdh.oeaw.ac.at/vocabs/defcthesaurus/finds_material/1.01> .

<https://acdh.oeaw.ac.at/vocabs/defcthesaurus/finds_material/1.01> skos:narrower <https://acdh.oeaw.ac.at/vocabs/defcthesaurus/organic/2.04> .

<https://acdh.oeaw.ac.at/vocabs/defcthesaurus/wood/3.32> a skos:Concept ;
	skos:prefLabel "wood"@en , "Holz"@de ;
	skos:definition "Wood is a porous and fibrous structural tissue found in the stems and roots of trees and other woody plants. It is an organic material, a natural composite of cellulose fibers (which are strong in tension) embedded in a matrix of lignin which resists comp" ;
	skos:inScheme <https://acdh.oeaw.ac.at/vocabs/defcthesaurus/FindsSchema> , <https://acdh.oeaw.ac.at/vocabs/defcthesaurus/FindsMaterial> ;
	skos:editorialNote "dc_finds_material;32" ;
	skos:broader <https://acdh.oeaw.ac.at/vocabs/defcthesaurus/organic/2.04> .

<https://acdh.oeaw.ac.at/vocabs/defcthesaurus/organic/2.04> skos:narrower <https://acdh.oeaw.ac.at/vocabs/defcthesaurus/wood/3.32> .

<https://acdh.oeaw.ac.at/vocabs/defcthesaurus/bone/3.5> a skos:Concept ;
	skos:prefLabel "bone"@en , "Knochen"@de ;
	skos:definition "Bone used as material for production of different kinds of objects (tools, figurines etc)." ;
	skos:inScheme <https://acdh.oeaw.ac.at/vocabs/defcthesaurus/FindsSchema> , <https://acdh.oeaw.ac.at/vocabs/defcthesaurus/FindsMaterial> ;
	skos:editorialNote "dc_finds_material;5" ;
	skos:broader <https://acdh.oeaw.ac.at/vocabs/defcthesaurus/organic/2.04> .

<https://acdh.oeaw.ac.at/vocabs/defcthesaurus/organic/2.04> skos:narrower <https://acdh.oeaw.ac.at/vocabs/defcthesaurus/bone/3.5> .

<https://acdh.oeaw.ac.at/vocabs/defcthesaurus/shell/3.6> a skos:Concept ;
	skos:prefLabel "shell"@en , "Schale"@de ;
	skos:definition "The hard protective outer case of a mollusc or crustacean." ;
	skos:inScheme <https://acdh.oeaw.ac.at/vocabs/defcthesaurus/FindsSchema> , <https://acdh.oeaw.ac.at/vocabs/defcthesaurus/FindsMaterial> ;
	skos:editorialNote "dc_finds_material;6" ;
	skos:broader <https://acdh.oeaw.ac.at/vocabs/defcthesaurus/organic/2.04> .

<https://acdh.oeaw.ac.at/vocabs/defcthesaurus/organic/2.04> skos:narrower <https://acdh.oeaw.ac.at/vocabs/defcthesaurus/shell/3.6> ;
	dc:source "http://dbpedia.org/page/Spondylus" .

<https://acdh.oeaw.ac.at/vocabs/defcthesaurus/spondylus_shell/4.4> a skos:Concept ;
	skos:prefLabel "spondylus shell"@en , "Stachelaustern"@de ;
	skos:definition "Spondylus is a genus of bivalve molluscs, the only genus in the family Spondylidae." ;
	skos:inScheme <https://acdh.oeaw.ac.at/vocabs/defcthesaurus/FindsSchema> , <https://acdh.oeaw.ac.at/vocabs/defcthesaurus/FindsMaterial> ;
	skos:editorialNote "dc_finds_material;4" ;
	skos:broader <https://acdh.oeaw.ac.at/vocabs/defcthesaurus/shell/3.6> .

<https://acdh.oeaw.ac.at/vocabs/defcthesaurus/shell/3.6> skos:narrower <https://acdh.oeaw.ac.at/vocabs/defcthesaurus/spondylus_shell/4.4> .

<https://acdh.oeaw.ac.at/vocabs/defcthesaurus/organic/2.04> dc:source "http://dbpedia.org/page/Cockle_(bivalve)" .

<https://acdh.oeaw.ac.at/vocabs/defcthesaurus/cardium_shell/4.36> a skos:Concept ;
	skos:prefLabel "cardium shell"@en , "Herzmuscheln"@de ;
	skos:altLabel "Cockle"@en , "cardium"@en ;
	skos:definition "A cockle is a small, edible, saltwater clam, a marine bivalve mollusc." ;
	skos:inScheme <https://acdh.oeaw.ac.at/vocabs/defcthesaurus/FindsSchema> , <https://acdh.oeaw.ac.at/vocabs/defcthesaurus/FindsMaterial> ;
	skos:editorialNote "dc_finds_material;36" ;
	skos:broader <https://acdh.oeaw.ac.at/vocabs/defcthesaurus/shell/3.6> .

<https://acdh.oeaw.ac.at/vocabs/defcthesaurus/shell/3.6> skos:narrower <https://acdh.oeaw.ac.at/vocabs/defcthesaurus/cardium_shell/4.36> .

<https://acdh.oeaw.ac.at/vocabs/defcthesaurus/antler/3.7> a skos:Concept ;
	skos:prefLabel "antler"@en , "Geweih"@de ;
	skos:definition "Antlers are extensions of the skull grown by members of the deer family." ;
	skos:inScheme <https://acdh.oeaw.ac.at/vocabs/defcthesaurus/FindsSchema> , <https://acdh.oeaw.ac.at/vocabs/defcthesaurus/FindsMaterial> ;
	skos:editorialNote "dc_finds_material;7" ;
	skos:broader <https://acdh.oeaw.ac.at/vocabs/defcthesaurus/organic/2.04> .

<https://acdh.oeaw.ac.at/vocabs/defcthesaurus/organic/2.04> skos:narrower <https://acdh.oeaw.ac.at/vocabs/defcthesaurus/antler/3.7> .

<https://acdh.oeaw.ac.at/vocabs/defcthesaurus/horn/3.8> a skos:Concept ;
	skos:prefLabel "horn"@en , "Horn"@de ;
	skos:definition "A horn is a pointed projection on the head of various animals consisting of a covering of keratin and other proteins surrounding a core of live bone." ;
	skos:inScheme <https://acdh.oeaw.ac.at/vocabs/defcthesaurus/FindsSchema> , <https://acdh.oeaw.ac.at/vocabs/defcthesaurus/FindsMaterial> ;
	skos:editorialNote "dc_finds_material;8" ;
	skos:broader <https://acdh.oeaw.ac.at/vocabs/defcthesaurus/organic/2.04> .

<https://acdh.oeaw.ac.at/vocabs/defcthesaurus/organic/2.04> skos:narrower <https://acdh.oeaw.ac.at/vocabs/defcthesaurus/horn/3.8> .

<https://acdh.oeaw.ac.at/vocabs/defcthesaurus/tooth/3.28> a skos:Concept ;
	skos:prefLabel "tooth"@en , "Zahn"@de ;
	skos:definition "A tooth (plural teeth) is a small, calcified, whitish structure found in the jaws (or mouths) of many vertebrates and used to break down food." ;
	skos:inScheme <https://acdh.oeaw.ac.at/vocabs/defcthesaurus/FindsSchema> , <https://acdh.oeaw.ac.at/vocabs/defcthesaurus/FindsMaterial> ;
	skos:editorialNote "dc_finds_material;28" ;
	skos:broader <https://acdh.oeaw.ac.at/vocabs/defcthesaurus/organic/2.04> .

<https://acdh.oeaw.ac.at/vocabs/defcthesaurus/organic/2.04> skos:narrower <https://acdh.oeaw.ac.at/vocabs/defcthesaurus/tooth/3.28> .

<https://acdh.oeaw.ac.at/vocabs/defcthesaurus/clay/2.19> a skos:Concept ;
	skos:prefLabel "clay"@en , "Ton"@de , "Ton"@la ;
	skos:altLabel "Bodenart"@de ;
	skos:definition "Clay, soil paricles the diameters of which are less than 0.005 mm; also a rock that is composed essentially of clay particles. Clay materials are plastic when wet, and coherent when dry. Clay has variety of use such as pottery making and as building material." ;
	skos:inScheme <https://acdh.oeaw.ac.at/vocabs/defcthesaurus/FindsSchema> , <https://acdh.oeaw.ac.at/vocabs/defcthesaurus/FindsMaterial> ;
	skos:editorialNote "dc_finds_material;19" ;
	skos:broader <https://acdh.oeaw.ac.at/vocabs/defcthesaurus/finds_material/1.01> .

<https://acdh.oeaw.ac.at/vocabs/defcthesaurus/finds_material/1.01> skos:narrower <https://acdh.oeaw.ac.at/vocabs/defcthesaurus/clay/2.19> .

<https://acdh.oeaw.ac.at/vocabs/defcthesaurus/fabric/2.3> a skos:Concept ;
	skos:prefLabel "fabric"@en , "Stoff"@de , "Stoff"@la ;
	skos:definition "Cloth produced by weaving or knitting textile fibres." ;
	skos:inScheme <https://acdh.oeaw.ac.at/vocabs/defcthesaurus/FindsSchema> , <https://acdh.oeaw.ac.at/vocabs/defcthesaurus/FindsMaterial> ;
	skos:editorialNote "dc_finds_material;3" ;
	skos:broader <https://acdh.oeaw.ac.at/vocabs/defcthesaurus/finds_material/1.01> .

<https://acdh.oeaw.ac.at/vocabs/defcthesaurus/finds_material/1.01> skos:narrower <https://acdh.oeaw.ac.at/vocabs/defcthesaurus/fabric/2.3> .

<https://acdh.oeaw.ac.at/vocabs/defcthesaurus/finds_type/1.02> a skos:Concept ;
	skos:prefLabel "finds type"@en , "Fundtypus"@de ;
	skos:definition "This term classifies material things that result from human endeavor, have aesthetic, cultural, historical, scientific, or other utilirarian value, and are by design or through collecting portable functional entities (animal remains, botany, small finds and lithics)." ;
	skos:inScheme <https://acdh.oeaw.ac.at/vocabs/defcthesaurus/FindsSchema> , <https://acdh.oeaw.ac.at/vocabs/defcthesaurus/NotInDatabase> ;
	skos:editorialNote "dc_not_in_database;02" .

<https://acdh.oeaw.ac.at/vocabs/defcthesaurus/FindsType> a skos:ConceptScheme ;
	rdfs:comment "A concept schema related to the particular finds properties." .

<https://acdh.oeaw.ac.at/vocabs/defcthesaurus/animal_remains/2.1> a skos:Concept ;
	skos:prefLabel "animal remains"@en , "Tier체berreste"@de , "Tier체berreste"@la ;
	skos:altLabel "faunal remains"@en ;
	skos:definition "The items left behind when an animal dies such as bones, shells, hair, chitin, scales, hides, proteins and DNA." ;
	skos:inScheme <https://acdh.oeaw.ac.at/vocabs/defcthesaurus/FindsSchema> , <https://acdh.oeaw.ac.at/vocabs/defcthesaurus/FindsType> ;
	skos:editorialNote "dc_finds_type;1" ;
	skos:broader <https://acdh.oeaw.ac.at/vocabs/defcthesaurus/finds_type/1.02> .

<https://acdh.oeaw.ac.at/vocabs/defcthesaurus/finds_type/1.02> skos:narrower <https://acdh.oeaw.ac.at/vocabs/defcthesaurus/animal_remains/2.1> .

<https://acdh.oeaw.ac.at/vocabs/defcthesaurus/FindsAnimalRemainsCompletness> a skos:ConceptScheme ;
	rdfs:comment "A concept schema related to the particular finds properties." .

<https://acdh.oeaw.ac.at/vocabs/defcthesaurus/completness_of_animal_remains/3.05> a skos:Concept ;
	skos:prefLabel "completness of animal remains"@en ;
	skos:inScheme <https://acdh.oeaw.ac.at/vocabs/defcthesaurus/FindsSchema> ;
	skos:broader <https://acdh.oeaw.ac.at/vocabs/defcthesaurus/animal_remains/2.1> .

<https://acdh.oeaw.ac.at/vocabs/defcthesaurus/complete/4.1> a skos:Concept ;
	skos:prefLabel "complete"@en ;
	skos:definition "The animal remains found were complete." ;
	skos:inScheme <https://acdh.oeaw.ac.at/vocabs/defcthesaurus/FindsSchema> , <https://acdh.oeaw.ac.at/vocabs/defcthesaurus/FindsAnimalRemainsCompletness> ;
	skos:editorialNote "dc_finds_animal_remains_completness;1" ;
	skos:broader <https://acdh.oeaw.ac.at/vocabs/defcthesaurus/completness_of_animal_remains/3.05> .

<https://acdh.oeaw.ac.at/vocabs/defcthesaurus/completness_of_animal_remains/3.05> skos:narrower <https://acdh.oeaw.ac.at/vocabs/defcthesaurus/complete/4.1> .

<https://acdh.oeaw.ac.at/vocabs/defcthesaurus/animal_remains/2.1> skos:narrower <https://acdh.oeaw.ac.at/vocabs/defcthesaurus/completness_of_animal_remains/3.05> .

<https://acdh.oeaw.ac.at/vocabs/defcthesaurus/incomplete/4.2> a skos:Concept ;
	skos:prefLabel "incomplete"@en ;
	skos:definition "The animal remains found were incomplete." ;
	skos:inScheme <https://acdh.oeaw.ac.at/vocabs/defcthesaurus/FindsSchema> , <https://acdh.oeaw.ac.at/vocabs/defcthesaurus/FindsAnimalRemainsCompletness> ;
	skos:editorialNote "dc_finds_animal_remains_completness;2" ;
	skos:broader <https://acdh.oeaw.ac.at/vocabs/defcthesaurus/completness_of_animal_remains/3.05> .

<https://acdh.oeaw.ac.at/vocabs/defcthesaurus/completness_of_animal_remains/3.05> skos:narrower <https://acdh.oeaw.ac.at/vocabs/defcthesaurus/incomplete/4.2> .

<https://acdh.oeaw.ac.at/vocabs/defcthesaurus/animal_remains_species/3.06> a skos:Concept ;
	skos:prefLabel "animal remains species"@en ;
	skos:inScheme <https://acdh.oeaw.ac.at/vocabs/defcthesaurus/FindsSchema> ;
	skos:broader <https://acdh.oeaw.ac.at/vocabs/defcthesaurus/animal_remains/2.1> .

<https://acdh.oeaw.ac.at/vocabs/defcthesaurus/mammal/4.020> a skos:Concept ;
	skos:prefLabel "mammal"@en ;
	skos:inScheme <https://acdh.oeaw.ac.at/vocabs/defcthesaurus/FindsSchema> , <https://acdh.oeaw.ac.at/vocabs/defcthesaurus/NotInDatabase> ;
	skos:editorialNote "dc_not_in_database;020" ;
	skos:broader <https://acdh.oeaw.ac.at/vocabs/defcthesaurus/animal_remains_species/3.06> .

<https://acdh.oeaw.ac.at/vocabs/defcthesaurus/animal_remains_species/3.06> skos:narrower <https://acdh.oeaw.ac.at/vocabs/defcthesaurus/mammal/4.020> .

<https://acdh.oeaw.ac.at/vocabs/defcthesaurus/animal_remains/2.1> skos:narrower <https://acdh.oeaw.ac.at/vocabs/defcthesaurus/animal_remains_species/3.06> .

<https://acdh.oeaw.ac.at/vocabs/defcthesaurus/FindsAnimalRemainsSpecies> a skos:ConceptScheme ;
	rdfs:comment "A concept schema related to the particular finds properties." .

<https://acdh.oeaw.ac.at/vocabs/defcthesaurus/wild_board/5.1> a skos:Concept ;
	skos:prefLabel "wild board"@en , "Wildschwein"@de , "Sus scrofa"@la ;
	dc:source "http://eol.org/pages/328663/overview" ;
	skos:inScheme <https://acdh.oeaw.ac.at/vocabs/defcthesaurus/FindsSchema> , <https://acdh.oeaw.ac.at/vocabs/defcthesaurus/FindsAnimalRemainsSpecies> ;
	skos:editorialNote "dc_finds_animal_remains_species;1" ;
	skos:broader <https://acdh.oeaw.ac.at/vocabs/defcthesaurus/mammal/4.020> .

<https://acdh.oeaw.ac.at/vocabs/defcthesaurus/mammal/4.020> skos:narrower <https://acdh.oeaw.ac.at/vocabs/defcthesaurus/wild_board/5.1> .

<https://acdh.oeaw.ac.at/vocabs/defcthesaurus/wild_sheep/5.7> a skos:Concept ;
	skos:prefLabel "wild sheep"@en , "Wildschaf"@de , "Ovis orientalis"@la ;
	dc:source "http://eol.org/pages/4447671/overview" ;
	skos:inScheme <https://acdh.oeaw.ac.at/vocabs/defcthesaurus/FindsSchema> , <https://acdh.oeaw.ac.at/vocabs/defcthesaurus/FindsAnimalRemainsSpecies> ;
	skos:editorialNote "dc_finds_animal_remains_species;7" ;
	skos:broader <https://acdh.oeaw.ac.at/vocabs/defcthesaurus/mammal/4.020> .

<https://acdh.oeaw.ac.at/vocabs/defcthesaurus/mammal/4.020> skos:narrower <https://acdh.oeaw.ac.at/vocabs/defcthesaurus/wild_sheep/5.7> .

<https://acdh.oeaw.ac.at/vocabs/defcthesaurus/wild_goat/5.9> a skos:Concept ;
	skos:prefLabel "wild goat"@en , "Wildziege"@de , "Capra aegagrus"@la ;
	dc:source "http://eol.org/pages/2870013/overview" ;
	skos:inScheme <https://acdh.oeaw.ac.at/vocabs/defcthesaurus/FindsSchema> , <https://acdh.oeaw.ac.at/vocabs/defcthesaurus/FindsAnimalRemainsSpecies> ;
	skos:editorialNote "dc_finds_animal_remains_species;9" ;
	skos:broader <https://acdh.oeaw.ac.at/vocabs/defcthesaurus/mammal/4.020> .

<https://acdh.oeaw.ac.at/vocabs/defcthesaurus/mammal/4.020> skos:narrower <https://acdh.oeaw.ac.at/vocabs/defcthesaurus/wild_goat/5.9> .

<https://acdh.oeaw.ac.at/vocabs/defcthesaurus/wildcat/5.24> a skos:Concept ;
	skos:prefLabel "wildcat"@en , "Wildkatze"@de , "Felis silvestris"@la ;
	skos:altLabel "wild cat"@en ;
	dc:source "http://eol.org/pages/328605/overview" ;
	skos:inScheme <https://acdh.oeaw.ac.at/vocabs/defcthesaurus/FindsSchema> , <https://acdh.oeaw.ac.at/vocabs/defcthesaurus/FindsAnimalRemainsSpecies> ;
	skos:editorialNote "dc_finds_animal_remains_species;24" ;
	skos:broader <https://acdh.oeaw.ac.at/vocabs/defcthesaurus/mammal/4.020> .

<https://acdh.oeaw.ac.at/vocabs/defcthesaurus/mammal/4.020> skos:narrower <https://acdh.oeaw.ac.at/vocabs/defcthesaurus/wildcat/5.24> .

<https://acdh.oeaw.ac.at/vocabs/defcthesaurus/wild_cattle/5.38> a skos:Concept ;
	skos:prefLabel "wild cattle"@en , "Wildrind"@de ;
	skos:inScheme <https://acdh.oeaw.ac.at/vocabs/defcthesaurus/FindsSchema> , <https://acdh.oeaw.ac.at/vocabs/defcthesaurus/FindsAnimalRemainsSpecies> ;
	skos:editorialNote "dc_finds_animal_remains_species;38" ;
	skos:broader <https://acdh.oeaw.ac.at/vocabs/defcthesaurus/mammal/4.020> .

<https://acdh.oeaw.ac.at/vocabs/defcthesaurus/mammal/4.020> skos:narrower <https://acdh.oeaw.ac.at/vocabs/defcthesaurus/wild_cattle/5.38> .

<https://acdh.oeaw.ac.at/vocabs/defcthesaurus/hare/5.12> a skos:Concept ;
	skos:prefLabel "hare"@en , "Hase"@de , "Lepus europaeus"@la ;
	dc:source "http://eol.org/pages/118009/overview" ;
	skos:inScheme <https://acdh.oeaw.ac.at/vocabs/defcthesaurus/FindsSchema> , <https://acdh.oeaw.ac.at/vocabs/defcthesaurus/FindsAnimalRemainsSpecies> ;
	skos:editorialNote "dc_finds_animal_remains_species;12" ;
	skos:broader <https://acdh.oeaw.ac.at/vocabs/defcthesaurus/mammal/4.020> .

<https://acdh.oeaw.ac.at/vocabs/defcthesaurus/mammal/4.020> skos:narrower <https://acdh.oeaw.ac.at/vocabs/defcthesaurus/hare/5.12> .

<https://acdh.oeaw.ac.at/vocabs/defcthesaurus/finds_type/1.02> dc:source "http://eol.org/pages/328649/overview" .

<https://acdh.oeaw.ac.at/vocabs/defcthesaurus/mammal/4.020> dc:source "http://eol.org/pages/328649/overview" .

<https://acdh.oeaw.ac.at/vocabs/defcthesaurus/deer/5.036> a skos:Concept ;
	skos:prefLabel "deer"@en ;
	skos:inScheme <https://acdh.oeaw.ac.at/vocabs/defcthesaurus/FindsSchema> ;
	skos:broader <https://acdh.oeaw.ac.at/vocabs/defcthesaurus/mammal/4.020> .

<https://acdh.oeaw.ac.at/vocabs/defcthesaurus/red_deer/6.13> a skos:Concept ;
	skos:prefLabel "red deer"@en , "Rothirsch"@de , "Cervus elaphus"@la ;
	skos:inScheme <https://acdh.oeaw.ac.at/vocabs/defcthesaurus/FindsSchema> , <https://acdh.oeaw.ac.at/vocabs/defcthesaurus/FindsAnimalRemainsSpecies> ;
	skos:editorialNote "dc_finds_animal_remains_species;02" ;
	skos:broader <https://acdh.oeaw.ac.at/vocabs/defcthesaurus/deer/5.036> .

<https://acdh.oeaw.ac.at/vocabs/defcthesaurus/deer/5.036> skos:narrower <https://acdh.oeaw.ac.at/vocabs/defcthesaurus/red_deer/6.13> .

<https://acdh.oeaw.ac.at/vocabs/defcthesaurus/mammal/4.020> skos:narrower <https://acdh.oeaw.ac.at/vocabs/defcthesaurus/deer/5.036> .

<https://acdh.oeaw.ac.at/vocabs/defcthesaurus/finds_type/1.02> dc:source "http://eol.org/pages/308479/overview" .

<https://acdh.oeaw.ac.at/vocabs/defcthesaurus/mammal/4.020> dc:source "http://eol.org/pages/308479/overview" .

<https://acdh.oeaw.ac.at/vocabs/defcthesaurus/roe_deer/6.23> a skos:Concept ;
	skos:prefLabel "roe deer"@en , "Reh"@de , "Capreolus capreolus"@la ;
	skos:inScheme <https://acdh.oeaw.ac.at/vocabs/defcthesaurus/FindsSchema> , <https://acdh.oeaw.ac.at/vocabs/defcthesaurus/FindsAnimalRemainsSpecies> ;
	skos:editorialNote "dc_finds_animal_remains_species;02" ;
	skos:broader <https://acdh.oeaw.ac.at/vocabs/defcthesaurus/deer/5.036> .

<https://acdh.oeaw.ac.at/vocabs/defcthesaurus/deer/5.036> skos:narrower <https://acdh.oeaw.ac.at/vocabs/defcthesaurus/roe_deer/6.23> .

<https://acdh.oeaw.ac.at/vocabs/defcthesaurus/finds_type/1.02> dc:source "http://eol.org/pages/313992/overview" .

<https://acdh.oeaw.ac.at/vocabs/defcthesaurus/mammal/4.020> dc:source "http://eol.org/pages/313992/overview" .

<https://acdh.oeaw.ac.at/vocabs/defcthesaurus/fallow_deer/6.14> a skos:Concept ;
	skos:prefLabel "fallow deer"@en , "Damhirsch"@de , "Dama dama"@la ;
	skos:inScheme <https://acdh.oeaw.ac.at/vocabs/defcthesaurus/FindsSchema> , <https://acdh.oeaw.ac.at/vocabs/defcthesaurus/FindsAnimalRemainsSpecies> ;
	skos:editorialNote "dc_finds_animal_remains_species;02" ;
	skos:broader <https://acdh.oeaw.ac.at/vocabs/defcthesaurus/deer/5.036> .

<https://acdh.oeaw.ac.at/vocabs/defcthesaurus/deer/5.036> skos:narrower <https://acdh.oeaw.ac.at/vocabs/defcthesaurus/fallow_deer/6.14> .

<https://acdh.oeaw.ac.at/vocabs/defcthesaurus/aurochs/5.4> a skos:Concept ;
	skos:prefLabel "aurochs"@en , "Auerochs"@de , "Bos primigenius"@la ;
	dc:source "http://eol.org/pages/10408207/overview" ;
	skos:inScheme <https://acdh.oeaw.ac.at/vocabs/defcthesaurus/FindsSchema> , <https://acdh.oeaw.ac.at/vocabs/defcthesaurus/FindsAnimalRemainsSpecies> ;
	skos:editorialNote "dc_finds_animal_remains_species;4" ;
	skos:broader <https://acdh.oeaw.ac.at/vocabs/defcthesaurus/mammal/4.020> .

<https://acdh.oeaw.ac.at/vocabs/defcthesaurus/mammal/4.020> skos:narrower <https://acdh.oeaw.ac.at/vocabs/defcthesaurus/aurochs/5.4> .

<https://acdh.oeaw.ac.at/vocabs/defcthesaurus/chamois/5.40> a skos:Concept ;
	skos:prefLabel "chamois"@en , "Gams"@de , "Rupicapra rupicapra"@la ;
	dc:source "http://eol.org/pages/331073/overview" ;
	skos:inScheme <https://acdh.oeaw.ac.at/vocabs/defcthesaurus/FindsSchema> , <https://acdh.oeaw.ac.at/vocabs/defcthesaurus/FindsAnimalRemainsSpecies> ;
	skos:editorialNote "dc_finds_animal_remains_species;40" ;
	skos:broader <https://acdh.oeaw.ac.at/vocabs/defcthesaurus/mammal/4.020> .

<https://acdh.oeaw.ac.at/vocabs/defcthesaurus/mammal/4.020> skos:narrower <https://acdh.oeaw.ac.at/vocabs/defcthesaurus/chamois/5.40> .

<https://acdh.oeaw.ac.at/vocabs/defcthesaurus/gazelle/5.37> a skos:Concept ;
	skos:prefLabel "gazelle"@en , "Gazelle"@de ;
	skos:inScheme <https://acdh.oeaw.ac.at/vocabs/defcthesaurus/FindsSchema> , <https://acdh.oeaw.ac.at/vocabs/defcthesaurus/FindsAnimalRemainsSpecies> ;
	skos:editorialNote "dc_finds_animal_remains_species;37" ;
	skos:broader <https://acdh.oeaw.ac.at/vocabs/defcthesaurus/mammal/4.020> .

<https://acdh.oeaw.ac.at/vocabs/defcthesaurus/mammal/4.020> skos:narrower <https://acdh.oeaw.ac.at/vocabs/defcthesaurus/gazelle/5.37> .

<https://acdh.oeaw.ac.at/vocabs/defcthesaurus/wolf/5.26> a skos:Concept ;
	skos:prefLabel "wolf"@en , "Wolf"@de , "Canis lupus"@la ;
	dc:source "http://eol.org/pages/328607/overview" ;
	skos:inScheme <https://acdh.oeaw.ac.at/vocabs/defcthesaurus/FindsSchema> , <https://acdh.oeaw.ac.at/vocabs/defcthesaurus/FindsAnimalRemainsSpecies> ;
	skos:editorialNote "dc_finds_animal_remains_species;26" ;
	skos:broader <https://acdh.oeaw.ac.at/vocabs/defcthesaurus/mammal/4.020> .

<https://acdh.oeaw.ac.at/vocabs/defcthesaurus/mammal/4.020> skos:narrower <https://acdh.oeaw.ac.at/vocabs/defcthesaurus/wolf/5.26> .

<https://acdh.oeaw.ac.at/vocabs/defcthesaurus/red_fox/5.25> a skos:Concept ;
	skos:prefLabel "red fox"@en , "roter Fuchs"@de , "Vulpes vulpes"@la ;
	dc:source "http://eol.org/pages/328609/overview" ;
	skos:inScheme <https://acdh.oeaw.ac.at/vocabs/defcthesaurus/FindsSchema> , <https://acdh.oeaw.ac.at/vocabs/defcthesaurus/FindsAnimalRemainsSpecies> ;
	skos:editorialNote "dc_finds_animal_remains_species;25" ;
	skos:broader <https://acdh.oeaw.ac.at/vocabs/defcthesaurus/mammal/4.020> .

<https://acdh.oeaw.ac.at/vocabs/defcthesaurus/mammal/4.020> skos:narrower <https://acdh.oeaw.ac.at/vocabs/defcthesaurus/red_fox/5.25> .

<https://acdh.oeaw.ac.at/vocabs/defcthesaurus/beaver/5.28> a skos:Concept ;
	skos:prefLabel "beaver"@en , "Biber"@de , "Castor fiber"@la ;
	dc:source "http://eol.org/pages/1036116/overview" ;
	skos:inScheme <https://acdh.oeaw.ac.at/vocabs/defcthesaurus/FindsSchema> , <https://acdh.oeaw.ac.at/vocabs/defcthesaurus/FindsAnimalRemainsSpecies> ;
	skos:editorialNote "dc_finds_animal_remains_species;28" ;
	skos:broader <https://acdh.oeaw.ac.at/vocabs/defcthesaurus/mammal/4.020> .

<https://acdh.oeaw.ac.at/vocabs/defcthesaurus/mammal/4.020> skos:narrower <https://acdh.oeaw.ac.at/vocabs/defcthesaurus/beaver/5.28> .

<https://acdh.oeaw.ac.at/vocabs/defcthesaurus/brown_bear/5.22> a skos:Concept ;
	skos:prefLabel "brown bear"@en , "Braunb채r"@de , "Ursus arctos"@la ;
	dc:source "http://eol.org/pages/328581/overview" ;
	skos:inScheme <https://acdh.oeaw.ac.at/vocabs/defcthesaurus/FindsSchema> , <https://acdh.oeaw.ac.at/vocabs/defcthesaurus/FindsAnimalRemainsSpecies> ;
	skos:editorialNote "dc_finds_animal_remains_species;22" ;
	skos:broader <https://acdh.oeaw.ac.at/vocabs/defcthesaurus/mammal/4.020> .

<https://acdh.oeaw.ac.at/vocabs/defcthesaurus/mammal/4.020> skos:narrower <https://acdh.oeaw.ac.at/vocabs/defcthesaurus/brown_bear/5.22> .

<https://acdh.oeaw.ac.at/vocabs/defcthesaurus/donkey/5.21> a skos:Concept ;
	skos:prefLabel "donkey"@en , "Esel"@de , "Equus asinus"@la ;
	dc:source "http://eol.org/pages/328647/overview" ;
	skos:inScheme <https://acdh.oeaw.ac.at/vocabs/defcthesaurus/FindsSchema> , <https://acdh.oeaw.ac.at/vocabs/defcthesaurus/FindsAnimalRemainsSpecies> ;
	skos:editorialNote "dc_finds_animal_remains_species;21" ;
	skos:broader <https://acdh.oeaw.ac.at/vocabs/defcthesaurus/mammal/4.020> .

<https://acdh.oeaw.ac.at/vocabs/defcthesaurus/mammal/4.020> skos:narrower <https://acdh.oeaw.ac.at/vocabs/defcthesaurus/donkey/5.21> .

<https://acdh.oeaw.ac.at/vocabs/defcthesaurus/mouse/5.20> a skos:Concept ;
	skos:prefLabel "mouse"@en , "Maus"@de , "Muridea"@la ;
	dc:source "http://eol.org/pages/8698/overview" ;
	skos:inScheme <https://acdh.oeaw.ac.at/vocabs/defcthesaurus/FindsSchema> , <https://acdh.oeaw.ac.at/vocabs/defcthesaurus/FindsAnimalRemainsSpecies> ;
	skos:editorialNote "dc_finds_animal_remains_species;20" ;
	skos:broader <https://acdh.oeaw.ac.at/vocabs/defcthesaurus/mammal/4.020> .

<https://acdh.oeaw.ac.at/vocabs/defcthesaurus/mammal/4.020> skos:narrower <https://acdh.oeaw.ac.at/vocabs/defcthesaurus/mouse/5.20> .

<https://acdh.oeaw.ac.at/vocabs/defcthesaurus/water_vole/5.19> a skos:Concept ;
	skos:prefLabel "water vole"@en , "Schermaus"@de ;
	skos:inScheme <https://acdh.oeaw.ac.at/vocabs/defcthesaurus/FindsSchema> , <https://acdh.oeaw.ac.at/vocabs/defcthesaurus/FindsAnimalRemainsSpecies> ;
	skos:editorialNote "dc_finds_animal_remains_species;19" ;
	skos:broader <https://acdh.oeaw.ac.at/vocabs/defcthesaurus/mammal/4.020> .

<https://acdh.oeaw.ac.at/vocabs/defcthesaurus/mammal/4.020> skos:narrower <https://acdh.oeaw.ac.at/vocabs/defcthesaurus/water_vole/5.19> .

<https://acdh.oeaw.ac.at/vocabs/defcthesaurus/pig/5.2> a skos:Concept ;
	skos:prefLabel "pig"@en , "Schwein"@de , "Sus scrofa domesticus"@la ;
	dc:source "http://eol.org/pages/4445650/overview" ;
	skos:inScheme <https://acdh.oeaw.ac.at/vocabs/defcthesaurus/FindsSchema> , <https://acdh.oeaw.ac.at/vocabs/defcthesaurus/FindsAnimalRemainsSpecies> ;
	skos:editorialNote "dc_finds_animal_remains_species;2" ;
	skos:broader <https://acdh.oeaw.ac.at/vocabs/defcthesaurus/mammal/4.020> .

<https://acdh.oeaw.ac.at/vocabs/defcthesaurus/mammal/4.020> skos:narrower <https://acdh.oeaw.ac.at/vocabs/defcthesaurus/pig/5.2> .

<https://acdh.oeaw.ac.at/vocabs/defcthesaurus/cattle/5.3> a skos:Concept ;
	skos:prefLabel "cattle"@en , "Rind"@de , "Bos taurus"@la ;
	dc:source "http://eol.org/pages/328699/overview" ;
	skos:inScheme <https://acdh.oeaw.ac.at/vocabs/defcthesaurus/FindsSchema> , <https://acdh.oeaw.ac.at/vocabs/defcthesaurus/FindsAnimalRemainsSpecies> ;
	skos:editorialNote "dc_finds_animal_remains_species;3" ;
	skos:broader <https://acdh.oeaw.ac.at/vocabs/defcthesaurus/mammal/4.020> .

<https://acdh.oeaw.ac.at/vocabs/defcthesaurus/mammal/4.020> skos:narrower <https://acdh.oeaw.ac.at/vocabs/defcthesaurus/cattle/5.3> .

<https://acdh.oeaw.ac.at/vocabs/defcthesaurus/sheep/goat/5.5> a skos:Concept ;
	skos:prefLabel "sheep/goat"@en , "Schaf/Ziege"@de , "Ovis/Capra"@la ;
	skos:inScheme <https://acdh.oeaw.ac.at/vocabs/defcthesaurus/FindsSchema> , <https://acdh.oeaw.ac.at/vocabs/defcthesaurus/FindsAnimalRemainsSpecies> ;
	skos:editorialNote "dc_finds_animal_remains_species;5" ;
	skos:broader <https://acdh.oeaw.ac.at/vocabs/defcthesaurus/mammal/4.020> .

<https://acdh.oeaw.ac.at/vocabs/defcthesaurus/mammal/4.020> skos:narrower <https://acdh.oeaw.ac.at/vocabs/defcthesaurus/sheep/goat/5.5> .

<https://acdh.oeaw.ac.at/vocabs/defcthesaurus/sheep/5.6> a skos:Concept ;
	skos:prefLabel "sheep"@en , "Schaf"@de , "Ovis aries"@la ;
	dc:source "http://eol.org/pages/311906/overview" ;
	skos:inScheme <https://acdh.oeaw.ac.at/vocabs/defcthesaurus/FindsSchema> , <https://acdh.oeaw.ac.at/vocabs/defcthesaurus/FindsAnimalRemainsSpecies> ;
	skos:editorialNote "dc_finds_animal_remains_species;6" ;
	skos:broader <https://acdh.oeaw.ac.at/vocabs/defcthesaurus/mammal/4.020> .

<https://acdh.oeaw.ac.at/vocabs/defcthesaurus/mammal/4.020> skos:narrower <https://acdh.oeaw.ac.at/vocabs/defcthesaurus/sheep/5.6> .

<https://acdh.oeaw.ac.at/vocabs/defcthesaurus/goat/5.8> a skos:Concept ;
	skos:prefLabel "goat"@en , "Ziege"@de , "Capra hircus"@la ;
	dc:source "http://eol.org/pages/328660/overview" ;
	skos:inScheme <https://acdh.oeaw.ac.at/vocabs/defcthesaurus/FindsSchema> , <https://acdh.oeaw.ac.at/vocabs/defcthesaurus/FindsAnimalRemainsSpecies> ;
	skos:editorialNote "dc_finds_animal_remains_species;8" ;
	skos:broader <https://acdh.oeaw.ac.at/vocabs/defcthesaurus/mammal/4.020> .

<https://acdh.oeaw.ac.at/vocabs/defcthesaurus/mammal/4.020> skos:narrower <https://acdh.oeaw.ac.at/vocabs/defcthesaurus/goat/5.8> .

<https://acdh.oeaw.ac.at/vocabs/defcthesaurus/dog/5.10> a skos:Concept ;
	skos:prefLabel "dog"@en , "Hund"@de , "Canis familiaris"@la ;
	dc:source "http://eol.org/pages/1228387/overview" ;
	skos:inScheme <https://acdh.oeaw.ac.at/vocabs/defcthesaurus/FindsSchema> , <https://acdh.oeaw.ac.at/vocabs/defcthesaurus/FindsAnimalRemainsSpecies> ;
	skos:editorialNote "dc_finds_animal_remains_species;10" ;
	skos:broader <https://acdh.oeaw.ac.at/vocabs/defcthesaurus/mammal/4.020> .

<https://acdh.oeaw.ac.at/vocabs/defcthesaurus/mammal/4.020> skos:narrower <https://acdh.oeaw.ac.at/vocabs/defcthesaurus/dog/5.10> .

<https://acdh.oeaw.ac.at/vocabs/defcthesaurus/horse/5.11> a skos:Concept ;
	skos:prefLabel "horse"@en , "Pferd"@de , "Equus caballus"@la ;
	dc:source "http://eol.org/pages/328648/overview" ;
	skos:inScheme <https://acdh.oeaw.ac.at/vocabs/defcthesaurus/FindsSchema> , <https://acdh.oeaw.ac.at/vocabs/defcthesaurus/FindsAnimalRemainsSpecies> ;
	skos:editorialNote "dc_finds_animal_remains_species;11" ;
	skos:broader <https://acdh.oeaw.ac.at/vocabs/defcthesaurus/mammal/4.020> .

<https://acdh.oeaw.ac.at/vocabs/defcthesaurus/mammal/4.020> skos:narrower <https://acdh.oeaw.ac.at/vocabs/defcthesaurus/horse/5.11> .

<https://acdh.oeaw.ac.at/vocabs/defcthesaurus/onager/5.39> a skos:Concept ;
	skos:prefLabel "onager"@en ;
	skos:inScheme <https://acdh.oeaw.ac.at/vocabs/defcthesaurus/FindsSchema> , <https://acdh.oeaw.ac.at/vocabs/defcthesaurus/FindsAnimalRemainsSpecies> ;
	skos:editorialNote "dc_finds_animal_remains_species;39" ;
	skos:broader <https://acdh.oeaw.ac.at/vocabs/defcthesaurus/mammal/4.020> .

<https://acdh.oeaw.ac.at/vocabs/defcthesaurus/mammal/4.020> skos:narrower <https://acdh.oeaw.ac.at/vocabs/defcthesaurus/onager/5.39> .

<https://acdh.oeaw.ac.at/vocabs/defcthesaurus/game/5.15> a skos:Concept ;
	skos:prefLabel "game"@en , "Wild"@de ;
	skos:inScheme <https://acdh.oeaw.ac.at/vocabs/defcthesaurus/FindsSchema> , <https://acdh.oeaw.ac.at/vocabs/defcthesaurus/FindsAnimalRemainsSpecies> ;
	skos:editorialNote "dc_finds_animal_remains_species;15" ;
	skos:broader <https://acdh.oeaw.ac.at/vocabs/defcthesaurus/mammal/4.020> .

<https://acdh.oeaw.ac.at/vocabs/defcthesaurus/mammal/4.020> skos:narrower <https://acdh.oeaw.ac.at/vocabs/defcthesaurus/game/5.15> .

<https://acdh.oeaw.ac.at/vocabs/defcthesaurus/hare/5.27> a skos:Concept ;
	skos:prefLabel "hare"@en , "Hase"@de , "Lepus timidus"@la ;
	dc:source "http://eol.org/pages/133022/overview" ;
	skos:inScheme <https://acdh.oeaw.ac.at/vocabs/defcthesaurus/FindsSchema> , <https://acdh.oeaw.ac.at/vocabs/defcthesaurus/FindsAnimalRemainsSpecies> ;
	skos:editorialNote "dc_finds_animal_remains_species;27" ;
	skos:broader <https://acdh.oeaw.ac.at/vocabs/defcthesaurus/mammal/4.020> .

<https://acdh.oeaw.ac.at/vocabs/defcthesaurus/mammal/4.020> skos:narrower <https://acdh.oeaw.ac.at/vocabs/defcthesaurus/hare/5.27> .

<https://acdh.oeaw.ac.at/vocabs/defcthesaurus/animal_remains/2.1> dc:source "http://eol.org/pages/695/overview" .

<https://acdh.oeaw.ac.at/vocabs/defcthesaurus/bird/4.36> a skos:Concept ;
	skos:prefLabel "bird"@en , "Vogel"@de , "Aves"@la ;
	dc:source "http://eol.org/pages/695/overview" ;
	skos:inScheme <https://acdh.oeaw.ac.at/vocabs/defcthesaurus/FindsSchema> , <https://acdh.oeaw.ac.at/vocabs/defcthesaurus/FindsAnimalRemainsSpecies> ;
	skos:editorialNote "dc_finds_animal_remains_species;36" ;
	skos:broader <https://acdh.oeaw.ac.at/vocabs/defcthesaurus/animal_remains_species/3.06> .

<https://acdh.oeaw.ac.at/vocabs/defcthesaurus/animal_remains_species/3.06> skos:narrower <https://acdh.oeaw.ac.at/vocabs/defcthesaurus/bird/4.36> .

<https://acdh.oeaw.ac.at/vocabs/defcthesaurus/chicken/5.40> a skos:Concept ;
	skos:prefLabel "chicken"@en , "Huhn"@de , "Gallus gallus domesticus"@la ;
	dc:source "http://eol.org/pages/45890770/overview" ;
	skos:inScheme <https://acdh.oeaw.ac.at/vocabs/defcthesaurus/FindsSchema> , <https://acdh.oeaw.ac.at/vocabs/defcthesaurus/FindsAnimalRemainsSpecies> ;
	skos:editorialNote "dc_finds_animal_remains_species;40" ;
	skos:broader <https://acdh.oeaw.ac.at/vocabs/defcthesaurus/bird/4.36> .

<https://acdh.oeaw.ac.at/vocabs/defcthesaurus/bird/4.36> skos:narrower <https://acdh.oeaw.ac.at/vocabs/defcthesaurus/chicken/5.40> .

<https://acdh.oeaw.ac.at/vocabs/defcthesaurus/finds_type/1.02> dc:source "http://eol.org/pages/1047334/overview" .

<https://acdh.oeaw.ac.at/vocabs/defcthesaurus/bird/4.36> dc:source "http://eol.org/pages/1047334/overview" .

<https://acdh.oeaw.ac.at/vocabs/defcthesaurus/goose/5.037> a skos:Concept ;
	skos:prefLabel "goose"@en ;
	skos:inScheme <https://acdh.oeaw.ac.at/vocabs/defcthesaurus/FindsSchema> ;
	skos:broader <https://acdh.oeaw.ac.at/vocabs/defcthesaurus/bird/4.36> .

<https://acdh.oeaw.ac.at/vocabs/defcthesaurus/graylag_goose/6.31> a skos:Concept ;
	skos:prefLabel "graylag goose"@en , "Graugans"@de , "Anser anser"@la ;
	skos:inScheme <https://acdh.oeaw.ac.at/vocabs/defcthesaurus/FindsSchema> , <https://acdh.oeaw.ac.at/vocabs/defcthesaurus/FindsAnimalRemainsSpecies> ;
	skos:editorialNote "dc_finds_animal_remains_species;02" ;
	skos:broader <https://acdh.oeaw.ac.at/vocabs/defcthesaurus/goose/5.037> .

<https://acdh.oeaw.ac.at/vocabs/defcthesaurus/goose/5.037> skos:narrower <https://acdh.oeaw.ac.at/vocabs/defcthesaurus/graylag_goose/6.31> .

<https://acdh.oeaw.ac.at/vocabs/defcthesaurus/bird/4.36> skos:narrower <https://acdh.oeaw.ac.at/vocabs/defcthesaurus/goose/5.037> .

<https://acdh.oeaw.ac.at/vocabs/defcthesaurus/finds_type/1.02> dc:source "http://eol.org/pages/1048449/overview" .

<https://acdh.oeaw.ac.at/vocabs/defcthesaurus/bird/4.36> dc:source "http://eol.org/pages/1048449/overview" .

<https://acdh.oeaw.ac.at/vocabs/defcthesaurus/bean_goose/6.32> a skos:Concept ;
	skos:prefLabel "bean goose"@en , "Staatgans"@de , "Anser fabalis"@la ;
	skos:inScheme <https://acdh.oeaw.ac.at/vocabs/defcthesaurus/FindsSchema> , <https://acdh.oeaw.ac.at/vocabs/defcthesaurus/FindsAnimalRemainsSpecies> ;
	skos:editorialNote "dc_finds_animal_remains_species;02" ;
	skos:broader <https://acdh.oeaw.ac.at/vocabs/defcthesaurus/goose/5.037> .

<https://acdh.oeaw.ac.at/vocabs/defcthesaurus/goose/5.037> skos:narrower <https://acdh.oeaw.ac.at/vocabs/defcthesaurus/bean_goose/6.32> .

<https://acdh.oeaw.ac.at/vocabs/defcthesaurus/finds_type/1.02> dc:source "http://eol.org/pages/1047918/overview" .

<https://acdh.oeaw.ac.at/vocabs/defcthesaurus/bird/4.36> dc:source "http://eol.org/pages/1047918/overview" .

<https://acdh.oeaw.ac.at/vocabs/defcthesaurus/duck/5.038> a skos:Concept ;
	skos:prefLabel "duck"@en ;
	skos:inScheme <https://acdh.oeaw.ac.at/vocabs/defcthesaurus/FindsSchema> ;
	skos:broader <https://acdh.oeaw.ac.at/vocabs/defcthesaurus/bird/4.36> .

<https://acdh.oeaw.ac.at/vocabs/defcthesaurus/mallard_duck/6.33> a skos:Concept ;
	skos:prefLabel "mallard duck"@en , "Stockente"@de , "Anas platyrhynchos"@la ;
	skos:altLabel "duck"@en , "Ente"@de ;
	skos:inScheme <https://acdh.oeaw.ac.at/vocabs/defcthesaurus/FindsSchema> , <https://acdh.oeaw.ac.at/vocabs/defcthesaurus/FindsAnimalRemainsSpecies> ;
	skos:editorialNote "dc_finds_animal_remains_species;02" ;
	skos:broader <https://acdh.oeaw.ac.at/vocabs/defcthesaurus/duck/5.038> .

<https://acdh.oeaw.ac.at/vocabs/defcthesaurus/duck/5.038> skos:narrower <https://acdh.oeaw.ac.at/vocabs/defcthesaurus/mallard_duck/6.33> .

<https://acdh.oeaw.ac.at/vocabs/defcthesaurus/bird/4.36> skos:narrower <https://acdh.oeaw.ac.at/vocabs/defcthesaurus/duck/5.038> .

<https://acdh.oeaw.ac.at/vocabs/defcthesaurus/partirdge/5.34> a skos:Concept ;
	skos:prefLabel "partirdge"@en , "Rebhuhn"@de ;
	skos:inScheme <https://acdh.oeaw.ac.at/vocabs/defcthesaurus/FindsSchema> , <https://acdh.oeaw.ac.at/vocabs/defcthesaurus/FindsAnimalRemainsSpecies> ;
	skos:editorialNote "dc_finds_animal_remains_species;34" ;
	skos:broader <https://acdh.oeaw.ac.at/vocabs/defcthesaurus/bird/4.36> .

<https://acdh.oeaw.ac.at/vocabs/defcthesaurus/bird/4.36> skos:narrower <https://acdh.oeaw.ac.at/vocabs/defcthesaurus/partirdge/5.34> .

<https://acdh.oeaw.ac.at/vocabs/defcthesaurus/great_bustard/5.30> a skos:Concept ;
	skos:prefLabel "great bustard"@en , "Grotrappe"@de , "Otis tarda"@la ;
	dc:source "http://eol.org/pages/915364/overview" ;
	skos:inScheme <https://acdh.oeaw.ac.at/vocabs/defcthesaurus/FindsSchema> , <https://acdh.oeaw.ac.at/vocabs/defcthesaurus/FindsAnimalRemainsSpecies> ;
	skos:editorialNote "dc_finds_animal_remains_species;30" ;
	skos:broader <https://acdh.oeaw.ac.at/vocabs/defcthesaurus/bird/4.36> .

<https://acdh.oeaw.ac.at/vocabs/defcthesaurus/bird/4.36> skos:narrower <https://acdh.oeaw.ac.at/vocabs/defcthesaurus/great_bustard/5.30> .

<https://acdh.oeaw.ac.at/vocabs/defcthesaurus/animal_remains/2.1> dc:source "http://eol.org/pages/10567249/overview" .

<https://acdh.oeaw.ac.at/vocabs/defcthesaurus/reptile/4.35> a skos:Concept ;
	skos:prefLabel "reptile"@en , "Reptil"@de ;
	skos:inScheme <https://acdh.oeaw.ac.at/vocabs/defcthesaurus/FindsSchema> , <https://acdh.oeaw.ac.at/vocabs/defcthesaurus/FindsAnimalRemainsSpecies> ;
	skos:editorialNote "dc_finds_animal_remains_species;35" ;
	skos:broader <https://acdh.oeaw.ac.at/vocabs/defcthesaurus/animal_remains_species/3.06> .

<https://acdh.oeaw.ac.at/vocabs/defcthesaurus/animal_remains_species/3.06> skos:narrower <https://acdh.oeaw.ac.at/vocabs/defcthesaurus/reptile/4.35> .

<https://acdh.oeaw.ac.at/vocabs/defcthesaurus/tortoise/5.29> a skos:Concept ;
	skos:prefLabel "tortoise"@en , "Schildkr철te"@de ;
	skos:inScheme <https://acdh.oeaw.ac.at/vocabs/defcthesaurus/FindsSchema> , <https://acdh.oeaw.ac.at/vocabs/defcthesaurus/FindsAnimalRemainsSpecies> ;
	skos:editorialNote "dc_finds_animal_remains_species;29" ;
	skos:broader <https://acdh.oeaw.ac.at/vocabs/defcthesaurus/reptile/4.35> .

<https://acdh.oeaw.ac.at/vocabs/defcthesaurus/reptile/4.35> skos:narrower <https://acdh.oeaw.ac.at/vocabs/defcthesaurus/tortoise/5.29> .

<https://acdh.oeaw.ac.at/vocabs/defcthesaurus/animal_remains/2.1> dc:source "http://dbpedia.org/page/Fish" .

<https://acdh.oeaw.ac.at/vocabs/defcthesaurus/fish/4.16> a skos:Concept ;
	skos:prefLabel "fish"@en , "Fisch"@de ;
	skos:inScheme <https://acdh.oeaw.ac.at/vocabs/defcthesaurus/FindsSchema> , <https://acdh.oeaw.ac.at/vocabs/defcthesaurus/FindsAnimalRemainsSpecies> ;
	skos:editorialNote "dc_finds_animal_remains_species;16" ;
	skos:broader <https://acdh.oeaw.ac.at/vocabs/defcthesaurus/animal_remains_species/3.06> .

<https://acdh.oeaw.ac.at/vocabs/defcthesaurus/animal_remains_species/3.06> skos:narrower <https://acdh.oeaw.ac.at/vocabs/defcthesaurus/fish/4.16> .

<https://acdh.oeaw.ac.at/vocabs/defcthesaurus/tuna/5.18> a skos:Concept ;
	skos:prefLabel "tuna"@en , "Thunfisch"@de , "Thunnus"@la ;
	dc:source "http://eol.org/pages/25172/overview" ;
	skos:inScheme <https://acdh.oeaw.ac.at/vocabs/defcthesaurus/FindsSchema> , <https://acdh.oeaw.ac.at/vocabs/defcthesaurus/FindsAnimalRemainsSpecies> ;
	skos:editorialNote "dc_finds_animal_remains_species;18" ;
	skos:broader <https://acdh.oeaw.ac.at/vocabs/defcthesaurus/fish/4.16> .

<https://acdh.oeaw.ac.at/vocabs/defcthesaurus/fish/4.16> skos:narrower <https://acdh.oeaw.ac.at/vocabs/defcthesaurus/tuna/5.18> .

<https://acdh.oeaw.ac.at/vocabs/defcthesaurus/animal_remains/2.1> dc:source "http://eol.org/pages/2195/overview" .

<https://acdh.oeaw.ac.at/vocabs/defcthesaurus/molluscs/4.17> a skos:Concept ;
	skos:prefLabel "molluscs"@en , "Mollusken"@de ;
	skos:altLabel "mollusca"@en ;
	skos:inScheme <https://acdh.oeaw.ac.at/vocabs/defcthesaurus/FindsSchema> , <https://acdh.oeaw.ac.at/vocabs/defcthesaurus/FindsAnimalRemainsSpecies> ;
	skos:editorialNote "dc_finds_animal_remains_species;17" ;
	skos:broader <https://acdh.oeaw.ac.at/vocabs/defcthesaurus/animal_remains_species/3.06> .

<https://acdh.oeaw.ac.at/vocabs/defcthesaurus/animal_remains_species/3.06> skos:narrower <https://acdh.oeaw.ac.at/vocabs/defcthesaurus/molluscs/4.17> .

<https://acdh.oeaw.ac.at/vocabs/defcthesaurus/AnimalRemainsPart> a skos:ConceptScheme ;
	rdfs:comment "A concept schema related to the particular finds properties." .

<https://acdh.oeaw.ac.at/vocabs/defcthesaurus/animal_remains_part/3.07> a skos:Concept ;
	skos:prefLabel "animal remains part"@en ;
	skos:inScheme <https://acdh.oeaw.ac.at/vocabs/defcthesaurus/FindsSchema> ;
	skos:broader <https://acdh.oeaw.ac.at/vocabs/defcthesaurus/animal_remains/2.1> .

<https://acdh.oeaw.ac.at/vocabs/defcthesaurus/bone/4.021> a skos:Concept ;
	skos:prefLabel "bone"@en ;
	skos:inScheme <https://acdh.oeaw.ac.at/vocabs/defcthesaurus/FindsSchema> ;
	skos:broader <https://acdh.oeaw.ac.at/vocabs/defcthesaurus/animal_remains_part/3.07> .

<https://acdh.oeaw.ac.at/vocabs/defcthesaurus/extremity/5.4> a skos:Concept ;
	skos:prefLabel "extremity"@en , "Gliedma"@de ;
	skos:altLabel "Extrimit채t"@de ;
	skos:definition "A jointed, or prehensile, appendage of the human or other animal body." ;
	skos:inScheme <https://acdh.oeaw.ac.at/vocabs/defcthesaurus/FindsSchema> , <https://acdh.oeaw.ac.at/vocabs/defcthesaurus/AnimalRemainsPart> ;
	skos:editorialNote "dc_animal_remains_part;4" ;
	skos:broader <https://acdh.oeaw.ac.at/vocabs/defcthesaurus/bone/4.021> .

<https://acdh.oeaw.ac.at/vocabs/defcthesaurus/bone/4.021> skos:narrower <https://acdh.oeaw.ac.at/vocabs/defcthesaurus/extremity/5.4> .

<https://acdh.oeaw.ac.at/vocabs/defcthesaurus/animal_remains_part/3.07> skos:narrower <https://acdh.oeaw.ac.at/vocabs/defcthesaurus/bone/4.021> .

<https://acdh.oeaw.ac.at/vocabs/defcthesaurus/animal_remains/2.1> skos:narrower <https://acdh.oeaw.ac.at/vocabs/defcthesaurus/animal_remains_part/3.07> .

<https://acdh.oeaw.ac.at/vocabs/defcthesaurus/hindlimb/6.2> a skos:Concept ;
	skos:prefLabel "hindlimb"@en ;
	skos:definition "Either of the two back limbs of an animal." ;
	skos:inScheme <https://acdh.oeaw.ac.at/vocabs/defcthesaurus/FindsSchema> , <https://acdh.oeaw.ac.at/vocabs/defcthesaurus/AnimalRemainsPart> ;
	skos:editorialNote "dc_animal_remains_part;02" ;
	skos:broader <https://acdh.oeaw.ac.at/vocabs/defcthesaurus/extremity/5.4> .

<https://acdh.oeaw.ac.at/vocabs/defcthesaurus/extremity/5.4> skos:narrower <https://acdh.oeaw.ac.at/vocabs/defcthesaurus/hindlimb/6.2> .

<https://acdh.oeaw.ac.at/vocabs/defcthesaurus/forelimb/6.3> a skos:Concept ;
	skos:prefLabel "forelimb"@en ;
	skos:definition "Either of the front limbs of an animal; a foreleg, wing, flipper, etc." ;
	skos:inScheme <https://acdh.oeaw.ac.at/vocabs/defcthesaurus/FindsSchema> , <https://acdh.oeaw.ac.at/vocabs/defcthesaurus/AnimalRemainsPart> ;
	skos:editorialNote "dc_animal_remains_part;02" ;
	skos:broader <https://acdh.oeaw.ac.at/vocabs/defcthesaurus/extremity/5.4> .

<https://acdh.oeaw.ac.at/vocabs/defcthesaurus/extremity/5.4> skos:narrower <https://acdh.oeaw.ac.at/vocabs/defcthesaurus/forelimb/6.3> .

<https://acdh.oeaw.ac.at/vocabs/defcthesaurus/skull/5.1> a skos:Concept ;
	skos:prefLabel "skull"@en , "cranium"@la ;
	skos:definition "A bone framework enclosing the brain of a vertebrate; the skeleton of a person's or animal's head." ;
	dc:source "https://en.oxforddictionaries.com/definition/skull" ;
	skos:inScheme <https://acdh.oeaw.ac.at/vocabs/defcthesaurus/FindsSchema> , <https://acdh.oeaw.ac.at/vocabs/defcthesaurus/AnimalRemainsPart> ;
	skos:editorialNote "dc_animal_remains_part;1" ;
	skos:broader <https://acdh.oeaw.ac.at/vocabs/defcthesaurus/bone/4.021> .

<https://acdh.oeaw.ac.at/vocabs/defcthesaurus/bone/4.021> skos:narrower <https://acdh.oeaw.ac.at/vocabs/defcthesaurus/skull/5.1> .

<https://acdh.oeaw.ac.at/vocabs/defcthesaurus/body/5.5> a skos:Concept ;
	skos:prefLabel "body"@en , "Torso"@de ;
	skos:inScheme <https://acdh.oeaw.ac.at/vocabs/defcthesaurus/FindsSchema> , <https://acdh.oeaw.ac.at/vocabs/defcthesaurus/AnimalRemainsPart> ;
	skos:editorialNote "dc_animal_remains_part;5" ;
	skos:broader <https://acdh.oeaw.ac.at/vocabs/defcthesaurus/bone/4.021> .

<https://acdh.oeaw.ac.at/vocabs/defcthesaurus/bone/4.021> skos:narrower <https://acdh.oeaw.ac.at/vocabs/defcthesaurus/body/5.5> .

<https://acdh.oeaw.ac.at/vocabs/defcthesaurus/jaw/5.6> a skos:Concept ;
	skos:prefLabel "jaw"@en ;
	skos:definition "Either of a par of bones that form the framework of the mouth of vertebrate animals, usually containing teeth and including a movable lower jaw (mandible) and fixed upper jaw (maxilla)." ;
	skos:inScheme <https://acdh.oeaw.ac.at/vocabs/defcthesaurus/FindsSchema> , <https://acdh.oeaw.ac.at/vocabs/defcthesaurus/AnimalRemainsPart> ;
	skos:editorialNote "dc_animal_remains_part;6" ;
	skos:broader <https://acdh.oeaw.ac.at/vocabs/defcthesaurus/bone/4.021> .

<https://acdh.oeaw.ac.at/vocabs/defcthesaurus/bone/4.021> skos:narrower <https://acdh.oeaw.ac.at/vocabs/defcthesaurus/jaw/5.6> .

<https://acdh.oeaw.ac.at/vocabs/defcthesaurus/antler/5.8> a skos:Concept ;
	skos:prefLabel "antler"@en , "Geweih"@de ;
	skos:definition "Each of the branched horns on the head of an adult deer (typically a male one), which are made of bone and are grown and cast annually." ;
	skos:inScheme <https://acdh.oeaw.ac.at/vocabs/defcthesaurus/FindsSchema> , <https://acdh.oeaw.ac.at/vocabs/defcthesaurus/AnimalRemainsPart> ;
	skos:editorialNote "dc_animal_remains_part;8" ;
	skos:broader <https://acdh.oeaw.ac.at/vocabs/defcthesaurus/bone/4.021> .

<https://acdh.oeaw.ac.at/vocabs/defcthesaurus/bone/4.021> skos:narrower <https://acdh.oeaw.ac.at/vocabs/defcthesaurus/antler/5.8> .

<https://acdh.oeaw.ac.at/vocabs/defcthesaurus/animal_remains/2.1> dc:source "https://en.oxforddictionaries.com/definition/horn" .

<https://acdh.oeaw.ac.at/vocabs/defcthesaurus/horn/4.7> a skos:Concept ;
	skos:prefLabel "horn"@en , "Horn"@de ;
	skos:definition "A hard permanent outgrowth, often curved and pointed, found in pairs on the heads of cattle, sheep, goats, giraffes, etc. and consisting of a core of bone encased in keratinized skin." ;
	skos:inScheme <https://acdh.oeaw.ac.at/vocabs/defcthesaurus/FindsSchema> , <https://acdh.oeaw.ac.at/vocabs/defcthesaurus/AnimalRemainsPart> ;
	skos:editorialNote "dc_animal_remains_part;7" ;
	skos:broader <https://acdh.oeaw.ac.at/vocabs/defcthesaurus/animal_remains_part/3.07> .

<https://acdh.oeaw.ac.at/vocabs/defcthesaurus/animal_remains_part/3.07> skos:narrower <https://acdh.oeaw.ac.at/vocabs/defcthesaurus/horn/4.7> .

<https://acdh.oeaw.ac.at/vocabs/defcthesaurus/animal_remains/2.1> dc:source "https://en.oxforddictionaries.com/definition/tooth" .

<https://acdh.oeaw.ac.at/vocabs/defcthesaurus/tooth/4.11> a skos:Concept ;
	skos:prefLabel "tooth"@en , "Zahn"@de ;
	skos:definition "Each of a set of hard, bony enamel-coated structures in the jaws of most vertebrates, used for biting and chewing." ;
	skos:inScheme <https://acdh.oeaw.ac.at/vocabs/defcthesaurus/FindsSchema> , <https://acdh.oeaw.ac.at/vocabs/defcthesaurus/AnimalRemainsPart> ;
	skos:editorialNote "dc_animal_remains_part;11" ;
	skos:broader <https://acdh.oeaw.ac.at/vocabs/defcthesaurus/animal_remains_part/3.07> .

<https://acdh.oeaw.ac.at/vocabs/defcthesaurus/animal_remains_part/3.07> skos:narrower <https://acdh.oeaw.ac.at/vocabs/defcthesaurus/tooth/4.11> .

<https://acdh.oeaw.ac.at/vocabs/defcthesaurus/tusk/5.12> a skos:Concept ;
	skos:prefLabel "tusk"@en , "Stozahn"@de ;
	skos:definition "A long pointed tooth, especially one which protrudes from the closed mouth, as in the elephant, walrus, or wild boar." ;
	skos:inScheme <https://acdh.oeaw.ac.at/vocabs/defcthesaurus/FindsSchema> , <https://acdh.oeaw.ac.at/vocabs/defcthesaurus/AnimalRemainsPart> ;
	skos:editorialNote "dc_animal_remains_part;12" ;
	skos:broader <https://acdh.oeaw.ac.at/vocabs/defcthesaurus/tooth/4.11> .

<https://acdh.oeaw.ac.at/vocabs/defcthesaurus/tooth/4.11> skos:narrower <https://acdh.oeaw.ac.at/vocabs/defcthesaurus/tusk/5.12> .

<https://acdh.oeaw.ac.at/vocabs/defcthesaurus/animal_remains/2.1> dc:source "https://en.oxforddictionaries.com/definition/claw" .

<https://acdh.oeaw.ac.at/vocabs/defcthesaurus/claw/4.10> a skos:Concept ;
	skos:prefLabel "claw"@en , "Kralle"@de ;
	skos:definition "A curved pointed horny nail on each digit of the foot in birds, lizards, and some mammals." ;
	skos:inScheme <https://acdh.oeaw.ac.at/vocabs/defcthesaurus/FindsSchema> , <https://acdh.oeaw.ac.at/vocabs/defcthesaurus/AnimalRemainsPart> ;
	skos:editorialNote "dc_animal_remains_part;10" ;
	skos:broader <https://acdh.oeaw.ac.at/vocabs/defcthesaurus/animal_remains_part/3.07> .

<https://acdh.oeaw.ac.at/vocabs/defcthesaurus/animal_remains_part/3.07> skos:narrower <https://acdh.oeaw.ac.at/vocabs/defcthesaurus/claw/4.10> .

<https://acdh.oeaw.ac.at/vocabs/defcthesaurus/unknown/4.9> a skos:Concept ;
	skos:prefLabel "unknown"@en ;
	skos:inScheme <https://acdh.oeaw.ac.at/vocabs/defcthesaurus/FindsSchema> , <https://acdh.oeaw.ac.at/vocabs/defcthesaurus/AnimalRemainsPart> ;
	skos:editorialNote "dc_animal_remains_part;9" ;
	skos:broader <https://acdh.oeaw.ac.at/vocabs/defcthesaurus/animal_remains_part/3.07> .

<https://acdh.oeaw.ac.at/vocabs/defcthesaurus/animal_remains_part/3.07> skos:narrower <https://acdh.oeaw.ac.at/vocabs/defcthesaurus/unknown/4.9> .

<https://acdh.oeaw.ac.at/vocabs/defcthesaurus/botany/2.2> a skos:Concept ;
	skos:prefLabel "botany"@en , "Botanische R체ckst채nde"@de , "Botanische R체ckst채nde"@la ;
	skos:altLabel "plant remains"@en ;
	skos:definition "Remains of plants cultivated or used by man in ancient times and plants of ancient environment, which have survived in archaeological contexts." ;
	skos:inScheme <https://acdh.oeaw.ac.at/vocabs/defcthesaurus/FindsSchema> , <https://acdh.oeaw.ac.at/vocabs/defcthesaurus/FindsType> ;
	skos:editorialNote "dc_finds_type;2" ;
	skos:broader <https://acdh.oeaw.ac.at/vocabs/defcthesaurus/finds_type/1.02> .

<https://acdh.oeaw.ac.at/vocabs/defcthesaurus/finds_type/1.02> skos:narrower <https://acdh.oeaw.ac.at/vocabs/defcthesaurus/botany/2.2> .

<https://acdh.oeaw.ac.at/vocabs/defcthesaurus/grain_crop/3.08> a skos:Concept ;
	skos:prefLabel "grain crop"@en , "Getreidesorte"@de ;
	skos:inScheme <https://acdh.oeaw.ac.at/vocabs/defcthesaurus/FindsSchema> , <https://acdh.oeaw.ac.at/vocabs/defcthesaurus/NotInDatabase> ;
	skos:editorialNote "dc_not_in_database;08" ;
	skos:broader <https://acdh.oeaw.ac.at/vocabs/defcthesaurus/botany/2.2> .

<https://acdh.oeaw.ac.at/vocabs/defcthesaurus/botany/2.2> skos:narrower <https://acdh.oeaw.ac.at/vocabs/defcthesaurus/grain_crop/3.08> .

<https://acdh.oeaw.ac.at/vocabs/defcthesaurus/cereal/4.022> a skos:Concept ;
	skos:prefLabel "cereal"@en , "Getreide"@de ;
	skos:inScheme <https://acdh.oeaw.ac.at/vocabs/defcthesaurus/FindsSchema> , <https://acdh.oeaw.ac.at/vocabs/defcthesaurus/NotInDatabase> ;
	skos:editorialNote "dc_not_in_database;022" ;
	skos:broader <https://acdh.oeaw.ac.at/vocabs/defcthesaurus/grain_crop/3.08> .

<https://acdh.oeaw.ac.at/vocabs/defcthesaurus/grain_crop/3.08> skos:narrower <https://acdh.oeaw.ac.at/vocabs/defcthesaurus/cereal/4.022> .

<https://acdh.oeaw.ac.at/vocabs/defcthesaurus/BotanySpecies> a skos:ConceptScheme ;
	rdfs:comment "A concept schema related to the particular finds properties." .

<https://acdh.oeaw.ac.at/vocabs/defcthesaurus/barley/5.2> a skos:Concept ;
	skos:prefLabel "barley"@en , "Gerste"@de , "Hordeum vulgare"@la ;
	dc:source "http://eol.org/pages/1114455/overview" ;
	skos:inScheme <https://acdh.oeaw.ac.at/vocabs/defcthesaurus/FindsSchema> , <https://acdh.oeaw.ac.at/vocabs/defcthesaurus/BotanySpecies> ;
	skos:editorialNote "dc_botany_species;2" ;
	skos:broader <https://acdh.oeaw.ac.at/vocabs/defcthesaurus/cereal/4.022> .

<https://acdh.oeaw.ac.at/vocabs/defcthesaurus/cereal/4.022> skos:narrower <https://acdh.oeaw.ac.at/vocabs/defcthesaurus/barley/5.2> .

<https://acdh.oeaw.ac.at/vocabs/defcthesaurus/wild_barley/5.18> a skos:Concept ;
	skos:prefLabel "wild barley"@en , "Wilde Gerste"@de , "Hordeum vulgare subsp. spontaneum"@la ;
	dc:source "http://eol.org/pages/1114455/overview" ;
	skos:inScheme <https://acdh.oeaw.ac.at/vocabs/defcthesaurus/FindsSchema> , <https://acdh.oeaw.ac.at/vocabs/defcthesaurus/BotanySpecies> ;
	skos:editorialNote "dc_botany_species;18" ;
	skos:broader <https://acdh.oeaw.ac.at/vocabs/defcthesaurus/cereal/4.022> .

<https://acdh.oeaw.ac.at/vocabs/defcthesaurus/cereal/4.022> skos:narrower <https://acdh.oeaw.ac.at/vocabs/defcthesaurus/wild_barley/5.18> .

<https://acdh.oeaw.ac.at/vocabs/defcthesaurus/wheat/5.39> a skos:Concept ;
	skos:prefLabel "wheat"@en , "Weizen"@de , "Tritcum aestivum"@la ;
	dc:source "http://eol.org/pages/1115240/overview" ;
	skos:inScheme <https://acdh.oeaw.ac.at/vocabs/defcthesaurus/FindsSchema> , <https://acdh.oeaw.ac.at/vocabs/defcthesaurus/BotanySpecies> ;
	skos:editorialNote "dc_botany_species;39" ;
	skos:broader <https://acdh.oeaw.ac.at/vocabs/defcthesaurus/cereal/4.022> .

<https://acdh.oeaw.ac.at/vocabs/defcthesaurus/cereal/4.022> skos:narrower <https://acdh.oeaw.ac.at/vocabs/defcthesaurus/wheat/5.39> .

<https://acdh.oeaw.ac.at/vocabs/defcthesaurus/finds_type/1.02> dc:source "http://eol.org/pages/1115242/overview" .

<https://acdh.oeaw.ac.at/vocabs/defcthesaurus/cereal/4.022> dc:source "http://eol.org/pages/1115242/overview" .

<https://acdh.oeaw.ac.at/vocabs/defcthesaurus/einkorn_wheat/6.6> a skos:Concept ;
	skos:prefLabel "einkorn wheat"@en , "Einkorn"@de , "Triticum monococcum"@la ;
	skos:inScheme <https://acdh.oeaw.ac.at/vocabs/defcthesaurus/FindsSchema> , <https://acdh.oeaw.ac.at/vocabs/defcthesaurus/BotanySpecies> ;
	skos:editorialNote "dc_botany_species;02" ;
	skos:broader <https://acdh.oeaw.ac.at/vocabs/defcthesaurus/wheat/5.39> .

<https://acdh.oeaw.ac.at/vocabs/defcthesaurus/wheat/5.39> skos:narrower <https://acdh.oeaw.ac.at/vocabs/defcthesaurus/einkorn_wheat/6.6> .

<https://acdh.oeaw.ac.at/vocabs/defcthesaurus/finds_type/1.02> dc:source "http://eol.org/data_objects/32398343" .

<https://acdh.oeaw.ac.at/vocabs/defcthesaurus/cereal/4.022> dc:source "http://eol.org/data_objects/32398343" .

<https://acdh.oeaw.ac.at/vocabs/defcthesaurus/wild_einkorn/6.21> a skos:Concept ;
	skos:prefLabel "wild einkorn"@en , "Wilder Einkorn"@de , "Triticum monococcum subsp. baeoticum"@la ;
	skos:inScheme <https://acdh.oeaw.ac.at/vocabs/defcthesaurus/FindsSchema> , <https://acdh.oeaw.ac.at/vocabs/defcthesaurus/BotanySpecies> ;
	skos:editorialNote "dc_botany_species;02" ;
	skos:broader <https://acdh.oeaw.ac.at/vocabs/defcthesaurus/wheat/5.39> .

<https://acdh.oeaw.ac.at/vocabs/defcthesaurus/wheat/5.39> skos:narrower <https://acdh.oeaw.ac.at/vocabs/defcthesaurus/wild_einkorn/6.21> .

<https://acdh.oeaw.ac.at/vocabs/defcthesaurus/finds_type/1.02> dc:source "http://eol.org/pages/1114086/overview" .

<https://acdh.oeaw.ac.at/vocabs/defcthesaurus/cereal/4.022> dc:source "http://eol.org/pages/1114086/overview" .

<https://acdh.oeaw.ac.at/vocabs/defcthesaurus/emmer_wheat/6.7> a skos:Concept ;
	skos:prefLabel "emmer wheat"@en , "Emmer"@de , "Triticum turgidum subsp. dicoccum"@la ;
	skos:inScheme <https://acdh.oeaw.ac.at/vocabs/defcthesaurus/FindsSchema> , <https://acdh.oeaw.ac.at/vocabs/defcthesaurus/BotanySpecies> ;
	skos:editorialNote "dc_botany_species;02" ;
	skos:broader <https://acdh.oeaw.ac.at/vocabs/defcthesaurus/wheat/5.39> .

<https://acdh.oeaw.ac.at/vocabs/defcthesaurus/wheat/5.39> skos:narrower <https://acdh.oeaw.ac.at/vocabs/defcthesaurus/emmer_wheat/6.7> .

<https://acdh.oeaw.ac.at/vocabs/defcthesaurus/finds_type/1.02> dc:source "http://eol.org/pages/5835380/overview" .

<https://acdh.oeaw.ac.at/vocabs/defcthesaurus/cereal/4.022> dc:source "http://eol.org/pages/5835380/overview" .

<https://acdh.oeaw.ac.at/vocabs/defcthesaurus/wild_emmer/6.22> a skos:Concept ;
	skos:prefLabel "wild emmer"@en , "Wilder Emmer"@de , "Triticum turgidum subsp. dicoccoides"@la ;
	skos:inScheme <https://acdh.oeaw.ac.at/vocabs/defcthesaurus/FindsSchema> , <https://acdh.oeaw.ac.at/vocabs/defcthesaurus/BotanySpecies> ;
	skos:editorialNote "dc_botany_species;02" ;
	skos:broader <https://acdh.oeaw.ac.at/vocabs/defcthesaurus/wheat/5.39> .

<https://acdh.oeaw.ac.at/vocabs/defcthesaurus/wheat/5.39> skos:narrower <https://acdh.oeaw.ac.at/vocabs/defcthesaurus/wild_emmer/6.22> .

<https://acdh.oeaw.ac.at/vocabs/defcthesaurus/millet/5.039> a skos:Concept ;
	skos:prefLabel "millet"@en ;
	skos:inScheme <https://acdh.oeaw.ac.at/vocabs/defcthesaurus/FindsSchema> , <https://acdh.oeaw.ac.at/vocabs/defcthesaurus/NotInDatabase> ;
	skos:editorialNote "dc_not_in_database;039" ;
	skos:broader <https://acdh.oeaw.ac.at/vocabs/defcthesaurus/cereal/4.022> .

<https://acdh.oeaw.ac.at/vocabs/defcthesaurus/cereal/4.022> skos:narrower <https://acdh.oeaw.ac.at/vocabs/defcthesaurus/millet/5.039> .

<https://acdh.oeaw.ac.at/vocabs/defcthesaurus/finds_type/1.02> dc:source "http://eol.org/pages/1114498/overview" .

<https://acdh.oeaw.ac.at/vocabs/defcthesaurus/cereal/4.022> dc:source "http://eol.org/pages/1114498/overview" .

<https://acdh.oeaw.ac.at/vocabs/defcthesaurus/broomcorn_millet/6.4> a skos:Concept ;
	skos:prefLabel "broomcorn millet"@en , "Rispenhirse"@de , "Panicum miliaceum"@la ;
	skos:inScheme <https://acdh.oeaw.ac.at/vocabs/defcthesaurus/FindsSchema> , <https://acdh.oeaw.ac.at/vocabs/defcthesaurus/BotanySpecies> ;
	skos:editorialNote "dc_botany_species;02" ;
	skos:broader <https://acdh.oeaw.ac.at/vocabs/defcthesaurus/millet/5.039> .

<https://acdh.oeaw.ac.at/vocabs/defcthesaurus/millet/5.039> skos:narrower <https://acdh.oeaw.ac.at/vocabs/defcthesaurus/broomcorn_millet/6.4> .

<https://acdh.oeaw.ac.at/vocabs/defcthesaurus/finds_type/1.02> dc:source "http://eol.org/pages/1114673/overview" .

<https://acdh.oeaw.ac.at/vocabs/defcthesaurus/cereal/4.022> dc:source "http://eol.org/pages/1114673/overview" .

<https://acdh.oeaw.ac.at/vocabs/defcthesaurus/foxtail_millet/6.10> a skos:Concept ;
	skos:prefLabel "foxtail millet"@en , "Kolbenhirse"@de , "Setaria italica"@la ;
	skos:inScheme <https://acdh.oeaw.ac.at/vocabs/defcthesaurus/FindsSchema> , <https://acdh.oeaw.ac.at/vocabs/defcthesaurus/BotanySpecies> ;
	skos:editorialNote "dc_botany_species;02" ;
	skos:broader <https://acdh.oeaw.ac.at/vocabs/defcthesaurus/millet/5.039> .

<https://acdh.oeaw.ac.at/vocabs/defcthesaurus/millet/5.039> skos:narrower <https://acdh.oeaw.ac.at/vocabs/defcthesaurus/foxtail_millet/6.10> .

<https://acdh.oeaw.ac.at/vocabs/defcthesaurus/rye/5.17> a skos:Concept ;
	skos:prefLabel "rye"@en , "Roggen"@de , "Secale cereale"@la ;
	dc:source "http://eol.org/pages/1115159/overview" ;
	skos:inScheme <https://acdh.oeaw.ac.at/vocabs/defcthesaurus/FindsSchema> , <https://acdh.oeaw.ac.at/vocabs/defcthesaurus/BotanySpecies> ;
	skos:editorialNote "dc_botany_species;17" ;
	skos:broader <https://acdh.oeaw.ac.at/vocabs/defcthesaurus/cereal/4.022> .

<https://acdh.oeaw.ac.at/vocabs/defcthesaurus/cereal/4.022> skos:narrower <https://acdh.oeaw.ac.at/vocabs/defcthesaurus/rye/5.17> .

<https://acdh.oeaw.ac.at/vocabs/defcthesaurus/oat/5.37> a skos:Concept ;
	skos:prefLabel "oat"@en , "Hafer"@de , "Avana"@la ;
	dc:source "http://dbpedia.org/page/Oat" ;
	skos:inScheme <https://acdh.oeaw.ac.at/vocabs/defcthesaurus/FindsSchema> , <https://acdh.oeaw.ac.at/vocabs/defcthesaurus/BotanySpecies> ;
	skos:editorialNote "dc_botany_species;37" ;
	skos:broader <https://acdh.oeaw.ac.at/vocabs/defcthesaurus/cereal/4.022> .

<https://acdh.oeaw.ac.at/vocabs/defcthesaurus/cereal/4.022> skos:narrower <https://acdh.oeaw.ac.at/vocabs/defcthesaurus/oat/5.37> .

<https://acdh.oeaw.ac.at/vocabs/defcthesaurus/pulse/4.32> a skos:Concept ;
	skos:prefLabel "pulse"@en , "H체lsenfrucht"@de ;
	skos:altLabel "Legume"@en ;
	skos:inScheme <https://acdh.oeaw.ac.at/vocabs/defcthesaurus/FindsSchema> , <https://acdh.oeaw.ac.at/vocabs/defcthesaurus/BotanySpecies> ;
	skos:editorialNote "dc_botany_species;32" ;
	skos:broader <https://acdh.oeaw.ac.at/vocabs/defcthesaurus/grain_crop/3.08> .

<https://acdh.oeaw.ac.at/vocabs/defcthesaurus/grain_crop/3.08> skos:narrower <https://acdh.oeaw.ac.at/vocabs/defcthesaurus/pulse/4.32> .

<https://acdh.oeaw.ac.at/vocabs/defcthesaurus/fava_bean/5.8> a skos:Concept ;
	skos:prefLabel "fava bean"@en , "Ackerbohne"@de , "Vicia faba"@la ;
	dc:source "http://eol.org/pages/703202/overview" ;
	skos:inScheme <https://acdh.oeaw.ac.at/vocabs/defcthesaurus/FindsSchema> , <https://acdh.oeaw.ac.at/vocabs/defcthesaurus/BotanySpecies> ;
	skos:editorialNote "dc_botany_species;8" ;
	skos:broader <https://acdh.oeaw.ac.at/vocabs/defcthesaurus/pulse/4.32> .

<https://acdh.oeaw.ac.at/vocabs/defcthesaurus/pulse/4.32> skos:narrower <https://acdh.oeaw.ac.at/vocabs/defcthesaurus/fava_bean/5.8> .

<https://acdh.oeaw.ac.at/vocabs/defcthesaurus/pea/5.14> a skos:Concept ;
	skos:prefLabel "pea"@en , "Erbse"@de , "Pisum sativum"@la ;
	dc:source "http://eol.org/pages/703192/overview" ;
	skos:inScheme <https://acdh.oeaw.ac.at/vocabs/defcthesaurus/FindsSchema> , <https://acdh.oeaw.ac.at/vocabs/defcthesaurus/BotanySpecies> ;
	skos:editorialNote "dc_botany_species;14" ;
	skos:broader <https://acdh.oeaw.ac.at/vocabs/defcthesaurus/pulse/4.32> .

<https://acdh.oeaw.ac.at/vocabs/defcthesaurus/pulse/4.32> skos:narrower <https://acdh.oeaw.ac.at/vocabs/defcthesaurus/pea/5.14> .

<https://acdh.oeaw.ac.at/vocabs/defcthesaurus/finds_type/1.02> dc:source "http://eol.org/pages/685208/overview" .

<https://acdh.oeaw.ac.at/vocabs/defcthesaurus/pulse/4.32> dc:source "http://eol.org/pages/685208/overview" .

<https://acdh.oeaw.ac.at/vocabs/defcthesaurus/chickpea/6.5> a skos:Concept ;
	skos:prefLabel "chickpea"@en , "Kichererbse"@de , "Cicer arietinum"@la ;
	skos:inScheme <https://acdh.oeaw.ac.at/vocabs/defcthesaurus/FindsSchema> , <https://acdh.oeaw.ac.at/vocabs/defcthesaurus/BotanySpecies> ;
	skos:editorialNote "dc_botany_species;02" ;
	skos:broader <https://acdh.oeaw.ac.at/vocabs/defcthesaurus/pea/5.14> .

<https://acdh.oeaw.ac.at/vocabs/defcthesaurus/pea/5.14> skos:narrower <https://acdh.oeaw.ac.at/vocabs/defcthesaurus/chickpea/6.5> .

<https://acdh.oeaw.ac.at/vocabs/defcthesaurus/finds_type/1.02> dc:source "http://eol.org/pages/643350/overview" .

<https://acdh.oeaw.ac.at/vocabs/defcthesaurus/pulse/4.32> dc:source "http://eol.org/pages/643350/overview" .

<https://acdh.oeaw.ac.at/vocabs/defcthesaurus/wild_chickpea/6.20> a skos:Concept ;
	skos:prefLabel "wild chickpea"@en , "Wilde Kirchererbse"@de , "Cicer reticulatum"@la ;
	skos:inScheme <https://acdh.oeaw.ac.at/vocabs/defcthesaurus/FindsSchema> , <https://acdh.oeaw.ac.at/vocabs/defcthesaurus/BotanySpecies> ;
	skos:editorialNote "dc_botany_species;02" ;
	skos:broader <https://acdh.oeaw.ac.at/vocabs/defcthesaurus/pea/5.14> .

<https://acdh.oeaw.ac.at/vocabs/defcthesaurus/pea/5.14> skos:narrower <https://acdh.oeaw.ac.at/vocabs/defcthesaurus/wild_chickpea/6.20> .

<https://acdh.oeaw.ac.at/vocabs/defcthesaurus/finds_type/1.02> dc:source "http://eol.org/pages/703183/overview" .

<https://acdh.oeaw.ac.at/vocabs/defcthesaurus/pulse/4.32> dc:source "http://eol.org/pages/703183/overview" .

<https://acdh.oeaw.ac.at/vocabs/defcthesaurus/grass_pea/6.11> a skos:Concept ;
	skos:prefLabel "grass pea"@en , "Saat-Platterbse"@de , "Lathyrus sativus"@la ;
	skos:inScheme <https://acdh.oeaw.ac.at/vocabs/defcthesaurus/FindsSchema> , <https://acdh.oeaw.ac.at/vocabs/defcthesaurus/BotanySpecies> ;
	skos:editorialNote "dc_botany_species;02" ;
	skos:broader <https://acdh.oeaw.ac.at/vocabs/defcthesaurus/pea/5.14> .

<https://acdh.oeaw.ac.at/vocabs/defcthesaurus/pea/5.14> skos:narrower <https://acdh.oeaw.ac.at/vocabs/defcthesaurus/grass_pea/6.11> .

<https://acdh.oeaw.ac.at/vocabs/defcthesaurus/finds_type/1.02> dc:source "http://eol.org/pages/1230334/overview" .

<https://acdh.oeaw.ac.at/vocabs/defcthesaurus/pulse/4.32> dc:source "http://eol.org/pages/1230334/overview" .

<https://acdh.oeaw.ac.at/vocabs/defcthesaurus/wild_pea/6.25> a skos:Concept ;
	skos:prefLabel "wild pea"@en , "Wilde Erbse"@de , "Pisum humile"@la ;
	skos:inScheme <https://acdh.oeaw.ac.at/vocabs/defcthesaurus/FindsSchema> , <https://acdh.oeaw.ac.at/vocabs/defcthesaurus/BotanySpecies> ;
	skos:editorialNote "dc_botany_species;02" ;
	skos:broader <https://acdh.oeaw.ac.at/vocabs/defcthesaurus/pea/5.14> .

<https://acdh.oeaw.ac.at/vocabs/defcthesaurus/pea/5.14> skos:narrower <https://acdh.oeaw.ac.at/vocabs/defcthesaurus/wild_pea/6.25> .

<https://acdh.oeaw.ac.at/vocabs/defcthesaurus/vetch/5.33> a skos:Concept ;
	skos:prefLabel "vetch"@en , "Wicke"@de , "Vicia"@la ;
	dc:source "http://eol.org/pages/13463/overview" ;
	skos:inScheme <https://acdh.oeaw.ac.at/vocabs/defcthesaurus/FindsSchema> , <https://acdh.oeaw.ac.at/vocabs/defcthesaurus/BotanySpecies> ;
	skos:editorialNote "dc_botany_species;33" ;
	skos:broader <https://acdh.oeaw.ac.at/vocabs/defcthesaurus/pulse/4.32> .

<https://acdh.oeaw.ac.at/vocabs/defcthesaurus/pulse/4.32> skos:narrower <https://acdh.oeaw.ac.at/vocabs/defcthesaurus/vetch/5.33> .

<https://acdh.oeaw.ac.at/vocabs/defcthesaurus/finds_type/1.02> dc:source "http://eol.org/pages/703201/overview" .

<https://acdh.oeaw.ac.at/vocabs/defcthesaurus/pulse/4.32> dc:source "http://eol.org/pages/703201/overview" .

<https://acdh.oeaw.ac.at/vocabs/defcthesaurus/bitter_vetch/6.3> a skos:Concept ;
	skos:prefLabel "bitter vetch"@en , "Linsen-Wicke"@de , "Vicia ervilia"@la ;
	skos:inScheme <https://acdh.oeaw.ac.at/vocabs/defcthesaurus/FindsSchema> , <https://acdh.oeaw.ac.at/vocabs/defcthesaurus/BotanySpecies> ;
	skos:editorialNote "dc_botany_species;02" ;
	skos:broader <https://acdh.oeaw.ac.at/vocabs/defcthesaurus/vetch/5.33> .

<https://acdh.oeaw.ac.at/vocabs/defcthesaurus/vetch/5.33> skos:narrower <https://acdh.oeaw.ac.at/vocabs/defcthesaurus/bitter_vetch/6.3> .

<https://acdh.oeaw.ac.at/vocabs/defcthesaurus/wild_bitter_vetch/6.19> a skos:Concept ;
	skos:prefLabel "wild bitter vetch"@en , "Wilde Linsen-Wicke"@de , "Vicia ervilia"@la ;
	skos:inScheme <https://acdh.oeaw.ac.at/vocabs/defcthesaurus/FindsSchema> , <https://acdh.oeaw.ac.at/vocabs/defcthesaurus/BotanySpecies> ;
	skos:editorialNote "dc_botany_species;02" ;
	skos:broader <https://acdh.oeaw.ac.at/vocabs/defcthesaurus/vetch/5.33> .

<https://acdh.oeaw.ac.at/vocabs/defcthesaurus/vetch/5.33> skos:narrower <https://acdh.oeaw.ac.at/vocabs/defcthesaurus/wild_bitter_vetch/6.19> .

<https://acdh.oeaw.ac.at/vocabs/defcthesaurus/lentil/5.13> a skos:Concept ;
	skos:prefLabel "lentil"@en , "Linsen-Wicke"@de , "Lens culinaris"@la ;
	skos:altLabel "Linsen"@de ;
	dc:source "http://eol.org/pages/647510/overview" ;
	skos:inScheme <https://acdh.oeaw.ac.at/vocabs/defcthesaurus/FindsSchema> , <https://acdh.oeaw.ac.at/vocabs/defcthesaurus/BotanySpecies> ;
	skos:editorialNote "dc_botany_species;13" ;
	skos:broader <https://acdh.oeaw.ac.at/vocabs/defcthesaurus/pulse/4.32> .

<https://acdh.oeaw.ac.at/vocabs/defcthesaurus/pulse/4.32> skos:narrower <https://acdh.oeaw.ac.at/vocabs/defcthesaurus/lentil/5.13> .

<https://acdh.oeaw.ac.at/vocabs/defcthesaurus/wild_lentil/5.24> a skos:Concept ;
	skos:prefLabel "wild lentil"@en , "Wilde Linse"@de , "Lens orientalis"@la ;
	dc:source "http://eol.org/pages/1230180/overview" ;
	skos:inScheme <https://acdh.oeaw.ac.at/vocabs/defcthesaurus/FindsSchema> , <https://acdh.oeaw.ac.at/vocabs/defcthesaurus/BotanySpecies> ;
	skos:editorialNote "dc_botany_species;24" ;
	skos:broader <https://acdh.oeaw.ac.at/vocabs/defcthesaurus/pulse/4.32> .

<https://acdh.oeaw.ac.at/vocabs/defcthesaurus/pulse/4.32> skos:narrower <https://acdh.oeaw.ac.at/vocabs/defcthesaurus/wild_lentil/5.24> .

<https://acdh.oeaw.ac.at/vocabs/defcthesaurus/botany/2.2> dc:source "http://eol.org/pages/581568/overview" .

<https://acdh.oeaw.ac.at/vocabs/defcthesaurus/flax/4.9> a skos:Concept ;
	skos:prefLabel "flax"@en , "Gemeiner Lein/Flachs"@de , "Linum usitatissimum"@la ;
	dc:source "http://eol.org/pages/581568/overview" ;
	skos:inScheme <https://acdh.oeaw.ac.at/vocabs/defcthesaurus/FindsSchema> , <https://acdh.oeaw.ac.at/vocabs/defcthesaurus/BotanySpecies> ;
	skos:editorialNote "dc_botany_species;9" ;
	skos:broader <https://acdh.oeaw.ac.at/vocabs/defcthesaurus/grain_crop/3.08> .

<https://acdh.oeaw.ac.at/vocabs/defcthesaurus/grain_crop/3.08> skos:narrower <https://acdh.oeaw.ac.at/vocabs/defcthesaurus/flax/4.9> .

<https://acdh.oeaw.ac.at/vocabs/defcthesaurus/botany/2.2> dc:source "http://eol.org/pages/581539/overview" .

<https://acdh.oeaw.ac.at/vocabs/defcthesaurus/wild_flax/4.23> a skos:Concept ;
	skos:prefLabel "wild flax"@en , "Wilder Flachs"@de , "Linum bienne"@la ;
	dc:source "http://eol.org/pages/581539/overview" ;
	skos:inScheme <https://acdh.oeaw.ac.at/vocabs/defcthesaurus/FindsSchema> , <https://acdh.oeaw.ac.at/vocabs/defcthesaurus/BotanySpecies> ;
	skos:editorialNote "dc_botany_species;23" ;
	skos:broader <https://acdh.oeaw.ac.at/vocabs/defcthesaurus/grain_crop/3.08> .

<https://acdh.oeaw.ac.at/vocabs/defcthesaurus/grain_crop/3.08> skos:narrower <https://acdh.oeaw.ac.at/vocabs/defcthesaurus/wild_flax/4.23> .

<https://acdh.oeaw.ac.at/vocabs/defcthesaurus/botany/2.2> dc:source "http://eol.org/pages/594796/overview" .

<https://acdh.oeaw.ac.at/vocabs/defcthesaurus/poppy/4.16> a skos:Concept ;
	skos:prefLabel "poppy"@en , "Mohn"@de , "Papaver somniferum"@la ;
	dc:source "http://eol.org/pages/594796/overview" ;
	skos:inScheme <https://acdh.oeaw.ac.at/vocabs/defcthesaurus/FindsSchema> , <https://acdh.oeaw.ac.at/vocabs/defcthesaurus/BotanySpecies> ;
	skos:editorialNote "dc_botany_species;16" ;
	skos:broader <https://acdh.oeaw.ac.at/vocabs/defcthesaurus/grain_crop/3.08> .

<https://acdh.oeaw.ac.at/vocabs/defcthesaurus/grain_crop/3.08> skos:narrower <https://acdh.oeaw.ac.at/vocabs/defcthesaurus/poppy/4.16> .

<https://acdh.oeaw.ac.at/vocabs/defcthesaurus/hemp/3.12> a skos:Concept ;
	skos:prefLabel "hemp"@en , "Hanf"@de , "Cannabis sativa"@la ;
	skos:inScheme <https://acdh.oeaw.ac.at/vocabs/defcthesaurus/FindsSchema> , <https://acdh.oeaw.ac.at/vocabs/defcthesaurus/BotanySpecies> ;
	skos:editorialNote "dc_botany_species;12" ;
	skos:broader <https://acdh.oeaw.ac.at/vocabs/defcthesaurus/botany/2.2> .

<https://acdh.oeaw.ac.at/vocabs/defcthesaurus/botany/2.2> skos:narrower <https://acdh.oeaw.ac.at/vocabs/defcthesaurus/hemp/3.12> ;
	dc:source "http://eol.org/pages/301091/overview" .

<https://acdh.oeaw.ac.at/vocabs/defcthesaurus/fruit/3.09> a skos:Concept ;
	skos:prefLabel "fruit"@en ;
	skos:inScheme <https://acdh.oeaw.ac.at/vocabs/defcthesaurus/FindsSchema> ;
	skos:broader <https://acdh.oeaw.ac.at/vocabs/defcthesaurus/botany/2.2> .

<https://acdh.oeaw.ac.at/vocabs/defcthesaurus/apricot/4.1> a skos:Concept ;
	skos:prefLabel "apricot"@en , "Aprikose"@de , "Armeniaca vulgaris"@la ;
	dc:source "http://eol.org/pages/301091/overview" ;
	skos:inScheme <https://acdh.oeaw.ac.at/vocabs/defcthesaurus/FindsSchema> , <https://acdh.oeaw.ac.at/vocabs/defcthesaurus/BotanySpecies> ;
	skos:editorialNote "dc_botany_species;1" ;
	skos:broader <https://acdh.oeaw.ac.at/vocabs/defcthesaurus/fruit/3.09> .

<https://acdh.oeaw.ac.at/vocabs/defcthesaurus/fruit/3.09> skos:narrower <https://acdh.oeaw.ac.at/vocabs/defcthesaurus/apricot/4.1> .

<https://acdh.oeaw.ac.at/vocabs/defcthesaurus/botany/2.2> skos:narrower <https://acdh.oeaw.ac.at/vocabs/defcthesaurus/fruit/3.09> ;
	dc:source "http://eol.org/pages/631649/overview" .

<https://acdh.oeaw.ac.at/vocabs/defcthesaurus/peach/4.15> a skos:Concept ;
	skos:prefLabel "peach"@en , "Pfirsich"@de , "Persica vulgaris"@la ;
	dc:source "http://eol.org/pages/631649/overview" ;
	skos:inScheme <https://acdh.oeaw.ac.at/vocabs/defcthesaurus/FindsSchema> , <https://acdh.oeaw.ac.at/vocabs/defcthesaurus/BotanySpecies> ;
	skos:editorialNote "dc_botany_species;15" ;
	skos:broader <https://acdh.oeaw.ac.at/vocabs/defcthesaurus/fruit/3.09> .

<https://acdh.oeaw.ac.at/vocabs/defcthesaurus/fruit/3.09> skos:narrower <https://acdh.oeaw.ac.at/vocabs/defcthesaurus/peach/4.15> .

<https://acdh.oeaw.ac.at/vocabs/defcthesaurus/botany/2.2> dc:source "http://dbpedia.org/page/Olive" .

<https://acdh.oeaw.ac.at/vocabs/defcthesaurus/olive/4.26> a skos:Concept ;
	skos:prefLabel "olive"@en , "Olive"@de ;
	skos:inScheme <https://acdh.oeaw.ac.at/vocabs/defcthesaurus/FindsSchema> , <https://acdh.oeaw.ac.at/vocabs/defcthesaurus/BotanySpecies> ;
	skos:editorialNote "dc_botany_species;26" ;
	skos:broader <https://acdh.oeaw.ac.at/vocabs/defcthesaurus/fruit/3.09> .

<https://acdh.oeaw.ac.at/vocabs/defcthesaurus/fruit/3.09> skos:narrower <https://acdh.oeaw.ac.at/vocabs/defcthesaurus/olive/4.26> .

<https://acdh.oeaw.ac.at/vocabs/defcthesaurus/botany/2.2> dc:source "http://dbpedia.org/page/Ficus" .

<https://acdh.oeaw.ac.at/vocabs/defcthesaurus/fig/4.27> a skos:Concept ;
	skos:prefLabel "fig"@en , "Feige"@de , "Ficus"@la ;
	dc:source "http://dbpedia.org/page/Ficus" ;
	skos:inScheme <https://acdh.oeaw.ac.at/vocabs/defcthesaurus/FindsSchema> , <https://acdh.oeaw.ac.at/vocabs/defcthesaurus/BotanySpecies> ;
	skos:editorialNote "dc_botany_species;27" ;
	skos:broader <https://acdh.oeaw.ac.at/vocabs/defcthesaurus/fruit/3.09> .

<https://acdh.oeaw.ac.at/vocabs/defcthesaurus/fruit/3.09> skos:narrower <https://acdh.oeaw.ac.at/vocabs/defcthesaurus/fig/4.27> .

<https://acdh.oeaw.ac.at/vocabs/defcthesaurus/botany/2.2> dc:source "http://dbpedia.org/page/Blackberry" .

<https://acdh.oeaw.ac.at/vocabs/defcthesaurus/blackberry/4.36> a skos:Concept ;
	skos:prefLabel "blackberry"@en , "Brombeere"@de ;
	skos:inScheme <https://acdh.oeaw.ac.at/vocabs/defcthesaurus/FindsSchema> , <https://acdh.oeaw.ac.at/vocabs/defcthesaurus/BotanySpecies> ;
	skos:editorialNote "dc_botany_species;36" ;
	skos:broader <https://acdh.oeaw.ac.at/vocabs/defcthesaurus/fruit/3.09> .

<https://acdh.oeaw.ac.at/vocabs/defcthesaurus/fruit/3.09> skos:narrower <https://acdh.oeaw.ac.at/vocabs/defcthesaurus/blackberry/4.36> .

<https://acdh.oeaw.ac.at/vocabs/defcthesaurus/botany/2.2> dc:source "http://eol.org/pages/38383/overview" .

<https://acdh.oeaw.ac.at/vocabs/defcthesaurus/grape/4.29> a skos:Concept ;
	skos:prefLabel "grape"@en , "Traube"@de , "Vitis"@la ;
	dc:source "http://eol.org/pages/38383/overview" ;
	skos:inScheme <https://acdh.oeaw.ac.at/vocabs/defcthesaurus/FindsSchema> , <https://acdh.oeaw.ac.at/vocabs/defcthesaurus/BotanySpecies> ;
	skos:editorialNote "dc_botany_species;29" ;
	skos:broader <https://acdh.oeaw.ac.at/vocabs/defcthesaurus/fruit/3.09> .

<https://acdh.oeaw.ac.at/vocabs/defcthesaurus/fruit/3.09> skos:narrower <https://acdh.oeaw.ac.at/vocabs/defcthesaurus/grape/4.29> .

<https://acdh.oeaw.ac.at/vocabs/defcthesaurus/botany/2.2> dc:source "http://eol.org/pages/301085/overview" .

<https://acdh.oeaw.ac.at/vocabs/defcthesaurus/wild_plum/4.45> a skos:Concept ;
	skos:prefLabel "wild plum"@en , "Wilde Pflaume"@de , "Prunus americana"@la ;
	dc:source "http://eol.org/pages/301085/overview" ;
	skos:inScheme <https://acdh.oeaw.ac.at/vocabs/defcthesaurus/FindsSchema> , <https://acdh.oeaw.ac.at/vocabs/defcthesaurus/BotanySpecies> ;
	skos:editorialNote "dc_botany_species;45" ;
	skos:broader <https://acdh.oeaw.ac.at/vocabs/defcthesaurus/fruit/3.09> .

<https://acdh.oeaw.ac.at/vocabs/defcthesaurus/fruit/3.09> skos:narrower <https://acdh.oeaw.ac.at/vocabs/defcthesaurus/wild_plum/4.45> .

<https://acdh.oeaw.ac.at/vocabs/defcthesaurus/botany/2.2> dc:source "http://eol.org/pages/29915/overview" .

<https://acdh.oeaw.ac.at/vocabs/defcthesaurus/apple/4.41> a skos:Concept ;
	skos:prefLabel "apple"@en , "Apfel"@de , "Malus"@la ;
	dc:source "http://eol.org/pages/29915/overview" ;
	skos:inScheme <https://acdh.oeaw.ac.at/vocabs/defcthesaurus/FindsSchema> , <https://acdh.oeaw.ac.at/vocabs/defcthesaurus/BotanySpecies> ;
	skos:editorialNote "dc_botany_species;41" ;
	skos:broader <https://acdh.oeaw.ac.at/vocabs/defcthesaurus/fruit/3.09> .

<https://acdh.oeaw.ac.at/vocabs/defcthesaurus/fruit/3.09> skos:narrower <https://acdh.oeaw.ac.at/vocabs/defcthesaurus/apple/4.41> .

<https://acdh.oeaw.ac.at/vocabs/defcthesaurus/botany/2.2> dc:source "http://eol.org/pages/29920/overview" .

<https://acdh.oeaw.ac.at/vocabs/defcthesaurus/pear/4.42> a skos:Concept ;
	skos:prefLabel "pear"@en , "Birne"@de , "Pyrus"@la ;
	dc:source "http://eol.org/pages/29920/overview" ;
	skos:inScheme <https://acdh.oeaw.ac.at/vocabs/defcthesaurus/FindsSchema> , <https://acdh.oeaw.ac.at/vocabs/defcthesaurus/BotanySpecies> ;
	skos:editorialNote "dc_botany_species;42" ;
	skos:broader <https://acdh.oeaw.ac.at/vocabs/defcthesaurus/fruit/3.09> .

<https://acdh.oeaw.ac.at/vocabs/defcthesaurus/fruit/3.09> skos:narrower <https://acdh.oeaw.ac.at/vocabs/defcthesaurus/pear/4.42> .

<https://acdh.oeaw.ac.at/vocabs/defcthesaurus/botany/2.2> dc:source "http://dbpedia.org/page/Nut_(fruit)" .

<https://acdh.oeaw.ac.at/vocabs/defcthesaurus/nuts/4.31> a skos:Concept ;
	skos:prefLabel "nuts"@en , "Nu"@de ;
	skos:inScheme <https://acdh.oeaw.ac.at/vocabs/defcthesaurus/FindsSchema> , <https://acdh.oeaw.ac.at/vocabs/defcthesaurus/BotanySpecies> ;
	skos:editorialNote "dc_botany_species;31" ;
	skos:broader <https://acdh.oeaw.ac.at/vocabs/defcthesaurus/fruit/3.09> .

<https://acdh.oeaw.ac.at/vocabs/defcthesaurus/fruit/3.09> skos:narrower <https://acdh.oeaw.ac.at/vocabs/defcthesaurus/nuts/4.31> .

<https://acdh.oeaw.ac.at/vocabs/defcthesaurus/pistachio/5.28> a skos:Concept ;
	skos:prefLabel "pistachio"@en , "Pistazie"@de , "Pistacia"@la ;
	skos:altLabel "Pistache"@de ;
	dc:source "http://eol.org/pages/50516/overview" ;
	skos:inScheme <https://acdh.oeaw.ac.at/vocabs/defcthesaurus/FindsSchema> , <https://acdh.oeaw.ac.at/vocabs/defcthesaurus/BotanySpecies> ;
	skos:editorialNote "dc_botany_species;28" ;
	skos:broader <https://acdh.oeaw.ac.at/vocabs/defcthesaurus/nuts/4.31> .

<https://acdh.oeaw.ac.at/vocabs/defcthesaurus/nuts/4.31> skos:narrower <https://acdh.oeaw.ac.at/vocabs/defcthesaurus/pistachio/5.28> .

<https://acdh.oeaw.ac.at/vocabs/defcthesaurus/almond/5.30> a skos:Concept ;
	skos:prefLabel "almond"@en , "Mandel"@de , "Prunus amygdalus"@la ;
	dc:source "http://eol.org/pages/231567/overview" ;
	skos:inScheme <https://acdh.oeaw.ac.at/vocabs/defcthesaurus/FindsSchema> , <https://acdh.oeaw.ac.at/vocabs/defcthesaurus/BotanySpecies> ;
	skos:editorialNote "dc_botany_species;30" ;
	skos:broader <https://acdh.oeaw.ac.at/vocabs/defcthesaurus/nuts/4.31> .

<https://acdh.oeaw.ac.at/vocabs/defcthesaurus/nuts/4.31> skos:narrower <https://acdh.oeaw.ac.at/vocabs/defcthesaurus/almond/5.30> .

<https://acdh.oeaw.ac.at/vocabs/defcthesaurus/acorn/5.35> a skos:Concept ;
	skos:prefLabel "acorn"@en , "Eichel"@de ;
	skos:inScheme <https://acdh.oeaw.ac.at/vocabs/defcthesaurus/FindsSchema> , <https://acdh.oeaw.ac.at/vocabs/defcthesaurus/BotanySpecies> ;
	skos:editorialNote "dc_botany_species;35" ;
	skos:broader <https://acdh.oeaw.ac.at/vocabs/defcthesaurus/nuts/4.31> .

<https://acdh.oeaw.ac.at/vocabs/defcthesaurus/nuts/4.31> skos:narrower <https://acdh.oeaw.ac.at/vocabs/defcthesaurus/acorn/5.35> .

<https://acdh.oeaw.ac.at/vocabs/defcthesaurus/sea_club-rush/3.34> a skos:Concept ;
	skos:prefLabel "sea club-rush"@en , "Strandbinse"@de , "Schoenoplectus"@la ;
	skos:inScheme <https://acdh.oeaw.ac.at/vocabs/defcthesaurus/FindsSchema> , <https://acdh.oeaw.ac.at/vocabs/defcthesaurus/BotanySpecies> ;
	skos:editorialNote "dc_botany_species;34" ;
	skos:broader <https://acdh.oeaw.ac.at/vocabs/defcthesaurus/botany/2.2> .

<https://acdh.oeaw.ac.at/vocabs/defcthesaurus/botany/2.2> skos:narrower <https://acdh.oeaw.ac.at/vocabs/defcthesaurus/sea_club-rush/3.34> .

<https://acdh.oeaw.ac.at/vocabs/defcthesaurus/black_nightshade/3.38> a skos:Concept ;
	skos:prefLabel "black nightshade"@en , "schwarzes Nachtschattengew채chs"@de , "Chenopodiacea"@la ;
	skos:inScheme <https://acdh.oeaw.ac.at/vocabs/defcthesaurus/FindsSchema> , <https://acdh.oeaw.ac.at/vocabs/defcthesaurus/BotanySpecies> ;
	skos:editorialNote "dc_botany_species;38" ;
	skos:broader <https://acdh.oeaw.ac.at/vocabs/defcthesaurus/botany/2.2> .

<https://acdh.oeaw.ac.at/vocabs/defcthesaurus/botany/2.2> skos:narrower <https://acdh.oeaw.ac.at/vocabs/defcthesaurus/black_nightshade/3.38> .

<https://acdh.oeaw.ac.at/vocabs/defcthesaurus/buckthorn/3.43> a skos:Concept ;
	skos:prefLabel "buckthorn"@en , "Dorn"@de , "Rhammus"@la ;
	skos:inScheme <https://acdh.oeaw.ac.at/vocabs/defcthesaurus/FindsSchema> , <https://acdh.oeaw.ac.at/vocabs/defcthesaurus/BotanySpecies> ;
	skos:editorialNote "dc_botany_species;43" ;
	skos:broader <https://acdh.oeaw.ac.at/vocabs/defcthesaurus/botany/2.2> .

<https://acdh.oeaw.ac.at/vocabs/defcthesaurus/botany/2.2> skos:narrower <https://acdh.oeaw.ac.at/vocabs/defcthesaurus/buckthorn/3.43> .

<https://acdh.oeaw.ac.at/vocabs/defcthesaurus/pine/3.44> a skos:Concept ;
	skos:prefLabel "pine"@en , "Kiefer"@de , "Pinus pinea"@la ;
	skos:inScheme <https://acdh.oeaw.ac.at/vocabs/defcthesaurus/FindsSchema> , <https://acdh.oeaw.ac.at/vocabs/defcthesaurus/BotanySpecies> ;
	skos:editorialNote "dc_botany_species;44" ;
	skos:broader <https://acdh.oeaw.ac.at/vocabs/defcthesaurus/botany/2.2> .

<https://acdh.oeaw.ac.at/vocabs/defcthesaurus/botany/2.2> skos:narrower <https://acdh.oeaw.ac.at/vocabs/defcthesaurus/pine/3.44> .

<https://acdh.oeaw.ac.at/vocabs/defcthesaurus/lithics/2.3> a skos:Concept ;
	skos:prefLabel "lithics"@en , "Steinwerkzeug"@de , "Steinwerkzeug"@la ;
	skos:altLabel "Stone tool"@en , "Steinger채t"@de ;
	skos:inScheme <https://acdh.oeaw.ac.at/vocabs/defcthesaurus/FindsSchema> , <https://acdh.oeaw.ac.at/vocabs/defcthesaurus/FindsType> ;
	skos:editorialNote "dc_finds_type;3" ;
	skos:broader <https://acdh.oeaw.ac.at/vocabs/defcthesaurus/finds_type/1.02> .

<https://acdh.oeaw.ac.at/vocabs/defcthesaurus/finds_type/1.02> skos:narrower <https://acdh.oeaw.ac.at/vocabs/defcthesaurus/lithics/2.3> .

<https://acdh.oeaw.ac.at/vocabs/defcthesaurus/retouched_tool/3.010> a skos:Concept ;
	skos:prefLabel "retouched tool"@en ;
	skos:inScheme <https://acdh.oeaw.ac.at/vocabs/defcthesaurus/FindsSchema> , <https://acdh.oeaw.ac.at/vocabs/defcthesaurus/NotInDatabase> ;
	skos:editorialNote "dc_not_in_database;010" ;
	skos:broader <https://acdh.oeaw.ac.at/vocabs/defcthesaurus/lithics/2.3> .

<https://acdh.oeaw.ac.at/vocabs/defcthesaurus/lithics/2.3> skos:narrower <https://acdh.oeaw.ac.at/vocabs/defcthesaurus/retouched_tool/3.010> .

<https://acdh.oeaw.ac.at/vocabs/defcthesaurus/FindsLithicsRetouchedTools> a skos:ConceptScheme ;
	rdfs:comment "A concept schema related to the particular finds properties." .

<https://acdh.oeaw.ac.at/vocabs/defcthesaurus/backed_bladelet/4.1> a skos:Concept ;
	skos:prefLabel "backed bladelet"@en ;
	skos:definition "A small  blade with one edge blunted, belongs to the category of microliths." ;
	skos:inScheme <https://acdh.oeaw.ac.at/vocabs/defcthesaurus/FindsSchema> , <https://acdh.oeaw.ac.at/vocabs/defcthesaurus/FindsLithicsRetouchedTools> ;
	skos:editorialNote "dc_finds_lithics_retouched_tools;1" ;
	skos:broader <https://acdh.oeaw.ac.at/vocabs/defcthesaurus/retouched_tool/3.010> .

<https://acdh.oeaw.ac.at/vocabs/defcthesaurus/retouched_tool/3.010> skos:narrower <https://acdh.oeaw.ac.at/vocabs/defcthesaurus/backed_bladelet/4.1> .

<https://acdh.oeaw.ac.at/vocabs/defcthesaurus/lithics/2.3> dc:source "Inizan, M.-L., M. Reduron-Ballinger, H. Roche, J. Tixier 1999, Technology and Terminology of Knapped Stone. Nanterre: CREP., D. Srejovic (ed) 1997, Arheolo큄ki Leksikon." .

<https://acdh.oeaw.ac.at/vocabs/defcthesaurus/burin/4.2> a skos:Concept ;
	skos:prefLabel "burin"@en , "Stichel"@de ;
	skos:definition "A specialized engraving tool which bears a negative surface created by the removal of a burin spall (cut diagonally downward from the part of the blade/flake edge)." ;
	skos:inScheme <https://acdh.oeaw.ac.at/vocabs/defcthesaurus/FindsSchema> , <https://acdh.oeaw.ac.at/vocabs/defcthesaurus/FindsLithicsRetouchedTools> ;
	skos:editorialNote "dc_finds_lithics_retouched_tools;2" ;
	skos:broader <https://acdh.oeaw.ac.at/vocabs/defcthesaurus/retouched_tool/3.010> .

<https://acdh.oeaw.ac.at/vocabs/defcthesaurus/retouched_tool/3.010> skos:narrower <https://acdh.oeaw.ac.at/vocabs/defcthesaurus/burin/4.2> .

<https://acdh.oeaw.ac.at/vocabs/defcthesaurus/챌ay철n체_tool/4.3> a skos:Concept ;
	skos:prefLabel "챌ay철n체 tool"@en , "ay철n체 Werkzeug"@de ;
	skos:definition "A particular type of retouched blade appearing in the region of the Upper Mesopotamia during the Pre-Pottery Neolithic, named after the site of ay철n체. Function unknown due to the dull edges and special type fo the retouch." ;
	skos:inScheme <https://acdh.oeaw.ac.at/vocabs/defcthesaurus/FindsSchema> , <https://acdh.oeaw.ac.at/vocabs/defcthesaurus/FindsLithicsRetouchedTools> ;
	skos:editorialNote "dc_finds_lithics_retouched_tools;3" ;
	skos:broader <https://acdh.oeaw.ac.at/vocabs/defcthesaurus/retouched_tool/3.010> .

<https://acdh.oeaw.ac.at/vocabs/defcthesaurus/retouched_tool/3.010> skos:narrower <https://acdh.oeaw.ac.at/vocabs/defcthesaurus/챌ay철n체_tool/4.3> .

<https://acdh.oeaw.ac.at/vocabs/defcthesaurus/cicrular_scraper/4.4> a skos:Concept ;
	skos:prefLabel "cicrular scraper"@en ;
	skos:altLabel "round scraper"@en ;
	skos:definition "A discoid scraper with completely retouched convex edge. Synonym: round scraper, discoid scraper." ;
	skos:inScheme <https://acdh.oeaw.ac.at/vocabs/defcthesaurus/FindsSchema> , <https://acdh.oeaw.ac.at/vocabs/defcthesaurus/FindsLithicsRetouchedTools> ;
	skos:editorialNote "dc_finds_lithics_retouched_tools;4" ;
	skos:broader <https://acdh.oeaw.ac.at/vocabs/defcthesaurus/retouched_tool/3.010> .

<https://acdh.oeaw.ac.at/vocabs/defcthesaurus/retouched_tool/3.010> skos:narrower <https://acdh.oeaw.ac.at/vocabs/defcthesaurus/cicrular_scraper/4.4> .

<https://acdh.oeaw.ac.at/vocabs/defcthesaurus/denticulate/4.5> a skos:Concept ;
	skos:prefLabel "denticulate"@en , "gez채hnt"@de ;
	skos:altLabel "denticulated tool"@en ;
	skos:definition "A blade or flake with several small tooth-like (dentate or serrated) notches on the working edge." ;
	skos:inScheme <https://acdh.oeaw.ac.at/vocabs/defcthesaurus/FindsSchema> , <https://acdh.oeaw.ac.at/vocabs/defcthesaurus/FindsLithicsRetouchedTools> ;
	skos:editorialNote "dc_finds_lithics_retouched_tools;5" ;
	skos:broader <https://acdh.oeaw.ac.at/vocabs/defcthesaurus/retouched_tool/3.010> .

<https://acdh.oeaw.ac.at/vocabs/defcthesaurus/retouched_tool/3.010> skos:narrower <https://acdh.oeaw.ac.at/vocabs/defcthesaurus/denticulate/4.5> .

<https://acdh.oeaw.ac.at/vocabs/defcthesaurus/double_truncation/4.6> a skos:Concept ;
	skos:prefLabel "double truncation"@en ;
	skos:definition "A blade with a steep retouch made on both broken ends." ;
	skos:inScheme <https://acdh.oeaw.ac.at/vocabs/defcthesaurus/FindsSchema> , <https://acdh.oeaw.ac.at/vocabs/defcthesaurus/FindsLithicsRetouchedTools> ;
	skos:editorialNote "dc_finds_lithics_retouched_tools;6" ;
	skos:broader <https://acdh.oeaw.ac.at/vocabs/defcthesaurus/retouched_tool/3.010> .

<https://acdh.oeaw.ac.at/vocabs/defcthesaurus/retouched_tool/3.010> skos:narrower <https://acdh.oeaw.ac.at/vocabs/defcthesaurus/double_truncation/4.6> .

<https://acdh.oeaw.ac.at/vocabs/defcthesaurus/double-baked_blade/4.7> a skos:Concept ;
	skos:prefLabel "double-baked blade"@en ;
	skos:definition "A blade with both blunted edges. According to size, backed blades are different from backed bladelets, which belong to the category of microliths." ;
	skos:inScheme <https://acdh.oeaw.ac.at/vocabs/defcthesaurus/FindsSchema> , <https://acdh.oeaw.ac.at/vocabs/defcthesaurus/FindsLithicsRetouchedTools> ;
	skos:editorialNote "dc_finds_lithics_retouched_tools;7" ;
	skos:broader <https://acdh.oeaw.ac.at/vocabs/defcthesaurus/retouched_tool/3.010> .

<https://acdh.oeaw.ac.at/vocabs/defcthesaurus/retouched_tool/3.010> skos:narrower <https://acdh.oeaw.ac.at/vocabs/defcthesaurus/double-baked_blade/4.7> .

<https://acdh.oeaw.ac.at/vocabs/defcthesaurus/drill/4.8> a skos:Concept ;
	skos:prefLabel "drill"@en , "Bohrer"@de ;
	skos:altLabel "preforator"@en , "borer"@en ;
	skos:definition "A blade (or rarely flake) where a retoch forms a pointed end used for making holes." ;
	skos:inScheme <https://acdh.oeaw.ac.at/vocabs/defcthesaurus/FindsSchema> , <https://acdh.oeaw.ac.at/vocabs/defcthesaurus/FindsLithicsRetouchedTools> ;
	skos:editorialNote "dc_finds_lithics_retouched_tools;8" ;
	skos:broader <https://acdh.oeaw.ac.at/vocabs/defcthesaurus/retouched_tool/3.010> .

<https://acdh.oeaw.ac.at/vocabs/defcthesaurus/retouched_tool/3.010> skos:narrower <https://acdh.oeaw.ac.at/vocabs/defcthesaurus/drill/4.8> .

<https://acdh.oeaw.ac.at/vocabs/defcthesaurus/end-scraper_on_blade/4.9> a skos:Concept ;
	skos:prefLabel "end-scraper on blade"@en , "Kratzerstirn auf Klinge"@de ;
	skos:definition "A tool with retouches on a single edge at one end of a blade, accross its long axis. The retouched of a scraper is bigger than 60째. The tool was possibly used for flensing or softening hides and to dress skins." ;
	skos:inScheme <https://acdh.oeaw.ac.at/vocabs/defcthesaurus/FindsSchema> , <https://acdh.oeaw.ac.at/vocabs/defcthesaurus/FindsLithicsRetouchedTools> ;
	skos:editorialNote "dc_finds_lithics_retouched_tools;9" ;
	skos:broader <https://acdh.oeaw.ac.at/vocabs/defcthesaurus/retouched_tool/3.010> .

<https://acdh.oeaw.ac.at/vocabs/defcthesaurus/retouched_tool/3.010> skos:narrower <https://acdh.oeaw.ac.at/vocabs/defcthesaurus/end-scraper_on_blade/4.9> .

<https://acdh.oeaw.ac.at/vocabs/defcthesaurus/end-scraper_on_flake/4.10> a skos:Concept ;
	skos:prefLabel "end-scraper on flake"@en , "Kratzerstirn auf Abschlag"@de ;
	skos:definition "A tool with retouches on a single edge at one end of a flake, accross its long axis. The retouched of a scraper is bigger than 60째. The tool was possibly used for flensing or softening hides and to dress skins." ;
	skos:inScheme <https://acdh.oeaw.ac.at/vocabs/defcthesaurus/FindsSchema> , <https://acdh.oeaw.ac.at/vocabs/defcthesaurus/FindsLithicsRetouchedTools> ;
	skos:editorialNote "dc_finds_lithics_retouched_tools;10" ;
	skos:broader <https://acdh.oeaw.ac.at/vocabs/defcthesaurus/retouched_tool/3.010> .

<https://acdh.oeaw.ac.at/vocabs/defcthesaurus/retouched_tool/3.010> skos:narrower <https://acdh.oeaw.ac.at/vocabs/defcthesaurus/end-scraper_on_flake/4.10> .

<https://acdh.oeaw.ac.at/vocabs/defcthesaurus/high_scraper/4.11> a skos:Concept ;
	skos:prefLabel "high scraper"@en ;
	skos:altLabel "thick scraper"@en ;
	skos:definition "An end- or circular scraper with the retouch making scraper edge angle almost 90째." ;
	skos:inScheme <https://acdh.oeaw.ac.at/vocabs/defcthesaurus/FindsSchema> , <https://acdh.oeaw.ac.at/vocabs/defcthesaurus/FindsLithicsRetouchedTools> ;
	skos:editorialNote "dc_finds_lithics_retouched_tools;11" ;
	skos:broader <https://acdh.oeaw.ac.at/vocabs/defcthesaurus/retouched_tool/3.010> .

<https://acdh.oeaw.ac.at/vocabs/defcthesaurus/retouched_tool/3.010> skos:narrower <https://acdh.oeaw.ac.at/vocabs/defcthesaurus/high_scraper/4.11> .

<https://acdh.oeaw.ac.at/vocabs/defcthesaurus/knife/4.12> a skos:Concept ;
	skos:prefLabel "knife"@en ;
	skos:definition "A backed blade; a cutting instrument composed of a blade and a handle into which it is fixed, either rigidly or with a joint." ;
	skos:inScheme <https://acdh.oeaw.ac.at/vocabs/defcthesaurus/FindsSchema> , <https://acdh.oeaw.ac.at/vocabs/defcthesaurus/FindsLithicsRetouchedTools> ;
	skos:editorialNote "dc_finds_lithics_retouched_tools;12" ;
	skos:broader <https://acdh.oeaw.ac.at/vocabs/defcthesaurus/retouched_tool/3.010> .

<https://acdh.oeaw.ac.at/vocabs/defcthesaurus/retouched_tool/3.010> skos:narrower <https://acdh.oeaw.ac.at/vocabs/defcthesaurus/knife/4.12> .

<https://acdh.oeaw.ac.at/vocabs/defcthesaurus/micro_end-scraper/4.13> a skos:Concept ;
	skos:prefLabel "micro end-scraper"@en , "Mikrokratzer"@de ;
	skos:altLabel "micro end scraper"@en ;
	skos:definition "Every scraper with the length or width less than 25mm. According to the size, it can belong to the category of microliths." ;
	skos:inScheme <https://acdh.oeaw.ac.at/vocabs/defcthesaurus/FindsSchema> , <https://acdh.oeaw.ac.at/vocabs/defcthesaurus/FindsLithicsRetouchedTools> ;
	skos:editorialNote "dc_finds_lithics_retouched_tools;13" ;
	skos:broader <https://acdh.oeaw.ac.at/vocabs/defcthesaurus/retouched_tool/3.010> .

<https://acdh.oeaw.ac.at/vocabs/defcthesaurus/retouched_tool/3.010> skos:narrower <https://acdh.oeaw.ac.at/vocabs/defcthesaurus/micro_end-scraper/4.13> .

<https://acdh.oeaw.ac.at/vocabs/defcthesaurus/notch/4.14> a skos:Concept ;
	skos:prefLabel "notch"@en , "Kerbe"@de ;
	skos:altLabel "notched tool"@en ;
	skos:definition "A term describing a tool with the delineation of an edge, indicating a sharp dent, generaly concave, sometimes V-shaped, with a small curvature radius, and created by carious retouch techniques." ;
	skos:inScheme <https://acdh.oeaw.ac.at/vocabs/defcthesaurus/FindsSchema> , <https://acdh.oeaw.ac.at/vocabs/defcthesaurus/FindsLithicsRetouchedTools> ;
	skos:editorialNote "dc_finds_lithics_retouched_tools;14" ;
	skos:broader <https://acdh.oeaw.ac.at/vocabs/defcthesaurus/retouched_tool/3.010> .

<https://acdh.oeaw.ac.at/vocabs/defcthesaurus/retouched_tool/3.010> skos:narrower <https://acdh.oeaw.ac.at/vocabs/defcthesaurus/notch/4.14> .

<https://acdh.oeaw.ac.at/vocabs/defcthesaurus/projectile_point/4.15> a skos:Concept ;
	skos:prefLabel "projectile point"@en , "Projektilspitze"@de ;
	skos:altLabel "arrowhead"@en , "point"@en ;
	skos:definition "A pointed retouched artefact, with or without tang for hafting, used for the purposes of hunting or warfare." ;
	skos:inScheme <https://acdh.oeaw.ac.at/vocabs/defcthesaurus/FindsSchema> , <https://acdh.oeaw.ac.at/vocabs/defcthesaurus/FindsLithicsRetouchedTools> ;
	skos:editorialNote "dc_finds_lithics_retouched_tools;15" ;
	skos:broader <https://acdh.oeaw.ac.at/vocabs/defcthesaurus/retouched_tool/3.010> .

<https://acdh.oeaw.ac.at/vocabs/defcthesaurus/retouched_tool/3.010> skos:narrower <https://acdh.oeaw.ac.at/vocabs/defcthesaurus/projectile_point/4.15> .

<https://acdh.oeaw.ac.at/vocabs/defcthesaurus/retouched_blade/4.16> a skos:Concept ;
	skos:prefLabel "retouched blade"@en , "retuschierte Klinge"@de ;
	skos:definition "A blade with retouch on one or both edges." ;
	skos:inScheme <https://acdh.oeaw.ac.at/vocabs/defcthesaurus/FindsSchema> , <https://acdh.oeaw.ac.at/vocabs/defcthesaurus/FindsLithicsRetouchedTools> ;
	skos:editorialNote "dc_finds_lithics_retouched_tools;16" ;
	skos:broader <https://acdh.oeaw.ac.at/vocabs/defcthesaurus/retouched_tool/3.010> .

<https://acdh.oeaw.ac.at/vocabs/defcthesaurus/retouched_tool/3.010> skos:narrower <https://acdh.oeaw.ac.at/vocabs/defcthesaurus/retouched_blade/4.16> .

<https://acdh.oeaw.ac.at/vocabs/defcthesaurus/retouched_flake/4.17> a skos:Concept ;
	skos:prefLabel "retouched flake"@en , "retuschirter Abschlag"@de ;
	skos:definition "A flake with retouches on one or both edges." ;
	skos:inScheme <https://acdh.oeaw.ac.at/vocabs/defcthesaurus/FindsSchema> , <https://acdh.oeaw.ac.at/vocabs/defcthesaurus/FindsLithicsRetouchedTools> ;
	skos:editorialNote "dc_finds_lithics_retouched_tools;17" ;
	skos:broader <https://acdh.oeaw.ac.at/vocabs/defcthesaurus/retouched_tool/3.010> .

<https://acdh.oeaw.ac.at/vocabs/defcthesaurus/retouched_tool/3.010> skos:narrower <https://acdh.oeaw.ac.at/vocabs/defcthesaurus/retouched_flake/4.17> .

<https://acdh.oeaw.ac.at/vocabs/defcthesaurus/segment/4.18> a skos:Concept ;
	skos:prefLabel "segment"@en ;
	skos:altLabel "lunate"@en ;
	skos:definition "A geometric microlith, made on a blade or bladelet and shaped like a half moon; the backing is along a curved arc opposite a straight unretouched edge. It was hafted, possibly as a projectile tip or as part of a cutting tool." ;
	skos:inScheme <https://acdh.oeaw.ac.at/vocabs/defcthesaurus/FindsSchema> , <https://acdh.oeaw.ac.at/vocabs/defcthesaurus/FindsLithicsRetouchedTools> ;
	skos:editorialNote "dc_finds_lithics_retouched_tools;18" ;
	skos:broader <https://acdh.oeaw.ac.at/vocabs/defcthesaurus/retouched_tool/3.010> .

<https://acdh.oeaw.ac.at/vocabs/defcthesaurus/retouched_tool/3.010> skos:narrower <https://acdh.oeaw.ac.at/vocabs/defcthesaurus/segment/4.18> .

<https://acdh.oeaw.ac.at/vocabs/defcthesaurus/sickle_blade/4.19> a skos:Concept ;
	skos:prefLabel "sickle blade"@en ;
	skos:definition "A blade (rarely flake) with the gloss which occurs on the edge of the artefact, and which is caused by the wear of the blade against the phytoliths in the grasses being reaped. Usually inserted in a bone, antler or wooden handle, as a part of composite to" ;
	skos:inScheme <https://acdh.oeaw.ac.at/vocabs/defcthesaurus/FindsSchema> , <https://acdh.oeaw.ac.at/vocabs/defcthesaurus/FindsLithicsRetouchedTools> ;
	skos:editorialNote "dc_finds_lithics_retouched_tools;19" ;
	skos:broader <https://acdh.oeaw.ac.at/vocabs/defcthesaurus/retouched_tool/3.010> .

<https://acdh.oeaw.ac.at/vocabs/defcthesaurus/retouched_tool/3.010> skos:narrower <https://acdh.oeaw.ac.at/vocabs/defcthesaurus/sickle_blade/4.19> .

<https://acdh.oeaw.ac.at/vocabs/defcthesaurus/side-scraper/4.20> a skos:Concept ;
	skos:prefLabel "side-scraper"@en , "Schaber"@de ;
	skos:altLabel "side scraper"@en ;
	skos:definition "A tool with a retouch on one or both lateral edge of a flake." ;
	skos:inScheme <https://acdh.oeaw.ac.at/vocabs/defcthesaurus/FindsSchema> , <https://acdh.oeaw.ac.at/vocabs/defcthesaurus/FindsLithicsRetouchedTools> ;
	skos:editorialNote "dc_finds_lithics_retouched_tools;20" ;
	skos:broader <https://acdh.oeaw.ac.at/vocabs/defcthesaurus/retouched_tool/3.010> .

<https://acdh.oeaw.ac.at/vocabs/defcthesaurus/retouched_tool/3.010> skos:narrower <https://acdh.oeaw.ac.at/vocabs/defcthesaurus/side-scraper/4.20> .

<https://acdh.oeaw.ac.at/vocabs/defcthesaurus/splinter/4.21> a skos:Concept ;
	skos:prefLabel "splinter"@en , "Tr체mmer"@de ;
	skos:altLabel "Non-flake"@en ;
	skos:definition "A type of chipped stone artifact manufactured by the bipolar percussion technique, used for spliting a wood on two pieces. synonym: piece esquillee." ;
	skos:inScheme <https://acdh.oeaw.ac.at/vocabs/defcthesaurus/FindsSchema> , <https://acdh.oeaw.ac.at/vocabs/defcthesaurus/FindsLithicsRetouchedTools> ;
	skos:editorialNote "dc_finds_lithics_retouched_tools;21" ;
	skos:broader <https://acdh.oeaw.ac.at/vocabs/defcthesaurus/retouched_tool/3.010> .

<https://acdh.oeaw.ac.at/vocabs/defcthesaurus/retouched_tool/3.010> skos:narrower <https://acdh.oeaw.ac.at/vocabs/defcthesaurus/splinter/4.21> .

<https://acdh.oeaw.ac.at/vocabs/defcthesaurus/trapeze/4.22> a skos:Concept ;
	skos:prefLabel "trapeze"@en , "Trapez"@de ;
	skos:definition "A geometric microlith whose outline has four sides - two lateral nearly parallel sides with the longer one being the cutting edge and the shorter opposite edge backed or not-backed. Also called transverse arrowhead." ;
	skos:inScheme <https://acdh.oeaw.ac.at/vocabs/defcthesaurus/FindsSchema> , <https://acdh.oeaw.ac.at/vocabs/defcthesaurus/FindsLithicsRetouchedTools> ;
	skos:editorialNote "dc_finds_lithics_retouched_tools;22" ;
	skos:broader <https://acdh.oeaw.ac.at/vocabs/defcthesaurus/retouched_tool/3.010> .

<https://acdh.oeaw.ac.at/vocabs/defcthesaurus/retouched_tool/3.010> skos:narrower <https://acdh.oeaw.ac.at/vocabs/defcthesaurus/trapeze/4.22> .

<https://acdh.oeaw.ac.at/vocabs/defcthesaurus/truncation/4.23> a skos:Concept ;
	skos:prefLabel "truncation"@en , "Endretusche"@de ;
	skos:definition "A blade with a steep retouch made on a broken end." ;
	skos:inScheme <https://acdh.oeaw.ac.at/vocabs/defcthesaurus/FindsSchema> , <https://acdh.oeaw.ac.at/vocabs/defcthesaurus/FindsLithicsRetouchedTools> ;
	skos:editorialNote "dc_finds_lithics_retouched_tools;23" ;
	skos:broader <https://acdh.oeaw.ac.at/vocabs/defcthesaurus/retouched_tool/3.010> .

<https://acdh.oeaw.ac.at/vocabs/defcthesaurus/retouched_tool/3.010> skos:narrower <https://acdh.oeaw.ac.at/vocabs/defcthesaurus/truncation/4.23> .

<https://acdh.oeaw.ac.at/vocabs/defcthesaurus/unretouched_tool/3.011> a skos:Concept ;
	skos:prefLabel "unretouched tool"@en ;
	skos:inScheme <https://acdh.oeaw.ac.at/vocabs/defcthesaurus/FindsSchema> , <https://acdh.oeaw.ac.at/vocabs/defcthesaurus/NotInDatabase> ;
	skos:editorialNote "dc_not_in_database;011" ;
	skos:broader <https://acdh.oeaw.ac.at/vocabs/defcthesaurus/lithics/2.3> .

<https://acdh.oeaw.ac.at/vocabs/defcthesaurus/lithics/2.3> skos:narrower <https://acdh.oeaw.ac.at/vocabs/defcthesaurus/unretouched_tool/3.011> .

<https://acdh.oeaw.ac.at/vocabs/defcthesaurus/FindsLithicsUnretouchedTools> a skos:ConceptScheme ;
	rdfs:comment "A concept schema related to the particular finds properties." .

<https://acdh.oeaw.ac.at/vocabs/defcthesaurus/lithics/2.3> dc:source "Kipfer, B. A. Dictionary of Artifacts 2007. Blackwell Publishing, Oxford.p.37" .

<https://acdh.oeaw.ac.at/vocabs/defcthesaurus/blade/4.1> a skos:Concept ;
	skos:prefLabel "blade"@en , "Klinge"@de ;
	skos:definition "A long, narrow, sharp-edged, thin flake of stone, used especially as a tool. This flake was detached by striking from a prepared core, often with a hammer. Ist length is usually at least twice the width. The blade may be a tool in itself, or may be the bl" ;
	skos:inScheme <https://acdh.oeaw.ac.at/vocabs/defcthesaurus/FindsSchema> , <https://acdh.oeaw.ac.at/vocabs/defcthesaurus/FindsLithicsUnretouchedTools> ;
	skos:editorialNote "dc_finds_lithics_unretouched_tools;1" ;
	skos:broader <https://acdh.oeaw.ac.at/vocabs/defcthesaurus/unretouched_tool/3.011> .

<https://acdh.oeaw.ac.at/vocabs/defcthesaurus/unretouched_tool/3.011> skos:narrower <https://acdh.oeaw.ac.at/vocabs/defcthesaurus/blade/4.1> .

<https://acdh.oeaw.ac.at/vocabs/defcthesaurus/bladelet/4.2> a skos:Concept ;
	skos:prefLabel "bladelet"@en ;
	skos:definition "A narrow blade which usually can be defined with the width less than 12mm. (Micro-blade would be then a small blade with the width under 8mm)." ;
	skos:inScheme <https://acdh.oeaw.ac.at/vocabs/defcthesaurus/FindsSchema> , <https://acdh.oeaw.ac.at/vocabs/defcthesaurus/FindsLithicsUnretouchedTools> ;
	skos:editorialNote "dc_finds_lithics_unretouched_tools;2" ;
	skos:broader <https://acdh.oeaw.ac.at/vocabs/defcthesaurus/unretouched_tool/3.011> .

<https://acdh.oeaw.ac.at/vocabs/defcthesaurus/unretouched_tool/3.011> skos:narrower <https://acdh.oeaw.ac.at/vocabs/defcthesaurus/bladelet/4.2> .

<https://acdh.oeaw.ac.at/vocabs/defcthesaurus/flake/4.3> a skos:Concept ;
	skos:prefLabel "flake"@en , "Abschlag"@de ;
	skos:inScheme <https://acdh.oeaw.ac.at/vocabs/defcthesaurus/FindsSchema> , <https://acdh.oeaw.ac.at/vocabs/defcthesaurus/FindsLithicsUnretouchedTools> ;
	skos:editorialNote "dc_finds_lithics_unretouched_tools;3" ;
	skos:broader <https://acdh.oeaw.ac.at/vocabs/defcthesaurus/unretouched_tool/3.011> .

<https://acdh.oeaw.ac.at/vocabs/defcthesaurus/unretouched_tool/3.011> skos:narrower <https://acdh.oeaw.ac.at/vocabs/defcthesaurus/flake/4.3> .

<https://acdh.oeaw.ac.at/vocabs/defcthesaurus/microblade/4.4> a skos:Concept ;
	skos:prefLabel "microblade"@en ;
	skos:inScheme <https://acdh.oeaw.ac.at/vocabs/defcthesaurus/FindsSchema> , <https://acdh.oeaw.ac.at/vocabs/defcthesaurus/FindsLithicsUnretouchedTools> ;
	skos:editorialNote "dc_finds_lithics_unretouched_tools;4" ;
	skos:broader <https://acdh.oeaw.ac.at/vocabs/defcthesaurus/unretouched_tool/3.011> .

<https://acdh.oeaw.ac.at/vocabs/defcthesaurus/unretouched_tool/3.011> skos:narrower <https://acdh.oeaw.ac.at/vocabs/defcthesaurus/microblade/4.4> .

<https://acdh.oeaw.ac.at/vocabs/defcthesaurus/y_blade/4.5> a skos:Concept ;
	skos:prefLabel "y blade"@en , "Y Klinge"@de ;
	skos:inScheme <https://acdh.oeaw.ac.at/vocabs/defcthesaurus/FindsSchema> , <https://acdh.oeaw.ac.at/vocabs/defcthesaurus/FindsLithicsUnretouchedTools> ;
	skos:editorialNote "dc_finds_lithics_unretouched_tools;5" ;
	skos:broader <https://acdh.oeaw.ac.at/vocabs/defcthesaurus/unretouched_tool/3.011> .

<https://acdh.oeaw.ac.at/vocabs/defcthesaurus/unretouched_tool/3.011> skos:narrower <https://acdh.oeaw.ac.at/vocabs/defcthesaurus/y_blade/4.5> .

<https://acdh.oeaw.ac.at/vocabs/defcthesaurus/core/3.012> a skos:Concept ;
	skos:prefLabel "core"@en , "Kerne"@de ;
	skos:inScheme <https://acdh.oeaw.ac.at/vocabs/defcthesaurus/FindsSchema> , <https://acdh.oeaw.ac.at/vocabs/defcthesaurus/NotInDatabase> ;
	skos:editorialNote "dc_not_in_database;012" ;
	skos:broader <https://acdh.oeaw.ac.at/vocabs/defcthesaurus/lithics/2.3> .

<https://acdh.oeaw.ac.at/vocabs/defcthesaurus/lithics/2.3> skos:narrower <https://acdh.oeaw.ac.at/vocabs/defcthesaurus/core/3.012> .

<https://acdh.oeaw.ac.at/vocabs/defcthesaurus/FindsLithicsCoreShape> a skos:ConceptScheme ;
	rdfs:comment "A concept schema related to the particular finds properties." .

<https://acdh.oeaw.ac.at/vocabs/defcthesaurus/lithics/2.3> dc:source "OREA" .

<https://acdh.oeaw.ac.at/vocabs/defcthesaurus/bidirectional_core/4.1> a skos:Concept ;
	skos:prefLabel "bidirectional core"@en , "bidirektionaler Kern"@de ;
	skos:altLabel "bifacial core"@en , "Bi-directional core"@en ;
	skos:definition "A core with two, opposed knapping platforms." ;
	skos:inScheme <https://acdh.oeaw.ac.at/vocabs/defcthesaurus/FindsSchema> , <https://acdh.oeaw.ac.at/vocabs/defcthesaurus/FindsLithicsCoreShape> ;
	skos:editorialNote "dc_finds_lithics_core_shape;1" ;
	skos:broader <https://acdh.oeaw.ac.at/vocabs/defcthesaurus/core/3.012> .

<https://acdh.oeaw.ac.at/vocabs/defcthesaurus/core/3.012> skos:narrower <https://acdh.oeaw.ac.at/vocabs/defcthesaurus/bidirectional_core/4.1> .

<https://acdh.oeaw.ac.at/vocabs/defcthesaurus/blade_core/4.2> a skos:Concept ;
	skos:prefLabel "blade core"@en , "Klingenkern"@de ;
	skos:altLabel "Blade-core"@en ;
	skos:definition "A core which main reduction leads to the detachment of blades (aim of knapping-blades)." ;
	skos:inScheme <https://acdh.oeaw.ac.at/vocabs/defcthesaurus/FindsSchema> , <https://acdh.oeaw.ac.at/vocabs/defcthesaurus/FindsLithicsCoreShape> ;
	skos:editorialNote "dc_finds_lithics_core_shape;2" ;
	skos:broader <https://acdh.oeaw.ac.at/vocabs/defcthesaurus/core/3.012> .

<https://acdh.oeaw.ac.at/vocabs/defcthesaurus/core/3.012> skos:narrower <https://acdh.oeaw.ac.at/vocabs/defcthesaurus/blade_core/4.2> .

<https://acdh.oeaw.ac.at/vocabs/defcthesaurus/bullet_core/4.3> a skos:Concept ;
	skos:prefLabel "bullet core"@en , "Bullet core"@de ;
	skos:definition "A blade core which completeexhaustion leads to the bullet shape." ;
	skos:inScheme <https://acdh.oeaw.ac.at/vocabs/defcthesaurus/FindsSchema> , <https://acdh.oeaw.ac.at/vocabs/defcthesaurus/FindsLithicsCoreShape> ;
	skos:editorialNote "dc_finds_lithics_core_shape;3" ;
	skos:broader <https://acdh.oeaw.ac.at/vocabs/defcthesaurus/core/3.012> .

<https://acdh.oeaw.ac.at/vocabs/defcthesaurus/core/3.012> skos:narrower <https://acdh.oeaw.ac.at/vocabs/defcthesaurus/bullet_core/4.3> .

<https://acdh.oeaw.ac.at/vocabs/defcthesaurus/conical_core/4.4> a skos:Concept ;
	skos:prefLabel "conical core"@en ;
	skos:definition "A blade core of a conical shape." ;
	skos:inScheme <https://acdh.oeaw.ac.at/vocabs/defcthesaurus/FindsSchema> , <https://acdh.oeaw.ac.at/vocabs/defcthesaurus/FindsLithicsCoreShape> ;
	skos:editorialNote "dc_finds_lithics_core_shape;4" ;
	skos:broader <https://acdh.oeaw.ac.at/vocabs/defcthesaurus/core/3.012> .

<https://acdh.oeaw.ac.at/vocabs/defcthesaurus/core/3.012> skos:narrower <https://acdh.oeaw.ac.at/vocabs/defcthesaurus/conical_core/4.4> .

<https://acdh.oeaw.ac.at/vocabs/defcthesaurus/core_fragment/4.5> a skos:Concept ;
	skos:prefLabel "core fragment"@en ;
	skos:definition "A fragment of a core (regardless typology, used when the core is incomplete, or the main type cannot be determined due to fragmentation)" ;
	skos:inScheme <https://acdh.oeaw.ac.at/vocabs/defcthesaurus/FindsSchema> , <https://acdh.oeaw.ac.at/vocabs/defcthesaurus/FindsLithicsCoreShape> ;
	skos:editorialNote "dc_finds_lithics_core_shape;5" ;
	skos:broader <https://acdh.oeaw.ac.at/vocabs/defcthesaurus/core/3.012> .

<https://acdh.oeaw.ac.at/vocabs/defcthesaurus/core/3.012> skos:narrower <https://acdh.oeaw.ac.at/vocabs/defcthesaurus/core_fragment/4.5> .

<https://acdh.oeaw.ac.at/vocabs/defcthesaurus/core_preparation/3.013> a skos:Concept ;
	skos:prefLabel "core preparation"@en ;
	skos:inScheme <https://acdh.oeaw.ac.at/vocabs/defcthesaurus/FindsSchema> ;
	skos:broader <https://acdh.oeaw.ac.at/vocabs/defcthesaurus/lithics/2.3> .

<https://acdh.oeaw.ac.at/vocabs/defcthesaurus/cortical_blade/4.6> a skos:Concept ;
	skos:prefLabel "cortical blade"@en ;
	skos:inScheme <https://acdh.oeaw.ac.at/vocabs/defcthesaurus/FindsSchema> , <https://acdh.oeaw.ac.at/vocabs/defcthesaurus/FindsLithicsCoreShape> ;
	skos:editorialNote "dc_finds_lithics_core_shape;6" ;
	skos:broader <https://acdh.oeaw.ac.at/vocabs/defcthesaurus/core_preparation/3.013> .

<https://acdh.oeaw.ac.at/vocabs/defcthesaurus/core_preparation/3.013> skos:narrower <https://acdh.oeaw.ac.at/vocabs/defcthesaurus/cortical_blade/4.6> .

<https://acdh.oeaw.ac.at/vocabs/defcthesaurus/lithics/2.3> skos:narrower <https://acdh.oeaw.ac.at/vocabs/defcthesaurus/core_preparation/3.013> .

<https://acdh.oeaw.ac.at/vocabs/defcthesaurus/crested_blade/4.7> a skos:Concept ;
	skos:prefLabel "crested blade"@en ;
	skos:inScheme <https://acdh.oeaw.ac.at/vocabs/defcthesaurus/FindsSchema> , <https://acdh.oeaw.ac.at/vocabs/defcthesaurus/FindsLithicsCoreShape> ;
	skos:editorialNote "dc_finds_lithics_core_shape;7" ;
	skos:broader <https://acdh.oeaw.ac.at/vocabs/defcthesaurus/core_preparation/3.013> .

<https://acdh.oeaw.ac.at/vocabs/defcthesaurus/core_preparation/3.013> skos:narrower <https://acdh.oeaw.ac.at/vocabs/defcthesaurus/crested_blade/4.7> .

<https://acdh.oeaw.ac.at/vocabs/defcthesaurus/crested_flake/4.8> a skos:Concept ;
	skos:prefLabel "crested flake"@en ;
	skos:inScheme <https://acdh.oeaw.ac.at/vocabs/defcthesaurus/FindsSchema> , <https://acdh.oeaw.ac.at/vocabs/defcthesaurus/FindsLithicsCoreShape> ;
	skos:editorialNote "dc_finds_lithics_core_shape;8" ;
	skos:broader <https://acdh.oeaw.ac.at/vocabs/defcthesaurus/core_preparation/3.013> .

<https://acdh.oeaw.ac.at/vocabs/defcthesaurus/core_preparation/3.013> skos:narrower <https://acdh.oeaw.ac.at/vocabs/defcthesaurus/crested_flake/4.8> .

<https://acdh.oeaw.ac.at/vocabs/defcthesaurus/flake_core/4.9> a skos:Concept ;
	skos:prefLabel "flake core"@en , "Abschlagkern"@de ;
	skos:altLabel "Flake-core"@en ;
	skos:definition "A core which main reduction leads to thedetachment of flakes (aim of knapping-flakes)." ;
	skos:inScheme <https://acdh.oeaw.ac.at/vocabs/defcthesaurus/FindsSchema> , <https://acdh.oeaw.ac.at/vocabs/defcthesaurus/FindsLithicsCoreShape> ;
	skos:editorialNote "dc_finds_lithics_core_shape;9" ;
	skos:broader <https://acdh.oeaw.ac.at/vocabs/defcthesaurus/core/3.012> .

<https://acdh.oeaw.ac.at/vocabs/defcthesaurus/core/3.012> skos:narrower <https://acdh.oeaw.ac.at/vocabs/defcthesaurus/flake_core/4.9> .

<https://acdh.oeaw.ac.at/vocabs/defcthesaurus/naviform_core/4.10> a skos:Concept ;
	skos:prefLabel "naviform core"@en ;
	skos:definition "Aspecial type of bidirectional core (most common for the area of the Near East)." ;
	skos:inScheme <https://acdh.oeaw.ac.at/vocabs/defcthesaurus/FindsSchema> , <https://acdh.oeaw.ac.at/vocabs/defcthesaurus/FindsLithicsCoreShape> ;
	skos:editorialNote "dc_finds_lithics_core_shape;10" ;
	skos:broader <https://acdh.oeaw.ac.at/vocabs/defcthesaurus/core/3.012> .

<https://acdh.oeaw.ac.at/vocabs/defcthesaurus/core/3.012> skos:narrower <https://acdh.oeaw.ac.at/vocabs/defcthesaurus/naviform_core/4.10> .

<https://acdh.oeaw.ac.at/vocabs/defcthesaurus/tablet/4.11> a skos:Concept ;
	skos:prefLabel "tablet"@en ;
	skos:inScheme <https://acdh.oeaw.ac.at/vocabs/defcthesaurus/FindsSchema> , <https://acdh.oeaw.ac.at/vocabs/defcthesaurus/FindsLithicsCoreShape> ;
	skos:editorialNote "dc_finds_lithics_core_shape;11" ;
	skos:broader <https://acdh.oeaw.ac.at/vocabs/defcthesaurus/core_preparation/3.013> .

<https://acdh.oeaw.ac.at/vocabs/defcthesaurus/core_preparation/3.013> skos:narrower <https://acdh.oeaw.ac.at/vocabs/defcthesaurus/tablet/4.11> .

<https://acdh.oeaw.ac.at/vocabs/defcthesaurus/unidirectional_core/4.12> a skos:Concept ;
	skos:prefLabel "unidirectional core"@en , "unidirektionaler Kern"@de ;
	skos:definition "A core with the main detachment from the one single platform" ;
	skos:inScheme <https://acdh.oeaw.ac.at/vocabs/defcthesaurus/FindsSchema> , <https://acdh.oeaw.ac.at/vocabs/defcthesaurus/FindsLithicsCoreShape> ;
	skos:editorialNote "dc_finds_lithics_core_shape;12" ;
	skos:broader <https://acdh.oeaw.ac.at/vocabs/defcthesaurus/core/3.012> .

<https://acdh.oeaw.ac.at/vocabs/defcthesaurus/core/3.012> skos:narrower <https://acdh.oeaw.ac.at/vocabs/defcthesaurus/unidirectional_core/4.12> .

<https://acdh.oeaw.ac.at/vocabs/defcthesaurus/wedge-shaped_core/4.13> a skos:Concept ;
	skos:prefLabel "wedge-shaped core"@en ;
	skos:definition "Anunidirectional blade core with crested back, usually determined by a frontal reduction. (*when the reduction is all around the platform, the core is conical, while the systematic, regular blade detachment finally leads to bullet core shape)." ;
	skos:inScheme <https://acdh.oeaw.ac.at/vocabs/defcthesaurus/FindsSchema> , <https://acdh.oeaw.ac.at/vocabs/defcthesaurus/FindsLithicsCoreShape> ;
	skos:editorialNote "dc_finds_lithics_core_shape;13" ;
	skos:broader <https://acdh.oeaw.ac.at/vocabs/defcthesaurus/core/3.012> .

<https://acdh.oeaw.ac.at/vocabs/defcthesaurus/core/3.012> skos:narrower <https://acdh.oeaw.ac.at/vocabs/defcthesaurus/wedge-shaped_core/4.13> .

<https://acdh.oeaw.ac.at/vocabs/defcthesaurus/lithic_production/3.014> a skos:Concept ;
	skos:prefLabel "lithic production"@en ;
	skos:inScheme <https://acdh.oeaw.ac.at/vocabs/defcthesaurus/FindsSchema> , <https://acdh.oeaw.ac.at/vocabs/defcthesaurus/NotInDatabase> ;
	skos:editorialNote "dc_not_in_database;014" ;
	skos:broader <https://acdh.oeaw.ac.at/vocabs/defcthesaurus/lithics/2.3> .

<https://acdh.oeaw.ac.at/vocabs/defcthesaurus/lithics/2.3> skos:narrower <https://acdh.oeaw.ac.at/vocabs/defcthesaurus/lithic_production/3.014> .

<https://acdh.oeaw.ac.at/vocabs/defcthesaurus/lithics_technology/4.023> a skos:Concept ;
	skos:prefLabel "lithics technology"@en , "Technologie"@de ;
	skos:inScheme <https://acdh.oeaw.ac.at/vocabs/defcthesaurus/FindsSchema> , <https://acdh.oeaw.ac.at/vocabs/defcthesaurus/NotInDatabase> ;
	skos:editorialNote "dc_not_in_database;023" ;
	skos:broader <https://acdh.oeaw.ac.at/vocabs/defcthesaurus/lithic_production/3.014> .

<https://acdh.oeaw.ac.at/vocabs/defcthesaurus/lithic_production/3.014> skos:narrower <https://acdh.oeaw.ac.at/vocabs/defcthesaurus/lithics_technology/4.023> .

<https://acdh.oeaw.ac.at/vocabs/defcthesaurus/FindsLithicsTechnology> a skos:ConceptScheme ;
	rdfs:comment "A concept schema related to the particular finds properties." .

<https://acdh.oeaw.ac.at/vocabs/defcthesaurus/direct_percussion/5.1> a skos:Concept ;
	skos:prefLabel "direct percussion"@en ;
	skos:definition "The action of striking one object with another. Direct percussion is directly applies by a hammer." ;
	skos:inScheme <https://acdh.oeaw.ac.at/vocabs/defcthesaurus/FindsSchema> , <https://acdh.oeaw.ac.at/vocabs/defcthesaurus/FindsLithicsTechnology> ;
	skos:editorialNote "dc_finds_lithics_technology;1" ;
	skos:broader <https://acdh.oeaw.ac.at/vocabs/defcthesaurus/lithics_technology/4.023> .

<https://acdh.oeaw.ac.at/vocabs/defcthesaurus/lithics_technology/4.023> skos:narrower <https://acdh.oeaw.ac.at/vocabs/defcthesaurus/direct_percussion/5.1> .

<https://acdh.oeaw.ac.at/vocabs/defcthesaurus/indirect_percussion/5.2> a skos:Concept ;
	skos:prefLabel "indirect percussion"@en ;
	skos:definition "The action of striking one object with another. Indirect percussion involves an intermediate object (a punch) as well as a hammer." ;
	skos:inScheme <https://acdh.oeaw.ac.at/vocabs/defcthesaurus/FindsSchema> , <https://acdh.oeaw.ac.at/vocabs/defcthesaurus/FindsLithicsTechnology> ;
	skos:editorialNote "dc_finds_lithics_technology;2" ;
	skos:broader <https://acdh.oeaw.ac.at/vocabs/defcthesaurus/lithics_technology/4.023> .

<https://acdh.oeaw.ac.at/vocabs/defcthesaurus/lithics_technology/4.023> skos:narrower <https://acdh.oeaw.ac.at/vocabs/defcthesaurus/indirect_percussion/5.2> .

<https://acdh.oeaw.ac.at/vocabs/defcthesaurus/pressure_technique/5.3> a skos:Concept ;
	skos:prefLabel "pressure technique"@en ;
	skos:definition "Application of pressure to fracture raw materials. Pressure is applied with the narrow end of a tool made of wood, antler, bone or metal." ;
	skos:inScheme <https://acdh.oeaw.ac.at/vocabs/defcthesaurus/FindsSchema> , <https://acdh.oeaw.ac.at/vocabs/defcthesaurus/FindsLithicsTechnology> ;
	skos:editorialNote "dc_finds_lithics_technology;3" ;
	skos:broader <https://acdh.oeaw.ac.at/vocabs/defcthesaurus/lithics_technology/4.023> .

<https://acdh.oeaw.ac.at/vocabs/defcthesaurus/lithics_technology/4.023> skos:narrower <https://acdh.oeaw.ac.at/vocabs/defcthesaurus/pressure_technique/5.3> .

<https://acdh.oeaw.ac.at/vocabs/defcthesaurus/lithics_industry/4.024> a skos:Concept ;
	skos:prefLabel "lithics industry"@en , "Industrie"@de ;
	skos:inScheme <https://acdh.oeaw.ac.at/vocabs/defcthesaurus/FindsSchema> , <https://acdh.oeaw.ac.at/vocabs/defcthesaurus/NotInDatabase> ;
	skos:editorialNote "dc_not_in_database;024" ;
	skos:broader <https://acdh.oeaw.ac.at/vocabs/defcthesaurus/lithic_production/3.014> .

<https://acdh.oeaw.ac.at/vocabs/defcthesaurus/lithic_production/3.014> skos:narrower <https://acdh.oeaw.ac.at/vocabs/defcthesaurus/lithics_industry/4.024> .

<https://acdh.oeaw.ac.at/vocabs/defcthesaurus/FindsLithicsIndustry> a skos:ConceptScheme ;
	rdfs:comment "A concept schema related to the particular finds properties." .

<https://acdh.oeaw.ac.at/vocabs/defcthesaurus/blade_industry/5.1> a skos:Concept ;
	skos:prefLabel "blade industry"@en ;
	skos:definition "Human action applied to raw materials in order to transform them into blades." ;
	skos:inScheme <https://acdh.oeaw.ac.at/vocabs/defcthesaurus/FindsSchema> , <https://acdh.oeaw.ac.at/vocabs/defcthesaurus/FindsLithicsIndustry> ;
	skos:editorialNote "dc_finds_lithics_industry;1" ;
	skos:broader <https://acdh.oeaw.ac.at/vocabs/defcthesaurus/lithics_industry/4.024> .

<https://acdh.oeaw.ac.at/vocabs/defcthesaurus/lithics_industry/4.024> skos:narrower <https://acdh.oeaw.ac.at/vocabs/defcthesaurus/blade_industry/5.1> .

<https://acdh.oeaw.ac.at/vocabs/defcthesaurus/flake_industry/5.2> a skos:Concept ;
	skos:prefLabel "flake industry"@en ;
	skos:definition "Human action applied to raw materials in order to transform them into flakes." ;
	skos:inScheme <https://acdh.oeaw.ac.at/vocabs/defcthesaurus/FindsSchema> , <https://acdh.oeaw.ac.at/vocabs/defcthesaurus/FindsLithicsIndustry> ;
	skos:editorialNote "dc_finds_lithics_industry;2" ;
	skos:broader <https://acdh.oeaw.ac.at/vocabs/defcthesaurus/lithics_industry/4.024> .

<https://acdh.oeaw.ac.at/vocabs/defcthesaurus/lithics_industry/4.024> skos:narrower <https://acdh.oeaw.ac.at/vocabs/defcthesaurus/flake_industry/5.2> .

<https://acdh.oeaw.ac.at/vocabs/defcthesaurus/microlithic_industry/5.3> a skos:Concept ;
	skos:prefLabel "microlithic industry"@en ;
	skos:definition "Human action applied to raw materials in order to transform them into microliths." ;
	skos:inScheme <https://acdh.oeaw.ac.at/vocabs/defcthesaurus/FindsSchema> , <https://acdh.oeaw.ac.at/vocabs/defcthesaurus/FindsLithicsIndustry> ;
	skos:editorialNote "dc_finds_lithics_industry;3" ;
	skos:broader <https://acdh.oeaw.ac.at/vocabs/defcthesaurus/lithics_industry/4.024> .

<https://acdh.oeaw.ac.at/vocabs/defcthesaurus/lithics_industry/4.024> skos:narrower <https://acdh.oeaw.ac.at/vocabs/defcthesaurus/microlithic_industry/5.3> .

<https://acdh.oeaw.ac.at/vocabs/defcthesaurus/lithic_material/3.015> a skos:Concept ;
	skos:prefLabel "lithic material"@en , "Rohmaterial"@de ;
	skos:definition "Material from which lithic object was made of." ;
	skos:inScheme <https://acdh.oeaw.ac.at/vocabs/defcthesaurus/FindsSchema> , <https://acdh.oeaw.ac.at/vocabs/defcthesaurus/NotInDatabase> ;
	skos:editorialNote "dc_not_in_database;015" ;
	skos:broader <https://acdh.oeaw.ac.at/vocabs/defcthesaurus/lithics/2.3> .

<https://acdh.oeaw.ac.at/vocabs/defcthesaurus/lithics/2.3> skos:narrower <https://acdh.oeaw.ac.at/vocabs/defcthesaurus/lithic_material/3.015> .

<https://acdh.oeaw.ac.at/vocabs/defcthesaurus/stone/4.025> a skos:Concept ;
	skos:prefLabel "stone"@en , "Stein"@de , "rock"@la ;
	skos:definition "Different kinds of stone used to produce lithics." ;
	dc:source "OREA" ;
	skos:inScheme <https://acdh.oeaw.ac.at/vocabs/defcthesaurus/FindsSchema> , <https://acdh.oeaw.ac.at/vocabs/defcthesaurus/NotInDatabase> ;
	skos:editorialNote "dc_not_in_database;025" ;
	skos:broader <https://acdh.oeaw.ac.at/vocabs/defcthesaurus/lithic_material/3.015> .

<https://acdh.oeaw.ac.at/vocabs/defcthesaurus/lithic_material/3.015> skos:narrower <https://acdh.oeaw.ac.at/vocabs/defcthesaurus/stone/4.025> .

<https://acdh.oeaw.ac.at/vocabs/defcthesaurus/FindsLithicsRawMaterial> a skos:ConceptScheme ;
	rdfs:comment "A concept schema related to the particular finds properties." .

<https://acdh.oeaw.ac.at/vocabs/defcthesaurus/obsidian/5.1> a skos:Concept ;
	skos:prefLabel "obsidian"@en , "Obsidian"@de ;
	skos:definition "Obsidian, natural glass of volcanic origin that is formed by the rapid cooling of viscous lava. Obsidian is extremely rich in silica, low in water, and has a chemical composition similar to rhyolite. Used to produce lithics." ;
	skos:inScheme <https://acdh.oeaw.ac.at/vocabs/defcthesaurus/FindsSchema> , <https://acdh.oeaw.ac.at/vocabs/defcthesaurus/FindsLithicsRawMaterial> ;
	skos:editorialNote "dc_finds_lithics_raw_material;1" ;
	skos:broader <https://acdh.oeaw.ac.at/vocabs/defcthesaurus/stone/4.025> .

<https://acdh.oeaw.ac.at/vocabs/defcthesaurus/stone/4.025> skos:narrower <https://acdh.oeaw.ac.at/vocabs/defcthesaurus/obsidian/5.1> .

<https://acdh.oeaw.ac.at/vocabs/defcthesaurus/chert/5.3> a skos:Concept ;
	skos:prefLabel "chert"@en , "Kieselschiefer"@de ;
	skos:altLabel "Gestein"@de ;
	skos:definition "Chert is a very fine-grained quarz and a silica mineral. Several varieties are included under the general term: jasper, chalcedony, agate, flint, porcelanite, and novaculite. In Neolithic it was used for tools and weapon." ;
	skos:inScheme <https://acdh.oeaw.ac.at/vocabs/defcthesaurus/FindsSchema> , <https://acdh.oeaw.ac.at/vocabs/defcthesaurus/FindsLithicsRawMaterial> ;
	skos:editorialNote "dc_finds_lithics_raw_material;3" ;
	skos:broader <https://acdh.oeaw.ac.at/vocabs/defcthesaurus/stone/4.025> .

<https://acdh.oeaw.ac.at/vocabs/defcthesaurus/stone/4.025> skos:narrower <https://acdh.oeaw.ac.at/vocabs/defcthesaurus/chert/5.3> .

<https://acdh.oeaw.ac.at/vocabs/defcthesaurus/finds_type/1.02> dc:source "Encyclopaedia Britannica - https://www.britannica.com/science/chert#ref272901" .

<https://acdh.oeaw.ac.at/vocabs/defcthesaurus/flint/6.2> a skos:Concept ;
	skos:prefLabel "flint"@en , "Flint"@de ;
	skos:definition "Flint os a fine-grained quarz and a silica mineral included under the general term chert. In Neolithic it was used as material source for tools and weapons." ;
	skos:inScheme <https://acdh.oeaw.ac.at/vocabs/defcthesaurus/FindsSchema> , <https://acdh.oeaw.ac.at/vocabs/defcthesaurus/FindsLithicsRawMaterial> ;
	skos:editorialNote "dc_finds_lithics_raw_material;02" ;
	skos:broader <https://acdh.oeaw.ac.at/vocabs/defcthesaurus/chert/5.3> .

<https://acdh.oeaw.ac.at/vocabs/defcthesaurus/chert/5.3> skos:narrower <https://acdh.oeaw.ac.at/vocabs/defcthesaurus/flint/6.2> .

<https://acdh.oeaw.ac.at/vocabs/defcthesaurus/finds_type/1.02> dc:source "https://en.wikipedia.org/wiki/Radiolarite" .

<https://acdh.oeaw.ac.at/vocabs/defcthesaurus/radiolarite/6.9> a skos:Concept ;
	skos:prefLabel "radiolarite"@en , "Radiolarit"@de ;
	skos:definition "Radiolarite is a siliceous, comparatively hard, fine-grained, chert-like, and homogeneous sedimentary rock that is composed predominantly of the microscopic remains of radiolarians used to make stone tools and weapons." ;
	skos:inScheme <https://acdh.oeaw.ac.at/vocabs/defcthesaurus/FindsSchema> , <https://acdh.oeaw.ac.at/vocabs/defcthesaurus/FindsLithicsRawMaterial> ;
	skos:editorialNote "dc_finds_lithics_raw_material;02" ;
	skos:broader <https://acdh.oeaw.ac.at/vocabs/defcthesaurus/chert/5.3> .

<https://acdh.oeaw.ac.at/vocabs/defcthesaurus/chert/5.3> skos:narrower <https://acdh.oeaw.ac.at/vocabs/defcthesaurus/radiolarite/6.9> .

<https://acdh.oeaw.ac.at/vocabs/defcthesaurus/chalcedony/5.4> a skos:Concept ;
	skos:prefLabel "chalcedony"@en , "Chalzedon"@de ;
	skos:definition "A very fine-grained (cryptocrystalline) variety of the silica mineral quartz. A form of chert, it occurs in concretionary, mammillated, or stalactitic forms of waxy lustre and has a compact fibrous structure, a fine splintery fracture, and a great variety. Used to produce lithics." ;
	skos:inScheme <https://acdh.oeaw.ac.at/vocabs/defcthesaurus/FindsSchema> , <https://acdh.oeaw.ac.at/vocabs/defcthesaurus/FindsLithicsRawMaterial> ;
	skos:editorialNote "dc_finds_lithics_raw_material;4" ;
	skos:broader <https://acdh.oeaw.ac.at/vocabs/defcthesaurus/stone/4.025> .

<https://acdh.oeaw.ac.at/vocabs/defcthesaurus/stone/4.025> skos:narrower <https://acdh.oeaw.ac.at/vocabs/defcthesaurus/chalcedony/5.4> .

<https://acdh.oeaw.ac.at/vocabs/defcthesaurus/jasper/5.5> a skos:Concept ;
	skos:prefLabel "jasper"@en , "Jaspis"@de ;
	skos:definition "An opaque, fine-grained or dense variety of the silica mineral chert that exhibits various colours. Chiefly brick red to brownish red, it owes its colour to admixed hematite; but when it occurs with clay admixed, the colour is a yellowish white or gray. Used to produce lithics." ;
	skos:inScheme <https://acdh.oeaw.ac.at/vocabs/defcthesaurus/FindsSchema> , <https://acdh.oeaw.ac.at/vocabs/defcthesaurus/FindsLithicsRawMaterial> ;
	skos:editorialNote "dc_finds_lithics_raw_material;5" ;
	skos:broader <https://acdh.oeaw.ac.at/vocabs/defcthesaurus/stone/4.025> .

<https://acdh.oeaw.ac.at/vocabs/defcthesaurus/stone/4.025> skos:narrower <https://acdh.oeaw.ac.at/vocabs/defcthesaurus/jasper/5.5> .

<https://acdh.oeaw.ac.at/vocabs/defcthesaurus/quartz/5.6> a skos:Concept ;
	skos:prefLabel "quartz"@en ;
	skos:definition "Widely distributed mineral of many varieties that consists primarily of silica, or silicon dioxide (SiO2). Used to produce lithics." ;
	skos:inScheme <https://acdh.oeaw.ac.at/vocabs/defcthesaurus/FindsSchema> , <https://acdh.oeaw.ac.at/vocabs/defcthesaurus/FindsLithicsRawMaterial> ;
	skos:editorialNote "dc_finds_lithics_raw_material;6" ;
	skos:broader <https://acdh.oeaw.ac.at/vocabs/defcthesaurus/stone/4.025> .

<https://acdh.oeaw.ac.at/vocabs/defcthesaurus/stone/4.025> skos:narrower <https://acdh.oeaw.ac.at/vocabs/defcthesaurus/quartz/5.6> .

<https://acdh.oeaw.ac.at/vocabs/defcthesaurus/quartzite/5.8> a skos:Concept ;
	skos:prefLabel "quartzite"@en , "Quarzit"@de ;
	skos:definition "A sandstone that has been converted into a solid quartz rock. Unlike sandstones, quartzites are free from pores and have a smooth fracture. Used to produce lithics." ;
	skos:inScheme <https://acdh.oeaw.ac.at/vocabs/defcthesaurus/FindsSchema> , <https://acdh.oeaw.ac.at/vocabs/defcthesaurus/FindsLithicsRawMaterial> ;
	skos:editorialNote "dc_finds_lithics_raw_material;8" ;
	skos:broader <https://acdh.oeaw.ac.at/vocabs/defcthesaurus/stone/4.025> .

<https://acdh.oeaw.ac.at/vocabs/defcthesaurus/stone/4.025> skos:narrower <https://acdh.oeaw.ac.at/vocabs/defcthesaurus/quartzite/5.8> .

<https://acdh.oeaw.ac.at/vocabs/defcthesaurus/mineral/4.026> a skos:Concept ;
	skos:prefLabel "mineral"@en ;
	skos:definition "A mineral used to produce lithics." ;
	skos:inScheme <https://acdh.oeaw.ac.at/vocabs/defcthesaurus/FindsSchema> , <https://acdh.oeaw.ac.at/vocabs/defcthesaurus/NotInDatabase> ;
	skos:editorialNote "dc_not_in_database;026" ;
	skos:broader <https://acdh.oeaw.ac.at/vocabs/defcthesaurus/lithic_material/3.015> .

<https://acdh.oeaw.ac.at/vocabs/defcthesaurus/lithic_material/3.015> skos:narrower <https://acdh.oeaw.ac.at/vocabs/defcthesaurus/mineral/4.026> .

<https://acdh.oeaw.ac.at/vocabs/defcthesaurus/rock_crystal/5.7> a skos:Concept ;
	skos:prefLabel "rock crystal"@en , "Bergkristall"@de ;
	skos:definition "Rock crystal, transparent variety of the silica mineral quartz that is valued for its clarity and total lack of colour or flaws. Used for carving (lithics)." ;
	skos:inScheme <https://acdh.oeaw.ac.at/vocabs/defcthesaurus/FindsSchema> , <https://acdh.oeaw.ac.at/vocabs/defcthesaurus/FindsLithicsRawMaterial> ;
	skos:editorialNote "dc_finds_lithics_raw_material;7" ;
	skos:broader <https://acdh.oeaw.ac.at/vocabs/defcthesaurus/mineral/4.026> .

<https://acdh.oeaw.ac.at/vocabs/defcthesaurus/mineral/4.026> skos:narrower <https://acdh.oeaw.ac.at/vocabs/defcthesaurus/rock_crystal/5.7> .

<https://acdh.oeaw.ac.at/vocabs/defcthesaurus/small_finds/2.5> a skos:Concept ;
	skos:prefLabel "small finds"@en , "Kleinfund"@de , "Kleinfund"@la ;
	skos:definition "Artifacts that can be picked up and transported, as opposed to features excluding pottery, stone tools and organic finds." ;
	skos:inScheme <https://acdh.oeaw.ac.at/vocabs/defcthesaurus/FindsSchema> , <https://acdh.oeaw.ac.at/vocabs/defcthesaurus/FindsType> ;
	skos:editorialNote "dc_finds_type;5" ;
	skos:broader <https://acdh.oeaw.ac.at/vocabs/defcthesaurus/finds_type/1.02> .

<https://acdh.oeaw.ac.at/vocabs/defcthesaurus/finds_type/1.02> skos:narrower <https://acdh.oeaw.ac.at/vocabs/defcthesaurus/small_finds/2.5> .

<https://acdh.oeaw.ac.at/vocabs/defcthesaurus/SmallFindsCategory> a skos:ConceptScheme ;
	rdfs:comment "A concept schema related to the particular finds properties." .

<https://acdh.oeaw.ac.at/vocabs/defcthesaurus/tool/3.1> a skos:Concept ;
	skos:prefLabel "tool"@en , "Werkzeug"@de ;
	skos:definition "A device or implement, especially one held in the hand, used to carry out a particular function." ;
	skos:inScheme <https://acdh.oeaw.ac.at/vocabs/defcthesaurus/FindsSchema> , <https://acdh.oeaw.ac.at/vocabs/defcthesaurus/SmallFindsCategory> ;
	skos:editorialNote "dc_small_finds_category;1" ;
	skos:broader <https://acdh.oeaw.ac.at/vocabs/defcthesaurus/small_finds/2.5> .

<https://acdh.oeaw.ac.at/vocabs/defcthesaurus/small_finds/2.5> skos:narrower <https://acdh.oeaw.ac.at/vocabs/defcthesaurus/tool/3.1> .

<https://acdh.oeaw.ac.at/vocabs/defcthesaurus/fishing_object/4.027> a skos:Concept ;
	skos:prefLabel "fishing object"@en ;
	skos:definition "An object used for fishing." ;
	skos:inScheme <https://acdh.oeaw.ac.at/vocabs/defcthesaurus/FindsSchema> , <https://acdh.oeaw.ac.at/vocabs/defcthesaurus/NotInDatabase> ;
	skos:editorialNote "dc_not_in_database;027" ;
	skos:broader <https://acdh.oeaw.ac.at/vocabs/defcthesaurus/tool/3.1> .

<https://acdh.oeaw.ac.at/vocabs/defcthesaurus/tool/3.1> skos:narrower <https://acdh.oeaw.ac.at/vocabs/defcthesaurus/fishing_object/4.027> .

<https://acdh.oeaw.ac.at/vocabs/defcthesaurus/FindsSmallFindsType> a skos:ConceptScheme ;
	rdfs:comment "A concept schema related to the particular finds properties." .

<https://acdh.oeaw.ac.at/vocabs/defcthesaurus/fish_hook/5.45> a skos:Concept ;
	skos:prefLabel "fish hook"@en , "Angelhacken"@de ;
	skos:definition "An artifact of two basic types: the bait hook and lure hook. Varied in form throughout the Pacific, they are made of bone, shell, tortoise shell, or wood." ;
	skos:inScheme <https://acdh.oeaw.ac.at/vocabs/defcthesaurus/FindsSchema> , <https://acdh.oeaw.ac.at/vocabs/defcthesaurus/FindsSmallFindsType> ;
	skos:editorialNote "dc_finds_small_finds_type;45" ;
	skos:broader <https://acdh.oeaw.ac.at/vocabs/defcthesaurus/fishing_object/4.027> .

<https://acdh.oeaw.ac.at/vocabs/defcthesaurus/fishing_object/4.027> skos:narrower <https://acdh.oeaw.ac.at/vocabs/defcthesaurus/fish_hook/5.45> .

<https://acdh.oeaw.ac.at/vocabs/defcthesaurus/net_sinker/5.51> a skos:Concept ;
	skos:prefLabel "net sinker"@en , "Netzsenker"@de ;
	skos:altLabel "net weight"@en , " sinker"@en , "Netzgewicht"@de ;
	skos:definition "A term applied loosely to any perforated stone or terra cotta object that may have been used to keep a fishing net vertical in the water." ;
	skos:inScheme <https://acdh.oeaw.ac.at/vocabs/defcthesaurus/FindsSchema> , <https://acdh.oeaw.ac.at/vocabs/defcthesaurus/FindsSmallFindsType> ;
	skos:editorialNote "dc_finds_small_finds_type;51" ;
	skos:broader <https://acdh.oeaw.ac.at/vocabs/defcthesaurus/fishing_object/4.027> .

<https://acdh.oeaw.ac.at/vocabs/defcthesaurus/fishing_object/4.027> skos:narrower <https://acdh.oeaw.ac.at/vocabs/defcthesaurus/net_sinker/5.51> .

<https://acdh.oeaw.ac.at/vocabs/defcthesaurus/anchor/5.93> a skos:Concept ;
	skos:prefLabel "anchor"@en , "Anker"@de ;
	skos:definition "A heavy object used to moor a ship to the sea bottom, typically having a metal shank with a pair of curved, barbed flukes." ;
	skos:inScheme <https://acdh.oeaw.ac.at/vocabs/defcthesaurus/FindsSchema> , <https://acdh.oeaw.ac.at/vocabs/defcthesaurus/FindsSmallFindsType> ;
	skos:editorialNote "dc_finds_small_finds_type;93" ;
	skos:broader <https://acdh.oeaw.ac.at/vocabs/defcthesaurus/fishing_object/4.027> .

<https://acdh.oeaw.ac.at/vocabs/defcthesaurus/fishing_object/4.027> skos:narrower <https://acdh.oeaw.ac.at/vocabs/defcthesaurus/anchor/5.93> .

<https://acdh.oeaw.ac.at/vocabs/defcthesaurus/small_finds/2.5> dc:source "Kipfer, B. A. Dictionary of Artifacts 2007. Blackwell Publishing, Oxford.p.140" .

<https://acdh.oeaw.ac.at/vocabs/defcthesaurus/hammer/4.46> a skos:Concept ;
	skos:prefLabel "hammer"@en , "Hammer"@de ;
	skos:definition "A hand tool with a heavy rigid head and a handle; used to deliver an impulsive force by striking." ;
	skos:inScheme <https://acdh.oeaw.ac.at/vocabs/defcthesaurus/FindsSchema> , <https://acdh.oeaw.ac.at/vocabs/defcthesaurus/FindsSmallFindsType> ;
	skos:editorialNote "dc_finds_small_finds_type;46" ;
	skos:broader <https://acdh.oeaw.ac.at/vocabs/defcthesaurus/tool/3.1> .

<https://acdh.oeaw.ac.at/vocabs/defcthesaurus/tool/3.1> skos:narrower <https://acdh.oeaw.ac.at/vocabs/defcthesaurus/hammer/4.46> .

<https://acdh.oeaw.ac.at/vocabs/defcthesaurus/small_finds/2.5> dc:source "Kipfer, B. A. Dictionary of Artifacts 2007. Blackwell Publishing, Oxford.p.300." .

<https://acdh.oeaw.ac.at/vocabs/defcthesaurus/spoon/4.48> a skos:Concept ;
	skos:prefLabel "spoon"@en , "L철ffel"@de ;
	skos:definition "An implement consisting of a small, shallow oval or round bowl on a long handle, used for eating, stirring, and serving food." ;
	skos:inScheme <https://acdh.oeaw.ac.at/vocabs/defcthesaurus/FindsSchema> , <https://acdh.oeaw.ac.at/vocabs/defcthesaurus/FindsSmallFindsType> ;
	skos:editorialNote "dc_finds_small_finds_type;48" ;
	skos:broader <https://acdh.oeaw.ac.at/vocabs/defcthesaurus/tool/3.1> .

<https://acdh.oeaw.ac.at/vocabs/defcthesaurus/tool/3.1> skos:narrower <https://acdh.oeaw.ac.at/vocabs/defcthesaurus/spoon/4.48> .

<https://acdh.oeaw.ac.at/vocabs/defcthesaurus/small_finds/2.5> dc:source "Kipfer, B. A. Dictionary of Artifacts 2007. Blackwell Publishing, Oxford.p.136" .

<https://acdh.oeaw.ac.at/vocabs/defcthesaurus/grinding_stone/4.52> a skos:Concept ;
	skos:prefLabel "grinding stone"@en , "Reibstein"@de ;
	skos:definition "Any lithic (stone) artifact used to process plants for food, medicines, cosmetics, or pigments. The grinding was done on a flat or concave surface." ;
	skos:inScheme <https://acdh.oeaw.ac.at/vocabs/defcthesaurus/FindsSchema> , <https://acdh.oeaw.ac.at/vocabs/defcthesaurus/FindsSmallFindsType> ;
	skos:editorialNote "dc_finds_small_finds_type;52" ;
	skos:broader <https://acdh.oeaw.ac.at/vocabs/defcthesaurus/tool/3.1> .

<https://acdh.oeaw.ac.at/vocabs/defcthesaurus/tool/3.1> skos:narrower <https://acdh.oeaw.ac.at/vocabs/defcthesaurus/grinding_stone/4.52> .

<https://acdh.oeaw.ac.at/vocabs/defcthesaurus/small_finds/2.5> dc:source "Kipfer, B. A. Dictionary of Artifacts 2007. Blackwell Publishing, Oxford.p.297" .

<https://acdh.oeaw.ac.at/vocabs/defcthesaurus/spatula/4.55> a skos:Concept ;
	skos:prefLabel "spatula"@en , "Spatula"@de ;
	skos:definition "A tool, usually of bone, lime, wood, ebony, turtleshell, etc., consisting of a broad but thin blade. It served many general purposes  spreading, mixing, scooping, lifting  including burnishing pottery, workworking pelts, spooning flour, etc." ;
	skos:inScheme <https://acdh.oeaw.ac.at/vocabs/defcthesaurus/FindsSchema> , <https://acdh.oeaw.ac.at/vocabs/defcthesaurus/FindsSmallFindsType> ;
	skos:editorialNote "dc_finds_small_finds_type;55" ;
	skos:broader <https://acdh.oeaw.ac.at/vocabs/defcthesaurus/tool/3.1> .

<https://acdh.oeaw.ac.at/vocabs/defcthesaurus/tool/3.1> skos:narrower <https://acdh.oeaw.ac.at/vocabs/defcthesaurus/spatula/4.55> .

<https://acdh.oeaw.ac.at/vocabs/defcthesaurus/textile_equipment/4.028> a skos:Concept ;
	skos:prefLabel "textile equipment"@en ;
	skos:definition "Equipment used in production of textile materials." ;
	skos:inScheme <https://acdh.oeaw.ac.at/vocabs/defcthesaurus/FindsSchema> , <https://acdh.oeaw.ac.at/vocabs/defcthesaurus/NotInDatabase> ;
	skos:editorialNote "dc_not_in_database;028" ;
	skos:broader <https://acdh.oeaw.ac.at/vocabs/defcthesaurus/tool/3.1> .

<https://acdh.oeaw.ac.at/vocabs/defcthesaurus/tool/3.1> skos:narrower <https://acdh.oeaw.ac.at/vocabs/defcthesaurus/textile_equipment/4.028> .

<https://acdh.oeaw.ac.at/vocabs/defcthesaurus/spindle_whorl/5.56> a skos:Concept ;
	skos:prefLabel "spindle whorl"@en , "Spinnwirtel"@de ;
	skos:definition "A circular object with a central perforation intended to act as a fly wheel on a spindle, giving momentum to its rotation  an artifact providing evidence of the spinning of thread. It maintained the momentum of the spindle rotated by the spinner while he" ;
	skos:inScheme <https://acdh.oeaw.ac.at/vocabs/defcthesaurus/FindsSchema> , <https://acdh.oeaw.ac.at/vocabs/defcthesaurus/FindsSmallFindsType> ;
	skos:editorialNote "dc_finds_small_finds_type;56" ;
	skos:broader <https://acdh.oeaw.ac.at/vocabs/defcthesaurus/textile_equipment/4.028> .

<https://acdh.oeaw.ac.at/vocabs/defcthesaurus/textile_equipment/4.028> skos:narrower <https://acdh.oeaw.ac.at/vocabs/defcthesaurus/spindle_whorl/5.56> .

<https://acdh.oeaw.ac.at/vocabs/defcthesaurus/loom_weight/5.71> a skos:Concept ;
	skos:prefLabel "loom weight"@en , "Webgewicht"@de ;
	skos:altLabel "loomweight"@en ;
	skos:definition "A perforated stone or ceramic block used for stretching the threads forming the warp or the weft on a loom." ;
	skos:inScheme <https://acdh.oeaw.ac.at/vocabs/defcthesaurus/FindsSchema> , <https://acdh.oeaw.ac.at/vocabs/defcthesaurus/FindsSmallFindsType> ;
	skos:editorialNote "dc_finds_small_finds_type;71" ;
	skos:broader <https://acdh.oeaw.ac.at/vocabs/defcthesaurus/textile_equipment/4.028> .

<https://acdh.oeaw.ac.at/vocabs/defcthesaurus/textile_equipment/4.028> skos:narrower <https://acdh.oeaw.ac.at/vocabs/defcthesaurus/loom_weight/5.71> .

<https://acdh.oeaw.ac.at/vocabs/defcthesaurus/shuttle/5.75> a skos:Concept ;
	skos:prefLabel "shuttle"@en , "Weberschiffchen"@de ;
	skos:definition "A device in a loom for passing or shooting the weft thread through the shed from one side of the web to the other, usually consisting of a boat-shaped piece of wood containing a bobbin on which the weft thread is wound." ;
	skos:inScheme <https://acdh.oeaw.ac.at/vocabs/defcthesaurus/FindsSchema> , <https://acdh.oeaw.ac.at/vocabs/defcthesaurus/FindsSmallFindsType> ;
	skos:editorialNote "dc_finds_small_finds_type;75" ;
	skos:broader <https://acdh.oeaw.ac.at/vocabs/defcthesaurus/textile_equipment/4.028> .

<https://acdh.oeaw.ac.at/vocabs/defcthesaurus/textile_equipment/4.028> skos:narrower <https://acdh.oeaw.ac.at/vocabs/defcthesaurus/shuttle/5.75> .

<https://acdh.oeaw.ac.at/vocabs/defcthesaurus/needle/5.50> a skos:Concept ;
	skos:prefLabel "needle"@en , "Nadel"@de ;
	skos:definition "A very thin pointed piece of metal or bone with a hole or eye for thread at the blunter end, used in sewing." ;
	skos:inScheme <https://acdh.oeaw.ac.at/vocabs/defcthesaurus/FindsSchema> , <https://acdh.oeaw.ac.at/vocabs/defcthesaurus/FindsSmallFindsType> ;
	skos:editorialNote "dc_finds_small_finds_type;50" ;
	skos:broader <https://acdh.oeaw.ac.at/vocabs/defcthesaurus/textile_equipment/4.028> .

<https://acdh.oeaw.ac.at/vocabs/defcthesaurus/textile_equipment/4.028> skos:narrower <https://acdh.oeaw.ac.at/vocabs/defcthesaurus/needle/5.50> .

<https://acdh.oeaw.ac.at/vocabs/defcthesaurus/small_finds/2.5> dc:source "Kipfer, B. A. Dictionary of Artifacts 2007. Blackwell Publishing, Oxford.p.22" .

<https://acdh.oeaw.ac.at/vocabs/defcthesaurus/axe/4.57> a skos:Concept ;
	skos:prefLabel "axe"@en , "Axt"@de ;
	skos:altLabel "ax"@en ;
	skos:definition "A flat, heavy cutting tool of stone or metal (bronze) in which the cutting edge is parallel to the haft and which might have the head and handle in one piece. Its main function was for woodworking (hewing, cleaving, or chopping trees) but it was also used as a weapon of war, as the battle ax." ;
	skos:inScheme <https://acdh.oeaw.ac.at/vocabs/defcthesaurus/FindsSchema> , <https://acdh.oeaw.ac.at/vocabs/defcthesaurus/FindsSmallFindsType> ;
	skos:editorialNote "dc_finds_small_finds_type;57" ;
	skos:broader <https://acdh.oeaw.ac.at/vocabs/defcthesaurus/tool/3.1> .

<https://acdh.oeaw.ac.at/vocabs/defcthesaurus/tool/3.1> skos:narrower <https://acdh.oeaw.ac.at/vocabs/defcthesaurus/axe/4.57> .

<https://acdh.oeaw.ac.at/vocabs/defcthesaurus/grinding_equipment/4.029> a skos:Concept ;
	skos:prefLabel "grinding equipment"@en ;
	skos:definition "Tools used for grinding." ;
	skos:inScheme <https://acdh.oeaw.ac.at/vocabs/defcthesaurus/FindsSchema> , <https://acdh.oeaw.ac.at/vocabs/defcthesaurus/NotInDatabase> ;
	skos:editorialNote "dc_not_in_database;029" ;
	skos:broader <https://acdh.oeaw.ac.at/vocabs/defcthesaurus/tool/3.1> .

<https://acdh.oeaw.ac.at/vocabs/defcthesaurus/tool/3.1> skos:narrower <https://acdh.oeaw.ac.at/vocabs/defcthesaurus/grinding_equipment/4.029> .

<https://acdh.oeaw.ac.at/vocabs/defcthesaurus/grindstone/5.58> a skos:Concept ;
	skos:prefLabel "grindstone"@en , "Schleifstein"@de ;
	skos:altLabel "grinding stone"@en , "sharpening stone"@en ;
	skos:definition "A revolving stone used to sharpen or polish by grinding." ;
	skos:inScheme <https://acdh.oeaw.ac.at/vocabs/defcthesaurus/FindsSchema> , <https://acdh.oeaw.ac.at/vocabs/defcthesaurus/FindsSmallFindsType> ;
	skos:editorialNote "dc_finds_small_finds_type;58" ;
	skos:broader <https://acdh.oeaw.ac.at/vocabs/defcthesaurus/grinding_equipment/4.029> .

<https://acdh.oeaw.ac.at/vocabs/defcthesaurus/grinding_equipment/4.029> skos:narrower <https://acdh.oeaw.ac.at/vocabs/defcthesaurus/grindstone/5.58> .

<https://acdh.oeaw.ac.at/vocabs/defcthesaurus/mortar/5.49> a skos:Concept ;
	skos:prefLabel "mortar"@en , "M철rser"@de ;
	skos:definition "Part of an ancient device for processing plant foods, usually used with a pestle. It was a stone or wooden receptacle with a cupshaped depression." ;
	skos:inScheme <https://acdh.oeaw.ac.at/vocabs/defcthesaurus/FindsSchema> , <https://acdh.oeaw.ac.at/vocabs/defcthesaurus/FindsSmallFindsType> ;
	skos:editorialNote "dc_finds_small_finds_type;49" ;
	skos:broader <https://acdh.oeaw.ac.at/vocabs/defcthesaurus/grinding_equipment/4.029> .

<https://acdh.oeaw.ac.at/vocabs/defcthesaurus/grinding_equipment/4.029> skos:narrower <https://acdh.oeaw.ac.at/vocabs/defcthesaurus/mortar/5.49> .

<https://acdh.oeaw.ac.at/vocabs/defcthesaurus/pestle/5.60> a skos:Concept ;
	skos:prefLabel "pestle"@en , "St철el"@de ;
	skos:definition "Club-shaped (oblong cylindrical or subcylindrical) implement of stone used for pounding, crushing, or grinding substances in a mortar." ;
	skos:inScheme <https://acdh.oeaw.ac.at/vocabs/defcthesaurus/FindsSchema> , <https://acdh.oeaw.ac.at/vocabs/defcthesaurus/FindsSmallFindsType> ;
	skos:editorialNote "dc_finds_small_finds_type;60" ;
	skos:broader <https://acdh.oeaw.ac.at/vocabs/defcthesaurus/grinding_equipment/4.029> .

<https://acdh.oeaw.ac.at/vocabs/defcthesaurus/grinding_equipment/4.029> skos:narrower <https://acdh.oeaw.ac.at/vocabs/defcthesaurus/pestle/5.60> .

<https://acdh.oeaw.ac.at/vocabs/defcthesaurus/small_finds/2.5> dc:source "Kipfer, B. A. Dictionary of Artifacts 2007. Blackwell Publishing, Oxford.p.242" .

<https://acdh.oeaw.ac.at/vocabs/defcthesaurus/pintadera/4.59> a skos:Concept ;
	skos:prefLabel "pintadera"@en , "Pintadera"@de ;
	skos:altLabel "stamp"@en , "Stampel"@de ;
	skos:definition "A small object, usually of terra cotta, consisting of a decorative stamp with a knob at the back for holding. The stamping surface is flat, concave, or convex. It has been suggested that they served to apply pigments to the human skin in repeat patterns as an alternative to tattooing." ;
	skos:inScheme <https://acdh.oeaw.ac.at/vocabs/defcthesaurus/FindsSchema> , <https://acdh.oeaw.ac.at/vocabs/defcthesaurus/FindsSmallFindsType> ;
	skos:editorialNote "dc_finds_small_finds_type;59" ;
	skos:broader <https://acdh.oeaw.ac.at/vocabs/defcthesaurus/tool/3.1> .

<https://acdh.oeaw.ac.at/vocabs/defcthesaurus/tool/3.1> skos:narrower <https://acdh.oeaw.ac.at/vocabs/defcthesaurus/pintadera/4.59> .

<https://acdh.oeaw.ac.at/vocabs/defcthesaurus/small_finds/2.5> dc:source "Kipfer, B. A. Dictionary of Artifacts 2007. Blackwell Publishing, Oxford.p.284" .

<https://acdh.oeaw.ac.at/vocabs/defcthesaurus/seal/4.62> a skos:Concept ;
	skos:prefLabel "seal"@en , "Siegel"@de ;
	skos:definition "A device for impressing characteristic marks into a soft surface, such as wet clay or wax, to indicate ownership or authenticity. Seals were made of bone, ivory, stone, or wood and had an intaglio design and were in the form of stamps or cylinder seals." ;
	skos:inScheme <https://acdh.oeaw.ac.at/vocabs/defcthesaurus/FindsSchema> , <https://acdh.oeaw.ac.at/vocabs/defcthesaurus/FindsSmallFindsType> ;
	skos:editorialNote "dc_finds_small_finds_type;62" ;
	skos:broader <https://acdh.oeaw.ac.at/vocabs/defcthesaurus/tool/3.1> .

<https://acdh.oeaw.ac.at/vocabs/defcthesaurus/tool/3.1> skos:narrower <https://acdh.oeaw.ac.at/vocabs/defcthesaurus/seal/4.62> .

<https://acdh.oeaw.ac.at/vocabs/defcthesaurus/small_finds/2.5> dc:source "Kipfer, B. A. Dictionary of Artifacts 2007. Blackwell Publishing, Oxford.p.96" .

<https://acdh.oeaw.ac.at/vocabs/defcthesaurus/disc/4.63> a skos:Concept ;
	skos:prefLabel "disc"@en , "Scheibe"@de ;
	skos:definition "A stone artifact circular in shape and concave on both sides usually of quartz, granite, flint, hematite, slate, or basalt. They range from 0.25 to 23 cm in diameter and from 0.5 to 9 kg in weight. Some have a hole through the center and others have flanges around the edges.They seemed to have a ceremonial or ritual purpose or were used for mixing herbs or medicines." ;
	skos:inScheme <https://acdh.oeaw.ac.at/vocabs/defcthesaurus/FindsSchema> , <https://acdh.oeaw.ac.at/vocabs/defcthesaurus/FindsSmallFindsType> ;
	skos:editorialNote "dc_finds_small_finds_type;63" ;
	skos:broader <https://acdh.oeaw.ac.at/vocabs/defcthesaurus/tool/3.1> .

<https://acdh.oeaw.ac.at/vocabs/defcthesaurus/tool/3.1> skos:narrower <https://acdh.oeaw.ac.at/vocabs/defcthesaurus/disc/4.63> .

<https://acdh.oeaw.ac.at/vocabs/defcthesaurus/small_finds/2.5> dc:source "Kipfer, B. A. Dictionary of Artifacts 2007. Blackwell Publishing, Oxford.p.50" .

<https://acdh.oeaw.ac.at/vocabs/defcthesaurus/burnisher/4.65> a skos:Concept ;
	skos:prefLabel "burnisher"@en , "Polierer"@de ;
	skos:altLabel "smoother"@en ;
	skos:definition "A tool used to polish the surface of an artifact." ;
	skos:inScheme <https://acdh.oeaw.ac.at/vocabs/defcthesaurus/FindsSchema> , <https://acdh.oeaw.ac.at/vocabs/defcthesaurus/FindsSmallFindsType> ;
	skos:editorialNote "dc_finds_small_finds_type;65" ;
	skos:broader <https://acdh.oeaw.ac.at/vocabs/defcthesaurus/tool/3.1> .

<https://acdh.oeaw.ac.at/vocabs/defcthesaurus/tool/3.1> skos:narrower <https://acdh.oeaw.ac.at/vocabs/defcthesaurus/burnisher/4.65> .

<https://acdh.oeaw.ac.at/vocabs/defcthesaurus/small_finds/2.5> dc:source "Kipfer, B. A. Dictionary of Artifacts 2007. Blackwell Publishing, Oxford.p.5" .

<https://acdh.oeaw.ac.at/vocabs/defcthesaurus/adze/4.66> a skos:Concept ;
	skos:prefLabel "adze"@en , "Krummaxt"@de ;
	skos:definition "A cutting tool, similar to an ax, in which the blade is set at right angles to the handle or haft. One of the earliest tools, it was widely distribute in Stone Age cultures in the form of a handheld stone chipped to form a blade." ;
	skos:inScheme <https://acdh.oeaw.ac.at/vocabs/defcthesaurus/FindsSchema> , <https://acdh.oeaw.ac.at/vocabs/defcthesaurus/FindsSmallFindsType> ;
	skos:editorialNote "dc_finds_small_finds_type;66" ;
	skos:broader <https://acdh.oeaw.ac.at/vocabs/defcthesaurus/tool/3.1> .

<https://acdh.oeaw.ac.at/vocabs/defcthesaurus/tool/3.1> skos:narrower <https://acdh.oeaw.ac.at/vocabs/defcthesaurus/adze/4.66> .

<https://acdh.oeaw.ac.at/vocabs/defcthesaurus/small_finds/2.5> dc:source "Kipfer, B. A. Dictionary of Artifacts 2007. Blackwell Publishing, Oxford.p.87" .

<https://acdh.oeaw.ac.at/vocabs/defcthesaurus/crucible/4.67> a skos:Concept ;
	skos:prefLabel "crucible"@en , "Schmelztiegel"@de ;
	skos:definition "A small, coarse pottery (or other refractory material) vessel used for holding molten metal during melting, testing, or casting." ;
	skos:inScheme <https://acdh.oeaw.ac.at/vocabs/defcthesaurus/FindsSchema> , <https://acdh.oeaw.ac.at/vocabs/defcthesaurus/FindsSmallFindsType> ;
	skos:editorialNote "dc_finds_small_finds_type;67" ;
	skos:broader <https://acdh.oeaw.ac.at/vocabs/defcthesaurus/tool/3.1> .

<https://acdh.oeaw.ac.at/vocabs/defcthesaurus/tool/3.1> skos:narrower <https://acdh.oeaw.ac.at/vocabs/defcthesaurus/crucible/4.67> .

<https://acdh.oeaw.ac.at/vocabs/defcthesaurus/small_finds/2.5> dc:source "Kipfer, B. A. Dictionary of Artifacts 2007. Blackwell Publishing, Oxford.p.37" .

<https://acdh.oeaw.ac.at/vocabs/defcthesaurus/blade/4.68> a skos:Concept ;
	skos:prefLabel "blade"@en , "Klinge"@de ;
	skos:definition "A long, narrow, sharp-edged, thin flake of stone, used especially as a tool. This flake was detached by striking from a prepared core, often with a hammer. Ist length is usually at least twice the width. The blade may be a tool in itself, or may be the blank from which a two-edged knife, burin, or spokeshave was manufactured." ;
	skos:inScheme <https://acdh.oeaw.ac.at/vocabs/defcthesaurus/FindsSchema> , <https://acdh.oeaw.ac.at/vocabs/defcthesaurus/FindsSmallFindsType> ;
	skos:editorialNote "dc_finds_small_finds_type;68" ;
	skos:broader <https://acdh.oeaw.ac.at/vocabs/defcthesaurus/tool/3.1> .

<https://acdh.oeaw.ac.at/vocabs/defcthesaurus/tool/3.1> skos:narrower <https://acdh.oeaw.ac.at/vocabs/defcthesaurus/blade/4.68> .

<https://acdh.oeaw.ac.at/vocabs/defcthesaurus/small_finds/2.5> dc:source "Kipfer, B. A. Dictionary of Artifacts 2007. Blackwell Publishing, Oxford.p.67" .

<https://acdh.oeaw.ac.at/vocabs/defcthesaurus/chisel/4.69> a skos:Concept ;
	skos:prefLabel "chisel"@en , "Meisel"@de ;
	skos:definition "A long-bladed hand tool with a beveled cutting edge, stuck with a hammer or mallet to cut or shape wood, stone, or metal." ;
	skos:inScheme <https://acdh.oeaw.ac.at/vocabs/defcthesaurus/FindsSchema> , <https://acdh.oeaw.ac.at/vocabs/defcthesaurus/FindsSmallFindsType> ;
	skos:editorialNote "dc_finds_small_finds_type;69" ;
	skos:broader <https://acdh.oeaw.ac.at/vocabs/defcthesaurus/tool/3.1> .

<https://acdh.oeaw.ac.at/vocabs/defcthesaurus/tool/3.1> skos:narrower <https://acdh.oeaw.ac.at/vocabs/defcthesaurus/chisel/4.69> .

<https://acdh.oeaw.ac.at/vocabs/defcthesaurus/small_finds/2.5> dc:source "Kipfer, B. A. Dictionary of Artifacts 2007. Blackwell Publishing, Oxford.p.282" .

<https://acdh.oeaw.ac.at/vocabs/defcthesaurus/scraper/4.74> a skos:Concept ;
	skos:prefLabel "scraper"@en , "Schaber"@de ;
	skos:altLabel "weaving bobbin"@en , "bobbin"@en ;
	skos:definition "A retouched flake tool with a thick working edge; a flake tool that has been sharpened on one edge and left blunt on other edges to allow grasping, probably used to scrape (dress) animal hides." ;
	skos:inScheme <https://acdh.oeaw.ac.at/vocabs/defcthesaurus/FindsSchema> , <https://acdh.oeaw.ac.at/vocabs/defcthesaurus/FindsSmallFindsType> ;
	skos:editorialNote "dc_finds_small_finds_type;74" ;
	skos:broader <https://acdh.oeaw.ac.at/vocabs/defcthesaurus/tool/3.1> .

<https://acdh.oeaw.ac.at/vocabs/defcthesaurus/tool/3.1> skos:narrower <https://acdh.oeaw.ac.at/vocabs/defcthesaurus/scraper/4.74> .

<https://acdh.oeaw.ac.at/vocabs/defcthesaurus/awl/4.87> a skos:Concept ;
	skos:prefLabel "awl"@en , "Ahle"@de ;
	skos:altLabel "piercer"@en , "pin"@en , "Pfriem"@de ;
	skos:definition "A small tool consisting of a thin, tapering, sharp-pointed blade of bone, flint, or metal used for piercing holes, making decorations, or in assisting basketweaving." ;
	skos:inScheme <https://acdh.oeaw.ac.at/vocabs/defcthesaurus/FindsSchema> , <https://acdh.oeaw.ac.at/vocabs/defcthesaurus/FindsSmallFindsType> ;
	skos:editorialNote "dc_finds_small_finds_type;87" ;
	skos:broader <https://acdh.oeaw.ac.at/vocabs/defcthesaurus/tool/3.1> .

<https://acdh.oeaw.ac.at/vocabs/defcthesaurus/tool/3.1> skos:narrower <https://acdh.oeaw.ac.at/vocabs/defcthesaurus/awl/4.87> .

<https://acdh.oeaw.ac.at/vocabs/defcthesaurus/small_finds/2.5> dc:source "Kipfer, B. A. Dictionary of Artifacts 2007. Blackwell Publishing, Oxford.p.114" .

<https://acdh.oeaw.ac.at/vocabs/defcthesaurus/fire_dog/4.90> a skos:Concept ;
	skos:prefLabel "fire dog"@en , "Feuerbock"@de ;
	skos:altLabel "fire-dog"@en ;
	skos:definition "An instrument consisting of an iron bar held horizontally at one end by an upright support, used to ensure the proper burning of a fire. A pair of these were put at each side of the hearth or fireplace to support burning wood; the end of a long could rest on the crosspiece, which was supported by two uprights." ;
	skos:inScheme <https://acdh.oeaw.ac.at/vocabs/defcthesaurus/FindsSchema> , <https://acdh.oeaw.ac.at/vocabs/defcthesaurus/FindsSmallFindsType> ;
	skos:editorialNote "dc_finds_small_finds_type;90" ;
	skos:broader <https://acdh.oeaw.ac.at/vocabs/defcthesaurus/tool/3.1> .

<https://acdh.oeaw.ac.at/vocabs/defcthesaurus/tool/3.1> skos:narrower <https://acdh.oeaw.ac.at/vocabs/defcthesaurus/fire_dog/4.90> .

<https://acdh.oeaw.ac.at/vocabs/defcthesaurus/small_finds/2.5> dc:source "Kipfer, B. A. Dictionary of Artifacts 2007. Blackwell Publishing, Oxford.p.287" .

<https://acdh.oeaw.ac.at/vocabs/defcthesaurus/shaft_straightener/4.95> a skos:Concept ;
	skos:prefLabel "shaft straightener"@en , "Schaftgl채tter"@de ;
	skos:altLabel "Schaftstrecker"@de ;
	skos:definition "An artifact made from a coarse, often volcanic, stone, with a groove used as a rasp to finish spears and arrowshafts." ;
	skos:inScheme <https://acdh.oeaw.ac.at/vocabs/defcthesaurus/FindsSchema> , <https://acdh.oeaw.ac.at/vocabs/defcthesaurus/FindsSmallFindsType> ;
	skos:editorialNote "dc_finds_small_finds_type;95" ;
	skos:broader <https://acdh.oeaw.ac.at/vocabs/defcthesaurus/tool/3.1> .

<https://acdh.oeaw.ac.at/vocabs/defcthesaurus/tool/3.1> skos:narrower <https://acdh.oeaw.ac.at/vocabs/defcthesaurus/shaft_straightener/4.95> .

<https://acdh.oeaw.ac.at/vocabs/defcthesaurus/small_finds/2.5> dc:source "http://dbpedia.org/page/Tally_stick" .

<https://acdh.oeaw.ac.at/vocabs/defcthesaurus/tally_stick/4.100> a skos:Concept ;
	skos:prefLabel "tally stick"@en , "Kerbholz"@de ;
	skos:definition "A tally (or tally stick) was an ancient memory aid device used to record and document numbers, quantities, or even messages." ;
	skos:inScheme <https://acdh.oeaw.ac.at/vocabs/defcthesaurus/FindsSchema> , <https://acdh.oeaw.ac.at/vocabs/defcthesaurus/FindsSmallFindsType> ;
	skos:editorialNote "dc_finds_small_finds_type;100" ;
	skos:broader <https://acdh.oeaw.ac.at/vocabs/defcthesaurus/tool/3.1> .

<https://acdh.oeaw.ac.at/vocabs/defcthesaurus/tool/3.1> skos:narrower <https://acdh.oeaw.ac.at/vocabs/defcthesaurus/tally_stick/4.100> .

<https://acdh.oeaw.ac.at/vocabs/defcthesaurus/small_finds/2.5> dc:source "Kipfer, B. A. Dictionary of Artifacts 2007. Blackwell Publishing, Oxford.p 319" .

<https://acdh.oeaw.ac.at/vocabs/defcthesaurus/tip/4.101> a skos:Concept ;
	skos:prefLabel "tip"@en , "Spitze"@de ;
	skos:altLabel "shaft"@en ;
	skos:definition "Top and bottom of a point or blade." ;
	skos:inScheme <https://acdh.oeaw.ac.at/vocabs/defcthesaurus/FindsSchema> , <https://acdh.oeaw.ac.at/vocabs/defcthesaurus/FindsSmallFindsType> ;
	skos:editorialNote "dc_finds_small_finds_type;101" ;
	skos:broader <https://acdh.oeaw.ac.at/vocabs/defcthesaurus/tool/3.1> .

<https://acdh.oeaw.ac.at/vocabs/defcthesaurus/tool/3.1> skos:narrower <https://acdh.oeaw.ac.at/vocabs/defcthesaurus/tip/4.101> .

<https://acdh.oeaw.ac.at/vocabs/defcthesaurus/small_finds/2.5> dc:source "Kipfer, B. A. Dictionary of Artifacts 2007. Blackwell Publishing, Oxford.p 290" .

<https://acdh.oeaw.ac.at/vocabs/defcthesaurus/sickle_implement/4.107> a skos:Concept ;
	skos:prefLabel "sickle implement"@en , "Sichel"@de ;
	skos:altLabel "sickle element"@en , "sickle"@en ;
	skos:definition "A knife for reaping corn, first used by Neolithic man, made of flint blades mounted in a wooden or bone haft." ;
	skos:inScheme <https://acdh.oeaw.ac.at/vocabs/defcthesaurus/FindsSchema> , <https://acdh.oeaw.ac.at/vocabs/defcthesaurus/FindsSmallFindsType> ;
	skos:editorialNote "dc_finds_small_finds_type;107" ;
	skos:broader <https://acdh.oeaw.ac.at/vocabs/defcthesaurus/tool/3.1> .

<https://acdh.oeaw.ac.at/vocabs/defcthesaurus/tool/3.1> skos:narrower <https://acdh.oeaw.ac.at/vocabs/defcthesaurus/sickle_implement/4.107> .

<https://acdh.oeaw.ac.at/vocabs/defcthesaurus/small_finds/2.5> dc:source "Kipfer, B. A. Dictionary of Artifacts 2007. Blackwell Publishing, Oxford.p 337" .

<https://acdh.oeaw.ac.at/vocabs/defcthesaurus/weight/4.112> a skos:Concept ;
	skos:prefLabel "weight"@en , "Gewicht"@de ;
	skos:definition "Stone, clay, or metal object of standard weight used in measurement on balances or scales of some kind; an object used to weigh something down or to measure the weight of another object." ;
	skos:inScheme <https://acdh.oeaw.ac.at/vocabs/defcthesaurus/FindsSchema> , <https://acdh.oeaw.ac.at/vocabs/defcthesaurus/FindsSmallFindsType> ;
	skos:editorialNote "dc_finds_small_finds_type;112" ;
	skos:broader <https://acdh.oeaw.ac.at/vocabs/defcthesaurus/tool/3.1> .

<https://acdh.oeaw.ac.at/vocabs/defcthesaurus/tool/3.1> skos:narrower <https://acdh.oeaw.ac.at/vocabs/defcthesaurus/weight/4.112> .

<https://acdh.oeaw.ac.at/vocabs/defcthesaurus/small_finds/2.5> dc:source "Kipfer, B. A. Dictionary of Artifacts 2007. Blackwell Publishing, Oxford.p 79" .

<https://acdh.oeaw.ac.at/vocabs/defcthesaurus/cone/4.119> a skos:Concept ;
	skos:prefLabel "cone"@en , "Kegel"@de ;
	skos:definition "Small, elongated pyramid made of controlled mixtures of ceramic materials in a numbered sequence that softens and bends when heated." ;
	skos:inScheme <https://acdh.oeaw.ac.at/vocabs/defcthesaurus/FindsSchema> , <https://acdh.oeaw.ac.at/vocabs/defcthesaurus/FindsSmallFindsType> ;
	skos:editorialNote "dc_finds_small_finds_type;119" ;
	skos:broader <https://acdh.oeaw.ac.at/vocabs/defcthesaurus/tool/3.1> .

<https://acdh.oeaw.ac.at/vocabs/defcthesaurus/tool/3.1> skos:narrower <https://acdh.oeaw.ac.at/vocabs/defcthesaurus/cone/4.119> .

<https://acdh.oeaw.ac.at/vocabs/defcthesaurus/small_finds/2.5> dc:source "Kipfer, B. A. Dictionary of Artifacts 2007. Blackwell Publishing, Oxford.p 26" .

<https://acdh.oeaw.ac.at/vocabs/defcthesaurus/ball/4.120> a skos:Concept ;
	skos:prefLabel "ball"@en , "Ball"@de ;
	skos:definition "A round object used in games." ;
	skos:inScheme <https://acdh.oeaw.ac.at/vocabs/defcthesaurus/FindsSchema> , <https://acdh.oeaw.ac.at/vocabs/defcthesaurus/FindsSmallFindsType> ;
	skos:editorialNote "dc_finds_small_finds_type;120" ;
	skos:broader <https://acdh.oeaw.ac.at/vocabs/defcthesaurus/tool/3.1> .

<https://acdh.oeaw.ac.at/vocabs/defcthesaurus/tool/3.1> skos:narrower <https://acdh.oeaw.ac.at/vocabs/defcthesaurus/ball/4.120> .

<https://acdh.oeaw.ac.at/vocabs/defcthesaurus/small_finds/2.5> dc:source "Inizan, M.-L., M. Reduron-Ballinger, H. Roche, J. Tixier 1999, Technology and Terminology of Knapped Stone. Nanterre: CREP., D. Srejovic (ed) 1997, Arheolo큄ki Leksikon." .

<https://acdh.oeaw.ac.at/vocabs/defcthesaurus/drill/4.121> a skos:Concept ;
	skos:prefLabel "drill"@en , "Bohrer"@de ;
	skos:altLabel "Preforator"@en , "borer"@en ;
	skos:definition "A blade (or rarely flake) where a retoch forms a pointed end used for making holes." ;
	skos:inScheme <https://acdh.oeaw.ac.at/vocabs/defcthesaurus/FindsSchema> , <https://acdh.oeaw.ac.at/vocabs/defcthesaurus/FindsSmallFindsType> ;
	skos:editorialNote "dc_finds_small_finds_type;121" ;
	skos:broader <https://acdh.oeaw.ac.at/vocabs/defcthesaurus/tool/3.1> .

<https://acdh.oeaw.ac.at/vocabs/defcthesaurus/tool/3.1> skos:narrower <https://acdh.oeaw.ac.at/vocabs/defcthesaurus/drill/4.121> .

<https://acdh.oeaw.ac.at/vocabs/defcthesaurus/small_finds/2.5> dc:source "Kipfer, B. A. Dictionary of Artifacts 2007. Blackwell Publishing, Oxford.p. 166." .

<https://acdh.oeaw.ac.at/vocabs/defcthesaurus/knife/4.122> a skos:Concept ;
	skos:prefLabel "knife"@en , "Messer"@de ;
	skos:definition "A backed blade; a cutting instrument composed of a blade and a handle into which it is fixed, either rigidly or with a joint." ;
	skos:inScheme <https://acdh.oeaw.ac.at/vocabs/defcthesaurus/FindsSchema> , <https://acdh.oeaw.ac.at/vocabs/defcthesaurus/FindsSmallFindsType> ;
	skos:editorialNote "dc_finds_small_finds_type;122" ;
	skos:broader <https://acdh.oeaw.ac.at/vocabs/defcthesaurus/tool/3.1> .

<https://acdh.oeaw.ac.at/vocabs/defcthesaurus/tool/3.1> skos:narrower <https://acdh.oeaw.ac.at/vocabs/defcthesaurus/knife/4.122> .

<https://acdh.oeaw.ac.at/vocabs/defcthesaurus/small_finds/2.5> dc:source "Kipfer, B. A. Dictionary of Artifacts 2007. Blackwell Publishing, Oxford.p. 139" .

<https://acdh.oeaw.ac.at/vocabs/defcthesaurus/haft/4.123> a skos:Concept ;
	skos:prefLabel "haft"@en , "Griff"@de ;
	skos:altLabel "Heft"@de ;
	skos:definition "A handle of a compound weapon or a tool - such as an adze, awl, ax, or knife." ;
	skos:inScheme <https://acdh.oeaw.ac.at/vocabs/defcthesaurus/FindsSchema> , <https://acdh.oeaw.ac.at/vocabs/defcthesaurus/FindsSmallFindsType> ;
	skos:editorialNote "dc_finds_small_finds_type;123" ;
	skos:broader <https://acdh.oeaw.ac.at/vocabs/defcthesaurus/tool/3.1> .

<https://acdh.oeaw.ac.at/vocabs/defcthesaurus/tool/3.1> skos:narrower <https://acdh.oeaw.ac.at/vocabs/defcthesaurus/haft/4.123> .

<https://acdh.oeaw.ac.at/vocabs/defcthesaurus/knob/4.130> a skos:Concept ;
	skos:prefLabel "knob"@en , "Griff"@de ;
	skos:inScheme <https://acdh.oeaw.ac.at/vocabs/defcthesaurus/FindsSchema> , <https://acdh.oeaw.ac.at/vocabs/defcthesaurus/FindsSmallFindsType> ;
	skos:editorialNote "dc_finds_small_finds_type;130" ;
	skos:broader <https://acdh.oeaw.ac.at/vocabs/defcthesaurus/tool/3.1> .

<https://acdh.oeaw.ac.at/vocabs/defcthesaurus/tool/3.1> skos:narrower <https://acdh.oeaw.ac.at/vocabs/defcthesaurus/knob/4.130> .

<https://acdh.oeaw.ac.at/vocabs/defcthesaurus/small_finds/2.5> dc:source "Kipfer, B. A. Dictionary of Artifacts 2007. Blackwell Publishing, Oxford.p. 146" .

<https://acdh.oeaw.ac.at/vocabs/defcthesaurus/hoe/4.131> a skos:Concept ;
	skos:prefLabel "hoe"@en , "Hacke"@de ;
	skos:definition "A digging implement consisting of a blade set at right angles to a long handle (haft). Early hoes had stone or wooden blades." ;
	skos:inScheme <https://acdh.oeaw.ac.at/vocabs/defcthesaurus/FindsSchema> , <https://acdh.oeaw.ac.at/vocabs/defcthesaurus/FindsSmallFindsType> ;
	skos:editorialNote "dc_finds_small_finds_type;131" ;
	skos:broader <https://acdh.oeaw.ac.at/vocabs/defcthesaurus/tool/3.1> .

<https://acdh.oeaw.ac.at/vocabs/defcthesaurus/tool/3.1> skos:narrower <https://acdh.oeaw.ac.at/vocabs/defcthesaurus/hoe/4.131> .

<https://acdh.oeaw.ac.at/vocabs/defcthesaurus/small_finds/2.5> dc:source "Kipfer, B. A. Dictionary of Artifacts 2007. Blackwell Publishing, Oxford.p. 240" .

<https://acdh.oeaw.ac.at/vocabs/defcthesaurus/pickaxe/4.132> a skos:Concept ;
	skos:prefLabel "pickaxe"@en , "Spitzhacke"@de ;
	skos:altLabel "pickax"@en , "Pickel"@de ;
	skos:definition "A pick with a point at one end and a cutting blade at the other end." ;
	skos:inScheme <https://acdh.oeaw.ac.at/vocabs/defcthesaurus/FindsSchema> , <https://acdh.oeaw.ac.at/vocabs/defcthesaurus/FindsSmallFindsType> ;
	skos:editorialNote "dc_finds_small_finds_type;132" ;
	skos:broader <https://acdh.oeaw.ac.at/vocabs/defcthesaurus/tool/3.1> .

<https://acdh.oeaw.ac.at/vocabs/defcthesaurus/tool/3.1> skos:narrower <https://acdh.oeaw.ac.at/vocabs/defcthesaurus/pickaxe/4.132> .

<https://acdh.oeaw.ac.at/vocabs/defcthesaurus/coil/4.133> a skos:Concept ;
	skos:prefLabel "coil"@en , "Spule"@de ;
	skos:inScheme <https://acdh.oeaw.ac.at/vocabs/defcthesaurus/FindsSchema> , <https://acdh.oeaw.ac.at/vocabs/defcthesaurus/FindsSmallFindsType> ;
	skos:editorialNote "dc_finds_small_finds_type;133" ;
	skos:broader <https://acdh.oeaw.ac.at/vocabs/defcthesaurus/tool/3.1> .

<https://acdh.oeaw.ac.at/vocabs/defcthesaurus/tool/3.1> skos:narrower <https://acdh.oeaw.ac.at/vocabs/defcthesaurus/coil/4.133> .

<https://acdh.oeaw.ac.at/vocabs/defcthesaurus/chipped_disk/4.134> a skos:Concept ;
	skos:prefLabel "chipped disk"@en ;
	skos:inScheme <https://acdh.oeaw.ac.at/vocabs/defcthesaurus/FindsSchema> , <https://acdh.oeaw.ac.at/vocabs/defcthesaurus/FindsSmallFindsType> ;
	skos:editorialNote "dc_finds_small_finds_type;134" ;
	skos:broader <https://acdh.oeaw.ac.at/vocabs/defcthesaurus/tool/3.1> .

<https://acdh.oeaw.ac.at/vocabs/defcthesaurus/tool/3.1> skos:narrower <https://acdh.oeaw.ac.at/vocabs/defcthesaurus/chipped_disk/4.134> .

<https://acdh.oeaw.ac.at/vocabs/defcthesaurus/weapon/4.030> a skos:Concept ;
	skos:prefLabel "weapon"@en , "Waffe"@de ;
	skos:inScheme <https://acdh.oeaw.ac.at/vocabs/defcthesaurus/FindsSchema> , <https://acdh.oeaw.ac.at/vocabs/defcthesaurus/NotInDatabase> ;
	skos:editorialNote "dc_not_in_database;030" ;
	skos:broader <https://acdh.oeaw.ac.at/vocabs/defcthesaurus/tool/3.1> .

<https://acdh.oeaw.ac.at/vocabs/defcthesaurus/tool/3.1> skos:narrower <https://acdh.oeaw.ac.at/vocabs/defcthesaurus/weapon/4.030> .

<https://acdh.oeaw.ac.at/vocabs/defcthesaurus/mace_head/5.44> a skos:Concept ;
	skos:prefLabel "mace head"@en , "Keulenkopf"@de ;
	skos:definition "A small club like weapon, usually of stone, crafted to fit snugly in the hand, for pounding. It often had a perforated head and was attached to a shaft of wood (or ivory or hom), often tapering toward the end that was gripped." ;
	skos:inScheme <https://acdh.oeaw.ac.at/vocabs/defcthesaurus/FindsSchema> , <https://acdh.oeaw.ac.at/vocabs/defcthesaurus/FindsSmallFindsType> ;
	skos:editorialNote "dc_finds_small_finds_type;44" ;
	skos:broader <https://acdh.oeaw.ac.at/vocabs/defcthesaurus/weapon/4.030> .

<https://acdh.oeaw.ac.at/vocabs/defcthesaurus/weapon/4.030> skos:narrower <https://acdh.oeaw.ac.at/vocabs/defcthesaurus/mace_head/5.44> .

<https://acdh.oeaw.ac.at/vocabs/defcthesaurus/slingstone/5.53> a skos:Concept ;
	skos:prefLabel "slingstone"@en , "Schleudergeschoss"@de ;
	skos:altLabel "sling bullet"@en ;
	skos:definition "A stone used as a blunt projectile with a sling." ;
	skos:inScheme <https://acdh.oeaw.ac.at/vocabs/defcthesaurus/FindsSchema> , <https://acdh.oeaw.ac.at/vocabs/defcthesaurus/FindsSmallFindsType> ;
	skos:editorialNote "dc_finds_small_finds_type;53" ;
	skos:broader <https://acdh.oeaw.ac.at/vocabs/defcthesaurus/weapon/4.030> .

<https://acdh.oeaw.ac.at/vocabs/defcthesaurus/weapon/4.030> skos:narrower <https://acdh.oeaw.ac.at/vocabs/defcthesaurus/slingstone/5.53> .

<https://acdh.oeaw.ac.at/vocabs/defcthesaurus/projectile_point/5.70> a skos:Concept ;
	skos:prefLabel "projectile point"@en , "Projektilspitze"@de ;
	skos:altLabel "arrowhead"@en , "point"@en , "Pfeilspitze"@de ;
	skos:definition "A pointed retouched artefact, with or without tang for hafting, used for the purposes of hunting or warfare." ;
	skos:inScheme <https://acdh.oeaw.ac.at/vocabs/defcthesaurus/FindsSchema> , <https://acdh.oeaw.ac.at/vocabs/defcthesaurus/FindsSmallFindsType> ;
	skos:editorialNote "dc_finds_small_finds_type;70" ;
	skos:broader <https://acdh.oeaw.ac.at/vocabs/defcthesaurus/weapon/4.030> .

<https://acdh.oeaw.ac.at/vocabs/defcthesaurus/weapon/4.030> skos:narrower <https://acdh.oeaw.ac.at/vocabs/defcthesaurus/projectile_point/5.70> .

<https://acdh.oeaw.ac.at/vocabs/defcthesaurus/byblos_point/6.116> a skos:Concept ;
	skos:prefLabel "byblos point"@en ;
	skos:definition "A large, heavy arrowhead, usually carelessly made and asymetrical." ;
	skos:inScheme <https://acdh.oeaw.ac.at/vocabs/defcthesaurus/FindsSchema> , <https://acdh.oeaw.ac.at/vocabs/defcthesaurus/FindsSmallFindsType> ;
	skos:editorialNote "dc_finds_small_finds_type;02" ;
	skos:broader <https://acdh.oeaw.ac.at/vocabs/defcthesaurus/projectile_point/5.70> .

<https://acdh.oeaw.ac.at/vocabs/defcthesaurus/projectile_point/5.70> skos:narrower <https://acdh.oeaw.ac.at/vocabs/defcthesaurus/byblos_point/6.116> .

<https://acdh.oeaw.ac.at/vocabs/defcthesaurus/nemrik_point/6.117> a skos:Concept ;
	skos:prefLabel "nemrik point"@en ;
	skos:definition "A diamond-shaped point named after the Nemrik site in today Iraq." ;
	skos:inScheme <https://acdh.oeaw.ac.at/vocabs/defcthesaurus/FindsSchema> , <https://acdh.oeaw.ac.at/vocabs/defcthesaurus/FindsSmallFindsType> ;
	skos:editorialNote "dc_finds_small_finds_type;02" ;
	skos:broader <https://acdh.oeaw.ac.at/vocabs/defcthesaurus/projectile_point/5.70> .

<https://acdh.oeaw.ac.at/vocabs/defcthesaurus/projectile_point/5.70> skos:narrower <https://acdh.oeaw.ac.at/vocabs/defcthesaurus/nemrik_point/6.117> .

<https://acdh.oeaw.ac.at/vocabs/defcthesaurus/dagger/5.72> a skos:Concept ;
	skos:prefLabel "dagger"@en , "Dolch"@de ;
	skos:definition "A short knife with a pointed and edged blade, used as a weapon." ;
	skos:inScheme <https://acdh.oeaw.ac.at/vocabs/defcthesaurus/FindsSchema> , <https://acdh.oeaw.ac.at/vocabs/defcthesaurus/FindsSmallFindsType> ;
	skos:editorialNote "dc_finds_small_finds_type;72" ;
	skos:broader <https://acdh.oeaw.ac.at/vocabs/defcthesaurus/weapon/4.030> .

<https://acdh.oeaw.ac.at/vocabs/defcthesaurus/weapon/4.030> skos:narrower <https://acdh.oeaw.ac.at/vocabs/defcthesaurus/dagger/5.72> .

<https://acdh.oeaw.ac.at/vocabs/defcthesaurus/spear/5.113> a skos:Concept ;
	skos:prefLabel "spear"@en , "Speer"@de ;
	skos:altLabel "Lanze"@de ;
	skos:definition "A pole weapon with a sharp point, either thrown or thrust at an enemy or prey." ;
	skos:inScheme <https://acdh.oeaw.ac.at/vocabs/defcthesaurus/FindsSchema> , <https://acdh.oeaw.ac.at/vocabs/defcthesaurus/FindsSmallFindsType> ;
	skos:editorialNote "dc_finds_small_finds_type;113" ;
	skos:broader <https://acdh.oeaw.ac.at/vocabs/defcthesaurus/weapon/4.030> .

<https://acdh.oeaw.ac.at/vocabs/defcthesaurus/weapon/4.030> skos:narrower <https://acdh.oeaw.ac.at/vocabs/defcthesaurus/spear/5.113> .

<https://acdh.oeaw.ac.at/vocabs/defcthesaurus/other/4.109> a skos:Concept ;
	skos:prefLabel "other"@en ;
	skos:inScheme <https://acdh.oeaw.ac.at/vocabs/defcthesaurus/FindsSchema> , <https://acdh.oeaw.ac.at/vocabs/defcthesaurus/FindsSmallFindsType> ;
	skos:editorialNote "dc_finds_small_finds_type;109" ;
	skos:broader <https://acdh.oeaw.ac.at/vocabs/defcthesaurus/tool/3.1> .

<https://acdh.oeaw.ac.at/vocabs/defcthesaurus/tool/3.1> skos:narrower <https://acdh.oeaw.ac.at/vocabs/defcthesaurus/other/4.109> .

<https://acdh.oeaw.ac.at/vocabs/defcthesaurus/unknown/4.111> a skos:Concept ;
	skos:prefLabel "unknown"@en ;
	skos:inScheme <https://acdh.oeaw.ac.at/vocabs/defcthesaurus/FindsSchema> , <https://acdh.oeaw.ac.at/vocabs/defcthesaurus/FindsSmallFindsType> ;
	skos:editorialNote "dc_finds_small_finds_type;111" ;
	skos:broader <https://acdh.oeaw.ac.at/vocabs/defcthesaurus/tool/3.1> .

<https://acdh.oeaw.ac.at/vocabs/defcthesaurus/tool/3.1> skos:narrower <https://acdh.oeaw.ac.at/vocabs/defcthesaurus/unknown/4.111> .

<https://acdh.oeaw.ac.at/vocabs/defcthesaurus/jewellery/3.2> a skos:Concept ;
	skos:prefLabel "jewellery"@en , "Schmuck"@de ;
	skos:altLabel "jewelry"@en ;
	skos:definition "Jewellery or jewelry consists of small decorative items worn for personal adornment, such as brooches, rings, necklaces, earrings, and bracelets. Jewellery may be attached to the body or the clothes, and the term is restricted to durable ornaments, exclud" ;
	skos:inScheme <https://acdh.oeaw.ac.at/vocabs/defcthesaurus/FindsSchema> , <https://acdh.oeaw.ac.at/vocabs/defcthesaurus/SmallFindsCategory> ;
	skos:editorialNote "dc_small_finds_category;2" ;
	skos:broader <https://acdh.oeaw.ac.at/vocabs/defcthesaurus/small_finds/2.5> .

<https://acdh.oeaw.ac.at/vocabs/defcthesaurus/small_finds/2.5> skos:narrower <https://acdh.oeaw.ac.at/vocabs/defcthesaurus/jewellery/3.2> ;
	dc:source "Kipfer, B. A. Dictionary of Artifacts 2007. Blackwell Publishing, Oxford.p.236" .

<https://acdh.oeaw.ac.at/vocabs/defcthesaurus/pendant/4.76> a skos:Concept ;
	skos:prefLabel "pendant"@en , "Anh채nger"@de ;
	skos:definition "An adronment that hangs from a piece of jewelry (necklace or earring)." ;
	skos:inScheme <https://acdh.oeaw.ac.at/vocabs/defcthesaurus/FindsSchema> , <https://acdh.oeaw.ac.at/vocabs/defcthesaurus/FindsSmallFindsType> ;
	skos:editorialNote "dc_finds_small_finds_type;76" ;
	skos:broader <https://acdh.oeaw.ac.at/vocabs/defcthesaurus/jewellery/3.2> .

<https://acdh.oeaw.ac.at/vocabs/defcthesaurus/jewellery/3.2> skos:narrower <https://acdh.oeaw.ac.at/vocabs/defcthesaurus/pendant/4.76> .

<https://acdh.oeaw.ac.at/vocabs/defcthesaurus/small_finds/2.5> dc:source "Kipfer, B. A. Dictionary of Artifacts 2007. Blackwell Publishing, Oxford.p.45" .

<https://acdh.oeaw.ac.at/vocabs/defcthesaurus/bracelet/4.77> a skos:Concept ;
	skos:prefLabel "bracelet"@en , "Armreif"@de ;
	skos:definition "An ornamental band or chain worn on the wrist or arm." ;
	skos:inScheme <https://acdh.oeaw.ac.at/vocabs/defcthesaurus/FindsSchema> , <https://acdh.oeaw.ac.at/vocabs/defcthesaurus/FindsSmallFindsType> ;
	skos:editorialNote "dc_finds_small_finds_type;77" ;
	skos:broader <https://acdh.oeaw.ac.at/vocabs/defcthesaurus/jewellery/3.2> .

<https://acdh.oeaw.ac.at/vocabs/defcthesaurus/jewellery/3.2> skos:narrower <https://acdh.oeaw.ac.at/vocabs/defcthesaurus/bracelet/4.77> .

<https://acdh.oeaw.ac.at/vocabs/defcthesaurus/small_finds/2.5> dc:source "Kipfer, B. A. Dictionary of Artifacts 2007. Blackwell Publishing, Oxford.p.32" .

<https://acdh.oeaw.ac.at/vocabs/defcthesaurus/bead/4.78> a skos:Concept ;
	skos:prefLabel "bead"@en , "Perle"@de ;
	skos:definition "A small, circular, tubular, or oblong ornament with a perforated center; usually made from shell, stone, bone, or glass." ;
	skos:inScheme <https://acdh.oeaw.ac.at/vocabs/defcthesaurus/FindsSchema> , <https://acdh.oeaw.ac.at/vocabs/defcthesaurus/FindsSmallFindsType> ;
	skos:editorialNote "dc_finds_small_finds_type;78" ;
	skos:broader <https://acdh.oeaw.ac.at/vocabs/defcthesaurus/jewellery/3.2> .

<https://acdh.oeaw.ac.at/vocabs/defcthesaurus/jewellery/3.2> skos:narrower <https://acdh.oeaw.ac.at/vocabs/defcthesaurus/bead/4.78> .

<https://acdh.oeaw.ac.at/vocabs/defcthesaurus/small_finds/2.5> dc:source "http://dbpedia.org/page/Plug_(jewellery)" .

<https://acdh.oeaw.ac.at/vocabs/defcthesaurus/ear_plug/4.79> a skos:Concept ;
	skos:prefLabel "ear plug"@en , "Ohrstecker"@de ;
	skos:altLabel "plug"@en , "earspool"@en ;
	skos:definition "A short cylindrical piece of jewellery commonly worn in larger-gauge body piercings." ;
	skos:inScheme <https://acdh.oeaw.ac.at/vocabs/defcthesaurus/FindsSchema> , <https://acdh.oeaw.ac.at/vocabs/defcthesaurus/FindsSmallFindsType> ;
	skos:editorialNote "dc_finds_small_finds_type;79" ;
	skos:broader <https://acdh.oeaw.ac.at/vocabs/defcthesaurus/jewellery/3.2> .

<https://acdh.oeaw.ac.at/vocabs/defcthesaurus/jewellery/3.2> skos:narrower <https://acdh.oeaw.ac.at/vocabs/defcthesaurus/ear_plug/4.79> .

<https://acdh.oeaw.ac.at/vocabs/defcthesaurus/small_finds/2.5> dc:source "Kipfer, B. A. Dictionary of Artifacts 2007. Blackwell Publishing, Oxford.p.212" .

<https://acdh.oeaw.ac.at/vocabs/defcthesaurus/necklace/4.80> a skos:Concept ;
	skos:prefLabel "necklace"@en , "Halskette"@de ;
	skos:definition "A chain, band, or cord, often ornamented with beads, pearls, jewels, etc., worn around the neck." ;
	skos:inScheme <https://acdh.oeaw.ac.at/vocabs/defcthesaurus/FindsSchema> , <https://acdh.oeaw.ac.at/vocabs/defcthesaurus/FindsSmallFindsType> ;
	skos:editorialNote "dc_finds_small_finds_type;80" ;
	skos:broader <https://acdh.oeaw.ac.at/vocabs/defcthesaurus/jewellery/3.2> .

<https://acdh.oeaw.ac.at/vocabs/defcthesaurus/jewellery/3.2> skos:narrower <https://acdh.oeaw.ac.at/vocabs/defcthesaurus/necklace/4.80> .

<https://acdh.oeaw.ac.at/vocabs/defcthesaurus/small_finds/2.5> dc:source "http://dbpedia.org/page/Earring" .

<https://acdh.oeaw.ac.at/vocabs/defcthesaurus/earring/4.81> a skos:Concept ;
	skos:prefLabel "earring"@en , "Ohrring"@de ;
	skos:definition "An earring is a piece of jewellery attached to the ear via a piercing in the earlobe or another external part of the ear." ;
	skos:inScheme <https://acdh.oeaw.ac.at/vocabs/defcthesaurus/FindsSchema> , <https://acdh.oeaw.ac.at/vocabs/defcthesaurus/FindsSmallFindsType> ;
	skos:editorialNote "dc_finds_small_finds_type;81" ;
	skos:broader <https://acdh.oeaw.ac.at/vocabs/defcthesaurus/jewellery/3.2> .

<https://acdh.oeaw.ac.at/vocabs/defcthesaurus/jewellery/3.2> skos:narrower <https://acdh.oeaw.ac.at/vocabs/defcthesaurus/earring/4.81> .

<https://acdh.oeaw.ac.at/vocabs/defcthesaurus/small_finds/2.5> dc:source "Kipfer, B. A. Dictionary of Artifacts 2007. Blackwell Publishing, Oxford.p 271" .

<https://acdh.oeaw.ac.at/vocabs/defcthesaurus/ring/4.103> a skos:Concept ;
	skos:prefLabel "ring"@en , "Ring"@de ;
	skos:definition "A small circular band, typically of precious metal and often set with one or more gemstones, worn on a finger as an ornament or a token of marriage, engagement, or autority." ;
	skos:inScheme <https://acdh.oeaw.ac.at/vocabs/defcthesaurus/FindsSchema> , <https://acdh.oeaw.ac.at/vocabs/defcthesaurus/FindsSmallFindsType> ;
	skos:editorialNote "dc_finds_small_finds_type;103" ;
	skos:broader <https://acdh.oeaw.ac.at/vocabs/defcthesaurus/jewellery/3.2> .

<https://acdh.oeaw.ac.at/vocabs/defcthesaurus/jewellery/3.2> skos:narrower <https://acdh.oeaw.ac.at/vocabs/defcthesaurus/ring/4.103> .

<https://acdh.oeaw.ac.at/vocabs/defcthesaurus/small_finds/2.5> dc:source "Kipfer, B. A. Dictionary of Artifacts 2007. Blackwell Publishing, Oxford.p 171" .

<https://acdh.oeaw.ac.at/vocabs/defcthesaurus/labret/4.106> a skos:Concept ;
	skos:prefLabel "labret"@en , "Lippenpflock"@de ;
	skos:altLabel "lip plug"@en ;
	skos:definition "A lip plug or ornament inserted in an incision in the lower lip, often made of shell, bone, ivory, metal, stone, wood, or pottery." ;
	skos:inScheme <https://acdh.oeaw.ac.at/vocabs/defcthesaurus/FindsSchema> , <https://acdh.oeaw.ac.at/vocabs/defcthesaurus/FindsSmallFindsType> ;
	skos:editorialNote "dc_finds_small_finds_type;106" ;
	skos:broader <https://acdh.oeaw.ac.at/vocabs/defcthesaurus/jewellery/3.2> .

<https://acdh.oeaw.ac.at/vocabs/defcthesaurus/jewellery/3.2> skos:narrower <https://acdh.oeaw.ac.at/vocabs/defcthesaurus/labret/4.106> .

<https://acdh.oeaw.ac.at/vocabs/defcthesaurus/small_finds/2.5> dc:source "https://en.oxforddictionaries.com/definition/ornament" .

<https://acdh.oeaw.ac.at/vocabs/defcthesaurus/ornament/4.124> a skos:Concept ;
	skos:prefLabel "ornament"@en , "Ornament"@de ;
	skos:definition "A thing used or serving to make something look more attractive but usually having no practical purpose," ;
	skos:inScheme <https://acdh.oeaw.ac.at/vocabs/defcthesaurus/FindsSchema> , <https://acdh.oeaw.ac.at/vocabs/defcthesaurus/FindsSmallFindsType> ;
	skos:editorialNote "dc_finds_small_finds_type;124" ;
	skos:broader <https://acdh.oeaw.ac.at/vocabs/defcthesaurus/jewellery/3.2> .

<https://acdh.oeaw.ac.at/vocabs/defcthesaurus/jewellery/3.2> skos:narrower <https://acdh.oeaw.ac.at/vocabs/defcthesaurus/ornament/4.124> .

<https://acdh.oeaw.ac.at/vocabs/defcthesaurus/small_finds/2.5> dc:source "Kipfer, B. A. Dictionary of Artifacts 2007. Blackwell Publishing, Oxford.p. 154" .

<https://acdh.oeaw.ac.at/vocabs/defcthesaurus/inlay/4.125> a skos:Concept ;
	skos:prefLabel "inlay"@en , "Einlegearbeit"@de ;
	skos:definition "Placement of one material, either glass or metal, into a prepared depression (reservoir) on the surface of an item for decorative purposes." ;
	skos:inScheme <https://acdh.oeaw.ac.at/vocabs/defcthesaurus/FindsSchema> , <https://acdh.oeaw.ac.at/vocabs/defcthesaurus/FindsSmallFindsType> ;
	skos:editorialNote "dc_finds_small_finds_type;125" ;
	skos:broader <https://acdh.oeaw.ac.at/vocabs/defcthesaurus/jewellery/3.2> .

<https://acdh.oeaw.ac.at/vocabs/defcthesaurus/jewellery/3.2> skos:narrower <https://acdh.oeaw.ac.at/vocabs/defcthesaurus/inlay/4.125> .

<https://acdh.oeaw.ac.at/vocabs/defcthesaurus/small_finds/2.5> dc:source "Kipfer, B. A. Dictionary of Artifacts 2007. Blackwell Publishing, Oxford.p. 13" .

<https://acdh.oeaw.ac.at/vocabs/defcthesaurus/appliqu챕/4.126> a skos:Concept ;
	skos:prefLabel "appliqu챕"@en , "Applikation"@de ;
	skos:definition "Decoration or ornament applied to or laid on another material, such as metal on wood or embroidery on cloth; a ceramic finishing techniques that involves joining shaped pieces of a plastic body to a leather-hard surface by pressure. The applied pieces can" ;
	skos:inScheme <https://acdh.oeaw.ac.at/vocabs/defcthesaurus/FindsSchema> , <https://acdh.oeaw.ac.at/vocabs/defcthesaurus/FindsSmallFindsType> ;
	skos:editorialNote "dc_finds_small_finds_type;126" ;
	skos:broader <https://acdh.oeaw.ac.at/vocabs/defcthesaurus/jewellery/3.2> .

<https://acdh.oeaw.ac.at/vocabs/defcthesaurus/jewellery/3.2> skos:narrower <https://acdh.oeaw.ac.at/vocabs/defcthesaurus/appliqu챕/4.126> .

<https://acdh.oeaw.ac.at/vocabs/defcthesaurus/small_finds/2.5> dc:source "https://en.oxforddictionaries.com/definition/nose_ring" .

<https://acdh.oeaw.ac.at/vocabs/defcthesaurus/nose_ring/4.127> a skos:Concept ;
	skos:prefLabel "nose ring"@en , "Nasenring"@de ;
	skos:definition "A ring worn in a person쨈s nose as a piece of jewellery." ;
	skos:inScheme <https://acdh.oeaw.ac.at/vocabs/defcthesaurus/FindsSchema> , <https://acdh.oeaw.ac.at/vocabs/defcthesaurus/FindsSmallFindsType> ;
	skos:editorialNote "dc_finds_small_finds_type;127" ;
	skos:broader <https://acdh.oeaw.ac.at/vocabs/defcthesaurus/jewellery/3.2> .

<https://acdh.oeaw.ac.at/vocabs/defcthesaurus/jewellery/3.2> skos:narrower <https://acdh.oeaw.ac.at/vocabs/defcthesaurus/nose_ring/4.127> .

<https://acdh.oeaw.ac.at/vocabs/defcthesaurus/small_finds/2.5> dc:source "Kipfer, B. A. Dictionary of Artifacts 2007. Blackwell Publishing, Oxford.p. 241" .

<https://acdh.oeaw.ac.at/vocabs/defcthesaurus/pin/4.128> a skos:Concept ;
	skos:prefLabel "pin"@en , "Nadel"@de ;
	skos:definition "One of the simplest artifacts, consisting of a narrow metal or bone shaft with a point at one end and usually some sort of decorative head at the other. Ist function was to secure garments (ancestral to the fibula), or, sometimes, the hair." ;
	skos:inScheme <https://acdh.oeaw.ac.at/vocabs/defcthesaurus/FindsSchema> , <https://acdh.oeaw.ac.at/vocabs/defcthesaurus/FindsSmallFindsType> ;
	skos:editorialNote "dc_finds_small_finds_type;128" ;
	skos:broader <https://acdh.oeaw.ac.at/vocabs/defcthesaurus/jewellery/3.2> .

<https://acdh.oeaw.ac.at/vocabs/defcthesaurus/jewellery/3.2> skos:narrower <https://acdh.oeaw.ac.at/vocabs/defcthesaurus/pin/4.128> .

<https://acdh.oeaw.ac.at/vocabs/defcthesaurus/other/4.108> a skos:Concept ;
	skos:prefLabel "other"@en ;
	skos:inScheme <https://acdh.oeaw.ac.at/vocabs/defcthesaurus/FindsSchema> , <https://acdh.oeaw.ac.at/vocabs/defcthesaurus/FindsSmallFindsType> ;
	skos:editorialNote "dc_finds_small_finds_type;108" ;
	skos:broader <https://acdh.oeaw.ac.at/vocabs/defcthesaurus/jewellery/3.2> .

<https://acdh.oeaw.ac.at/vocabs/defcthesaurus/jewellery/3.2> skos:narrower <https://acdh.oeaw.ac.at/vocabs/defcthesaurus/other/4.108> .

<https://acdh.oeaw.ac.at/vocabs/defcthesaurus/unknown/4.110> a skos:Concept ;
	skos:prefLabel "unknown"@en ;
	skos:inScheme <https://acdh.oeaw.ac.at/vocabs/defcthesaurus/FindsSchema> , <https://acdh.oeaw.ac.at/vocabs/defcthesaurus/FindsSmallFindsType> ;
	skos:editorialNote "dc_finds_small_finds_type;110" ;
	skos:broader <https://acdh.oeaw.ac.at/vocabs/defcthesaurus/jewellery/3.2> .

<https://acdh.oeaw.ac.at/vocabs/defcthesaurus/jewellery/3.2> skos:narrower <https://acdh.oeaw.ac.at/vocabs/defcthesaurus/unknown/4.110> .

<https://acdh.oeaw.ac.at/vocabs/defcthesaurus/figurine/3.3> a skos:Concept ;
	skos:prefLabel "figurine"@en , "Statuette"@de ;
	skos:altLabel "terracotta"@en , " stattuete"@en , "kleine Statue"@de ;
	skos:definition "A figurine or statuette is a small statue that represents a human, deity or animal, or in practice a pair or small group of them." ;
	skos:inScheme <https://acdh.oeaw.ac.at/vocabs/defcthesaurus/FindsSchema> , <https://acdh.oeaw.ac.at/vocabs/defcthesaurus/SmallFindsCategory> ;
	skos:editorialNote "dc_small_finds_category;3" ;
	skos:broader <https://acdh.oeaw.ac.at/vocabs/defcthesaurus/small_finds/2.5> .

<https://acdh.oeaw.ac.at/vocabs/defcthesaurus/small_finds/2.5> skos:narrower <https://acdh.oeaw.ac.at/vocabs/defcthesaurus/figurine/3.3> ;
	dc:source "OREA" .

<https://acdh.oeaw.ac.at/vocabs/defcthesaurus/table/4.61> a skos:Concept ;
	skos:prefLabel "table"@en , "Tisch"@de ;
	skos:definition "A figurine shaped in form of a table." ;
	skos:inScheme <https://acdh.oeaw.ac.at/vocabs/defcthesaurus/FindsSchema> , <https://acdh.oeaw.ac.at/vocabs/defcthesaurus/FindsSmallFindsType> ;
	skos:editorialNote "dc_finds_small_finds_type;61" ;
	skos:broader <https://acdh.oeaw.ac.at/vocabs/defcthesaurus/figurine/3.3> .

<https://acdh.oeaw.ac.at/vocabs/defcthesaurus/figurine/3.3> skos:narrower <https://acdh.oeaw.ac.at/vocabs/defcthesaurus/table/4.61> .

<https://acdh.oeaw.ac.at/vocabs/defcthesaurus/small_finds/2.5> dc:source "Kipfer, B. A. Dictionary of Artifacts 2007. Blackwell Publishing, Oxford.p.113" .

<https://acdh.oeaw.ac.at/vocabs/defcthesaurus/stone_figurine/4.82> a skos:Concept ;
	skos:prefLabel "stone figurine"@en , "Steinfigur"@de ;
	skos:definition "A small carved figure of a human or animal of stone." ;
	skos:inScheme <https://acdh.oeaw.ac.at/vocabs/defcthesaurus/FindsSchema> , <https://acdh.oeaw.ac.at/vocabs/defcthesaurus/FindsSmallFindsType> ;
	skos:editorialNote "dc_finds_small_finds_type;82" ;
	skos:broader <https://acdh.oeaw.ac.at/vocabs/defcthesaurus/figurine/3.3> .

<https://acdh.oeaw.ac.at/vocabs/defcthesaurus/figurine/3.3> skos:narrower <https://acdh.oeaw.ac.at/vocabs/defcthesaurus/stone_figurine/4.82> .

<https://acdh.oeaw.ac.at/vocabs/defcthesaurus/zoomorphic_figurine/4.83> a skos:Concept ;
	skos:prefLabel "zoomorphic figurine"@en , "Zoomorphe Figur"@de ;
	skos:definition "A small carved or sculpted figure of an animal, usually of clay, stone, wood, or metal." ;
	skos:inScheme <https://acdh.oeaw.ac.at/vocabs/defcthesaurus/FindsSchema> , <https://acdh.oeaw.ac.at/vocabs/defcthesaurus/FindsSmallFindsType> ;
	skos:editorialNote "dc_finds_small_finds_type;83" ;
	skos:broader <https://acdh.oeaw.ac.at/vocabs/defcthesaurus/figurine/3.3> .

<https://acdh.oeaw.ac.at/vocabs/defcthesaurus/figurine/3.3> skos:narrower <https://acdh.oeaw.ac.at/vocabs/defcthesaurus/zoomorphic_figurine/4.83> .

<https://acdh.oeaw.ac.at/vocabs/defcthesaurus/anthropomorphic_figurine/4.84> a skos:Concept ;
	skos:prefLabel "anthropomorphic figurine"@en , "Anthropomorphe Figur"@de ;
	skos:definition "A small carved or sculpted figure of a human, usually of clay, stone, wood, or metal." ;
	skos:inScheme <https://acdh.oeaw.ac.at/vocabs/defcthesaurus/FindsSchema> , <https://acdh.oeaw.ac.at/vocabs/defcthesaurus/FindsSmallFindsType> ;
	skos:editorialNote "dc_finds_small_finds_type;84" ;
	skos:broader <https://acdh.oeaw.ac.at/vocabs/defcthesaurus/figurine/3.3> .

<https://acdh.oeaw.ac.at/vocabs/defcthesaurus/figurine/3.3> skos:narrower <https://acdh.oeaw.ac.at/vocabs/defcthesaurus/anthropomorphic_figurine/4.84> .

<https://acdh.oeaw.ac.at/vocabs/defcthesaurus/male_figurine/5.85> a skos:Concept ;
	skos:prefLabel "male figurine"@en , "M채nnliche Figur"@de ;
	skos:definition "A small carved or sculpted figure of a male human, usually of clay, stone, wood, or metal." ;
	skos:inScheme <https://acdh.oeaw.ac.at/vocabs/defcthesaurus/FindsSchema> , <https://acdh.oeaw.ac.at/vocabs/defcthesaurus/FindsSmallFindsType> ;
	skos:editorialNote "dc_finds_small_finds_type;85" ;
	skos:broader <https://acdh.oeaw.ac.at/vocabs/defcthesaurus/anthropomorphic_figurine/4.84> .

<https://acdh.oeaw.ac.at/vocabs/defcthesaurus/anthropomorphic_figurine/4.84> skos:narrower <https://acdh.oeaw.ac.at/vocabs/defcthesaurus/male_figurine/5.85> .

<https://acdh.oeaw.ac.at/vocabs/defcthesaurus/finds_type/1.02> dc:source "Kipfer, B. A. Dictionary of Artifacts 2007. Blackwell Publishing, Oxford.p.113" .

<https://acdh.oeaw.ac.at/vocabs/defcthesaurus/phallus/6.89> a skos:Concept ;
	skos:prefLabel "phallus"@en , "Phallus"@de ;
	skos:definition "A small carved or sculpted figure of a phallus, usually of clay, stone, wood, or metal." ;
	skos:inScheme <https://acdh.oeaw.ac.at/vocabs/defcthesaurus/FindsSchema> , <https://acdh.oeaw.ac.at/vocabs/defcthesaurus/FindsSmallFindsType> ;
	skos:editorialNote "dc_finds_small_finds_type;02" ;
	skos:broader <https://acdh.oeaw.ac.at/vocabs/defcthesaurus/male_figurine/5.85> .

<https://acdh.oeaw.ac.at/vocabs/defcthesaurus/male_figurine/5.85> skos:narrower <https://acdh.oeaw.ac.at/vocabs/defcthesaurus/phallus/6.89> .

<https://acdh.oeaw.ac.at/vocabs/defcthesaurus/female_figurine/5.86> a skos:Concept ;
	skos:prefLabel "female figurine"@en , "Weibliche Figur"@de ;
	skos:definition "A small carved or sculpted figure of a female human, usually of clay, stone, wood, or metal." ;
	skos:inScheme <https://acdh.oeaw.ac.at/vocabs/defcthesaurus/FindsSchema> , <https://acdh.oeaw.ac.at/vocabs/defcthesaurus/FindsSmallFindsType> ;
	skos:editorialNote "dc_finds_small_finds_type;86" ;
	skos:broader <https://acdh.oeaw.ac.at/vocabs/defcthesaurus/anthropomorphic_figurine/4.84> .

<https://acdh.oeaw.ac.at/vocabs/defcthesaurus/anthropomorphic_figurine/4.84> skos:narrower <https://acdh.oeaw.ac.at/vocabs/defcthesaurus/female_figurine/5.86> .

<https://acdh.oeaw.ac.at/vocabs/defcthesaurus/acrolith/5.92> a skos:Concept ;
	skos:prefLabel "acrolith"@en , "Akrolith"@de ;
	skos:definition "A Greek statue, of which the head and extremities were of stone or marble and the trunk crafted of wood which was either gilt or draped." ;
	skos:inScheme <https://acdh.oeaw.ac.at/vocabs/defcthesaurus/FindsSchema> , <https://acdh.oeaw.ac.at/vocabs/defcthesaurus/FindsSmallFindsType> ;
	skos:editorialNote "dc_finds_small_finds_type;92" ;
	skos:broader <https://acdh.oeaw.ac.at/vocabs/defcthesaurus/anthropomorphic_figurine/4.84> .

<https://acdh.oeaw.ac.at/vocabs/defcthesaurus/anthropomorphic_figurine/4.84> skos:narrower <https://acdh.oeaw.ac.at/vocabs/defcthesaurus/acrolith/5.92> .

<https://acdh.oeaw.ac.at/vocabs/defcthesaurus/house_model/4.88> a skos:Concept ;
	skos:prefLabel "house model"@en , "Hausmodell"@de ;
	skos:definition "A small carved or sculpted model of a house, usually of clay or stone." ;
	skos:inScheme <https://acdh.oeaw.ac.at/vocabs/defcthesaurus/FindsSchema> , <https://acdh.oeaw.ac.at/vocabs/defcthesaurus/FindsSmallFindsType> ;
	skos:editorialNote "dc_finds_small_finds_type;88" ;
	skos:broader <https://acdh.oeaw.ac.at/vocabs/defcthesaurus/figurine/3.3> .

<https://acdh.oeaw.ac.at/vocabs/defcthesaurus/figurine/3.3> skos:narrower <https://acdh.oeaw.ac.at/vocabs/defcthesaurus/house_model/4.88> .

<https://acdh.oeaw.ac.at/vocabs/defcthesaurus/thin_plate/4.104> a skos:Concept ;
	skos:prefLabel "thin plate"@en , "Pl채ttchen"@de ;
	skos:definition "Decorated small ceramic plates of an unknown function." ;
	skos:inScheme <https://acdh.oeaw.ac.at/vocabs/defcthesaurus/FindsSchema> , <https://acdh.oeaw.ac.at/vocabs/defcthesaurus/FindsSmallFindsType> ;
	skos:editorialNote "dc_finds_small_finds_type;104" ;
	skos:broader <https://acdh.oeaw.ac.at/vocabs/defcthesaurus/figurine/3.3> .

<https://acdh.oeaw.ac.at/vocabs/defcthesaurus/figurine/3.3> skos:narrower <https://acdh.oeaw.ac.at/vocabs/defcthesaurus/thin_plate/4.104> .

<https://acdh.oeaw.ac.at/vocabs/defcthesaurus/other/4.99> a skos:Concept ;
	skos:prefLabel "other"@en ;
	skos:inScheme <https://acdh.oeaw.ac.at/vocabs/defcthesaurus/FindsSchema> , <https://acdh.oeaw.ac.at/vocabs/defcthesaurus/FindsSmallFindsType> ;
	skos:editorialNote "dc_finds_small_finds_type;99" ;
	skos:broader <https://acdh.oeaw.ac.at/vocabs/defcthesaurus/figurine/3.3> .

<https://acdh.oeaw.ac.at/vocabs/defcthesaurus/figurine/3.3> skos:narrower <https://acdh.oeaw.ac.at/vocabs/defcthesaurus/other/4.99> .

<https://acdh.oeaw.ac.at/vocabs/defcthesaurus/unknown/4.98> a skos:Concept ;
	skos:prefLabel "unknown"@en ;
	skos:inScheme <https://acdh.oeaw.ac.at/vocabs/defcthesaurus/FindsSchema> , <https://acdh.oeaw.ac.at/vocabs/defcthesaurus/FindsSmallFindsType> ;
	skos:editorialNote "dc_finds_small_finds_type;98" ;
	skos:broader <https://acdh.oeaw.ac.at/vocabs/defcthesaurus/figurine/3.3> .

<https://acdh.oeaw.ac.at/vocabs/defcthesaurus/figurine/3.3> skos:narrower <https://acdh.oeaw.ac.at/vocabs/defcthesaurus/unknown/4.98> .

<https://acdh.oeaw.ac.at/vocabs/defcthesaurus/other/3.4> a skos:Concept ;
	skos:prefLabel "other"@en ;
	skos:definition "A small find that is not a figurine, tool nor jewlry" ;
	skos:inScheme <https://acdh.oeaw.ac.at/vocabs/defcthesaurus/FindsSchema> , <https://acdh.oeaw.ac.at/vocabs/defcthesaurus/SmallFindsCategory> ;
	skos:editorialNote "dc_small_finds_category;4" ;
	skos:broader <https://acdh.oeaw.ac.at/vocabs/defcthesaurus/small_finds/2.5> .

<https://acdh.oeaw.ac.at/vocabs/defcthesaurus/small_finds/2.5> skos:narrower <https://acdh.oeaw.ac.at/vocabs/defcthesaurus/other/3.4> ;
	dc:source "Kipfer, B. A. Dictionary of Artifacts 2007. Blackwell Publishing, Oxford.p.33" .

<https://acdh.oeaw.ac.at/vocabs/defcthesaurus/belt_hook/4.54> a skos:Concept ;
	skos:prefLabel "belt hook"@en , "G체rtelhaken"@de ;
	skos:definition "A small decorative and functional object used as a garment hook" ;
	skos:inScheme <https://acdh.oeaw.ac.at/vocabs/defcthesaurus/FindsSchema> , <https://acdh.oeaw.ac.at/vocabs/defcthesaurus/FindsSmallFindsType> ;
	skos:editorialNote "dc_finds_small_finds_type;54" ;
	skos:broader <https://acdh.oeaw.ac.at/vocabs/defcthesaurus/other/3.4> .

<https://acdh.oeaw.ac.at/vocabs/defcthesaurus/other/3.4> skos:narrower <https://acdh.oeaw.ac.at/vocabs/defcthesaurus/belt_hook/4.54> .

<https://acdh.oeaw.ac.at/vocabs/defcthesaurus/small_finds/2.5> dc:source "https://en.oxforddictionaries.com/definition/plaque" .

<https://acdh.oeaw.ac.at/vocabs/defcthesaurus/plaque/4.73> a skos:Concept ;
	skos:prefLabel "plaque"@en , "Platte"@de ;
	skos:definition "An ornamental tablet, typically of metal or wood, that is fixed ro a wall or other surface in commemmoration." ;
	skos:inScheme <https://acdh.oeaw.ac.at/vocabs/defcthesaurus/FindsSchema> , <https://acdh.oeaw.ac.at/vocabs/defcthesaurus/FindsSmallFindsType> ;
	skos:editorialNote "dc_finds_small_finds_type;73" ;
	skos:broader <https://acdh.oeaw.ac.at/vocabs/defcthesaurus/other/3.4> .

<https://acdh.oeaw.ac.at/vocabs/defcthesaurus/other/3.4> skos:narrower <https://acdh.oeaw.ac.at/vocabs/defcthesaurus/plaque/4.73> .

<https://acdh.oeaw.ac.at/vocabs/defcthesaurus/small_finds/2.5> dc:source "Kipfer, B. A. Dictionary of Artifacts 2007. Blackwell Publishing, Oxford.p.333" .

<https://acdh.oeaw.ac.at/vocabs/defcthesaurus/vessel/4.94> a skos:Concept ;
	skos:prefLabel "vessel"@en , "Gef채"@de ;
	skos:definition "An object used as a container (especially for liquids) typically of clay." ;
	skos:inScheme <https://acdh.oeaw.ac.at/vocabs/defcthesaurus/FindsSchema> , <https://acdh.oeaw.ac.at/vocabs/defcthesaurus/FindsSmallFindsType> ;
	skos:editorialNote "dc_finds_small_finds_type;94" ;
	skos:broader <https://acdh.oeaw.ac.at/vocabs/defcthesaurus/other/3.4> .

<https://acdh.oeaw.ac.at/vocabs/defcthesaurus/other/3.4> skos:narrower <https://acdh.oeaw.ac.at/vocabs/defcthesaurus/vessel/4.94> .

<https://acdh.oeaw.ac.at/vocabs/defcthesaurus/small_finds/2.5> dc:source "Kipfer, B. A. Dictionary of Artifacts 2007. Blackwell Publishing, Oxford.p 51" .

<https://acdh.oeaw.ac.at/vocabs/defcthesaurus/button/4.102> a skos:Concept ;
	skos:prefLabel "button"@en , "Knopf"@de ;
	skos:definition "Small, usually disklike, pieces of bone, metal, stone, or other solid material that have holes or a shank through which they are sewn on to garments. Buttons are used to fasten or close a garment and are sometimes purely decorative." ;
	skos:inScheme <https://acdh.oeaw.ac.at/vocabs/defcthesaurus/FindsSchema> , <https://acdh.oeaw.ac.at/vocabs/defcthesaurus/FindsSmallFindsType> ;
	skos:editorialNote "dc_finds_small_finds_type;102" ;
	skos:broader <https://acdh.oeaw.ac.at/vocabs/defcthesaurus/other/3.4> .

<https://acdh.oeaw.ac.at/vocabs/defcthesaurus/other/3.4> skos:narrower <https://acdh.oeaw.ac.at/vocabs/defcthesaurus/button/4.102> .

<https://acdh.oeaw.ac.at/vocabs/defcthesaurus/token/4.105> a skos:Concept ;
	skos:prefLabel "token"@en , "Zeichen"@de ;
	skos:definition "Small artifacts, generally of clay, made into cones, shperes, disks, or cylinders, tetrahedrons with usually plain surface. Such objects were used on Early Neolithic sites in western Asia as counters to keep records of goods." ;
	skos:inScheme <https://acdh.oeaw.ac.at/vocabs/defcthesaurus/FindsSchema> , <https://acdh.oeaw.ac.at/vocabs/defcthesaurus/FindsSmallFindsType> ;
	skos:editorialNote "dc_finds_small_finds_type;105" ;
	skos:broader <https://acdh.oeaw.ac.at/vocabs/defcthesaurus/other/3.4> .

<https://acdh.oeaw.ac.at/vocabs/defcthesaurus/other/3.4> skos:narrower <https://acdh.oeaw.ac.at/vocabs/defcthesaurus/token/4.105> .

<https://acdh.oeaw.ac.at/vocabs/defcthesaurus/small_finds/2.5> dc:source "Kipfer, B. A. Dictionary of Artifacts 2007. Blackwell Publishing, Oxford.p 154" .

<https://acdh.oeaw.ac.at/vocabs/defcthesaurus/inscription/4.114> a skos:Concept ;
	skos:prefLabel "inscription"@en , "Inschrift"@de ;
	skos:definition "Something that is inscribed; the act of inscribing. It is writing or any type cut into or raised upon a hard surface - clay, wood, stone, metal, etc. - and therefore endures." ;
	skos:inScheme <https://acdh.oeaw.ac.at/vocabs/defcthesaurus/FindsSchema> , <https://acdh.oeaw.ac.at/vocabs/defcthesaurus/FindsSmallFindsType> ;
	skos:editorialNote "dc_finds_small_finds_type;114" ;
	skos:broader <https://acdh.oeaw.ac.at/vocabs/defcthesaurus/other/3.4> .

<https://acdh.oeaw.ac.at/vocabs/defcthesaurus/other/3.4> skos:narrower <https://acdh.oeaw.ac.at/vocabs/defcthesaurus/inscription/4.114> .

<https://acdh.oeaw.ac.at/vocabs/defcthesaurus/small_finds/2.5> dc:source "Kipfer, B. A. Dictionary of Artifacts 2007. Blackwell Publishing, Oxford.p 99" .

<https://acdh.oeaw.ac.at/vocabs/defcthesaurus/dugout/4.115> a skos:Concept ;
	skos:prefLabel "dugout"@en , "Einbaum"@de ;
	skos:definition "A simple canoe made from a single tree hollowed out by burning or chopping." ;
	skos:inScheme <https://acdh.oeaw.ac.at/vocabs/defcthesaurus/FindsSchema> , <https://acdh.oeaw.ac.at/vocabs/defcthesaurus/FindsSmallFindsType> ;
	skos:editorialNote "dc_finds_small_finds_type;115" ;
	skos:broader <https://acdh.oeaw.ac.at/vocabs/defcthesaurus/other/3.4> .

<https://acdh.oeaw.ac.at/vocabs/defcthesaurus/other/3.4> skos:narrower <https://acdh.oeaw.ac.at/vocabs/defcthesaurus/dugout/4.115> .

<https://acdh.oeaw.ac.at/vocabs/defcthesaurus/small_finds/2.5> dc:source "Kipfer, B. A. Dictionary of Artifacts 2007. Blackwell Publishing, Oxford.p 341" .

<https://acdh.oeaw.ac.at/vocabs/defcthesaurus/wire/4.118> a skos:Concept ;
	skos:prefLabel "wire"@en , "Draht"@de ;
	skos:definition "Metal drawn out into a thin flexible thread or rod." ;
	skos:inScheme <https://acdh.oeaw.ac.at/vocabs/defcthesaurus/FindsSchema> , <https://acdh.oeaw.ac.at/vocabs/defcthesaurus/FindsSmallFindsType> ;
	skos:editorialNote "dc_finds_small_finds_type;118" ;
	skos:broader <https://acdh.oeaw.ac.at/vocabs/defcthesaurus/other/3.4> .

<https://acdh.oeaw.ac.at/vocabs/defcthesaurus/other/3.4> skos:narrower <https://acdh.oeaw.ac.at/vocabs/defcthesaurus/wire/4.118> .

<https://acdh.oeaw.ac.at/vocabs/defcthesaurus/small_finds/2.5> dc:source "Kipfer, B. A. Dictionary of Artifacts 2007. Blackwell Publishing, Oxford.p. 99" .

<https://acdh.oeaw.ac.at/vocabs/defcthesaurus/dross/4.129> a skos:Concept ;
	skos:prefLabel "dross"@en , "Schrott"@de ;
	skos:definition "Scum formed by oxidation at the surface of molten merals." ;
	skos:inScheme <https://acdh.oeaw.ac.at/vocabs/defcthesaurus/FindsSchema> , <https://acdh.oeaw.ac.at/vocabs/defcthesaurus/FindsSmallFindsType> ;
	skos:editorialNote "dc_finds_small_finds_type;129" ;
	skos:broader <https://acdh.oeaw.ac.at/vocabs/defcthesaurus/other/3.4> .

<https://acdh.oeaw.ac.at/vocabs/defcthesaurus/other/3.4> skos:narrower <https://acdh.oeaw.ac.at/vocabs/defcthesaurus/dross/4.129> .

<https://acdh.oeaw.ac.at/vocabs/defcthesaurus/pottery/2.4> a skos:Concept ;
	skos:prefLabel "pottery"@en , "Keramik"@de , "Keramik"@la ;
	skos:inScheme <https://acdh.oeaw.ac.at/vocabs/defcthesaurus/FindsSchema> , <https://acdh.oeaw.ac.at/vocabs/defcthesaurus/FindsType> ;
	skos:editorialNote "dc_finds_type;4" ;
	skos:broader <https://acdh.oeaw.ac.at/vocabs/defcthesaurus/finds_type/1.02> .

<https://acdh.oeaw.ac.at/vocabs/defcthesaurus/finds_type/1.02> skos:narrower <https://acdh.oeaw.ac.at/vocabs/defcthesaurus/pottery/2.4> .

<https://acdh.oeaw.ac.at/vocabs/defcthesaurus/FindsPotteryForm> a skos:ConceptScheme ;
	rdfs:comment "A concept schema related to the particular finds properties." .

<https://acdh.oeaw.ac.at/vocabs/defcthesaurus/pottery/2.4> dc:source "OREA" .

<https://acdh.oeaw.ac.at/vocabs/defcthesaurus/pottery_form/3.016> a skos:Concept ;
	skos:prefLabel "pottery form"@en ;
	skos:inScheme <https://acdh.oeaw.ac.at/vocabs/defcthesaurus/FindsSchema> ;
	skos:broader <https://acdh.oeaw.ac.at/vocabs/defcthesaurus/pottery/2.4> .

<https://acdh.oeaw.ac.at/vocabs/defcthesaurus/amphora/4.119> a skos:Concept ;
	skos:prefLabel "amphora"@en , "Amphore"@de ;
	skos:definition "Big closed storage vessel with narrow neck and mouth and usually with two handles at the top. The body is usually oval and long, with a pointed bottom." ;
	skos:inScheme <https://acdh.oeaw.ac.at/vocabs/defcthesaurus/FindsSchema> , <https://acdh.oeaw.ac.at/vocabs/defcthesaurus/FindsPotteryForm> ;
	skos:editorialNote "dc_finds_pottery_form;119" ;
	skos:broader <https://acdh.oeaw.ac.at/vocabs/defcthesaurus/pottery_form/3.016> .

<https://acdh.oeaw.ac.at/vocabs/defcthesaurus/pottery_form/3.016> skos:narrower <https://acdh.oeaw.ac.at/vocabs/defcthesaurus/amphora/4.119> .

<https://acdh.oeaw.ac.at/vocabs/defcthesaurus/pottery/2.4> skos:narrower <https://acdh.oeaw.ac.at/vocabs/defcthesaurus/pottery_form/3.016> .

<https://acdh.oeaw.ac.at/vocabs/defcthesaurus/anthropomorphic_vessel/4.99> a skos:Concept ;
	skos:prefLabel "anthropomorphic vessel"@en , "Anthropomorphes Gef채"@de ;
	skos:definition "Jar-like containers that have a human form." ;
	skos:inScheme <https://acdh.oeaw.ac.at/vocabs/defcthesaurus/FindsSchema> , <https://acdh.oeaw.ac.at/vocabs/defcthesaurus/FindsPotteryForm> ;
	skos:editorialNote "dc_finds_pottery_form;99" ;
	skos:broader <https://acdh.oeaw.ac.at/vocabs/defcthesaurus/pottery_form/3.016> .

<https://acdh.oeaw.ac.at/vocabs/defcthesaurus/pottery_form/3.016> skos:narrower <https://acdh.oeaw.ac.at/vocabs/defcthesaurus/anthropomorphic_vessel/4.99> .

<https://acdh.oeaw.ac.at/vocabs/defcthesaurus/pottery/2.4> dc:source "Kipfer, B. A. Dictionary of Artifacts 2007. Blackwell Publishing, Oxford.p 18" .

<https://acdh.oeaw.ac.at/vocabs/defcthesaurus/askos/4.101> a skos:Concept ;
	skos:prefLabel "askos"@en , "Askos"@de ;
	skos:definition "An assymetrical vessel, often squat and duck-shaped, with an off-center mouth, convex top, and single arching handle." ;
	skos:inScheme <https://acdh.oeaw.ac.at/vocabs/defcthesaurus/FindsSchema> , <https://acdh.oeaw.ac.at/vocabs/defcthesaurus/FindsPotteryForm> ;
	skos:editorialNote "dc_finds_pottery_form;101" ;
	skos:broader <https://acdh.oeaw.ac.at/vocabs/defcthesaurus/pottery_form/3.016> .

<https://acdh.oeaw.ac.at/vocabs/defcthesaurus/pottery_form/3.016> skos:narrower <https://acdh.oeaw.ac.at/vocabs/defcthesaurus/askos/4.101> .

<https://acdh.oeaw.ac.at/vocabs/defcthesaurus/pottery/2.4> dc:source "http://www.bible.ca/archeology/bible-archeology-pottery-glossary-dictionary-encyclopedia.htm" .

<https://acdh.oeaw.ac.at/vocabs/defcthesaurus/baking_pan/4.103> a skos:Concept ;
	skos:prefLabel "baking pan"@en , "Backplatte"@de ;
	skos:definition "A shallow platter with flat bottom and long handle apparently used for food preparation." ;
	skos:inScheme <https://acdh.oeaw.ac.at/vocabs/defcthesaurus/FindsSchema> , <https://acdh.oeaw.ac.at/vocabs/defcthesaurus/FindsPotteryForm> ;
	skos:editorialNote "dc_finds_pottery_form;103" ;
	skos:broader <https://acdh.oeaw.ac.at/vocabs/defcthesaurus/pottery_form/3.016> .

<https://acdh.oeaw.ac.at/vocabs/defcthesaurus/pottery_form/3.016> skos:narrower <https://acdh.oeaw.ac.at/vocabs/defcthesaurus/baking_pan/4.103> .

<https://acdh.oeaw.ac.at/vocabs/defcthesaurus/basin/4.122> a skos:Concept ;
	skos:prefLabel "basin"@en , "Becken"@de ;
	skos:definition "A medium-to-large (diameter), intermediate-to-deep bowl." ;
	skos:inScheme <https://acdh.oeaw.ac.at/vocabs/defcthesaurus/FindsSchema> , <https://acdh.oeaw.ac.at/vocabs/defcthesaurus/FindsPotteryForm> ;
	skos:editorialNote "dc_finds_pottery_form;122" ;
	skos:broader <https://acdh.oeaw.ac.at/vocabs/defcthesaurus/pottery_form/3.016> .

<https://acdh.oeaw.ac.at/vocabs/defcthesaurus/pottery_form/3.016> skos:narrower <https://acdh.oeaw.ac.at/vocabs/defcthesaurus/basin/4.122> .

<https://acdh.oeaw.ac.at/vocabs/defcthesaurus/bowl/4.115> a skos:Concept ;
	skos:prefLabel "bowl"@en , "Sch체ssel"@de ;
	skos:definition "A container whose height can measure from 1/3 to equal the amount of ist maximum diameter." ;
	skos:inScheme <https://acdh.oeaw.ac.at/vocabs/defcthesaurus/FindsSchema> , <https://acdh.oeaw.ac.at/vocabs/defcthesaurus/FindsPotteryForm> ;
	skos:editorialNote "dc_finds_pottery_form;115" ;
	skos:broader <https://acdh.oeaw.ac.at/vocabs/defcthesaurus/pottery_form/3.016> .

<https://acdh.oeaw.ac.at/vocabs/defcthesaurus/pottery_form/3.016> skos:narrower <https://acdh.oeaw.ac.at/vocabs/defcthesaurus/bowl/4.115> .

<https://acdh.oeaw.ac.at/vocabs/defcthesaurus/collared_bowl/5.146> a skos:Concept ;
	skos:prefLabel "collared bowl"@en , "Kragenschale"@de ;
	skos:definition "A shallow open vessel with a raised band or series of bands at the base of the neck." ;
	skos:inScheme <https://acdh.oeaw.ac.at/vocabs/defcthesaurus/FindsSchema> , <https://acdh.oeaw.ac.at/vocabs/defcthesaurus/FindsPotteryForm> ;
	skos:editorialNote "dc_finds_pottery_form;146" ;
	skos:broader <https://acdh.oeaw.ac.at/vocabs/defcthesaurus/bowl/4.115> .

<https://acdh.oeaw.ac.at/vocabs/defcthesaurus/bowl/4.115> skos:narrower <https://acdh.oeaw.ac.at/vocabs/defcthesaurus/collared_bowl/5.146> .

<https://acdh.oeaw.ac.at/vocabs/defcthesaurus/flat_based_oval_bowl/5.193> a skos:Concept ;
	skos:prefLabel "flat based oval bowl"@en , "ovale Sch체ssel mit flachem Boden"@de ;
	skos:definition "A shallow open vessel of oval shape and flat lower portion." ;
	skos:inScheme <https://acdh.oeaw.ac.at/vocabs/defcthesaurus/FindsSchema> , <https://acdh.oeaw.ac.at/vocabs/defcthesaurus/FindsPotteryForm> ;
	skos:editorialNote "dc_finds_pottery_form;193" ;
	skos:broader <https://acdh.oeaw.ac.at/vocabs/defcthesaurus/bowl/4.115> .

<https://acdh.oeaw.ac.at/vocabs/defcthesaurus/bowl/4.115> skos:narrower <https://acdh.oeaw.ac.at/vocabs/defcthesaurus/flat_based_oval_bowl/5.193> .

<https://acdh.oeaw.ac.at/vocabs/defcthesaurus/deep_bowl/5.178> a skos:Concept ;
	skos:prefLabel "deep bowl"@en , "Sch체ssel"@de ;
	skos:definition "A low open vessel with rim diameter same or smaller than height." ;
	skos:inScheme <https://acdh.oeaw.ac.at/vocabs/defcthesaurus/FindsSchema> , <https://acdh.oeaw.ac.at/vocabs/defcthesaurus/FindsPotteryForm> ;
	skos:editorialNote "dc_finds_pottery_form;178" ;
	skos:broader <https://acdh.oeaw.ac.at/vocabs/defcthesaurus/bowl/4.115> .

<https://acdh.oeaw.ac.at/vocabs/defcthesaurus/bowl/4.115> skos:narrower <https://acdh.oeaw.ac.at/vocabs/defcthesaurus/deep_bowl/5.178> .

<https://acdh.oeaw.ac.at/vocabs/defcthesaurus/dimini_bowl/5.129> a skos:Concept ;
	skos:prefLabel "dimini bowl"@en , "Dimini Schale"@de ;
	skos:altLabel "phiale"@en ;
	skos:definition "A vessel with a conical body, flat base, and strongly inverted rim. Sets of two or four small string-hole lugs are placed symmetrically arround the rim. Interior and exterior surface are fully covered with various geometrical design elements and patterns." ;
	skos:inScheme <https://acdh.oeaw.ac.at/vocabs/defcthesaurus/FindsSchema> , <https://acdh.oeaw.ac.at/vocabs/defcthesaurus/FindsPotteryForm> ;
	skos:editorialNote "dc_finds_pottery_form;129" ;
	skos:broader <https://acdh.oeaw.ac.at/vocabs/defcthesaurus/bowl/4.115> .

<https://acdh.oeaw.ac.at/vocabs/defcthesaurus/bowl/4.115> skos:narrower <https://acdh.oeaw.ac.at/vocabs/defcthesaurus/dimini_bowl/5.129> .

<https://acdh.oeaw.ac.at/vocabs/defcthesaurus/dome-shaped_shallow_bowl/5.108> a skos:Concept ;
	skos:prefLabel "dome-shaped shallow bowl"@en , "Kalottenf철rmige Schale"@de ;
	skos:definition "A hemispherical low open vessel with a rim diameter double than the height." ;
	skos:inScheme <https://acdh.oeaw.ac.at/vocabs/defcthesaurus/FindsSchema> , <https://acdh.oeaw.ac.at/vocabs/defcthesaurus/FindsPotteryForm> ;
	skos:editorialNote "dc_finds_pottery_form;108" ;
	skos:broader <https://acdh.oeaw.ac.at/vocabs/defcthesaurus/bowl/4.115> .

<https://acdh.oeaw.ac.at/vocabs/defcthesaurus/bowl/4.115> skos:narrower <https://acdh.oeaw.ac.at/vocabs/defcthesaurus/dome-shaped_shallow_bowl/5.108> .

<https://acdh.oeaw.ac.at/vocabs/defcthesaurus/narrow-mouthed_shallow_bowl/5.109> a skos:Concept ;
	skos:prefLabel "narrow-mouthed shallow bowl"@en , "Engmundige Schale"@de ;
	skos:definition "A low open vessel with narrow mouth and with a rim diameter double than the height." ;
	skos:inScheme <https://acdh.oeaw.ac.at/vocabs/defcthesaurus/FindsSchema> , <https://acdh.oeaw.ac.at/vocabs/defcthesaurus/FindsPotteryForm> ;
	skos:editorialNote "dc_finds_pottery_form;109" ;
	skos:broader <https://acdh.oeaw.ac.at/vocabs/defcthesaurus/bowl/4.115> .

<https://acdh.oeaw.ac.at/vocabs/defcthesaurus/bowl/4.115> skos:narrower <https://acdh.oeaw.ac.at/vocabs/defcthesaurus/narrow-mouthed_shallow_bowl/5.109> .

<https://acdh.oeaw.ac.at/vocabs/defcthesaurus/shallow_bowl/5.116> a skos:Concept ;
	skos:prefLabel "shallow bowl"@en , "Schale"@de ;
	skos:definition "A low open vessel with a rim diameter double than the height." ;
	skos:inScheme <https://acdh.oeaw.ac.at/vocabs/defcthesaurus/FindsSchema> , <https://acdh.oeaw.ac.at/vocabs/defcthesaurus/FindsPotteryForm> ;
	skos:editorialNote "dc_finds_pottery_form;116" ;
	skos:broader <https://acdh.oeaw.ac.at/vocabs/defcthesaurus/bowl/4.115> .

<https://acdh.oeaw.ac.at/vocabs/defcthesaurus/bowl/4.115> skos:narrower <https://acdh.oeaw.ac.at/vocabs/defcthesaurus/shallow_bowl/5.116> .

<https://acdh.oeaw.ac.at/vocabs/defcthesaurus/shouldered_bowl/5.156> a skos:Concept ;
	skos:prefLabel "shouldered bowl"@en , "Schulterschale"@de ;
	skos:definition "Bowl with strong carination in its upper part typical for Thessaly." ;
	skos:inScheme <https://acdh.oeaw.ac.at/vocabs/defcthesaurus/FindsSchema> , <https://acdh.oeaw.ac.at/vocabs/defcthesaurus/FindsPotteryForm> ;
	skos:editorialNote "dc_finds_pottery_form;156" ;
	skos:broader <https://acdh.oeaw.ac.at/vocabs/defcthesaurus/bowl/4.115> .

<https://acdh.oeaw.ac.at/vocabs/defcthesaurus/bowl/4.115> skos:narrower <https://acdh.oeaw.ac.at/vocabs/defcthesaurus/shouldered_bowl/5.156> .

<https://acdh.oeaw.ac.at/vocabs/defcthesaurus/gouged_bowl/5.149> a skos:Concept ;
	skos:prefLabel "gouged bowl"@en , "Gouged Bowl"@de ;
	skos:definition "MN Urfirnis deep bowl with deep linear incisions in the interior of the bowl." ;
	skos:inScheme <https://acdh.oeaw.ac.at/vocabs/defcthesaurus/FindsSchema> , <https://acdh.oeaw.ac.at/vocabs/defcthesaurus/FindsPotteryForm> ;
	skos:editorialNote "dc_finds_pottery_form;149" ;
	skos:broader <https://acdh.oeaw.ac.at/vocabs/defcthesaurus/bowl/4.115> .

<https://acdh.oeaw.ac.at/vocabs/defcthesaurus/bowl/4.115> skos:narrower <https://acdh.oeaw.ac.at/vocabs/defcthesaurus/gouged_bowl/5.149> .

<https://acdh.oeaw.ac.at/vocabs/defcthesaurus/husking_bowl/5.190> a skos:Concept ;
	skos:prefLabel "husking bowl"@en , "Husking Bowl"@de ;
	skos:altLabel "husking tray"@en ;
	skos:definition "A bowl used for husking cereals." ;
	skos:inScheme <https://acdh.oeaw.ac.at/vocabs/defcthesaurus/FindsSchema> , <https://acdh.oeaw.ac.at/vocabs/defcthesaurus/FindsPotteryForm> ;
	skos:editorialNote "dc_finds_pottery_form;190" ;
	skos:broader <https://acdh.oeaw.ac.at/vocabs/defcthesaurus/bowl/4.115> .

<https://acdh.oeaw.ac.at/vocabs/defcthesaurus/bowl/4.115> skos:narrower <https://acdh.oeaw.ac.at/vocabs/defcthesaurus/husking_bowl/5.190> .

<https://acdh.oeaw.ac.at/vocabs/defcthesaurus/husking_bowl/5.196> a skos:Concept ;
	skos:prefLabel "husking bowl"@en ;
	skos:altLabel "husking tray"@en ;
	skos:definition "A bowl used for husking cereals." ;
	skos:inScheme <https://acdh.oeaw.ac.at/vocabs/defcthesaurus/FindsSchema> , <https://acdh.oeaw.ac.at/vocabs/defcthesaurus/FindsPotteryForm> ;
	skos:editorialNote "dc_finds_pottery_form;196" ;
	skos:broader <https://acdh.oeaw.ac.at/vocabs/defcthesaurus/bowl/4.115> .

<https://acdh.oeaw.ac.at/vocabs/defcthesaurus/bowl/4.115> skos:narrower <https://acdh.oeaw.ac.at/vocabs/defcthesaurus/husking_bowl/5.196> .

<https://acdh.oeaw.ac.at/vocabs/defcthesaurus/carinated_bowl/5.104> a skos:Concept ;
	skos:prefLabel "carinated bowl"@en , "Knickwandschale"@de ;
	skos:definition "A low, open vessel with bent walls." ;
	skos:inScheme <https://acdh.oeaw.ac.at/vocabs/defcthesaurus/FindsSchema> , <https://acdh.oeaw.ac.at/vocabs/defcthesaurus/FindsPotteryForm> ;
	skos:editorialNote "dc_finds_pottery_form;104" ;
	skos:broader <https://acdh.oeaw.ac.at/vocabs/defcthesaurus/bowl/4.115> .

<https://acdh.oeaw.ac.at/vocabs/defcthesaurus/bowl/4.115> skos:narrower <https://acdh.oeaw.ac.at/vocabs/defcthesaurus/carinated_bowl/5.104> .

<https://acdh.oeaw.ac.at/vocabs/defcthesaurus/finds_type/1.02> dc:source "OREA" .

<https://acdh.oeaw.ac.at/vocabs/defcthesaurus/carinated_bowl_with_inverted_rim/6.105> a skos:Concept ;
	skos:prefLabel "carinated bowl with inverted rim"@en , "Knickrandschale"@de ;
	skos:definition "A shallow, open vessel with upper part heavily contracting inwards." ;
	skos:inScheme <https://acdh.oeaw.ac.at/vocabs/defcthesaurus/FindsSchema> , <https://acdh.oeaw.ac.at/vocabs/defcthesaurus/FindsPotteryForm> ;
	skos:editorialNote "dc_finds_pottery_form;02" ;
	skos:broader <https://acdh.oeaw.ac.at/vocabs/defcthesaurus/carinated_bowl/5.104> .

<https://acdh.oeaw.ac.at/vocabs/defcthesaurus/carinated_bowl/5.104> skos:narrower <https://acdh.oeaw.ac.at/vocabs/defcthesaurus/carinated_bowl_with_inverted_rim/6.105> .

<https://acdh.oeaw.ac.at/vocabs/defcthesaurus/carinated_incurved_bowl/6.174> a skos:Concept ;
	skos:prefLabel "carinated incurved bowl"@en , "Einw채rts gekr체mmte Knickwandschale"@de ;
	skos:definition "A low, open vessel with inward bent walls." ;
	skos:inScheme <https://acdh.oeaw.ac.at/vocabs/defcthesaurus/FindsSchema> , <https://acdh.oeaw.ac.at/vocabs/defcthesaurus/FindsPotteryForm> ;
	skos:editorialNote "dc_finds_pottery_form;02" ;
	skos:broader <https://acdh.oeaw.ac.at/vocabs/defcthesaurus/carinated_bowl/5.104> .

<https://acdh.oeaw.ac.at/vocabs/defcthesaurus/carinated_bowl/5.104> skos:narrower <https://acdh.oeaw.ac.at/vocabs/defcthesaurus/carinated_incurved_bowl/6.174> .

<https://acdh.oeaw.ac.at/vocabs/defcthesaurus/jar/4.145> a skos:Concept ;
	skos:prefLabel "jar"@en , "Topf"@de ;
	skos:definition "An open vessel whose height can be equal or greater than their maximum diameter. They can occur in various sizes with various with or without necks." ;
	skos:inScheme <https://acdh.oeaw.ac.at/vocabs/defcthesaurus/FindsSchema> , <https://acdh.oeaw.ac.at/vocabs/defcthesaurus/FindsPotteryForm> ;
	skos:editorialNote "dc_finds_pottery_form;145" ;
	skos:broader <https://acdh.oeaw.ac.at/vocabs/defcthesaurus/pottery_form/3.016> .

<https://acdh.oeaw.ac.at/vocabs/defcthesaurus/pottery_form/3.016> skos:narrower <https://acdh.oeaw.ac.at/vocabs/defcthesaurus/jar/4.145> .

<https://acdh.oeaw.ac.at/vocabs/defcthesaurus/carinated_jar/5.175> a skos:Concept ;
	skos:prefLabel "carinated jar"@en , "Knickwandtopf"@de ;
	skos:definition "A closed vessel used for storage, preservation, or transportation of goods with two or non handles and bent walls." ;
	skos:inScheme <https://acdh.oeaw.ac.at/vocabs/defcthesaurus/FindsSchema> , <https://acdh.oeaw.ac.at/vocabs/defcthesaurus/FindsPotteryForm> ;
	skos:editorialNote "dc_finds_pottery_form;175" ;
	skos:broader <https://acdh.oeaw.ac.at/vocabs/defcthesaurus/jar/4.145> .

<https://acdh.oeaw.ac.at/vocabs/defcthesaurus/jar/4.145> skos:narrower <https://acdh.oeaw.ac.at/vocabs/defcthesaurus/carinated_jar/5.175> .

<https://acdh.oeaw.ac.at/vocabs/defcthesaurus/collared_jar/5.127> a skos:Concept ;
	skos:prefLabel "collared jar"@en , "Kragenhalsamphore"@de ;
	skos:definition "A closed vessel with two or non handles with a raised band or series of bands at the base of the neck." ;
	skos:inScheme <https://acdh.oeaw.ac.at/vocabs/defcthesaurus/FindsSchema> , <https://acdh.oeaw.ac.at/vocabs/defcthesaurus/FindsPotteryForm> ;
	skos:editorialNote "dc_finds_pottery_form;127" ;
	skos:broader <https://acdh.oeaw.ac.at/vocabs/defcthesaurus/jar/4.145> .

<https://acdh.oeaw.ac.at/vocabs/defcthesaurus/jar/4.145> skos:narrower <https://acdh.oeaw.ac.at/vocabs/defcthesaurus/collared_jar/5.127> .

<https://acdh.oeaw.ac.at/vocabs/defcthesaurus/funnel-necked_jar/5.180> a skos:Concept ;
	skos:prefLabel "funnel-necked jar"@en , "Trichterrandtopf"@de ;
	skos:definition "A high and open vessel with an expanded neck." ;
	skos:inScheme <https://acdh.oeaw.ac.at/vocabs/defcthesaurus/FindsSchema> , <https://acdh.oeaw.ac.at/vocabs/defcthesaurus/FindsPotteryForm> ;
	skos:editorialNote "dc_finds_pottery_form;180" ;
	skos:broader <https://acdh.oeaw.ac.at/vocabs/defcthesaurus/jar/4.145> .

<https://acdh.oeaw.ac.at/vocabs/defcthesaurus/jar/4.145> skos:narrower <https://acdh.oeaw.ac.at/vocabs/defcthesaurus/funnel-necked_jar/5.180> .

<https://acdh.oeaw.ac.at/vocabs/defcthesaurus/globular_jar/5.106> a skos:Concept ;
	skos:prefLabel "globular jar"@en , "Kugelf철rmiger Topf"@de ;
	skos:altLabel "Kugeltopf"@de ;
	skos:definition "A small narrow mouthed jar with hemispherical, ovoid, or spherical body." ;
	skos:inScheme <https://acdh.oeaw.ac.at/vocabs/defcthesaurus/FindsSchema> , <https://acdh.oeaw.ac.at/vocabs/defcthesaurus/FindsPotteryForm> ;
	skos:editorialNote "dc_finds_pottery_form;106" ;
	skos:broader <https://acdh.oeaw.ac.at/vocabs/defcthesaurus/jar/4.145> .

<https://acdh.oeaw.ac.at/vocabs/defcthesaurus/jar/4.145> skos:narrower <https://acdh.oeaw.ac.at/vocabs/defcthesaurus/globular_jar/5.106> .

<https://acdh.oeaw.ac.at/vocabs/defcthesaurus/hole-mouthed_jar/5.131> a skos:Concept ;
	skos:prefLabel "hole-mouthed jar"@en , "Engmundiges Gef채"@de ;
	skos:altLabel "holemouthed jar"@en , "bag-shaped vessel"@en , "Engmundiges Topf"@de , "Beutelf철rmiges Gef채"@de ;
	skos:definition "A jar with no rim or neck, rather the vessel lip attaches directily to the vessel wall." ;
	skos:inScheme <https://acdh.oeaw.ac.at/vocabs/defcthesaurus/FindsSchema> , <https://acdh.oeaw.ac.at/vocabs/defcthesaurus/FindsPotteryForm> ;
	skos:editorialNote "dc_finds_pottery_form;131" ;
	skos:broader <https://acdh.oeaw.ac.at/vocabs/defcthesaurus/jar/4.145> .

<https://acdh.oeaw.ac.at/vocabs/defcthesaurus/jar/4.145> skos:narrower <https://acdh.oeaw.ac.at/vocabs/defcthesaurus/hole-mouthed_jar/5.131> .

<https://acdh.oeaw.ac.at/vocabs/defcthesaurus/piriform_jar/4.152> a skos:Concept ;
	skos:prefLabel "piriform jar"@en , "Birnenf철rmiger Topf"@de ;
	skos:definition "A pear-shaped high and open vessel with a maximal diameter generally at the belly." ;
	skos:inScheme <https://acdh.oeaw.ac.at/vocabs/defcthesaurus/FindsSchema> , <https://acdh.oeaw.ac.at/vocabs/defcthesaurus/FindsPotteryForm> ;
	skos:editorialNote "dc_finds_pottery_form;152" ;
	skos:broader <https://acdh.oeaw.ac.at/vocabs/defcthesaurus/pottery_form/3.016> .

<https://acdh.oeaw.ac.at/vocabs/defcthesaurus/pottery_form/3.016> skos:narrower <https://acdh.oeaw.ac.at/vocabs/defcthesaurus/piriform_jar/4.152> .

<https://acdh.oeaw.ac.at/vocabs/defcthesaurus/chalice/4.185> a skos:Concept ;
	skos:prefLabel "chalice"@en , "Kelch"@de ;
	skos:definition "A cup with a foot/pedestal base." ;
	skos:inScheme <https://acdh.oeaw.ac.at/vocabs/defcthesaurus/FindsSchema> , <https://acdh.oeaw.ac.at/vocabs/defcthesaurus/FindsPotteryForm> ;
	skos:editorialNote "dc_finds_pottery_form;185" ;
	skos:broader <https://acdh.oeaw.ac.at/vocabs/defcthesaurus/pottery_form/3.016> .

<https://acdh.oeaw.ac.at/vocabs/defcthesaurus/pottery_form/3.016> skos:narrower <https://acdh.oeaw.ac.at/vocabs/defcthesaurus/chalice/4.185> .

<https://acdh.oeaw.ac.at/vocabs/defcthesaurus/cheese_pot/4.126> a skos:Concept ;
	skos:prefLabel "cheese pot"@en , "Cheese Pot"@de ;
	skos:definition "A flat open vessel with horizontal row of drillings under the rim." ;
	skos:inScheme <https://acdh.oeaw.ac.at/vocabs/defcthesaurus/FindsSchema> , <https://acdh.oeaw.ac.at/vocabs/defcthesaurus/FindsPotteryForm> ;
	skos:editorialNote "dc_finds_pottery_form;126" ;
	skos:broader <https://acdh.oeaw.ac.at/vocabs/defcthesaurus/pottery_form/3.016> .

<https://acdh.oeaw.ac.at/vocabs/defcthesaurus/pottery_form/3.016> skos:narrower <https://acdh.oeaw.ac.at/vocabs/defcthesaurus/cheese_pot/4.126> .

<https://acdh.oeaw.ac.at/vocabs/defcthesaurus/cup/4.107> a skos:Concept ;
	skos:prefLabel "cup"@en , "Tasse"@de ;
	skos:definition "A small open vessel for drinking from, usually with a handle." ;
	skos:inScheme <https://acdh.oeaw.ac.at/vocabs/defcthesaurus/FindsSchema> , <https://acdh.oeaw.ac.at/vocabs/defcthesaurus/FindsPotteryForm> ;
	skos:editorialNote "dc_finds_pottery_form;107" ;
	skos:broader <https://acdh.oeaw.ac.at/vocabs/defcthesaurus/pottery_form/3.016> .

<https://acdh.oeaw.ac.at/vocabs/defcthesaurus/pottery_form/3.016> skos:narrower <https://acdh.oeaw.ac.at/vocabs/defcthesaurus/cup/4.107> .

<https://acdh.oeaw.ac.at/vocabs/defcthesaurus/fikirtepe_box/4.111> a skos:Concept ;
	skos:prefLabel "fikirtepe box"@en , "Fikirtepe Box"@de ;
	skos:definition "A small angular vessel with four legs, decorated on the outside, typically found in Fikirtepe." ;
	skos:inScheme <https://acdh.oeaw.ac.at/vocabs/defcthesaurus/FindsSchema> , <https://acdh.oeaw.ac.at/vocabs/defcthesaurus/FindsPotteryForm> ;
	skos:editorialNote "dc_finds_pottery_form;111" ;
	skos:broader <https://acdh.oeaw.ac.at/vocabs/defcthesaurus/pottery_form/3.016> .

<https://acdh.oeaw.ac.at/vocabs/defcthesaurus/pottery_form/3.016> skos:narrower <https://acdh.oeaw.ac.at/vocabs/defcthesaurus/fikirtepe_box/4.111> .

<https://acdh.oeaw.ac.at/vocabs/defcthesaurus/fruitstand/4.130> a skos:Concept ;
	skos:prefLabel "fruitstand"@en , "Fruchtst채nder"@de ;
	skos:definition "A very low shallow bowl with a high pedestal." ;
	skos:inScheme <https://acdh.oeaw.ac.at/vocabs/defcthesaurus/FindsSchema> , <https://acdh.oeaw.ac.at/vocabs/defcthesaurus/FindsPotteryForm> ;
	skos:editorialNote "dc_finds_pottery_form;130" ;
	skos:broader <https://acdh.oeaw.ac.at/vocabs/defcthesaurus/pottery_form/3.016> .

<https://acdh.oeaw.ac.at/vocabs/defcthesaurus/pottery_form/3.016> skos:narrower <https://acdh.oeaw.ac.at/vocabs/defcthesaurus/fruitstand/4.130> .

<https://acdh.oeaw.ac.at/vocabs/defcthesaurus/goblet/4.201> a skos:Concept ;
	skos:prefLabel "goblet"@en , "Goblet Becher"@de ;
	skos:definition "A deep vessel with straight sides and pedestal, two liminal hoisting handles." ;
	skos:inScheme <https://acdh.oeaw.ac.at/vocabs/defcthesaurus/FindsSchema> , <https://acdh.oeaw.ac.at/vocabs/defcthesaurus/FindsPotteryForm> ;
	skos:editorialNote "dc_finds_pottery_form;201" ;
	skos:broader <https://acdh.oeaw.ac.at/vocabs/defcthesaurus/pottery_form/3.016> .

<https://acdh.oeaw.ac.at/vocabs/defcthesaurus/pottery_form/3.016> skos:narrower <https://acdh.oeaw.ac.at/vocabs/defcthesaurus/goblet/4.201> .

<https://acdh.oeaw.ac.at/vocabs/defcthesaurus/jug/4.110> a skos:Concept ;
	skos:prefLabel "jug"@en , "Krug"@de ;
	skos:definition "A closed vessel designed for pouring, usually with a pouring lip/spout. It may have one handle or nonetypically, one." ;
	skos:inScheme <https://acdh.oeaw.ac.at/vocabs/defcthesaurus/FindsSchema> , <https://acdh.oeaw.ac.at/vocabs/defcthesaurus/FindsPotteryForm> ;
	skos:editorialNote "dc_finds_pottery_form;110" ;
	skos:broader <https://acdh.oeaw.ac.at/vocabs/defcthesaurus/pottery_form/3.016> .

<https://acdh.oeaw.ac.at/vocabs/defcthesaurus/pottery_form/3.016> skos:narrower <https://acdh.oeaw.ac.at/vocabs/defcthesaurus/jug/4.110> .

<https://acdh.oeaw.ac.at/vocabs/defcthesaurus/ladle/4.133> a skos:Concept ;
	skos:prefLabel "ladle"@en , "Sch철pfkelle"@de ;
	skos:definition "A particular piece of cutlery in a form of a long-handled scoop used for ladling food of liquids." ;
	skos:inScheme <https://acdh.oeaw.ac.at/vocabs/defcthesaurus/FindsSchema> , <https://acdh.oeaw.ac.at/vocabs/defcthesaurus/FindsPotteryForm> ;
	skos:editorialNote "dc_finds_pottery_form;133" ;
	skos:broader <https://acdh.oeaw.ac.at/vocabs/defcthesaurus/pottery_form/3.016> .

<https://acdh.oeaw.ac.at/vocabs/defcthesaurus/pottery_form/3.016> skos:narrower <https://acdh.oeaw.ac.at/vocabs/defcthesaurus/ladle/4.133> .

<https://acdh.oeaw.ac.at/vocabs/defcthesaurus/lamp/4.134> a skos:Concept ;
	skos:prefLabel "lamp"@en , "Lampe"@de ;
	skos:definition "A vessel used to produce illumination." ;
	skos:inScheme <https://acdh.oeaw.ac.at/vocabs/defcthesaurus/FindsSchema> , <https://acdh.oeaw.ac.at/vocabs/defcthesaurus/FindsPotteryForm> ;
	skos:editorialNote "dc_finds_pottery_form;134" ;
	skos:broader <https://acdh.oeaw.ac.at/vocabs/defcthesaurus/pottery_form/3.016> .

<https://acdh.oeaw.ac.at/vocabs/defcthesaurus/pottery_form/3.016> skos:narrower <https://acdh.oeaw.ac.at/vocabs/defcthesaurus/lamp/4.134> .

<https://acdh.oeaw.ac.at/vocabs/defcthesaurus/lid/4.112> a skos:Concept ;
	skos:prefLabel "lid"@en , "Deckel"@de ;
	skos:definition "A shape used for covering vessels." ;
	skos:inScheme <https://acdh.oeaw.ac.at/vocabs/defcthesaurus/FindsSchema> , <https://acdh.oeaw.ac.at/vocabs/defcthesaurus/FindsPotteryForm> ;
	skos:editorialNote "dc_finds_pottery_form;112" ;
	skos:broader <https://acdh.oeaw.ac.at/vocabs/defcthesaurus/pottery_form/3.016> .

<https://acdh.oeaw.ac.at/vocabs/defcthesaurus/pottery_form/3.016> skos:narrower <https://acdh.oeaw.ac.at/vocabs/defcthesaurus/lid/4.112> .

<https://acdh.oeaw.ac.at/vocabs/defcthesaurus/mug/4.113> a skos:Concept ;
	skos:prefLabel "mug"@en , "Becher"@de ;
	skos:definition "A small, narrow, deep, drinking vessel with straight sides." ;
	skos:inScheme <https://acdh.oeaw.ac.at/vocabs/defcthesaurus/FindsSchema> , <https://acdh.oeaw.ac.at/vocabs/defcthesaurus/FindsPotteryForm> ;
	skos:editorialNote "dc_finds_pottery_form;113" ;
	skos:broader <https://acdh.oeaw.ac.at/vocabs/defcthesaurus/pottery_form/3.016> .

<https://acdh.oeaw.ac.at/vocabs/defcthesaurus/pottery_form/3.016> skos:narrower <https://acdh.oeaw.ac.at/vocabs/defcthesaurus/mug/4.113> .

<https://acdh.oeaw.ac.at/vocabs/defcthesaurus/ogee-pot/4.195> a skos:Concept ;
	skos:prefLabel "ogee-pot"@en ;
	skos:inScheme <https://acdh.oeaw.ac.at/vocabs/defcthesaurus/FindsSchema> , <https://acdh.oeaw.ac.at/vocabs/defcthesaurus/FindsPotteryForm> ;
	skos:editorialNote "dc_finds_pottery_form;195" ;
	skos:broader <https://acdh.oeaw.ac.at/vocabs/defcthesaurus/pottery_form/3.016> .

<https://acdh.oeaw.ac.at/vocabs/defcthesaurus/pottery_form/3.016> skos:narrower <https://acdh.oeaw.ac.at/vocabs/defcthesaurus/ogee-pot/4.195> .

<https://acdh.oeaw.ac.at/vocabs/defcthesaurus/pottery/2.4> dc:source "Kipfer, B. A. Dictionary of Artifacts 2007. Blackwell Publishing, Oxford.p 243" .

<https://acdh.oeaw.ac.at/vocabs/defcthesaurus/pithos/4.135> a skos:Concept ;
	skos:prefLabel "pithos"@en , "Pithos"@de ;
	skos:definition "A large storage vessel with thick walls with a narrow neck. On occasion they were also used for jar burial in the Aegean area." ;
	skos:inScheme <https://acdh.oeaw.ac.at/vocabs/defcthesaurus/FindsSchema> , <https://acdh.oeaw.ac.at/vocabs/defcthesaurus/FindsPotteryForm> ;
	skos:editorialNote "dc_finds_pottery_form;135" ;
	skos:broader <https://acdh.oeaw.ac.at/vocabs/defcthesaurus/pottery_form/3.016> .

<https://acdh.oeaw.ac.at/vocabs/defcthesaurus/pottery_form/3.016> skos:narrower <https://acdh.oeaw.ac.at/vocabs/defcthesaurus/pithos/4.135> .

<https://acdh.oeaw.ac.at/vocabs/defcthesaurus/plate/4.165> a skos:Concept ;
	skos:prefLabel "plate"@en , "Platte"@de ;
	skos:altLabel "Teller"@de ;
	skos:definition "A very low or even flat vessel." ;
	skos:inScheme <https://acdh.oeaw.ac.at/vocabs/defcthesaurus/FindsSchema> , <https://acdh.oeaw.ac.at/vocabs/defcthesaurus/FindsPotteryForm> ;
	skos:editorialNote "dc_finds_pottery_form;165" ;
	skos:broader <https://acdh.oeaw.ac.at/vocabs/defcthesaurus/pottery_form/3.016> .

<https://acdh.oeaw.ac.at/vocabs/defcthesaurus/pottery_form/3.016> skos:narrower <https://acdh.oeaw.ac.at/vocabs/defcthesaurus/plate/4.165> .

<https://acdh.oeaw.ac.at/vocabs/defcthesaurus/pyxis/4.166> a skos:Concept ;
	skos:prefLabel "pyxis"@en , "Pyxis"@de ;
	skos:definition "A cylindrical box-like vessel with angular shoulders and lid." ;
	skos:inScheme <https://acdh.oeaw.ac.at/vocabs/defcthesaurus/FindsSchema> , <https://acdh.oeaw.ac.at/vocabs/defcthesaurus/FindsPotteryForm> ;
	skos:editorialNote "dc_finds_pottery_form;166" ;
	skos:broader <https://acdh.oeaw.ac.at/vocabs/defcthesaurus/pottery_form/3.016> .

<https://acdh.oeaw.ac.at/vocabs/defcthesaurus/pottery_form/3.016> skos:narrower <https://acdh.oeaw.ac.at/vocabs/defcthesaurus/pyxis/4.166> .

<https://acdh.oeaw.ac.at/vocabs/defcthesaurus/rhyton/4.186> a skos:Concept ;
	skos:prefLabel "rhyton"@en , "Rhyton"@de ;
	skos:definition "Zoomorphic vessel in a shape of a horn used for drinking and pouring." ;
	skos:inScheme <https://acdh.oeaw.ac.at/vocabs/defcthesaurus/FindsSchema> , <https://acdh.oeaw.ac.at/vocabs/defcthesaurus/FindsPotteryForm> ;
	skos:editorialNote "dc_finds_pottery_form;186" ;
	skos:broader <https://acdh.oeaw.ac.at/vocabs/defcthesaurus/pottery_form/3.016> .

<https://acdh.oeaw.ac.at/vocabs/defcthesaurus/pottery_form/3.016> skos:narrower <https://acdh.oeaw.ac.at/vocabs/defcthesaurus/rhyton/4.186> .

<https://acdh.oeaw.ac.at/vocabs/defcthesaurus/scoop/4.136> a skos:Concept ;
	skos:prefLabel "scoop"@en , "Sch철pfgef채"@de ;
	skos:definition "A vessel used for scooping of liquids or solids." ;
	skos:inScheme <https://acdh.oeaw.ac.at/vocabs/defcthesaurus/FindsSchema> , <https://acdh.oeaw.ac.at/vocabs/defcthesaurus/FindsPotteryForm> ;
	skos:editorialNote "dc_finds_pottery_form;136" ;
	skos:broader <https://acdh.oeaw.ac.at/vocabs/defcthesaurus/pottery_form/3.016> .

<https://acdh.oeaw.ac.at/vocabs/defcthesaurus/pottery_form/3.016> skos:narrower <https://acdh.oeaw.ac.at/vocabs/defcthesaurus/scoop/4.136> .

<https://acdh.oeaw.ac.at/vocabs/defcthesaurus/sieve/4.117> a skos:Concept ;
	skos:prefLabel "sieve"@en , "Sieb"@de ;
	skos:definition "A container whose walls are completely or partially pierced used for separating liquids and solids." ;
	skos:inScheme <https://acdh.oeaw.ac.at/vocabs/defcthesaurus/FindsSchema> , <https://acdh.oeaw.ac.at/vocabs/defcthesaurus/FindsPotteryForm> ;
	skos:editorialNote "dc_finds_pottery_form;117" ;
	skos:broader <https://acdh.oeaw.ac.at/vocabs/defcthesaurus/pottery_form/3.016> .

<https://acdh.oeaw.ac.at/vocabs/defcthesaurus/pottery_form/3.016> skos:narrower <https://acdh.oeaw.ac.at/vocabs/defcthesaurus/sieve/4.117> .

<https://acdh.oeaw.ac.at/vocabs/defcthesaurus/skyphos/4.157> a skos:Concept ;
	skos:prefLabel "skyphos"@en , "Skyphos"@de ;
	skos:definition "A two-handled deep drinking cup." ;
	skos:inScheme <https://acdh.oeaw.ac.at/vocabs/defcthesaurus/FindsSchema> , <https://acdh.oeaw.ac.at/vocabs/defcthesaurus/FindsPotteryForm> ;
	skos:editorialNote "dc_finds_pottery_form;157" ;
	skos:broader <https://acdh.oeaw.ac.at/vocabs/defcthesaurus/pottery_form/3.016> .

<https://acdh.oeaw.ac.at/vocabs/defcthesaurus/pottery_form/3.016> skos:narrower <https://acdh.oeaw.ac.at/vocabs/defcthesaurus/skyphos/4.157> .

<https://acdh.oeaw.ac.at/vocabs/defcthesaurus/stand/4.169> a skos:Concept ;
	skos:prefLabel "stand"@en , "St채nder"@de ;
	skos:definition "A ceramic collar placed under a round or pointed bottom vessel in order to support or stabilize the vessel." ;
	skos:inScheme <https://acdh.oeaw.ac.at/vocabs/defcthesaurus/FindsSchema> , <https://acdh.oeaw.ac.at/vocabs/defcthesaurus/FindsPotteryForm> ;
	skos:editorialNote "dc_finds_pottery_form;169" ;
	skos:broader <https://acdh.oeaw.ac.at/vocabs/defcthesaurus/pottery_form/3.016> .

<https://acdh.oeaw.ac.at/vocabs/defcthesaurus/pottery_form/3.016> skos:narrower <https://acdh.oeaw.ac.at/vocabs/defcthesaurus/stand/4.169> .

<https://acdh.oeaw.ac.at/vocabs/defcthesaurus/tripod/4.137> a skos:Concept ;
	skos:prefLabel "tripod"@en , "Dreifu"@de ;
	skos:definition "A vessel standing on three legs." ;
	skos:inScheme <https://acdh.oeaw.ac.at/vocabs/defcthesaurus/FindsSchema> , <https://acdh.oeaw.ac.at/vocabs/defcthesaurus/FindsPotteryForm> ;
	skos:editorialNote "dc_finds_pottery_form;137" ;
	skos:broader <https://acdh.oeaw.ac.at/vocabs/defcthesaurus/pottery_form/3.016> .

<https://acdh.oeaw.ac.at/vocabs/defcthesaurus/pottery_form/3.016> skos:narrower <https://acdh.oeaw.ac.at/vocabs/defcthesaurus/tripod/4.137> .

<https://acdh.oeaw.ac.at/vocabs/defcthesaurus/tulip-shaped_beaker/4.118> a skos:Concept ;
	skos:prefLabel "tulip-shaped beaker"@en , "Tulpenf철rmger Becher"@de ;
	skos:definition "A handled cup in a form of a bell." ;
	skos:inScheme <https://acdh.oeaw.ac.at/vocabs/defcthesaurus/FindsSchema> , <https://acdh.oeaw.ac.at/vocabs/defcthesaurus/FindsPotteryForm> ;
	skos:editorialNote "dc_finds_pottery_form;118" ;
	skos:broader <https://acdh.oeaw.ac.at/vocabs/defcthesaurus/pottery_form/3.016> .

<https://acdh.oeaw.ac.at/vocabs/defcthesaurus/pottery_form/3.016> skos:narrower <https://acdh.oeaw.ac.at/vocabs/defcthesaurus/tulip-shaped_beaker/4.118> .

<https://acdh.oeaw.ac.at/vocabs/defcthesaurus/zoomorphic_vessel/4.100> a skos:Concept ;
	skos:prefLabel "zoomorphic vessel"@en , "Zoomorphes Gef채"@de ;
	skos:definition "Animal shaped vessel." ;
	skos:inScheme <https://acdh.oeaw.ac.at/vocabs/defcthesaurus/FindsSchema> , <https://acdh.oeaw.ac.at/vocabs/defcthesaurus/FindsPotteryForm> ;
	skos:editorialNote "dc_finds_pottery_form;100" ;
	skos:broader <https://acdh.oeaw.ac.at/vocabs/defcthesaurus/pottery_form/3.016> .

<https://acdh.oeaw.ac.at/vocabs/defcthesaurus/pottery_form/3.016> skos:narrower <https://acdh.oeaw.ac.at/vocabs/defcthesaurus/zoomorphic_vessel/4.100> .

<https://acdh.oeaw.ac.at/vocabs/defcthesaurus/pottery_fragment/3.017> a skos:Concept ;
	skos:prefLabel "pottery fragment"@en , "Keramikdetail"@de ;
	skos:inScheme <https://acdh.oeaw.ac.at/vocabs/defcthesaurus/FindsSchema> , <https://acdh.oeaw.ac.at/vocabs/defcthesaurus/NotInDatabase> ;
	skos:editorialNote "dc_not_in_database;017" ;
	skos:broader <https://acdh.oeaw.ac.at/vocabs/defcthesaurus/pottery/2.4> .

<https://acdh.oeaw.ac.at/vocabs/defcthesaurus/pottery/2.4> skos:narrower <https://acdh.oeaw.ac.at/vocabs/defcthesaurus/pottery_fragment/3.017> .

<https://acdh.oeaw.ac.at/vocabs/defcthesaurus/handle/4.031> a skos:Concept ;
	skos:prefLabel "handle"@en , "Henkel"@de ;
	skos:inScheme <https://acdh.oeaw.ac.at/vocabs/defcthesaurus/FindsSchema> , <https://acdh.oeaw.ac.at/vocabs/defcthesaurus/NotInDatabase> ;
	skos:editorialNote "dc_not_in_database;031" ;
	skos:broader <https://acdh.oeaw.ac.at/vocabs/defcthesaurus/pottery_fragment/3.017> .

<https://acdh.oeaw.ac.at/vocabs/defcthesaurus/pottery_fragment/3.017> skos:narrower <https://acdh.oeaw.ac.at/vocabs/defcthesaurus/handle/4.031> .

<https://acdh.oeaw.ac.at/vocabs/defcthesaurus/FindsPotteryDetail> a skos:ConceptScheme ;
	rdfs:comment "A concept schema related to the particular finds properties." .

<https://acdh.oeaw.ac.at/vocabs/defcthesaurus/round_bar_handle/5.109> a skos:Concept ;
	skos:prefLabel "round bar handle"@en , "Stabhenkel"@de ;
	skos:definition "Flattened handle with a round cross section." ;
	skos:inScheme <https://acdh.oeaw.ac.at/vocabs/defcthesaurus/FindsSchema> , <https://acdh.oeaw.ac.at/vocabs/defcthesaurus/FindsPotteryDetail> ;
	skos:editorialNote "dc_finds_pottery_detail;109" ;
	skos:broader <https://acdh.oeaw.ac.at/vocabs/defcthesaurus/handle/4.031> .

<https://acdh.oeaw.ac.at/vocabs/defcthesaurus/handle/4.031> skos:narrower <https://acdh.oeaw.ac.at/vocabs/defcthesaurus/round_bar_handle/5.109> .

<https://acdh.oeaw.ac.at/vocabs/defcthesaurus/bar_handle_with_knob/6.67> a skos:Concept ;
	skos:prefLabel "bar handle with knob"@en , "Stabhenkel mit Knubbe"@de ;
	skos:definition "Bar shaped handle with an applied knob." ;
	skos:inScheme <https://acdh.oeaw.ac.at/vocabs/defcthesaurus/FindsSchema> , <https://acdh.oeaw.ac.at/vocabs/defcthesaurus/FindsPotteryDetail> ;
	skos:editorialNote "dc_finds_pottery_detail;02" ;
	skos:broader <https://acdh.oeaw.ac.at/vocabs/defcthesaurus/round_bar_handle/5.109> .

<https://acdh.oeaw.ac.at/vocabs/defcthesaurus/round_bar_handle/5.109> skos:narrower <https://acdh.oeaw.ac.at/vocabs/defcthesaurus/bar_handle_with_knob/6.67> .

<https://acdh.oeaw.ac.at/vocabs/defcthesaurus/crescent-shaped_handle/5.171> a skos:Concept ;
	skos:prefLabel "crescent-shaped handle"@en , "Mondf철rmiger Henkel"@de ;
	skos:definition "(Half)moon shaped handle." ;
	skos:inScheme <https://acdh.oeaw.ac.at/vocabs/defcthesaurus/FindsSchema> , <https://acdh.oeaw.ac.at/vocabs/defcthesaurus/FindsPotteryDetail> ;
	skos:editorialNote "dc_finds_pottery_detail;171" ;
	skos:broader <https://acdh.oeaw.ac.at/vocabs/defcthesaurus/handle/4.031> .

<https://acdh.oeaw.ac.at/vocabs/defcthesaurus/handle/4.031> skos:narrower <https://acdh.oeaw.ac.at/vocabs/defcthesaurus/crescent-shaped_handle/5.171> .

<https://acdh.oeaw.ac.at/vocabs/defcthesaurus/tab_handle/5.96> a skos:Concept ;
	skos:prefLabel "tab handle"@en , "Grifflappen"@de ;
	skos:altLabel "hammer rims"@en ;
	skos:definition "Flat handle." ;
	skos:inScheme <https://acdh.oeaw.ac.at/vocabs/defcthesaurus/FindsSchema> , <https://acdh.oeaw.ac.at/vocabs/defcthesaurus/FindsPotteryDetail> ;
	skos:editorialNote "dc_finds_pottery_detail;96" ;
	skos:broader <https://acdh.oeaw.ac.at/vocabs/defcthesaurus/handle/4.031> .

<https://acdh.oeaw.ac.at/vocabs/defcthesaurus/handle/4.031> skos:narrower <https://acdh.oeaw.ac.at/vocabs/defcthesaurus/tab_handle/5.96> .

<https://acdh.oeaw.ac.at/vocabs/defcthesaurus/tab_handle/5.169> a skos:Concept ;
	skos:prefLabel "tab handle"@en , "Grifflappen"@de ;
	skos:altLabel "hammer rims"@en ;
	skos:definition "Flat handle." ;
	skos:inScheme <https://acdh.oeaw.ac.at/vocabs/defcthesaurus/FindsSchema> , <https://acdh.oeaw.ac.at/vocabs/defcthesaurus/FindsPotteryDetail> ;
	skos:editorialNote "dc_finds_pottery_detail;169" ;
	skos:broader <https://acdh.oeaw.ac.at/vocabs/defcthesaurus/handle/4.031> .

<https://acdh.oeaw.ac.at/vocabs/defcthesaurus/handle/4.031> skos:narrower <https://acdh.oeaw.ac.at/vocabs/defcthesaurus/tab_handle/5.169> .

<https://acdh.oeaw.ac.at/vocabs/defcthesaurus/double_tab_handle/6.97> a skos:Concept ;
	skos:prefLabel "double tab handle"@en , "Doppelter Grifflappen"@de ;
	skos:definition "Double flat handle." ;
	skos:inScheme <https://acdh.oeaw.ac.at/vocabs/defcthesaurus/FindsSchema> , <https://acdh.oeaw.ac.at/vocabs/defcthesaurus/FindsPotteryDetail> ;
	skos:editorialNote "dc_finds_pottery_detail;02" ;
	skos:broader <https://acdh.oeaw.ac.at/vocabs/defcthesaurus/tab_handle/5.96> .

<https://acdh.oeaw.ac.at/vocabs/defcthesaurus/tab_handle/5.96> skos:narrower <https://acdh.oeaw.ac.at/vocabs/defcthesaurus/double_tab_handle/6.97> .

<https://acdh.oeaw.ac.at/vocabs/defcthesaurus/wishbone_handle/5.93> a skos:Concept ;
	skos:prefLabel "wishbone handle"@en , "Gabelhenkel"@de ;
	skos:altLabel "Wishbonehenkel"@de ;
	skos:definition "A liminal horizontal loop handle with a bird-bone shape." ;
	skos:inScheme <https://acdh.oeaw.ac.at/vocabs/defcthesaurus/FindsSchema> , <https://acdh.oeaw.ac.at/vocabs/defcthesaurus/FindsPotteryDetail> ;
	skos:editorialNote "dc_finds_pottery_detail;93" ;
	skos:broader <https://acdh.oeaw.ac.at/vocabs/defcthesaurus/handle/4.031> .

<https://acdh.oeaw.ac.at/vocabs/defcthesaurus/handle/4.031> skos:narrower <https://acdh.oeaw.ac.at/vocabs/defcthesaurus/wishbone_handle/5.93> .

<https://acdh.oeaw.ac.at/vocabs/defcthesaurus/double-horned_wishbone_handle/6.156> a skos:Concept ;
	skos:prefLabel "double-horned wishbone handle"@en , "Wishbonehenkel mit doppelten Hornaufsatz"@de ;
	skos:definition "A liminal, horizontal, bird-bone shaped, loop handle with two objects applied that are narrow at one end and much wider at the other." ;
	skos:inScheme <https://acdh.oeaw.ac.at/vocabs/defcthesaurus/FindsSchema> , <https://acdh.oeaw.ac.at/vocabs/defcthesaurus/FindsPotteryDetail> ;
	skos:editorialNote "dc_finds_pottery_detail;02" ;
	skos:broader <https://acdh.oeaw.ac.at/vocabs/defcthesaurus/wishbone_handle/5.93> .

<https://acdh.oeaw.ac.at/vocabs/defcthesaurus/wishbone_handle/5.93> skos:narrower <https://acdh.oeaw.ac.at/vocabs/defcthesaurus/double-horned_wishbone_handle/6.156> .

<https://acdh.oeaw.ac.at/vocabs/defcthesaurus/knobbed_wishbone_handle/6.144> a skos:Concept ;
	skos:prefLabel "knobbed wishbone handle"@en , "Gabelhenkel mit Knubbe"@de ;
	skos:definition "A liminal horizontal birdbone shaped loop handle with round applications." ;
	skos:inScheme <https://acdh.oeaw.ac.at/vocabs/defcthesaurus/FindsSchema> , <https://acdh.oeaw.ac.at/vocabs/defcthesaurus/FindsPotteryDetail> ;
	skos:editorialNote "dc_finds_pottery_detail;02" ;
	skos:broader <https://acdh.oeaw.ac.at/vocabs/defcthesaurus/wishbone_handle/5.93> .

<https://acdh.oeaw.ac.at/vocabs/defcthesaurus/wishbone_handle/5.93> skos:narrower <https://acdh.oeaw.ac.at/vocabs/defcthesaurus/knobbed_wishbone_handle/6.144> .

<https://acdh.oeaw.ac.at/vocabs/defcthesaurus/pronged_wishbone_handle/6.148> a skos:Concept ;
	skos:prefLabel "pronged wishbone handle"@en , "Gabelhenkel mit Stabaufsatz"@de ;
	skos:definition "A liminal, horizontal, bird-bone shaped, loop handle with bar application." ;
	skos:inScheme <https://acdh.oeaw.ac.at/vocabs/defcthesaurus/FindsSchema> , <https://acdh.oeaw.ac.at/vocabs/defcthesaurus/FindsPotteryDetail> ;
	skos:editorialNote "dc_finds_pottery_detail;02" ;
	skos:broader <https://acdh.oeaw.ac.at/vocabs/defcthesaurus/wishbone_handle/5.93> .

<https://acdh.oeaw.ac.at/vocabs/defcthesaurus/wishbone_handle/5.93> skos:narrower <https://acdh.oeaw.ac.at/vocabs/defcthesaurus/pronged_wishbone_handle/6.148> .

<https://acdh.oeaw.ac.at/vocabs/defcthesaurus/ear_handle/5.118> a skos:Concept ;
	skos:prefLabel "ear handle"@en , "Ohrhenkel"@de ;
	skos:definition "A vertical loop handle in a shape of an ear." ;
	skos:inScheme <https://acdh.oeaw.ac.at/vocabs/defcthesaurus/FindsSchema> , <https://acdh.oeaw.ac.at/vocabs/defcthesaurus/FindsPotteryDetail> ;
	skos:editorialNote "dc_finds_pottery_detail;118" ;
	skos:broader <https://acdh.oeaw.ac.at/vocabs/defcthesaurus/handle/4.031> .

<https://acdh.oeaw.ac.at/vocabs/defcthesaurus/handle/4.031> skos:narrower <https://acdh.oeaw.ac.at/vocabs/defcthesaurus/ear_handle/5.118> .

<https://acdh.oeaw.ac.at/vocabs/defcthesaurus/elongated_handle/5.170> a skos:Concept ;
	skos:prefLabel "elongated handle"@en , "langezogener Henkel"@de ;
	skos:definition "A lug in a shape of an elephant쨈s head." ;
	skos:inScheme <https://acdh.oeaw.ac.at/vocabs/defcthesaurus/FindsSchema> , <https://acdh.oeaw.ac.at/vocabs/defcthesaurus/FindsPotteryDetail> ;
	skos:editorialNote "dc_finds_pottery_detail;170" ;
	skos:broader <https://acdh.oeaw.ac.at/vocabs/defcthesaurus/handle/4.031> .

<https://acdh.oeaw.ac.at/vocabs/defcthesaurus/handle/4.031> skos:narrower <https://acdh.oeaw.ac.at/vocabs/defcthesaurus/elongated_handle/5.170> .

<https://acdh.oeaw.ac.at/vocabs/defcthesaurus/strap_handle/5.78> a skos:Concept ;
	skos:prefLabel "strap handle"@en , "Bandhenkel"@de ;
	skos:definition "A handle made from a strip of clay and attached to the body of the pot at two points before firing." ;
	skos:inScheme <https://acdh.oeaw.ac.at/vocabs/defcthesaurus/FindsSchema> , <https://acdh.oeaw.ac.at/vocabs/defcthesaurus/FindsPotteryDetail> ;
	skos:editorialNote "dc_finds_pottery_detail;78" ;
	skos:broader <https://acdh.oeaw.ac.at/vocabs/defcthesaurus/handle/4.031> .

<https://acdh.oeaw.ac.at/vocabs/defcthesaurus/handle/4.031> skos:narrower <https://acdh.oeaw.ac.at/vocabs/defcthesaurus/strap_handle/5.78> .

<https://acdh.oeaw.ac.at/vocabs/defcthesaurus/finds_type/1.02> dc:source "Kipfer, B. A. Dictionary of Artifacts 2007. Blackwell Publishing, Oxford.p 305" .

<https://acdh.oeaw.ac.at/vocabs/defcthesaurus/high_strap_handle/6.119> a skos:Concept ;
	skos:prefLabel "high strap handle"@en , "Hochgezogener Bandhenkel"@de ;
	skos:definition "Hoisting handle made from a strip of clay and attached to the body of the pot at two points before firing." ;
	skos:inScheme <https://acdh.oeaw.ac.at/vocabs/defcthesaurus/FindsSchema> , <https://acdh.oeaw.ac.at/vocabs/defcthesaurus/FindsPotteryDetail> ;
	skos:editorialNote "dc_finds_pottery_detail;02" ;
	skos:broader <https://acdh.oeaw.ac.at/vocabs/defcthesaurus/strap_handle/5.78> .

<https://acdh.oeaw.ac.at/vocabs/defcthesaurus/strap_handle/5.78> skos:narrower <https://acdh.oeaw.ac.at/vocabs/defcthesaurus/high_strap_handle/6.119> .

<https://acdh.oeaw.ac.at/vocabs/defcthesaurus/high_strap_handle_with_knob/6.90> a skos:Concept ;
	skos:prefLabel "high strap handle with knob"@en , "Hochgezogener Bandhenkel mit Knubbe"@de ;
	skos:definition "Hoisting handle made from a strip of clay with round clay application of semicirucular cross section attached to the body of the pot at two points before firing." ;
	skos:inScheme <https://acdh.oeaw.ac.at/vocabs/defcthesaurus/FindsSchema> , <https://acdh.oeaw.ac.at/vocabs/defcthesaurus/FindsPotteryDetail> ;
	skos:editorialNote "dc_finds_pottery_detail;02" ;
	skos:broader <https://acdh.oeaw.ac.at/vocabs/defcthesaurus/strap_handle/5.78> .

<https://acdh.oeaw.ac.at/vocabs/defcthesaurus/strap_handle/5.78> skos:narrower <https://acdh.oeaw.ac.at/vocabs/defcthesaurus/high_strap_handle_with_knob/6.90> .

<https://acdh.oeaw.ac.at/vocabs/defcthesaurus/horned_strap_handle/6.92> a skos:Concept ;
	skos:prefLabel "horned strap handle"@en , "Bandhenkel mit Hornaufsatz"@de ;
	skos:definition "A handle made from a strip of clay with pointy (horn) application." ;
	skos:inScheme <https://acdh.oeaw.ac.at/vocabs/defcthesaurus/FindsSchema> , <https://acdh.oeaw.ac.at/vocabs/defcthesaurus/FindsPotteryDetail> ;
	skos:editorialNote "dc_finds_pottery_detail;02" ;
	skos:broader <https://acdh.oeaw.ac.at/vocabs/defcthesaurus/strap_handle/5.78> .

<https://acdh.oeaw.ac.at/vocabs/defcthesaurus/strap_handle/5.78> skos:narrower <https://acdh.oeaw.ac.at/vocabs/defcthesaurus/horned_strap_handle/6.92> .

<https://acdh.oeaw.ac.at/vocabs/defcthesaurus/miniature_strap_handle/6.147> a skos:Concept ;
	skos:prefLabel "miniature strap handle"@en , "Miniaturbandhenkel"@de ;
	skos:definition "A very small strip of clay attached to the vessel body before firing." ;
	skos:inScheme <https://acdh.oeaw.ac.at/vocabs/defcthesaurus/FindsSchema> , <https://acdh.oeaw.ac.at/vocabs/defcthesaurus/FindsPotteryDetail> ;
	skos:editorialNote "dc_finds_pottery_detail;02" ;
	skos:broader <https://acdh.oeaw.ac.at/vocabs/defcthesaurus/strap_handle/5.78> .

<https://acdh.oeaw.ac.at/vocabs/defcthesaurus/strap_handle/5.78> skos:narrower <https://acdh.oeaw.ac.at/vocabs/defcthesaurus/miniature_strap_handle/6.147> .

<https://acdh.oeaw.ac.at/vocabs/defcthesaurus/rim-attached_strap_handle/6.151> a skos:Concept ;
	skos:prefLabel "rim-attached strap handle"@en , "Randst채ndiger Bandhenkel"@de ;
	skos:definition "Liminal strip of clay attached to a vessel before firing." ;
	skos:inScheme <https://acdh.oeaw.ac.at/vocabs/defcthesaurus/FindsSchema> , <https://acdh.oeaw.ac.at/vocabs/defcthesaurus/FindsPotteryDetail> ;
	skos:editorialNote "dc_finds_pottery_detail;02" ;
	skos:broader <https://acdh.oeaw.ac.at/vocabs/defcthesaurus/strap_handle/5.78> .

<https://acdh.oeaw.ac.at/vocabs/defcthesaurus/strap_handle/5.78> skos:narrower <https://acdh.oeaw.ac.at/vocabs/defcthesaurus/rim-attached_strap_handle/6.151> .

<https://acdh.oeaw.ac.at/vocabs/defcthesaurus/strap_handle_with_knob/6.91> a skos:Concept ;
	skos:prefLabel "strap handle with knob"@en , "Bandhenkel mit Knubbe"@de ;
	skos:definition "A handle made from a strip of clay with round application, attached to the body of the pot at two points before firing." ;
	skos:inScheme <https://acdh.oeaw.ac.at/vocabs/defcthesaurus/FindsSchema> , <https://acdh.oeaw.ac.at/vocabs/defcthesaurus/FindsPotteryDetail> ;
	skos:editorialNote "dc_finds_pottery_detail;02" ;
	skos:broader <https://acdh.oeaw.ac.at/vocabs/defcthesaurus/strap_handle/5.78> .

<https://acdh.oeaw.ac.at/vocabs/defcthesaurus/strap_handle/5.78> skos:narrower <https://acdh.oeaw.ac.at/vocabs/defcthesaurus/strap_handle_with_knob/6.91> .

<https://acdh.oeaw.ac.at/vocabs/defcthesaurus/strap_handle_with_round_hole/6.149> a skos:Concept ;
	skos:prefLabel "strap handle with round hole"@en , "Bandhenkel mit rundem Loch"@de ;
	skos:definition "A handle made from a strip of clay with a round loop and attached to the body of the pot at two points before firing." ;
	skos:inScheme <https://acdh.oeaw.ac.at/vocabs/defcthesaurus/FindsSchema> , <https://acdh.oeaw.ac.at/vocabs/defcthesaurus/FindsPotteryDetail> ;
	skos:editorialNote "dc_finds_pottery_detail;02" ;
	skos:broader <https://acdh.oeaw.ac.at/vocabs/defcthesaurus/strap_handle/5.78> .

<https://acdh.oeaw.ac.at/vocabs/defcthesaurus/strap_handle/5.78> skos:narrower <https://acdh.oeaw.ac.at/vocabs/defcthesaurus/strap_handle_with_round_hole/6.149> .

<https://acdh.oeaw.ac.at/vocabs/defcthesaurus/winged_strap_handle/6.154> a skos:Concept ;
	skos:prefLabel "winged strap handle"@en , "gefl체gelte Bandhenkel"@de ;
	skos:definition "Strap handle with winged side." ;
	skos:inScheme <https://acdh.oeaw.ac.at/vocabs/defcthesaurus/FindsSchema> , <https://acdh.oeaw.ac.at/vocabs/defcthesaurus/FindsPotteryDetail> ;
	skos:editorialNote "dc_finds_pottery_detail;02" ;
	skos:broader <https://acdh.oeaw.ac.at/vocabs/defcthesaurus/strap_handle/5.78> .

<https://acdh.oeaw.ac.at/vocabs/defcthesaurus/strap_handle/5.78> skos:narrower <https://acdh.oeaw.ac.at/vocabs/defcthesaurus/winged_strap_handle/6.154> .

<https://acdh.oeaw.ac.at/vocabs/defcthesaurus/horned_handle/5.72> a skos:Concept ;
	skos:prefLabel "horned handle"@en , "Henkel mit Hornaufsatz"@de ;
	skos:altLabel "horn handle"@en , "Hornhenkel"@de ;
	skos:definition "A handle in a shape of a horn  wide at one end and pointy at the other, upper end or a handle with pointy applcations." ;
	skos:inScheme <https://acdh.oeaw.ac.at/vocabs/defcthesaurus/FindsSchema> , <https://acdh.oeaw.ac.at/vocabs/defcthesaurus/FindsPotteryDetail> ;
	skos:editorialNote "dc_finds_pottery_detail;72" ;
	skos:broader <https://acdh.oeaw.ac.at/vocabs/defcthesaurus/handle/4.031> .

<https://acdh.oeaw.ac.at/vocabs/defcthesaurus/handle/4.031> skos:narrower <https://acdh.oeaw.ac.at/vocabs/defcthesaurus/horned_handle/5.72> .

<https://acdh.oeaw.ac.at/vocabs/defcthesaurus/knobbed_handle/5.120> a skos:Concept ;
	skos:prefLabel "knobbed handle"@en , "Henkel mit aufgesetzter Knubbe"@de ;
	skos:definition "A handle with round application(s)." ;
	skos:inScheme <https://acdh.oeaw.ac.at/vocabs/defcthesaurus/FindsSchema> , <https://acdh.oeaw.ac.at/vocabs/defcthesaurus/FindsPotteryDetail> ;
	skos:editorialNote "dc_finds_pottery_detail;120" ;
	skos:broader <https://acdh.oeaw.ac.at/vocabs/defcthesaurus/handle/4.031> .

<https://acdh.oeaw.ac.at/vocabs/defcthesaurus/handle/4.031> skos:narrower <https://acdh.oeaw.ac.at/vocabs/defcthesaurus/knobbed_handle/5.120> .

<https://acdh.oeaw.ac.at/vocabs/defcthesaurus/mushroom_handle/5.75> a skos:Concept ;
	skos:prefLabel "mushroom handle"@en , "Henkel mit pilzf철rmigem Aufsatz"@de ;
	skos:altLabel "mushroom headed handle"@en ;
	skos:definition "A handle with an applied round object on a stem made of clay." ;
	skos:inScheme <https://acdh.oeaw.ac.at/vocabs/defcthesaurus/FindsSchema> , <https://acdh.oeaw.ac.at/vocabs/defcthesaurus/FindsPotteryDetail> ;
	skos:editorialNote "dc_finds_pottery_detail;75" ;
	skos:broader <https://acdh.oeaw.ac.at/vocabs/defcthesaurus/handle/4.031> .

<https://acdh.oeaw.ac.at/vocabs/defcthesaurus/handle/4.031> skos:narrower <https://acdh.oeaw.ac.at/vocabs/defcthesaurus/mushroom_handle/5.75> .

<https://acdh.oeaw.ac.at/vocabs/defcthesaurus/pronged_handle/5.130> a skos:Concept ;
	skos:prefLabel "pronged handle"@en , "Henkel mit Stabaufsatz"@de ;
	skos:definition "A handle with bar application." ;
	skos:inScheme <https://acdh.oeaw.ac.at/vocabs/defcthesaurus/FindsSchema> , <https://acdh.oeaw.ac.at/vocabs/defcthesaurus/FindsPotteryDetail> ;
	skos:editorialNote "dc_finds_pottery_detail;130" ;
	skos:broader <https://acdh.oeaw.ac.at/vocabs/defcthesaurus/handle/4.031> .

<https://acdh.oeaw.ac.at/vocabs/defcthesaurus/handle/4.031> skos:narrower <https://acdh.oeaw.ac.at/vocabs/defcthesaurus/pronged_handle/5.130> .

<https://acdh.oeaw.ac.at/vocabs/defcthesaurus/ring_handle/5.100> a skos:Concept ;
	skos:prefLabel "ring handle"@en , "Ringhenkel"@de ;
	skos:definition "A handle with a round loop." ;
	skos:inScheme <https://acdh.oeaw.ac.at/vocabs/defcthesaurus/FindsSchema> , <https://acdh.oeaw.ac.at/vocabs/defcthesaurus/FindsPotteryDetail> ;
	skos:editorialNote "dc_finds_pottery_detail;100" ;
	skos:broader <https://acdh.oeaw.ac.at/vocabs/defcthesaurus/handle/4.031> .

<https://acdh.oeaw.ac.at/vocabs/defcthesaurus/handle/4.031> skos:narrower <https://acdh.oeaw.ac.at/vocabs/defcthesaurus/ring_handle/5.100> .

<https://acdh.oeaw.ac.at/vocabs/defcthesaurus/small_ring_handle/6.102> a skos:Concept ;
	skos:prefLabel "small ring handle"@en , "kleiner Ringhenkel"@de ;
	skos:definition "A handle with a very small round loop." ;
	skos:inScheme <https://acdh.oeaw.ac.at/vocabs/defcthesaurus/FindsSchema> , <https://acdh.oeaw.ac.at/vocabs/defcthesaurus/FindsPotteryDetail> ;
	skos:editorialNote "dc_finds_pottery_detail;02" ;
	skos:broader <https://acdh.oeaw.ac.at/vocabs/defcthesaurus/ring_handle/5.100> .

<https://acdh.oeaw.ac.at/vocabs/defcthesaurus/ring_handle/5.100> skos:narrower <https://acdh.oeaw.ac.at/vocabs/defcthesaurus/small_ring_handle/6.102> .

<https://acdh.oeaw.ac.at/vocabs/defcthesaurus/triangular_ring_handle/6.101> a skos:Concept ;
	skos:prefLabel "triangular ring handle"@en , "dreieckiger Ringhenkel"@de ;
	skos:definition "Pyramid-shaped handle with a round loop." ;
	skos:inScheme <https://acdh.oeaw.ac.at/vocabs/defcthesaurus/FindsSchema> , <https://acdh.oeaw.ac.at/vocabs/defcthesaurus/FindsPotteryDetail> ;
	skos:editorialNote "dc_finds_pottery_detail;02" ;
	skos:broader <https://acdh.oeaw.ac.at/vocabs/defcthesaurus/ring_handle/5.100> .

<https://acdh.oeaw.ac.at/vocabs/defcthesaurus/ring_handle/5.100> skos:narrower <https://acdh.oeaw.ac.at/vocabs/defcthesaurus/triangular_ring_handle/6.101> .

<https://acdh.oeaw.ac.at/vocabs/defcthesaurus/lug/5.040> a skos:Concept ;
	skos:prefLabel "lug"@en ;
	skos:inScheme <https://acdh.oeaw.ac.at/vocabs/defcthesaurus/FindsSchema> , <https://acdh.oeaw.ac.at/vocabs/defcthesaurus/NotInDatabase> ;
	skos:editorialNote "dc_not_in_database;040" ;
	skos:broader <https://acdh.oeaw.ac.at/vocabs/defcthesaurus/handle/4.031> .

<https://acdh.oeaw.ac.at/vocabs/defcthesaurus/handle/4.031> skos:narrower <https://acdh.oeaw.ac.at/vocabs/defcthesaurus/lug/5.040> .

<https://acdh.oeaw.ac.at/vocabs/defcthesaurus/finds_type/1.02> dc:source "Coleman 1977" .

<https://acdh.oeaw.ac.at/vocabs/defcthesaurus/elephant_lug/6.68> a skos:Concept ;
	skos:prefLabel "elephant lug"@en , "R체sselhenkel"@de ;
	skos:definition "A lug in a shape of an elephant쨈s head." ;
	skos:inScheme <https://acdh.oeaw.ac.at/vocabs/defcthesaurus/FindsSchema> , <https://acdh.oeaw.ac.at/vocabs/defcthesaurus/FindsPotteryDetail> ;
	skos:editorialNote "dc_finds_pottery_detail;02" ;
	skos:broader <https://acdh.oeaw.ac.at/vocabs/defcthesaurus/lug/5.040> .

<https://acdh.oeaw.ac.at/vocabs/defcthesaurus/lug/5.040> skos:narrower <https://acdh.oeaw.ac.at/vocabs/defcthesaurus/elephant_lug/6.68> .

<https://acdh.oeaw.ac.at/vocabs/defcthesaurus/ledge_lug/6.70> a skos:Concept ;
	skos:prefLabel "ledge lug"@en , "Leistengriff"@de ;
	skos:definition "Bar shaped handhold added to the wall of a pot to assist in holding it." ;
	skos:inScheme <https://acdh.oeaw.ac.at/vocabs/defcthesaurus/FindsSchema> , <https://acdh.oeaw.ac.at/vocabs/defcthesaurus/FindsPotteryDetail> ;
	skos:editorialNote "dc_finds_pottery_detail;02" ;
	skos:broader <https://acdh.oeaw.ac.at/vocabs/defcthesaurus/lug/5.040> .

<https://acdh.oeaw.ac.at/vocabs/defcthesaurus/lug/5.040> skos:narrower <https://acdh.oeaw.ac.at/vocabs/defcthesaurus/ledge_lug/6.70> .

<https://acdh.oeaw.ac.at/vocabs/defcthesaurus/finds_type/1.02> dc:source "Kipfer, B. A. Dictionary of Artifacts 2007. Blackwell Publishing, Oxford.p 184" .

<https://acdh.oeaw.ac.at/vocabs/defcthesaurus/stringhole_lug/6.79> a skos:Concept ;
	skos:prefLabel "stringhole lug"@en , "Schnur철se"@de ;
	skos:altLabel "preforated lug"@en ;
	skos:definition "An ear-shaped protuberance added to the wall of a pot to assist in hodling it. After attachment it was perforated. The hole was designed to take a cord or thong only and it was not a true handle." ;
	skos:inScheme <https://acdh.oeaw.ac.at/vocabs/defcthesaurus/FindsSchema> , <https://acdh.oeaw.ac.at/vocabs/defcthesaurus/FindsPotteryDetail> ;
	skos:editorialNote "dc_finds_pottery_detail;02" ;
	skos:broader <https://acdh.oeaw.ac.at/vocabs/defcthesaurus/lug/5.040> .

<https://acdh.oeaw.ac.at/vocabs/defcthesaurus/lug/5.040> skos:narrower <https://acdh.oeaw.ac.at/vocabs/defcthesaurus/stringhole_lug/6.79> .

<https://acdh.oeaw.ac.at/vocabs/defcthesaurus/tubular_lug/6.80> a skos:Concept ;
	skos:prefLabel "tubular lug"@en , "R철hren철se"@de ;
	skos:altLabel "tubular handle"@en , "Griffplatte"@de ;
	skos:definition "Tunnel shaped not preforated protuberance added to the wall of a pot to assist in hodling it." ;
	skos:inScheme <https://acdh.oeaw.ac.at/vocabs/defcthesaurus/FindsSchema> , <https://acdh.oeaw.ac.at/vocabs/defcthesaurus/FindsPotteryDetail> ;
	skos:editorialNote "dc_finds_pottery_detail;02" ;
	skos:broader <https://acdh.oeaw.ac.at/vocabs/defcthesaurus/lug/5.040> .

<https://acdh.oeaw.ac.at/vocabs/defcthesaurus/lug/5.040> skos:narrower <https://acdh.oeaw.ac.at/vocabs/defcthesaurus/tubular_lug/6.80> .

<https://acdh.oeaw.ac.at/vocabs/defcthesaurus/spout/4.88> a skos:Concept ;
	skos:prefLabel "spout"@en , "Ausguss"@de ;
	skos:definition "A tube or lip projecting from a vessel, through which liquid can be poured." ;
	skos:inScheme <https://acdh.oeaw.ac.at/vocabs/defcthesaurus/FindsSchema> , <https://acdh.oeaw.ac.at/vocabs/defcthesaurus/FindsPotteryDetail> ;
	skos:editorialNote "dc_finds_pottery_detail;88" ;
	skos:broader <https://acdh.oeaw.ac.at/vocabs/defcthesaurus/pottery_fragment/3.017> .

<https://acdh.oeaw.ac.at/vocabs/defcthesaurus/pottery_fragment/3.017> skos:narrower <https://acdh.oeaw.ac.at/vocabs/defcthesaurus/spout/4.88> .

<https://acdh.oeaw.ac.at/vocabs/defcthesaurus/bridge_spout/5.138> a skos:Concept ;
	skos:prefLabel "bridge spout"@en , "T체llenausguss"@de ;
	skos:definition "Nozzle shaped appendage that restricts a secondary orifice occuring to one side of a vessel쨈s vertical axis, and typically on the vessel쨈s upper body or shoulder." ;
	skos:inScheme <https://acdh.oeaw.ac.at/vocabs/defcthesaurus/FindsSchema> , <https://acdh.oeaw.ac.at/vocabs/defcthesaurus/FindsPotteryDetail> ;
	skos:editorialNote "dc_finds_pottery_detail;138" ;
	skos:broader <https://acdh.oeaw.ac.at/vocabs/defcthesaurus/spout/4.88> .

<https://acdh.oeaw.ac.at/vocabs/defcthesaurus/spout/4.88> skos:narrower <https://acdh.oeaw.ac.at/vocabs/defcthesaurus/bridge_spout/5.138> .

<https://acdh.oeaw.ac.at/vocabs/defcthesaurus/v-shaped_spout/5.126> a skos:Concept ;
	skos:prefLabel "v-shaped spout"@en , "V-f철rmiger Ausguss"@de ;
	skos:definition "A V-shaped tube or lip projecting from a vessel, through which liquid can be poured." ;
	skos:inScheme <https://acdh.oeaw.ac.at/vocabs/defcthesaurus/FindsSchema> , <https://acdh.oeaw.ac.at/vocabs/defcthesaurus/FindsPotteryDetail> ;
	skos:editorialNote "dc_finds_pottery_detail;126" ;
	skos:broader <https://acdh.oeaw.ac.at/vocabs/defcthesaurus/spout/4.88> .

<https://acdh.oeaw.ac.at/vocabs/defcthesaurus/spout/4.88> skos:narrower <https://acdh.oeaw.ac.at/vocabs/defcthesaurus/v-shaped_spout/5.126> .

<https://acdh.oeaw.ac.at/vocabs/defcthesaurus/base/4.032> a skos:Concept ;
	skos:prefLabel "base"@en ;
	skos:inScheme <https://acdh.oeaw.ac.at/vocabs/defcthesaurus/FindsSchema> , <https://acdh.oeaw.ac.at/vocabs/defcthesaurus/NotInDatabase> ;
	skos:editorialNote "dc_not_in_database;032" ;
	skos:broader <https://acdh.oeaw.ac.at/vocabs/defcthesaurus/pottery_fragment/3.017> .

<https://acdh.oeaw.ac.at/vocabs/defcthesaurus/pottery_fragment/3.017> skos:narrower <https://acdh.oeaw.ac.at/vocabs/defcthesaurus/base/4.032> .

<https://acdh.oeaw.ac.at/vocabs/defcthesaurus/concave_flat_base/5.139> a skos:Concept ;
	skos:prefLabel "concave flat base"@en , "Konkaver Flachboden"@de ;
	skos:definition "Flat lower portion of a vessel from the lower boudary of the body to the place that would normally be in contact with the surface on which the vessel rested in a concave/inverted shape." ;
	skos:inScheme <https://acdh.oeaw.ac.at/vocabs/defcthesaurus/FindsSchema> , <https://acdh.oeaw.ac.at/vocabs/defcthesaurus/FindsPotteryDetail> ;
	skos:editorialNote "dc_finds_pottery_detail;139" ;
	skos:broader <https://acdh.oeaw.ac.at/vocabs/defcthesaurus/base/4.032> .

<https://acdh.oeaw.ac.at/vocabs/defcthesaurus/base/4.032> skos:narrower <https://acdh.oeaw.ac.at/vocabs/defcthesaurus/concave_flat_base/5.139> .

<https://acdh.oeaw.ac.at/vocabs/defcthesaurus/flat_base/5.86> a skos:Concept ;
	skos:prefLabel "flat base"@en , "Flachboden"@de ;
	skos:definition "Flat lower portion of a vessel from the lower boudary of the body to the place that would normally be in contact with the surface on which the vessel rested." ;
	skos:inScheme <https://acdh.oeaw.ac.at/vocabs/defcthesaurus/FindsSchema> , <https://acdh.oeaw.ac.at/vocabs/defcthesaurus/FindsPotteryDetail> ;
	skos:editorialNote "dc_finds_pottery_detail;86" ;
	skos:broader <https://acdh.oeaw.ac.at/vocabs/defcthesaurus/base/4.032> .

<https://acdh.oeaw.ac.at/vocabs/defcthesaurus/base/4.032> skos:narrower <https://acdh.oeaw.ac.at/vocabs/defcthesaurus/flat_base/5.86> .

<https://acdh.oeaw.ac.at/vocabs/defcthesaurus/ring_base/5.180> a skos:Concept ;
	skos:prefLabel "ring base"@en , "Standring"@de ;
	skos:definition "A circular clay band encircling the bottom of the vessel and often occurred on wheelmade vessels. This base may also be elevated." ;
	skos:inScheme <https://acdh.oeaw.ac.at/vocabs/defcthesaurus/FindsSchema> , <https://acdh.oeaw.ac.at/vocabs/defcthesaurus/FindsPotteryDetail> ;
	skos:editorialNote "dc_finds_pottery_detail;180" ;
	skos:broader <https://acdh.oeaw.ac.at/vocabs/defcthesaurus/base/4.032> .

<https://acdh.oeaw.ac.at/vocabs/defcthesaurus/base/4.032> skos:narrower <https://acdh.oeaw.ac.at/vocabs/defcthesaurus/ring_base/5.180> .

<https://acdh.oeaw.ac.at/vocabs/defcthesaurus/rounded_base/5.165> a skos:Concept ;
	skos:prefLabel "rounded base"@en , "Runder Boden"@de ;
	skos:definition "A curved part of the vessel which provides support with a semicircular cross-section." ;
	skos:inScheme <https://acdh.oeaw.ac.at/vocabs/defcthesaurus/FindsSchema> , <https://acdh.oeaw.ac.at/vocabs/defcthesaurus/FindsPotteryDetail> ;
	skos:editorialNote "dc_finds_pottery_detail;165" ;
	skos:broader <https://acdh.oeaw.ac.at/vocabs/defcthesaurus/base/4.032> .

<https://acdh.oeaw.ac.at/vocabs/defcthesaurus/base/4.032> skos:narrower <https://acdh.oeaw.ac.at/vocabs/defcthesaurus/rounded_base/5.165> .

<https://acdh.oeaw.ac.at/vocabs/defcthesaurus/rim/4.033> a skos:Concept ;
	skos:prefLabel "rim"@en ;
	skos:inScheme <https://acdh.oeaw.ac.at/vocabs/defcthesaurus/FindsSchema> ;
	skos:broader <https://acdh.oeaw.ac.at/vocabs/defcthesaurus/pottery_fragment/3.017> .

<https://acdh.oeaw.ac.at/vocabs/defcthesaurus/curved_tapered-up_rim/5.140> a skos:Concept ;
	skos:prefLabel "curved tapered-up rim"@en , "Gew철lbter, sich verj체gender Rand"@de ;
	skos:definition "Curved and thinned portion of a vessel closest to its orifice." ;
	skos:inScheme <https://acdh.oeaw.ac.at/vocabs/defcthesaurus/FindsSchema> , <https://acdh.oeaw.ac.at/vocabs/defcthesaurus/FindsPotteryDetail> ;
	skos:editorialNote "dc_finds_pottery_detail;140" ;
	skos:broader <https://acdh.oeaw.ac.at/vocabs/defcthesaurus/rim/4.033> .

<https://acdh.oeaw.ac.at/vocabs/defcthesaurus/rim/4.033> skos:narrower <https://acdh.oeaw.ac.at/vocabs/defcthesaurus/curved_tapered-up_rim/5.140> .

<https://acdh.oeaw.ac.at/vocabs/defcthesaurus/pottery_fragment/3.017> skos:narrower <https://acdh.oeaw.ac.at/vocabs/defcthesaurus/rim/4.033> .

<https://acdh.oeaw.ac.at/vocabs/defcthesaurus/everted_rim/5.173> a skos:Concept ;
	skos:prefLabel "everted rim"@en , "Ungest체lpter Rand"@de ;
	skos:definition "A rim that turns sharply outwards and upwards from the shoulder of the vessel." ;
	skos:inScheme <https://acdh.oeaw.ac.at/vocabs/defcthesaurus/FindsSchema> , <https://acdh.oeaw.ac.at/vocabs/defcthesaurus/FindsPotteryDetail> ;
	skos:editorialNote "dc_finds_pottery_detail;173" ;
	skos:broader <https://acdh.oeaw.ac.at/vocabs/defcthesaurus/rim/4.033> .

<https://acdh.oeaw.ac.at/vocabs/defcthesaurus/rim/4.033> skos:narrower <https://acdh.oeaw.ac.at/vocabs/defcthesaurus/everted_rim/5.173> .

<https://acdh.oeaw.ac.at/vocabs/defcthesaurus/flaring_rim/5.69> a skos:Concept ;
	skos:prefLabel "flaring rim"@en , "Ausladender Rand"@de ;
	skos:definition "Curved rim with outcurving inflections outside the vessel." ;
	skos:inScheme <https://acdh.oeaw.ac.at/vocabs/defcthesaurus/FindsSchema> , <https://acdh.oeaw.ac.at/vocabs/defcthesaurus/FindsPotteryDetail> ;
	skos:editorialNote "dc_finds_pottery_detail;69" ;
	skos:broader <https://acdh.oeaw.ac.at/vocabs/defcthesaurus/rim/4.033> .

<https://acdh.oeaw.ac.at/vocabs/defcthesaurus/rim/4.033> skos:narrower <https://acdh.oeaw.ac.at/vocabs/defcthesaurus/flaring_rim/5.69> .

<https://acdh.oeaw.ac.at/vocabs/defcthesaurus/flat-topped_rim/5.158> a skos:Concept ;
	skos:prefLabel "flat-topped rim"@en , "Flachrand"@de ;
	skos:definition "Horizontally flattened upper portion of a vessel." ;
	skos:inScheme <https://acdh.oeaw.ac.at/vocabs/defcthesaurus/FindsSchema> , <https://acdh.oeaw.ac.at/vocabs/defcthesaurus/FindsPotteryDetail> ;
	skos:editorialNote "dc_finds_pottery_detail;158" ;
	skos:broader <https://acdh.oeaw.ac.at/vocabs/defcthesaurus/rim/4.033> .

<https://acdh.oeaw.ac.at/vocabs/defcthesaurus/rim/4.033> skos:narrower <https://acdh.oeaw.ac.at/vocabs/defcthesaurus/flat-topped_rim/5.158> .

<https://acdh.oeaw.ac.at/vocabs/defcthesaurus/inside_bevelled_and_decorated_rim/5.73> a skos:Concept ;
	skos:prefLabel "inside bevelled and decorated rim"@en , "Innen abgestrichener Rand mit Verzierung"@de ;
	skos:definition "Uppoer part of the vessel with thickened inner side of lip, forming flat or slightly convex band, fairly sharply offset so that it ends with an angular or somewhat rounded inner edge." ;
	skos:inScheme <https://acdh.oeaw.ac.at/vocabs/defcthesaurus/FindsSchema> , <https://acdh.oeaw.ac.at/vocabs/defcthesaurus/FindsPotteryDetail> ;
	skos:editorialNote "dc_finds_pottery_detail;73" ;
	skos:broader <https://acdh.oeaw.ac.at/vocabs/defcthesaurus/rim/4.033> .

<https://acdh.oeaw.ac.at/vocabs/defcthesaurus/rim/4.033> skos:narrower <https://acdh.oeaw.ac.at/vocabs/defcthesaurus/inside_bevelled_and_decorated_rim/5.73> .

<https://acdh.oeaw.ac.at/vocabs/defcthesaurus/tapered-up_rim/5.157> a skos:Concept ;
	skos:prefLabel "tapered-up rim"@en , "Verj체ngender Rand"@de ;
	skos:definition "The upper portion of the vessel closest to its orifice that has been thinned." ;
	skos:inScheme <https://acdh.oeaw.ac.at/vocabs/defcthesaurus/FindsSchema> , <https://acdh.oeaw.ac.at/vocabs/defcthesaurus/FindsPotteryDetail> ;
	skos:editorialNote "dc_finds_pottery_detail;157" ;
	skos:broader <https://acdh.oeaw.ac.at/vocabs/defcthesaurus/rim/4.033> .

<https://acdh.oeaw.ac.at/vocabs/defcthesaurus/rim/4.033> skos:narrower <https://acdh.oeaw.ac.at/vocabs/defcthesaurus/tapered-up_rim/5.157> .

<https://acdh.oeaw.ac.at/vocabs/defcthesaurus/thickened_rim/5.166> a skos:Concept ;
	skos:prefLabel "thickened rim"@en , "Verdickter Rand"@de ;
	skos:definition "The upper portion of the vessel closest to its orifice that has been thickened." ;
	skos:inScheme <https://acdh.oeaw.ac.at/vocabs/defcthesaurus/FindsSchema> , <https://acdh.oeaw.ac.at/vocabs/defcthesaurus/FindsPotteryDetail> ;
	skos:editorialNote "dc_finds_pottery_detail;166" ;
	skos:broader <https://acdh.oeaw.ac.at/vocabs/defcthesaurus/rim/4.033> .

<https://acdh.oeaw.ac.at/vocabs/defcthesaurus/rim/4.033> skos:narrower <https://acdh.oeaw.ac.at/vocabs/defcthesaurus/thickened_rim/5.166> .

<https://acdh.oeaw.ac.at/vocabs/defcthesaurus/offset_rim/5.163> a skos:Concept ;
	skos:prefLabel "offset rim"@en , "Abgesetzter Rand"@de ;
	skos:definition "Offset rims are either in-set or out-set from the vessel wall, resulting in either an inverted or everted rim profile." ;
	skos:inScheme <https://acdh.oeaw.ac.at/vocabs/defcthesaurus/FindsSchema> , <https://acdh.oeaw.ac.at/vocabs/defcthesaurus/FindsPotteryDetail> ;
	skos:editorialNote "dc_finds_pottery_detail;163" ;
	skos:broader <https://acdh.oeaw.ac.at/vocabs/defcthesaurus/rim/4.033> .

<https://acdh.oeaw.ac.at/vocabs/defcthesaurus/rim/4.033> skos:narrower <https://acdh.oeaw.ac.at/vocabs/defcthesaurus/offset_rim/5.163> .

<https://acdh.oeaw.ac.at/vocabs/defcthesaurus/rolled_rim/5.77> a skos:Concept ;
	skos:prefLabel "rolled rim"@en , "eingerollter Rand"@de ;
	skos:definition "Inwards thickened rim with round cross section." ;
	skos:inScheme <https://acdh.oeaw.ac.at/vocabs/defcthesaurus/FindsSchema> , <https://acdh.oeaw.ac.at/vocabs/defcthesaurus/FindsPotteryDetail> ;
	skos:editorialNote "dc_finds_pottery_detail;77" ;
	skos:broader <https://acdh.oeaw.ac.at/vocabs/defcthesaurus/rim/4.033> .

<https://acdh.oeaw.ac.at/vocabs/defcthesaurus/rim/4.033> skos:narrower <https://acdh.oeaw.ac.at/vocabs/defcthesaurus/rolled_rim/5.77> .

<https://acdh.oeaw.ac.at/vocabs/defcthesaurus/foot/4.71> a skos:Concept ;
	skos:prefLabel "foot"@en , "Bein"@de ;
	skos:altLabel "Leg"@en , "Fu"@de ;
	skos:definition "Supporting lower part of the vessel such as a tripod, normally attached to the base or vessel bottom after the vessel has got its form." ;
	skos:inScheme <https://acdh.oeaw.ac.at/vocabs/defcthesaurus/FindsSchema> , <https://acdh.oeaw.ac.at/vocabs/defcthesaurus/FindsPotteryDetail> ;
	skos:editorialNote "dc_finds_pottery_detail;71" ;
	skos:broader <https://acdh.oeaw.ac.at/vocabs/defcthesaurus/pottery_fragment/3.017> .

<https://acdh.oeaw.ac.at/vocabs/defcthesaurus/pottery_fragment/3.017> skos:narrower <https://acdh.oeaw.ac.at/vocabs/defcthesaurus/foot/4.71> .

<https://acdh.oeaw.ac.at/vocabs/defcthesaurus/fenestrated_pedestal/5.160> a skos:Concept ;
	skos:prefLabel "fenestrated pedestal"@en , "Durchbrochener Sockel"@de ;
	skos:altLabel "Durchbrochener Fu"@de , "Standfu"@de ;
	skos:definition "A free-standing raised vessel bottom with openings in its walls." ;
	skos:inScheme <https://acdh.oeaw.ac.at/vocabs/defcthesaurus/FindsSchema> , <https://acdh.oeaw.ac.at/vocabs/defcthesaurus/FindsPotteryDetail> ;
	skos:editorialNote "dc_finds_pottery_detail;160" ;
	skos:broader <https://acdh.oeaw.ac.at/vocabs/defcthesaurus/foot/4.71> .

<https://acdh.oeaw.ac.at/vocabs/defcthesaurus/foot/4.71> skos:narrower <https://acdh.oeaw.ac.at/vocabs/defcthesaurus/fenestrated_pedestal/5.160> .

<https://acdh.oeaw.ac.at/vocabs/defcthesaurus/pedestal_base/5.76> a skos:Concept ;
	skos:prefLabel "pedestal base"@en , "Standfu"@de ;
	skos:altLabel "Pedestal"@en , "Sockel"@de ;
	skos:inScheme <https://acdh.oeaw.ac.at/vocabs/defcthesaurus/FindsSchema> , <https://acdh.oeaw.ac.at/vocabs/defcthesaurus/FindsPotteryDetail> ;
	skos:editorialNote "dc_finds_pottery_detail;76" ;
	skos:broader <https://acdh.oeaw.ac.at/vocabs/defcthesaurus/foot/4.71> .

<https://acdh.oeaw.ac.at/vocabs/defcthesaurus/foot/4.71> skos:narrower <https://acdh.oeaw.ac.at/vocabs/defcthesaurus/pedestal_base/5.76> .

<https://acdh.oeaw.ac.at/vocabs/defcthesaurus/pedestal/5.164> a skos:Concept ;
	skos:prefLabel "pedestal"@en , "Sockel"@de ;
	skos:inScheme <https://acdh.oeaw.ac.at/vocabs/defcthesaurus/FindsSchema> , <https://acdh.oeaw.ac.at/vocabs/defcthesaurus/FindsPotteryDetail> ;
	skos:editorialNote "dc_finds_pottery_detail;164" ;
	skos:broader <https://acdh.oeaw.ac.at/vocabs/defcthesaurus/foot/4.71> .

<https://acdh.oeaw.ac.at/vocabs/defcthesaurus/foot/4.71> skos:narrower <https://acdh.oeaw.ac.at/vocabs/defcthesaurus/pedestal/5.164> .

<https://acdh.oeaw.ac.at/vocabs/defcthesaurus/pedestal/5.137> a skos:Concept ;
	skos:prefLabel "pedestal"@en , "Sockel"@de ;
	skos:inScheme <https://acdh.oeaw.ac.at/vocabs/defcthesaurus/FindsSchema> , <https://acdh.oeaw.ac.at/vocabs/defcthesaurus/FindsPotteryDetail> ;
	skos:editorialNote "dc_finds_pottery_detail;137" ;
	skos:broader <https://acdh.oeaw.ac.at/vocabs/defcthesaurus/foot/4.71> .

<https://acdh.oeaw.ac.at/vocabs/defcthesaurus/foot/4.71> skos:narrower <https://acdh.oeaw.ac.at/vocabs/defcthesaurus/pedestal/5.137> .

<https://acdh.oeaw.ac.at/vocabs/defcthesaurus/small_foot/5.167> a skos:Concept ;
	skos:prefLabel "small foot"@en , "Kleiner Fu"@de ;
	skos:definition "A small supporting lower part of the vessel, normally attached to the base or vessel bottom after the vessel has got its form." ;
	skos:inScheme <https://acdh.oeaw.ac.at/vocabs/defcthesaurus/FindsSchema> , <https://acdh.oeaw.ac.at/vocabs/defcthesaurus/FindsPotteryDetail> ;
	skos:editorialNote "dc_finds_pottery_detail;167" ;
	skos:broader <https://acdh.oeaw.ac.at/vocabs/defcthesaurus/foot/4.71> .

<https://acdh.oeaw.ac.at/vocabs/defcthesaurus/foot/4.71> skos:narrower <https://acdh.oeaw.ac.at/vocabs/defcthesaurus/small_foot/5.167> .

<https://acdh.oeaw.ac.at/vocabs/defcthesaurus/attachment/4.034> a skos:Concept ;
	skos:prefLabel "attachment"@en ;
	skos:inScheme <https://acdh.oeaw.ac.at/vocabs/defcthesaurus/FindsSchema> , <https://acdh.oeaw.ac.at/vocabs/defcthesaurus/NotInDatabase> ;
	skos:editorialNote "dc_not_in_database;034" ;
	skos:broader <https://acdh.oeaw.ac.at/vocabs/defcthesaurus/pottery_fragment/3.017> .

<https://acdh.oeaw.ac.at/vocabs/defcthesaurus/pottery_fragment/3.017> skos:narrower <https://acdh.oeaw.ac.at/vocabs/defcthesaurus/attachment/4.034> .

<https://acdh.oeaw.ac.at/vocabs/defcthesaurus/knob/5.74> a skos:Concept ;
	skos:prefLabel "knob"@en , "Knubbe"@de ;
	skos:definition "Round application with a semicircular cross section." ;
	skos:inScheme <https://acdh.oeaw.ac.at/vocabs/defcthesaurus/FindsSchema> , <https://acdh.oeaw.ac.at/vocabs/defcthesaurus/FindsPotteryDetail> ;
	skos:editorialNote "dc_finds_pottery_detail;74" ;
	skos:broader <https://acdh.oeaw.ac.at/vocabs/defcthesaurus/attachment/4.034> .

<https://acdh.oeaw.ac.at/vocabs/defcthesaurus/attachment/4.034> skos:narrower <https://acdh.oeaw.ac.at/vocabs/defcthesaurus/knob/5.74> .

<https://acdh.oeaw.ac.at/vocabs/defcthesaurus/knob-row/5.99> a skos:Concept ;
	skos:prefLabel "knob-row"@en , "Vertikale Knubbenreihe"@de ;
	skos:altLabel "knob row"@en ;
	skos:definition "Vertically applied series of round clay objects." ;
	skos:inScheme <https://acdh.oeaw.ac.at/vocabs/defcthesaurus/FindsSchema> , <https://acdh.oeaw.ac.at/vocabs/defcthesaurus/FindsPotteryDetail> ;
	skos:editorialNote "dc_finds_pottery_detail;99" ;
	skos:broader <https://acdh.oeaw.ac.at/vocabs/defcthesaurus/attachment/4.034> .

<https://acdh.oeaw.ac.at/vocabs/defcthesaurus/attachment/4.034> skos:narrower <https://acdh.oeaw.ac.at/vocabs/defcthesaurus/knob-row/5.99> .

<https://acdh.oeaw.ac.at/vocabs/defcthesaurus/rim_attachment/5.94> a skos:Concept ;
	skos:prefLabel "rim attachment"@en , "Randaufsatz"@de ;
	skos:definition "An add-on made of clay attached to the upper part of a vessel between the lip or margin and the side wall or neck of a vessel." ;
	skos:inScheme <https://acdh.oeaw.ac.at/vocabs/defcthesaurus/FindsSchema> , <https://acdh.oeaw.ac.at/vocabs/defcthesaurus/FindsPotteryDetail> ;
	skos:editorialNote "dc_finds_pottery_detail;94" ;
	skos:broader <https://acdh.oeaw.ac.at/vocabs/defcthesaurus/attachment/4.034> .

<https://acdh.oeaw.ac.at/vocabs/defcthesaurus/attachment/4.034> skos:narrower <https://acdh.oeaw.ac.at/vocabs/defcthesaurus/rim_attachment/5.94> .

<https://acdh.oeaw.ac.at/vocabs/defcthesaurus/zoomorphic_handle_attachment/5.81> a skos:Concept ;
	skos:prefLabel "zoomorphic handle attachment"@en , "Zoomorpher Griffaufsatz"@de ;
	skos:altLabel "Tierkopfgriff"@de ;
	skos:definition "A handhold in a shape of an animal." ;
	skos:inScheme <https://acdh.oeaw.ac.at/vocabs/defcthesaurus/FindsSchema> , <https://acdh.oeaw.ac.at/vocabs/defcthesaurus/FindsPotteryDetail> ;
	skos:editorialNote "dc_finds_pottery_detail;81" ;
	skos:broader <https://acdh.oeaw.ac.at/vocabs/defcthesaurus/attachment/4.034> .

<https://acdh.oeaw.ac.at/vocabs/defcthesaurus/attachment/4.034> skos:narrower <https://acdh.oeaw.ac.at/vocabs/defcthesaurus/zoomorphic_handle_attachment/5.81> .

<https://acdh.oeaw.ac.at/vocabs/defcthesaurus/pottery_decoration/3.018> a skos:Concept ;
	skos:prefLabel "pottery decoration"@en , "Keramikdekor"@de ;
	skos:inScheme <https://acdh.oeaw.ac.at/vocabs/defcthesaurus/FindsSchema> , <https://acdh.oeaw.ac.at/vocabs/defcthesaurus/NotInDatabase> ;
	skos:editorialNote "dc_not_in_database;018" ;
	skos:broader <https://acdh.oeaw.ac.at/vocabs/defcthesaurus/pottery/2.4> .

<https://acdh.oeaw.ac.at/vocabs/defcthesaurus/pottery/2.4> skos:narrower <https://acdh.oeaw.ac.at/vocabs/defcthesaurus/pottery_decoration/3.018> .

<https://acdh.oeaw.ac.at/vocabs/defcthesaurus/FindsPotteryDecoration> a skos:ConceptScheme ;
	rdfs:comment "A concept schema related to the particular finds properties." .

<https://acdh.oeaw.ac.at/vocabs/defcthesaurus/plastic_decoration/4.132> a skos:Concept ;
	skos:prefLabel "plastic decoration"@en , "Plastischer Dekor"@de ;
	skos:definition "Pottery with applied material on its surface such as clay or bead." ;
	skos:inScheme <https://acdh.oeaw.ac.at/vocabs/defcthesaurus/FindsSchema> , <https://acdh.oeaw.ac.at/vocabs/defcthesaurus/FindsPotteryDecoration> ;
	skos:editorialNote "dc_finds_pottery_decoration;132" ;
	skos:broader <https://acdh.oeaw.ac.at/vocabs/defcthesaurus/pottery_decoration/3.018> .

<https://acdh.oeaw.ac.at/vocabs/defcthesaurus/pottery_decoration/3.018> skos:narrower <https://acdh.oeaw.ac.at/vocabs/defcthesaurus/plastic_decoration/4.132> .

<https://acdh.oeaw.ac.at/vocabs/defcthesaurus/applied_disc/5.211> a skos:Concept ;
	skos:prefLabel "applied disc"@en , "Angesetzte Scheiben"@de ;
	skos:definition "Pottery decorated with a disc shaped application." ;
	skos:inScheme <https://acdh.oeaw.ac.at/vocabs/defcthesaurus/FindsSchema> , <https://acdh.oeaw.ac.at/vocabs/defcthesaurus/FindsPotteryDecoration> ;
	skos:editorialNote "dc_finds_pottery_decoration;211" ;
	skos:broader <https://acdh.oeaw.ac.at/vocabs/defcthesaurus/plastic_decoration/4.132> .

<https://acdh.oeaw.ac.at/vocabs/defcthesaurus/plastic_decoration/4.132> skos:narrower <https://acdh.oeaw.ac.at/vocabs/defcthesaurus/applied_disc/5.211> .

<https://acdh.oeaw.ac.at/vocabs/defcthesaurus/barbotine/5.240> a skos:Concept ;
	skos:prefLabel "barbotine"@en , "Barbotineverziert"@de ;
	skos:altLabel "slip trailing"@en , "Eingobenmalerei"@de ;
	skos:definition "Pottery decorated with a rather thick slip is used for decorating vessels." ;
	skos:inScheme <https://acdh.oeaw.ac.at/vocabs/defcthesaurus/FindsSchema> , <https://acdh.oeaw.ac.at/vocabs/defcthesaurus/FindsPotteryDecoration> ;
	skos:editorialNote "dc_finds_pottery_decoration;240" ;
	skos:broader <https://acdh.oeaw.ac.at/vocabs/defcthesaurus/plastic_decoration/4.132> .

<https://acdh.oeaw.ac.at/vocabs/defcthesaurus/plastic_decoration/4.132> skos:narrower <https://acdh.oeaw.ac.at/vocabs/defcthesaurus/barbotine/5.240> .

<https://acdh.oeaw.ac.at/vocabs/defcthesaurus/bead_inlay/5.118> a skos:Concept ;
	skos:prefLabel "bead inlay"@en , "Perleneinlage"@de ;
	skos:definition "Pellet inlay typical for Crete." ;
	skos:inScheme <https://acdh.oeaw.ac.at/vocabs/defcthesaurus/FindsSchema> , <https://acdh.oeaw.ac.at/vocabs/defcthesaurus/FindsPotteryDecoration> ;
	skos:editorialNote "dc_finds_pottery_decoration;118" ;
	skos:broader <https://acdh.oeaw.ac.at/vocabs/defcthesaurus/plastic_decoration/4.132> .

<https://acdh.oeaw.ac.at/vocabs/defcthesaurus/plastic_decoration/4.132> skos:narrower <https://acdh.oeaw.ac.at/vocabs/defcthesaurus/bead_inlay/5.118> .

<https://acdh.oeaw.ac.at/vocabs/defcthesaurus/granulata_ware/5.216> a skos:Concept ;
	skos:prefLabel "granulata ware"@en , "Granulatdekor"@de ;
	skos:altLabel "pellet decoration"@en ;
	skos:definition "Pottery covered with a coating of stones and then slipped with paint." ;
	skos:inScheme <https://acdh.oeaw.ac.at/vocabs/defcthesaurus/FindsSchema> , <https://acdh.oeaw.ac.at/vocabs/defcthesaurus/FindsPotteryDecoration> ;
	skos:editorialNote "dc_finds_pottery_decoration;216" ;
	skos:broader <https://acdh.oeaw.ac.at/vocabs/defcthesaurus/plastic_decoration/4.132> .

<https://acdh.oeaw.ac.at/vocabs/defcthesaurus/plastic_decoration/4.132> skos:narrower <https://acdh.oeaw.ac.at/vocabs/defcthesaurus/granulata_ware/5.216> .

<https://acdh.oeaw.ac.at/vocabs/defcthesaurus/plastic_cordon_decoration/5.225> a skos:Concept ;
	skos:prefLabel "plastic cordon decoration"@en , "Plastischer Banddekor"@de ;
	skos:definition "Pottery with a strip of clay added around the outside surface of a pot before firing for decoration or handling. The cordon(s) may be decorated in some way, for example with fingertip or stick impressions." ;
	skos:inScheme <https://acdh.oeaw.ac.at/vocabs/defcthesaurus/FindsSchema> , <https://acdh.oeaw.ac.at/vocabs/defcthesaurus/FindsPotteryDecoration> ;
	skos:editorialNote "dc_finds_pottery_decoration;225" ;
	skos:broader <https://acdh.oeaw.ac.at/vocabs/defcthesaurus/plastic_decoration/4.132> .

<https://acdh.oeaw.ac.at/vocabs/defcthesaurus/plastic_decoration/4.132> skos:narrower <https://acdh.oeaw.ac.at/vocabs/defcthesaurus/plastic_cordon_decoration/5.225> .

<https://acdh.oeaw.ac.at/vocabs/defcthesaurus/pointill챕_decoration/5.227> a skos:Concept ;
	skos:prefLabel "pointill챕 decoration"@en , "Pointill챕 Dekor"@de ;
	skos:definition "Pottery decoration by marking with dots." ;
	skos:inScheme <https://acdh.oeaw.ac.at/vocabs/defcthesaurus/FindsSchema> , <https://acdh.oeaw.ac.at/vocabs/defcthesaurus/FindsPotteryDecoration> ;
	skos:editorialNote "dc_finds_pottery_decoration;227" ;
	skos:broader <https://acdh.oeaw.ac.at/vocabs/defcthesaurus/plastic_decoration/4.132> .

<https://acdh.oeaw.ac.at/vocabs/defcthesaurus/plastic_decoration/4.132> skos:narrower <https://acdh.oeaw.ac.at/vocabs/defcthesaurus/pointill챕_decoration/5.227> .

<https://acdh.oeaw.ac.at/vocabs/defcthesaurus/incised/4.168> a skos:Concept ;
	skos:prefLabel "incised"@en , "Ritzverziert"@de ;
	skos:definition "Pottery decorated by cuts into the surface." ;
	skos:inScheme <https://acdh.oeaw.ac.at/vocabs/defcthesaurus/FindsSchema> , <https://acdh.oeaw.ac.at/vocabs/defcthesaurus/FindsPotteryDecoration> ;
	skos:editorialNote "dc_finds_pottery_decoration;168" ;
	skos:broader <https://acdh.oeaw.ac.at/vocabs/defcthesaurus/pottery_decoration/3.018> .

<https://acdh.oeaw.ac.at/vocabs/defcthesaurus/pottery_decoration/3.018> skos:narrower <https://acdh.oeaw.ac.at/vocabs/defcthesaurus/incised/4.168> .

<https://acdh.oeaw.ac.at/vocabs/defcthesaurus/coarse_urfirnis/5.164> a skos:Concept ;
	skos:prefLabel "coarse urfirnis"@en , "Grober Urfirnis"@de ;
	skos:definition "Coarse pottery decorated with a glaze-like paint." ;
	skos:inScheme <https://acdh.oeaw.ac.at/vocabs/defcthesaurus/FindsSchema> , <https://acdh.oeaw.ac.at/vocabs/defcthesaurus/FindsPotteryDecoration> ;
	skos:editorialNote "dc_finds_pottery_decoration;164" ;
	skos:broader <https://acdh.oeaw.ac.at/vocabs/defcthesaurus/incised/4.168> .

<https://acdh.oeaw.ac.at/vocabs/defcthesaurus/incised/4.168> skos:narrower <https://acdh.oeaw.ac.at/vocabs/defcthesaurus/coarse_urfirnis/5.164> .

<https://acdh.oeaw.ac.at/vocabs/defcthesaurus/excised/5.191> a skos:Concept ;
	skos:prefLabel "excised"@en , "Ware mit ausgeschnittenem Dekor"@de ;
	skos:definition "Pottery decoration produced by cutting strips or shapes out of the soft clay surface before firing." ;
	skos:inScheme <https://acdh.oeaw.ac.at/vocabs/defcthesaurus/FindsSchema> , <https://acdh.oeaw.ac.at/vocabs/defcthesaurus/FindsPotteryDecoration> ;
	skos:editorialNote "dc_finds_pottery_decoration;191" ;
	skos:broader <https://acdh.oeaw.ac.at/vocabs/defcthesaurus/incised/4.168> .

<https://acdh.oeaw.ac.at/vocabs/defcthesaurus/incised/4.168> skos:narrower <https://acdh.oeaw.ac.at/vocabs/defcthesaurus/excised/5.191> .

<https://acdh.oeaw.ac.at/vocabs/defcthesaurus/excised-with-graphite/5.192> a skos:Concept ;
	skos:prefLabel "excised-with-graphite"@en , "Ware mit ausgeschnittenem Dekor und Graphitbemalung"@de ;
	skos:altLabel "excised with graphite"@en ;
	skos:definition "Pottery decoration produced by cutting strips or shapes out of the soft clay surface before firing and painted with graphite paint." ;
	skos:inScheme <https://acdh.oeaw.ac.at/vocabs/defcthesaurus/FindsSchema> , <https://acdh.oeaw.ac.at/vocabs/defcthesaurus/FindsPotteryDecoration> ;
	skos:editorialNote "dc_finds_pottery_decoration;192" ;
	skos:broader <https://acdh.oeaw.ac.at/vocabs/defcthesaurus/incised/4.168> .

<https://acdh.oeaw.ac.at/vocabs/defcthesaurus/incised/4.168> skos:narrower <https://acdh.oeaw.ac.at/vocabs/defcthesaurus/excised-with-graphite/5.192> .

<https://acdh.oeaw.ac.at/vocabs/defcthesaurus/figure_relief_decoration/5.133> a skos:Concept ;
	skos:prefLabel "figure relief decoration"@en , "Fig체rlicher Reliefdekor"@de ;
	skos:definition "Pottery from which the decoration figure projects from the vessel by carving out the background." ;
	skos:inScheme <https://acdh.oeaw.ac.at/vocabs/defcthesaurus/FindsSchema> , <https://acdh.oeaw.ac.at/vocabs/defcthesaurus/FindsPotteryDecoration> ;
	skos:editorialNote "dc_finds_pottery_decoration;133" ;
	skos:broader <https://acdh.oeaw.ac.at/vocabs/defcthesaurus/incised/4.168> .

<https://acdh.oeaw.ac.at/vocabs/defcthesaurus/incised/4.168> skos:narrower <https://acdh.oeaw.ac.at/vocabs/defcthesaurus/figure_relief_decoration/5.133> .

<https://acdh.oeaw.ac.at/vocabs/defcthesaurus/grooved/5.123> a skos:Concept ;
	skos:prefLabel "grooved"@en , "Kanneliert"@de ;
	skos:altLabel "channeled"@en , "fluted"@en , "Kannelur"@de , "gerillt"@de ;
	skos:definition "Pottery decoration in which broad lines are drawn on the firm but unbaked pot surface. No clay is removed, as it is in excised decoration, nor is the surface itself broken, as with incised decoration." ;
	skos:inScheme <https://acdh.oeaw.ac.at/vocabs/defcthesaurus/FindsSchema> , <https://acdh.oeaw.ac.at/vocabs/defcthesaurus/FindsPotteryDecoration> ;
	skos:editorialNote "dc_finds_pottery_decoration;123" ;
	skos:broader <https://acdh.oeaw.ac.at/vocabs/defcthesaurus/incised/4.168> .

<https://acdh.oeaw.ac.at/vocabs/defcthesaurus/incised/4.168> skos:narrower <https://acdh.oeaw.ac.at/vocabs/defcthesaurus/grooved/5.123> .

<https://acdh.oeaw.ac.at/vocabs/defcthesaurus/grooved_with_graphite/5.197> a skos:Concept ;
	skos:prefLabel "grooved with graphite"@en , "Kanneliert, mit Graphitbemalung"@de ;
	skos:definition "Pottery decoration in which broad lines are drawn on the firm but unbaked pot surface and painted graphite paint." ;
	skos:inScheme <https://acdh.oeaw.ac.at/vocabs/defcthesaurus/FindsSchema> , <https://acdh.oeaw.ac.at/vocabs/defcthesaurus/FindsPotteryDecoration> ;
	skos:editorialNote "dc_finds_pottery_decoration;197" ;
	skos:broader <https://acdh.oeaw.ac.at/vocabs/defcthesaurus/incised/4.168> .

<https://acdh.oeaw.ac.at/vocabs/defcthesaurus/incised/4.168> skos:narrower <https://acdh.oeaw.ac.at/vocabs/defcthesaurus/grooved_with_graphite/5.197> .

<https://acdh.oeaw.ac.at/vocabs/defcthesaurus/impresso/5.126> a skos:Concept ;
	skos:prefLabel "impresso"@en , "Impresso"@de ;
	skos:definition "Pottery decorated by imprinting of the clay with different types of objects." ;
	skos:inScheme <https://acdh.oeaw.ac.at/vocabs/defcthesaurus/FindsSchema> , <https://acdh.oeaw.ac.at/vocabs/defcthesaurus/FindsPotteryDecoration> ;
	skos:editorialNote "dc_finds_pottery_decoration;126" ;
	skos:broader <https://acdh.oeaw.ac.at/vocabs/defcthesaurus/incised/4.168> .

<https://acdh.oeaw.ac.at/vocabs/defcthesaurus/incised/4.168> skos:narrower <https://acdh.oeaw.ac.at/vocabs/defcthesaurus/impresso/5.126> .

<https://acdh.oeaw.ac.at/vocabs/defcthesaurus/impresso_(a2)/5.151> a skos:Concept ;
	skos:prefLabel "impresso (a2)"@en , "Impresso (A2)"@de ;
	skos:definition "Pottery decorated by imprinting of the clay with different types of objects." ;
	skos:inScheme <https://acdh.oeaw.ac.at/vocabs/defcthesaurus/FindsSchema> , <https://acdh.oeaw.ac.at/vocabs/defcthesaurus/FindsPotteryDecoration> ;
	skos:editorialNote "dc_finds_pottery_decoration;151" ;
	skos:broader <https://acdh.oeaw.ac.at/vocabs/defcthesaurus/incised/4.168> .

<https://acdh.oeaw.ac.at/vocabs/defcthesaurus/incised/4.168> skos:narrower <https://acdh.oeaw.ac.at/vocabs/defcthesaurus/impresso_(a2)/5.151> .

<https://acdh.oeaw.ac.at/vocabs/defcthesaurus/incised_(款2)/5.153> a skos:Concept ;
	skos:prefLabel "incised (款2)"@en , "Ritzverziert (C2)"@de ;
	skos:definition "Pottery decorated by cuts into the surface." ;
	skos:inScheme <https://acdh.oeaw.ac.at/vocabs/defcthesaurus/FindsSchema> , <https://acdh.oeaw.ac.at/vocabs/defcthesaurus/FindsPotteryDecoration> ;
	skos:editorialNote "dc_finds_pottery_decoration;153" ;
	skos:broader <https://acdh.oeaw.ac.at/vocabs/defcthesaurus/incised/4.168> .

<https://acdh.oeaw.ac.at/vocabs/defcthesaurus/incised/4.168> skos:narrower <https://acdh.oeaw.ac.at/vocabs/defcthesaurus/incised_(款2)/5.153> .

<https://acdh.oeaw.ac.at/vocabs/defcthesaurus/incised_(b2)/5.152> a skos:Concept ;
	skos:prefLabel "incised (b2)"@en , "Ritzverziert (B2)"@de ;
	skos:definition "Pottery decorated by cuts into the surface." ;
	skos:inScheme <https://acdh.oeaw.ac.at/vocabs/defcthesaurus/FindsSchema> , <https://acdh.oeaw.ac.at/vocabs/defcthesaurus/FindsPotteryDecoration> ;
	skos:editorialNote "dc_finds_pottery_decoration;152" ;
	skos:broader <https://acdh.oeaw.ac.at/vocabs/defcthesaurus/incised/4.168> .

<https://acdh.oeaw.ac.at/vocabs/defcthesaurus/incised/4.168> skos:narrower <https://acdh.oeaw.ac.at/vocabs/defcthesaurus/incised_(b2)/5.152> .

<https://acdh.oeaw.ac.at/vocabs/defcthesaurus/incised-pointill챕_decoration/5.127> a skos:Concept ;
	skos:prefLabel "incised-pointill챕 decoration"@en , "Ritzverzierter-Pointill챕 Dekor"@de ;
	skos:definition "Pottery decoration by cuting dots in the surface." ;
	skos:inScheme <https://acdh.oeaw.ac.at/vocabs/defcthesaurus/FindsSchema> , <https://acdh.oeaw.ac.at/vocabs/defcthesaurus/FindsPotteryDecoration> ;
	skos:editorialNote "dc_finds_pottery_decoration;127" ;
	skos:broader <https://acdh.oeaw.ac.at/vocabs/defcthesaurus/incised/4.168> .

<https://acdh.oeaw.ac.at/vocabs/defcthesaurus/incised/4.168> skos:narrower <https://acdh.oeaw.ac.at/vocabs/defcthesaurus/incised-pointill챕_decoration/5.127> .

<https://acdh.oeaw.ac.at/vocabs/defcthesaurus/incrusted/5.122> a skos:Concept ;
	skos:prefLabel "incrusted"@en , "Inkrustiert"@de ;
	skos:definition "Pottery decoration by impressing of material into the surface of a ceramic object." ;
	skos:inScheme <https://acdh.oeaw.ac.at/vocabs/defcthesaurus/FindsSchema> , <https://acdh.oeaw.ac.at/vocabs/defcthesaurus/FindsPotteryDecoration> ;
	skos:editorialNote "dc_finds_pottery_decoration;122" ;
	skos:broader <https://acdh.oeaw.ac.at/vocabs/defcthesaurus/incised/4.168> .

<https://acdh.oeaw.ac.at/vocabs/defcthesaurus/incised/4.168> skos:narrower <https://acdh.oeaw.ac.at/vocabs/defcthesaurus/incrusted/5.122> .

<https://acdh.oeaw.ac.at/vocabs/defcthesaurus/mat-impressed/5.129> a skos:Concept ;
	skos:prefLabel "mat-impressed"@en , "Mattenabdr체cke"@de ;
	skos:definition "Pottery decorated by impressing of mat into the surface." ;
	skos:inScheme <https://acdh.oeaw.ac.at/vocabs/defcthesaurus/FindsSchema> , <https://acdh.oeaw.ac.at/vocabs/defcthesaurus/FindsPotteryDecoration> ;
	skos:editorialNote "dc_finds_pottery_decoration;129" ;
	skos:broader <https://acdh.oeaw.ac.at/vocabs/defcthesaurus/incised/4.168> .

<https://acdh.oeaw.ac.at/vocabs/defcthesaurus/incised/4.168> skos:narrower <https://acdh.oeaw.ac.at/vocabs/defcthesaurus/mat-impressed/5.129> .

<https://acdh.oeaw.ac.at/vocabs/defcthesaurus/pattern_jabbed/5.223> a skos:Concept ;
	skos:prefLabel "pattern jabbed"@en , "Eingedr체ckter Musterdekor"@de ;
	skos:definition "Pottery decorated by poking the clay with a pointed object." ;
	skos:inScheme <https://acdh.oeaw.ac.at/vocabs/defcthesaurus/FindsSchema> , <https://acdh.oeaw.ac.at/vocabs/defcthesaurus/FindsPotteryDecoration> ;
	skos:editorialNote "dc_finds_pottery_decoration;223" ;
	skos:broader <https://acdh.oeaw.ac.at/vocabs/defcthesaurus/incised/4.168> .

<https://acdh.oeaw.ac.at/vocabs/defcthesaurus/incised/4.168> skos:narrower <https://acdh.oeaw.ac.at/vocabs/defcthesaurus/pattern_jabbed/5.223> .

<https://acdh.oeaw.ac.at/vocabs/defcthesaurus/punched/5.229> a skos:Concept ;
	skos:prefLabel "punched"@en , "Lochdekor"@de ;
	skos:definition "Pierced/drilled pottery decoration." ;
	skos:inScheme <https://acdh.oeaw.ac.at/vocabs/defcthesaurus/FindsSchema> , <https://acdh.oeaw.ac.at/vocabs/defcthesaurus/FindsPotteryDecoration> ;
	skos:editorialNote "dc_finds_pottery_decoration;229" ;
	skos:broader <https://acdh.oeaw.ac.at/vocabs/defcthesaurus/incised/4.168> .

<https://acdh.oeaw.ac.at/vocabs/defcthesaurus/incised/4.168> skos:narrower <https://acdh.oeaw.ac.at/vocabs/defcthesaurus/punched/5.229> .

<https://acdh.oeaw.ac.at/vocabs/defcthesaurus/red_incrusted/5.203> a skos:Concept ;
	skos:prefLabel "red incrusted"@en , "Rot inkrustiert"@de ;
	skos:definition "The red slip was impressed into the surface of a ceramic vessel." ;
	skos:inScheme <https://acdh.oeaw.ac.at/vocabs/defcthesaurus/FindsSchema> , <https://acdh.oeaw.ac.at/vocabs/defcthesaurus/FindsPotteryDecoration> ;
	skos:editorialNote "dc_finds_pottery_decoration;203" ;
	skos:broader <https://acdh.oeaw.ac.at/vocabs/defcthesaurus/incised/4.168> .

<https://acdh.oeaw.ac.at/vocabs/defcthesaurus/incised/4.168> skos:narrower <https://acdh.oeaw.ac.at/vocabs/defcthesaurus/red_incrusted/5.203> .

<https://acdh.oeaw.ac.at/vocabs/defcthesaurus/rusticated/5.208> a skos:Concept ;
	skos:prefLabel "rusticated"@en , "rustiziert"@de ;
	skos:definition "Pottery with roughened surface which may or may not have an applied slip. The roughening may be achieved using fingers, fingernails, twigs, etc., and though it may be pure decoration, in most cases it is probably a device to prevent a greasy pot slipping" ;
	skos:inScheme <https://acdh.oeaw.ac.at/vocabs/defcthesaurus/FindsSchema> , <https://acdh.oeaw.ac.at/vocabs/defcthesaurus/FindsPotteryDecoration> ;
	skos:editorialNote "dc_finds_pottery_decoration;208" ;
	skos:broader <https://acdh.oeaw.ac.at/vocabs/defcthesaurus/incised/4.168> .

<https://acdh.oeaw.ac.at/vocabs/defcthesaurus/incised/4.168> skos:narrower <https://acdh.oeaw.ac.at/vocabs/defcthesaurus/rusticated/5.208> .

<https://acdh.oeaw.ac.at/vocabs/defcthesaurus/scored/5.233> a skos:Concept ;
	skos:prefLabel "scored"@en , "Eingekerbt"@de ;
	skos:altLabel "wiped"@en , "wiped ware"@en ;
	skos:definition "The surface of the vessels is decorated with rough vertical, diagonal, or horizontal lines wiped in the moist clay." ;
	skos:inScheme <https://acdh.oeaw.ac.at/vocabs/defcthesaurus/FindsSchema> , <https://acdh.oeaw.ac.at/vocabs/defcthesaurus/FindsPotteryDecoration> ;
	skos:editorialNote "dc_finds_pottery_decoration;233" ;
	skos:broader <https://acdh.oeaw.ac.at/vocabs/defcthesaurus/incised/4.168> .

<https://acdh.oeaw.ac.at/vocabs/defcthesaurus/incised/4.168> skos:narrower <https://acdh.oeaw.ac.at/vocabs/defcthesaurus/scored/5.233> .

<https://acdh.oeaw.ac.at/vocabs/defcthesaurus/shell_stamped/5.209> a skos:Concept ;
	skos:prefLabel "shell stamped"@en , "Mit einer Muschel gestempelt"@de ;
	skos:altLabel "cardium ware"@en ;
	skos:definition "Pottery decorated with imprints of marine mollusc shell (cockle-cerastoderma edule)" ;
	skos:inScheme <https://acdh.oeaw.ac.at/vocabs/defcthesaurus/FindsSchema> , <https://acdh.oeaw.ac.at/vocabs/defcthesaurus/FindsPotteryDecoration> ;
	skos:editorialNote "dc_finds_pottery_decoration;209" ;
	skos:broader <https://acdh.oeaw.ac.at/vocabs/defcthesaurus/incised/4.168> .

<https://acdh.oeaw.ac.at/vocabs/defcthesaurus/incised/4.168> skos:narrower <https://acdh.oeaw.ac.at/vocabs/defcthesaurus/shell_stamped/5.209> .

<https://acdh.oeaw.ac.at/vocabs/defcthesaurus/single_jabbed/5.235> a skos:Concept ;
	skos:prefLabel "single jabbed"@en , "Einzeln eingedr체ckter Musterdekor"@de ;
	skos:definition "Ware decorated with single engraved lines." ;
	skos:inScheme <https://acdh.oeaw.ac.at/vocabs/defcthesaurus/FindsSchema> , <https://acdh.oeaw.ac.at/vocabs/defcthesaurus/FindsPotteryDecoration> ;
	skos:editorialNote "dc_finds_pottery_decoration;235" ;
	skos:broader <https://acdh.oeaw.ac.at/vocabs/defcthesaurus/incised/4.168> .

<https://acdh.oeaw.ac.at/vocabs/defcthesaurus/incised/4.168> skos:narrower <https://acdh.oeaw.ac.at/vocabs/defcthesaurus/single_jabbed/5.235> .

<https://acdh.oeaw.ac.at/vocabs/defcthesaurus/painted/4.239> a skos:Concept ;
	skos:prefLabel "painted"@en , "Bemalt"@de ;
	skos:definition "Paint applied to pottery." ;
	skos:inScheme <https://acdh.oeaw.ac.at/vocabs/defcthesaurus/FindsSchema> , <https://acdh.oeaw.ac.at/vocabs/defcthesaurus/FindsPotteryDecoration> ;
	skos:editorialNote "dc_finds_pottery_decoration;239" ;
	skos:broader <https://acdh.oeaw.ac.at/vocabs/defcthesaurus/pottery_decoration/3.018> .

<https://acdh.oeaw.ac.at/vocabs/defcthesaurus/pottery_decoration/3.018> skos:narrower <https://acdh.oeaw.ac.at/vocabs/defcthesaurus/painted/4.239> .

<https://acdh.oeaw.ac.at/vocabs/defcthesaurus/pattern_painted/5.041> a skos:Concept ;
	skos:prefLabel "pattern painted"@en , "Musterbemalt"@de ;
	skos:inScheme <https://acdh.oeaw.ac.at/vocabs/defcthesaurus/FindsSchema> , <https://acdh.oeaw.ac.at/vocabs/defcthesaurus/NotInDatabase> ;
	skos:editorialNote "dc_not_in_database;041" ;
	skos:broader <https://acdh.oeaw.ac.at/vocabs/defcthesaurus/painted/4.239> .

<https://acdh.oeaw.ac.at/vocabs/defcthesaurus/painted/4.239> skos:narrower <https://acdh.oeaw.ac.at/vocabs/defcthesaurus/pattern_painted/5.041> .

<https://acdh.oeaw.ac.at/vocabs/defcthesaurus/finds_type/1.02> dc:source "Kipfer, B. A. Dictionary of Artifacts 2007. Blackwell Publishing, Oxford.p 248" .

<https://acdh.oeaw.ac.at/vocabs/defcthesaurus/polychrome/6.202> a skos:Concept ;
	skos:prefLabel "polychrome"@en , "Polychrom"@de ;
	skos:definition "Pottery that is decorated in more than two colors, but the term is also sometimes applied to pottery with more than one color." ;
	skos:inScheme <https://acdh.oeaw.ac.at/vocabs/defcthesaurus/FindsSchema> , <https://acdh.oeaw.ac.at/vocabs/defcthesaurus/FindsPotteryDecoration> ;
	skos:editorialNote "dc_finds_pottery_decoration;02" ;
	skos:broader <https://acdh.oeaw.ac.at/vocabs/defcthesaurus/pattern_painted/5.041> .

<https://acdh.oeaw.ac.at/vocabs/defcthesaurus/pattern_painted/5.041> skos:narrower <https://acdh.oeaw.ac.at/vocabs/defcthesaurus/polychrome/6.202> .

<https://acdh.oeaw.ac.at/vocabs/defcthesaurus/black_and_red_on_cream_(polychrome)_(棺3棺)/6.138> a skos:Concept ;
	skos:prefLabel "black and red on cream (polychrome) (棺3棺)"@en , "Schwarz und rot auf beige (polychrom) (B3b)"@de ;
	skos:definition "Pottery decorated with black and red paint on cream ground (polychrome)." ;
	skos:inScheme <https://acdh.oeaw.ac.at/vocabs/defcthesaurus/FindsSchema> , <https://acdh.oeaw.ac.at/vocabs/defcthesaurus/FindsPotteryDecoration> ;
	skos:editorialNote "dc_finds_pottery_decoration;02" ;
	skos:broader <https://acdh.oeaw.ac.at/vocabs/defcthesaurus/pattern_painted/5.041> .

<https://acdh.oeaw.ac.at/vocabs/defcthesaurus/pattern_painted/5.041> skos:narrower <https://acdh.oeaw.ac.at/vocabs/defcthesaurus/black_and_red_on_cream_(polychrome)_(棺3棺)/6.138> .

<https://acdh.oeaw.ac.at/vocabs/defcthesaurus/black_and_red_on_white_(polychrome)_(棺3款)/6.139> a skos:Concept ;
	skos:prefLabel "black and red on white (polychrome) (棺3款)"@en , "Schwarz und rot auf wei (polychrom) (B3c)"@de ;
	skos:definition "Pottery decorated with black and red paint on cream ground (polychrome)." ;
	skos:inScheme <https://acdh.oeaw.ac.at/vocabs/defcthesaurus/FindsSchema> , <https://acdh.oeaw.ac.at/vocabs/defcthesaurus/FindsPotteryDecoration> ;
	skos:editorialNote "dc_finds_pottery_decoration;02" ;
	skos:broader <https://acdh.oeaw.ac.at/vocabs/defcthesaurus/pattern_painted/5.041> .

<https://acdh.oeaw.ac.at/vocabs/defcthesaurus/pattern_painted/5.041> skos:narrower <https://acdh.oeaw.ac.at/vocabs/defcthesaurus/black_and_red_on_white_(polychrome)_(棺3款)/6.139> .

<https://acdh.oeaw.ac.at/vocabs/defcthesaurus/black_and_white_on_red_(polychrome)_(棺3棺)/6.140> a skos:Concept ;
	skos:prefLabel "black and white on red (polychrome) (棺3棺)"@en , "Schwarz und wei auf rot (polychrom) (B3b)"@de ;
	skos:definition "Pottery decorated with black and red paint on cream ground (polychrome)." ;
	skos:inScheme <https://acdh.oeaw.ac.at/vocabs/defcthesaurus/FindsSchema> , <https://acdh.oeaw.ac.at/vocabs/defcthesaurus/FindsPotteryDecoration> ;
	skos:editorialNote "dc_finds_pottery_decoration;02" ;
	skos:broader <https://acdh.oeaw.ac.at/vocabs/defcthesaurus/pattern_painted/5.041> .

<https://acdh.oeaw.ac.at/vocabs/defcthesaurus/pattern_painted/5.041> skos:narrower <https://acdh.oeaw.ac.at/vocabs/defcthesaurus/black_and_white_on_red_(polychrome)_(棺3棺)/6.140> .

<https://acdh.oeaw.ac.at/vocabs/defcthesaurus/black_on_grey/6.287> a skos:Concept ;
	skos:prefLabel "black on grey"@en , "schwarz auf grau"@de ;
	skos:definition "Pottery decorated with black paint added on grey ground." ;
	skos:inScheme <https://acdh.oeaw.ac.at/vocabs/defcthesaurus/FindsSchema> , <https://acdh.oeaw.ac.at/vocabs/defcthesaurus/FindsPotteryDecoration> ;
	skos:editorialNote "dc_finds_pottery_decoration;02" ;
	skos:broader <https://acdh.oeaw.ac.at/vocabs/defcthesaurus/pattern_painted/5.041> .

<https://acdh.oeaw.ac.at/vocabs/defcthesaurus/pattern_painted/5.041> skos:narrower <https://acdh.oeaw.ac.at/vocabs/defcthesaurus/black_on_grey/6.287> .

<https://acdh.oeaw.ac.at/vocabs/defcthesaurus/black_on_red/6.163> a skos:Concept ;
	skos:prefLabel "black on red"@en , "Schwarz auf rot"@de ;
	skos:altLabel "Galepsos ware"@en ;
	skos:definition "Pottery decorated with black paint added on red ground." ;
	skos:inScheme <https://acdh.oeaw.ac.at/vocabs/defcthesaurus/FindsSchema> , <https://acdh.oeaw.ac.at/vocabs/defcthesaurus/FindsPotteryDecoration> ;
	skos:editorialNote "dc_finds_pottery_decoration;02" ;
	skos:broader <https://acdh.oeaw.ac.at/vocabs/defcthesaurus/pattern_painted/5.041> .

<https://acdh.oeaw.ac.at/vocabs/defcthesaurus/pattern_painted/5.041> skos:narrower <https://acdh.oeaw.ac.at/vocabs/defcthesaurus/black_on_red/6.163> .

<https://acdh.oeaw.ac.at/vocabs/defcthesaurus/black_on_red_(棺3慣2b)/6.144> a skos:Concept ;
	skos:prefLabel "black on red (棺3慣2b)"@en , "Schwarz auf rot  (B3a2b)"@de ;
	skos:definition "Pottery decorated with black paint added on red ground." ;
	skos:inScheme <https://acdh.oeaw.ac.at/vocabs/defcthesaurus/FindsSchema> , <https://acdh.oeaw.ac.at/vocabs/defcthesaurus/FindsPotteryDecoration> ;
	skos:editorialNote "dc_finds_pottery_decoration;02" ;
	skos:broader <https://acdh.oeaw.ac.at/vocabs/defcthesaurus/pattern_painted/5.041> .

<https://acdh.oeaw.ac.at/vocabs/defcthesaurus/pattern_painted/5.041> skos:narrower <https://acdh.oeaw.ac.at/vocabs/defcthesaurus/black_on_red_(棺3慣2b)/6.144> .

<https://acdh.oeaw.ac.at/vocabs/defcthesaurus/black_on_white/6.279> a skos:Concept ;
	skos:prefLabel "black on white"@en , "schwarz auf wei"@de ;
	skos:definition "Pottery decorated with black paint added on white ground." ;
	skos:inScheme <https://acdh.oeaw.ac.at/vocabs/defcthesaurus/FindsSchema> , <https://acdh.oeaw.ac.at/vocabs/defcthesaurus/FindsPotteryDecoration> ;
	skos:editorialNote "dc_finds_pottery_decoration;02" ;
	skos:broader <https://acdh.oeaw.ac.at/vocabs/defcthesaurus/pattern_painted/5.041> .

<https://acdh.oeaw.ac.at/vocabs/defcthesaurus/pattern_painted/5.041> skos:narrower <https://acdh.oeaw.ac.at/vocabs/defcthesaurus/black_on_white/6.279> .

<https://acdh.oeaw.ac.at/vocabs/defcthesaurus/black_on_white_(b3慣3)/6.145> a skos:Concept ;
	skos:prefLabel "black on white (b3慣3)"@en , "Schwarz auf wei  (B3a3)"@de ;
	skos:definition "Pottery decorated with black paint added on white ground." ;
	skos:inScheme <https://acdh.oeaw.ac.at/vocabs/defcthesaurus/FindsSchema> , <https://acdh.oeaw.ac.at/vocabs/defcthesaurus/FindsPotteryDecoration> ;
	skos:editorialNote "dc_finds_pottery_decoration;02" ;
	skos:broader <https://acdh.oeaw.ac.at/vocabs/defcthesaurus/pattern_painted/5.041> .

<https://acdh.oeaw.ac.at/vocabs/defcthesaurus/pattern_painted/5.041> skos:narrower <https://acdh.oeaw.ac.at/vocabs/defcthesaurus/black_on_white_(b3慣3)/6.145> .

<https://acdh.oeaw.ac.at/vocabs/defcthesaurus/brown_on_buff/6.185> a skos:Concept ;
	skos:prefLabel "brown on buff"@en , "Braun auf hell"@de ;
	skos:definition "Pottery decorated with brown paint on buff ground." ;
	skos:inScheme <https://acdh.oeaw.ac.at/vocabs/defcthesaurus/FindsSchema> , <https://acdh.oeaw.ac.at/vocabs/defcthesaurus/FindsPotteryDecoration> ;
	skos:editorialNote "dc_finds_pottery_decoration;02" ;
	skos:broader <https://acdh.oeaw.ac.at/vocabs/defcthesaurus/pattern_painted/5.041> .

<https://acdh.oeaw.ac.at/vocabs/defcthesaurus/pattern_painted/5.041> skos:narrower <https://acdh.oeaw.ac.at/vocabs/defcthesaurus/brown_on_buff/6.185> .

<https://acdh.oeaw.ac.at/vocabs/defcthesaurus/brown_on_buff_(matt_painted)_(b3琯)/6.147> a skos:Concept ;
	skos:prefLabel "brown on buff (matt painted) (b3琯)"@en , "Braun auf hell (mattbemalt) (B3e)"@de ;
	skos:definition "Pottery decorated with brown paint on buff ground also known as matt-painted." ;
	skos:inScheme <https://acdh.oeaw.ac.at/vocabs/defcthesaurus/FindsSchema> , <https://acdh.oeaw.ac.at/vocabs/defcthesaurus/FindsPotteryDecoration> ;
	skos:editorialNote "dc_finds_pottery_decoration;02" ;
	skos:broader <https://acdh.oeaw.ac.at/vocabs/defcthesaurus/pattern_painted/5.041> .

<https://acdh.oeaw.ac.at/vocabs/defcthesaurus/pattern_painted/5.041> skos:narrower <https://acdh.oeaw.ac.at/vocabs/defcthesaurus/brown_on_buff_(matt_painted)_(b3琯)/6.147> .

<https://acdh.oeaw.ac.at/vocabs/defcthesaurus/brown_on_cream/6.262> a skos:Concept ;
	skos:prefLabel "brown on cream"@en , "Braun auf beige"@de ;
	skos:definition "Pottery decorated with brown paint on cream ground." ;
	skos:inScheme <https://acdh.oeaw.ac.at/vocabs/defcthesaurus/FindsSchema> , <https://acdh.oeaw.ac.at/vocabs/defcthesaurus/FindsPotteryDecoration> ;
	skos:editorialNote "dc_finds_pottery_decoration;02" ;
	skos:broader <https://acdh.oeaw.ac.at/vocabs/defcthesaurus/pattern_painted/5.041> .

<https://acdh.oeaw.ac.at/vocabs/defcthesaurus/pattern_painted/5.041> skos:narrower <https://acdh.oeaw.ac.at/vocabs/defcthesaurus/brown_on_cream/6.262> .

<https://acdh.oeaw.ac.at/vocabs/defcthesaurus/brown_on_cream_(b3慣2a)/6.148> a skos:Concept ;
	skos:prefLabel "brown on cream (b3慣2a)"@en , "Braun auf beige  (B3a2a)"@de ;
	skos:definition "Pottery decorated with brown paint on cream ground." ;
	skos:inScheme <https://acdh.oeaw.ac.at/vocabs/defcthesaurus/FindsSchema> , <https://acdh.oeaw.ac.at/vocabs/defcthesaurus/FindsPotteryDecoration> ;
	skos:editorialNote "dc_finds_pottery_decoration;02" ;
	skos:broader <https://acdh.oeaw.ac.at/vocabs/defcthesaurus/pattern_painted/5.041> .

<https://acdh.oeaw.ac.at/vocabs/defcthesaurus/pattern_painted/5.041> skos:narrower <https://acdh.oeaw.ac.at/vocabs/defcthesaurus/brown_on_cream_(b3慣2a)/6.148> .

<https://acdh.oeaw.ac.at/vocabs/defcthesaurus/brown_on_red/6.186> a skos:Concept ;
	skos:prefLabel "brown on red"@en , "Braun auf rot"@de ;
	skos:definition "Pottery decorated with brown paint on red ground." ;
	skos:inScheme <https://acdh.oeaw.ac.at/vocabs/defcthesaurus/FindsSchema> , <https://acdh.oeaw.ac.at/vocabs/defcthesaurus/FindsPotteryDecoration> ;
	skos:editorialNote "dc_finds_pottery_decoration;02" ;
	skos:broader <https://acdh.oeaw.ac.at/vocabs/defcthesaurus/pattern_painted/5.041> .

<https://acdh.oeaw.ac.at/vocabs/defcthesaurus/pattern_painted/5.041> skos:narrower <https://acdh.oeaw.ac.at/vocabs/defcthesaurus/brown_on_red/6.186> .

<https://acdh.oeaw.ac.at/vocabs/defcthesaurus/brown_on_yellow/6.283> a skos:Concept ;
	skos:prefLabel "brown on yellow"@en , "braun auf gelb"@de ;
	skos:definition "Pottery decorated with brown paint on yellow ground." ;
	skos:inScheme <https://acdh.oeaw.ac.at/vocabs/defcthesaurus/FindsSchema> , <https://acdh.oeaw.ac.at/vocabs/defcthesaurus/FindsPotteryDecoration> ;
	skos:editorialNote "dc_finds_pottery_decoration;02" ;
	skos:broader <https://acdh.oeaw.ac.at/vocabs/defcthesaurus/pattern_painted/5.041> .

<https://acdh.oeaw.ac.at/vocabs/defcthesaurus/pattern_painted/5.041> skos:narrower <https://acdh.oeaw.ac.at/vocabs/defcthesaurus/brown_on_yellow/6.283> .

<https://acdh.oeaw.ac.at/vocabs/defcthesaurus/graphite_painted/6.194> a skos:Concept ;
	skos:prefLabel "graphite painted"@en , "Graphitbemalt"@de ;
	skos:definition "Pottery decorated with graphite paint." ;
	skos:inScheme <https://acdh.oeaw.ac.at/vocabs/defcthesaurus/FindsSchema> , <https://acdh.oeaw.ac.at/vocabs/defcthesaurus/FindsPotteryDecoration> ;
	skos:editorialNote "dc_finds_pottery_decoration;02" ;
	skos:broader <https://acdh.oeaw.ac.at/vocabs/defcthesaurus/pattern_painted/5.041> .

<https://acdh.oeaw.ac.at/vocabs/defcthesaurus/pattern_painted/5.041> skos:narrower <https://acdh.oeaw.ac.at/vocabs/defcthesaurus/graphite_painted/6.194> .

<https://acdh.oeaw.ac.at/vocabs/defcthesaurus/grey_on_grey/6.277> a skos:Concept ;
	skos:prefLabel "grey on grey"@en , "grau auf grau"@de ;
	skos:definition "Pottery decorated with grey paint on grey ground." ;
	skos:inScheme <https://acdh.oeaw.ac.at/vocabs/defcthesaurus/FindsSchema> , <https://acdh.oeaw.ac.at/vocabs/defcthesaurus/FindsPotteryDecoration> ;
	skos:editorialNote "dc_finds_pottery_decoration;02" ;
	skos:broader <https://acdh.oeaw.ac.at/vocabs/defcthesaurus/pattern_painted/5.041> .

<https://acdh.oeaw.ac.at/vocabs/defcthesaurus/pattern_painted/5.041> skos:narrower <https://acdh.oeaw.ac.at/vocabs/defcthesaurus/grey_on_grey/6.277> .

<https://acdh.oeaw.ac.at/vocabs/defcthesaurus/grey_on_grey_(款1棺)/6.150> a skos:Concept ;
	skos:prefLabel "grey on grey (款1棺)"@en , "Grau auf grau (C1b)"@de ;
	skos:definition "Pottery decorated with grey paint on grey ground." ;
	skos:inScheme <https://acdh.oeaw.ac.at/vocabs/defcthesaurus/FindsSchema> , <https://acdh.oeaw.ac.at/vocabs/defcthesaurus/FindsPotteryDecoration> ;
	skos:editorialNote "dc_finds_pottery_decoration;02" ;
	skos:broader <https://acdh.oeaw.ac.at/vocabs/defcthesaurus/pattern_painted/5.041> .

<https://acdh.oeaw.ac.at/vocabs/defcthesaurus/pattern_painted/5.041> skos:narrower <https://acdh.oeaw.ac.at/vocabs/defcthesaurus/grey_on_grey_(款1棺)/6.150> .

<https://acdh.oeaw.ac.at/vocabs/defcthesaurus/grey_ware/6.246> a skos:Concept ;
	skos:prefLabel "grey ware"@en , "grau Ware"@de ;
	skos:definition "Grey ware." ;
	skos:inScheme <https://acdh.oeaw.ac.at/vocabs/defcthesaurus/FindsSchema> , <https://acdh.oeaw.ac.at/vocabs/defcthesaurus/FindsPotteryDecoration> ;
	skos:editorialNote "dc_finds_pottery_decoration;02" ;
	skos:broader <https://acdh.oeaw.ac.at/vocabs/defcthesaurus/pattern_painted/5.041> .

<https://acdh.oeaw.ac.at/vocabs/defcthesaurus/pattern_painted/5.041> skos:narrower <https://acdh.oeaw.ac.at/vocabs/defcthesaurus/grey_ware/6.246> .

<https://acdh.oeaw.ac.at/vocabs/defcthesaurus/halaf_painted/6.125> a skos:Concept ;
	skos:prefLabel "halaf painted"@en , "Halaf Bemalung"@de ;
	skos:definition "Pottery decorated by imprinting of the clay with different types of objects." ;
	skos:inScheme <https://acdh.oeaw.ac.at/vocabs/defcthesaurus/FindsSchema> , <https://acdh.oeaw.ac.at/vocabs/defcthesaurus/FindsPotteryDecoration> ;
	skos:editorialNote "dc_finds_pottery_decoration;02" ;
	skos:broader <https://acdh.oeaw.ac.at/vocabs/defcthesaurus/pattern_painted/5.041> .

<https://acdh.oeaw.ac.at/vocabs/defcthesaurus/pattern_painted/5.041> skos:narrower <https://acdh.oeaw.ac.at/vocabs/defcthesaurus/halaf_painted/6.125> .

<https://acdh.oeaw.ac.at/vocabs/defcthesaurus/matt_brown_on_white/6.199> a skos:Concept ;
	skos:prefLabel "matt brown on white"@en , "Matt bemalt, braun auf wei"@de ;
	skos:definition "Pottery decorated with matt brown paint on white ground." ;
	skos:inScheme <https://acdh.oeaw.ac.at/vocabs/defcthesaurus/FindsSchema> , <https://acdh.oeaw.ac.at/vocabs/defcthesaurus/FindsPotteryDecoration> ;
	skos:editorialNote "dc_finds_pottery_decoration;02" ;
	skos:broader <https://acdh.oeaw.ac.at/vocabs/defcthesaurus/pattern_painted/5.041> .

<https://acdh.oeaw.ac.at/vocabs/defcthesaurus/pattern_painted/5.041> skos:narrower <https://acdh.oeaw.ac.at/vocabs/defcthesaurus/matt_brown_on_white/6.199> .

<https://acdh.oeaw.ac.at/vocabs/defcthesaurus/finds_type/1.02> dc:source "Kipfer, B. A. Dictionary of Artifacts 2007. Blackwell Publishing, Oxford.p. 191" .

<https://acdh.oeaw.ac.at/vocabs/defcthesaurus/matt_painted/6.169> a skos:Concept ;
	skos:prefLabel "matt painted"@en , "Matt bemalt"@de ;
	skos:altLabel "Matt-painted"@en ;
	skos:definition "Pottery with simple decoration in manganese-based purple-black paint on a pale ground. Matt-painted pottery has been found in the nearer islands to mainland Greece and even as far as Crete and the Anatolian coast." ;
	skos:inScheme <https://acdh.oeaw.ac.at/vocabs/defcthesaurus/FindsSchema> , <https://acdh.oeaw.ac.at/vocabs/defcthesaurus/FindsPotteryDecoration> ;
	skos:editorialNote "dc_finds_pottery_decoration;02" ;
	skos:broader <https://acdh.oeaw.ac.at/vocabs/defcthesaurus/pattern_painted/5.041> .

<https://acdh.oeaw.ac.at/vocabs/defcthesaurus/pattern_painted/5.041> skos:narrower <https://acdh.oeaw.ac.at/vocabs/defcthesaurus/matt_painted/6.169> .

<https://acdh.oeaw.ac.at/vocabs/defcthesaurus/red_on_brown/6.204> a skos:Concept ;
	skos:prefLabel "red on brown"@en , "Rot auf braun"@de ;
	skos:definition "Pottery painted with red paint on brown ground." ;
	skos:inScheme <https://acdh.oeaw.ac.at/vocabs/defcthesaurus/FindsSchema> , <https://acdh.oeaw.ac.at/vocabs/defcthesaurus/FindsPotteryDecoration> ;
	skos:editorialNote "dc_finds_pottery_decoration;02" ;
	skos:broader <https://acdh.oeaw.ac.at/vocabs/defcthesaurus/pattern_painted/5.041> .

<https://acdh.oeaw.ac.at/vocabs/defcthesaurus/pattern_painted/5.041> skos:narrower <https://acdh.oeaw.ac.at/vocabs/defcthesaurus/red_on_brown/6.204> .

<https://acdh.oeaw.ac.at/vocabs/defcthesaurus/red_on_buff/6.230> a skos:Concept ;
	skos:prefLabel "red on buff"@en , "Rot auf hell"@de ;
	skos:definition "Pottery painted with red paint on buff ground." ;
	skos:inScheme <https://acdh.oeaw.ac.at/vocabs/defcthesaurus/FindsSchema> , <https://acdh.oeaw.ac.at/vocabs/defcthesaurus/FindsPotteryDecoration> ;
	skos:editorialNote "dc_finds_pottery_decoration;02" ;
	skos:broader <https://acdh.oeaw.ac.at/vocabs/defcthesaurus/pattern_painted/5.041> .

<https://acdh.oeaw.ac.at/vocabs/defcthesaurus/pattern_painted/5.041> skos:narrower <https://acdh.oeaw.ac.at/vocabs/defcthesaurus/red_on_buff/6.230> .

<https://acdh.oeaw.ac.at/vocabs/defcthesaurus/red_on_red/6.268> a skos:Concept ;
	skos:prefLabel "red on red"@en , "rot auf rot"@de ;
	skos:definition "Pottery painted with red paint on red ground." ;
	skos:inScheme <https://acdh.oeaw.ac.at/vocabs/defcthesaurus/FindsSchema> , <https://acdh.oeaw.ac.at/vocabs/defcthesaurus/FindsPotteryDecoration> ;
	skos:editorialNote "dc_finds_pottery_decoration;02" ;
	skos:broader <https://acdh.oeaw.ac.at/vocabs/defcthesaurus/pattern_painted/5.041> .

<https://acdh.oeaw.ac.at/vocabs/defcthesaurus/pattern_painted/5.041> skos:narrower <https://acdh.oeaw.ac.at/vocabs/defcthesaurus/red_on_red/6.268> .

<https://acdh.oeaw.ac.at/vocabs/defcthesaurus/red_on_red_(a3款)/6.158> a skos:Concept ;
	skos:prefLabel "red on red (a3款)"@en , "Rot on red (A3c)"@de ;
	skos:definition "Pottery painted with red paint on red ground." ;
	skos:inScheme <https://acdh.oeaw.ac.at/vocabs/defcthesaurus/FindsSchema> , <https://acdh.oeaw.ac.at/vocabs/defcthesaurus/FindsPotteryDecoration> ;
	skos:editorialNote "dc_finds_pottery_decoration;02" ;
	skos:broader <https://acdh.oeaw.ac.at/vocabs/defcthesaurus/pattern_painted/5.041> .

<https://acdh.oeaw.ac.at/vocabs/defcthesaurus/pattern_painted/5.041> skos:narrower <https://acdh.oeaw.ac.at/vocabs/defcthesaurus/red_on_red_(a3款)/6.158> .

<https://acdh.oeaw.ac.at/vocabs/defcthesaurus/red_on_white/6.290> a skos:Concept ;
	skos:prefLabel "red on white"@en , "Rot auf wei"@de ;
	skos:definition "Pottery painted with red paint on white ground." ;
	skos:inScheme <https://acdh.oeaw.ac.at/vocabs/defcthesaurus/FindsSchema> , <https://acdh.oeaw.ac.at/vocabs/defcthesaurus/FindsPotteryDecoration> ;
	skos:editorialNote "dc_finds_pottery_decoration;02" ;
	skos:broader <https://acdh.oeaw.ac.at/vocabs/defcthesaurus/pattern_painted/5.041> .

<https://acdh.oeaw.ac.at/vocabs/defcthesaurus/pattern_painted/5.041> skos:narrower <https://acdh.oeaw.ac.at/vocabs/defcthesaurus/red_on_white/6.290> .

<https://acdh.oeaw.ac.at/vocabs/defcthesaurus/red_on_white_(a3)/6.157> a skos:Concept ;
	skos:prefLabel "red on white (a3)"@en , "Rot auf wei (A3b)"@de ;
	skos:definition "Pottery painted with red paint on white ground." ;
	skos:inScheme <https://acdh.oeaw.ac.at/vocabs/defcthesaurus/FindsSchema> , <https://acdh.oeaw.ac.at/vocabs/defcthesaurus/FindsPotteryDecoration> ;
	skos:editorialNote "dc_finds_pottery_decoration;02" ;
	skos:broader <https://acdh.oeaw.ac.at/vocabs/defcthesaurus/pattern_painted/5.041> .

<https://acdh.oeaw.ac.at/vocabs/defcthesaurus/pattern_painted/5.041> skos:narrower <https://acdh.oeaw.ac.at/vocabs/defcthesaurus/red_on_white_(a3)/6.157> .

<https://acdh.oeaw.ac.at/vocabs/defcthesaurus/red_on_yellow/6.282> a skos:Concept ;
	skos:prefLabel "red on yellow"@en , "rot auf gelb"@de ;
	skos:definition "Pottery painted with red paint on yellow ground." ;
	skos:inScheme <https://acdh.oeaw.ac.at/vocabs/defcthesaurus/FindsSchema> , <https://acdh.oeaw.ac.at/vocabs/defcthesaurus/FindsPotteryDecoration> ;
	skos:editorialNote "dc_finds_pottery_decoration;02" ;
	skos:broader <https://acdh.oeaw.ac.at/vocabs/defcthesaurus/pattern_painted/5.041> .

<https://acdh.oeaw.ac.at/vocabs/defcthesaurus/pattern_painted/5.041> skos:narrower <https://acdh.oeaw.ac.at/vocabs/defcthesaurus/red_on_yellow/6.282> .

<https://acdh.oeaw.ac.at/vocabs/defcthesaurus/white_on_black/6.181> a skos:Concept ;
	skos:prefLabel "white on black"@en , "Wei auf schwarz"@de ;
	skos:definition "Pottery painted with white paint on black ground." ;
	skos:inScheme <https://acdh.oeaw.ac.at/vocabs/defcthesaurus/FindsSchema> , <https://acdh.oeaw.ac.at/vocabs/defcthesaurus/FindsPotteryDecoration> ;
	skos:editorialNote "dc_finds_pottery_decoration;02" ;
	skos:broader <https://acdh.oeaw.ac.at/vocabs/defcthesaurus/pattern_painted/5.041> .

<https://acdh.oeaw.ac.at/vocabs/defcthesaurus/pattern_painted/5.041> skos:narrower <https://acdh.oeaw.ac.at/vocabs/defcthesaurus/white_on_black/6.181> .

<https://acdh.oeaw.ac.at/vocabs/defcthesaurus/white_on_red/6.137> a skos:Concept ;
	skos:prefLabel "white on red"@en , "Wei auf rot"@de ;
	skos:definition "Pottery painted with white paint on red ground." ;
	skos:inScheme <https://acdh.oeaw.ac.at/vocabs/defcthesaurus/FindsSchema> , <https://acdh.oeaw.ac.at/vocabs/defcthesaurus/FindsPotteryDecoration> ;
	skos:editorialNote "dc_finds_pottery_decoration;02" ;
	skos:broader <https://acdh.oeaw.ac.at/vocabs/defcthesaurus/pattern_painted/5.041> .

<https://acdh.oeaw.ac.at/vocabs/defcthesaurus/pattern_painted/5.041> skos:narrower <https://acdh.oeaw.ac.at/vocabs/defcthesaurus/white_on_red/6.137> .

<https://acdh.oeaw.ac.at/vocabs/defcthesaurus/white_on_red_(棺3慣1)/6.161> a skos:Concept ;
	skos:prefLabel "white on red (棺3慣1)"@en , "Wei auf rot (B3a1)"@de ;
	skos:definition "Pottery painted with white paint on red ground." ;
	skos:inScheme <https://acdh.oeaw.ac.at/vocabs/defcthesaurus/FindsSchema> , <https://acdh.oeaw.ac.at/vocabs/defcthesaurus/FindsPotteryDecoration> ;
	skos:editorialNote "dc_finds_pottery_decoration;02" ;
	skos:broader <https://acdh.oeaw.ac.at/vocabs/defcthesaurus/pattern_painted/5.041> .

<https://acdh.oeaw.ac.at/vocabs/defcthesaurus/pattern_painted/5.041> skos:narrower <https://acdh.oeaw.ac.at/vocabs/defcthesaurus/white_on_red_(棺3慣1)/6.161> .

<https://acdh.oeaw.ac.at/vocabs/defcthesaurus/white_on_red_(a3慣)/6.160> a skos:Concept ;
	skos:prefLabel "white on red (a3慣)"@en , "Wei auf rot (A3a)"@de ;
	skos:definition "Pottery painted with white paint on red ground." ;
	skos:inScheme <https://acdh.oeaw.ac.at/vocabs/defcthesaurus/FindsSchema> , <https://acdh.oeaw.ac.at/vocabs/defcthesaurus/FindsPotteryDecoration> ;
	skos:editorialNote "dc_finds_pottery_decoration;02" ;
	skos:broader <https://acdh.oeaw.ac.at/vocabs/defcthesaurus/pattern_painted/5.041> .

<https://acdh.oeaw.ac.at/vocabs/defcthesaurus/pattern_painted/5.041> skos:narrower <https://acdh.oeaw.ac.at/vocabs/defcthesaurus/white_on_red_(a3慣)/6.160> .

<https://acdh.oeaw.ac.at/vocabs/defcthesaurus/monochrome/5.265> a skos:Concept ;
	skos:prefLabel "monochrome"@en , "Monochrom"@de ;
	skos:definition "Pottery painted with one or maximally two colors." ;
	skos:inScheme <https://acdh.oeaw.ac.at/vocabs/defcthesaurus/FindsSchema> , <https://acdh.oeaw.ac.at/vocabs/defcthesaurus/FindsPotteryDecoration> ;
	skos:editorialNote "dc_finds_pottery_decoration;265" ;
	skos:broader <https://acdh.oeaw.ac.at/vocabs/defcthesaurus/painted/4.239> .

<https://acdh.oeaw.ac.at/vocabs/defcthesaurus/painted/4.239> skos:narrower <https://acdh.oeaw.ac.at/vocabs/defcthesaurus/monochrome/5.265> .

<https://acdh.oeaw.ac.at/vocabs/defcthesaurus/monochrome_black/6.245> a skos:Concept ;
	skos:prefLabel "monochrome black"@en , "Monochrom schwarz"@de ;
	skos:definition "Pottery painted with black paint on black ground." ;
	skos:inScheme <https://acdh.oeaw.ac.at/vocabs/defcthesaurus/FindsSchema> , <https://acdh.oeaw.ac.at/vocabs/defcthesaurus/FindsPotteryDecoration> ;
	skos:editorialNote "dc_finds_pottery_decoration;02" ;
	skos:broader <https://acdh.oeaw.ac.at/vocabs/defcthesaurus/monochrome/5.265> .

<https://acdh.oeaw.ac.at/vocabs/defcthesaurus/monochrome/5.265> skos:narrower <https://acdh.oeaw.ac.at/vocabs/defcthesaurus/monochrome_black/6.245> .

<https://acdh.oeaw.ac.at/vocabs/defcthesaurus/monochrome_brown/6.130> a skos:Concept ;
	skos:prefLabel "monochrome brown"@en , "Monochrom braun"@de ;
	skos:definition "Pottery painted with brown paint on brown ground." ;
	skos:inScheme <https://acdh.oeaw.ac.at/vocabs/defcthesaurus/FindsSchema> , <https://acdh.oeaw.ac.at/vocabs/defcthesaurus/FindsPotteryDecoration> ;
	skos:editorialNote "dc_finds_pottery_decoration;02" ;
	skos:broader <https://acdh.oeaw.ac.at/vocabs/defcthesaurus/monochrome/5.265> .

<https://acdh.oeaw.ac.at/vocabs/defcthesaurus/monochrome/5.265> skos:narrower <https://acdh.oeaw.ac.at/vocabs/defcthesaurus/monochrome_brown/6.130> .

<https://acdh.oeaw.ac.at/vocabs/defcthesaurus/monochrome_grey/6.294> a skos:Concept ;
	skos:prefLabel "monochrome grey"@en , "monochrom grau"@de ;
	skos:definition "Pottery painted with grey paint on grey ground." ;
	skos:inScheme <https://acdh.oeaw.ac.at/vocabs/defcthesaurus/FindsSchema> , <https://acdh.oeaw.ac.at/vocabs/defcthesaurus/FindsPotteryDecoration> ;
	skos:editorialNote "dc_finds_pottery_decoration;02" ;
	skos:broader <https://acdh.oeaw.ac.at/vocabs/defcthesaurus/monochrome/5.265> .

<https://acdh.oeaw.ac.at/vocabs/defcthesaurus/monochrome/5.265> skos:narrower <https://acdh.oeaw.ac.at/vocabs/defcthesaurus/monochrome_grey/6.294> .

<https://acdh.oeaw.ac.at/vocabs/defcthesaurus/monochrome_orange/6.200> a skos:Concept ;
	skos:prefLabel "monochrome orange"@en , "monochrom orange"@de ;
	skos:definition "Pottery painted with orange paint on orange ground." ;
	skos:inScheme <https://acdh.oeaw.ac.at/vocabs/defcthesaurus/FindsSchema> , <https://acdh.oeaw.ac.at/vocabs/defcthesaurus/FindsPotteryDecoration> ;
	skos:editorialNote "dc_finds_pottery_decoration;02" ;
	skos:broader <https://acdh.oeaw.ac.at/vocabs/defcthesaurus/monochrome/5.265> .

<https://acdh.oeaw.ac.at/vocabs/defcthesaurus/monochrome/5.265> skos:narrower <https://acdh.oeaw.ac.at/vocabs/defcthesaurus/monochrome_orange/6.200> .

<https://acdh.oeaw.ac.at/vocabs/defcthesaurus/monochrome_red/6.249> a skos:Concept ;
	skos:prefLabel "monochrome red"@en , "Monochrom rot"@de ;
	skos:definition "Pottery painted with red paint on red ground." ;
	skos:inScheme <https://acdh.oeaw.ac.at/vocabs/defcthesaurus/FindsSchema> , <https://acdh.oeaw.ac.at/vocabs/defcthesaurus/FindsPotteryDecoration> ;
	skos:editorialNote "dc_finds_pottery_decoration;02" ;
	skos:broader <https://acdh.oeaw.ac.at/vocabs/defcthesaurus/monochrome/5.265> .

<https://acdh.oeaw.ac.at/vocabs/defcthesaurus/monochrome/5.265> skos:narrower <https://acdh.oeaw.ac.at/vocabs/defcthesaurus/monochrome_red/6.249> .

<https://acdh.oeaw.ac.at/vocabs/defcthesaurus/monochrome_red_(a1)/6.154> a skos:Concept ;
	skos:prefLabel "monochrome red (a1)"@en , "Monochrom rot  (A1)"@de ;
	skos:definition "Pottery painted with one color without decoration." ;
	skos:inScheme <https://acdh.oeaw.ac.at/vocabs/defcthesaurus/FindsSchema> , <https://acdh.oeaw.ac.at/vocabs/defcthesaurus/FindsPotteryDecoration> ;
	skos:editorialNote "dc_finds_pottery_decoration;02" ;
	skos:broader <https://acdh.oeaw.ac.at/vocabs/defcthesaurus/monochrome/5.265> .

<https://acdh.oeaw.ac.at/vocabs/defcthesaurus/monochrome/5.265> skos:narrower <https://acdh.oeaw.ac.at/vocabs/defcthesaurus/monochrome_red_(a1)/6.154> .

<https://acdh.oeaw.ac.at/vocabs/defcthesaurus/finds_type/1.02> dc:source "Kipfer, B. A. Dictionary of Artifacts 2007. Blackwell Publishing, Oxford.p. 329" .

<https://acdh.oeaw.ac.at/vocabs/defcthesaurus/monochrome_undecorated_(b1)/6.155> a skos:Concept ;
	skos:prefLabel "monochrome undecorated (b1)"@en , "Monochrom undekoriert (B1)"@de ;
	skos:definition "Pottery decorated with glaze-like paint. The pottery has a buff fabric decorated with a dark lustrous slip or glaze. The sauce boat and the askos are the most norable shapes." ;
	skos:inScheme <https://acdh.oeaw.ac.at/vocabs/defcthesaurus/FindsSchema> , <https://acdh.oeaw.ac.at/vocabs/defcthesaurus/FindsPotteryDecoration> ;
	skos:editorialNote "dc_finds_pottery_decoration;02" ;
	skos:broader <https://acdh.oeaw.ac.at/vocabs/defcthesaurus/monochrome/5.265> .

<https://acdh.oeaw.ac.at/vocabs/defcthesaurus/monochrome/5.265> skos:narrower <https://acdh.oeaw.ac.at/vocabs/defcthesaurus/monochrome_undecorated_(b1)/6.155> .

<https://acdh.oeaw.ac.at/vocabs/defcthesaurus/monochrome_urfirnis/6.171> a skos:Concept ;
	skos:prefLabel "monochrome urfirnis"@en , "Monochromer Urfirnis"@de ;
	skos:definition "Pottery painted with white paint on white ground." ;
	skos:inScheme <https://acdh.oeaw.ac.at/vocabs/defcthesaurus/FindsSchema> , <https://acdh.oeaw.ac.at/vocabs/defcthesaurus/FindsPotteryDecoration> ;
	skos:editorialNote "dc_finds_pottery_decoration;02" ;
	skos:broader <https://acdh.oeaw.ac.at/vocabs/defcthesaurus/monochrome/5.265> .

<https://acdh.oeaw.ac.at/vocabs/defcthesaurus/monochrome/5.265> skos:narrower <https://acdh.oeaw.ac.at/vocabs/defcthesaurus/monochrome_urfirnis/6.171> .

<https://acdh.oeaw.ac.at/vocabs/defcthesaurus/monochrome_white/6.301> a skos:Concept ;
	skos:prefLabel "monochrome white"@en , "monochrom wei"@de ;
	skos:definition "Pottery painted with yellow paint on yellow ground." ;
	skos:inScheme <https://acdh.oeaw.ac.at/vocabs/defcthesaurus/FindsSchema> , <https://acdh.oeaw.ac.at/vocabs/defcthesaurus/FindsPotteryDecoration> ;
	skos:editorialNote "dc_finds_pottery_decoration;02" ;
	skos:broader <https://acdh.oeaw.ac.at/vocabs/defcthesaurus/monochrome/5.265> .

<https://acdh.oeaw.ac.at/vocabs/defcthesaurus/monochrome/5.265> skos:narrower <https://acdh.oeaw.ac.at/vocabs/defcthesaurus/monochrome_white/6.301> .

<https://acdh.oeaw.ac.at/vocabs/defcthesaurus/monochrome_yellow/6.286> a skos:Concept ;
	skos:prefLabel "monochrome yellow"@en , "monochrom gelb"@de ;
	skos:definition "Orange ware made from well purified clay." ;
	skos:inScheme <https://acdh.oeaw.ac.at/vocabs/defcthesaurus/FindsSchema> , <https://acdh.oeaw.ac.at/vocabs/defcthesaurus/FindsPotteryDecoration> ;
	skos:editorialNote "dc_finds_pottery_decoration;02" ;
	skos:broader <https://acdh.oeaw.ac.at/vocabs/defcthesaurus/monochrome/5.265> .

<https://acdh.oeaw.ac.at/vocabs/defcthesaurus/monochrome/5.265> skos:narrower <https://acdh.oeaw.ac.at/vocabs/defcthesaurus/monochrome_yellow/6.286> .

<https://acdh.oeaw.ac.at/vocabs/defcthesaurus/orange_fine_ware/6.259> a skos:Concept ;
	skos:prefLabel "orange fine ware"@en , "orange fein Ware"@de ;
	skos:inScheme <https://acdh.oeaw.ac.at/vocabs/defcthesaurus/FindsSchema> , <https://acdh.oeaw.ac.at/vocabs/defcthesaurus/FindsPotteryDecoration> ;
	skos:editorialNote "dc_finds_pottery_decoration;02" ;
	skos:broader <https://acdh.oeaw.ac.at/vocabs/defcthesaurus/monochrome/5.265> .

<https://acdh.oeaw.ac.at/vocabs/defcthesaurus/monochrome/5.265> skos:narrower <https://acdh.oeaw.ac.at/vocabs/defcthesaurus/orange_fine_ware/6.259> .

<https://acdh.oeaw.ac.at/vocabs/defcthesaurus/pink_ware/6.273> a skos:Concept ;
	skos:prefLabel "pink ware"@en , "Rosa Ware"@de ;
	skos:definition "Ware of pink color." ;
	skos:inScheme <https://acdh.oeaw.ac.at/vocabs/defcthesaurus/FindsSchema> , <https://acdh.oeaw.ac.at/vocabs/defcthesaurus/FindsPotteryDecoration> ;
	skos:editorialNote "dc_finds_pottery_decoration;02" ;
	skos:broader <https://acdh.oeaw.ac.at/vocabs/defcthesaurus/monochrome/5.265> .

<https://acdh.oeaw.ac.at/vocabs/defcthesaurus/monochrome/5.265> skos:narrower <https://acdh.oeaw.ac.at/vocabs/defcthesaurus/pink_ware/6.273> .

<https://acdh.oeaw.ac.at/vocabs/defcthesaurus/white/6.275> a skos:Concept ;
	skos:prefLabel "white"@en , "Wei"@de ;
	skos:definition "White painted pottery decoration." ;
	skos:inScheme <https://acdh.oeaw.ac.at/vocabs/defcthesaurus/FindsSchema> , <https://acdh.oeaw.ac.at/vocabs/defcthesaurus/FindsPotteryDecoration> ;
	skos:editorialNote "dc_finds_pottery_decoration;02" ;
	skos:broader <https://acdh.oeaw.ac.at/vocabs/defcthesaurus/monochrome/5.265> .

<https://acdh.oeaw.ac.at/vocabs/defcthesaurus/monochrome/5.265> skos:narrower <https://acdh.oeaw.ac.at/vocabs/defcthesaurus/white/6.275> .

<https://acdh.oeaw.ac.at/vocabs/defcthesaurus/pottery_surface_treatment/3.019> a skos:Concept ;
	skos:prefLabel "pottery surface treatment"@en , "Oberfl채chenbehandlung"@de ;
	skos:inScheme <https://acdh.oeaw.ac.at/vocabs/defcthesaurus/FindsSchema> , <https://acdh.oeaw.ac.at/vocabs/defcthesaurus/NotInDatabase> ;
	skos:editorialNote "dc_not_in_database;019" ;
	skos:broader <https://acdh.oeaw.ac.at/vocabs/defcthesaurus/pottery/2.4> .

<https://acdh.oeaw.ac.at/vocabs/defcthesaurus/pottery/2.4> skos:narrower <https://acdh.oeaw.ac.at/vocabs/defcthesaurus/pottery_surface_treatment/3.019> .

<https://acdh.oeaw.ac.at/vocabs/defcthesaurus/burnished/4.297> a skos:Concept ;
	skos:prefLabel "burnished"@en , "Gegl채ttet"@de ;
	skos:definition "Surface treatment of rubbing and smooting the surface of a vessel when it is leather-hard (before firing) with a hard tool made out of wood, stone or bone in order to obtain a bright, even, compact, and non-porous surface." ;
	skos:inScheme <https://acdh.oeaw.ac.at/vocabs/defcthesaurus/FindsSchema> , <https://acdh.oeaw.ac.at/vocabs/defcthesaurus/FindsPotteryDecoration> ;
	skos:editorialNote "dc_finds_pottery_decoration;297" ;
	skos:broader <https://acdh.oeaw.ac.at/vocabs/defcthesaurus/pottery_surface_treatment/3.019> .

<https://acdh.oeaw.ac.at/vocabs/defcthesaurus/pottery_surface_treatment/3.019> skos:narrower <https://acdh.oeaw.ac.at/vocabs/defcthesaurus/burnished/4.297> .

<https://acdh.oeaw.ac.at/vocabs/defcthesaurus/black_burnished/5.271> a skos:Concept ;
	skos:prefLabel "black burnished"@en , "Schwarz gegl채ttet"@de ;
	skos:definition "Burnished black ware." ;
	skos:inScheme <https://acdh.oeaw.ac.at/vocabs/defcthesaurus/FindsSchema> , <https://acdh.oeaw.ac.at/vocabs/defcthesaurus/FindsPotteryDecoration> ;
	skos:editorialNote "dc_finds_pottery_decoration;271" ;
	skos:broader <https://acdh.oeaw.ac.at/vocabs/defcthesaurus/burnished/4.297> .

<https://acdh.oeaw.ac.at/vocabs/defcthesaurus/burnished/4.297> skos:narrower <https://acdh.oeaw.ac.at/vocabs/defcthesaurus/black_burnished/5.271> .

<https://acdh.oeaw.ac.at/vocabs/defcthesaurus/black_burnished_larisa_(款1慣)/5.141> a skos:Concept ;
	skos:prefLabel "black burnished larisa (款1慣)"@en , "Schwarz gegl채ttet Larisa (C1a A5a/c)"@de ;
	skos:definition "Burnished black ware type \"Larisa\" named after the site in Greece." ;
	skos:inScheme <https://acdh.oeaw.ac.at/vocabs/defcthesaurus/FindsSchema> , <https://acdh.oeaw.ac.at/vocabs/defcthesaurus/FindsPotteryDecoration> ;
	skos:editorialNote "dc_finds_pottery_decoration;141" ;
	skos:broader <https://acdh.oeaw.ac.at/vocabs/defcthesaurus/burnished/4.297> .

<https://acdh.oeaw.ac.at/vocabs/defcthesaurus/burnished/4.297> skos:narrower <https://acdh.oeaw.ac.at/vocabs/defcthesaurus/black_burnished_larisa_(款1慣)/5.141> .

<https://acdh.oeaw.ac.at/vocabs/defcthesaurus/black_burnished_with_channeled_decoration_(款1慣3)/5.142> a skos:Concept ;
	skos:prefLabel "black burnished with channeled decoration (款1慣3)"@en , "Schwarz gegl채ttet, kanneliert  (C1a3)"@de ;
	skos:definition "Burnished black ware with channeled/fluted decoration." ;
	skos:inScheme <https://acdh.oeaw.ac.at/vocabs/defcthesaurus/FindsSchema> , <https://acdh.oeaw.ac.at/vocabs/defcthesaurus/FindsPotteryDecoration> ;
	skos:editorialNote "dc_finds_pottery_decoration;142" ;
	skos:broader <https://acdh.oeaw.ac.at/vocabs/defcthesaurus/burnished/4.297> .

<https://acdh.oeaw.ac.at/vocabs/defcthesaurus/burnished/4.297> skos:narrower <https://acdh.oeaw.ac.at/vocabs/defcthesaurus/black_burnished_with_channeled_decoration_(款1慣3)/5.142> .

<https://acdh.oeaw.ac.at/vocabs/defcthesaurus/black_burnished_with_white_paint_(款1慣1)/5.143> a skos:Concept ;
	skos:prefLabel "black burnished with white paint (款1慣1)"@en , "Schwarz gegl채ttet mit weier Bemalung (C1a1)"@de ;
	skos:definition "Burnished black ware decorated with white paint." ;
	skos:inScheme <https://acdh.oeaw.ac.at/vocabs/defcthesaurus/FindsSchema> , <https://acdh.oeaw.ac.at/vocabs/defcthesaurus/FindsPotteryDecoration> ;
	skos:editorialNote "dc_finds_pottery_decoration;143" ;
	skos:broader <https://acdh.oeaw.ac.at/vocabs/defcthesaurus/burnished/4.297> .

<https://acdh.oeaw.ac.at/vocabs/defcthesaurus/burnished/4.297> skos:narrower <https://acdh.oeaw.ac.at/vocabs/defcthesaurus/black_burnished_with_white_paint_(款1慣1)/5.143> .

<https://acdh.oeaw.ac.at/vocabs/defcthesaurus/black_pattern_burnished_(款1慣2)/5.146> a skos:Concept ;
	skos:prefLabel "black pattern burnished (款1慣2)"@en , "Schwarz mustergegl채ttet  (C1a2)"@de ;
	skos:altLabel "Politurmuster"@de ;
	skos:definition "Black ware decorated with burnished patterns, normally the inside of the open bowls." ;
	skos:inScheme <https://acdh.oeaw.ac.at/vocabs/defcthesaurus/FindsSchema> , <https://acdh.oeaw.ac.at/vocabs/defcthesaurus/FindsPotteryDecoration> ;
	skos:editorialNote "dc_finds_pottery_decoration;146" ;
	skos:broader <https://acdh.oeaw.ac.at/vocabs/defcthesaurus/burnished/4.297> .

<https://acdh.oeaw.ac.at/vocabs/defcthesaurus/burnished/4.297> skos:narrower <https://acdh.oeaw.ac.at/vocabs/defcthesaurus/black_pattern_burnished_(款1慣2)/5.146> .

<https://acdh.oeaw.ac.at/vocabs/defcthesaurus/black/red_burnished_arapi/5.307> a skos:Concept ;
	skos:prefLabel "black/red burnished arapi"@en , "schwarz/rot gegl채ttet Arapi"@de ;
	skos:definition "Burnished ware with red respectively black interior respectively exterior surface typical for Thessaly." ;
	skos:inScheme <https://acdh.oeaw.ac.at/vocabs/defcthesaurus/FindsSchema> , <https://acdh.oeaw.ac.at/vocabs/defcthesaurus/FindsPotteryDecoration> ;
	skos:editorialNote "dc_finds_pottery_decoration;307" ;
	skos:broader <https://acdh.oeaw.ac.at/vocabs/defcthesaurus/burnished/4.297> .

<https://acdh.oeaw.ac.at/vocabs/defcthesaurus/burnished/4.297> skos:narrower <https://acdh.oeaw.ac.at/vocabs/defcthesaurus/black/red_burnished_arapi/5.307> .

<https://acdh.oeaw.ac.at/vocabs/defcthesaurus/brown_burnished/5.120> a skos:Concept ;
	skos:prefLabel "brown burnished"@en , "Braun gegl채ttet"@de ;
	skos:altLabel "BBW"@en ;
	skos:definition "Burnished brown ware." ;
	skos:inScheme <https://acdh.oeaw.ac.at/vocabs/defcthesaurus/FindsSchema> , <https://acdh.oeaw.ac.at/vocabs/defcthesaurus/FindsPotteryDecoration> ;
	skos:editorialNote "dc_finds_pottery_decoration;120" ;
	skos:broader <https://acdh.oeaw.ac.at/vocabs/defcthesaurus/burnished/4.297> .

<https://acdh.oeaw.ac.at/vocabs/defcthesaurus/burnished/4.297> skos:narrower <https://acdh.oeaw.ac.at/vocabs/defcthesaurus/brown_burnished/5.120> .

<https://acdh.oeaw.ac.at/vocabs/defcthesaurus/dark_faced_burished_ware_(dfbw)/5.247> a skos:Concept ;
	skos:prefLabel "dark faced burished ware (dfbw)"@en , "Gegl채ttete Keramik mit dunklem berzug"@de ;
	skos:definition "Burnished ware decorated with dark slip." ;
	skos:inScheme <https://acdh.oeaw.ac.at/vocabs/defcthesaurus/FindsSchema> , <https://acdh.oeaw.ac.at/vocabs/defcthesaurus/FindsPotteryDecoration> ;
	skos:editorialNote "dc_finds_pottery_decoration;247" ;
	skos:broader <https://acdh.oeaw.ac.at/vocabs/defcthesaurus/burnished/4.297> .

<https://acdh.oeaw.ac.at/vocabs/defcthesaurus/burnished/4.297> skos:narrower <https://acdh.oeaw.ac.at/vocabs/defcthesaurus/dark_faced_burished_ware_(dfbw)/5.247> .

<https://acdh.oeaw.ac.at/vocabs/defcthesaurus/grey_burnished/5.289> a skos:Concept ;
	skos:prefLabel "grey burnished"@en , "grau gegl채ttet"@de ;
	skos:definition "Burnished ware with fine grey surface typical for Thessaly." ;
	skos:inScheme <https://acdh.oeaw.ac.at/vocabs/defcthesaurus/FindsSchema> , <https://acdh.oeaw.ac.at/vocabs/defcthesaurus/FindsPotteryDecoration> ;
	skos:editorialNote "dc_finds_pottery_decoration;289" ;
	skos:broader <https://acdh.oeaw.ac.at/vocabs/defcthesaurus/burnished/4.297> .

<https://acdh.oeaw.ac.at/vocabs/defcthesaurus/burnished/4.297> skos:narrower <https://acdh.oeaw.ac.at/vocabs/defcthesaurus/grey_burnished/5.289> .

<https://acdh.oeaw.ac.at/vocabs/defcthesaurus/monochrome_burnished/5.170> a skos:Concept ;
	skos:prefLabel "monochrome burnished"@en , "Monochrom gegl채ttet"@de ;
	skos:definition "Burnished pottery painted with one color." ;
	skos:inScheme <https://acdh.oeaw.ac.at/vocabs/defcthesaurus/FindsSchema> , <https://acdh.oeaw.ac.at/vocabs/defcthesaurus/FindsPotteryDecoration> ;
	skos:editorialNote "dc_finds_pottery_decoration;170" ;
	skos:broader <https://acdh.oeaw.ac.at/vocabs/defcthesaurus/burnished/4.297> .

<https://acdh.oeaw.ac.at/vocabs/defcthesaurus/burnished/4.297> skos:narrower <https://acdh.oeaw.ac.at/vocabs/defcthesaurus/monochrome_burnished/5.170> .

<https://acdh.oeaw.ac.at/vocabs/defcthesaurus/pattern_burnished/5.131> a skos:Concept ;
	skos:prefLabel "pattern burnished"@en , "Politurmusterverziert"@de ;
	skos:definition "Pottery decorated by burnished patterns." ;
	skos:inScheme <https://acdh.oeaw.ac.at/vocabs/defcthesaurus/FindsSchema> , <https://acdh.oeaw.ac.at/vocabs/defcthesaurus/FindsPotteryDecoration> ;
	skos:editorialNote "dc_finds_pottery_decoration;131" ;
	skos:broader <https://acdh.oeaw.ac.at/vocabs/defcthesaurus/burnished/4.297> .

<https://acdh.oeaw.ac.at/vocabs/defcthesaurus/burnished/4.297> skos:narrower <https://acdh.oeaw.ac.at/vocabs/defcthesaurus/pattern_burnished/5.131> .

<https://acdh.oeaw.ac.at/vocabs/defcthesaurus/polychrome_burnished/5.243> a skos:Concept ;
	skos:prefLabel "polychrome burnished"@en , "Polychrom gegl채ttet"@de ;
	skos:definition "Pottery painted with more than two colors and polished before firing." ;
	skos:inScheme <https://acdh.oeaw.ac.at/vocabs/defcthesaurus/FindsSchema> , <https://acdh.oeaw.ac.at/vocabs/defcthesaurus/FindsPotteryDecoration> ;
	skos:editorialNote "dc_finds_pottery_decoration;243" ;
	skos:broader <https://acdh.oeaw.ac.at/vocabs/defcthesaurus/burnished/4.297> .

<https://acdh.oeaw.ac.at/vocabs/defcthesaurus/burnished/4.297> skos:narrower <https://acdh.oeaw.ac.at/vocabs/defcthesaurus/polychrome_burnished/5.243> .

<https://acdh.oeaw.ac.at/vocabs/defcthesaurus/red_burnished/5.248> a skos:Concept ;
	skos:prefLabel "red burnished"@en , "Rot gegl채ttet"@de ;
	skos:definition "The red slip was applied onto the vessel and burnished." ;
	skos:inScheme <https://acdh.oeaw.ac.at/vocabs/defcthesaurus/FindsSchema> , <https://acdh.oeaw.ac.at/vocabs/defcthesaurus/FindsPotteryDecoration> ;
	skos:editorialNote "dc_finds_pottery_decoration;248" ;
	skos:broader <https://acdh.oeaw.ac.at/vocabs/defcthesaurus/burnished/4.297> .

<https://acdh.oeaw.ac.at/vocabs/defcthesaurus/burnished/4.297> skos:narrower <https://acdh.oeaw.ac.at/vocabs/defcthesaurus/red_burnished/5.248> .

<https://acdh.oeaw.ac.at/vocabs/defcthesaurus/red_burnished_(b1)/5.156> a skos:Concept ;
	skos:prefLabel "red burnished (b1)"@en , "Rot gegl채ttet (B1)"@de ;
	skos:definition "The red slip was applied onto the vessel and burnished." ;
	skos:inScheme <https://acdh.oeaw.ac.at/vocabs/defcthesaurus/FindsSchema> , <https://acdh.oeaw.ac.at/vocabs/defcthesaurus/FindsPotteryDecoration> ;
	skos:editorialNote "dc_finds_pottery_decoration;156" ;
	skos:broader <https://acdh.oeaw.ac.at/vocabs/defcthesaurus/burnished/4.297> .

<https://acdh.oeaw.ac.at/vocabs/defcthesaurus/burnished/4.297> skos:narrower <https://acdh.oeaw.ac.at/vocabs/defcthesaurus/red_burnished_(b1)/5.156> .

<https://acdh.oeaw.ac.at/vocabs/defcthesaurus/rippled_burnished/5.231> a skos:Concept ;
	skos:prefLabel "rippled burnished"@en , "Wellig gegl채ttet"@de ;
	skos:altLabel "rippled"@de ;
	skos:definition "A technique of pottery burnish in which the whole surface is worked into ripples, in extreme examples it approaches fluting." ;
	skos:inScheme <https://acdh.oeaw.ac.at/vocabs/defcthesaurus/FindsSchema> , <https://acdh.oeaw.ac.at/vocabs/defcthesaurus/FindsPotteryDecoration> ;
	skos:editorialNote "dc_finds_pottery_decoration;231" ;
	skos:broader <https://acdh.oeaw.ac.at/vocabs/defcthesaurus/burnished/4.297> .

<https://acdh.oeaw.ac.at/vocabs/defcthesaurus/burnished/4.297> skos:narrower <https://acdh.oeaw.ac.at/vocabs/defcthesaurus/rippled_burnished/5.231> .

<https://acdh.oeaw.ac.at/vocabs/defcthesaurus/scribble_burnished/5.234> a skos:Concept ;
	skos:prefLabel "scribble burnished"@en , "Geschmiergegl채ttet"@de ;
	skos:definition "MN Urfirnis ware with irregular burnishing lines typical for Southern Greece." ;
	skos:inScheme <https://acdh.oeaw.ac.at/vocabs/defcthesaurus/FindsSchema> , <https://acdh.oeaw.ac.at/vocabs/defcthesaurus/FindsPotteryDecoration> ;
	skos:editorialNote "dc_finds_pottery_decoration;234" ;
	skos:broader <https://acdh.oeaw.ac.at/vocabs/defcthesaurus/burnished/4.297> .

<https://acdh.oeaw.ac.at/vocabs/defcthesaurus/burnished/4.297> skos:narrower <https://acdh.oeaw.ac.at/vocabs/defcthesaurus/scribble_burnished/5.234> .

<https://acdh.oeaw.ac.at/vocabs/defcthesaurus/stroke-and_pattern_burnished/5.178> a skos:Concept ;
	skos:prefLabel "stroke-and pattern burnished"@en , "Strich- und mustergegl채ttet"@de ;
	skos:altLabel "Pattern-burnished"@de , "stroke-burnished"@de ;
	skos:definition "Pottery decorated with network patterns. In stroke burnish, the surface is completey polished, but the marks of the burnished, a pebble or bone slip, remain distinct." ;
	skos:inScheme <https://acdh.oeaw.ac.at/vocabs/defcthesaurus/FindsSchema> , <https://acdh.oeaw.ac.at/vocabs/defcthesaurus/FindsPotteryDecoration> ;
	skos:editorialNote "dc_finds_pottery_decoration;178" ;
	skos:broader <https://acdh.oeaw.ac.at/vocabs/defcthesaurus/burnished/4.297> .

<https://acdh.oeaw.ac.at/vocabs/defcthesaurus/burnished/4.297> skos:narrower <https://acdh.oeaw.ac.at/vocabs/defcthesaurus/stroke-and_pattern_burnished/5.178> .

<https://acdh.oeaw.ac.at/vocabs/defcthesaurus/pottery/2.4> dc:source "Kipfer, B. A. Dictionary of Artifacts 2007. Blackwell Publishing, Oxford.p 264" .

<https://acdh.oeaw.ac.at/vocabs/defcthesaurus/black_slipped/4.258> a skos:Concept ;
	skos:prefLabel "black slipped"@en , "schwarzer berzug"@de ;
	skos:definition "Any pottery to which a slip, a thin layer of fine clay, is applied to pottery before firing by dipping the pot into a thick liquid mixture of clay and water. Slip decorates the fabric, is often chosen to bake to a color such as red and makes the pot more" ;
	skos:inScheme <https://acdh.oeaw.ac.at/vocabs/defcthesaurus/FindsSchema> , <https://acdh.oeaw.ac.at/vocabs/defcthesaurus/FindsPotteryDecoration> ;
	skos:editorialNote "dc_finds_pottery_decoration;258" ;
	skos:broader <https://acdh.oeaw.ac.at/vocabs/defcthesaurus/pottery_surface_treatment/3.019> .

<https://acdh.oeaw.ac.at/vocabs/defcthesaurus/pottery_surface_treatment/3.019> skos:narrower <https://acdh.oeaw.ac.at/vocabs/defcthesaurus/black_slipped/4.258> .

<https://acdh.oeaw.ac.at/vocabs/defcthesaurus/black_topped/4.242> a skos:Concept ;
	skos:prefLabel "black topped"@en , "Black topped"@de ;
	skos:definition "Pottery with blackened rim, that was most likely added after firing in the kiln." ;
	skos:inScheme <https://acdh.oeaw.ac.at/vocabs/defcthesaurus/FindsSchema> , <https://acdh.oeaw.ac.at/vocabs/defcthesaurus/FindsPotteryDecoration> ;
	skos:editorialNote "dc_finds_pottery_decoration;242" ;
	skos:broader <https://acdh.oeaw.ac.at/vocabs/defcthesaurus/pottery_surface_treatment/3.019> .

<https://acdh.oeaw.ac.at/vocabs/defcthesaurus/pottery_surface_treatment/3.019> skos:narrower <https://acdh.oeaw.ac.at/vocabs/defcthesaurus/black_topped/4.242> .

<https://acdh.oeaw.ac.at/vocabs/defcthesaurus/brushed/4.213> a skos:Concept ;
	skos:prefLabel "brushed"@en , "Geb체rstet"@de ;
	skos:definition "Pottery with brushed surface." ;
	skos:inScheme <https://acdh.oeaw.ac.at/vocabs/defcthesaurus/FindsSchema> , <https://acdh.oeaw.ac.at/vocabs/defcthesaurus/FindsPotteryDecoration> ;
	skos:editorialNote "dc_finds_pottery_decoration;213" ;
	skos:broader <https://acdh.oeaw.ac.at/vocabs/defcthesaurus/pottery_surface_treatment/3.019> .

<https://acdh.oeaw.ac.at/vocabs/defcthesaurus/pottery_surface_treatment/3.019> skos:narrower <https://acdh.oeaw.ac.at/vocabs/defcthesaurus/brushed/4.213> .

<https://acdh.oeaw.ac.at/vocabs/defcthesaurus/coarse/4.252> a skos:Concept ;
	skos:prefLabel "coarse"@en , "grob"@de ;
	skos:altLabel "coarse ware"@en ;
	skos:definition "Sherds or vessels with a coarser appearance that is achieved throzgh thicker walls, large-sized grit inclusions and the absence of careful surface treatment." ;
	skos:inScheme <https://acdh.oeaw.ac.at/vocabs/defcthesaurus/FindsSchema> , <https://acdh.oeaw.ac.at/vocabs/defcthesaurus/FindsPotteryDecoration> ;
	skos:editorialNote "dc_finds_pottery_decoration;252" ;
	skos:broader <https://acdh.oeaw.ac.at/vocabs/defcthesaurus/pottery_surface_treatment/3.019> .

<https://acdh.oeaw.ac.at/vocabs/defcthesaurus/pottery_surface_treatment/3.019> skos:narrower <https://acdh.oeaw.ac.at/vocabs/defcthesaurus/coarse/4.252> .

<https://acdh.oeaw.ac.at/vocabs/defcthesaurus/pottery/2.4> dc:source "Keighley 1986, 364" .

<https://acdh.oeaw.ac.at/vocabs/defcthesaurus/gray_lustre/4.195> a skos:Concept ;
	skos:prefLabel "gray lustre"@en , "Grauer Glanzton"@de ;
	skos:definition "Smoothed ware with soapy grey surface typical for Eastern Macedonia, Sitagroi." ;
	skos:inScheme <https://acdh.oeaw.ac.at/vocabs/defcthesaurus/FindsSchema> , <https://acdh.oeaw.ac.at/vocabs/defcthesaurus/FindsPotteryDecoration> ;
	skos:editorialNote "dc_finds_pottery_decoration;195" ;
	skos:broader <https://acdh.oeaw.ac.at/vocabs/defcthesaurus/pottery_surface_treatment/3.019> .

<https://acdh.oeaw.ac.at/vocabs/defcthesaurus/pottery_surface_treatment/3.019> skos:narrower <https://acdh.oeaw.ac.at/vocabs/defcthesaurus/gray_lustre/4.195> .

<https://acdh.oeaw.ac.at/vocabs/defcthesaurus/patterned_urfirnis/4.173> a skos:Concept ;
	skos:prefLabel "patterned urfirnis"@en , "Musterverzierter Urfirnis"@de ;
	skos:definition "Pattern painted decoration with loustrous paint." ;
	skos:inScheme <https://acdh.oeaw.ac.at/vocabs/defcthesaurus/FindsSchema> , <https://acdh.oeaw.ac.at/vocabs/defcthesaurus/FindsPotteryDecoration> ;
	skos:editorialNote "dc_finds_pottery_decoration;173" ;
	skos:broader <https://acdh.oeaw.ac.at/vocabs/defcthesaurus/pottery_surface_treatment/3.019> .

<https://acdh.oeaw.ac.at/vocabs/defcthesaurus/pottery_surface_treatment/3.019> skos:narrower <https://acdh.oeaw.ac.at/vocabs/defcthesaurus/patterned_urfirnis/4.173> .

<https://acdh.oeaw.ac.at/vocabs/defcthesaurus/polished/4.228> a skos:Concept ;
	skos:prefLabel "polished"@en , "Poliert"@de ;
	skos:definition "Sufficiently dry ceramics in leather-hard stage is polished to compact its surface resulting in evenly smooth pottery." ;
	skos:inScheme <https://acdh.oeaw.ac.at/vocabs/defcthesaurus/FindsSchema> , <https://acdh.oeaw.ac.at/vocabs/defcthesaurus/FindsPotteryDecoration> ;
	skos:editorialNote "dc_finds_pottery_decoration;228" ;
	skos:broader <https://acdh.oeaw.ac.at/vocabs/defcthesaurus/pottery_surface_treatment/3.019> .

<https://acdh.oeaw.ac.at/vocabs/defcthesaurus/pottery_surface_treatment/3.019> skos:narrower <https://acdh.oeaw.ac.at/vocabs/defcthesaurus/polished/4.228> .

<https://acdh.oeaw.ac.at/vocabs/defcthesaurus/pottery/2.4> dc:source "Kipfer, B. A. Dictionary of Artifacts 2007. Blackwell Publishing, Oxford.p 271" .

<https://acdh.oeaw.ac.at/vocabs/defcthesaurus/rippled/4.177> a skos:Concept ;
	skos:prefLabel "rippled"@en , "Wellig"@de ;
	skos:altLabel "ripple burnished"@de ;
	skos:definition "A technique of pottery burnish in which the whole surface is worked into ripples, in extreme examples it approaches fluting." ;
	skos:inScheme <https://acdh.oeaw.ac.at/vocabs/defcthesaurus/FindsSchema> , <https://acdh.oeaw.ac.at/vocabs/defcthesaurus/FindsPotteryDecoration> ;
	skos:editorialNote "dc_finds_pottery_decoration;177" ;
	skos:broader <https://acdh.oeaw.ac.at/vocabs/defcthesaurus/pottery_surface_treatment/3.019> .

<https://acdh.oeaw.ac.at/vocabs/defcthesaurus/pottery_surface_treatment/3.019> skos:narrower <https://acdh.oeaw.ac.at/vocabs/defcthesaurus/rippled/4.177> .

<https://acdh.oeaw.ac.at/vocabs/defcthesaurus/slipped/4.302> a skos:Concept ;
	skos:prefLabel "slipped"@en , "Ware mit berzug"@de ;
	skos:altLabel "slip ware"@de ;
	skos:definition "Surface treatment of applying the slip (or coat) as a suspension of clay in water. It can be applied once or several times to the surface of the vessel with a brush, naked hand or a piece of cloth by dipping or pouring. It is applied to change the surface" ;
	skos:inScheme <https://acdh.oeaw.ac.at/vocabs/defcthesaurus/FindsSchema> , <https://acdh.oeaw.ac.at/vocabs/defcthesaurus/FindsPotteryDecoration> ;
	skos:editorialNote "dc_finds_pottery_decoration;302" ;
	skos:broader <https://acdh.oeaw.ac.at/vocabs/defcthesaurus/pottery_surface_treatment/3.019> .

<https://acdh.oeaw.ac.at/vocabs/defcthesaurus/pottery_surface_treatment/3.019> skos:narrower <https://acdh.oeaw.ac.at/vocabs/defcthesaurus/slipped/4.302> .

<https://acdh.oeaw.ac.at/vocabs/defcthesaurus/red_slipped/5.134> a skos:Concept ;
	skos:prefLabel "red slipped"@en , "Ware mit rotem berzug"@de ;
	skos:definition "Any pottery to which a slip, a thin layer of fine clay, is applied to pottery before firing by dipping the pot into a thick liquid mixture of clay and water. Slip decorates the fabric, is often chosen to bake to a color such as red and makes the pot more" ;
	skos:inScheme <https://acdh.oeaw.ac.at/vocabs/defcthesaurus/FindsSchema> , <https://acdh.oeaw.ac.at/vocabs/defcthesaurus/FindsPotteryDecoration> ;
	skos:editorialNote "dc_finds_pottery_decoration;134" ;
	skos:broader <https://acdh.oeaw.ac.at/vocabs/defcthesaurus/slipped/4.302> .

<https://acdh.oeaw.ac.at/vocabs/defcthesaurus/slipped/4.302> skos:narrower <https://acdh.oeaw.ac.at/vocabs/defcthesaurus/red_slipped/5.134> .

<https://acdh.oeaw.ac.at/vocabs/defcthesaurus/pottery/2.4> dc:source "http://www.ime.gr/chronos/01/en/nl/mn/mn_potfr.html" .

<https://acdh.oeaw.ac.at/vocabs/defcthesaurus/scraped_(a3琯)/4.159> a skos:Concept ;
	skos:prefLabel "scraped (a3琯)"@en , "Ausgewischt (A3e)"@de ;
	skos:definition "The whitish surface of the vessel is covered completely with a red colour, from which parallel bands are then scraped off. Typical for Thessaly and central Greece." ;
	skos:inScheme <https://acdh.oeaw.ac.at/vocabs/defcthesaurus/FindsSchema> , <https://acdh.oeaw.ac.at/vocabs/defcthesaurus/FindsPotteryDecoration> ;
	skos:editorialNote "dc_finds_pottery_decoration;159" ;
	skos:broader <https://acdh.oeaw.ac.at/vocabs/defcthesaurus/pottery_surface_treatment/3.019> .

<https://acdh.oeaw.ac.at/vocabs/defcthesaurus/pottery_surface_treatment/3.019> skos:narrower <https://acdh.oeaw.ac.at/vocabs/defcthesaurus/scraped_(a3琯)/4.159> .

<https://acdh.oeaw.ac.at/vocabs/defcthesaurus/smeared/4.260> a skos:Concept ;
	skos:prefLabel "smeared"@en , "Geschmiert"@de ;
	skos:altLabel "smooth ware"@de ;
	skos:definition "Middle Helladic smeared ware." ;
	skos:inScheme <https://acdh.oeaw.ac.at/vocabs/defcthesaurus/FindsSchema> , <https://acdh.oeaw.ac.at/vocabs/defcthesaurus/FindsPotteryDecoration> ;
	skos:editorialNote "dc_finds_pottery_decoration;260" ;
	skos:broader <https://acdh.oeaw.ac.at/vocabs/defcthesaurus/pottery_surface_treatment/3.019> .

<https://acdh.oeaw.ac.at/vocabs/defcthesaurus/pottery_surface_treatment/3.019> skos:narrower <https://acdh.oeaw.ac.at/vocabs/defcthesaurus/smeared/4.260> .

<https://acdh.oeaw.ac.at/vocabs/defcthesaurus/pottery/2.4> dc:source "Horvat, M. 1999, Keramika. Tehnologija keramike, tipologija lon철enine, kerami철ni arhiv. Filozofska fakulteta, Ljubljana. P. 25" .

<https://acdh.oeaw.ac.at/vocabs/defcthesaurus/smoothed/4.261> a skos:Concept ;
	skos:prefLabel "smoothed"@en , "Glatt gestrichen"@de ;
	skos:definition "Vessel that has been smoothed when still wet before drying and firing. The surface is wiped without additional use of water. Traces of wiping direction can be often observed." ;
	skos:inScheme <https://acdh.oeaw.ac.at/vocabs/defcthesaurus/FindsSchema> , <https://acdh.oeaw.ac.at/vocabs/defcthesaurus/FindsPotteryDecoration> ;
	skos:editorialNote "dc_finds_pottery_decoration;261" ;
	skos:broader <https://acdh.oeaw.ac.at/vocabs/defcthesaurus/pottery_surface_treatment/3.019> .

<https://acdh.oeaw.ac.at/vocabs/defcthesaurus/pottery_surface_treatment/3.019> skos:narrower <https://acdh.oeaw.ac.at/vocabs/defcthesaurus/smoothed/4.261> .

<https://acdh.oeaw.ac.at/vocabs/defcthesaurus/pottery/2.4> dc:source "Biers, W. R. 1969. Excavations at Phlius, 1924 the prehistoric deposits. Hesperia: The journal of the American School of Classical Studies at Athens. Vol. 38, No.4. pp. 443-458. P. 446" .

<https://acdh.oeaw.ac.at/vocabs/defcthesaurus/spongy/4.244> a skos:Concept ;
	skos:prefLabel "spongy"@en , "Spongy"@de ;
	skos:altLabel "spongy ware"@de ;
	skos:definition "The fabric of a spongy vessel is quite coarse and contains many inclusions of limestone and plant matter which exploded or burnt out upon firing, leaving the surface pitted." ;
	skos:inScheme <https://acdh.oeaw.ac.at/vocabs/defcthesaurus/FindsSchema> , <https://acdh.oeaw.ac.at/vocabs/defcthesaurus/FindsPotteryDecoration> ;
	skos:editorialNote "dc_finds_pottery_decoration;244" ;
	skos:broader <https://acdh.oeaw.ac.at/vocabs/defcthesaurus/pottery_surface_treatment/3.019> .

<https://acdh.oeaw.ac.at/vocabs/defcthesaurus/pottery_surface_treatment/3.019> skos:narrower <https://acdh.oeaw.ac.at/vocabs/defcthesaurus/spongy/4.244> .

<https://acdh.oeaw.ac.at/vocabs/defcthesaurus/unburnished/4.135> a skos:Concept ;
	skos:prefLabel "unburnished"@en , "Ungegl채ttet"@de ;
	skos:definition "A vessle that was not polished with a dull surface." ;
	skos:inScheme <https://acdh.oeaw.ac.at/vocabs/defcthesaurus/FindsSchema> , <https://acdh.oeaw.ac.at/vocabs/defcthesaurus/FindsPotteryDecoration> ;
	skos:editorialNote "dc_finds_pottery_decoration;135" ;
	skos:broader <https://acdh.oeaw.ac.at/vocabs/defcthesaurus/pottery_surface_treatment/3.019> .

<https://acdh.oeaw.ac.at/vocabs/defcthesaurus/pottery_surface_treatment/3.019> skos:narrower <https://acdh.oeaw.ac.at/vocabs/defcthesaurus/unburnished/4.135> .

<https://acdh.oeaw.ac.at/vocabs/defcthesaurus/wiped/4.237> a skos:Concept ;
	skos:prefLabel "wiped"@en , "Ausgewischt"@de ;
	skos:definition "Wiped surface." ;
	skos:inScheme <https://acdh.oeaw.ac.at/vocabs/defcthesaurus/FindsSchema> , <https://acdh.oeaw.ac.at/vocabs/defcthesaurus/FindsPotteryDecoration> ;
	skos:editorialNote "dc_finds_pottery_decoration;237" ;
	skos:broader <https://acdh.oeaw.ac.at/vocabs/defcthesaurus/pottery_surface_treatment/3.019> .

<https://acdh.oeaw.ac.at/vocabs/defcthesaurus/pottery_surface_treatment/3.019> skos:narrower <https://acdh.oeaw.ac.at/vocabs/defcthesaurus/wiped/4.237> .

<https://acdh.oeaw.ac.at/vocabs/defcthesaurus/topped/4.035> a skos:Concept ;
	skos:prefLabel "topped"@en ;
	skos:inScheme <https://acdh.oeaw.ac.at/vocabs/defcthesaurus/FindsSchema> , <https://acdh.oeaw.ac.at/vocabs/defcthesaurus/NotInDatabase> ;
	skos:editorialNote "dc_not_in_database;035" ;
	skos:broader <https://acdh.oeaw.ac.at/vocabs/defcthesaurus/pottery_surface_treatment/3.019> .

<https://acdh.oeaw.ac.at/vocabs/defcthesaurus/pottery_surface_treatment/3.019> skos:narrower <https://acdh.oeaw.ac.at/vocabs/defcthesaurus/topped/4.035> .

<https://acdh.oeaw.ac.at/vocabs/defcthesaurus/red_topped/5.284> a skos:Concept ;
	skos:prefLabel "red topped"@en , "red topped"@de ;
	skos:altLabel "Red-topped"@de ;
	skos:definition "Burnished ware with red oxidized rim and black surface typical for Northern Greece." ;
	skos:inScheme <https://acdh.oeaw.ac.at/vocabs/defcthesaurus/FindsSchema> , <https://acdh.oeaw.ac.at/vocabs/defcthesaurus/FindsPotteryDecoration> ;
	skos:editorialNote "dc_finds_pottery_decoration;284" ;
	skos:broader <https://acdh.oeaw.ac.at/vocabs/defcthesaurus/topped/4.035> .

<https://acdh.oeaw.ac.at/vocabs/defcthesaurus/topped/4.035> skos:narrower <https://acdh.oeaw.ac.at/vocabs/defcthesaurus/red_topped/5.284> .

<https://acdh.oeaw.ac.at/vocabs/defcthesaurus/white_topped/5.285> a skos:Concept ;
	skos:prefLabel "white topped"@en , "white topped"@de ;
	skos:definition "Ware with white crusted rim typical for Thessaly." ;
	skos:inScheme <https://acdh.oeaw.ac.at/vocabs/defcthesaurus/FindsSchema> , <https://acdh.oeaw.ac.at/vocabs/defcthesaurus/FindsPotteryDecoration> ;
	skos:editorialNote "dc_finds_pottery_decoration;285" ;
	skos:broader <https://acdh.oeaw.ac.at/vocabs/defcthesaurus/topped/4.035> .

<https://acdh.oeaw.ac.at/vocabs/defcthesaurus/topped/4.035> skos:narrower <https://acdh.oeaw.ac.at/vocabs/defcthesaurus/white_topped/5.285> .
