@prefix dc: <http://purl.org/dc/elements/1.1/> .
@prefix foaf: <http://xmlns.com/foaf/0.1/> .
@prefix owl: <http://www.w3.org/2002/07/owl#> .
@prefix rdf: <http://www.w3.org/1999/02/22-rdf-syntax-ns#> .
@prefix rdfs: <http://www.w3.org/2000/01/rdf-schema#> .
@prefix skos: <http://www.w3.org/2004/02/skos/core#> .
@prefix xml: <http://www.w3.org/XML/1998/namespace> .
@prefix xsd: <http://www.w3.org/2001/XMLSchema#> .

<http://id.acdh.oeaw.ac.at/defc/thesaurus/PeriodDatedby> a skos:ConceptScheme ;
    rdfs:comment "A concept schema related to the Area and Research Event in the database." .

<http://id.acdh.oeaw.ac.at/defc/thesaurus/PeriodDatingmethod> a skos:ConceptScheme ;
    rdfs:comment "A concept schema related to the Area and Research Event in the database." .

<http://id.acdh.oeaw.ac.at/defc/thesaurus/SiteTopography> a skos:ConceptScheme ;
    rdfs:comment "A concept schema related to the particular Site properties." .

<http://id.acdh.oeaw.ac.at/defc/thesaurus/geographic_location/1.098> a skos:Concept ;
    dc:source "OREA" ;
    skos:definition "The location of the site."@en ;
    skos:editorialNote "dc_not_in_database;098" ;
    skos:inScheme <http://id.acdh.oeaw.ac.at/defc/thesaurus/SiteSchema>,
        "NotInDatabase" ;
    skos:prefLabel "geographic location"@en .

<http://id.acdh.oeaw.ac.at/defc/thesaurus/ritual_activity/1.044> a skos:Concept ;
    skos:editorialNote "dc_not_in_database;044" ;
    skos:inScheme <http://id.acdh.oeaw.ac.at/defc/thesaurus/InterpretationSchema>,
        <http://id.acdh.oeaw.ac.at/defc/thesaurus/NotInDatabase> ;
    skos:prefLabel "ritual activity"@en .

<http://id.acdh.oeaw.ac.at/defc/thesaurus/topography/1.099> a skos:Concept ;
    dc:source "OREA" ;
    skos:definition "The location of the site based on the natural and artifical physical features of an area."@en ;
    skos:editorialNote "dc_not_in_database;099" ;
    skos:inScheme <http://id.acdh.oeaw.ac.at/defc/thesaurus/SiteSchema>,
        "NotInDatabase" ;
    skos:narrower <http://id.acdh.oeaw.ac.at/defc/thesaurus/coast/2.1>,
        <http://id.acdh.oeaw.ac.at/defc/thesaurus/hill/2.2>,
        <http://id.acdh.oeaw.ac.at/defc/thesaurus/hillside/2.3>,
        <http://id.acdh.oeaw.ac.at/defc/thesaurus/inland/2.4>,
        <http://id.acdh.oeaw.ac.at/defc/thesaurus/mountain_top/2.6>,
        <http://id.acdh.oeaw.ac.at/defc/thesaurus/plain/2.7>,
        <http://id.acdh.oeaw.ac.at/defc/thesaurus/river_delta/2.8>,
        <http://id.acdh.oeaw.ac.at/defc/thesaurus/valley_bottom/2.5> ;
    skos:prefLabel "topography"@en .

<archaeobotany:_macro-botany/3.2> a skos:Concept ;
    dc:source "OREA" ;
    skos:altLabel " macro botany"@en,
        "macro-botany"@en ;
    skos:broader <http://id.acdh.oeaw.ac.at/defc/thesaurus/archeobotany/2.058> ;
    skos:definition "Analysis of plant remains from archaeological sites visible with the naked eye." ;
    skos:editorialNote "dc_researchevent_special_analysis;2" ;
    skos:inScheme <http://id.acdh.oeaw.ac.at/defc/thesaurus/ResearchEventSchema>,
        <http://id.acdh.oeaw.ac.at/defc/thesaurus/ResearcheventSpecialAnalysis> ;
    skos:prefLabel "Makrobotanik"@de,
        "archaeobotany: macro-botany"@en .

<archaeobotany:_pollen/3.3> a skos:Concept ;
    dc:source "Kipfer, B. A. Encyclopedic Dictionary of Archaeology. Kluwer Academic/Plenum Publishers, New York." ;
    skos:altLabel " pollen analysis"@en,
        "pollen"@en ;
    skos:broader <http://id.acdh.oeaw.ac.at/defc/thesaurus/archeobotany/2.058> ;
    skos:definition "The study of pollen grains in soil samples from an archaeological site, which provides information on ancient human use of plansts and plant resources." ;
    skos:editorialNote "dc_researchevent_special_analysis;3" ;
    skos:inScheme <http://id.acdh.oeaw.ac.at/defc/thesaurus/ResearchEventSchema>,
        <http://id.acdh.oeaw.ac.at/defc/thesaurus/ResearcheventSpecialAnalysis> ;
    skos:prefLabel "Pollenanalyse"@de,
        "archaeobotany: pollen"@en .

<ceramics:_sourcing/3.4> a skos:Concept ;
    dc:source "OREA" ;
    skos:altLabel " sourcing"@en,
        "ceramics sourcing"@en ;
    skos:broader <http://id.acdh.oeaw.ac.at/defc/thesaurus/ceramic_analysis/2.059> ;
    skos:definition "An analysis to find out where the ceramics came from." ;
    skos:editorialNote "dc_researchevent_special_analysis;4" ;
    skos:inScheme <http://id.acdh.oeaw.ac.at/defc/thesaurus/ResearchEventSchema>,
        <http://id.acdh.oeaw.ac.at/defc/thesaurus/ResearcheventSpecialAnalysis> ;
    skos:prefLabel "Herkunftanalyse"@de,
        "ceramics: sourcing"@en .

<ceramics:_thin_section_analysis/3.5> a skos:Concept ;
    dc:source "OREA" ;
    skos:altLabel " thin section"@en,
        "thin section analysis"@en ;
    skos:broader <http://id.acdh.oeaw.ac.at/defc/thesaurus/ceramic_analysis/2.059> ;
    skos:definition "A laboratory preparation of pottery (or other materials such as rock, mineral, soil, bones) for tracing the movement of pottery and assicuated trade through provenance determination." ;
    skos:editorialNote "dc_researchevent_special_analysis;5" ;
    skos:inScheme <http://id.acdh.oeaw.ac.at/defc/thesaurus/ResearchEventSchema>,
        <http://id.acdh.oeaw.ac.at/defc/thesaurus/ResearcheventSpecialAnalysis> ;
    skos:prefLabel "Dünnschliffanalyse"@de,
        "ceramics: thin section analysis"@en .

<dating:_archaeomagnetism/3.6> a skos:Concept ;
    dc:source "http://thesaurus.historicengland.org.uk/thesaurus_term.asp?thes_no=56&term_no=14214" ;
    skos:broader <http://id.acdh.oeaw.ac.at/defc/thesaurus/dating/2.060> ;
    skos:definition "Measures the remanent magnetisation direction of mafnetic minerals. Useful for dating fired structures, in-situ since their last firing, and for sediments settling from non turbulent water bodies. In the UK, calibration data extends back to 1 BC." ;
    skos:editorialNote "dc_researchevent_special_analysis;6" ;
    skos:inScheme <http://id.acdh.oeaw.ac.at/defc/thesaurus/ResearchEventSchema>,
        <http://id.acdh.oeaw.ac.at/defc/thesaurus/ResearcheventSpecialAnalysis> ;
    skos:prefLabel "Archäomagnetismus"@de,
        "dating: archaeomagnetism"@en .

<dating:_dendrochronology/3.7> a skos:Concept ;
    dc:source "http://thesaurus.historicengland.org.uk/thesaurus_term.asp?thes_no=56&term_no=142131" ;
    skos:altLabel "dendrochronology"@en ;
    skos:broader <http://id.acdh.oeaw.ac.at/defc/thesaurus/dating/2.060> ;
    skos:definition "The measuring of annual tree-ring growth shown by most tree species in temperated regions. Regional chronologies are required to date any particular priece of wood, the longest of which, for Germany, works for the present to approximately 14 years ago." ;
    skos:editorialNote "dc_researchevent_special_analysis;7" ;
    skos:inScheme <http://id.acdh.oeaw.ac.at/defc/thesaurus/ResearchEventSchema>,
        <http://id.acdh.oeaw.ac.at/defc/thesaurus/ResearcheventSpecialAnalysis> ;
    skos:prefLabel "Dendrochronologie"@de,
        "dating: dendrochronology"@en .

<dating:_lead_isotope_dating/3.8> a skos:Concept ;
    dc:source "http://thesaurus.historicengland.org.uk/thesaurus_term.asp?thes_no=56&term_no=142155" ;
    skos:altLabel "lead isotope dating"@en ;
    skos:broader <http://id.acdh.oeaw.ac.at/defc/thesaurus/dating/2.060> ;
    skos:definition "A technique which uses the measurement of decay in radioactive lead (Pb) isotopes to determine a date. Useful for sediments and lead-based paints between 1 and 4 years old." ;
    skos:editorialNote "dc_researchevent_special_analysis;8" ;
    skos:inScheme <http://id.acdh.oeaw.ac.at/defc/thesaurus/ResearchEventSchema>,
        <http://id.acdh.oeaw.ac.at/defc/thesaurus/ResearcheventSpecialAnalysis> ;
    skos:prefLabel "Bleiisotopendatierung"@de,
        "dating: lead isotope dating"@en .

<dating:_luminescence_dating/3.9> a skos:Concept ;
    dc:source "http://thesaurus.historicengland.org.uk/thesaurus_term.asp?thes_no=56&term_no=142155" ;
    skos:altLabel " luminescence dating"@en,
        "luminescence"@en ;
    skos:broader <http://id.acdh.oeaw.ac.at/defc/thesaurus/dating/2.060> ;
    skos:definition "A range of techniques that use the build up of charge stored within a crystalline material to estimate its age." ;
    skos:editorialNote "dc_researchevent_special_analysis;9" ;
    skos:inScheme <http://id.acdh.oeaw.ac.at/defc/thesaurus/ResearchEventSchema>,
        <http://id.acdh.oeaw.ac.at/defc/thesaurus/ResearcheventSpecialAnalysis> ;
    skos:prefLabel "Lumineszenz"@de,
        "dating: luminescence dating"@en .

<dating:_mitochondrial_dna/3.10> a skos:Concept ;
    dc:source "http://thesaurus.historicengland.org.uk/thesaurus_term.asp?thes_no=56&term_no=14217" ;
    skos:altLabel "mitochondrial DNA"@en ;
    skos:broader <http://id.acdh.oeaw.ac.at/defc/thesaurus/dating/2.060> ;
    skos:definition "A dating technique for the founding of individual populations based on the assumption of steady rates of mutation in mitochondrial D_NA. Sometimes used to produce dates for stratigraphic layers containing fossil specimens of populations." ;
    skos:editorialNote "dc_researchevent_special_analysis;10" ;
    skos:inScheme <http://id.acdh.oeaw.ac.at/defc/thesaurus/ResearchEventSchema>,
        <http://id.acdh.oeaw.ac.at/defc/thesaurus/ResearcheventSpecialAnalysis> ;
    skos:prefLabel "Mitochondrien-DNA"@de,
        "dating: mitochondrial dna"@en .

<dating:_oxygen_isotope_analysis/3.11> a skos:Concept ;
    dc:source "http://thesaurus.historicengland.org.uk/thesaurus_term.asp?thes_no=56&term_no=142178" ;
    skos:altLabel "oxygen isotope analysis"@en ;
    skos:broader <http://id.acdh.oeaw.ac.at/defc/thesaurus/dating/2.060> ;
    skos:definition "The use of oxygen (O) isotope rations in ice or ocean sedimet cores to data global environmental change." ;
    skos:editorialNote "dc_researchevent_special_analysis;11" ;
    skos:inScheme <http://id.acdh.oeaw.ac.at/defc/thesaurus/ResearchEventSchema>,
        <http://id.acdh.oeaw.ac.at/defc/thesaurus/ResearcheventSpecialAnalysis> ;
    skos:prefLabel "Sauerstoffisotopenanalyse"@de,
        "dating: oxygen isotope analysis"@en .

<dating:_radiocarbon_dating/3.12> a skos:Concept ;
    dc:source "http://thesaurus.historicengland.org.uk/thesaurus_term.asp?thes_no=56&term_no=142188" ;
    skos:altLabel " C14 dating"@en,
        "C14"@en ;
    skos:broader <http://id.acdh.oeaw.ac.at/defc/thesaurus/dating/2.060> ;
    skos:definition "The measurement of the ration of the radioactive Carbon 14 (C-14) isotope and non-radioactive carbon isotopes. Useful for dating organic materials such as wood and bone between 5 and 45 years old." ;
    skos:editorialNote "dc_researchevent_special_analysis;12" ;
    skos:inScheme <http://id.acdh.oeaw.ac.at/defc/thesaurus/ResearchEventSchema>,
        <http://id.acdh.oeaw.ac.at/defc/thesaurus/ResearcheventSpecialAnalysis> ;
    skos:prefLabel "C14-Datierung"@de,
        "dating: radiocarbon dating"@en .

<excavation:_rescue/4.2> a skos:Concept ;
    dc:source "http://thesaurus.historicengland.org.uk/thesaurus_term.asp?thes_no=566&term_no=145157" ;
    skos:altLabel "rescue excavation"@en ;
    skos:broader <http://id.acdh.oeaw.ac.at/defc/thesaurus/excavation/3.049> ;
    skos:definition "Controlled investigation, recording and removal of archaeological deposits under threat of destruction from building development." ;
    skos:editorialNote "dc_researchevet_researchtype;2" ;
    skos:inScheme <http://id.acdh.oeaw.ac.at/defc/thesaurus/ResearchEventSchema>,
        <http://id.acdh.oeaw.ac.at/defc/thesaurus/ResearchevetResearchtype> ;
    skos:prefLabel "Rettungsgrabung"@de,
        "excavation: rescue"@en .

<excavation:_research/4.3> a skos:Concept ;
    dc:source "http://thesaurus.historicengland.org.uk/thesaurus_term.asp?thes_no=566&term_no=14735" ;
    skos:altLabel "research excavation"@en ;
    skos:broader <http://id.acdh.oeaw.ac.at/defc/thesaurus/excavation/3.049> ;
    skos:definition "Controlled investigation, recording and removal of archaeological deposits in targeted areas in order to answer specific questions relating to a particular archaeological site or landscape." ;
    skos:editorialNote "dc_researchevet_researchtype;3" ;
    skos:inScheme <http://id.acdh.oeaw.ac.at/defc/thesaurus/ResearchEventSchema>,
        <http://id.acdh.oeaw.ac.at/defc/thesaurus/ResearchevetResearchtype> ;
    skos:prefLabel "Forschungsgrabung"@de,
        "excavation: research"@en .

<excavation:_underwater/4.4> a skos:Concept ;
    dc:source "http://thesaurus.historicengland.org.uk/thesaurus_term.asp?thes_no=566&term_no=163244" ;
    skos:altLabel "underwater excavation"@en ;
    skos:broader <http://id.acdh.oeaw.ac.at/defc/thesaurus/excavation/3.049> ;
    skos:definition "Controlled intrusive fieldwork which examines, records and interprets arechaeological depostis, features and structures and, as appripriate, retrieves artefacts and ecofats within a specific underwater area." ;
    skos:editorialNote "dc_researchevet_researchtype;4" ;
    skos:inScheme <http://id.acdh.oeaw.ac.at/defc/thesaurus/ResearchEventSchema>,
        <http://id.acdh.oeaw.ac.at/defc/thesaurus/ResearchevetResearchtype> ;
    skos:prefLabel "Unterwassergrabung"@de,
        "excavation: underwater"@en .

<excavation:_undetermined/4.5> a skos:Concept ;
    skos:broader <http://id.acdh.oeaw.ac.at/defc/thesaurus/excavation/3.049> ;
    skos:editorialNote "dc_researchevet_researchtype;5" ;
    skos:inScheme <http://id.acdh.oeaw.ac.at/defc/thesaurus/ResearchEventSchema>,
        <http://id.acdh.oeaw.ac.at/defc/thesaurus/ResearchevetResearchtype> ;
    skos:prefLabel "excavation: undetermined"@en .

<http://id.acdh.oeaw.ac.at/defc/thesaurus/DNA_analysis/2.13> a skos:Concept ;
    dc:source "OREA" ;
    skos:broader <http://id.acdh.oeaw.ac.at/defc/thesaurus/special_analysis/1.057> ;
    skos:definition "Any technique used to analyze genes and DNA to identify individuals by characteristics of their DNA." ;
    skos:editorialNote "dc_researchevent_special_analysis/2.13" ;
    skos:inScheme <http://id.acdh.oeaw.ac.at/defc/thesaurus/ResearchEventSchema>,
        <http://id.acdh.oeaw.ac.at/defc/thesaurus/ResearcheventSpecialAnalysis> ;
    skos:prefLabel "DNA-Analyse"@de,
        "DNA analysis"@en .

<http://id.acdh.oeaw.ac.at/defc/thesaurus/acorn/5.35> a skos:Concept ;
    dc:source "http://dbpedia.org/page/Acorn" ;
    skos:broader <http://id.acdh.oeaw.ac.at/defc/thesaurus/nuts/4.31> ;
    skos:editorialNote "dc_botany_species;35" ;
    skos:inScheme <http://id.acdh.oeaw.ac.at/defc/thesaurus/BotanySpecies>,
        <http://id.acdh.oeaw.ac.at/defc/thesaurus/FindsSchema> ;
    skos:prefLabel "Eichel"@de,
        "acorn"@en .

<http://id.acdh.oeaw.ac.at/defc/thesaurus/acrolith/5.92> a skos:Concept ;
    dc:source "Kipfer, B. A. Dictionary of Artifacts 2007. Blackwell Publishing, Oxford.p 4" ;
    skos:broader <http://id.acdh.oeaw.ac.at/defc/thesaurus/anthropomorphic_figurine/4.84> ;
    skos:definition "A Greek statue, of which the head and extremities were of stone or marble and the trunk crafted of wood which was either gilt or draped." ;
    skos:editorialNote "dc_finds_small_finds_type;92" ;
    skos:inScheme <http://id.acdh.oeaw.ac.at/defc/thesaurus/FindsSchema>,
        <http://id.acdh.oeaw.ac.at/defc/thesaurus/FindsSmallFindsType> ;
    skos:prefLabel "Akrolith"@de,
        "acrolith"@en .

<http://id.acdh.oeaw.ac.at/defc/thesaurus/adult-mature_(19-45)/6.6> a skos:Concept ;
    skos:broader <http://id.acdh.oeaw.ac.at/defc/thesaurus/age_group/5.097> ;
    skos:editorialNote "dc_area_agegroups;6" ;
    skos:inScheme <http://id.acdh.oeaw.ac.at/defc/thesaurus/AreaAgegroups>,
        <http://id.acdh.oeaw.ac.at/defc/thesaurus/AreaSchema> ;
    skos:prefLabel "adult-mature (19-45)"@en .

<http://id.acdh.oeaw.ac.at/defc/thesaurus/adult/6.15> a skos:Concept ;
    skos:broader <http://id.acdh.oeaw.ac.at/defc/thesaurus/age_group/5.097> ;
    skos:editorialNote "dc_area_agegroups;15" ;
    skos:inScheme <http://id.acdh.oeaw.ac.at/defc/thesaurus/AreaAgegroups>,
        <http://id.acdh.oeaw.ac.at/defc/thesaurus/AreaSchema> ;
    skos:prefLabel "adult"@en .

<http://id.acdh.oeaw.ac.at/defc/thesaurus/adult_(19-40)/6.5> a skos:Concept ;
    skos:broader <http://id.acdh.oeaw.ac.at/defc/thesaurus/age_group/5.097> ;
    skos:editorialNote "dc_area_agegroups;5" ;
    skos:inScheme <http://id.acdh.oeaw.ac.at/defc/thesaurus/AreaAgegroups>,
        <http://id.acdh.oeaw.ac.at/defc/thesaurus/AreaSchema> ;
    skos:prefLabel "adult (19-40)"@en .

<http://id.acdh.oeaw.ac.at/defc/thesaurus/adze/4.66> a skos:Concept ;
    dc:source "Kipfer, B. A. Dictionary of Artifacts 2007. Blackwell Publishing, Oxford.p.5" ;
    skos:broader <http://id.acdh.oeaw.ac.at/defc/thesaurus/tool/3.1> ;
    skos:definition "A cutting tool, similar to an ax, in which the blade is set at right angles to the handle or haft. One of the earliest tools, it was widely distribute in Stone Age cultures in the form of a handheld stone chipped to form a blade." ;
    skos:editorialNote "dc_finds_small_finds_type;66" ;
    skos:inScheme <http://id.acdh.oeaw.ac.at/defc/thesaurus/FindsSchema>,
        <http://id.acdh.oeaw.ac.at/defc/thesaurus/FindsSmallFindsType> ;
    skos:prefLabel "Krummaxt"@de,
        "adze"@en .

<http://id.acdh.oeaw.ac.at/defc/thesaurus/aerial_photograph_interpretation/4.12> a skos:Concept ;
    dc:source "http://thesaurus.historicengland.org.uk/thesaurus_term.asp?thes_no=566&term_no=147552" ;
    skos:broader <http://id.acdh.oeaw.ac.at/defc/thesaurus/heritage_assessment/3.055> ;
    skos:definition "The interpretation of information on aerial photographs usually resulting in the production of maps and records of archaeological sites and landscapes. Many aerial photographs may be consulted for a single analytical survey." ;
    skos:editorialNote "dc_researchevet_researchtype;12" ;
    skos:inScheme <http://id.acdh.oeaw.ac.at/defc/thesaurus/ResearchEventSchema>,
        <http://id.acdh.oeaw.ac.at/defc/thesaurus/ResearchevetResearchtype> ;
    skos:prefLabel "Luftbildauswertung"@de,
        "aerial photograph interpretation"@en .

<http://id.acdh.oeaw.ac.at/defc/thesaurus/agate/3.27> a skos:Concept ;
    dc:source "http://dbpedia.org/page/Agate" ;
    skos:broader <http://id.acdh.oeaw.ac.at/defc/thesaurus/stone/2.1> ;
    skos:definition "Cryptocrystalline variety of silica, chiefly chalcedony, characterised by its fineness of grain and brightness of color." ;
    skos:editorialNote "dc_finds_material;27" ;
    skos:inScheme <http://id.acdh.oeaw.ac.at/defc/thesaurus/FindsMaterial>,
        <http://id.acdh.oeaw.ac.at/defc/thesaurus/FindsSchema> ;
    skos:prefLabel "Achat"@de,
        "agate"@en .

<http://id.acdh.oeaw.ac.at/defc/thesaurus/age_not_specified/6.10> a skos:Concept ;
    dc:source "OREA" ;
    skos:broader <http://id.acdh.oeaw.ac.at/defc/thesaurus/age_group/5.097> ;
    skos:definition "The age of human remains has not been specified." ;
    skos:editorialNote "dc_area_agegroups;10" ;
    skos:inScheme <http://id.acdh.oeaw.ac.at/defc/thesaurus/AreaAgegroups>,
        <http://id.acdh.oeaw.ac.at/defc/thesaurus/AreaSchema> ;
    skos:prefLabel "age not specified"@en .

<http://id.acdh.oeaw.ac.at/defc/thesaurus/airborne_laser_scanning_(ALS)/4.21> a skos:Concept ;
    dc:source "OREA" ;
    skos:altLabel " airborne laser scanning"@en,
        " lidar"@en,
        "ALS"@en,
        "LIDAR"@en,
        "LiDAR"@en ;
    skos:broader <http://id.acdh.oeaw.ac.at/defc/thesaurus/remote_sensing/3.056> ;
    skos:definition "Light detection and ranging device is mounted on an aircraft to recird reflected laser pulses. The data can be used to produce digital elevation models." ;
    skos:editorialNote "dc_researchevet_researchtype;21" ;
    skos:inScheme <http://id.acdh.oeaw.ac.at/defc/thesaurus/ResearchEventSchema>,
        <http://id.acdh.oeaw.ac.at/defc/thesaurus/ResearchevetResearchtype> ;
    skos:prefLabel "Airborne laser scanning (ALS)"@de,
        "airborne laser scanning (ALS)"@en .

<http://id.acdh.oeaw.ac.at/defc/thesaurus/almond/5.30> a skos:Concept ;
    dc:source "http://eol.org/pages/231567/overview" ;
    skos:broader <http://id.acdh.oeaw.ac.at/defc/thesaurus/nuts/4.31> ;
    skos:editorialNote "dc_botany_species;30" ;
    skos:inScheme <http://id.acdh.oeaw.ac.at/defc/thesaurus/BotanySpecies>,
        <http://id.acdh.oeaw.ac.at/defc/thesaurus/FindsSchema> ;
    skos:prefLabel "Mandel"@de,
        "almond"@en,
        "Prunus amygdalus"@la .

<http://id.acdh.oeaw.ac.at/defc/thesaurus/altar/5.33> a skos:Concept ;
    dc:source "Kipfer, B. A. Encyclopedic Dictionary of Archaeology. Kluwer Academic/Plenum Publishers, New York." ;
    skos:altLabel "Altar"@de ;
    skos:broader <http://id.acdh.oeaw.ac.at/defc/thesaurus/ritual/4.079> ;
    skos:definition "An elevated table or podium on which to place or sacrifice offerings to the deities." ;
    skos:editorialNote "dc_area_specialfeatures;33" ;
    skos:inScheme <http://id.acdh.oeaw.ac.at/defc/thesaurus/AreaSchema>,
        <http://id.acdh.oeaw.ac.at/defc/thesaurus/AreaSpecialfeatures> ;
    skos:prefLabel "altar"@en .

<http://id.acdh.oeaw.ac.at/defc/thesaurus/amphora/4.119> a skos:Concept ;
    dc:source "OREA" ;
    skos:broader <http://id.acdh.oeaw.ac.at/defc/thesaurus/pottery_form/3.016> ;
    skos:definition "Big closed storage vessel with narrow neck and mouth and usually with two handles at the top. The body is usually oval and long, with a pointed bottom." ;
    skos:editorialNote "dc_finds_pottery_form;119" ;
    skos:inScheme <http://id.acdh.oeaw.ac.at/defc/thesaurus/FindsPotteryForm>,
        <http://id.acdh.oeaw.ac.at/defc/thesaurus/FindsSchema> ;
    skos:prefLabel "Amphore"@de,
        "amphora"@en .

<http://id.acdh.oeaw.ac.at/defc/thesaurus/anchor/5.93> a skos:Concept ;
    dc:source "Kipfer, B. A. Dictionary of Artifacts 2007. Blackwell Publishing, Oxford.p.10" ;
    skos:broader <http://id.acdh.oeaw.ac.at/defc/thesaurus/fishing_object/4.027> ;
    skos:definition "A heavy object used to moor a ship to the sea bottom, typically having a metal shank with a pair of curved, barbed flukes." ;
    skos:editorialNote "dc_finds_small_finds_type;93" ;
    skos:inScheme <http://id.acdh.oeaw.ac.at/defc/thesaurus/FindsSchema>,
        <http://id.acdh.oeaw.ac.at/defc/thesaurus/FindsSmallFindsType> ;
    skos:prefLabel "Anker"@de,
        "anchor"@en .

<http://id.acdh.oeaw.ac.at/defc/thesaurus/andesit/3.29> a skos:Concept ;
    dc:source "http://dbpedia.org/page/Andesite" ;
    skos:broader <http://id.acdh.oeaw.ac.at/defc/thesaurus/stone/2.1> ;
    skos:definition "An extrusive igneous, volcanic rock, of intermediate composition, with aphanitic to porphyritic texture." ;
    skos:editorialNote "dc_finds_material;29" ;
    skos:inScheme <http://id.acdh.oeaw.ac.at/defc/thesaurus/FindsMaterial>,
        <http://id.acdh.oeaw.ac.at/defc/thesaurus/FindsSchema> ;
    skos:prefLabel "Andesit"@de,
        "andesit"@en .

<http://id.acdh.oeaw.ac.at/defc/thesaurus/animal_husbandry/2.3> a skos:Concept ;
    dc:source "OREA" ;
    skos:broader <http://id.acdh.oeaw.ac.at/defc/thesaurus/subsistence/1.043> ;
    skos:definition "The care and raising of animals." ;
    skos:editorialNote "dc_interpretation_subsistencetype;3" ;
    skos:inScheme <http://id.acdh.oeaw.ac.at/defc/thesaurus/InterpretationSchema>,
        <http://id.acdh.oeaw.ac.at/defc/thesaurus/InterpretationSubsistencetype> ;
    skos:prefLabel "Viehzucht"@de,
        "animal husbandry"@en .

<http://id.acdh.oeaw.ac.at/defc/thesaurus/animal_remains_report/2.1> a skos:Concept ;
    dc:source "http://www.ucl.ac.uk/archaeology/research/tags/zooarchaeology" ;
    skos:altLabel "Archäozoologie"@de,
        " archaeozoology"@en,
        "zooarchaeology"@en ;
    skos:broader <http://id.acdh.oeaw.ac.at/defc/thesaurus/special_analysis/1.057> ;
    skos:definition "The study of animal remains from archaeological sites." ;
    skos:editorialNote "dc_researchevent_special_analysis/2.1" ;
    skos:inScheme <http://id.acdh.oeaw.ac.at/defc/thesaurus/ResearchEventSchema>,
        <http://id.acdh.oeaw.ac.at/defc/thesaurus/ResearcheventSpecialAnalysis> ;
    skos:prefLabel "archäozoologischer Bericht"@de,
        "animal remains report"@en .

<http://id.acdh.oeaw.ac.at/defc/thesaurus/anthropomorphic_vessel/4.99> a skos:Concept ;
    dc:source "OREA" ;
    skos:broader <http://id.acdh.oeaw.ac.at/defc/thesaurus/pottery_form/3.016> ;
    skos:definition "Jar-like containers that have a human form." ;
    skos:editorialNote "dc_finds_pottery_form;99" ;
    skos:inScheme <http://id.acdh.oeaw.ac.at/defc/thesaurus/FindsPotteryForm>,
        <http://id.acdh.oeaw.ac.at/defc/thesaurus/FindsSchema> ;
    skos:prefLabel "Anthropomorphes Gefäß"@de,
        "anthropomorphic vessel"@en .

<http://id.acdh.oeaw.ac.at/defc/thesaurus/antiquarian_observation/4.13> a skos:Concept ;
    dc:source "http://thesaurus.historicengland.org.uk/thesaurus_term.asp?thes_no=566&term_no=14634" ;
    skos:broader <http://id.acdh.oeaw.ac.at/defc/thesaurus/heritage_assessment/3.055> ;
    skos:definition "Observations made by antiquarians - those who studied sites and landscapes prior to archaeology and architectural history becoming established disciplined in the 19th century - and reported through publivation or from unpublished manuscripts." ;
    skos:editorialNote "dc_researchevet_researchtype;13" ;
    skos:inScheme <http://id.acdh.oeaw.ac.at/defc/thesaurus/ResearchEventSchema>,
        <http://id.acdh.oeaw.ac.at/defc/thesaurus/ResearchevetResearchtype> ;
    skos:prefLabel "Altgrabung/-untersuchung"@de,
        "antiquarian observation"@en .

<http://id.acdh.oeaw.ac.at/defc/thesaurus/antler/3.7> a skos:Concept ;
    dc:source "http://dbpedia.org/page/Antler" ;
    skos:broader <http://id.acdh.oeaw.ac.at/defc/thesaurus/organic/2.4> ;
    skos:definition "Antlers are extensions of the skull grown by members of the deer family." ;
    skos:editorialNote "dc_finds_material;7" ;
    skos:inScheme <http://id.acdh.oeaw.ac.at/defc/thesaurus/FindsMaterial>,
        <http://id.acdh.oeaw.ac.at/defc/thesaurus/FindsSchema> ;
    skos:prefLabel "Geweih"@de,
        "antler"@en .

<http://id.acdh.oeaw.ac.at/defc/thesaurus/antler/5.8> a skos:Concept ;
    dc:source "https://en.oxforddictionaries.com/definition/antler" ;
    skos:broader <http://id.acdh.oeaw.ac.at/defc/thesaurus/bone/4.021> ;
    skos:definition "Each of the branched horns on the head of an adult deer (typically a male one), which are made of bone and are grown and cast annually." ;
    skos:editorialNote "dc_animal_remains_part;8" ;
    skos:inScheme <http://id.acdh.oeaw.ac.at/defc/thesaurus/AnimalRemainsPart>,
        <http://id.acdh.oeaw.ac.at/defc/thesaurus/FindsSchema> ;
    skos:prefLabel "Geweih"@de,
        "antler"@en .

<http://id.acdh.oeaw.ac.at/defc/thesaurus/apple/4.41> a skos:Concept ;
    dc:source "http://eol.org/pages/29915/overview" ;
    skos:broader <http://id.acdh.oeaw.ac.at/defc/thesaurus/fruit/3.09> ;
    skos:editorialNote "dc_botany_species;41" ;
    skos:inScheme <http://id.acdh.oeaw.ac.at/defc/thesaurus/BotanySpecies>,
        <http://id.acdh.oeaw.ac.at/defc/thesaurus/FindsSchema> ;
    skos:prefLabel "Apfel"@de,
        "apple"@en,
        "Malus"@la .

<http://id.acdh.oeaw.ac.at/defc/thesaurus/applied_disc/5.211> a skos:Concept ;
    dc:source "OREA" ;
    skos:broader <http://id.acdh.oeaw.ac.at/defc/thesaurus/plastic_decoration/4.132> ;
    skos:definition "Pottery decorated with a disc shaped application." ;
    skos:editorialNote "dc_finds_pottery_decoration;211" ;
    skos:inScheme <http://id.acdh.oeaw.ac.at/defc/thesaurus/FindsPotteryDecoration>,
        <http://id.acdh.oeaw.ac.at/defc/thesaurus/FindsSchema> ;
    skos:prefLabel "Angesetzte Scheiben"@de,
        "applied disc"@en .

<http://id.acdh.oeaw.ac.at/defc/thesaurus/appliqué/4.126> a skos:Concept ;
    dc:source "Kipfer, B. A. Dictionary of Artifacts 2007. Blackwell Publishing, Oxford.p. 13" ;
    skos:broader <http://id.acdh.oeaw.ac.at/defc/thesaurus/jewellery/3.2> ;
    skos:definition "Decoration or ornament applied to or laid on another material, such as metal on wood or embroidery on cloth; a ceramic finishing techniques that involves joining shaped pieces of a plastic body to a leather-hard surface by pressure. The applied pieces can" ;
    skos:editorialNote "dc_finds_small_finds_type;126" ;
    skos:inScheme <http://id.acdh.oeaw.ac.at/defc/thesaurus/FindsSchema>,
        <http://id.acdh.oeaw.ac.at/defc/thesaurus/FindsSmallFindsType> ;
    skos:prefLabel "Applikation"@de,
        "appliqué"@en .

<http://id.acdh.oeaw.ac.at/defc/thesaurus/apricot/4.1> a skos:Concept ;
    dc:source "http://eol.org/pages/301091/overview" ;
    skos:broader <http://id.acdh.oeaw.ac.at/defc/thesaurus/fruit/3.09> ;
    skos:editorialNote "dc_botany_species;1" ;
    skos:inScheme <http://id.acdh.oeaw.ac.at/defc/thesaurus/BotanySpecies>,
        <http://id.acdh.oeaw.ac.at/defc/thesaurus/FindsSchema> ;
    skos:prefLabel "Aprikose"@de,
        "apricot"@en,
        "Armeniaca vulgaris"@la .

<http://id.acdh.oeaw.ac.at/defc/thesaurus/apsidal/5.1> a skos:Concept ;
    dc:source "OREA (M. Brami)" ;
    skos:broader <http://id.acdh.oeaw.ac.at/defc/thesaurus/building_shape/4.076> ;
    skos:definition "A building with a semi-circular recess on one side." ;
    skos:editorialNote "dc_area_constructionshape;1" ;
    skos:inScheme <http://id.acdh.oeaw.ac.at/defc/thesaurus/AreaConstructionshape>,
        <http://id.acdh.oeaw.ac.at/defc/thesaurus/AreaSchema> ;
    skos:prefLabel "apsidal"@en .

<http://id.acdh.oeaw.ac.at/defc/thesaurus/architectural_survey/4.14> a skos:Concept ;
    dc:source "http://thesaurus.historicengland.org.uk/thesaurus_term.asp?thes_no=566&term_no=14511" ;
    skos:broader <http://id.acdh.oeaw.ac.at/defc/thesaurus/field_survey/3.052> ;
    skos:definition "Recording and analysis of built structures utilising close obervation as well as manual or electronic survey equipment such as GPS and REDM (Reflectorless Electromagnetic Distance measurement). Includes research, fieldwork and report." ;
    skos:editorialNote "dc_researchevet_researchtype;14" ;
    skos:inScheme <http://id.acdh.oeaw.ac.at/defc/thesaurus/ResearchEventSchema>,
        <http://id.acdh.oeaw.ac.at/defc/thesaurus/ResearchevetResearchtype> ;
    skos:prefLabel "Bauaufnahme"@de,
        "architectural survey"@en .

<http://id.acdh.oeaw.ac.at/defc/thesaurus/askos/4.101> a skos:Concept ;
    dc:source "Kipfer, B. A. Dictionary of Artifacts 2007. Blackwell Publishing, Oxford.p 18" ;
    skos:broader <http://id.acdh.oeaw.ac.at/defc/thesaurus/pottery_form/3.016> ;
    skos:definition "An assymetrical vessel, often squat and duck-shaped, with an off-center mouth, convex top, and single arching handle." ;
    skos:editorialNote "dc_finds_pottery_form;101" ;
    skos:inScheme <http://id.acdh.oeaw.ac.at/defc/thesaurus/FindsPotteryForm>,
        <http://id.acdh.oeaw.ac.at/defc/thesaurus/FindsSchema> ;
    skos:prefLabel "Askos"@de,
        "askos"@en .

<http://id.acdh.oeaw.ac.at/defc/thesaurus/aurochs/5.4> a skos:Concept ;
    dc:source "http://eol.org/pages/10408207/overview" ;
    skos:broader <http://id.acdh.oeaw.ac.at/defc/thesaurus/mammal/4.020> ;
    skos:editorialNote "dc_finds_animal_remains_species;4" ;
    skos:inScheme <http://id.acdh.oeaw.ac.at/defc/thesaurus/FindsAnimalRemainsSpecies>,
        <http://id.acdh.oeaw.ac.at/defc/thesaurus/FindsSchema> ;
    skos:prefLabel "Auerochs"@de,
        "aurochs"@en,
        "Bos primigenius"@la .

<http://id.acdh.oeaw.ac.at/defc/thesaurus/awl/4.87> a skos:Concept ;
    dc:source "Kipfer, B. A. Dictionary of Artifacts 2007. Blackwell Publishing, Oxford.p.22" ;
    skos:altLabel "Pfriem"@de,
        "piercer"@en,
        "pin"@en ;
    skos:broader <http://id.acdh.oeaw.ac.at/defc/thesaurus/tool/3.1> ;
    skos:definition "A small tool consisting of a thin, tapering, sharp-pointed blade of bone, flint, or metal used for piercing holes, making decorations, or in assisting basketweaving." ;
    skos:editorialNote "dc_finds_small_finds_type;87" ;
    skos:inScheme <http://id.acdh.oeaw.ac.at/defc/thesaurus/FindsSchema>,
        <http://id.acdh.oeaw.ac.at/defc/thesaurus/FindsSmallFindsType> ;
    skos:prefLabel "Ahle"@de,
        "awl"@en .

<http://id.acdh.oeaw.ac.at/defc/thesaurus/axe/4.57> a skos:Concept ;
    dc:source "Kipfer, B. A. Dictionary of Artifacts 2007. Blackwell Publishing, Oxford.p.22" ;
    skos:altLabel "ax"@en ;
    skos:broader <http://id.acdh.oeaw.ac.at/defc/thesaurus/tool/3.1> ;
    skos:definition "A flat, heavy cutting tool of stone or metal (bronze) in which the cutting edge is parallel to the haft and which might have the head and handle in one piece. Its main function was for woodworking (hewing, cleaving, or chopping trees) but it was also used as a weapon of war, as the battle ax." ;
    skos:editorialNote "dc_finds_small_finds_type;57" ;
    skos:inScheme <http://id.acdh.oeaw.ac.at/defc/thesaurus/FindsSchema>,
        <http://id.acdh.oeaw.ac.at/defc/thesaurus/FindsSmallFindsType> ;
    skos:prefLabel "Axt"@de,
        "axe"@en .

<http://id.acdh.oeaw.ac.at/defc/thesaurus/backed_bladelet/4.1> a skos:Concept ;
    dc:source "Inizan, M.-L., M. Reduron-Ballinger, H. Roche, J. Tixier 1999, Technology and Terminology of Knapped Stone. Nanterre: CREP., D. Srejovic (ed) 1997, Arheološki Leksikon." ;
    skos:broader <http://id.acdh.oeaw.ac.at/defc/thesaurus/retouched_tool/3.010> ;
    skos:definition "A small  blade with one edge blunted, belongs to the category of microliths." ;
    skos:editorialNote "dc_finds_lithics_retouched_tools;1" ;
    skos:inScheme <http://id.acdh.oeaw.ac.at/defc/thesaurus/FindsLithicsRetouchedTools>,
        <http://id.acdh.oeaw.ac.at/defc/thesaurus/FindsSchema> ;
    skos:prefLabel "backed bladelet"@en .

<http://id.acdh.oeaw.ac.at/defc/thesaurus/baking_pan/4.103> a skos:Concept ;
    dc:source "http://www.bible.ca/archeology/bible-archeology-pottery-glossary-dictionary-encyclopedia.htm" ;
    skos:broader <http://id.acdh.oeaw.ac.at/defc/thesaurus/pottery_form/3.016> ;
    skos:definition "A shallow platter with flat bottom and long handle apparently used for food preparation." ;
    skos:editorialNote "dc_finds_pottery_form;103" ;
    skos:inScheme <http://id.acdh.oeaw.ac.at/defc/thesaurus/FindsPotteryForm>,
        <http://id.acdh.oeaw.ac.at/defc/thesaurus/FindsSchema> ;
    skos:prefLabel "Backplatte"@de,
        "baking pan"@en .

<http://id.acdh.oeaw.ac.at/defc/thesaurus/ball/4.120> a skos:Concept ;
    dc:source "Kipfer, B. A. Dictionary of Artifacts 2007. Blackwell Publishing, Oxford.p 26" ;
    skos:broader <http://id.acdh.oeaw.ac.at/defc/thesaurus/tool/3.1> ;
    skos:definition "A round object used in games." ;
    skos:editorialNote "dc_finds_small_finds_type;120" ;
    skos:inScheme <http://id.acdh.oeaw.ac.at/defc/thesaurus/FindsSchema>,
        <http://id.acdh.oeaw.ac.at/defc/thesaurus/FindsSmallFindsType> ;
    skos:prefLabel "Ball"@de,
        "ball"@en .

<http://id.acdh.oeaw.ac.at/defc/thesaurus/bar_handle_with_knob/6.67> a skos:Concept ;
    dc:source "OREA" ;
    skos:broader <http://id.acdh.oeaw.ac.at/defc/thesaurus/round_bar_handle/5.109> ;
    skos:definition "Bar shaped handle with an applied knob." ;
    skos:editorialNote "dc_finds_pottery_detail;67" ;
    skos:inScheme <http://id.acdh.oeaw.ac.at/defc/thesaurus/FindsPotteryDetail>,
        <http://id.acdh.oeaw.ac.at/defc/thesaurus/FindsSchema> ;
    skos:prefLabel "Stabhenkel mit Knubbe"@de,
        "bar handle with knob"@en .

<http://id.acdh.oeaw.ac.at/defc/thesaurus/barbotine/5.240> a skos:Concept ;
    dc:source "OREA" ;
    skos:altLabel "Eingobenmalerei"@de,
        "slip trailing"@en ;
    skos:broader <http://id.acdh.oeaw.ac.at/defc/thesaurus/plastic_decoration/4.132> ;
    skos:definition "Pottery decorated with a rather thick slip is used for decorating vessels." ;
    skos:editorialNote "dc_finds_pottery_decoration;240" ;
    skos:inScheme <http://id.acdh.oeaw.ac.at/defc/thesaurus/FindsPotteryDecoration>,
        <http://id.acdh.oeaw.ac.at/defc/thesaurus/FindsSchema> ;
    skos:prefLabel "Barbotineverziert"@de,
        "barbotine"@en .

<http://id.acdh.oeaw.ac.at/defc/thesaurus/barley/5.2> a skos:Concept ;
    dc:source "http://eol.org/pages/1114455/overview" ;
    skos:broader <http://id.acdh.oeaw.ac.at/defc/thesaurus/cereal/4.022> ;
    skos:editorialNote "dc_botany_species;2" ;
    skos:inScheme <http://id.acdh.oeaw.ac.at/defc/thesaurus/BotanySpecies>,
        <http://id.acdh.oeaw.ac.at/defc/thesaurus/FindsSchema> ;
    skos:prefLabel "Gerste"@de,
        "barley"@en,
        "Hordeum vulgare"@la .

<http://id.acdh.oeaw.ac.at/defc/thesaurus/basalt/3.20> a skos:Concept ;
    dc:source "http://dbpedia.org/page/Basalt" ;
    skos:broader <http://id.acdh.oeaw.ac.at/defc/thesaurus/stone/2.1> ;
    skos:definition "A common extrusive igneous (volcanic) rock formed from the rapid cooling of basaltic lava exposed at or very near the surface." ;
    skos:editorialNote "dc_finds_material;20" ;
    skos:inScheme <http://id.acdh.oeaw.ac.at/defc/thesaurus/FindsMaterial>,
        <http://id.acdh.oeaw.ac.at/defc/thesaurus/FindsSchema> ;
    skos:prefLabel "Basalt"@de,
        "basalt"@en .

<http://id.acdh.oeaw.ac.at/defc/thesaurus/basin/4.122> a skos:Concept ;
    dc:source "http://www.bible.ca/archeology/bible-archeology-pottery-glossary-dictionary-encyclopedia.htm" ;
    skos:broader <http://id.acdh.oeaw.ac.at/defc/thesaurus/pottery_form/3.016> ;
    skos:definition "A medium-to-large (diameter), intermediate-to-deep bowl." ;
    skos:editorialNote "dc_finds_pottery_form;122" ;
    skos:inScheme <http://id.acdh.oeaw.ac.at/defc/thesaurus/FindsPotteryForm>,
        <http://id.acdh.oeaw.ac.at/defc/thesaurus/FindsSchema> ;
    skos:prefLabel "Becken"@de,
        "basin"@en .

<http://id.acdh.oeaw.ac.at/defc/thesaurus/basin/5.29> a skos:Concept ;
    dc:source "M. Brami, PhD after Catalhoyuk Research Project http://www.catalhoyuk.com/database/catal/help_glossary1.asp" ;
    skos:altLabel "Becken"@de ;
    skos:broader <http://id.acdh.oeaw.ac.at/defc/thesaurus/installation/4.078> ;
    skos:definition "Similar to a bin (a clay or plaster structure with upstanding edges) but with a shallow bowl and a low rim" ;
    skos:editorialNote "dc_area_specialfeatures;29" ;
    skos:inScheme <http://id.acdh.oeaw.ac.at/defc/thesaurus/AreaSchema>,
        <http://id.acdh.oeaw.ac.at/defc/thesaurus/AreaSpecialfeatures> ;
    skos:prefLabel "basin"@en .

<http://id.acdh.oeaw.ac.at/defc/thesaurus/bead/4.78> a skos:Concept ;
    dc:source "Kipfer, B. A. Dictionary of Artifacts 2007. Blackwell Publishing, Oxford.p.32" ;
    skos:broader <http://id.acdh.oeaw.ac.at/defc/thesaurus/jewellery/3.2> ;
    skos:definition "A small, circular, tubular, or oblong ornament with a perforated center; usually made from shell, stone, bone, or glass." ;
    skos:editorialNote "dc_finds_small_finds_type;78" ;
    skos:inScheme <http://id.acdh.oeaw.ac.at/defc/thesaurus/FindsSchema>,
        <http://id.acdh.oeaw.ac.at/defc/thesaurus/FindsSmallFindsType> ;
    skos:prefLabel "Perle"@de,
        "bead"@en .

<http://id.acdh.oeaw.ac.at/defc/thesaurus/bead_inlay/5.118> a skos:Concept ;
    dc:source "Tomkins 2007" ;
    skos:broader <http://id.acdh.oeaw.ac.at/defc/thesaurus/plastic_decoration/4.132> ;
    skos:definition "Pellet inlay typical for Crete." ;
    skos:editorialNote "dc_finds_pottery_decoration;118" ;
    skos:inScheme <http://id.acdh.oeaw.ac.at/defc/thesaurus/FindsPotteryDecoration>,
        <http://id.acdh.oeaw.ac.at/defc/thesaurus/FindsSchema> ;
    skos:prefLabel "Perleneinlage"@de,
        "bead inlay"@en .

<http://id.acdh.oeaw.ac.at/defc/thesaurus/beak_spouted_jug/5.216> a skos:Concept ;
    skos:broader <http://id.acdh.oeaw.ac.at/defc/thesaurus/jug/4.110> ;
    skos:editorialNote "dc_finds_pottery_form;216" ;
    skos:inScheme <http://id.acdh.oeaw.ac.at/defc/thesaurus/FindsPotteryForm>,
        <http://id.acdh.oeaw.ac.at/defc/thesaurus/FindsSchema> ;
    skos:prefLabel "Schnabelkanne"@de,
        "beak spouted jug"@en .

<http://id.acdh.oeaw.ac.at/defc/thesaurus/bean_goose/6.32> a skos:Concept ;
    dc:source "http://eol.org/pages/1048449/overview" ;
    skos:broader <http://id.acdh.oeaw.ac.at/defc/thesaurus/goose/5.037> ;
    skos:editorialNote "dc_finds_animal_remains_species;32" ;
    skos:inScheme <http://id.acdh.oeaw.ac.at/defc/thesaurus/FindsAnimalRemainsSpecies>,
        <http://id.acdh.oeaw.ac.at/defc/thesaurus/FindsSchema> ;
    skos:prefLabel "Staatgans"@de,
        "bean goose"@en,
        "Anser fabalis"@la .

<http://id.acdh.oeaw.ac.at/defc/thesaurus/beaver/5.28> a skos:Concept ;
    dc:source "http://eol.org/pages/1036116/overview" ;
    skos:broader <http://id.acdh.oeaw.ac.at/defc/thesaurus/mammal/4.020> ;
    skos:editorialNote "dc_finds_animal_remains_species;28" ;
    skos:inScheme <http://id.acdh.oeaw.ac.at/defc/thesaurus/FindsAnimalRemainsSpecies>,
        <http://id.acdh.oeaw.ac.at/defc/thesaurus/FindsSchema> ;
    skos:prefLabel "Biber"@de,
        "beaver"@en,
        "Castor fiber"@la .

<http://id.acdh.oeaw.ac.at/defc/thesaurus/belt_hook/4.54> a skos:Concept ;
    dc:source "Kipfer, B. A. Dictionary of Artifacts 2007. Blackwell Publishing, Oxford.p.33" ;
    skos:broader <http://id.acdh.oeaw.ac.at/defc/thesaurus/other/3.4> ;
    skos:definition "A small decorative and functional object used as a garment hook" ;
    skos:editorialNote "dc_finds_small_finds_type;54" ;
    skos:inScheme <http://id.acdh.oeaw.ac.at/defc/thesaurus/FindsSchema>,
        <http://id.acdh.oeaw.ac.at/defc/thesaurus/FindsSmallFindsType> ;
    skos:prefLabel "Gürtelhaken"@de,
        "belt hook"@en .

<http://id.acdh.oeaw.ac.at/defc/thesaurus/bench/5.1> a skos:Concept ;
    dc:source "M. Brami, PhD after Catalhoyuk Research Project http://www.catalhoyuk.com/database/catal/help_glossary1.asp" ;
    skos:altLabel "Bank"@de ;
    skos:broader <http://id.acdh.oeaw.ac.at/defc/thesaurus/installation/4.078> ;
    skos:definition "A high narrow platform." ;
    skos:editorialNote "dc_area_specialfeatures;1" ;
    skos:inScheme <http://id.acdh.oeaw.ac.at/defc/thesaurus/AreaSchema>,
        <http://id.acdh.oeaw.ac.at/defc/thesaurus/AreaSpecialfeatures> ;
    skos:prefLabel "bench"@en .

<http://id.acdh.oeaw.ac.at/defc/thesaurus/bidirectional_core/4.1> a skos:Concept ;
    dc:source "OREA" ;
    skos:altLabel "Bi-directional core"@en,
        "bifacial core"@en ;
    skos:broader <http://id.acdh.oeaw.ac.at/defc/thesaurus/core/3.012> ;
    skos:definition "A core with two, opposed knapping platforms." ;
    skos:editorialNote "dc_finds_lithics_core_shape;1" ;
    skos:inScheme <http://id.acdh.oeaw.ac.at/defc/thesaurus/FindsLithicsCoreShape>,
        <http://id.acdh.oeaw.ac.at/defc/thesaurus/FindsSchema> ;
    skos:prefLabel "bidirektionaler Kern"@de,
        "bidirectional core"@en .

<http://id.acdh.oeaw.ac.at/defc/thesaurus/bitter_vetch/6.3> a skos:Concept ;
    dc:source "http://eol.org/pages/703201/overview" ;
    skos:broader <http://id.acdh.oeaw.ac.at/defc/thesaurus/vetch/5.33> ;
    skos:editorialNote "dc_botany_species;3" ;
    skos:inScheme <http://id.acdh.oeaw.ac.at/defc/thesaurus/BotanySpecies>,
        <http://id.acdh.oeaw.ac.at/defc/thesaurus/FindsSchema> ;
    skos:prefLabel "Linsen-Wicke"@de,
        "bitter vetch"@en,
        "Vicia ervilia"@la .

<http://id.acdh.oeaw.ac.at/defc/thesaurus/black/red_burnished_arapi/5.307> a skos:Concept ;
    dc:source "Hauptmann - Milojcic 1969" ;
    skos:broader <http://id.acdh.oeaw.ac.at/defc/thesaurus/burnished/4.297> ;
    skos:definition "Burnished ware with red respectively black interior respectively exterior surface typical for Thessaly." ;
    skos:editorialNote "dc_finds_pottery_decoration;307" ;
    skos:inScheme <http://id.acdh.oeaw.ac.at/defc/thesaurus/FindsPotteryDecoration>,
        <http://id.acdh.oeaw.ac.at/defc/thesaurus/FindsSchema> ;
    skos:prefLabel "schwarz/rot geglättet Arapi"@de,
        "black/red burnished arapi"@en .

<http://id.acdh.oeaw.ac.at/defc/thesaurus/black_and_red_on_cream_(polychrome)_(β3β)/6.138> a skos:Concept ;
    dc:source "OREA" ;
    skos:broader <http://id.acdh.oeaw.ac.at/defc/thesaurus/pattern_painted/5.041> ;
    skos:definition "Pottery decorated with black and red paint on cream ground (polychrome)." ;
    skos:editorialNote "dc_finds_pottery_decoration;138" ;
    skos:inScheme <http://id.acdh.oeaw.ac.at/defc/thesaurus/FindsPotteryDecoration>,
        <http://id.acdh.oeaw.ac.at/defc/thesaurus/FindsSchema> ;
    skos:prefLabel "Schwarz und rot auf beige (polychrom) (B3b)"@de,
        "black and red on cream (polychrome) (β3β)"@en .

<http://id.acdh.oeaw.ac.at/defc/thesaurus/black_and_red_on_white_(polychrome)_(β3γ)/6.139> a skos:Concept ;
    dc:source "OREA" ;
    skos:broader <http://id.acdh.oeaw.ac.at/defc/thesaurus/pattern_painted/5.041> ;
    skos:definition "Pottery decorated with black and red paint on cream ground (polychrome)." ;
    skos:editorialNote "dc_finds_pottery_decoration;139" ;
    skos:inScheme <http://id.acdh.oeaw.ac.at/defc/thesaurus/FindsPotteryDecoration>,
        <http://id.acdh.oeaw.ac.at/defc/thesaurus/FindsSchema> ;
    skos:prefLabel "Schwarz und rot auf weiß (polychrom) (B3c)"@de,
        "black and red on white (polychrome) (β3γ)"@en .

<http://id.acdh.oeaw.ac.at/defc/thesaurus/black_and_white_on_red_(polychrome)_(β3β)/6.140> a skos:Concept ;
    dc:source "OREA" ;
    skos:broader <http://id.acdh.oeaw.ac.at/defc/thesaurus/pattern_painted/5.041> ;
    skos:definition "Pottery decorated with black and red paint on cream ground (polychrome)." ;
    skos:editorialNote "dc_finds_pottery_decoration;140" ;
    skos:inScheme <http://id.acdh.oeaw.ac.at/defc/thesaurus/FindsPotteryDecoration>,
        <http://id.acdh.oeaw.ac.at/defc/thesaurus/FindsSchema> ;
    skos:prefLabel "Schwarz und weiß auf rot (polychrom) (B3b)"@de,
        "black and white on red (polychrome) (β3β)"@en .

<http://id.acdh.oeaw.ac.at/defc/thesaurus/black_burnished/5.271> a skos:Concept ;
    dc:source "OREA" ;
    skos:broader <http://id.acdh.oeaw.ac.at/defc/thesaurus/burnished/4.297> ;
    skos:definition "Burnished black ware." ;
    skos:editorialNote "dc_finds_pottery_decoration;271" ;
    skos:inScheme <http://id.acdh.oeaw.ac.at/defc/thesaurus/FindsPotteryDecoration>,
        <http://id.acdh.oeaw.ac.at/defc/thesaurus/FindsSchema> ;
    skos:prefLabel "Schwarz geglättet"@de,
        "black burnished"@en .

<http://id.acdh.oeaw.ac.at/defc/thesaurus/black_burnished_with_channeled_decoration_(γ1α3)/5.142> a skos:Concept ;
    dc:source "OREA" ;
    skos:broader <http://id.acdh.oeaw.ac.at/defc/thesaurus/burnished/4.297> ;
    skos:definition "Burnished black ware with channeled/fluted decoration." ;
    skos:editorialNote "dc_finds_pottery_decoration;142" ;
    skos:inScheme <http://id.acdh.oeaw.ac.at/defc/thesaurus/FindsPotteryDecoration>,
        <http://id.acdh.oeaw.ac.at/defc/thesaurus/FindsSchema> ;
    skos:prefLabel "Schwarz geglättet, kanneliert  (C1a3)"@de,
        "black burnished with channeled decoration (γ1α3)"@en .

<http://id.acdh.oeaw.ac.at/defc/thesaurus/black_burnished_with_white_paint_(γ1α1)/5.143> a skos:Concept ;
    dc:source "OREA" ;
    skos:broader <http://id.acdh.oeaw.ac.at/defc/thesaurus/burnished/4.297> ;
    skos:definition "Burnished black ware decorated with white paint." ;
    skos:editorialNote "dc_finds_pottery_decoration;143" ;
    skos:inScheme <http://id.acdh.oeaw.ac.at/defc/thesaurus/FindsPotteryDecoration>,
        <http://id.acdh.oeaw.ac.at/defc/thesaurus/FindsSchema> ;
    skos:prefLabel "Schwarz geglättet mit weißer Bemalung (C1a1)"@de,
        "black burnished with white paint (γ1α1)"@en .

<http://id.acdh.oeaw.ac.at/defc/thesaurus/black_burnished_“larisa”_(γ1α)/5.141> a skos:Concept ;
    dc:source "OREA" ;
    skos:broader <http://id.acdh.oeaw.ac.at/defc/thesaurus/burnished/4.297> ;
    skos:definition "Burnished black ware type \"Larisa\" named after the site in Greece." ;
    skos:editorialNote "dc_finds_pottery_decoration;141" ;
    skos:inScheme <http://id.acdh.oeaw.ac.at/defc/thesaurus/FindsPotteryDecoration>,
        <http://id.acdh.oeaw.ac.at/defc/thesaurus/FindsSchema> ;
    skos:prefLabel "Schwarz geglättet “Larisa” (C1a A5a/c)"@de,
        "black burnished “larisa” (γ1α)"@en .

<http://id.acdh.oeaw.ac.at/defc/thesaurus/black_nightshade/3.38> a skos:Concept ;
    dc:source "http://dbpedia.org/page/Black_nightshade" ;
    skos:broader <http://id.acdh.oeaw.ac.at/defc/thesaurus/botany/2.2> ;
    skos:editorialNote "dc_botany_species;38" ;
    skos:inScheme <http://id.acdh.oeaw.ac.at/defc/thesaurus/BotanySpecies>,
        <http://id.acdh.oeaw.ac.at/defc/thesaurus/FindsSchema> ;
    skos:prefLabel "schwarzes Nachtschattengewächs"@de,
        "black nightshade"@en,
        "Chenopodiacea"@la .

<http://id.acdh.oeaw.ac.at/defc/thesaurus/black_on_grey/6.287> a skos:Concept ;
    dc:source "OREA" ;
    skos:broader <http://id.acdh.oeaw.ac.at/defc/thesaurus/pattern_painted/5.041> ;
    skos:definition "Pottery decorated with black paint added on grey ground." ;
    skos:editorialNote "dc_finds_pottery_decoration;287" ;
    skos:inScheme <http://id.acdh.oeaw.ac.at/defc/thesaurus/FindsPotteryDecoration>,
        <http://id.acdh.oeaw.ac.at/defc/thesaurus/FindsSchema> ;
    skos:prefLabel "schwarz auf grau"@de,
        "black on grey"@en .

<http://id.acdh.oeaw.ac.at/defc/thesaurus/black_on_red/6.163> a skos:Concept ;
    dc:source "OREA" ;
    skos:altLabel "Galepsos ware"@en ;
    skos:broader <http://id.acdh.oeaw.ac.at/defc/thesaurus/pattern_painted/5.041> ;
    skos:definition "Pottery decorated with black paint added on red ground." ;
    skos:editorialNote "dc_finds_pottery_decoration;163" ;
    skos:inScheme <http://id.acdh.oeaw.ac.at/defc/thesaurus/FindsPotteryDecoration>,
        <http://id.acdh.oeaw.ac.at/defc/thesaurus/FindsSchema> ;
    skos:prefLabel "Schwarz auf rot"@de,
        "black on red"@en .

<http://id.acdh.oeaw.ac.at/defc/thesaurus/black_on_red_(β3α2b)/6.144> a skos:Concept ;
    dc:source "OREA" ;
    skos:broader <http://id.acdh.oeaw.ac.at/defc/thesaurus/pattern_painted/5.041> ;
    skos:definition "Pottery decorated with black paint added on red ground." ;
    skos:editorialNote "dc_finds_pottery_decoration;144" ;
    skos:inScheme <http://id.acdh.oeaw.ac.at/defc/thesaurus/FindsPotteryDecoration>,
        <http://id.acdh.oeaw.ac.at/defc/thesaurus/FindsSchema> ;
    skos:prefLabel "Schwarz auf rot  (B3a2b)"@de,
        "black on red (β3α2b)"@en .

<http://id.acdh.oeaw.ac.at/defc/thesaurus/black_on_white/6.279> a skos:Concept ;
    dc:source "OREA" ;
    skos:broader <http://id.acdh.oeaw.ac.at/defc/thesaurus/pattern_painted/5.041> ;
    skos:definition "Pottery decorated with black paint added on white ground." ;
    skos:editorialNote "dc_finds_pottery_decoration;279" ;
    skos:inScheme <http://id.acdh.oeaw.ac.at/defc/thesaurus/FindsPotteryDecoration>,
        <http://id.acdh.oeaw.ac.at/defc/thesaurus/FindsSchema> ;
    skos:prefLabel "schwarz auf weiß"@de,
        "black on white"@en .

<http://id.acdh.oeaw.ac.at/defc/thesaurus/black_on_white_(b3α3)/6.145> a skos:Concept ;
    dc:source "OREA" ;
    skos:broader <http://id.acdh.oeaw.ac.at/defc/thesaurus/pattern_painted/5.041> ;
    skos:definition "Pottery decorated with black paint added on white ground." ;
    skos:editorialNote "dc_finds_pottery_decoration;145" ;
    skos:inScheme <http://id.acdh.oeaw.ac.at/defc/thesaurus/FindsPotteryDecoration>,
        <http://id.acdh.oeaw.ac.at/defc/thesaurus/FindsSchema> ;
    skos:prefLabel "Schwarz auf weiß  (B3a3)"@de,
        "black on white (b3α3)"@en .

<http://id.acdh.oeaw.ac.at/defc/thesaurus/black_pattern_burnished_(γ1α2)/5.146> a skos:Concept ;
    dc:source "OREA" ;
    skos:altLabel "Politurmuster"@de ;
    skos:broader <http://id.acdh.oeaw.ac.at/defc/thesaurus/burnished/4.297> ;
    skos:definition "Black ware decorated with burnished patterns, normally the inside of the open bowls." ;
    skos:editorialNote "dc_finds_pottery_decoration;146" ;
    skos:inScheme <http://id.acdh.oeaw.ac.at/defc/thesaurus/FindsPotteryDecoration>,
        <http://id.acdh.oeaw.ac.at/defc/thesaurus/FindsSchema> ;
    skos:prefLabel "Schwarz mustergeglättet  (C1a2)"@de,
        "black pattern burnished (γ1α2)"@en .

<http://id.acdh.oeaw.ac.at/defc/thesaurus/black_slipped/4.258> a skos:Concept ;
    dc:source "Kipfer, B. A. Dictionary of Artifacts 2007. Blackwell Publishing, Oxford.p 264" ;
    skos:broader <http://id.acdh.oeaw.ac.at/defc/thesaurus/pottery_surface_treatment/3.019> ;
    skos:definition "Any pottery to which a slip, a thin layer of fine clay, is applied to pottery before firing by dipping the pot into a thick liquid mixture of clay and water. Slip decorates the fabric, is often chosen to bake to a color such as red and makes the pot more" ;
    skos:editorialNote "dc_finds_pottery_decoration;258" ;
    skos:inScheme <http://id.acdh.oeaw.ac.at/defc/thesaurus/FindsPotteryDecoration>,
        <http://id.acdh.oeaw.ac.at/defc/thesaurus/FindsSchema> ;
    skos:prefLabel "schwarzer Überzug"@de,
        "black slipped"@en .

<http://id.acdh.oeaw.ac.at/defc/thesaurus/black_topped/4.242> a skos:Concept ;
    dc:source "OREA" ;
    skos:broader <http://id.acdh.oeaw.ac.at/defc/thesaurus/pottery_surface_treatment/3.019> ;
    skos:definition "Pottery with blackened rim, that was most likely added after firing in the kiln." ;
    skos:editorialNote "dc_finds_pottery_decoration;242" ;
    skos:inScheme <http://id.acdh.oeaw.ac.at/defc/thesaurus/FindsPotteryDecoration>,
        <http://id.acdh.oeaw.ac.at/defc/thesaurus/FindsSchema> ;
    skos:prefLabel "Black topped"@de,
        "black topped"@en .

<http://id.acdh.oeaw.ac.at/defc/thesaurus/blackberry/4.36> a skos:Concept ;
    dc:source "http://dbpedia.org/page/Blackberry" ;
    skos:broader <http://id.acdh.oeaw.ac.at/defc/thesaurus/fruit/3.09> ;
    skos:editorialNote "dc_botany_species;36" ;
    skos:inScheme <http://id.acdh.oeaw.ac.at/defc/thesaurus/BotanySpecies>,
        <http://id.acdh.oeaw.ac.at/defc/thesaurus/FindsSchema> ;
    skos:prefLabel "Brombeere"@de,
        "blackberry"@en .

<http://id.acdh.oeaw.ac.at/defc/thesaurus/blade/4.1> a skos:Concept ;
    dc:source "Kipfer, B. A. Dictionary of Artifacts 2007. Blackwell Publishing, Oxford.p.37" ;
    skos:broader <http://id.acdh.oeaw.ac.at/defc/thesaurus/unretouched_tool/3.011> ;
    skos:definition "A long, narrow, sharp-edged, thin flake of stone, used especially as a tool. This flake was detached by striking from a prepared core, often with a hammer. Ist length is usually at least twice the width. The blade may be a tool in itself, or may be the bl" ;
    skos:editorialNote "dc_finds_lithics_unretouched_tools;1" ;
    skos:inScheme <http://id.acdh.oeaw.ac.at/defc/thesaurus/FindsLithicsUnretouchedTools>,
        <http://id.acdh.oeaw.ac.at/defc/thesaurus/FindsSchema> ;
    skos:prefLabel "Klinge"@de,
        "blade"@en .

<http://id.acdh.oeaw.ac.at/defc/thesaurus/blade/4.68> a skos:Concept ;
    dc:source "Kipfer, B. A. Dictionary of Artifacts 2007. Blackwell Publishing, Oxford.p.37" ;
    skos:broader <http://id.acdh.oeaw.ac.at/defc/thesaurus/tool/3.1> ;
    skos:definition "A long, narrow, sharp-edged, thin flake of stone, used especially as a tool. This flake was detached by striking from a prepared core, often with a hammer. Ist length is usually at least twice the width. The blade may be a tool in itself, or may be the blank from which a two-edged knife, burin, or spokeshave was manufactured." ;
    skos:editorialNote "dc_finds_small_finds_type;68" ;
    skos:inScheme <http://id.acdh.oeaw.ac.at/defc/thesaurus/FindsSchema>,
        <http://id.acdh.oeaw.ac.at/defc/thesaurus/FindsSmallFindsType> ;
    skos:prefLabel "Klinge"@de,
        "blade"@en .

<http://id.acdh.oeaw.ac.at/defc/thesaurus/blade_core/4.2> a skos:Concept ;
    dc:source "OREA" ;
    skos:altLabel "Blade-core"@en ;
    skos:broader <http://id.acdh.oeaw.ac.at/defc/thesaurus/core/3.012> ;
    skos:definition "A core which main reduction leads to the detachment of blades (aim of knapping-blades)." ;
    skos:editorialNote "dc_finds_lithics_core_shape;2" ;
    skos:inScheme <http://id.acdh.oeaw.ac.at/defc/thesaurus/FindsLithicsCoreShape>,
        <http://id.acdh.oeaw.ac.at/defc/thesaurus/FindsSchema> ;
    skos:prefLabel "Klingenkern"@de,
        "blade core"@en .

<http://id.acdh.oeaw.ac.at/defc/thesaurus/blade_industry/5.1> a skos:Concept ;
    dc:source "Inizan, M.-L., M. Reduron-Ballinger, H. Roche, J. Tixier 1999, Technology and Terminology of Knapped Stone. Nanterre: CREP. p. 143." ;
    skos:broader <http://id.acdh.oeaw.ac.at/defc/thesaurus/lithics_industry/4.024> ;
    skos:definition "Human action applied to raw materials in order to transform them into blades." ;
    skos:editorialNote "dc_finds_lithics_industry;1" ;
    skos:inScheme <http://id.acdh.oeaw.ac.at/defc/thesaurus/FindsLithicsIndustry>,
        <http://id.acdh.oeaw.ac.at/defc/thesaurus/FindsSchema> ;
    skos:prefLabel "blade industry"@en .

<http://id.acdh.oeaw.ac.at/defc/thesaurus/bladelet/4.2> a skos:Concept ;
    dc:source "Inizan, M.-L., M. Reduron-Ballinger, H. Roche, J. Tixier 1999, Technology and Terminology of Knapped Stone. Nanterre: CREP., D. Srejovic (ed) 1997, Arheološki Leksikon." ;
    skos:broader <http://id.acdh.oeaw.ac.at/defc/thesaurus/unretouched_tool/3.011> ;
    skos:definition "A narrow blade which usually can be defined with the width less than 12mm. (Micro-blade would be then a small blade with the width under 8mm)." ;
    skos:editorialNote "dc_finds_lithics_unretouched_tools;2" ;
    skos:inScheme <http://id.acdh.oeaw.ac.at/defc/thesaurus/FindsLithicsUnretouchedTools>,
        <http://id.acdh.oeaw.ac.at/defc/thesaurus/FindsSchema> ;
    skos:prefLabel "bladelet"@en .

<http://id.acdh.oeaw.ac.at/defc/thesaurus/body/5.5> a skos:Concept ;
    skos:broader <http://id.acdh.oeaw.ac.at/defc/thesaurus/bone/4.021> ;
    skos:editorialNote "dc_animal_remains_part;5" ;
    skos:inScheme <http://id.acdh.oeaw.ac.at/defc/thesaurus/AnimalRemainsPart>,
        <http://id.acdh.oeaw.ac.at/defc/thesaurus/FindsSchema> ;
    skos:prefLabel "Torso"@de,
        "body"@en .

<http://id.acdh.oeaw.ac.at/defc/thesaurus/bone/3.5> a skos:Concept ;
    dc:source "OREA" ;
    skos:broader <http://id.acdh.oeaw.ac.at/defc/thesaurus/organic/2.4> ;
    skos:definition "Bone used as material for production of different kinds of objects (tools, figurines etc)." ;
    skos:editorialNote "dc_finds_material;5" ;
    skos:inScheme <http://id.acdh.oeaw.ac.at/defc/thesaurus/FindsMaterial>,
        <http://id.acdh.oeaw.ac.at/defc/thesaurus/FindsSchema> ;
    skos:prefLabel "Knochen"@de,
        "bone"@en .

<http://id.acdh.oeaw.ac.at/defc/thesaurus/bone/4.2> a skos:Concept ;
    dc:source "https://en.oxforddictionaries.com/definition/us/bone" ;
    skos:broader <http://id.acdh.oeaw.ac.at/defc/thesaurus/dating_material/3.046> ;
    skos:definition "Any of the pieces of hard, whitish tissue making up the skeleton in humans and other vertebrates. It can be used for radiocarbon dating." ;
    skos:editorialNote "dc_period_datedby;2" ;
    skos:inScheme <http://id.acdh.oeaw.ac.at/defc/thesaurus/PeriodSchema> ;
    skos:prefLabel "Knochen"@de,
        "bone"@en .

<http://id.acdh.oeaw.ac.at/defc/thesaurus/bone_tool_production/2.6> a skos:Concept ;
    dc:source "OREA" ;
    skos:broader <http://id.acdh.oeaw.ac.at/defc/thesaurus/production/1.042> ;
    skos:definition "The activity of making physical items of bone that can be afterwards used to achive a certain goal." ;
    skos:editorialNote "dc_interpretation_productiontype;6" ;
    skos:inScheme <http://id.acdh.oeaw.ac.at/defc/thesaurus/InterpretationProductiontype>,
        <http://id.acdh.oeaw.ac.at/defc/thesaurus/InterpretationSchema> ;
    skos:prefLabel "Produktion von Knochenwekzeugen"@de,
        "bone tool production"@en .

<http://id.acdh.oeaw.ac.at/defc/thesaurus/borehole_survey/3.1> a skos:Concept ;
    dc:source "http://thesaurus.historicengland.org.uk/thesaurus_term.asp?thes_no=566&term_no=145112" ;
    skos:broader <http://id.acdh.oeaw.ac.at/defc/thesaurus/intrusive/2.048> ;
    skos:definition "Type of survey involving the drilling of deep and narrow shafts in the gorund used to describe deposits, understand stratigraphy and collect cores amples." ;
    skos:editorialNote "dc_researchevet_researchtype;1" ;
    skos:inScheme <http://id.acdh.oeaw.ac.at/defc/thesaurus/ResearchEventSchema>,
        <http://id.acdh.oeaw.ac.at/defc/thesaurus/ResearchevetResearchtype> ;
    skos:prefLabel "Bohrung"@de,
        "borehole survey"@en .

<http://id.acdh.oeaw.ac.at/defc/thesaurus/bothros/5.21> a skos:Concept ;
    dc:source "https://de.wikipedia.org/wiki/Bothros" ;
    skos:broader <http://id.acdh.oeaw.ac.at/defc/thesaurus/ritual/4.079> ;
    skos:definition "A pit or depression used for various purposes such as storage or waste, but mostly related to cult activities such as sacrifice in ancient Greece." ;
    skos:editorialNote "dc_area_specialfeatures;21" ;
    skos:inScheme <http://id.acdh.oeaw.ac.at/defc/thesaurus/AreaSchema>,
        <http://id.acdh.oeaw.ac.at/defc/thesaurus/AreaSpecialfeatures> ;
    skos:prefLabel "bothros"@en .

<http://id.acdh.oeaw.ac.at/defc/thesaurus/bracelet/4.77> a skos:Concept ;
    dc:source "Kipfer, B. A. Dictionary of Artifacts 2007. Blackwell Publishing, Oxford.p.45" ;
    skos:broader <http://id.acdh.oeaw.ac.at/defc/thesaurus/jewellery/3.2> ;
    skos:definition "An ornamental band or chain worn on the wrist or arm." ;
    skos:editorialNote "dc_finds_small_finds_type;77" ;
    skos:inScheme <http://id.acdh.oeaw.ac.at/defc/thesaurus/FindsSchema>,
        <http://id.acdh.oeaw.ac.at/defc/thesaurus/FindsSmallFindsType> ;
    skos:prefLabel "Armreif"@de,
        "bracelet"@en .

<http://id.acdh.oeaw.ac.at/defc/thesaurus/bridge_spout/5.138> a skos:Concept ;
    dc:source "Kipfer, B. A. Dictionary of Artifacts 2007. Blackwell Publishing, Oxford.p 300" ;
    skos:broader <http://id.acdh.oeaw.ac.at/defc/thesaurus/spout/4.88> ;
    skos:definition "Nozzle shaped appendage that restricts a secondary orifice occuring to one side of a vessel´s vertical axis, and typically on the vessel´s upper body or shoulder." ;
    skos:editorialNote "dc_finds_pottery_detail;138" ;
    skos:inScheme <http://id.acdh.oeaw.ac.at/defc/thesaurus/FindsPotteryDetail>,
        <http://id.acdh.oeaw.ac.at/defc/thesaurus/FindsSchema> ;
    skos:prefLabel "Tüllenausguss"@de,
        "bridge spout"@en .

<http://id.acdh.oeaw.ac.at/defc/thesaurus/broomcorn_millet/6.4> a skos:Concept ;
    dc:source "http://eol.org/pages/1114498/overview" ;
    skos:broader <http://id.acdh.oeaw.ac.at/defc/thesaurus/millet/5.039> ;
    skos:editorialNote "dc_botany_species;4" ;
    skos:inScheme <http://id.acdh.oeaw.ac.at/defc/thesaurus/BotanySpecies>,
        <http://id.acdh.oeaw.ac.at/defc/thesaurus/FindsSchema> ;
    skos:prefLabel "Rispenhirse"@de,
        "broomcorn millet"@en,
        "Panicum miliaceum"@la .

<http://id.acdh.oeaw.ac.at/defc/thesaurus/brown_bear/5.22> a skos:Concept ;
    dc:source "http://eol.org/pages/328581/overview" ;
    skos:broader <http://id.acdh.oeaw.ac.at/defc/thesaurus/mammal/4.020> ;
    skos:editorialNote "dc_finds_animal_remains_species;22" ;
    skos:inScheme <http://id.acdh.oeaw.ac.at/defc/thesaurus/FindsAnimalRemainsSpecies>,
        <http://id.acdh.oeaw.ac.at/defc/thesaurus/FindsSchema> ;
    skos:prefLabel "Braunbär"@de,
        "brown bear"@en,
        "Ursus arctos"@la .

<http://id.acdh.oeaw.ac.at/defc/thesaurus/brown_burnished/5.120> a skos:Concept ;
    dc:source "OREA" ;
    skos:altLabel "BBW"@en ;
    skos:broader <http://id.acdh.oeaw.ac.at/defc/thesaurus/burnished/4.297> ;
    skos:definition "Burnished brown ware." ;
    skos:editorialNote "dc_finds_pottery_decoration;120" ;
    skos:inScheme <http://id.acdh.oeaw.ac.at/defc/thesaurus/FindsPotteryDecoration>,
        <http://id.acdh.oeaw.ac.at/defc/thesaurus/FindsSchema> ;
    skos:prefLabel "Braun geglättet"@de,
        "brown burnished"@en .

<http://id.acdh.oeaw.ac.at/defc/thesaurus/brown_on_buff/6.185> a skos:Concept ;
    dc:source "OREA" ;
    skos:broader <http://id.acdh.oeaw.ac.at/defc/thesaurus/pattern_painted/5.041> ;
    skos:definition "Pottery decorated with brown paint on buff ground." ;
    skos:editorialNote "dc_finds_pottery_decoration;185" ;
    skos:inScheme <http://id.acdh.oeaw.ac.at/defc/thesaurus/FindsPotteryDecoration>,
        <http://id.acdh.oeaw.ac.at/defc/thesaurus/FindsSchema> ;
    skos:prefLabel "Braun auf hell"@de,
        "brown on buff"@en .

<http://id.acdh.oeaw.ac.at/defc/thesaurus/brown_on_buff_(matt_painted)_(b3ε)/6.147> a skos:Concept ;
    dc:source "OREA" ;
    skos:broader <http://id.acdh.oeaw.ac.at/defc/thesaurus/pattern_painted/5.041> ;
    skos:definition "Pottery decorated with brown paint on buff ground also known as matt-painted." ;
    skos:editorialNote "dc_finds_pottery_decoration;147" ;
    skos:inScheme <http://id.acdh.oeaw.ac.at/defc/thesaurus/FindsPotteryDecoration>,
        <http://id.acdh.oeaw.ac.at/defc/thesaurus/FindsSchema> ;
    skos:prefLabel "Braun auf hell (mattbemalt) (B3e)"@de,
        "brown on buff (matt painted) (b3ε)"@en .

<http://id.acdh.oeaw.ac.at/defc/thesaurus/brown_on_cream/6.262> a skos:Concept ;
    dc:source "OREA" ;
    skos:broader <http://id.acdh.oeaw.ac.at/defc/thesaurus/pattern_painted/5.041> ;
    skos:definition "Pottery decorated with brown paint on cream ground." ;
    skos:editorialNote "dc_finds_pottery_decoration;262" ;
    skos:inScheme <http://id.acdh.oeaw.ac.at/defc/thesaurus/FindsPotteryDecoration>,
        <http://id.acdh.oeaw.ac.at/defc/thesaurus/FindsSchema> ;
    skos:prefLabel "Braun auf beige"@de,
        "brown on cream"@en .

<http://id.acdh.oeaw.ac.at/defc/thesaurus/brown_on_cream_(b3α2a)/6.148> a skos:Concept ;
    dc:source "OREA" ;
    skos:broader <http://id.acdh.oeaw.ac.at/defc/thesaurus/pattern_painted/5.041> ;
    skos:definition "Pottery decorated with brown paint on cream ground." ;
    skos:editorialNote "dc_finds_pottery_decoration;148" ;
    skos:inScheme <http://id.acdh.oeaw.ac.at/defc/thesaurus/FindsPotteryDecoration>,
        <http://id.acdh.oeaw.ac.at/defc/thesaurus/FindsSchema> ;
    skos:prefLabel "Braun auf beige  (B3a2a)"@de,
        "brown on cream (b3α2a)"@en .

<http://id.acdh.oeaw.ac.at/defc/thesaurus/brown_on_red/6.186> a skos:Concept ;
    dc:source "OREA" ;
    skos:broader <http://id.acdh.oeaw.ac.at/defc/thesaurus/pattern_painted/5.041> ;
    skos:definition "Pottery decorated with brown paint on red ground." ;
    skos:editorialNote "dc_finds_pottery_decoration;186" ;
    skos:inScheme <http://id.acdh.oeaw.ac.at/defc/thesaurus/FindsPotteryDecoration>,
        <http://id.acdh.oeaw.ac.at/defc/thesaurus/FindsSchema> ;
    skos:prefLabel "Braun auf rot"@de,
        "brown on red"@en .

<http://id.acdh.oeaw.ac.at/defc/thesaurus/brown_on_yellow/6.283> a skos:Concept ;
    dc:source "OREA" ;
    skos:broader <http://id.acdh.oeaw.ac.at/defc/thesaurus/pattern_painted/5.041> ;
    skos:definition "Pottery decorated with brown paint on yellow ground." ;
    skos:editorialNote "dc_finds_pottery_decoration;283" ;
    skos:inScheme <http://id.acdh.oeaw.ac.at/defc/thesaurus/FindsPotteryDecoration>,
        <http://id.acdh.oeaw.ac.at/defc/thesaurus/FindsSchema> ;
    skos:prefLabel "braun auf gelb"@de,
        "brown on yellow"@en .

<http://id.acdh.oeaw.ac.at/defc/thesaurus/brushed/4.213> a skos:Concept ;
    dc:source "OREA" ;
    skos:broader <http://id.acdh.oeaw.ac.at/defc/thesaurus/pottery_surface_treatment/3.019> ;
    skos:definition "Pottery with brushed surface." ;
    skos:editorialNote "dc_finds_pottery_decoration;213" ;
    skos:inScheme <http://id.acdh.oeaw.ac.at/defc/thesaurus/FindsPotteryDecoration>,
        <http://id.acdh.oeaw.ac.at/defc/thesaurus/FindsSchema> ;
    skos:prefLabel "Gebürstet"@de,
        "brushed"@en .

<http://id.acdh.oeaw.ac.at/defc/thesaurus/buckthorn/3.43> a skos:Concept ;
    dc:source "http://eol.org/pages/2880478/overview" ;
    skos:broader <http://id.acdh.oeaw.ac.at/defc/thesaurus/botany/2.2> ;
    skos:editorialNote "dc_botany_species;43" ;
    skos:inScheme <http://id.acdh.oeaw.ac.at/defc/thesaurus/BotanySpecies>,
        <http://id.acdh.oeaw.ac.at/defc/thesaurus/FindsSchema> ;
    skos:prefLabel "Dorn"@de,
        "buckthorn"@en,
        "Rhammus"@la .

<http://id.acdh.oeaw.ac.at/defc/thesaurus/bullet_core/4.3> a skos:Concept ;
    dc:source "OREA" ;
    skos:broader <http://id.acdh.oeaw.ac.at/defc/thesaurus/core/3.012> ;
    skos:definition "A blade core which complete exhaustion leads to the bullet shape." ;
    skos:editorialNote "dc_finds_lithics_core_shape;3" ;
    skos:inScheme <http://id.acdh.oeaw.ac.at/defc/thesaurus/FindsLithicsCoreShape>,
        <http://id.acdh.oeaw.ac.at/defc/thesaurus/FindsSchema> ;
    skos:prefLabel "Bullet core"@de,
        "bullet core"@en .

<http://id.acdh.oeaw.ac.at/defc/thesaurus/burin/4.2> a skos:Concept ;
    dc:source "Inizan, M.-L., M. Reduron-Ballinger, H. Roche, J. Tixier 1999, Technology and Terminology of Knapped Stone. Nanterre: CREP., D. Srejovic (ed) 1997, Arheološki Leksikon." ;
    skos:broader <http://id.acdh.oeaw.ac.at/defc/thesaurus/retouched_tool/3.010> ;
    skos:definition "A specialized engraving tool which bears a negative surface created by the removal of a burin spall (cut diagonally downward from the part of the blade/flake edge)." ;
    skos:editorialNote "dc_finds_lithics_retouched_tools;2" ;
    skos:inScheme <http://id.acdh.oeaw.ac.at/defc/thesaurus/FindsLithicsRetouchedTools>,
        <http://id.acdh.oeaw.ac.at/defc/thesaurus/FindsSchema> ;
    skos:prefLabel "Stichel"@de,
        "burin"@en .

<http://id.acdh.oeaw.ac.at/defc/thesaurus/burnisher/4.65> a skos:Concept ;
    dc:source "Kipfer, B. A. Dictionary of Artifacts 2007. Blackwell Publishing, Oxford.p.50" ;
    skos:altLabel "smoother"@en ;
    skos:broader <http://id.acdh.oeaw.ac.at/defc/thesaurus/tool/3.1> ;
    skos:definition "A tool used to polish the surface of an artifact." ;
    skos:editorialNote "dc_finds_small_finds_type;65" ;
    skos:inScheme <http://id.acdh.oeaw.ac.at/defc/thesaurus/FindsSchema>,
        <http://id.acdh.oeaw.ac.at/defc/thesaurus/FindsSmallFindsType> ;
    skos:prefLabel "Polierer"@de,
        "burnisher"@en .

<http://id.acdh.oeaw.ac.at/defc/thesaurus/button/4.102> a skos:Concept ;
    dc:source "Kipfer, B. A. Dictionary of Artifacts 2007. Blackwell Publishing, Oxford.p 51" ;
    skos:broader <http://id.acdh.oeaw.ac.at/defc/thesaurus/other/3.4> ;
    skos:definition "Small, usually disklike, pieces of bone, metal, stone, or other solid material that have holes or a shank through which they are sewn on to garments. Buttons are used to fasten or close a garment and are sometimes purely decorative." ;
    skos:editorialNote "dc_finds_small_finds_type;102" ;
    skos:inScheme <http://id.acdh.oeaw.ac.at/defc/thesaurus/FindsSchema>,
        <http://id.acdh.oeaw.ac.at/defc/thesaurus/FindsSmallFindsType> ;
    skos:prefLabel "Knopf"@de,
        "button"@en .

<http://id.acdh.oeaw.ac.at/defc/thesaurus/buttress/5.32> a skos:Concept ;
    dc:source "M. Brami, PhD after Catalhoyuk Research Project http://www.catalhoyuk.com/database/catal/help_glossary1.asp" ;
    skos:broader <http://id.acdh.oeaw.ac.at/defc/thesaurus/architecture/4.081> ;
    skos:definition "A projecting support built against a wall." ;
    skos:editorialNote "dc_area_specialfeatures;32" ;
    skos:inScheme <http://id.acdh.oeaw.ac.at/defc/thesaurus/AreaSchema>,
        <http://id.acdh.oeaw.ac.at/defc/thesaurus/AreaSpecialfeatures> ;
    skos:prefLabel "buttress"@en .

<http://id.acdh.oeaw.ac.at/defc/thesaurus/byblos_point/6.116> a skos:Concept ;
    dc:source "Gopher, A. 1994. Arrowheads of the Neolithic Levant. Wiona Lake, Eisenbrauns." ;
    skos:broader <http://id.acdh.oeaw.ac.at/defc/thesaurus/projectile_point/5.70> ;
    skos:definition "A large, heavy arrowhead, usually carelessly made and asymetrical." ;
    skos:editorialNote "dc_finds_small_finds_type;116" ;
    skos:inScheme <http://id.acdh.oeaw.ac.at/defc/thesaurus/FindsSchema>,
        <http://id.acdh.oeaw.ac.at/defc/thesaurus/FindsSmallFindsType> ;
    skos:prefLabel "byblos point"@en .

<http://id.acdh.oeaw.ac.at/defc/thesaurus/cairn/5.8> a skos:Concept ;
    dc:source "Kipfer, B. A. Encyclopedic Dictionary of Archaeology. Kluwer Academic/Plenum Publishers, New York. P.88." ;
    skos:broader <http://id.acdh.oeaw.ac.at/defc/thesaurus/grave_type/4.083> ;
    skos:definition "A pyramid of rough stones, raised for a memorial or mark of some kind, usually over a burial but also as a landmark or monument." ;
    skos:editorialNote "dc_area_gravetype;8" ;
    skos:inScheme <http://id.acdh.oeaw.ac.at/defc/thesaurus/AreaGravetype>,
        <http://id.acdh.oeaw.ac.at/defc/thesaurus/AreaSchema> ;
    skos:prefLabel "cairn"@en .

<http://id.acdh.oeaw.ac.at/defc/thesaurus/calcite/3.37> a skos:Concept ;
    dc:source "http://dbpedia.org/page/Calcite" ;
    skos:altLabel "Kalkspat"@de,
        "Kalzit"@de ;
    skos:broader <http://id.acdh.oeaw.ac.at/defc/thesaurus/mineral/2.3> ;
    skos:definition "Calcite is a carbonate mineral and the most stable polymorph of calcium carbonate (CaCO3)." ;
    skos:editorialNote "dc_finds_material;37" ;
    skos:inScheme <http://id.acdh.oeaw.ac.at/defc/thesaurus/FindsMaterial>,
        <http://id.acdh.oeaw.ac.at/defc/thesaurus/FindsSchema> ;
    skos:prefLabel "Calcit"@de,
        "calcite"@en .

<http://id.acdh.oeaw.ac.at/defc/thesaurus/cardium_shell/4.36> a skos:Concept ;
    dc:source "http://dbpedia.org/page/Cockle_(bivalve)" ;
    skos:altLabel "Cockle"@en,
        "cardium"@en ;
    skos:broader <http://id.acdh.oeaw.ac.at/defc/thesaurus/shell/3.6> ;
    skos:definition "A cockle is a small, edible, saltwater clam, a marine bivalve mollusc." ;
    skos:editorialNote "dc_finds_material;36" ;
    skos:inScheme <http://id.acdh.oeaw.ac.at/defc/thesaurus/FindsMaterial>,
        <http://id.acdh.oeaw.ac.at/defc/thesaurus/FindsSchema> ;
    skos:prefLabel "Herzmuscheln"@de,
        "cardium shell"@en .

<http://id.acdh.oeaw.ac.at/defc/thesaurus/carinated_bowl_with_inverted_rim/6.105> a skos:Concept ;
    dc:source "OREA" ;
    skos:broader <http://id.acdh.oeaw.ac.at/defc/thesaurus/carinated_bowl/5.104> ;
    skos:definition "A shallow, open vessel with upper part heavily contracting inwards." ;
    skos:editorialNote "dc_finds_pottery_form;105" ;
    skos:inScheme <http://id.acdh.oeaw.ac.at/defc/thesaurus/FindsPotteryForm>,
        <http://id.acdh.oeaw.ac.at/defc/thesaurus/FindsSchema> ;
    skos:prefLabel "Knickrandschale"@de,
        "carinated bowl with inverted rim"@en .

<http://id.acdh.oeaw.ac.at/defc/thesaurus/carinated_incurved_bowl/6.174> a skos:Concept ;
    dc:source "OREA" ;
    skos:broader <http://id.acdh.oeaw.ac.at/defc/thesaurus/carinated_bowl/5.104> ;
    skos:definition "A low, open vessel with inward bent walls." ;
    skos:editorialNote "dc_finds_pottery_form;174" ;
    skos:inScheme <http://id.acdh.oeaw.ac.at/defc/thesaurus/FindsPotteryForm>,
        <http://id.acdh.oeaw.ac.at/defc/thesaurus/FindsSchema> ;
    skos:prefLabel "Einwärts gekrümmte Knickwandschale"@de,
        "carinated incurved bowl"@en .

<http://id.acdh.oeaw.ac.at/defc/thesaurus/carinated_jar/5.175> a skos:Concept ;
    dc:source "OREA" ;
    skos:broader <http://id.acdh.oeaw.ac.at/defc/thesaurus/jar/4.145> ;
    skos:definition "A closed vessel used for storage, preservation, or transportation of goods with two or non handles and bent walls." ;
    skos:editorialNote "dc_finds_pottery_form;175" ;
    skos:inScheme <http://id.acdh.oeaw.ac.at/defc/thesaurus/FindsPotteryForm>,
        <http://id.acdh.oeaw.ac.at/defc/thesaurus/FindsSchema> ;
    skos:prefLabel "Knickwandtopf"@de,
        "carinated jar"@en .

<http://id.acdh.oeaw.ac.at/defc/thesaurus/cattle/5.3> a skos:Concept ;
    dc:source "http://eol.org/pages/328699/overview" ;
    skos:broader <http://id.acdh.oeaw.ac.at/defc/thesaurus/mammal/4.020> ;
    skos:editorialNote "dc_finds_animal_remains_species;3" ;
    skos:inScheme <http://id.acdh.oeaw.ac.at/defc/thesaurus/FindsAnimalRemainsSpecies>,
        <http://id.acdh.oeaw.ac.at/defc/thesaurus/FindsSchema> ;
    skos:prefLabel "Rind"@de,
        "cattle"@en,
        "Bos taurus"@la .

<http://id.acdh.oeaw.ac.at/defc/thesaurus/ceramics/4.5> a skos:Concept ;
    dc:source "Kipfer, B. A. Encyclopedic Dictionary of Archaeology. Kluwer Academic/Plenum Publishers, New York. P.103" ;
    skos:broader <http://id.acdh.oeaw.ac.at/defc/thesaurus/dating_material/3.046> ;
    skos:definition "Fired clay, normally belonging to pottery, figurine, or other ceramic industries. " ;
    skos:editorialNote "dc_period_datedby;5" ;
    skos:inScheme <http://id.acdh.oeaw.ac.at/defc/thesaurus/PeriodSchema> ;
    skos:prefLabel "Keramik"@de,
        "ceramics"@en .

<http://id.acdh.oeaw.ac.at/defc/thesaurus/chalcedony/3.13> a skos:Concept ;
    dc:source "https://www.britannica.com/topic/chalcedony" ;
    skos:broader <http://id.acdh.oeaw.ac.at/defc/thesaurus/stone/2.1> ;
    skos:definition "A very fine-grained (cryptocrystalline) variety of the silica mineral quartz. A form of chert, it occurs in concretionary, mammillated, or stalactitic forms of waxy lustre and has a compact fibrous structure, a fine splintery fracture." ;
    skos:editorialNote "dc_finds_material;13" ;
    skos:inScheme <http://id.acdh.oeaw.ac.at/defc/thesaurus/FindsMaterial>,
        <http://id.acdh.oeaw.ac.at/defc/thesaurus/FindsSchema> ;
    skos:prefLabel "Chalzedon"@de,
        "chalcedony"@en .

<http://id.acdh.oeaw.ac.at/defc/thesaurus/chalcedony/5.4> a skos:Concept ;
    dc:source "https://www.britannica.com/topic/chalcedony" ;
    skos:broader <http://id.acdh.oeaw.ac.at/defc/thesaurus/stone/4.025> ;
    skos:definition "A very fine-grained (cryptocrystalline) variety of the silica mineral quartz. A form of chert, it occurs in concretionary, mammillated, or stalactitic forms of waxy lustre and has a compact fibrous structure, a fine splintery fracture, and a great variety. Used to produce lithics." ;
    skos:editorialNote "dc_finds_lithics_raw_material;4" ;
    skos:inScheme <http://id.acdh.oeaw.ac.at/defc/thesaurus/FindsLithicsRawMaterial>,
        <http://id.acdh.oeaw.ac.at/defc/thesaurus/FindsSchema> ;
    skos:prefLabel "Chalzedon"@de,
        "chalcedony"@en .

<http://id.acdh.oeaw.ac.at/defc/thesaurus/chalice/4.185> a skos:Concept ;
    dc:source "OREA" ;
    skos:broader <http://id.acdh.oeaw.ac.at/defc/thesaurus/pottery_form/3.016> ;
    skos:definition "A cup with a foot/pedestal base." ;
    skos:editorialNote "dc_finds_pottery_form;185" ;
    skos:inScheme <http://id.acdh.oeaw.ac.at/defc/thesaurus/FindsPotteryForm>,
        <http://id.acdh.oeaw.ac.at/defc/thesaurus/FindsSchema> ;
    skos:prefLabel "Kelch"@de,
        "chalice"@en .

<http://id.acdh.oeaw.ac.at/defc/thesaurus/chamber_grave/5.7> a skos:Concept ;
    dc:source "0.0" ;
    skos:altLabel "crypt"@en ;
    skos:broader <http://id.acdh.oeaw.ac.at/defc/thesaurus/grave_type/4.083> ;
    skos:definition "A vault or subterranean chamber used as a burial place." ;
    skos:editorialNote "dc_area_gravetype;7" ;
    skos:inScheme <http://id.acdh.oeaw.ac.at/defc/thesaurus/AreaGravetype>,
        <http://id.acdh.oeaw.ac.at/defc/thesaurus/AreaSchema> ;
    skos:prefLabel "chamber grave"@en .

<http://id.acdh.oeaw.ac.at/defc/thesaurus/chamois/5.40> a skos:Concept ;
    dc:source "http://eol.org/pages/331073/overview" ;
    skos:broader <http://id.acdh.oeaw.ac.at/defc/thesaurus/mammal/4.020> ;
    skos:editorialNote "dc_finds_animal_remains_species;40" ;
    skos:inScheme <http://id.acdh.oeaw.ac.at/defc/thesaurus/FindsAnimalRemainsSpecies>,
        <http://id.acdh.oeaw.ac.at/defc/thesaurus/FindsSchema> ;
    skos:prefLabel "Gams"@de,
        "chamois"@en,
        "Rupicapra rupicapra"@la .

<http://id.acdh.oeaw.ac.at/defc/thesaurus/channel/5.2> a skos:Concept ;
    dc:source "OREA" ;
    skos:altLabel "Kanal"@de ;
    skos:broader <http://id.acdh.oeaw.ac.at/defc/thesaurus/installation/4.078> ;
    skos:definition " A gully or groove usually used to drain or channel water." ;
    skos:editorialNote "dc_area_specialfeatures;2" ;
    skos:inScheme <http://id.acdh.oeaw.ac.at/defc/thesaurus/AreaSchema>,
        <http://id.acdh.oeaw.ac.at/defc/thesaurus/AreaSpecialfeatures> ;
    skos:prefLabel "channel"@en .

<http://id.acdh.oeaw.ac.at/defc/thesaurus/charcoal/4.1> a skos:Concept ;
    dc:source "http://dbpedia.org/page/Charcoal" ;
    skos:broader <http://id.acdh.oeaw.ac.at/defc/thesaurus/dating_material/3.046> ;
    skos:definition "Charcoal is a light, black residue, consisting of carbon and any remaining ash, obtained by removing water and other volatile constituents from animal and vegetation substances. It can be used for dating analysis of an archaeological context." ;
    skos:editorialNote "dc_period_datedby;1" ;
    skos:inScheme <http://id.acdh.oeaw.ac.at/defc/thesaurus/PeriodSchema> ;
    skos:prefLabel "Holzkohle"@de,
        "charcoal"@en .

<http://id.acdh.oeaw.ac.at/defc/thesaurus/cheese_pot/4.126> a skos:Concept ;
    dc:source "OREA" ;
    skos:broader <http://id.acdh.oeaw.ac.at/defc/thesaurus/pottery_form/3.016> ;
    skos:definition "A flat open vessel with horizontal row of drillings under the rim." ;
    skos:editorialNote "dc_finds_pottery_form;126" ;
    skos:inScheme <http://id.acdh.oeaw.ac.at/defc/thesaurus/FindsPotteryForm>,
        <http://id.acdh.oeaw.ac.at/defc/thesaurus/FindsSchema> ;
    skos:prefLabel "“Cheese Pot”"@de,
        "cheese pot"@en .

<http://id.acdh.oeaw.ac.at/defc/thesaurus/chicken/5.40> a skos:Concept ;
    dc:source "http://eol.org/pages/45890770/overview" ;
    skos:broader <http://id.acdh.oeaw.ac.at/defc/thesaurus/bird/4.36> ;
    skos:editorialNote "dc_finds_animal_remains_species;40" ;
    skos:inScheme <http://id.acdh.oeaw.ac.at/defc/thesaurus/FindsAnimalRemainsSpecies>,
        <http://id.acdh.oeaw.ac.at/defc/thesaurus/FindsSchema> ;
    skos:prefLabel "Huhn"@de,
        "chicken"@en,
        "Gallus gallus domesticus"@la .

<http://id.acdh.oeaw.ac.at/defc/thesaurus/chickpea/6.5> a skos:Concept ;
    dc:source "http://eol.org/pages/685208/overview" ;
    skos:broader <http://id.acdh.oeaw.ac.at/defc/thesaurus/pea/5.14> ;
    skos:editorialNote "dc_botany_species;5" ;
    skos:inScheme <http://id.acdh.oeaw.ac.at/defc/thesaurus/BotanySpecies>,
        <http://id.acdh.oeaw.ac.at/defc/thesaurus/FindsSchema> ;
    skos:prefLabel "Kichererbse"@de,
        "chickpea"@en,
        "Cicer arietinum"@la .

<http://id.acdh.oeaw.ac.at/defc/thesaurus/chipped_disk/4.134> a skos:Concept ;
    skos:broader <http://id.acdh.oeaw.ac.at/defc/thesaurus/tool/3.1> ;
    skos:editorialNote "dc_finds_small_finds_type;134" ;
    skos:inScheme <http://id.acdh.oeaw.ac.at/defc/thesaurus/FindsSchema>,
        <http://id.acdh.oeaw.ac.at/defc/thesaurus/FindsSmallFindsType> ;
    skos:prefLabel "chipped disk"@en .

<http://id.acdh.oeaw.ac.at/defc/thesaurus/chipped_stone_tool_production/2.3> a skos:Concept ;
    dc:source "OREA" ;
    skos:broader <http://id.acdh.oeaw.ac.at/defc/thesaurus/production/1.042> ;
    skos:definition "The activity of making tools of cryptocrystalline materials by lithic reduction such as striking stone flakes from a core." ;
    skos:editorialNote "dc_interpretation_productiontype;3" ;
    skos:inScheme <http://id.acdh.oeaw.ac.at/defc/thesaurus/InterpretationProductiontype>,
        <http://id.acdh.oeaw.ac.at/defc/thesaurus/InterpretationSchema> ;
    skos:prefLabel "Produktion geschlagener Steinwekzeuge"@de,
        "chipped stone tool production"@en .

<http://id.acdh.oeaw.ac.at/defc/thesaurus/chisel/4.69> a skos:Concept ;
    dc:source "Kipfer, B. A. Dictionary of Artifacts 2007. Blackwell Publishing, Oxford.p.67" ;
    skos:broader <http://id.acdh.oeaw.ac.at/defc/thesaurus/tool/3.1> ;
    skos:definition "A long-bladed hand tool with a beveled cutting edge, stuck with a hammer or mallet to cut or shape wood, stone, or metal." ;
    skos:editorialNote "dc_finds_small_finds_type;69" ;
    skos:inScheme <http://id.acdh.oeaw.ac.at/defc/thesaurus/FindsSchema>,
        <http://id.acdh.oeaw.ac.at/defc/thesaurus/FindsSmallFindsType> ;
    skos:prefLabel "Meisel"@de,
        "chisel"@en .

<http://id.acdh.oeaw.ac.at/defc/thesaurus/chlorite/3.21> a skos:Concept ;
    dc:source "http://dbpedia.org/page/Chlorite" ;
    skos:broader <http://id.acdh.oeaw.ac.at/defc/thesaurus/mineral/2.3> ;
    skos:definition "A chlorite (compound) is a compound that contains this group,with chlorine in oxidation state +3. Chlorites are also known as salts of chlorous acid." ;
    skos:editorialNote "dc_finds_material;21" ;
    skos:inScheme <http://id.acdh.oeaw.ac.at/defc/thesaurus/FindsMaterial>,
        <http://id.acdh.oeaw.ac.at/defc/thesaurus/FindsSchema> ;
    skos:prefLabel "Chlorite"@de,
        "chlorite"@en .

<http://id.acdh.oeaw.ac.at/defc/thesaurus/cicrular_scraper/4.4> a skos:Concept ;
    dc:source "Inizan, M.-L., M. Reduron-Ballinger, H. Roche, J. Tixier 1999, Technology and Terminology of Knapped Stone. Nanterre: CREP., D. Srejovic (ed) 1997, Arheološki Leksikon." ;
    skos:altLabel "round scraper"@en ;
    skos:broader <http://id.acdh.oeaw.ac.at/defc/thesaurus/retouched_tool/3.010> ;
    skos:definition "A discoid scraper with completely retouched convex edge. Synonym: round scraper, discoid scraper." ;
    skos:editorialNote "dc_finds_lithics_retouched_tools;4" ;
    skos:inScheme <http://id.acdh.oeaw.ac.at/defc/thesaurus/FindsLithicsRetouchedTools>,
        <http://id.acdh.oeaw.ac.at/defc/thesaurus/FindsSchema> ;
    skos:prefLabel "cicrular scraper"@en .

<http://id.acdh.oeaw.ac.at/defc/thesaurus/circular/5.2> a skos:Concept ;
    dc:source "OREA" ;
    skos:broader <http://id.acdh.oeaw.ac.at/defc/thesaurus/building_shape/4.076> ;
    skos:definition "A building with a round ground plan." ;
    skos:editorialNote "dc_area_constructionshape;2" ;
    skos:inScheme <http://id.acdh.oeaw.ac.at/defc/thesaurus/AreaConstructionshape>,
        <http://id.acdh.oeaw.ac.at/defc/thesaurus/AreaSchema> ;
    skos:prefLabel "circular"@en .

<http://id.acdh.oeaw.ac.at/defc/thesaurus/cist_grave/5.1> a skos:Concept ;
    dc:source "Kipfer, B. A. Encyclopedic Dictionary of Archaeology. Kluwer Academic/Plenum Publishers, New York. P 119." ;
    skos:broader <http://id.acdh.oeaw.ac.at/defc/thesaurus/grave_type/4.083> ;
    skos:definition "A prehistoric coffin containing either a body or ashes, usually made of stone or a hollowed-put tree, of Europe and Asia. The grave might be lined with stones and covered with slabs or enclosed on four sides by stone slabs standing upright and cloed with" ;
    skos:editorialNote "dc_area_gravetype;1" ;
    skos:inScheme <http://id.acdh.oeaw.ac.at/defc/thesaurus/AreaGravetype>,
        <http://id.acdh.oeaw.ac.at/defc/thesaurus/AreaSchema> ;
    skos:prefLabel "Kistengrab"@de,
        "cist grave"@en .

<http://id.acdh.oeaw.ac.at/defc/thesaurus/claw/4.10> a skos:Concept ;
    dc:source "https://en.oxforddictionaries.com/definition/claw" ;
    skos:broader <http://id.acdh.oeaw.ac.at/defc/thesaurus/animal_remains_part/3.07> ;
    skos:definition "A curved pointed horny nail on each digit of the foot in birds, lizards, and some mammals." ;
    skos:editorialNote "dc_animal_remains_part;10" ;
    skos:inScheme <http://id.acdh.oeaw.ac.at/defc/thesaurus/AnimalRemainsPart>,
        <http://id.acdh.oeaw.ac.at/defc/thesaurus/FindsSchema> ;
    skos:prefLabel "Kralle"@de,
        "claw"@en .

<http://id.acdh.oeaw.ac.at/defc/thesaurus/clay/2.19> a skos:Concept ;
    dc:source "Encyclopaedia Britannica – https://www.britannica.com/science/clay-geology" ;
    skos:altLabel "Bodenart"@de ;
    skos:broader <http://id.acdh.oeaw.ac.at/defc/thesaurus/finds_material/1.01> ;
    skos:definition "Clay, soil paricles the diameters of which are less than 0.005 mm; also a rock that is composed essentially of clay particles. Clay materials are plastic when wet, and coherent when dry. Clay has variety of use such as pottery making and as building material." ;
    skos:editorialNote "dc_finds_material;19" ;
    skos:inScheme <http://id.acdh.oeaw.ac.at/defc/thesaurus/FindsMaterial>,
        <http://id.acdh.oeaw.ac.at/defc/thesaurus/FindsSchema> ;
    skos:prefLabel "Ton"@de,
        "clay"@en .

<http://id.acdh.oeaw.ac.at/defc/thesaurus/clay/4.6> a skos:Concept ;
    dc:source "Encyclopaedia Britannica – https://www.britannica.com/science/clay-geology" ;
    skos:altLabel "Bodenart"@de,
        "Ton"@de ;
    skos:broader <http://id.acdh.oeaw.ac.at/defc/thesaurus/raw_material/3.066> ;
    skos:definition "Clay, soil paricles the diameters of which are less than .5 mm; also a rock that is composed essentially of clay particles. Clay materials are plastic when wet, and coherent when dry. It has been extracetd from a quarry and has probably been used for pottery making and as building material." ;
    skos:editorialNote "dc_area_rawmaterial;6" ;
    skos:inScheme <http://id.acdh.oeaw.ac.at/defc/thesaurus/AreaRawmaterial>,
        <http://id.acdh.oeaw.ac.at/defc/thesaurus/AreaSchema> ;
    skos:prefLabel "Lehm"@de,
        "clay"@en .

<http://id.acdh.oeaw.ac.at/defc/thesaurus/clay_floor/6.22> a skos:Concept ;
    dc:source "OREA" ;
    skos:altLabel "Lehmboden"@de ;
    skos:broader <http://id.acdh.oeaw.ac.at/defc/thesaurus/floor/5.094> ;
    skos:definition "A clay layer on which people tread." ;
    skos:editorialNote "dc_area_specialfeatures;22" ;
    skos:inScheme <http://id.acdh.oeaw.ac.at/defc/thesaurus/AreaSchema>,
        <http://id.acdh.oeaw.ac.at/defc/thesaurus/AreaSpecialfeatures> ;
    skos:prefLabel "clay floor"@en .

<http://id.acdh.oeaw.ac.at/defc/thesaurus/clay_platform/6.26> a skos:Concept ;
    dc:source "M. Brami, PhD after Catalhoyuk Research Project http://www.catalhoyuk.com/database/catal/help_glossary1.asp" ;
    skos:broader <http://id.acdh.oeaw.ac.at/defc/thesaurus/platform/5.093> ;
    skos:definition "A raised flat clay surface with a ridge." ;
    skos:editorialNote "dc_area_specialfeatures;26" ;
    skos:inScheme <http://id.acdh.oeaw.ac.at/defc/thesaurus/AreaSchema>,
        <http://id.acdh.oeaw.ac.at/defc/thesaurus/AreaSpecialfeatures> ;
    skos:prefLabel "clay platform"@en .

<http://id.acdh.oeaw.ac.at/defc/thesaurus/clay_structure/5.16> a skos:Concept ;
    dc:source "OREA" ;
    skos:broader <http://id.acdh.oeaw.ac.at/defc/thesaurus/architecture/4.081> ;
    skos:definition "A clay-made construction." ;
    skos:editorialNote "dc_area_specialfeatures;16" ;
    skos:inScheme <http://id.acdh.oeaw.ac.at/defc/thesaurus/AreaSchema>,
        <http://id.acdh.oeaw.ac.at/defc/thesaurus/AreaSpecialfeatures> ;
    skos:prefLabel "clay structure"@en .

<http://id.acdh.oeaw.ac.at/defc/thesaurus/clay_structure/5.6> a skos:Concept ;
    dc:source "OREA" ;
    skos:broader <http://id.acdh.oeaw.ac.at/defc/thesaurus/occupation_evidence/4.088> ;
    skos:definition "A manmade construction of clay found inside of a cave or rockshelter as the evidence for human occupation." ;
    skos:editorialNote "dc_area_evidenceofocupation;6" ;
    skos:inScheme <http://id.acdh.oeaw.ac.at/defc/thesaurus/AreaEvidenceofocupation>,
        <http://id.acdh.oeaw.ac.at/defc/thesaurus/AreaSchema> ;
    skos:prefLabel "Lehmstruktur"@de,
        "clay structure"@en .

<http://id.acdh.oeaw.ac.at/defc/thesaurus/coarse/4.252> a skos:Concept ;
    dc:source "OREA" ;
    skos:altLabel "coarse ware"@en ;
    skos:broader <http://id.acdh.oeaw.ac.at/defc/thesaurus/pottery_surface_treatment/3.019> ;
    skos:definition "Sherds or vessels with a coarser appearance that is achieved throzgh thicker walls, large-sized grit inclusions and the absence of careful surface treatment." ;
    skos:editorialNote "dc_finds_pottery_decoration;252" ;
    skos:inScheme <http://id.acdh.oeaw.ac.at/defc/thesaurus/FindsPotteryDecoration>,
        <http://id.acdh.oeaw.ac.at/defc/thesaurus/FindsSchema> ;
    skos:prefLabel "grob"@de,
        "coarse"@en .

<http://id.acdh.oeaw.ac.at/defc/thesaurus/coarse_urfirnis/5.164> a skos:Concept ;
    dc:source "OREA" ;
    skos:broader <http://id.acdh.oeaw.ac.at/defc/thesaurus/incised/4.168> ;
    skos:definition "Coarse pottery decorated with a glaze-like paint." ;
    skos:editorialNote "dc_finds_pottery_decoration;164" ;
    skos:inScheme <http://id.acdh.oeaw.ac.at/defc/thesaurus/FindsPotteryDecoration>,
        <http://id.acdh.oeaw.ac.at/defc/thesaurus/FindsSchema> ;
    skos:prefLabel "Grober Urfirnis"@de,
        "coarse urfirnis"@en .

<http://id.acdh.oeaw.ac.at/defc/thesaurus/coast/2.1> a skos:Concept ;
    dc:source "https://en.oxforddictionaries.com/definition/coast" ;
    skos:broader "topography/1.099" ;
    skos:definition "A part of land adjoining or near the sea."@en ;
    skos:editorialNote "dc_site_topography;1" ;
    skos:inScheme <http://id.acdh.oeaw.ac.at/defc/thesaurus/SiteSchema>,
        "SiteTopography" ;
    skos:prefLabel "Küste"@de,
        "coast"@en .

<http://id.acdh.oeaw.ac.at/defc/thesaurus/coil/4.133> a skos:Concept ;
    skos:broader <http://id.acdh.oeaw.ac.at/defc/thesaurus/tool/3.1> ;
    skos:editorialNote "dc_finds_small_finds_type;133" ;
    skos:inScheme <http://id.acdh.oeaw.ac.at/defc/thesaurus/FindsSchema>,
        <http://id.acdh.oeaw.ac.at/defc/thesaurus/FindsSmallFindsType> ;
    skos:prefLabel "Spule"@de,
        "coil"@en .

<http://id.acdh.oeaw.ac.at/defc/thesaurus/collared_bowl/5.146> a skos:Concept ;
    dc:source "OREA" ;
    skos:broader <http://id.acdh.oeaw.ac.at/defc/thesaurus/bowl/4.115> ;
    skos:definition "A shallow open vessel with a raised band or series of bands at the base of the neck." ;
    skos:editorialNote "dc_finds_pottery_form;146" ;
    skos:inScheme <http://id.acdh.oeaw.ac.at/defc/thesaurus/FindsPotteryForm>,
        <http://id.acdh.oeaw.ac.at/defc/thesaurus/FindsSchema> ;
    skos:prefLabel "Kragenschale"@de,
        "collared bowl"@en .

<http://id.acdh.oeaw.ac.at/defc/thesaurus/collared_jar/5.127> a skos:Concept ;
    dc:source "OREA" ;
    skos:broader <http://id.acdh.oeaw.ac.at/defc/thesaurus/jar/4.145> ;
    skos:definition "A closed vessel with two or non handles with a raised band or series of bands at the base of the neck." ;
    skos:editorialNote "dc_finds_pottery_form;127" ;
    skos:inScheme <http://id.acdh.oeaw.ac.at/defc/thesaurus/FindsPotteryForm>,
        <http://id.acdh.oeaw.ac.at/defc/thesaurus/FindsSchema> ;
    skos:prefLabel "Kragenhalsamphore"@de,
        "collared jar"@en .

<http://id.acdh.oeaw.ac.at/defc/thesaurus/complete/4.1> a skos:Concept ;
    dc:source "OREA" ;
    skos:broader <http://id.acdh.oeaw.ac.at/defc/thesaurus/completness_of_animal_remains/3.05> ;
    skos:definition "The animal remains found were complete." ;
    skos:editorialNote "dc_finds_animal_remains_completness;1" ;
    skos:inScheme <http://id.acdh.oeaw.ac.at/defc/thesaurus/FindsAnimalRemainsCompletness>,
        <http://id.acdh.oeaw.ac.at/defc/thesaurus/FindsSchema> ;
    skos:prefLabel "complete"@en .

<http://id.acdh.oeaw.ac.at/defc/thesaurus/concave_flat_base/5.139> a skos:Concept ;
    dc:source "Kipfer, B. A. Dictionary of Artifacts 2007. Blackwell Publishing, Oxford.p 290" ;
    skos:broader <http://id.acdh.oeaw.ac.at/defc/thesaurus/base/4.032> ;
    skos:definition "Flat lower portion of a vessel from the lower boudary of the body to the place that would normally be in contact with the surface on which the vessel rested in a concave/inverted shape." ;
    skos:editorialNote "dc_finds_pottery_detail;139" ;
    skos:inScheme <http://id.acdh.oeaw.ac.at/defc/thesaurus/FindsPotteryDetail>,
        <http://id.acdh.oeaw.ac.at/defc/thesaurus/FindsSchema> ;
    skos:prefLabel "Konkaver Flachboden"@de,
        "concave flat base"@en .

<http://id.acdh.oeaw.ac.at/defc/thesaurus/concrete/6.16> a skos:Concept ;
    dc:source "Mollett, J. W. 1966 An Illustrated Dictionary of Art and Archaeology. American Archives of World Art Inc., New York, p. 86" ;
    skos:broader <http://id.acdh.oeaw.ac.at/defc/thesaurus/building_material/5.089> ;
    skos:definition "A construction material, a mixture of gravel, pebbles, or broken stone with cement." ;
    skos:editorialNote "dc_area_buildingtechnique;16" ;
    skos:inScheme <http://id.acdh.oeaw.ac.at/defc/thesaurus/AreaBuildingtechnique>,
        <http://id.acdh.oeaw.ac.at/defc/thesaurus/AreaSchema> ;
    skos:prefLabel "concrete"@en .

<http://id.acdh.oeaw.ac.at/defc/thesaurus/cone/4.119> a skos:Concept ;
    dc:source "Kipfer, B. A. Dictionary of Artifacts 2007. Blackwell Publishing, Oxford.p 79" ;
    skos:broader <http://id.acdh.oeaw.ac.at/defc/thesaurus/tool/3.1> ;
    skos:definition "Small, elongated pyramid made of controlled mixtures of ceramic materials in a numbered sequence that softens and bends when heated." ;
    skos:editorialNote "dc_finds_small_finds_type;119" ;
    skos:inScheme <http://id.acdh.oeaw.ac.at/defc/thesaurus/FindsSchema>,
        <http://id.acdh.oeaw.ac.at/defc/thesaurus/FindsSmallFindsType> ;
    skos:prefLabel "Kegel"@de,
        "cone"@en .

<http://id.acdh.oeaw.ac.at/defc/thesaurus/conical_core/4.4> a skos:Concept ;
    dc:source "OREA" ;
    skos:broader <http://id.acdh.oeaw.ac.at/defc/thesaurus/core/3.012> ;
    skos:definition "A blade core of a conical shape." ;
    skos:editorialNote "dc_finds_lithics_core_shape;4" ;
    skos:inScheme <http://id.acdh.oeaw.ac.at/defc/thesaurus/FindsLithicsCoreShape>,
        <http://id.acdh.oeaw.ac.at/defc/thesaurus/FindsSchema> ;
    skos:prefLabel "conical core"@en .

<http://id.acdh.oeaw.ac.at/defc/thesaurus/consecutive_burials/5.1> a skos:Concept ;
    dc:source "OREA" ;
    skos:broader <http://id.acdh.oeaw.ac.at/defc/thesaurus/grave_disturbance/4.084> ;
    skos:definition "The grave has been intersected with another grave." ;
    skos:editorialNote "dc_area_manipulationofgraves;1" ;
    skos:inScheme <http://id.acdh.oeaw.ac.at/defc/thesaurus/AreaManipulationofgraves>,
        <http://id.acdh.oeaw.ac.at/defc/thesaurus/AreaSchema> ;
    skos:prefLabel "Nachbestattung"@de,
        "consecutive burials"@en .

<http://id.acdh.oeaw.ac.at/defc/thesaurus/construction_of_settlement/5.2> a skos:Concept ;
    dc:source "OREA" ;
    skos:broader <http://id.acdh.oeaw.ac.at/defc/thesaurus/grave_disturbance/4.084> ;
    skos:definition "The grave has been disrupted because of building of a new settlement." ;
    skos:editorialNote "dc_area_manipulationofgraves;2" ;
    skos:inScheme <http://id.acdh.oeaw.ac.at/defc/thesaurus/AreaManipulationofgraves>,
        <http://id.acdh.oeaw.ac.at/defc/thesaurus/AreaSchema> ;
    skos:prefLabel "Störung durch nachfolgende Siedlung"@de,
        "construction of settlement"@en .

<http://id.acdh.oeaw.ac.at/defc/thesaurus/copper/3.31> a skos:Concept ;
    dc:source "http://dbpedia.org/page/Copper" ;
    skos:broader <http://id.acdh.oeaw.ac.at/defc/thesaurus/metal/2.9> ;
    skos:definition "Copper (Cu) is a reddish, extremely ductile metal that can be found in the free metallic state in nature." ;
    skos:editorialNote "dc_finds_material;31" ;
    skos:inScheme <http://id.acdh.oeaw.ac.at/defc/thesaurus/FindsMaterial>,
        <http://id.acdh.oeaw.ac.at/defc/thesaurus/FindsSchema> ;
    skos:prefLabel "Kupfer"@de,
        "copper"@en .

<http://id.acdh.oeaw.ac.at/defc/thesaurus/copper/5.2> a skos:Concept ;
    dc:source "Encyclopaedia Britannica - https://www.britannica.com/science/copper" ;
    skos:broader <http://id.acdh.oeaw.ac.at/defc/thesaurus/metal/4.7> ;
    skos:definition "Copper (Cu) is a reddish, extremely ductile metal that can be found in the free metallic state in nature. Extracted from a quarry site." ;
    skos:editorialNote "dc_area_rawmaterial;2" ;
    skos:inScheme <http://id.acdh.oeaw.ac.at/defc/thesaurus/AreaRawmaterial>,
        <http://id.acdh.oeaw.ac.at/defc/thesaurus/AreaSchema> ;
    skos:prefLabel "Kupfer"@de,
        "copper"@en .

<http://id.acdh.oeaw.ac.at/defc/thesaurus/core_fragment/4.5> a skos:Concept ;
    dc:source "OREA" ;
    skos:broader <http://id.acdh.oeaw.ac.at/defc/thesaurus/core/3.012> ;
    skos:definition "A fragment of a core (regardless typology, used when the core is incomplete, or the main type cannot be determined due to fragmentation) " ;
    skos:editorialNote "dc_finds_lithics_core_shape;5" ;
    skos:inScheme <http://id.acdh.oeaw.ac.at/defc/thesaurus/FindsLithicsCoreShape>,
        <http://id.acdh.oeaw.ac.at/defc/thesaurus/FindsSchema> ;
    skos:prefLabel "core fragment"@en .

<http://id.acdh.oeaw.ac.at/defc/thesaurus/cortical_blade/4.6> a skos:Concept ;
    skos:broader <http://id.acdh.oeaw.ac.at/defc/thesaurus/core_preparation/3.013> ;
    skos:editorialNote "dc_finds_lithics_core_shape;6" ;
    skos:inScheme <http://id.acdh.oeaw.ac.at/defc/thesaurus/FindsLithicsCoreShape>,
        <http://id.acdh.oeaw.ac.at/defc/thesaurus/FindsSchema> ;
    skos:prefLabel "cortical blade"@en .

<http://id.acdh.oeaw.ac.at/defc/thesaurus/courtyard/5.23> a skos:Concept ;
    dc:source "https://standards.phorio.com/?t=definition&code=6532938992" ;
    skos:broader <http://id.acdh.oeaw.ac.at/defc/thesaurus/place/4.082> ;
    skos:definition "An accessible open-air space surrounded on three or four sides." ;
    skos:editorialNote "dc_area_specialfeatures;23" ;
    skos:inScheme <http://id.acdh.oeaw.ac.at/defc/thesaurus/AreaSchema>,
        <http://id.acdh.oeaw.ac.at/defc/thesaurus/AreaSpecialfeatures> ;
    skos:prefLabel "courtyard"@en .

<http://id.acdh.oeaw.ac.at/defc/thesaurus/cremation/6.1> a skos:Concept ;
    skos:broader <http://id.acdh.oeaw.ac.at/defc/thesaurus/human_remains_type/5.096> ;
    skos:editorialNote "dc_area_typeofhumanremains;1" ;
    skos:inScheme <http://id.acdh.oeaw.ac.at/defc/thesaurus/AreaSchema>,
        <http://id.acdh.oeaw.ac.at/defc/thesaurus/AreaTypeofhumanremains> ;
    skos:prefLabel "cremation"@en .

<http://id.acdh.oeaw.ac.at/defc/thesaurus/crescent-shaped_handle/5.171> a skos:Concept ;
    dc:source "OREA" ;
    skos:broader <http://id.acdh.oeaw.ac.at/defc/thesaurus/handle/4.031> ;
    skos:definition "(Half)moon shaped handle." ;
    skos:editorialNote "dc_finds_pottery_detail;171" ;
    skos:inScheme <http://id.acdh.oeaw.ac.at/defc/thesaurus/FindsPotteryDetail>,
        <http://id.acdh.oeaw.ac.at/defc/thesaurus/FindsSchema> ;
    skos:prefLabel "Mondförmiger Henkel"@de,
        "crescent-shaped handle"@en .

<http://id.acdh.oeaw.ac.at/defc/thesaurus/crested_blade/4.7> a skos:Concept ;
    skos:broader <http://id.acdh.oeaw.ac.at/defc/thesaurus/core_preparation/3.013> ;
    skos:editorialNote "dc_finds_lithics_core_shape;7" ;
    skos:inScheme <http://id.acdh.oeaw.ac.at/defc/thesaurus/FindsLithicsCoreShape>,
        <http://id.acdh.oeaw.ac.at/defc/thesaurus/FindsSchema> ;
    skos:prefLabel "crested blade"@en .

<http://id.acdh.oeaw.ac.at/defc/thesaurus/crested_flake/4.8> a skos:Concept ;
    skos:broader <http://id.acdh.oeaw.ac.at/defc/thesaurus/core_preparation/3.013> ;
    skos:editorialNote "dc_finds_lithics_core_shape;8" ;
    skos:inScheme <http://id.acdh.oeaw.ac.at/defc/thesaurus/FindsLithicsCoreShape>,
        <http://id.acdh.oeaw.ac.at/defc/thesaurus/FindsSchema> ;
    skos:prefLabel "crested flake"@en .

<http://id.acdh.oeaw.ac.at/defc/thesaurus/crucible/4.67> a skos:Concept ;
    dc:source "Kipfer, B. A. Dictionary of Artifacts 2007. Blackwell Publishing, Oxford.p.87" ;
    skos:broader <http://id.acdh.oeaw.ac.at/defc/thesaurus/tool/3.1> ;
    skos:definition "A small, coarse pottery (or other refractory material) vessel used for holding molten metal during melting, testing, or casting." ;
    skos:editorialNote "dc_finds_small_finds_type;67" ;
    skos:inScheme <http://id.acdh.oeaw.ac.at/defc/thesaurus/FindsSchema>,
        <http://id.acdh.oeaw.ac.at/defc/thesaurus/FindsSmallFindsType> ;
    skos:prefLabel "Schmelztiegel"@de,
        "crucible"@en .

<http://id.acdh.oeaw.ac.at/defc/thesaurus/cup/4.107> a skos:Concept ;
    dc:source "OREA" ;
    skos:broader <http://id.acdh.oeaw.ac.at/defc/thesaurus/pottery_form/3.016> ;
    skos:definition "A small open vessel for drinking from, usually with a handle." ;
    skos:editorialNote "dc_finds_pottery_form;107" ;
    skos:inScheme <http://id.acdh.oeaw.ac.at/defc/thesaurus/FindsPotteryForm>,
        <http://id.acdh.oeaw.ac.at/defc/thesaurus/FindsSchema> ;
    skos:prefLabel "Tasse"@de,
        "cup"@en .

<http://id.acdh.oeaw.ac.at/defc/thesaurus/curved_tapered-up_rim/5.140> a skos:Concept ;
    dc:source "OREA" ;
    skos:broader <http://id.acdh.oeaw.ac.at/defc/thesaurus/rim/4.033> ;
    skos:definition "Curved and thinned portion of a vessel closest to its orifice." ;
    skos:editorialNote "dc_finds_pottery_detail;140" ;
    skos:inScheme <http://id.acdh.oeaw.ac.at/defc/thesaurus/FindsPotteryDetail>,
        <http://id.acdh.oeaw.ac.at/defc/thesaurus/FindsSchema> ;
    skos:prefLabel "Gewölbter, sich verjügender Rand"@de,
        "curved tapered-up rim"@en .

<http://id.acdh.oeaw.ac.at/defc/thesaurus/dagger/5.72> a skos:Concept ;
    dc:source "https://en.oxforddictionaries.com/definition/dagger" ;
    skos:broader <http://id.acdh.oeaw.ac.at/defc/thesaurus/weapon/4.030> ;
    skos:definition "A short knife with a pointed and edged blade, used as a weapon." ;
    skos:editorialNote "dc_finds_small_finds_type;72" ;
    skos:inScheme <http://id.acdh.oeaw.ac.at/defc/thesaurus/FindsSchema>,
        <http://id.acdh.oeaw.ac.at/defc/thesaurus/FindsSmallFindsType> ;
    skos:prefLabel "Dolch"@de,
        "dagger"@en .

<http://id.acdh.oeaw.ac.at/defc/thesaurus/dark_faced_burished_ware_(dfbw)/5.247> a skos:Concept ;
    dc:source "OREA" ;
    skos:broader <http://id.acdh.oeaw.ac.at/defc/thesaurus/burnished/4.297> ;
    skos:definition "Burnished ware decorated with dark slip." ;
    skos:editorialNote "dc_finds_pottery_decoration;247" ;
    skos:inScheme <http://id.acdh.oeaw.ac.at/defc/thesaurus/FindsPotteryDecoration>,
        <http://id.acdh.oeaw.ac.at/defc/thesaurus/FindsSchema> ;
    skos:prefLabel "Geglättete Keramik mit dunklem Überzug"@de,
        "dark faced burished ware (dfbw)"@en .

<http://id.acdh.oeaw.ac.at/defc/thesaurus/deep_bowl/5.178> a skos:Concept ;
    dc:source "OREA" ;
    skos:broader <http://id.acdh.oeaw.ac.at/defc/thesaurus/bowl/4.115> ;
    skos:definition "A low open vessel with rim diameter same or smaller than height." ;
    skos:editorialNote "dc_finds_pottery_form;178" ;
    skos:inScheme <http://id.acdh.oeaw.ac.at/defc/thesaurus/FindsPotteryForm>,
        <http://id.acdh.oeaw.ac.at/defc/thesaurus/FindsSchema> ;
    skos:prefLabel "Schüssel"@de,
        "deep bowl"@en .

<http://id.acdh.oeaw.ac.at/defc/thesaurus/dendrochronology/4.2> a skos:Concept ;
    dc:source "http://thesaurus.historicengland.org.uk/thesaurus_term.asp?thes_no=560&term_no=142131" ;
    skos:broader <http://id.acdh.oeaw.ac.at/defc/thesaurus/dating_method/3.045> ;
    skos:definition "The measuring of annual tree-ring growth shown by most tree species in temperated regions. Regional chronologies are required to date any particular priece of wood, the longest of which, for Germany, works for the present to approximately 14000 years ago." ;
    skos:editorialNote "dc_period_datingmethod;2" ;
    skos:inScheme <http://id.acdh.oeaw.ac.at/defc/thesaurus/PeriodSchema> ;
    skos:prefLabel "Dendrochronologie"@de,
        "dendrochronology"@en .

<http://id.acdh.oeaw.ac.at/defc/thesaurus/denticulate/4.5> a skos:Concept ;
    dc:source "Inizan, M.-L., M. Reduron-Ballinger, H. Roche, J. Tixier 1999, Technology and Terminology of Knapped Stone. Nanterre: CREP., D. Srejovic (ed) 1997, Arheološki Leksikon." ;
    skos:altLabel "denticulated tool"@en ;
    skos:broader <http://id.acdh.oeaw.ac.at/defc/thesaurus/retouched_tool/3.010> ;
    skos:definition "A blade or flake with several small tooth-like (dentate or serrated) notches on the working edge." ;
    skos:editorialNote "dc_finds_lithics_retouched_tools;5" ;
    skos:inScheme <http://id.acdh.oeaw.ac.at/defc/thesaurus/FindsLithicsRetouchedTools>,
        <http://id.acdh.oeaw.ac.at/defc/thesaurus/FindsSchema> ;
    skos:prefLabel "gezähnt"@de,
        "denticulate"@en .

<http://id.acdh.oeaw.ac.at/defc/thesaurus/dimini_bowl/5.129> a skos:Concept ;
    dc:source "St. Souvatzi, A Social Archaeology of Households in Neolithic Greece. An Anthropological Approach (Cambridge 2008) 255." ;
    skos:altLabel "phiale"@en ;
    skos:broader <http://id.acdh.oeaw.ac.at/defc/thesaurus/bowl/4.115> ;
    skos:definition "A vessel with a conical body, flat base, and strongly inverted rim. Sets of two or four small string-hole lugs are placed symmetrically arround the rim. Interior and exterior surface are fully covered with various geometrical design elements and patterns." ;
    skos:editorialNote "dc_finds_pottery_form;129" ;
    skos:inScheme <http://id.acdh.oeaw.ac.at/defc/thesaurus/FindsPotteryForm>,
        <http://id.acdh.oeaw.ac.at/defc/thesaurus/FindsSchema> ;
    skos:prefLabel "Dimini Schale"@de,
        "dimini bowl"@en .

<http://id.acdh.oeaw.ac.at/defc/thesaurus/direct_percussion/5.1> a skos:Concept ;
    dc:source "Inizan, M.-L., M. Reduron-Ballinger, H. Roche, J. Tixier 1999, Technology and Terminology of Knapped Stone. Nanterre: CREP. p. 148." ;
    skos:broader <http://id.acdh.oeaw.ac.at/defc/thesaurus/lithics_technology/4.023> ;
    skos:definition "The action of striking one object with another. Direct percussion is directly applies by a hammer." ;
    skos:editorialNote "dc_finds_lithics_technology;1" ;
    skos:inScheme <http://id.acdh.oeaw.ac.at/defc/thesaurus/FindsLithicsTechnology>,
        <http://id.acdh.oeaw.ac.at/defc/thesaurus/FindsSchema> ;
    skos:prefLabel "direct percussion"@en .

<http://id.acdh.oeaw.ac.at/defc/thesaurus/disc/4.63> a skos:Concept ;
    dc:source "Kipfer, B. A. Dictionary of Artifacts 2007. Blackwell Publishing, Oxford.p.96" ;
    skos:broader <http://id.acdh.oeaw.ac.at/defc/thesaurus/tool/3.1> ;
    skos:definition "A stone artifact circular in shape and concave on both sides usually of quartz, granite, flint, hematite, slate, or basalt. They range from 0.25 to 23 cm in diameter and from 0.5 to 9 kg in weight. Some have a hole through the center and others have flanges around the edges.They seemed to have a ceremonial or ritual purpose or were used for mixing herbs or medicines." ;
    skos:editorialNote "dc_finds_small_finds_type;63" ;
    skos:inScheme <http://id.acdh.oeaw.ac.at/defc/thesaurus/FindsSchema>,
        <http://id.acdh.oeaw.ac.at/defc/thesaurus/FindsSmallFindsType> ;
    skos:prefLabel "Scheibe"@de,
        "disc"@en .

<http://id.acdh.oeaw.ac.at/defc/thesaurus/dog/5.10> a skos:Concept ;
    dc:source "http://eol.org/pages/1228387/overview" ;
    skos:broader <http://id.acdh.oeaw.ac.at/defc/thesaurus/mammal/4.020> ;
    skos:editorialNote "dc_finds_animal_remains_species;10" ;
    skos:inScheme <http://id.acdh.oeaw.ac.at/defc/thesaurus/FindsAnimalRemainsSpecies>,
        <http://id.acdh.oeaw.ac.at/defc/thesaurus/FindsSchema> ;
    skos:prefLabel "Hund"@de,
        "dog"@en,
        "Canis familiaris"@la .

<http://id.acdh.oeaw.ac.at/defc/thesaurus/dome-shaped_shallow_bowl/5.108> a skos:Concept ;
    dc:source "OREA" ;
    skos:broader <http://id.acdh.oeaw.ac.at/defc/thesaurus/bowl/4.115> ;
    skos:definition "A hemispherical low open vessel with a rim diameter double than the height." ;
    skos:editorialNote "dc_finds_pottery_form;108" ;
    skos:inScheme <http://id.acdh.oeaw.ac.at/defc/thesaurus/FindsPotteryForm>,
        <http://id.acdh.oeaw.ac.at/defc/thesaurus/FindsSchema> ;
    skos:prefLabel "Kalottenförmige Schale"@de,
        "dome-shaped shallow bowl"@en .

<http://id.acdh.oeaw.ac.at/defc/thesaurus/donkey/5.21> a skos:Concept ;
    dc:source "http://eol.org/pages/328647/overview" ;
    skos:broader <http://id.acdh.oeaw.ac.at/defc/thesaurus/mammal/4.020> ;
    skos:editorialNote "dc_finds_animal_remains_species;21" ;
    skos:inScheme <http://id.acdh.oeaw.ac.at/defc/thesaurus/FindsAnimalRemainsSpecies>,
        <http://id.acdh.oeaw.ac.at/defc/thesaurus/FindsSchema> ;
    skos:prefLabel "Esel"@de,
        "donkey"@en,
        "Equus asinus"@la .

<http://id.acdh.oeaw.ac.at/defc/thesaurus/double-baked_blade/4.7> a skos:Concept ;
    dc:source "Inizan, M.-L., M. Reduron-Ballinger, H. Roche, J. Tixier 1999, Technology and Terminology of Knapped Stone. Nanterre: CREP., D. Srejovic (ed) 1997, Arheološki Leksikon." ;
    skos:broader <http://id.acdh.oeaw.ac.at/defc/thesaurus/retouched_tool/3.010> ;
    skos:definition "A blade with both blunted edges. According to size, backed blades are different from backed bladelets, which belong to the category of microliths." ;
    skos:editorialNote "dc_finds_lithics_retouched_tools;7" ;
    skos:inScheme <http://id.acdh.oeaw.ac.at/defc/thesaurus/FindsLithicsRetouchedTools>,
        <http://id.acdh.oeaw.ac.at/defc/thesaurus/FindsSchema> ;
    skos:prefLabel "double-baked blade"@en .

<http://id.acdh.oeaw.ac.at/defc/thesaurus/double-horned_wishbone_handle/6.156> a skos:Concept ;
    dc:source "OREA" ;
    skos:broader <http://id.acdh.oeaw.ac.at/defc/thesaurus/wishbone_handle/5.93> ;
    skos:definition "A liminal, horizontal, bird-bone shaped, loop handle with two objects applied that are narrow at one end and much wider at the other." ;
    skos:editorialNote "dc_finds_pottery_detail;156" ;
    skos:inScheme <http://id.acdh.oeaw.ac.at/defc/thesaurus/FindsPotteryDetail>,
        <http://id.acdh.oeaw.ac.at/defc/thesaurus/FindsSchema> ;
    skos:prefLabel "Wishbonehenkel mit doppelten Hornaufsatz"@de,
        "double-horned wishbone handle"@en .

<http://id.acdh.oeaw.ac.at/defc/thesaurus/double_tab_handle/6.97> a skos:Concept ;
    dc:source "OREA" ;
    skos:broader <http://id.acdh.oeaw.ac.at/defc/thesaurus/tab_handle/5.96> ;
    skos:definition "Double flat handle." ;
    skos:editorialNote "dc_finds_pottery_detail;97" ;
    skos:inScheme <http://id.acdh.oeaw.ac.at/defc/thesaurus/FindsPotteryDetail>,
        <http://id.acdh.oeaw.ac.at/defc/thesaurus/FindsSchema> ;
    skos:prefLabel "Doppelter Grifflappen"@de,
        "double tab handle"@en .

<http://id.acdh.oeaw.ac.at/defc/thesaurus/double_truncation/4.6> a skos:Concept ;
    dc:source "Inizan, M.-L., M. Reduron-Ballinger, H. Roche, J. Tixier 1999, Technology and Terminology of Knapped Stone. Nanterre: CREP., D. Srejovic (ed) 1997, Arheološki Leksikon." ;
    skos:broader <http://id.acdh.oeaw.ac.at/defc/thesaurus/retouched_tool/3.010> ;
    skos:definition "A blade with a steep retouch made on both broken ends." ;
    skos:editorialNote "dc_finds_lithics_retouched_tools;6" ;
    skos:inScheme <http://id.acdh.oeaw.ac.at/defc/thesaurus/FindsLithicsRetouchedTools>,
        <http://id.acdh.oeaw.ac.at/defc/thesaurus/FindsSchema> ;
    skos:prefLabel "double truncation"@en .

<http://id.acdh.oeaw.ac.at/defc/thesaurus/drill/4.121> a skos:Concept ;
    dc:source "Inizan, M.-L., M. Reduron-Ballinger, H. Roche, J. Tixier 1999, Technology and Terminology of Knapped Stone. Nanterre: CREP., D. Srejovic (ed) 1997, Arheološki Leksikon." ;
    skos:altLabel "Preforator"@en,
        "borer"@en ;
    skos:broader <http://id.acdh.oeaw.ac.at/defc/thesaurus/tool/3.1> ;
    skos:definition "A blade (or rarely flake) where a retoch forms a pointed end used for making holes." ;
    skos:editorialNote "dc_finds_small_finds_type;121" ;
    skos:inScheme <http://id.acdh.oeaw.ac.at/defc/thesaurus/FindsSchema>,
        <http://id.acdh.oeaw.ac.at/defc/thesaurus/FindsSmallFindsType> ;
    skos:prefLabel "Bohrer"@de,
        "drill"@en .

<http://id.acdh.oeaw.ac.at/defc/thesaurus/drill/4.8> a skos:Concept ;
    dc:source "Inizan, M.-L., M. Reduron-Ballinger, H. Roche, J. Tixier 1999, Technology and Terminology of Knapped Stone. Nanterre: CREP., D. Srejovic (ed) 1997, Arheološki Leksikon." ;
    skos:altLabel "borer"@en,
        "preforator"@en ;
    skos:broader <http://id.acdh.oeaw.ac.at/defc/thesaurus/retouched_tool/3.010> ;
    skos:definition "A blade (or rarely flake) where a retoch forms a pointed end used for making holes." ;
    skos:editorialNote "dc_finds_lithics_retouched_tools;8" ;
    skos:inScheme <http://id.acdh.oeaw.ac.at/defc/thesaurus/FindsLithicsRetouchedTools>,
        <http://id.acdh.oeaw.ac.at/defc/thesaurus/FindsSchema> ;
    skos:prefLabel "Bohrer"@de,
        "drill"@en .

<http://id.acdh.oeaw.ac.at/defc/thesaurus/dross/4.129> a skos:Concept ;
    dc:source "Kipfer, B. A. Dictionary of Artifacts 2007. Blackwell Publishing, Oxford.p. 99" ;
    skos:broader <http://id.acdh.oeaw.ac.at/defc/thesaurus/other/3.4> ;
    skos:definition "Scum formed by oxidation at the surface of molten merals." ;
    skos:editorialNote "dc_finds_small_finds_type;129" ;
    skos:inScheme <http://id.acdh.oeaw.ac.at/defc/thesaurus/FindsSchema>,
        <http://id.acdh.oeaw.ac.at/defc/thesaurus/FindsSmallFindsType> ;
    skos:prefLabel "Schrott"@de,
        "dross"@en .

<http://id.acdh.oeaw.ac.at/defc/thesaurus/dugout/4.115> a skos:Concept ;
    dc:source "Kipfer, B. A. Dictionary of Artifacts 2007. Blackwell Publishing, Oxford.p 99" ;
    skos:broader <http://id.acdh.oeaw.ac.at/defc/thesaurus/other/3.4> ;
    skos:definition "A simple canoe made from a single tree hollowed out by burning or chopping." ;
    skos:editorialNote "dc_finds_small_finds_type;115" ;
    skos:inScheme <http://id.acdh.oeaw.ac.at/defc/thesaurus/FindsSchema>,
        <http://id.acdh.oeaw.ac.at/defc/thesaurus/FindsSmallFindsType> ;
    skos:prefLabel "Einbaum"@de,
        "dugout"@en .

<http://id.acdh.oeaw.ac.at/defc/thesaurus/ear_handle/5.118> a skos:Concept ;
    dc:source "OREA" ;
    skos:broader <http://id.acdh.oeaw.ac.at/defc/thesaurus/handle/4.031> ;
    skos:definition "A vertical loop handle in a shape of an ear." ;
    skos:editorialNote "dc_finds_pottery_detail;118" ;
    skos:inScheme <http://id.acdh.oeaw.ac.at/defc/thesaurus/FindsPotteryDetail>,
        <http://id.acdh.oeaw.ac.at/defc/thesaurus/FindsSchema> ;
    skos:prefLabel "Ohrhenkel"@de,
        "ear handle"@en .

<http://id.acdh.oeaw.ac.at/defc/thesaurus/ear_plug/4.79> a skos:Concept ;
    dc:source "http://dbpedia.org/page/Plug_(jewellery)" ;
    skos:altLabel "earspool"@en,
        "plug"@en ;
    skos:broader <http://id.acdh.oeaw.ac.at/defc/thesaurus/jewellery/3.2> ;
    skos:definition "A short cylindrical piece of jewellery commonly worn in larger-gauge body piercings." ;
    skos:editorialNote "dc_finds_small_finds_type;79" ;
    skos:inScheme <http://id.acdh.oeaw.ac.at/defc/thesaurus/FindsSchema>,
        <http://id.acdh.oeaw.ac.at/defc/thesaurus/FindsSmallFindsType> ;
    skos:prefLabel "Ohrstecker"@de,
        "ear plug"@en .

<http://id.acdh.oeaw.ac.at/defc/thesaurus/earring/4.81> a skos:Concept ;
    dc:source "http://dbpedia.org/page/Earring" ;
    skos:broader <http://id.acdh.oeaw.ac.at/defc/thesaurus/jewellery/3.2> ;
    skos:definition "An earring is a piece of jewellery attached to the ear via a piercing in the earlobe or another external part of the ear." ;
    skos:editorialNote "dc_finds_small_finds_type;81" ;
    skos:inScheme <http://id.acdh.oeaw.ac.at/defc/thesaurus/FindsSchema>,
        <http://id.acdh.oeaw.ac.at/defc/thesaurus/FindsSmallFindsType> ;
    skos:prefLabel "Ohrring"@de,
        "earring"@en .

<http://id.acdh.oeaw.ac.at/defc/thesaurus/einkorn_wheat/6.6> a skos:Concept ;
    dc:source "http://eol.org/pages/1115242/overview" ;
    skos:broader <http://id.acdh.oeaw.ac.at/defc/thesaurus/wheat/5.39> ;
    skos:editorialNote "dc_botany_species;6" ;
    skos:inScheme <http://id.acdh.oeaw.ac.at/defc/thesaurus/BotanySpecies>,
        <http://id.acdh.oeaw.ac.at/defc/thesaurus/FindsSchema> ;
    skos:prefLabel "Einkorn"@de,
        "einkorn wheat"@en,
        "Triticum monococcum"@la .

<http://id.acdh.oeaw.ac.at/defc/thesaurus/elephant_lug/6.68> a skos:Concept ;
    dc:source "Coleman 1977" ;
    skos:broader <http://id.acdh.oeaw.ac.at/defc/thesaurus/lug/5.040> ;
    skos:definition "A lug in a shape of an elephant´s head." ;
    skos:editorialNote "dc_finds_pottery_detail;68" ;
    skos:inScheme <http://id.acdh.oeaw.ac.at/defc/thesaurus/FindsPotteryDetail>,
        <http://id.acdh.oeaw.ac.at/defc/thesaurus/FindsSchema> ;
    skos:prefLabel "Rüsselhenkel"@de,
        "elephant lug"@en .

<http://id.acdh.oeaw.ac.at/defc/thesaurus/elongated_handle/5.170> a skos:Concept ;
    dc:source "Coleman 1977" ;
    skos:broader <http://id.acdh.oeaw.ac.at/defc/thesaurus/handle/4.031> ;
    skos:definition "A lug in a shape of an elephant´s head." ;
    skos:editorialNote "dc_finds_pottery_detail;170" ;
    skos:inScheme <http://id.acdh.oeaw.ac.at/defc/thesaurus/FindsPotteryDetail>,
        <http://id.acdh.oeaw.ac.at/defc/thesaurus/FindsSchema> ;
    skos:prefLabel "langezogener Henkel"@de,
        "elongated handle"@en .

<http://id.acdh.oeaw.ac.at/defc/thesaurus/elongated_prong_handle_with_knob/6.183> a skos:Concept ;
    skos:broader <http://id.acdh.oeaw.ac.at/defc/thesaurus/pronged_handle/5.130> ;
    skos:editorialNote "dc_finds_pottery_detail;183" ;
    skos:inScheme <http://id.acdh.oeaw.ac.at/defc/thesaurus/FindsPotteryDetail>,
        <http://id.acdh.oeaw.ac.at/defc/thesaurus/FindsSchema> ;
    skos:prefLabel "lang gezogener Stabhenkel mit Knubbe"@de,
        "elongated prong handle with knob"@en .

<http://id.acdh.oeaw.ac.at/defc/thesaurus/emmer_wheat/6.7> a skos:Concept ;
    dc:source "http://eol.org/pages/1114086/overview" ;
    skos:broader <http://id.acdh.oeaw.ac.at/defc/thesaurus/wheat/5.39> ;
    skos:editorialNote "dc_botany_species;7" ;
    skos:inScheme <http://id.acdh.oeaw.ac.at/defc/thesaurus/BotanySpecies>,
        <http://id.acdh.oeaw.ac.at/defc/thesaurus/FindsSchema> ;
    skos:prefLabel "Emmer"@de,
        "emmer wheat"@en,
        "Triticum turgidum subsp. dicoccum"@la .

<http://id.acdh.oeaw.ac.at/defc/thesaurus/enclosure_ditch/5.1> a skos:Concept ;
    dc:source "Kipfer, B. A. Encyclopedic Dictionary of Archaeology. Kluwer Academic/Plenum Publishers, New York." ;
    skos:altLabel "ditch"@en ;
    skos:broader <http://id.acdh.oeaw.ac.at/defc/thesaurus/settlement_enclosure/4.073> ;
    skos:definition "A common feature of archaeological sites in association with defensive structures, as means of drainage, or as a construction trench." ;
    skos:editorialNote "dc_area_settlementstructure;1" ;
    skos:inScheme <http://id.acdh.oeaw.ac.at/defc/thesaurus/AreaSchema>,
        <http://id.acdh.oeaw.ac.at/defc/thesaurus/AreaSettlementstructure> ;
    skos:prefLabel "Graben"@de,
        "enclosure ditch"@en .

<http://id.acdh.oeaw.ac.at/defc/thesaurus/enclosure_rampart/5.2> a skos:Concept ;
    dc:source "http://thesaurus.historicengland.org.uk/pastscape_term.asp?thes_no=1&term_no=68905" ;
    skos:altLabel "rampart"@en ;
    skos:broader <http://id.acdh.oeaw.ac.at/defc/thesaurus/settlement_enclosure/4.073> ;
    skos:definition "A protective earthen mound, often the main defence of a fortification." ;
    skos:editorialNote "dc_area_settlementstructure;2" ;
    skos:inScheme <http://id.acdh.oeaw.ac.at/defc/thesaurus/AreaSchema>,
        <http://id.acdh.oeaw.ac.at/defc/thesaurus/AreaSettlementstructure> ;
    skos:prefLabel "Wall"@de,
        "enclosure rampart"@en .

<http://id.acdh.oeaw.ac.at/defc/thesaurus/enclosure_undetermined/5.7> a skos:Concept ;
    dc:source "OREA" ;
    skos:broader <http://id.acdh.oeaw.ac.at/defc/thesaurus/settlement_enclosure/4.073> ;
    skos:definition "An enclosure of a settlement has been recognized, but not indentified." ;
    skos:editorialNote "dc_area_settlementstructure;7" ;
    skos:inScheme <http://id.acdh.oeaw.ac.at/defc/thesaurus/AreaSchema>,
        <http://id.acdh.oeaw.ac.at/defc/thesaurus/AreaSettlementstructure> ;
    skos:prefLabel "enclosure undetermined"@en .

<http://id.acdh.oeaw.ac.at/defc/thesaurus/enclosure_wall/5.3> a skos:Concept ;
    dc:source "http://thesaurus.historicengland.org.uk/thesaurus_term.asp?thes_no=546&term_no=138407" ;
    skos:altLabel "enclosure wall"@en ;
    skos:broader <http://id.acdh.oeaw.ac.at/defc/thesaurus/settlement_enclosure/4.073> ;
    skos:definition "An enclosing structure composed of bricks, stones, wood or similar materials, laid in courses." ;
    skos:editorialNote "dc_area_settlementstructure;3" ;
    skos:inScheme <http://id.acdh.oeaw.ac.at/defc/thesaurus/AreaSchema>,
        <http://id.acdh.oeaw.ac.at/defc/thesaurus/AreaSettlementstructure> ;
    skos:prefLabel "Mauer"@de,
        "enclosure wall"@en .

<http://id.acdh.oeaw.ac.at/defc/thesaurus/end-scraper_on_blade/4.9> a skos:Concept ;
    dc:source "Inizan, M.-L., M. Reduron-Ballinger, H. Roche, J. Tixier 1999, Technology and Terminology of Knapped Stone. Nanterre: CREP., D. Srejovic (ed) 1997, Arheološki Leksikon." ;
    skos:broader <http://id.acdh.oeaw.ac.at/defc/thesaurus/retouched_tool/3.010> ;
    skos:definition "A tool with retouches on a single edge at one end of a blade, accross its long axis. The retouched of a scraper is bigger than 60°. The tool was possibly used for flensing or softening hides and to dress skins." ;
    skos:editorialNote "dc_finds_lithics_retouched_tools;9" ;
    skos:inScheme <http://id.acdh.oeaw.ac.at/defc/thesaurus/FindsLithicsRetouchedTools>,
        <http://id.acdh.oeaw.ac.at/defc/thesaurus/FindsSchema> ;
    skos:prefLabel "Kratzerstirn auf Klinge"@de,
        "end-scraper on blade"@en .

<http://id.acdh.oeaw.ac.at/defc/thesaurus/end-scraper_on_flake/4.10> a skos:Concept ;
    dc:source "Inizan, M.-L., M. Reduron-Ballinger, H. Roche, J. Tixier 1999, Technology and Terminology of Knapped Stone. Nanterre: CREP., D. Srejovic (ed) 1997, Arheološki Leksikon." ;
    skos:broader <http://id.acdh.oeaw.ac.at/defc/thesaurus/retouched_tool/3.010> ;
    skos:definition "A tool with retouches on a single edge at one end of a flake, accross its long axis. The retouched of a scraper is bigger than 60°. The tool was possibly used for flensing or softening hides and to dress skins." ;
    skos:editorialNote "dc_finds_lithics_retouched_tools;10" ;
    skos:inScheme <http://id.acdh.oeaw.ac.at/defc/thesaurus/FindsLithicsRetouchedTools>,
        <http://id.acdh.oeaw.ac.at/defc/thesaurus/FindsSchema> ;
    skos:prefLabel "Kratzerstirn auf Abschlag"@de,
        "end-scraper on flake"@en .

<http://id.acdh.oeaw.ac.at/defc/thesaurus/everted_rim/5.173> a skos:Concept ;
    dc:source "Kipfer, B. A. Dictionary of Artifacts 2007. Blackwell Publishing, Oxford.p 109" ;
    skos:broader <http://id.acdh.oeaw.ac.at/defc/thesaurus/rim/4.033> ;
    skos:definition "A rim that turns sharply outwards and upwards from the shoulder of the vessel." ;
    skos:editorialNote "dc_finds_pottery_detail;173" ;
    skos:inScheme <http://id.acdh.oeaw.ac.at/defc/thesaurus/FindsPotteryDetail>,
        <http://id.acdh.oeaw.ac.at/defc/thesaurus/FindsSchema> ;
    skos:prefLabel "Ungestülpter Rand"@de,
        "everted rim"@en .

<http://id.acdh.oeaw.ac.at/defc/thesaurus/excised-with-graphite/5.192> a skos:Concept ;
    dc:source "OREA" ;
    skos:altLabel "excised with graphite"@en ;
    skos:broader <http://id.acdh.oeaw.ac.at/defc/thesaurus/incised/4.168> ;
    skos:definition "Pottery decoration produced by cutting strips or shapes out of the soft clay surface before firing and painted with graphite paint." ;
    skos:editorialNote "dc_finds_pottery_decoration;192" ;
    skos:inScheme <http://id.acdh.oeaw.ac.at/defc/thesaurus/FindsPotteryDecoration>,
        <http://id.acdh.oeaw.ac.at/defc/thesaurus/FindsSchema> ;
    skos:prefLabel "Ware mit ausgeschnittenem Dekor und Graphitbemalung"@de,
        "excised-with-graphite"@en .

<http://id.acdh.oeaw.ac.at/defc/thesaurus/excised/5.191> a skos:Concept ;
    dc:source "OREA" ;
    skos:broader <http://id.acdh.oeaw.ac.at/defc/thesaurus/incised/4.168> ;
    skos:definition "Pottery decoration produced by cutting strips or shapes out of the soft clay surface before firing." ;
    skos:editorialNote "dc_finds_pottery_decoration;191" ;
    skos:inScheme <http://id.acdh.oeaw.ac.at/defc/thesaurus/FindsPotteryDecoration>,
        <http://id.acdh.oeaw.ac.at/defc/thesaurus/FindsSchema> ;
    skos:prefLabel "Ware mit ausgeschnittenem Dekor"@de,
        "excised"@en .

<http://id.acdh.oeaw.ac.at/defc/thesaurus/extramural/5.2> a skos:Concept ;
    skos:broader <http://id.acdh.oeaw.ac.at/defc/thesaurus/grave_location/4.087> ;
    skos:editorialNote "dc_area_topography;2" ;
    skos:inScheme <http://id.acdh.oeaw.ac.at/defc/thesaurus/AreaSchema>,
        <http://id.acdh.oeaw.ac.at/defc/thesaurus/AreaTopography> ;
    skos:prefLabel "extramural"@en .

<http://id.acdh.oeaw.ac.at/defc/thesaurus/fabric/2.3> a skos:Concept ;
    dc:source "https://en.oxforddictionaries.com/definition/fabric" ;
    skos:broader <http://id.acdh.oeaw.ac.at/defc/thesaurus/finds_material/1.01> ;
    skos:definition "Cloth produced by weaving or knitting textile fibres." ;
    skos:editorialNote "dc_finds_material;3" ;
    skos:inScheme <http://id.acdh.oeaw.ac.at/defc/thesaurus/FindsMaterial>,
        <http://id.acdh.oeaw.ac.at/defc/thesaurus/FindsSchema> ;
    skos:prefLabel "Stoff"@de,
        "fabric"@en .

<http://id.acdh.oeaw.ac.at/defc/thesaurus/fallow_deer/6.14> a skos:Concept ;
    dc:source "http://eol.org/pages/313992/overview" ;
    skos:broader <http://id.acdh.oeaw.ac.at/defc/thesaurus/deer/5.036> ;
    skos:editorialNote "dc_finds_animal_remains_species;14" ;
    skos:inScheme <http://id.acdh.oeaw.ac.at/defc/thesaurus/FindsAnimalRemainsSpecies>,
        <http://id.acdh.oeaw.ac.at/defc/thesaurus/FindsSchema> ;
    skos:prefLabel "Damhirsch"@de,
        "fallow deer"@en,
        "Dama dama"@la .

<http://id.acdh.oeaw.ac.at/defc/thesaurus/farming/2.2> a skos:Concept ;
    dc:source "OREA" ;
    skos:broader <http://id.acdh.oeaw.ac.at/defc/thesaurus/subsistence/1.043> ;
    skos:definition "The activity of cultivating the land by growing crops." ;
    skos:editorialNote "dc_interpretation_subsistencetype;2" ;
    skos:inScheme <http://id.acdh.oeaw.ac.at/defc/thesaurus/InterpretationSchema>,
        <http://id.acdh.oeaw.ac.at/defc/thesaurus/InterpretationSubsistencetype> ;
    skos:prefLabel "Ackerbau"@de,
        "farming"@en .

<http://id.acdh.oeaw.ac.at/defc/thesaurus/fava_bean/5.8> a skos:Concept ;
    dc:source "http://eol.org/pages/703202/overview" ;
    skos:broader <http://id.acdh.oeaw.ac.at/defc/thesaurus/pulse/4.32> ;
    skos:editorialNote "dc_botany_species;8" ;
    skos:inScheme <http://id.acdh.oeaw.ac.at/defc/thesaurus/BotanySpecies>,
        <http://id.acdh.oeaw.ac.at/defc/thesaurus/FindsSchema> ;
    skos:prefLabel "Ackerbohne"@de,
        "fava bean"@en,
        "Vicia faba"@la .

<http://id.acdh.oeaw.ac.at/defc/thesaurus/female_figurine/5.86> a skos:Concept ;
    dc:source "Kipfer, B. A. Dictionary of Artifacts 2007. Blackwell Publishing, Oxford.p.113" ;
    skos:broader <http://id.acdh.oeaw.ac.at/defc/thesaurus/anthropomorphic_figurine/4.84> ;
    skos:definition "A small carved or sculpted figure of a female human, usually of clay, stone, wood, or metal." ;
    skos:editorialNote "dc_finds_small_finds_type;86" ;
    skos:inScheme <http://id.acdh.oeaw.ac.at/defc/thesaurus/FindsSchema>,
        <http://id.acdh.oeaw.ac.at/defc/thesaurus/FindsSmallFindsType> ;
    skos:prefLabel "Weibliche Figur"@de,
        "female figurine"@en .

<http://id.acdh.oeaw.ac.at/defc/thesaurus/female_individuals/6.2> a skos:Concept ;
    skos:broader <http://id.acdh.oeaw.ac.at/defc/thesaurus/sex/5.095> ;
    skos:editorialNote "dc_area_sexes;2" ;
    skos:inScheme <http://id.acdh.oeaw.ac.at/defc/thesaurus/AreaSchema>,
        <http://id.acdh.oeaw.ac.at/defc/thesaurus/AreaSexes> ;
    skos:prefLabel "weiblich"@de,
        "female individuals"@en .

<http://id.acdh.oeaw.ac.at/defc/thesaurus/fenestrated_pedestal/5.160> a skos:Concept ;
    dc:source "OREA" ;
    skos:altLabel "Durchbrochener Fuß"@de,
        "Standfuß"@de ;
    skos:broader <http://id.acdh.oeaw.ac.at/defc/thesaurus/foot/4.71> ;
    skos:definition "A free-standing raised vessel bottom with openings in its walls." ;
    skos:editorialNote "dc_finds_pottery_detail;160" ;
    skos:inScheme <http://id.acdh.oeaw.ac.at/defc/thesaurus/FindsPotteryDetail>,
        <http://id.acdh.oeaw.ac.at/defc/thesaurus/FindsSchema> ;
    skos:prefLabel "Durchbrochener Sockel"@de,
        "fenestrated pedestal"@en .

<http://id.acdh.oeaw.ac.at/defc/thesaurus/field_observation_(monitoring)/3.6> a skos:Concept ;
    dc:source "http://thesaurus.historicengland.org.uk/thesaurus_term.asp?thes_no=566&term_no=14513" ;
    skos:altLabel " Kontrolle"@de,
        "archäologische Beobachtung"@de,
        " monitoring"@en,
        "field observation"@en ;
    skos:broader <http://id.acdh.oeaw.ac.at/defc/thesaurus/intrusive/2.048> ;
    skos:definition "Periodic visits being made to a site by an archaeologist to record archaeological deposts and recover finds that have come to light since the previous cisit. An archaeological presence is not maintained during gorundwork as it is with a watching brief." ;
    skos:editorialNote "dc_researchevet_researchtype;6" ;
    skos:inScheme <http://id.acdh.oeaw.ac.at/defc/thesaurus/ResearchEventSchema>,
        <http://id.acdh.oeaw.ac.at/defc/thesaurus/ResearchevetResearchtype> ;
    skos:prefLabel "archäologische Beobachtung (Kontrolle)"@de,
        "field observation (monitoring)"@en .

<http://id.acdh.oeaw.ac.at/defc/thesaurus/field_walking_survey%3A_non-systematic%2F5.15> a skos:Concept ;
    dc:source "http://thesaurus.historicengland.org.uk/thesaurus_term.asp?thes_no=566&term_no=145176" ;
    skos:broader <http://id.acdh.oeaw.ac.at/defc/thesaurus/field_walking_survey/4.053> ;
    skos:definition "The unsystematic study of ground surfaces and collection of visible archaeological material." ;
    skos:editorialNote "dc_researchevet_researchtype;15" ;
    skos:inScheme <http://id.acdh.oeaw.ac.at/defc/thesaurus/ResearchEventSchema>,
        <http://id.acdh.oeaw.ac.at/defc/thesaurus/ResearchevetResearchtype> ;
    skos:prefLabel "unsystematisch Feldbegehung"@de,
        "field walking survey: non-systematic"@en .

<http://id.acdh.oeaw.ac.at/defc/thesaurus/field_walking_survey%3A_systematic%2F5.16> a skos:Concept ;
    dc:source "http://thesaurus.historicengland.org.uk/thesaurus_term.asp?thes_no=566&term_no=145132" ;
    skos:broader <http://id.acdh.oeaw.ac.at/defc/thesaurus/field_walking_survey/4.053> ;
    skos:definition "The systematic study of ground surfaces and collection of visible archaeological material. Fieldwalking can be carried out as line-walking, grid collection and transect or quadrant sampling. Any material recovered is logged and stored by sample unit." ;
    skos:editorialNote "dc_researchevet_researchtype;16" ;
    skos:inScheme <http://id.acdh.oeaw.ac.at/defc/thesaurus/ResearchEventSchema>,
        <http://id.acdh.oeaw.ac.at/defc/thesaurus/ResearchevetResearchtype> ;
    skos:prefLabel "systematisch Feldbegehung"@de,
        "field walking survey: systematic"@en .

<http://id.acdh.oeaw.ac.at/defc/thesaurus/field_walking_survey%3A_undetermined%2F5.11> a skos:Concept ;
    skos:broader <http://id.acdh.oeaw.ac.at/defc/thesaurus/field_walking_survey/4.053> ;
    skos:editorialNote "dc_researchevet_researchtype;11" ;
    skos:inScheme <http://id.acdh.oeaw.ac.at/defc/thesaurus/ResearchEventSchema>,
        <http://id.acdh.oeaw.ac.at/defc/thesaurus/ResearchevetResearchtype> ;
    skos:prefLabel "Feldbegehung: nicht bestimmt"@de,
        "field walking survey: undetermined"@en .

<http://id.acdh.oeaw.ac.at/defc/thesaurus/fig/4.27> a skos:Concept ;
    dc:source "http://dbpedia.org/page/Ficus" ;
    skos:broader <http://id.acdh.oeaw.ac.at/defc/thesaurus/fruit/3.09> ;
    skos:editorialNote "dc_botany_species;27" ;
    skos:inScheme <http://id.acdh.oeaw.ac.at/defc/thesaurus/BotanySpecies>,
        <http://id.acdh.oeaw.ac.at/defc/thesaurus/FindsSchema> ;
    skos:prefLabel "Feige"@de,
        "fig"@en,
        "Ficus"@la .

<http://id.acdh.oeaw.ac.at/defc/thesaurus/figure_relief_decoration/5.133> a skos:Concept ;
    dc:source "OREA" ;
    skos:broader <http://id.acdh.oeaw.ac.at/defc/thesaurus/incised/4.168> ;
    skos:definition "Pottery from which the decoration figure projects from the vessel by carving out the background." ;
    skos:editorialNote "dc_finds_pottery_decoration;133" ;
    skos:inScheme <http://id.acdh.oeaw.ac.at/defc/thesaurus/FindsPotteryDecoration>,
        <http://id.acdh.oeaw.ac.at/defc/thesaurus/FindsSchema> ;
    skos:prefLabel "Figürlicher Reliefdekor"@de,
        "figure relief decoration"@en .

<http://id.acdh.oeaw.ac.at/defc/thesaurus/fikirtepe_box/4.111> a skos:Concept ;
    dc:source "OREA" ;
    skos:broader <http://id.acdh.oeaw.ac.at/defc/thesaurus/pottery_form/3.016> ;
    skos:definition "A small angular vessel with four legs, decorated on the outside, typically found in Fikirtepe." ;
    skos:editorialNote "dc_finds_pottery_form;111" ;
    skos:inScheme <http://id.acdh.oeaw.ac.at/defc/thesaurus/FindsPotteryForm>,
        <http://id.acdh.oeaw.ac.at/defc/thesaurus/FindsSchema> ;
    skos:prefLabel "Fikirtepe Box"@de,
        "fikirtepe box"@en .

<http://id.acdh.oeaw.ac.at/defc/thesaurus/fire_dog/4.90> a skos:Concept ;
    dc:source "Kipfer, B. A. Dictionary of Artifacts 2007. Blackwell Publishing, Oxford.p.114" ;
    skos:altLabel "fire-dog"@en ;
    skos:broader <http://id.acdh.oeaw.ac.at/defc/thesaurus/tool/3.1> ;
    skos:definition "An instrument consisting of an iron bar held horizontally at one end by an upright support, used to ensure the proper burning of a fire. A pair of these were put at each side of the hearth or fireplace to support burning wood; the end of a long could rest on the crosspiece, which was supported by two uprights." ;
    skos:editorialNote "dc_finds_small_finds_type;90" ;
    skos:inScheme <http://id.acdh.oeaw.ac.at/defc/thesaurus/FindsSchema>,
        <http://id.acdh.oeaw.ac.at/defc/thesaurus/FindsSmallFindsType> ;
    skos:prefLabel "Feuerbock"@de,
        "fire dog"@en .

<http://id.acdh.oeaw.ac.at/defc/thesaurus/fireplace/5.1> a skos:Concept ;
    dc:source "OREA" ;
    skos:broader <http://id.acdh.oeaw.ac.at/defc/thesaurus/occupation_evidence/4.088> ;
    skos:definition "A specially built place in a cave or a rockshelter where a fire can be built marking the use of a cave by the early men." ;
    skos:editorialNote "dc_area_evidenceofocupation;1" ;
    skos:inScheme <http://id.acdh.oeaw.ac.at/defc/thesaurus/AreaEvidenceofocupation>,
        <http://id.acdh.oeaw.ac.at/defc/thesaurus/AreaSchema> ;
    skos:prefLabel "Feuerstelle"@de,
        "fireplace"@en .

<http://id.acdh.oeaw.ac.at/defc/thesaurus/fireplace/5.15> a skos:Concept ;
    dc:source "http://www.merriam-webster.com/dictionary/fireplace" ;
    skos:altLabel "Feuerstelle"@de ;
    skos:broader <http://id.acdh.oeaw.ac.at/defc/thesaurus/installation/4.078> ;
    skos:definition "A specially built place in a room where a fire can be built." ;
    skos:editorialNote "dc_area_specialfeatures;15" ;
    skos:inScheme <http://id.acdh.oeaw.ac.at/defc/thesaurus/AreaSchema>,
        <http://id.acdh.oeaw.ac.at/defc/thesaurus/AreaSpecialfeatures> ;
    skos:prefLabel "fireplace"@en .

<http://id.acdh.oeaw.ac.at/defc/thesaurus/fish_hook/5.45> a skos:Concept ;
    dc:source "Kipfer, B. A. Dictionary of Artifacts 2007. Blackwell Publishing, Oxford.p. 252." ;
    skos:broader <http://id.acdh.oeaw.ac.at/defc/thesaurus/fishing_object/4.027> ;
    skos:definition "An artifact of two basic types: the bait hook and lure hook. Varied in form throughout the Pacific, they are made of bone, shell, tortoise shell, or wood." ;
    skos:editorialNote "dc_finds_small_finds_type;45" ;
    skos:inScheme <http://id.acdh.oeaw.ac.at/defc/thesaurus/FindsSchema>,
        <http://id.acdh.oeaw.ac.at/defc/thesaurus/FindsSmallFindsType> ;
    skos:prefLabel "Angelhacken"@de,
        "fish hook"@en .

<http://id.acdh.oeaw.ac.at/defc/thesaurus/fishing/2.1> a skos:Concept ;
    dc:source "OREA" ;
    skos:broader <http://id.acdh.oeaw.ac.at/defc/thesaurus/subsistence/1.043> ;
    skos:definition "The activity of catching fish as a source of food." ;
    skos:editorialNote "dc_interpretation_subsistencetype;1" ;
    skos:inScheme <http://id.acdh.oeaw.ac.at/defc/thesaurus/InterpretationSchema>,
        <http://id.acdh.oeaw.ac.at/defc/thesaurus/InterpretationSubsistencetype> ;
    skos:prefLabel "Fischen"@de,
        "fishing"@en .

<http://id.acdh.oeaw.ac.at/defc/thesaurus/flake/4.3> a skos:Concept ;
    skos:broader <http://id.acdh.oeaw.ac.at/defc/thesaurus/unretouched_tool/3.011> ;
    skos:editorialNote "dc_finds_lithics_unretouched_tools;3" ;
    skos:inScheme <http://id.acdh.oeaw.ac.at/defc/thesaurus/FindsLithicsUnretouchedTools>,
        <http://id.acdh.oeaw.ac.at/defc/thesaurus/FindsSchema> ;
    skos:prefLabel "Abschlag"@de,
        "flake"@en .

<http://id.acdh.oeaw.ac.at/defc/thesaurus/flake_core/4.9> a skos:Concept ;
    dc:source "OREA" ;
    skos:altLabel "Flake-core"@en ;
    skos:broader <http://id.acdh.oeaw.ac.at/defc/thesaurus/core/3.12> ;
    skos:definition "A core which main reduction leads to the detachment of flakes (aim of knapping-flakes)." ;
    skos:editorialNote "dc_finds_lithics_core_shape;9" ;
    skos:inScheme <http://id.acdh.oeaw.ac.at/defc/thesaurus/FindsLithicsCoreShape>,
        <http://id.acdh.oeaw.ac.at/defc/thesaurus/FindsSchema> ;
    skos:prefLabel "Abschlagkern"@de,
        "flake core"@en .

<http://id.acdh.oeaw.ac.at/defc/thesaurus/flake_industry/5.2> a skos:Concept ;
    dc:source "Inizan, M.-L., M. Reduron-Ballinger, H. Roche, J. Tixier 1999, Technology and Terminology of Knapped Stone. Nanterre: CREP. p. 143." ;
    skos:broader <http://id.acdh.oeaw.ac.at/defc/thesaurus/lithics_industry/4.024> ;
    skos:definition "Human action applied to raw materials in order to transform them into flakes." ;
    skos:editorialNote "dc_finds_lithics_industry;2" ;
    skos:inScheme <http://id.acdh.oeaw.ac.at/defc/thesaurus/FindsLithicsIndustry>,
        <http://id.acdh.oeaw.ac.at/defc/thesaurus/FindsSchema> ;
    skos:prefLabel "flake industry"@en .

<http://id.acdh.oeaw.ac.at/defc/thesaurus/flaring_rim/5.69> a skos:Concept ;
    dc:source "OREA" ;
    skos:broader <http://id.acdh.oeaw.ac.at/defc/thesaurus/rim/4.033> ;
    skos:definition "Curved rim with outcurving inflections outside the vessel." ;
    skos:editorialNote "dc_finds_pottery_detail;69" ;
    skos:inScheme <http://id.acdh.oeaw.ac.at/defc/thesaurus/FindsPotteryDetail>,
        <http://id.acdh.oeaw.ac.at/defc/thesaurus/FindsSchema> ;
    skos:prefLabel "Ausladender Rand"@de,
        "flaring rim"@en .

<http://id.acdh.oeaw.ac.at/defc/thesaurus/flat-topped_rim/5.158> a skos:Concept ;
    dc:source "OREA" ;
    skos:broader <http://id.acdh.oeaw.ac.at/defc/thesaurus/rim/4.033> ;
    skos:definition "Horizontally flattened upper portion of a vessel." ;
    skos:editorialNote "dc_finds_pottery_detail;158" ;
    skos:inScheme <http://id.acdh.oeaw.ac.at/defc/thesaurus/FindsPotteryDetail>,
        <http://id.acdh.oeaw.ac.at/defc/thesaurus/FindsSchema> ;
    skos:prefLabel "Flachrand"@de,
        "flat-topped rim"@en .

<http://id.acdh.oeaw.ac.at/defc/thesaurus/flat_base/5.86> a skos:Concept ;
    dc:source "Kipfer, B. A. Dictionary of Artifacts 2007. Blackwell Publishing, Oxford.p 300" ;
    skos:broader <http://id.acdh.oeaw.ac.at/defc/thesaurus/base/4.032> ;
    skos:definition "Flat lower portion of a vessel from the lower boudary of the body to the place that would normally be in contact with the surface on which the vessel rested." ;
    skos:editorialNote "dc_finds_pottery_detail;86" ;
    skos:inScheme <http://id.acdh.oeaw.ac.at/defc/thesaurus/FindsPotteryDetail>,
        <http://id.acdh.oeaw.ac.at/defc/thesaurus/FindsSchema> ;
    skos:prefLabel "Flachboden"@de,
        "flat base"@en .

<http://id.acdh.oeaw.ac.at/defc/thesaurus/flat_based_oval_bowl/5.193> a skos:Concept ;
    dc:source "OREA" ;
    skos:broader <http://id.acdh.oeaw.ac.at/defc/thesaurus/bowl/4.115> ;
    skos:definition "A shallow open vessel of oval shape and flat lower portion." ;
    skos:editorialNote "dc_finds_pottery_form;193" ;
    skos:inScheme <http://id.acdh.oeaw.ac.at/defc/thesaurus/FindsPotteryForm>,
        <http://id.acdh.oeaw.ac.at/defc/thesaurus/FindsSchema> ;
    skos:prefLabel "ovale Schüssel mit flachem Boden"@de,
        "flat based oval bowl"@en .

<http://id.acdh.oeaw.ac.at/defc/thesaurus/flat_site/4.1> a skos:Concept ;
    dc:source "OREA" ;
    skos:broader <http://id.acdh.oeaw.ac.at/defc/thesaurus/settlment_type/3.068> ;
    skos:definition "A settlement erected in the low-lying area." ;
    skos:editorialNote "dc_area_settlementtype;1" ;
    skos:inScheme <http://id.acdh.oeaw.ac.at/defc/thesaurus/AreaSchema>,
        <http://id.acdh.oeaw.ac.at/defc/thesaurus/AreaSettlementtype> ;
    skos:prefLabel "Flachland"@de,
        "flat site"@en .

<http://id.acdh.oeaw.ac.at/defc/thesaurus/flax/4.9> a skos:Concept ;
    dc:source "http://eol.org/pages/581568/overview" ;
    skos:broader <http://id.acdh.oeaw.ac.at/defc/thesaurus/grain_crop/3.08> ;
    skos:editorialNote "dc_botany_species;9" ;
    skos:inScheme <http://id.acdh.oeaw.ac.at/defc/thesaurus/BotanySpecies>,
        <http://id.acdh.oeaw.ac.at/defc/thesaurus/FindsSchema> ;
    skos:prefLabel "Gemeiner Lein/Flachs"@de,
        "flax"@en,
        "Linum usitatissimum"@la .

<http://id.acdh.oeaw.ac.at/defc/thesaurus/flint/4.11> a skos:Concept ;
    dc:source "Encyclopaedia Britannica - https://www.britannica.com/science/chert#ref272901" ;
    skos:broader <http://id.acdh.oeaw.ac.at/defc/thesaurus/chert/3.12> ;
    skos:definition "Flint os a fine-grained quarz and a silica mineral included under the general term chert. In Neolithic it was used as material source for tools and weapons." ;
    skos:editorialNote "dc_finds_material;11" ;
    skos:inScheme <http://id.acdh.oeaw.ac.at/defc/thesaurus/FindsMaterial>,
        <http://id.acdh.oeaw.ac.at/defc/thesaurus/FindsSchema> ;
    skos:prefLabel "Flint"@de,
        "flint"@en .

<http://id.acdh.oeaw.ac.at/defc/thesaurus/flint/6.2> a skos:Concept ;
    dc:source "Encyclopaedia Britannica - https://www.britannica.com/science/chert#ref272901" ;
    skos:broader <http://id.acdh.oeaw.ac.at/defc/thesaurus/chert/5.3> ;
    skos:definition "Flint os a fine-grained quarz and a silica mineral included under the general term chert. In Neolithic it was used as material source for tools and weapons." ;
    skos:editorialNote "dc_finds_lithics_raw_material;2" ;
    skos:inScheme <http://id.acdh.oeaw.ac.at/defc/thesaurus/FindsLithicsRawMaterial>,
        <http://id.acdh.oeaw.ac.at/defc/thesaurus/FindsSchema> ;
    skos:prefLabel "Flint"@de,
        "flint"@en .

<http://id.acdh.oeaw.ac.at/defc/thesaurus/flint/6.4> a skos:Concept ;
    dc:source "Encyclopaedia Britannica - https://www.britannica.com/science/chert#ref272901" ;
    skos:broader <http://id.acdh.oeaw.ac.at/defc/thesaurus/chert/5.5> ;
    skos:definition "Flint os a fine-grained quarz and a silica mineral included under the general term chert. It has been extracted from a quarry site and probably used as material source for tools and weapons." ;
    skos:editorialNote "dc_area_rawmaterial;4" ;
    skos:inScheme <http://id.acdh.oeaw.ac.at/defc/thesaurus/AreaRawmaterial>,
        <http://id.acdh.oeaw.ac.at/defc/thesaurus/AreaSchema> ;
    skos:prefLabel "Flint"@de,
        "flint"@en .

<http://id.acdh.oeaw.ac.at/defc/thesaurus/forelimb/6.3> a skos:Concept ;
    dc:source "https://en.oxforddictionaries.com/definition/forelimb" ;
    skos:broader <http://id.acdh.oeaw.ac.at/defc/thesaurus/extremity/5.4> ;
    skos:definition "Either of the front limbs of an animal; a foreleg, wing, flipper, etc." ;
    skos:editorialNote "dc_animal_remains_part;3" ;
    skos:inScheme <http://id.acdh.oeaw.ac.at/defc/thesaurus/AnimalRemainsPart>,
        <http://id.acdh.oeaw.ac.at/defc/thesaurus/FindsSchema> ;
    skos:prefLabel "forelimb"@en .

<http://id.acdh.oeaw.ac.at/defc/thesaurus/foundation_trench/5.13> a skos:Concept ;
    dc:source "OREA" ;
    skos:broader <http://id.acdh.oeaw.ac.at/defc/thesaurus/building_technique/4.075> ;
    skos:definition "A trench or gully, packed with stone, earth or logs, used to support a wall.  " ;
    skos:editorialNote "dc_area_buildingtechnique;13" ;
    skos:inScheme <http://id.acdh.oeaw.ac.at/defc/thesaurus/AreaBuildingtechnique>,
        <http://id.acdh.oeaw.ac.at/defc/thesaurus/AreaSchema> ;
    skos:prefLabel "foundation trench"@en .

<http://id.acdh.oeaw.ac.at/defc/thesaurus/foxtail_millet/6.10> a skos:Concept ;
    dc:source "http://eol.org/pages/1114673/overview" ;
    skos:broader <http://id.acdh.oeaw.ac.at/defc/thesaurus/millet/5.039> ;
    skos:editorialNote "dc_botany_species;10" ;
    skos:inScheme <http://id.acdh.oeaw.ac.at/defc/thesaurus/BotanySpecies>,
        <http://id.acdh.oeaw.ac.at/defc/thesaurus/FindsSchema> ;
    skos:prefLabel "Kolbenhirse"@de,
        "foxtail millet"@en,
        "Setaria italica"@la .

<http://id.acdh.oeaw.ac.at/defc/thesaurus/fruitstand/4.130> a skos:Concept ;
    dc:source "OREA" ;
    skos:broader <http://id.acdh.oeaw.ac.at/defc/thesaurus/pottery_form/3.016> ;
    skos:definition "A very low shallow bowl with a high pedestal." ;
    skos:editorialNote "dc_finds_pottery_form;130" ;
    skos:inScheme <http://id.acdh.oeaw.ac.at/defc/thesaurus/FindsPotteryForm>,
        <http://id.acdh.oeaw.ac.at/defc/thesaurus/FindsSchema> ;
    skos:prefLabel "Fruchtständer"@de,
        "fruitstand"@en .

<http://id.acdh.oeaw.ac.at/defc/thesaurus/funnel-necked_jar/5.180> a skos:Concept ;
    dc:source "OREA" ;
    skos:broader <http://id.acdh.oeaw.ac.at/defc/thesaurus/jar/4.145> ;
    skos:definition "A high and open vessel with an expanded neck." ;
    skos:editorialNote "dc_finds_pottery_form;180" ;
    skos:inScheme <http://id.acdh.oeaw.ac.at/defc/thesaurus/FindsPotteryForm>,
        <http://id.acdh.oeaw.ac.at/defc/thesaurus/FindsSchema> ;
    skos:prefLabel "Trichterrandtopf"@de,
        "funnel-necked jar"@en .

<http://id.acdh.oeaw.ac.at/defc/thesaurus/game/5.15> a skos:Concept ;
    skos:broader <http://id.acdh.oeaw.ac.at/defc/thesaurus/mammal/4.020> ;
    skos:editorialNote "dc_finds_animal_remains_species;15" ;
    skos:inScheme <http://id.acdh.oeaw.ac.at/defc/thesaurus/FindsAnimalRemainsSpecies>,
        <http://id.acdh.oeaw.ac.at/defc/thesaurus/FindsSchema> ;
    skos:prefLabel "Wild"@de,
        "game"@en .

<http://id.acdh.oeaw.ac.at/defc/thesaurus/gathering/2.5> a skos:Concept ;
    dc:source "OREA" ;
    skos:broader <http://id.acdh.oeaw.ac.at/defc/thesaurus/subsistence/1.043> ;
    skos:definition "The activity of collecting wild plants and their fruits." ;
    skos:editorialNote "dc_interpretation_subsistencetype;5" ;
    skos:inScheme <http://id.acdh.oeaw.ac.at/defc/thesaurus/InterpretationSchema>,
        <http://id.acdh.oeaw.ac.at/defc/thesaurus/InterpretationSubsistencetype> ;
    skos:prefLabel "Sammeln"@de,
        "gathering"@en .

<http://id.acdh.oeaw.ac.at/defc/thesaurus/gazelle/5.37> a skos:Concept ;
    dc:source "http://eol.org/pages/15584/overview" ;
    skos:broader <http://id.acdh.oeaw.ac.at/defc/thesaurus/mammal/4.020> ;
    skos:editorialNote "dc_finds_animal_remains_species;37" ;
    skos:inScheme <http://id.acdh.oeaw.ac.at/defc/thesaurus/FindsAnimalRemainsSpecies>,
        <http://id.acdh.oeaw.ac.at/defc/thesaurus/FindsSchema> ;
    skos:prefLabel "Gazelle"@de,
        "gazelle"@en .

<http://id.acdh.oeaw.ac.at/defc/thesaurus/geological_research/3.26> a skos:Concept ;
    dc:source "https://en.oxforddictionaries.com/definition/mineralogy" ;
    skos:altLabel "Geologie"@de,
        "geology"@en ;
    skos:broader <http://id.acdh.oeaw.ac.at/defc/thesaurus/non-intrusive/2.051> ;
    skos:definition "The scientific tudy of minerals." ;
    skos:editorialNote "dc_researchevet_researchtype;26" ;
    skos:inScheme <http://id.acdh.oeaw.ac.at/defc/thesaurus/ResearchEventSchema>,
        <http://id.acdh.oeaw.ac.at/defc/thesaurus/ResearchevetResearchtype> ;
    skos:prefLabel "geologische Auswertung"@de,
        "geological research"@en .

<http://id.acdh.oeaw.ac.at/defc/thesaurus/geophysical_survey%3A_magnetic%2F5.17> a skos:Concept ;
    dc:source "http://thesaurus.historicengland.org.uk/thesaurus_term.asp?thes_no=566&term_no=145144" ;
    skos:altLabel "Geomagnetik"@de,
        " magnetometry"@en,
        "magnetometry survey"@en ;
    skos:broader <http://id.acdh.oeaw.ac.at/defc/thesaurus/geophysical_survey/4.054> ;
    skos:definition "Survey using a magnetometer, a device capable detecting various in magnetic susceptibility between topsoils, subsoils and rocks, can also be used in a maritime context to detect variations in the magnetic field of seabed sediments." ;
    skos:editorialNote "dc_researchevet_researchtype;17" ;
    skos:inScheme <http://id.acdh.oeaw.ac.at/defc/thesaurus/ResearchEventSchema>,
        <http://id.acdh.oeaw.ac.at/defc/thesaurus/ResearchevetResearchtype> ;
    skos:prefLabel "geomagnetische Messung"@de,
        "geophysical survey: magnetic"@en .

<http://id.acdh.oeaw.ac.at/defc/thesaurus/geophysical_survey%3A_radar%2F5.18> a skos:Concept ;
    dc:source "http://thesaurus.historicengland.org.uk/thesaurus_term.asp?thes_no=566&term_no=145135" ;
    skos:altLabel " ground penetrating radar"@en,
        "GPR"@en,
        "ground penetratig radar survey"@en ;
    skos:broader <http://id.acdh.oeaw.ac.at/defc/thesaurus/geophysical_survey/4.054> ;
    skos:definition "A technique that measures the amount of time it takes pulses of electromagnetic energy sent into the ground, from a transmitter, to reflect back from the interfaces between layers and other subsurface features in order to produce a subsurface profile." ;
    skos:editorialNote "dc_researchevet_researchtype;18" ;
    skos:inScheme <http://id.acdh.oeaw.ac.at/defc/thesaurus/ResearchEventSchema>,
        <http://id.acdh.oeaw.ac.at/defc/thesaurus/ResearchevetResearchtype> ;
    skos:prefLabel "Bodenradarmessung"@de,
        "geophysical survey: radar"@en .

<http://id.acdh.oeaw.ac.at/defc/thesaurus/globular_jar/5.106> a skos:Concept ;
    dc:source "OREA" ;
    skos:altLabel "Kugeltopf"@de ;
    skos:broader <http://id.acdh.oeaw.ac.at/defc/thesaurus/jar/4.145> ;
    skos:definition "A small narrow mouthed jar with hemispherical, ovoid, or spherical body." ;
    skos:editorialNote "dc_finds_pottery_form;106" ;
    skos:inScheme <http://id.acdh.oeaw.ac.at/defc/thesaurus/FindsPotteryForm>,
        <http://id.acdh.oeaw.ac.at/defc/thesaurus/FindsSchema> ;
    skos:prefLabel "Kugelförmiger Topf"@de,
        "globular jar"@en .

<http://id.acdh.oeaw.ac.at/defc/thesaurus/goat/5.8> a skos:Concept ;
    dc:source "http://eol.org/pages/328660/overview" ;
    skos:broader <http://id.acdh.oeaw.ac.at/defc/thesaurus/mammal/4.020> ;
    skos:editorialNote "dc_finds_animal_remains_species;8" ;
    skos:inScheme <http://id.acdh.oeaw.ac.at/defc/thesaurus/FindsAnimalRemainsSpecies>,
        <http://id.acdh.oeaw.ac.at/defc/thesaurus/FindsSchema> ;
    skos:prefLabel "Ziege"@de,
        "goat"@en,
        "Capra hircus"@la .

<http://id.acdh.oeaw.ac.at/defc/thesaurus/goblet/4.201> a skos:Concept ;
    dc:source "OREA" ;
    skos:broader <http://id.acdh.oeaw.ac.at/defc/thesaurus/pottery_form/3.016> ;
    skos:definition "A deep vessel with straight sides and pedestal, two liminal hoisting handles." ;
    skos:editorialNote "dc_finds_pottery_form;201" ;
    skos:inScheme <http://id.acdh.oeaw.ac.at/defc/thesaurus/FindsPotteryForm>,
        <http://id.acdh.oeaw.ac.at/defc/thesaurus/FindsSchema> ;
    skos:prefLabel "Goblet Becher"@de,
        "goblet"@en .

<http://id.acdh.oeaw.ac.at/defc/thesaurus/gold/3.34> a skos:Concept ;
    dc:source "http://dbpedia.org/page/Gold" ;
    skos:broader <http://id.acdh.oeaw.ac.at/defc/thesaurus/metal/2.9> ;
    skos:definition "Gold is a chemical element with symbol Au (from Latin: aurum) and atomic number 79. In its purest form, it is a bright, slightly reddish yellow, dense, soft, malleable and ductile metal." ;
    skos:editorialNote "dc_finds_material;34" ;
    skos:inScheme <http://id.acdh.oeaw.ac.at/defc/thesaurus/FindsMaterial>,
        <http://id.acdh.oeaw.ac.at/defc/thesaurus/FindsSchema> ;
    skos:prefLabel "Gold"@de,
        "gold"@en .

<http://id.acdh.oeaw.ac.at/defc/thesaurus/gouged_bowl/5.149> a skos:Concept ;
    dc:source "Vitelli 1993, 185-187" ;
    skos:broader <http://id.acdh.oeaw.ac.at/defc/thesaurus/bowl/4.115> ;
    skos:definition "MN Urfirnis deep bowl with deep linear incisions in the interior of the bowl." ;
    skos:editorialNote "dc_finds_pottery_form;149" ;
    skos:inScheme <http://id.acdh.oeaw.ac.at/defc/thesaurus/FindsPotteryForm>,
        <http://id.acdh.oeaw.ac.at/defc/thesaurus/FindsSchema> ;
    skos:prefLabel "”Gouged Bowl”"@de,
        "gouged bowl"@en .

<http://id.acdh.oeaw.ac.at/defc/thesaurus/grain/4.3> a skos:Concept ;
    dc:source "https://en.oxforddictionaries.com/definition/grain" ;
    skos:broader <http://id.acdh.oeaw.ac.at/defc/thesaurus/dating_material/3.046> ;
    skos:definition "Wheat or any other cultivated cereal used as food. " ;
    skos:editorialNote "dc_period_datedby;3" ;
    skos:inScheme <http://id.acdh.oeaw.ac.at/defc/thesaurus/PeriodSchema> ;
    skos:prefLabel "Korn"@de,
        "grain"@en .

<http://id.acdh.oeaw.ac.at/defc/thesaurus/granite/3.24> a skos:Concept ;
    dc:source "http://dbpedia.org/page/Granite" ;
    skos:broader <http://id.acdh.oeaw.ac.at/defc/thesaurus/stone/2.1> ;
    skos:definition "A common type of felsic intrusive igneous rock that is granular and phaneritic in texture. Granites can be predominantly white, pink, or gray in color, depending on their mineralogy." ;
    skos:editorialNote "dc_finds_material;24" ;
    skos:inScheme <http://id.acdh.oeaw.ac.at/defc/thesaurus/FindsMaterial>,
        <http://id.acdh.oeaw.ac.at/defc/thesaurus/FindsSchema> ;
    skos:prefLabel "Granit"@de,
        "granite"@en .

<http://id.acdh.oeaw.ac.at/defc/thesaurus/granulata_ware/5.216> a skos:Concept ;
    dc:source "OREA" ;
    skos:altLabel "pellet decoration"@en ;
    skos:broader <http://id.acdh.oeaw.ac.at/defc/thesaurus/plastic_decoration/4.132> ;
    skos:definition "Pottery covered with a coating of stones and then slipped with paint." ;
    skos:editorialNote "dc_finds_pottery_decoration;216" ;
    skos:inScheme <http://id.acdh.oeaw.ac.at/defc/thesaurus/FindsPotteryDecoration>,
        <http://id.acdh.oeaw.ac.at/defc/thesaurus/FindsSchema> ;
    skos:prefLabel "Granulatdekor"@de,
        "granulata ware"@en .

<http://id.acdh.oeaw.ac.at/defc/thesaurus/grape/4.29> a skos:Concept ;
    dc:source "http://eol.org/pages/38383/overview" ;
    skos:broader <http://id.acdh.oeaw.ac.at/defc/thesaurus/fruit/3.09> ;
    skos:editorialNote "dc_botany_species;29" ;
    skos:inScheme <http://id.acdh.oeaw.ac.at/defc/thesaurus/BotanySpecies>,
        <http://id.acdh.oeaw.ac.at/defc/thesaurus/FindsSchema> ;
    skos:prefLabel "Traube"@de,
        "grape"@en,
        "Vitis"@la .

<http://id.acdh.oeaw.ac.at/defc/thesaurus/graphite_painted/6.194> a skos:Concept ;
    dc:source "OREA" ;
    skos:broader <http://id.acdh.oeaw.ac.at/defc/thesaurus/pattern_painted/5.041> ;
    skos:definition "Pottery decorated with graphite paint." ;
    skos:editorialNote "dc_finds_pottery_decoration;194" ;
    skos:inScheme <http://id.acdh.oeaw.ac.at/defc/thesaurus/FindsPotteryDecoration>,
        <http://id.acdh.oeaw.ac.at/defc/thesaurus/FindsSchema> ;
    skos:prefLabel "Graphitbemalt"@de,
        "graphite painted"@en .

<http://id.acdh.oeaw.ac.at/defc/thesaurus/grass_pea/6.11> a skos:Concept ;
    dc:source "http://eol.org/pages/703183/overview" ;
    skos:broader <http://id.acdh.oeaw.ac.at/defc/thesaurus/pea/5.14> ;
    skos:editorialNote "dc_botany_species;11" ;
    skos:inScheme <http://id.acdh.oeaw.ac.at/defc/thesaurus/BotanySpecies>,
        <http://id.acdh.oeaw.ac.at/defc/thesaurus/FindsSchema> ;
    skos:prefLabel "Saat-Platterbse"@de,
        "grass pea"@en,
        "Lathyrus sativus"@la .

<http://id.acdh.oeaw.ac.at/defc/thesaurus/gray_lustre/4.195> a skos:Concept ;
    dc:source "Keighley 1986, 364" ;
    skos:broader <http://id.acdh.oeaw.ac.at/defc/thesaurus/pottery_surface_treatment/3.019> ;
    skos:definition "Smoothed ware with soapy grey surface typical for Eastern Macedonia, Sitagroi." ;
    skos:editorialNote "dc_finds_pottery_decoration;195" ;
    skos:inScheme <http://id.acdh.oeaw.ac.at/defc/thesaurus/FindsPotteryDecoration>,
        <http://id.acdh.oeaw.ac.at/defc/thesaurus/FindsSchema> ;
    skos:prefLabel "Grauer Glanzton"@de,
        "gray lustre"@en .

<http://id.acdh.oeaw.ac.at/defc/thesaurus/graylag_goose/6.31> a skos:Concept ;
    dc:source "http://eol.org/pages/1047334/overview" ;
    skos:broader <http://id.acdh.oeaw.ac.at/defc/thesaurus/goose/5.037> ;
    skos:editorialNote "dc_finds_animal_remains_species;31" ;
    skos:inScheme <http://id.acdh.oeaw.ac.at/defc/thesaurus/FindsAnimalRemainsSpecies>,
        <http://id.acdh.oeaw.ac.at/defc/thesaurus/FindsSchema> ;
    skos:prefLabel "Graugans"@de,
        "graylag goose"@en,
        "Anser anser"@la .

<http://id.acdh.oeaw.ac.at/defc/thesaurus/great_bustard/5.30> a skos:Concept ;
    dc:source "http://eol.org/pages/915364/overview" ;
    skos:broader <http://id.acdh.oeaw.ac.at/defc/thesaurus/bird/4.36> ;
    skos:editorialNote "dc_finds_animal_remains_species;30" ;
    skos:inScheme <http://id.acdh.oeaw.ac.at/defc/thesaurus/FindsAnimalRemainsSpecies>,
        <http://id.acdh.oeaw.ac.at/defc/thesaurus/FindsSchema> ;
    skos:prefLabel "Großtrappe"@de,
        "great bustard"@en,
        "Otis tarda"@la .

<http://id.acdh.oeaw.ac.at/defc/thesaurus/green_stone/3.33> a skos:Concept ;
    dc:source "0" ;
    skos:altLabel "Jade"@de,
        "jade"@en ;
    skos:broader <http://id.acdh.oeaw.ac.at/defc/thesaurus/stone/2.1> ;
    skos:editorialNote "dc_finds_material;33" ;
    skos:inScheme <http://id.acdh.oeaw.ac.at/defc/thesaurus/FindsMaterial>,
        <http://id.acdh.oeaw.ac.at/defc/thesaurus/FindsSchema> ;
    skos:prefLabel "Grünstein"@de,
        "green stone"@en .

<http://id.acdh.oeaw.ac.at/defc/thesaurus/grey_burnished/5.289> a skos:Concept ;
    dc:source "Hauptmann - Milojcic 1969" ;
    skos:broader <http://id.acdh.oeaw.ac.at/defc/thesaurus/burnished/4.297> ;
    skos:definition "Burnished ware with fine grey surface typical for Thessaly." ;
    skos:editorialNote "dc_finds_pottery_decoration;289" ;
    skos:inScheme <http://id.acdh.oeaw.ac.at/defc/thesaurus/FindsPotteryDecoration>,
        <http://id.acdh.oeaw.ac.at/defc/thesaurus/FindsSchema> ;
    skos:prefLabel "grau geglättet"@de,
        "grey burnished"@en .

<http://id.acdh.oeaw.ac.at/defc/thesaurus/grey_on_grey/6.277> a skos:Concept ;
    dc:source "OREA" ;
    skos:broader <http://id.acdh.oeaw.ac.at/defc/thesaurus/pattern_painted/5.041> ;
    skos:definition "Pottery decorated with grey paint on grey ground." ;
    skos:editorialNote "dc_finds_pottery_decoration;277" ;
    skos:inScheme <http://id.acdh.oeaw.ac.at/defc/thesaurus/FindsPotteryDecoration>,
        <http://id.acdh.oeaw.ac.at/defc/thesaurus/FindsSchema> ;
    skos:prefLabel "grau auf grau"@de,
        "grey on grey"@en .

<http://id.acdh.oeaw.ac.at/defc/thesaurus/grey_on_grey_(γ1β)/6.150> a skos:Concept ;
    dc:source "OREA" ;
    skos:broader <http://id.acdh.oeaw.ac.at/defc/thesaurus/pattern_painted/5.041> ;
    skos:definition "Pottery decorated with grey paint on grey ground." ;
    skos:editorialNote "dc_finds_pottery_decoration;150" ;
    skos:inScheme <http://id.acdh.oeaw.ac.at/defc/thesaurus/FindsPotteryDecoration>,
        <http://id.acdh.oeaw.ac.at/defc/thesaurus/FindsSchema> ;
    skos:prefLabel "Grau auf grau (C1b)"@de,
        "grey on grey (γ1β)"@en .

<http://id.acdh.oeaw.ac.at/defc/thesaurus/grey_ware/6.246> a skos:Concept ;
    dc:source "OREA" ;
    skos:broader <http://id.acdh.oeaw.ac.at/defc/thesaurus/pattern_painted/5.041> ;
    skos:definition "Grey ware." ;
    skos:editorialNote "dc_finds_pottery_decoration;246" ;
    skos:inScheme <http://id.acdh.oeaw.ac.at/defc/thesaurus/FindsPotteryDecoration>,
        <http://id.acdh.oeaw.ac.at/defc/thesaurus/FindsSchema> ;
    skos:prefLabel "grau Ware"@de,
        "grey ware"@en .

<http://id.acdh.oeaw.ac.at/defc/thesaurus/grinding_stone/4.52> a skos:Concept ;
    dc:source "Kipfer, B. A. Dictionary of Artifacts 2007. Blackwell Publishing, Oxford.p.136" ;
    skos:broader <http://id.acdh.oeaw.ac.at/defc/thesaurus/tool/3.1> ;
    skos:definition "Any lithic (stone) artifact used to process plants for food, medicines, cosmetics, or pigments. The grinding was done on a flat or concave surface." ;
    skos:editorialNote "dc_finds_small_finds_type;52" ;
    skos:inScheme <http://id.acdh.oeaw.ac.at/defc/thesaurus/FindsSchema>,
        <http://id.acdh.oeaw.ac.at/defc/thesaurus/FindsSmallFindsType> ;
    skos:prefLabel "Reibstein"@de,
        "grinding stone"@en .

<http://id.acdh.oeaw.ac.at/defc/thesaurus/grindstone/5.58> a skos:Concept ;
    dc:source "Kipfer, B. A. Dictionary of Artifacts 2007. Blackwell Publishing, Oxford.p.136" ;
    skos:altLabel "grinding stone"@en,
        "sharpening stone"@en ;
    skos:broader <http://id.acdh.oeaw.ac.at/defc/thesaurus/grinding_equipment/4.029> ;
    skos:definition "A revolving stone used to sharpen or polish by grinding." ;
    skos:editorialNote "dc_finds_small_finds_type;58" ;
    skos:inScheme <http://id.acdh.oeaw.ac.at/defc/thesaurus/FindsSchema>,
        <http://id.acdh.oeaw.ac.at/defc/thesaurus/FindsSmallFindsType> ;
    skos:prefLabel "Schleifstein"@de,
        "grindstone"@en .

<http://id.acdh.oeaw.ac.at/defc/thesaurus/grooved/5.123> a skos:Concept ;
    dc:source "Kipfer, B. A. Dictionary of Artifacts 2007. Blackwell Publishing, Oxford.p. 136" ;
    skos:altLabel "Kannelur"@de,
        "gerillt"@de,
        "channeled"@en,
        "fluted"@en ;
    skos:broader <http://id.acdh.oeaw.ac.at/defc/thesaurus/incised/4.168> ;
    skos:definition "Pottery decoration in which broad lines are drawn on the firm but unbaked pot surface. No clay is removed, as it is in excised decoration, nor is the surface itself broken, as with incised decoration." ;
    skos:editorialNote "dc_finds_pottery_decoration;123" ;
    skos:inScheme <http://id.acdh.oeaw.ac.at/defc/thesaurus/FindsPotteryDecoration>,
        <http://id.acdh.oeaw.ac.at/defc/thesaurus/FindsSchema> ;
    skos:prefLabel "Kanneliert"@de,
        "grooved"@en .

<http://id.acdh.oeaw.ac.at/defc/thesaurus/grooved_with_graphite/5.197> a skos:Concept ;
    dc:source "OREA" ;
    skos:broader <http://id.acdh.oeaw.ac.at/defc/thesaurus/incised/4.168> ;
    skos:definition "Pottery decoration in which broad lines are drawn on the firm but unbaked pot surface and painted graphite paint." ;
    skos:editorialNote "dc_finds_pottery_decoration;197" ;
    skos:inScheme <http://id.acdh.oeaw.ac.at/defc/thesaurus/FindsPotteryDecoration>,
        <http://id.acdh.oeaw.ac.at/defc/thesaurus/FindsSchema> ;
    skos:prefLabel "Kanneliert, mit Graphitbemalung"@de,
        "grooved with graphite"@en .

<http://id.acdh.oeaw.ac.at/defc/thesaurus/haft/4.123> a skos:Concept ;
    dc:source "Kipfer, B. A. Dictionary of Artifacts 2007. Blackwell Publishing, Oxford.p. 139" ;
    skos:altLabel "Heft"@de ;
    skos:broader <http://id.acdh.oeaw.ac.at/defc/thesaurus/tool/3.1> ;
    skos:definition "A handle of a compound weapon or a tool - such as an adze, awl, ax, or knife." ;
    skos:editorialNote "dc_finds_small_finds_type;123" ;
    skos:inScheme <http://id.acdh.oeaw.ac.at/defc/thesaurus/FindsSchema>,
        <http://id.acdh.oeaw.ac.at/defc/thesaurus/FindsSmallFindsType> ;
    skos:prefLabel "Griff"@de,
        "haft"@en .

<http://id.acdh.oeaw.ac.at/defc/thesaurus/halaf_painted/6.125> a skos:Concept ;
    dc:source "OREA" ;
    skos:broader <http://id.acdh.oeaw.ac.at/defc/thesaurus/pattern_painted/5.041> ;
    skos:definition "Pottery decorated by imprinting of the clay with different types of objects." ;
    skos:editorialNote "dc_finds_pottery_decoration;125" ;
    skos:inScheme <http://id.acdh.oeaw.ac.at/defc/thesaurus/FindsPotteryDecoration>,
        <http://id.acdh.oeaw.ac.at/defc/thesaurus/FindsSchema> ;
    skos:prefLabel "Halaf Bemalung"@de,
        "halaf painted"@en .

<http://id.acdh.oeaw.ac.at/defc/thesaurus/hammer/4.46> a skos:Concept ;
    dc:source "Kipfer, B. A. Dictionary of Artifacts 2007. Blackwell Publishing, Oxford.p.140" ;
    skos:broader <http://id.acdh.oeaw.ac.at/defc/thesaurus/tool/3.1> ;
    skos:definition "A hand tool with a heavy rigid head and a handle; used to deliver an impulsive force by striking." ;
    skos:editorialNote "dc_finds_small_finds_type;46" ;
    skos:inScheme <http://id.acdh.oeaw.ac.at/defc/thesaurus/FindsSchema>,
        <http://id.acdh.oeaw.ac.at/defc/thesaurus/FindsSmallFindsType> ;
    skos:prefLabel "Hammer"@de,
        "hammer"@en .

<http://id.acdh.oeaw.ac.at/defc/thesaurus/handle_with_knob/5.182> a skos:Concept ;
    skos:broader <http://id.acdh.oeaw.ac.at/defc/thesaurus/handle/4.031> ;
    skos:editorialNote "dc_finds_pottery_detail;182" ;
    skos:inScheme <http://id.acdh.oeaw.ac.at/defc/thesaurus/FindsPotteryDetail>,
        <http://id.acdh.oeaw.ac.at/defc/thesaurus/FindsSchema> ;
    skos:prefLabel "Griff mit Knubbe"@de,
        "handle with knob"@en .

<http://id.acdh.oeaw.ac.at/defc/thesaurus/hare/5.12> a skos:Concept ;
    dc:source "http://eol.org/pages/118009/overview" ;
    skos:broader <http://id.acdh.oeaw.ac.at/defc/thesaurus/mammal/4.020> ;
    skos:editorialNote "dc_finds_animal_remains_species;12" ;
    skos:inScheme <http://id.acdh.oeaw.ac.at/defc/thesaurus/FindsAnimalRemainsSpecies>,
        <http://id.acdh.oeaw.ac.at/defc/thesaurus/FindsSchema> ;
    skos:prefLabel "Hase"@de,
        "hare"@en,
        "Lepus europaeus"@la .

<http://id.acdh.oeaw.ac.at/defc/thesaurus/hare/5.27> a skos:Concept ;
    dc:source "http://eol.org/pages/133022/overview" ;
    skos:broader <http://id.acdh.oeaw.ac.at/defc/thesaurus/mammal/4.020> ;
    skos:editorialNote "dc_finds_animal_remains_species;27" ;
    skos:inScheme <http://id.acdh.oeaw.ac.at/defc/thesaurus/FindsAnimalRemainsSpecies>,
        <http://id.acdh.oeaw.ac.at/defc/thesaurus/FindsSchema> ;
    skos:prefLabel "Hase"@de,
        "hare"@en,
        "Lepus timidus"@la .

<http://id.acdh.oeaw.ac.at/defc/thesaurus/hearth/5.3> a skos:Concept ;
    dc:source "M. Brami, PhD after Catalhoyuk Research Project http://www.catalhoyuk.com/database/catal/help_glossary1.asp" ;
    skos:altLabel "Herd"@de ;
    skos:broader <http://id.acdh.oeaw.ac.at/defc/thesaurus/installation/4.078> ;
    skos:definition "A fire installation that lacks a superstructure." ;
    skos:editorialNote "dc_area_specialfeatures;3" ;
    skos:inScheme <http://id.acdh.oeaw.ac.at/defc/thesaurus/AreaSchema>,
        <http://id.acdh.oeaw.ac.at/defc/thesaurus/AreaSpecialfeatures> ;
    skos:prefLabel "hearth"@en .

<http://id.acdh.oeaw.ac.at/defc/thesaurus/hearth/5.7> a skos:Concept ;
    dc:source "OREA" ;
    skos:broader <http://id.acdh.oeaw.ac.at/defc/thesaurus/occupation_evidence/4.088> ;
    skos:definition "The slab or place on which a fire is made inside or in the vicinity of a cave or a rockshelter as an evidence of human occupation." ;
    skos:editorialNote "dc_area_evidenceofocupation;7" ;
    skos:inScheme <http://id.acdh.oeaw.ac.at/defc/thesaurus/AreaEvidenceofocupation>,
        <http://id.acdh.oeaw.ac.at/defc/thesaurus/AreaSchema> ;
    skos:prefLabel "Herd"@de,
        "hearth"@en .

<http://id.acdh.oeaw.ac.at/defc/thesaurus/hemp/3.12> a skos:Concept ;
    dc:source "http://eol.org/pages/594919/overview" ;
    skos:broader <http://id.acdh.oeaw.ac.at/defc/thesaurus/botany/2.2> ;
    skos:editorialNote "dc_botany_species;12" ;
    skos:inScheme <http://id.acdh.oeaw.ac.at/defc/thesaurus/BotanySpecies>,
        <http://id.acdh.oeaw.ac.at/defc/thesaurus/FindsSchema> ;
    skos:prefLabel "Hanf"@de,
        "hemp"@en,
        "Cannabis sativa"@la .

<http://id.acdh.oeaw.ac.at/defc/thesaurus/high_scraper/4.11> a skos:Concept ;
    dc:source "Inizan, M.-L., M. Reduron-Ballinger, H. Roche, J. Tixier 1999, Technology and Terminology of Knapped Stone. Nanterre: CREP., D. Srejovic (ed) 1997, Arheološki Leksikon." ;
    skos:altLabel "thick scraper"@en ;
    skos:broader <http://id.acdh.oeaw.ac.at/defc/thesaurus/retouched_tool/3.010> ;
    skos:definition "An end- or circular scraper with the retouch making scraper edge angle almost 90°." ;
    skos:editorialNote "dc_finds_lithics_retouched_tools;11" ;
    skos:inScheme <http://id.acdh.oeaw.ac.at/defc/thesaurus/FindsLithicsRetouchedTools>,
        <http://id.acdh.oeaw.ac.at/defc/thesaurus/FindsSchema> ;
    skos:prefLabel "high scraper"@en .

<http://id.acdh.oeaw.ac.at/defc/thesaurus/high_strap_handle/6.119> a skos:Concept ;
    dc:source "Kipfer, B. A. Dictionary of Artifacts 2007. Blackwell Publishing, Oxford.p 305" ;
    skos:broader <http://id.acdh.oeaw.ac.at/defc/thesaurus/strap_handle/5.78> ;
    skos:definition "Hoisting handle made from a strip of clay and attached to the body of the pot at two points before firing." ;
    skos:editorialNote "dc_finds_pottery_detail;119" ;
    skos:inScheme <http://id.acdh.oeaw.ac.at/defc/thesaurus/FindsPotteryDetail>,
        <http://id.acdh.oeaw.ac.at/defc/thesaurus/FindsSchema> ;
    skos:prefLabel "Hochgezogener Bandhenkel"@de,
        "high strap handle"@en .

<http://id.acdh.oeaw.ac.at/defc/thesaurus/high_strap_handle_with_knob/6.90> a skos:Concept ;
    dc:source "OREA" ;
    skos:broader <http://id.acdh.oeaw.ac.at/defc/thesaurus/strap_handle/5.78> ;
    skos:definition "Hoisting handle made from a strip of clay with round clay application of semicirucular cross section attached to the body of the pot at two points before firing." ;
    skos:editorialNote "dc_finds_pottery_detail;90" ;
    skos:inScheme <http://id.acdh.oeaw.ac.at/defc/thesaurus/FindsPotteryDetail>,
        <http://id.acdh.oeaw.ac.at/defc/thesaurus/FindsSchema> ;
    skos:prefLabel "Hochgezogener Bandhenkel mit Knubbe"@de,
        "high strap handle with knob"@en .

<http://id.acdh.oeaw.ac.at/defc/thesaurus/hill/2.2> a skos:Concept ;
    dc:source "https://en.oxforddictionaries.com/definition/hill" ;
    skos:broader "topography/1.099" ;
    skos:definition "A naturally raised area of land, not as high as a moutain."@en ;
    skos:editorialNote "dc_site_topography;2" ;
    skos:inScheme <http://id.acdh.oeaw.ac.at/defc/thesaurus/SiteSchema>,
        "SiteTopography" ;
    skos:prefLabel "Hügel"@de,
        "hill"@en .

<http://id.acdh.oeaw.ac.at/defc/thesaurus/hillside/2.3> a skos:Concept ;
    dc:source "https://en.oxforddictionaries.com/definition/hillside" ;
    skos:altLabel "Abhang"@de,
        "slope"@en ;
    skos:broader "topography/1.099" ;
    skos:definition "The sloping side of a hill."@en ;
    skos:editorialNote "dc_site_topography;3" ;
    skos:inScheme <http://id.acdh.oeaw.ac.at/defc/thesaurus/SiteSchema>,
        "SiteTopography" ;
    skos:prefLabel "Hang"@de,
        "hillside"@en .

<http://id.acdh.oeaw.ac.at/defc/thesaurus/hindlimb/6.2> a skos:Concept ;
    dc:source "https://en.oxforddictionaries.com/definition/hindlimb" ;
    skos:broader <http://id.acdh.oeaw.ac.at/defc/thesaurus/extremity/5.4> ;
    skos:definition "Either of the two back limbs of an animal." ;
    skos:editorialNote "dc_animal_remains_part;2" ;
    skos:inScheme <http://id.acdh.oeaw.ac.at/defc/thesaurus/AnimalRemainsPart>,
        <http://id.acdh.oeaw.ac.at/defc/thesaurus/FindsSchema> ;
    skos:prefLabel "hindlimb"@en .

<http://id.acdh.oeaw.ac.at/defc/thesaurus/hoe/4.131> a skos:Concept ;
    dc:source "Kipfer, B. A. Dictionary of Artifacts 2007. Blackwell Publishing, Oxford.p. 146" ;
    skos:broader <http://id.acdh.oeaw.ac.at/defc/thesaurus/tool/3.1> ;
    skos:definition "A digging implement consisting of a blade set at right angles to a long handle (haft). Early hoes had stone or wooden blades." ;
    skos:editorialNote "dc_finds_small_finds_type;131" ;
    skos:inScheme <http://id.acdh.oeaw.ac.at/defc/thesaurus/FindsSchema>,
        <http://id.acdh.oeaw.ac.at/defc/thesaurus/FindsSmallFindsType> ;
    skos:prefLabel "Hacke"@de,
        "hoe"@en .

<http://id.acdh.oeaw.ac.at/defc/thesaurus/hole-mouthed_jar/5.131> a skos:Concept ;
    dc:source "OREA" ;
    skos:altLabel "Beutelförmiges Gefäß"@de,
        "Engmundiges Topf"@de,
        "bag-shaped vessel"@en,
        "holemouthed jar"@en ;
    skos:broader <http://id.acdh.oeaw.ac.at/defc/thesaurus/jar/4.145> ;
    skos:definition "A jar with no rim or neck, rather the vessel lip attaches directily to the vessel wall." ;
    skos:editorialNote "dc_finds_pottery_form;131" ;
    skos:inScheme <http://id.acdh.oeaw.ac.at/defc/thesaurus/FindsPotteryForm>,
        <http://id.acdh.oeaw.ac.at/defc/thesaurus/FindsSchema> ;
    skos:prefLabel "Engmundiges Gefäß"@de,
        "hole-mouthed jar"@en .

<http://id.acdh.oeaw.ac.at/defc/thesaurus/hole/5.24> a skos:Concept ;
    dc:source "https://en.oxforddictionaries.com/definition/hole" ;
    skos:broader <http://id.acdh.oeaw.ac.at/defc/thesaurus/installation/4.078> ;
    skos:definition "A hollow place in a surface, natural or man-made." ;
    skos:editorialNote "dc_area_specialfeatures;24" ;
    skos:inScheme <http://id.acdh.oeaw.ac.at/defc/thesaurus/AreaSchema>,
        <http://id.acdh.oeaw.ac.at/defc/thesaurus/AreaSpecialfeatures> ;
    skos:prefLabel "hole"@en .

<http://id.acdh.oeaw.ac.at/defc/thesaurus/horn/3.8> a skos:Concept ;
    dc:source "http://dbpedia.org/page/Horn_(anatomy)" ;
    skos:broader <http://id.acdh.oeaw.ac.at/defc/thesaurus/organic/2.4> ;
    skos:definition "A horn is a pointed projection on the head of various animals consisting of a covering of keratin and other proteins surrounding a core of live bone." ;
    skos:editorialNote "dc_finds_material;8" ;
    skos:inScheme <http://id.acdh.oeaw.ac.at/defc/thesaurus/FindsMaterial>,
        <http://id.acdh.oeaw.ac.at/defc/thesaurus/FindsSchema> ;
    skos:prefLabel "Horn"@de,
        "horn"@en .

<http://id.acdh.oeaw.ac.at/defc/thesaurus/horn/4.7> a skos:Concept ;
    dc:source "https://en.oxforddictionaries.com/definition/horn" ;
    skos:broader <http://id.acdh.oeaw.ac.at/defc/thesaurus/animal_remains_part/3.07> ;
    skos:definition "A hard permanent outgrowth, often curved and pointed, found in pairs on the heads of cattle, sheep, goats, giraffes, etc. and consisting of a core of bone encased in keratinized skin." ;
    skos:editorialNote "dc_animal_remains_part;7" ;
    skos:inScheme <http://id.acdh.oeaw.ac.at/defc/thesaurus/AnimalRemainsPart>,
        <http://id.acdh.oeaw.ac.at/defc/thesaurus/FindsSchema> ;
    skos:prefLabel "Horn"@de,
        "horn"@en .

<http://id.acdh.oeaw.ac.at/defc/thesaurus/horned_handle/5.72> a skos:Concept ;
    dc:source "OREA" ;
    skos:altLabel "Hornhenkel"@de,
        "horn handle"@en ;
    skos:broader <http://id.acdh.oeaw.ac.at/defc/thesaurus/handle/4.031> ;
    skos:definition "A handle in a shape of a horn – wide at one end and pointy at the other, upper end or a handle with pointy applcations." ;
    skos:editorialNote "dc_finds_pottery_detail;72" ;
    skos:inScheme <http://id.acdh.oeaw.ac.at/defc/thesaurus/FindsPotteryDetail>,
        <http://id.acdh.oeaw.ac.at/defc/thesaurus/FindsSchema> ;
    skos:prefLabel "Henkel mit Hornaufsatz"@de,
        "horned handle"@en .

<http://id.acdh.oeaw.ac.at/defc/thesaurus/horned_strap_handle/6.92> a skos:Concept ;
    dc:source "OREA" ;
    skos:broader <http://id.acdh.oeaw.ac.at/defc/thesaurus/strap_handle/5.78> ;
    skos:definition "A handle made from a strip of clay with pointy (horn) application." ;
    skos:editorialNote "dc_finds_pottery_detail;92" ;
    skos:inScheme <http://id.acdh.oeaw.ac.at/defc/thesaurus/FindsPotteryDetail>,
        <http://id.acdh.oeaw.ac.at/defc/thesaurus/FindsSchema> ;
    skos:prefLabel "Bandhenkel mit Hornaufsatz"@de,
        "horned strap handle"@en .

<http://id.acdh.oeaw.ac.at/defc/thesaurus/horse/5.11> a skos:Concept ;
    dc:source "http://eol.org/pages/328648/overview" ;
    skos:broader <http://id.acdh.oeaw.ac.at/defc/thesaurus/mammal/4.020> ;
    skos:editorialNote "dc_finds_animal_remains_species;11" ;
    skos:inScheme <http://id.acdh.oeaw.ac.at/defc/thesaurus/FindsAnimalRemainsSpecies>,
        <http://id.acdh.oeaw.ac.at/defc/thesaurus/FindsSchema> ;
    skos:prefLabel "Pferd"@de,
        "horse"@en,
        "Equus caballus"@la .

<http://id.acdh.oeaw.ac.at/defc/thesaurus/house_model/4.88> a skos:Concept ;
    dc:source "OREA" ;
    skos:broader <http://id.acdh.oeaw.ac.at/defc/thesaurus/figurine/3.3> ;
    skos:definition "A small carved or sculpted model of a house, usually of clay or stone." ;
    skos:editorialNote "dc_finds_small_finds_type;88" ;
    skos:inScheme <http://id.acdh.oeaw.ac.at/defc/thesaurus/FindsSchema>,
        <http://id.acdh.oeaw.ac.at/defc/thesaurus/FindsSmallFindsType> ;
    skos:prefLabel "Hausmodell"@de,
        "house model"@en .

<http://id.acdh.oeaw.ac.at/defc/thesaurus/houses_agglutinated/5.5> a skos:Concept ;
    dc:source "OREA (M. Brami)" ;
    skos:broader <http://id.acdh.oeaw.ac.at/defc/thesaurus/house_layout/4.074> ;
    skos:definition "Tightly clustered buildings." ;
    skos:editorialNote "dc_area_settlementstructure;5" ;
    skos:inScheme <http://id.acdh.oeaw.ac.at/defc/thesaurus/AreaSchema>,
        <http://id.acdh.oeaw.ac.at/defc/thesaurus/AreaSettlementstructure> ;
    skos:prefLabel "Agglutunierende Häuser"@de,
        "houses agglutinated"@en .

<http://id.acdh.oeaw.ac.at/defc/thesaurus/houses_free-standing/5.4> a skos:Concept ;
    dc:source "OREA (M. Brami)" ;
    skos:broader <http://id.acdh.oeaw.ac.at/defc/thesaurus/house_layout/4.074> ;
    skos:definition "A building which is not attached nor supported by another building." ;
    skos:editorialNote "dc_area_settlementstructure;4" ;
    skos:inScheme <http://id.acdh.oeaw.ac.at/defc/thesaurus/AreaSchema>,
        <http://id.acdh.oeaw.ac.at/defc/thesaurus/AreaSettlementstructure> ;
    skos:prefLabel "Freistehende Häuser"@de,
        "houses free-standing"@en .

<http://id.acdh.oeaw.ac.at/defc/thesaurus/houses_radial/5.6> a skos:Concept ;
    dc:source "OREA" ;
    skos:broader <http://id.acdh.oeaw.ac.at/defc/thesaurus/house_layout/4.074> ;
    skos:definition "Houses arranged in radial plan." ;
    skos:editorialNote "dc_area_settlementstructure;6" ;
    skos:inScheme <http://id.acdh.oeaw.ac.at/defc/thesaurus/AreaSchema>,
        <http://id.acdh.oeaw.ac.at/defc/thesaurus/AreaSettlementstructure> ;
    skos:prefLabel "Ringformige Häuser"@de,
        "houses radial"@en .

<http://id.acdh.oeaw.ac.at/defc/thesaurus/human_remains_absence/5.1> a skos:Concept ;
    dc:source "OREA" ;
    skos:broader <http://id.acdh.oeaw.ac.at/defc/thesaurus/human_remains/4.085> ;
    skos:definition "Human remains were not found on the site." ;
    skos:editorialNote "dc_area_evidenceofgraveshumanremains;1" ;
    skos:inScheme <http://id.acdh.oeaw.ac.at/defc/thesaurus/AreaEvidenceofgraveshumanremains>,
        <http://id.acdh.oeaw.ac.at/defc/thesaurus/AreaSchema> ;
    skos:prefLabel "human remains absence"@en .

<http://id.acdh.oeaw.ac.at/defc/thesaurus/human_remains_presence/5.2> a skos:Concept ;
    dc:source "OREA" ;
    skos:broader <http://id.acdh.oeaw.ac.at/defc/thesaurus/human_remains/4.085> ;
    skos:definition "Human remains were found on the site." ;
    skos:editorialNote "dc_area_evidenceofgraveshumanremains;2" ;
    skos:inScheme <http://id.acdh.oeaw.ac.at/defc/thesaurus/AreaEvidenceofgraveshumanremains>,
        <http://id.acdh.oeaw.ac.at/defc/thesaurus/AreaSchema> ;
    skos:prefLabel "human remains presence"@en .

<http://id.acdh.oeaw.ac.at/defc/thesaurus/human_remains_report/2.14> a skos:Concept ;
    dc:source "http://www.sfu.museum/forensics/eng/pg_media-media_pg/anthropologie-anthropology/" ;
    skos:broader <http://id.acdh.oeaw.ac.at/defc/thesaurus/special_analysis/1.057> ;
    skos:definition "Skeletal remains analyzed for sex, age at death, stature, and possible causes of death." ;
    skos:editorialNote "dc_researchevent_special_analysis/2.14" ;
    skos:inScheme <http://id.acdh.oeaw.ac.at/defc/thesaurus/ResearchEventSchema>,
        <http://id.acdh.oeaw.ac.at/defc/thesaurus/ResearcheventSpecialAnalysis> ;
    skos:prefLabel "Bericht physische Athropologie"@de,
        "human remains report"@en .

<http://id.acdh.oeaw.ac.at/defc/thesaurus/hunting/2.4> a skos:Concept ;
    dc:source "OREA" ;
    skos:broader <http://id.acdh.oeaw.ac.at/defc/thesaurus/subsistence/1.043> ;
    skos:definition "The activity of hunting wild animals or game for food, fur, bone (for bone tool production) etc." ;
    skos:editorialNote "dc_interpretation_subsistencetype;4" ;
    skos:inScheme <http://id.acdh.oeaw.ac.at/defc/thesaurus/InterpretationSchema>,
        <http://id.acdh.oeaw.ac.at/defc/thesaurus/InterpretationSubsistencetype> ;
    skos:prefLabel "Jagd"@de,
        "hunting"@en .

<http://id.acdh.oeaw.ac.at/defc/thesaurus/husking_bowl/5.190> a skos:Concept ;
    dc:source "OREA" ;
    skos:altLabel "husking tray"@en ;
    skos:broader <http://id.acdh.oeaw.ac.at/defc/thesaurus/bowl/4.115> ;
    skos:definition "A bowl used for husking cereals." ;
    skos:editorialNote "dc_finds_pottery_form;190" ;
    skos:inScheme <http://id.acdh.oeaw.ac.at/defc/thesaurus/FindsPotteryForm>,
        <http://id.acdh.oeaw.ac.at/defc/thesaurus/FindsSchema> ;
    skos:prefLabel "“Husking Bowl”"@de,
        "husking bowl"@en .

<http://id.acdh.oeaw.ac.at/defc/thesaurus/husking_bowl/5.196> a skos:Concept ;
    dc:source "OREA" ;
    skos:altLabel "husking tray"@en ;
    skos:broader <http://id.acdh.oeaw.ac.at/defc/thesaurus/bowl/4.115> ;
    skos:definition "A bowl used for husking cereals." ;
    skos:editorialNote "dc_finds_pottery_form;196" ;
    skos:inScheme <http://id.acdh.oeaw.ac.at/defc/thesaurus/FindsPotteryForm>,
        <http://id.acdh.oeaw.ac.at/defc/thesaurus/FindsSchema> ;
    skos:prefLabel "husking bowl"@en .

<http://id.acdh.oeaw.ac.at/defc/thesaurus/impresso/5.126> a skos:Concept ;
    dc:source "OREA" ;
    skos:broader <http://id.acdh.oeaw.ac.at/defc/thesaurus/incised/4.168> ;
    skos:definition "Pottery decorated by imprinting of the clay with different types of objects." ;
    skos:editorialNote "dc_finds_pottery_decoration;126" ;
    skos:inScheme <http://id.acdh.oeaw.ac.at/defc/thesaurus/FindsPotteryDecoration>,
        <http://id.acdh.oeaw.ac.at/defc/thesaurus/FindsSchema> ;
    skos:prefLabel "Impresso"@de,
        "impresso"@en .

<http://id.acdh.oeaw.ac.at/defc/thesaurus/impresso_(a2)/5.151> a skos:Concept ;
    dc:source "OREA" ;
    skos:broader <http://id.acdh.oeaw.ac.at/defc/thesaurus/incised/4.168> ;
    skos:definition "Pottery decorated by imprinting of the clay with different types of objects." ;
    skos:editorialNote "dc_finds_pottery_decoration;151" ;
    skos:inScheme <http://id.acdh.oeaw.ac.at/defc/thesaurus/FindsPotteryDecoration>,
        <http://id.acdh.oeaw.ac.at/defc/thesaurus/FindsSchema> ;
    skos:prefLabel "Impresso (A2)"@de,
        "impresso (a2)"@en .

<http://id.acdh.oeaw.ac.at/defc/thesaurus/in_cave/5.3> a skos:Concept ;
    skos:broader <http://id.acdh.oeaw.ac.at/defc/thesaurus/grave_location/4.087> ;
    skos:editorialNote "dc_area_topography;3" ;
    skos:inScheme <http://id.acdh.oeaw.ac.at/defc/thesaurus/AreaSchema>,
        <http://id.acdh.oeaw.ac.at/defc/thesaurus/AreaTopography> ;
    skos:prefLabel "in cave"@en .

<http://id.acdh.oeaw.ac.at/defc/thesaurus/incised-pointillé_decoration/5.127> a skos:Concept ;
    dc:source "Kipfer, B. A. Dictionary of Artifacts 2007. Blackwell Publishing, Oxford.p. 247" ;
    skos:broader <http://id.acdh.oeaw.ac.at/defc/thesaurus/incised/4.168> ;
    skos:definition "Pottery decoration by cuting dots in the surface." ;
    skos:editorialNote "dc_finds_pottery_decoration;127" ;
    skos:inScheme <http://id.acdh.oeaw.ac.at/defc/thesaurus/FindsPotteryDecoration>,
        <http://id.acdh.oeaw.ac.at/defc/thesaurus/FindsSchema> ;
    skos:prefLabel "Ritzverzierter-Pointillé Dekor"@de,
        "incised-pointillé decoration"@en .

<http://id.acdh.oeaw.ac.at/defc/thesaurus/incised_(b2)/5.152> a skos:Concept ;
    dc:source "OREA" ;
    skos:broader <http://id.acdh.oeaw.ac.at/defc/thesaurus/incised/4.168> ;
    skos:definition "Pottery decorated by cuts into the surface." ;
    skos:editorialNote "dc_finds_pottery_decoration;152" ;
    skos:inScheme <http://id.acdh.oeaw.ac.at/defc/thesaurus/FindsPotteryDecoration>,
        <http://id.acdh.oeaw.ac.at/defc/thesaurus/FindsSchema> ;
    skos:prefLabel "Ritzverziert (B2)"@de,
        "incised (b2)"@en .

<http://id.acdh.oeaw.ac.at/defc/thesaurus/incised_(γ2)/5.153> a skos:Concept ;
    dc:source "OREA" ;
    skos:broader <http://id.acdh.oeaw.ac.at/defc/thesaurus/incised/4.168> ;
    skos:definition "Pottery decorated by cuts into the surface." ;
    skos:editorialNote "dc_finds_pottery_decoration;153" ;
    skos:inScheme <http://id.acdh.oeaw.ac.at/defc/thesaurus/FindsPotteryDecoration>,
        <http://id.acdh.oeaw.ac.at/defc/thesaurus/FindsSchema> ;
    skos:prefLabel "Ritzverziert (C2)"@de,
        "incised (γ2)"@en .

<http://id.acdh.oeaw.ac.at/defc/thesaurus/incomplete/4.2> a skos:Concept ;
    dc:source "OREA" ;
    skos:broader <http://id.acdh.oeaw.ac.at/defc/thesaurus/completness_of_animal_remains/3.05> ;
    skos:definition "The animal remains found were incomplete." ;
    skos:editorialNote "dc_finds_animal_remains_completness;2" ;
    skos:inScheme <http://id.acdh.oeaw.ac.at/defc/thesaurus/FindsAnimalRemainsCompletness>,
        <http://id.acdh.oeaw.ac.at/defc/thesaurus/FindsSchema> ;
    skos:prefLabel "incomplete"@en .

<http://id.acdh.oeaw.ac.at/defc/thesaurus/incrusted/5.122> a skos:Concept ;
    dc:source "Kipfer, B. A. Dictionary of Artifacts 2007. Blackwell Publishing, Oxford.p. 153" ;
    skos:broader <http://id.acdh.oeaw.ac.at/defc/thesaurus/incised/4.168> ;
    skos:definition "Pottery decoration by impressing of material into the surface of a ceramic object." ;
    skos:editorialNote "dc_finds_pottery_decoration;122" ;
    skos:inScheme <http://id.acdh.oeaw.ac.at/defc/thesaurus/FindsPotteryDecoration>,
        <http://id.acdh.oeaw.ac.at/defc/thesaurus/FindsSchema> ;
    skos:prefLabel "Inkrustiert"@de,
        "incrusted"@en .

<http://id.acdh.oeaw.ac.at/defc/thesaurus/indirect_percussion/5.2> a skos:Concept ;
    dc:source "Inizan, M.-L., M. Reduron-Ballinger, H. Roche, J. Tixier 1999, Technology and Terminology of Knapped Stone. Nanterre: CREP. p. 148." ;
    skos:broader <http://id.acdh.oeaw.ac.at/defc/thesaurus/lithics_technology/4.023> ;
    skos:definition "The action of striking one object with another. Indirect percussion involves an intermediate object (a punch) as well as a hammer." ;
    skos:editorialNote "dc_finds_lithics_technology;2" ;
    skos:inScheme <http://id.acdh.oeaw.ac.at/defc/thesaurus/FindsLithicsTechnology>,
        <http://id.acdh.oeaw.ac.at/defc/thesaurus/FindsSchema> ;
    skos:prefLabel "indirect percussion"@en .

<http://id.acdh.oeaw.ac.at/defc/thesaurus/infans_i_(0-6)/6.2> a skos:Concept ;
    skos:broader <http://id.acdh.oeaw.ac.at/defc/thesaurus/age_group/5.097> ;
    skos:editorialNote "dc_area_agegroups;2" ;
    skos:inScheme <http://id.acdh.oeaw.ac.at/defc/thesaurus/AreaAgegroups>,
        <http://id.acdh.oeaw.ac.at/defc/thesaurus/AreaSchema> ;
    skos:prefLabel "infans i (0-6)"@en .

<http://id.acdh.oeaw.ac.at/defc/thesaurus/infans_ii_(7-12)/6.3> a skos:Concept ;
    skos:broader <http://id.acdh.oeaw.ac.at/defc/thesaurus/age_group/5.097> ;
    skos:editorialNote "dc_area_agegroups;3" ;
    skos:inScheme <http://id.acdh.oeaw.ac.at/defc/thesaurus/AreaAgegroups>,
        <http://id.acdh.oeaw.ac.at/defc/thesaurus/AreaSchema> ;
    skos:prefLabel "infans ii (7-12)"@en .

<http://id.acdh.oeaw.ac.at/defc/thesaurus/inhumation/6.2> a skos:Concept ;
    skos:broader <http://id.acdh.oeaw.ac.at/defc/thesaurus/human_remains_type/5.096> ;
    skos:editorialNote "dc_area_typeofhumanremains;2" ;
    skos:inScheme <http://id.acdh.oeaw.ac.at/defc/thesaurus/AreaSchema>,
        <http://id.acdh.oeaw.ac.at/defc/thesaurus/AreaTypeofhumanremains> ;
    skos:prefLabel "inhumation"@en .

<http://id.acdh.oeaw.ac.at/defc/thesaurus/inland/2.4> a skos:Concept ;
    dc:source "https://en.oxforddictionaries.com/definition/inland" ;
    skos:broader "topography/1.099" ;
    skos:definition "Situated in the interior rather than on the coast."@en ;
    skos:editorialNote "dc_site_topography;4" ;
    skos:inScheme <http://id.acdh.oeaw.ac.at/defc/thesaurus/SiteSchema>,
        "SiteTopography" ;
    skos:prefLabel "Im Landesinneren"@de,
        "inland"@en .

<http://id.acdh.oeaw.ac.at/defc/thesaurus/inlay/4.125> a skos:Concept ;
    dc:source "Kipfer, B. A. Dictionary of Artifacts 2007. Blackwell Publishing, Oxford.p. 154" ;
    skos:broader <http://id.acdh.oeaw.ac.at/defc/thesaurus/jewellery/3.2> ;
    skos:definition "Placement of one material, either glass or metal, into a prepared depression (reservoir) on the surface of an item for decorative purposes." ;
    skos:editorialNote "dc_finds_small_finds_type;125" ;
    skos:inScheme <http://id.acdh.oeaw.ac.at/defc/thesaurus/FindsSchema>,
        <http://id.acdh.oeaw.ac.at/defc/thesaurus/FindsSmallFindsType> ;
    skos:prefLabel "Einlegearbeit"@de,
        "inlay"@en .

<http://id.acdh.oeaw.ac.at/defc/thesaurus/inscription/4.114> a skos:Concept ;
    dc:source "Kipfer, B. A. Dictionary of Artifacts 2007. Blackwell Publishing, Oxford.p 154" ;
    skos:broader <http://id.acdh.oeaw.ac.at/defc/thesaurus/other/3.4> ;
    skos:definition "Something that is inscribed; the act of inscribing. It is writing or any type cut into or raised upon a hard surface - clay, wood, stone, metal, etc. - and therefore endures." ;
    skos:editorialNote "dc_finds_small_finds_type;114" ;
    skos:inScheme <http://id.acdh.oeaw.ac.at/defc/thesaurus/FindsSchema>,
        <http://id.acdh.oeaw.ac.at/defc/thesaurus/FindsSmallFindsType> ;
    skos:prefLabel "Inschrift"@de,
        "inscription"@en .

<http://id.acdh.oeaw.ac.at/defc/thesaurus/inside_bevelled_and_decorated_rim/5.73> a skos:Concept ;
    dc:source "Blegen 1950, 58." ;
    skos:broader <http://id.acdh.oeaw.ac.at/defc/thesaurus/rim/4.033> ;
    skos:definition "Uppoer part of the vessel with thickened inner side of lip, forming flat or slightly convex band, fairly sharply offset so that it ends with an angular or somewhat rounded inner edge." ;
    skos:editorialNote "dc_finds_pottery_detail;73" ;
    skos:inScheme <http://id.acdh.oeaw.ac.at/defc/thesaurus/FindsPotteryDetail>,
        <http://id.acdh.oeaw.ac.at/defc/thesaurus/FindsSchema> ;
    skos:prefLabel "Innen abgestrichener Rand mit Verzierung"@de,
        "inside bevelled and decorated rim"@en .

<http://id.acdh.oeaw.ac.at/defc/thesaurus/intramural/5.1> a skos:Concept ;
    skos:broader <http://id.acdh.oeaw.ac.at/defc/thesaurus/grave_location/4.087> ;
    skos:editorialNote "dc_area_topography;1" ;
    skos:inScheme <http://id.acdh.oeaw.ac.at/defc/thesaurus/AreaSchema>,
        <http://id.acdh.oeaw.ac.at/defc/thesaurus/AreaTopography> ;
    skos:prefLabel "intramural"@en .

<http://id.acdh.oeaw.ac.at/defc/thesaurus/jasper/3.14> a skos:Concept ;
    dc:source "https://www.britannica.com/topic/jasper-mineral" ;
    skos:broader <http://id.acdh.oeaw.ac.at/defc/thesaurus/stone/2.1> ;
    skos:definition "An opaque, fine-grained or dense variety of the silica mineral chert that exhibits various colours. Chiefly brick red to brownish red, it owes its colour to admixed hematite; but when it occurs with clay admixed, the colour is a yellowish white or gray, o" ;
    skos:editorialNote "dc_finds_material;14" ;
    skos:inScheme <http://id.acdh.oeaw.ac.at/defc/thesaurus/FindsMaterial>,
        <http://id.acdh.oeaw.ac.at/defc/thesaurus/FindsSchema> ;
    skos:prefLabel "Jaspis"@de,
        "jasper"@en .

<http://id.acdh.oeaw.ac.at/defc/thesaurus/jasper/5.5> a skos:Concept ;
    dc:source "https://www.britannica.com/topic/jasper-mineral" ;
    skos:broader <http://id.acdh.oeaw.ac.at/defc/thesaurus/stone/4.025> ;
    skos:definition "An opaque, fine-grained or dense variety of the silica mineral chert that exhibits various colours. Chiefly brick red to brownish red, it owes its colour to admixed hematite; but when it occurs with clay admixed, the colour is a yellowish white or gray. Used to produce lithics." ;
    skos:editorialNote "dc_finds_lithics_raw_material;5" ;
    skos:inScheme <http://id.acdh.oeaw.ac.at/defc/thesaurus/FindsLithicsRawMaterial>,
        <http://id.acdh.oeaw.ac.at/defc/thesaurus/FindsSchema> ;
    skos:prefLabel "Jaspis"@de,
        "jasper"@en .

<http://id.acdh.oeaw.ac.at/defc/thesaurus/jaw/5.6> a skos:Concept ;
    dc:source "https://www.britannica.com/science/jaw" ;
    skos:broader <http://id.acdh.oeaw.ac.at/defc/thesaurus/bone/4.021> ;
    skos:definition "Either of a par of bones that form the framework of the mouth of vertebrate animals, usually containing teeth and including a movable lower jaw (mandible) and fixed upper jaw (maxilla)." ;
    skos:editorialNote "dc_animal_remains_part;6" ;
    skos:inScheme <http://id.acdh.oeaw.ac.at/defc/thesaurus/AnimalRemainsPart>,
        <http://id.acdh.oeaw.ac.at/defc/thesaurus/FindsSchema> ;
    skos:prefLabel "jaw"@en .

<http://id.acdh.oeaw.ac.at/defc/thesaurus/jewellery_production/2.9> a skos:Concept ;
    dc:source "OREA" ;
    skos:broader <http://id.acdh.oeaw.ac.at/defc/thesaurus/production/1.042> ;
    skos:definition "The activity of making physical items used as personal ornament." ;
    skos:editorialNote "dc_interpretation_productiontype;9" ;
    skos:inScheme <http://id.acdh.oeaw.ac.at/defc/thesaurus/InterpretationProductiontype>,
        <http://id.acdh.oeaw.ac.at/defc/thesaurus/InterpretationSchema> ;
    skos:prefLabel "Schmukproduktion"@de,
        "jewellery production"@en .

<http://id.acdh.oeaw.ac.at/defc/thesaurus/juvenile_(13-18)/6.4> a skos:Concept ;
    skos:broader <http://id.acdh.oeaw.ac.at/defc/thesaurus/age_group/5.097> ;
    skos:editorialNote "dc_area_agegroups;4" ;
    skos:inScheme <http://id.acdh.oeaw.ac.at/defc/thesaurus/AreaAgegroups>,
        <http://id.acdh.oeaw.ac.at/defc/thesaurus/AreaSchema> ;
    skos:prefLabel "juvenile (13-18)"@en .

<http://id.acdh.oeaw.ac.at/defc/thesaurus/kiliya_figurine/5.136> a skos:Concept ;
    skos:broader <http://id.acdh.oeaw.ac.at/defc/thesaurus/anthropomorphic_figurine/4.84> ;
    skos:editorialNote "dc_finds_small_finds_type;136" ;
    skos:inScheme <http://id.acdh.oeaw.ac.at/defc/thesaurus/FindsSchema>,
        <http://id.acdh.oeaw.ac.at/defc/thesaurus/FindsSmallFindsType> ;
    skos:prefLabel "Figurine Typ Kiliya"@de,
        "Kiliya figurine"@en .

<http://id.acdh.oeaw.ac.at/defc/thesaurus/kiln/5.36> a skos:Concept ;
    dc:source "http://dbpedia.org/page/Kiln" ;
    skos:altLabel "Brennofen"@de ;
    skos:broader <http://id.acdh.oeaw.ac.at/defc/thesaurus/installation/4.078> ;
    skos:definition "A kiln is a thermally insulated chamber, a type of oven, that produces temperatures sufficient to complete hardening and drying of clay, metal etc." ;
    skos:editorialNote "dc_area_specialfeatures;36" ;
    skos:inScheme <http://id.acdh.oeaw.ac.at/defc/thesaurus/AreaSchema>,
        <http://id.acdh.oeaw.ac.at/defc/thesaurus/AreaSpecialfeatures> ;
    skos:prefLabel "kiln"@en .

<http://id.acdh.oeaw.ac.at/defc/thesaurus/knife/4.12> a skos:Concept ;
    dc:source "Kipfer, B. A. Dictionary of Artifacts 2007. Blackwell Publishing, Oxford.p. 166." ;
    skos:broader <http://id.acdh.oeaw.ac.at/defc/thesaurus/retouched_tool/3.010> ;
    skos:definition "A backed blade; a cutting instrument composed of a blade and a handle into which it is fixed, either rigidly or with a joint." ;
    skos:editorialNote "dc_finds_lithics_retouched_tools;12" ;
    skos:inScheme <http://id.acdh.oeaw.ac.at/defc/thesaurus/FindsLithicsRetouchedTools>,
        <http://id.acdh.oeaw.ac.at/defc/thesaurus/FindsSchema> ;
    skos:prefLabel "knife"@en .

<http://id.acdh.oeaw.ac.at/defc/thesaurus/knife/4.122> a skos:Concept ;
    dc:source "Kipfer, B. A. Dictionary of Artifacts 2007. Blackwell Publishing, Oxford.p. 166." ;
    skos:broader <http://id.acdh.oeaw.ac.at/defc/thesaurus/tool/3.1> ;
    skos:definition "A backed blade; a cutting instrument composed of a blade and a handle into which it is fixed, either rigidly or with a joint." ;
    skos:editorialNote "dc_finds_small_finds_type;122" ;
    skos:inScheme <http://id.acdh.oeaw.ac.at/defc/thesaurus/FindsSchema>,
        <http://id.acdh.oeaw.ac.at/defc/thesaurus/FindsSmallFindsType> ;
    skos:prefLabel "Messer"@de,
        "knife"@en .

<http://id.acdh.oeaw.ac.at/defc/thesaurus/knob-row/5.99> a skos:Concept ;
    dc:source "OREA" ;
    skos:altLabel "knob row"@en ;
    skos:broader <http://id.acdh.oeaw.ac.at/defc/thesaurus/attachment/4.034> ;
    skos:definition "Vertically applied series of round clay objects." ;
    skos:editorialNote "dc_finds_pottery_detail;99" ;
    skos:inScheme <http://id.acdh.oeaw.ac.at/defc/thesaurus/FindsPotteryDetail>,
        <http://id.acdh.oeaw.ac.at/defc/thesaurus/FindsSchema> ;
    skos:prefLabel "Vertikale Knubbenreihe"@de,
        "knob-row"@en .

<http://id.acdh.oeaw.ac.at/defc/thesaurus/knob/4.130> a skos:Concept ;
    skos:broader <http://id.acdh.oeaw.ac.at/defc/thesaurus/tool/3.1> ;
    skos:editorialNote "dc_finds_small_finds_type;130" ;
    skos:inScheme <http://id.acdh.oeaw.ac.at/defc/thesaurus/FindsSchema>,
        <http://id.acdh.oeaw.ac.at/defc/thesaurus/FindsSmallFindsType> ;
    skos:prefLabel "Griff"@de,
        "knob"@en .

<http://id.acdh.oeaw.ac.at/defc/thesaurus/knob/5.74> a skos:Concept ;
    dc:source "OREA" ;
    skos:broader <http://id.acdh.oeaw.ac.at/defc/thesaurus/attachment/4.034> ;
    skos:definition "Round application with a semicircular cross section." ;
    skos:editorialNote "dc_finds_pottery_detail;74" ;
    skos:inScheme <http://id.acdh.oeaw.ac.at/defc/thesaurus/FindsPotteryDetail>,
        <http://id.acdh.oeaw.ac.at/defc/thesaurus/FindsSchema> ;
    skos:prefLabel "Knubbe"@de,
        "knob"@en .

<http://id.acdh.oeaw.ac.at/defc/thesaurus/knobbed_handle/5.120> a skos:Concept ;
    dc:source "OREA" ;
    skos:broader <http://id.acdh.oeaw.ac.at/defc/thesaurus/handle/4.031> ;
    skos:definition "A handle with round application(s)." ;
    skos:editorialNote "dc_finds_pottery_detail;120" ;
    skos:inScheme <http://id.acdh.oeaw.ac.at/defc/thesaurus/FindsPotteryDetail>,
        <http://id.acdh.oeaw.ac.at/defc/thesaurus/FindsSchema> ;
    skos:prefLabel "Henkel mit aufgesetzter Knubbe"@de,
        "knobbed handle"@en .

<http://id.acdh.oeaw.ac.at/defc/thesaurus/knobbed_wishbone_handle/6.144> a skos:Concept ;
    dc:source "OREA" ;
    skos:broader <http://id.acdh.oeaw.ac.at/defc/thesaurus/wishbone_handle/5.93> ;
    skos:definition "A liminal horizontal birdbone shaped loop handle with round applications." ;
    skos:editorialNote "dc_finds_pottery_detail;144" ;
    skos:inScheme <http://id.acdh.oeaw.ac.at/defc/thesaurus/FindsPotteryDetail>,
        <http://id.acdh.oeaw.ac.at/defc/thesaurus/FindsSchema> ;
    skos:prefLabel "Gabelhenkel mit Knubbe"@de,
        "knobbed wishbone handle"@en .

<http://id.acdh.oeaw.ac.at/defc/thesaurus/labret/4.106> a skos:Concept ;
    dc:source "Kipfer, B. A. Dictionary of Artifacts 2007. Blackwell Publishing, Oxford.p 171" ;
    skos:altLabel "lip plug"@en ;
    skos:broader <http://id.acdh.oeaw.ac.at/defc/thesaurus/jewellery/3.2> ;
    skos:definition "A lip plug or ornament inserted in an incision in the lower lip, often made of shell, bone, ivory, metal, stone, wood, or pottery." ;
    skos:editorialNote "dc_finds_small_finds_type;106" ;
    skos:inScheme <http://id.acdh.oeaw.ac.at/defc/thesaurus/FindsSchema>,
        <http://id.acdh.oeaw.ac.at/defc/thesaurus/FindsSmallFindsType> ;
    skos:prefLabel "Lippenpflock"@de,
        "labret"@en .

<http://id.acdh.oeaw.ac.at/defc/thesaurus/ladle/4.133> a skos:Concept ;
    dc:source "OREA" ;
    skos:broader <http://id.acdh.oeaw.ac.at/defc/thesaurus/pottery_form/3.016> ;
    skos:definition "A particular piece of cutlery in a form of a long-handled scoop used for ladling food of liquids." ;
    skos:editorialNote "dc_finds_pottery_form;133" ;
    skos:inScheme <http://id.acdh.oeaw.ac.at/defc/thesaurus/FindsPotteryForm>,
        <http://id.acdh.oeaw.ac.at/defc/thesaurus/FindsSchema> ;
    skos:prefLabel "Schöpfkelle"@de,
        "ladle"@en .

<http://id.acdh.oeaw.ac.at/defc/thesaurus/lamp/4.134> a skos:Concept ;
    dc:source "OREA" ;
    skos:broader <http://id.acdh.oeaw.ac.at/defc/thesaurus/pottery_form/3.016> ;
    skos:definition "A vessel used to produce illumination." ;
    skos:editorialNote "dc_finds_pottery_form;134" ;
    skos:inScheme <http://id.acdh.oeaw.ac.at/defc/thesaurus/FindsPotteryForm>,
        <http://id.acdh.oeaw.ac.at/defc/thesaurus/FindsSchema> ;
    skos:prefLabel "Lampe"@de,
        "lamp"@en .

<http://id.acdh.oeaw.ac.at/defc/thesaurus/laser_scanning_survey/4.19> a skos:Concept ;
    dc:source "http://thesaurus.historicengland.org.uk/thesaurus_term.asp?thes_no=566&term_no=146342" ;
    skos:altLabel "LS"@en ;
    skos:broader <http://id.acdh.oeaw.ac.at/defc/thesaurus/field_survey/3.052> ;
    skos:definition "The recording of a surface, or surfaces, using scanning technologies, to create a 3D model of the target structure/object." ;
    skos:editorialNote "dc_researchevet_researchtype;19" ;
    skos:inScheme <http://id.acdh.oeaw.ac.at/defc/thesaurus/ResearchEventSchema>,
        <http://id.acdh.oeaw.ac.at/defc/thesaurus/ResearchevetResearchtype> ;
    skos:prefLabel "Laserscanning"@de,
        "laser scanning survey"@en .

<http://id.acdh.oeaw.ac.at/defc/thesaurus/lead/5.10> a skos:Concept ;
    dc:source "The Concise Oxford Dictionary of Archaeology" ;
    skos:broader <http://id.acdh.oeaw.ac.at/defc/thesaurus/metal/4.7> ;
    skos:definition "A soft, heavy, silvery-coloured metal (Pb) with a low melting point that was alloyed with copper and tin to make bronze tools and weapons. Extracted from a quarry site." ;
    skos:editorialNote "dc_area_rawmaterial;10" ;
    skos:inScheme <http://id.acdh.oeaw.ac.at/defc/thesaurus/AreaRawmaterial>,
        <http://id.acdh.oeaw.ac.at/defc/thesaurus/AreaSchema> ;
    skos:prefLabel "Blei"@de,
        "lead"@en .

<http://id.acdh.oeaw.ac.at/defc/thesaurus/ledge_lug/6.70> a skos:Concept ;
    dc:source "OREA" ;
    skos:broader <http://id.acdh.oeaw.ac.at/defc/thesaurus/lug/5.040> ;
    skos:definition "Bar shaped handhold added to the wall of a pot to assist in holding it." ;
    skos:editorialNote "dc_finds_pottery_detail;70" ;
    skos:inScheme <http://id.acdh.oeaw.ac.at/defc/thesaurus/FindsPotteryDetail>,
        <http://id.acdh.oeaw.ac.at/defc/thesaurus/FindsSchema> ;
    skos:prefLabel "Leistengriff"@de,
        "ledge lug"@en .

<http://id.acdh.oeaw.ac.at/defc/thesaurus/lentil/5.13> a skos:Concept ;
    dc:source "http://eol.org/pages/647510/overview" ;
    skos:altLabel "Linsen"@de ;
    skos:broader <http://id.acdh.oeaw.ac.at/defc/thesaurus/pulse/4.32> ;
    skos:editorialNote "dc_botany_species;13" ;
    skos:inScheme <http://id.acdh.oeaw.ac.at/defc/thesaurus/BotanySpecies>,
        <http://id.acdh.oeaw.ac.at/defc/thesaurus/FindsSchema> ;
    skos:prefLabel "Linsen-Wicke"@de,
        "lentil"@en,
        "Lens culinaris"@la .

<http://id.acdh.oeaw.ac.at/defc/thesaurus/lid/4.112> a skos:Concept ;
    dc:source "OREA" ;
    skos:broader <http://id.acdh.oeaw.ac.at/defc/thesaurus/pottery_form/3.016> ;
    skos:definition "A shape used for covering vessels." ;
    skos:editorialNote "dc_finds_pottery_form;112" ;
    skos:inScheme <http://id.acdh.oeaw.ac.at/defc/thesaurus/FindsPotteryForm>,
        <http://id.acdh.oeaw.ac.at/defc/thesaurus/FindsSchema> ;
    skos:prefLabel "Deckel"@de,
        "lid"@en .

<http://id.acdh.oeaw.ac.at/defc/thesaurus/limestone/3.22> a skos:Concept ;
    dc:source "http://dbpedia.org/page/Limestone" ;
    skos:broader <http://id.acdh.oeaw.ac.at/defc/thesaurus/stone/2.1> ;
    skos:definition "Limestone is a sedimentary rock composed largely of the minerals calcite and aragonite, which are different crystal forms of calcium carbonate (CaCO3).  Used as a building material or production of smaller objects." ;
    skos:editorialNote "dc_finds_material;22" ;
    skos:inScheme <http://id.acdh.oeaw.ac.at/defc/thesaurus/FindsMaterial>,
        <http://id.acdh.oeaw.ac.at/defc/thesaurus/FindsSchema> ;
    skos:prefLabel "Kalkstein"@de,
        "limestone"@en .

<http://id.acdh.oeaw.ac.at/defc/thesaurus/limestone/5.3> a skos:Concept ;
    skos:broader <http://id.acdh.oeaw.ac.at/defc/thesaurus/stone/4.072> ;
    skos:definition "A sedimentary rock most commoly formed in clear, warm, shallow marine waters. It was extracted from a quarry site and probably used as building material." ;
    skos:editorialNote "dc_area_rawmaterial;3" ;
    skos:inScheme <http://id.acdh.oeaw.ac.at/defc/thesaurus/AreaRawmaterial>,
        <http://id.acdh.oeaw.ac.at/defc/thesaurus/AreaSchema> ;
    skos:prefLabel "Kalkstein"@de,
        "limestone"@en .

<http://id.acdh.oeaw.ac.at/defc/thesaurus/limestone_floor/6.20> a skos:Concept ;
    dc:source "https://en.oxforddictionaries.com/definition/floor" ;
    skos:broader <http://id.acdh.oeaw.ac.at/defc/thesaurus/floor/5.092> ;
    skos:definition "The lower surface of a room, on which one may walk, made of limestone." ;
    skos:editorialNote "dc_area_buildingtechnique;20" ;
    skos:inScheme <http://id.acdh.oeaw.ac.at/defc/thesaurus/AreaBuildingtechnique>,
        <http://id.acdh.oeaw.ac.at/defc/thesaurus/AreaSchema> ;
    skos:prefLabel "Kalksteinboden"@de,
        "limestone floor"@en .

<http://id.acdh.oeaw.ac.at/defc/thesaurus/longhouse/5.1> a skos:Concept ;
    dc:source "OREA (M. Brami)" ;
    skos:broader <http://id.acdh.oeaw.ac.at/defc/thesaurus/building_type/4.077> ;
    skos:definition "A rectangular buidling with a strong imbalance in the lenght:width ratio. Typical for the Central European Neolithic (Linearbandkeramik Culture)." ;
    skos:editorialNote "dc_area_constructiontype;1" ;
    skos:inScheme <http://id.acdh.oeaw.ac.at/defc/thesaurus/AreaConstructiontype>,
        <http://id.acdh.oeaw.ac.at/defc/thesaurus/AreaSchema> ;
    skos:prefLabel "longhouse"@en .

<http://id.acdh.oeaw.ac.at/defc/thesaurus/loom_weight/5.71> a skos:Concept ;
    dc:source "Kipfer, B. A. Dictionary of Artifacts 2007. Blackwell Publishing, Oxford.p.182" ;
    skos:altLabel "loomweight"@en ;
    skos:broader <http://id.acdh.oeaw.ac.at/defc/thesaurus/textile_equipment/4.028> ;
    skos:definition "A perforated stone or ceramic block used for stretching the threads forming the warp or the weft on a loom." ;
    skos:editorialNote "dc_finds_small_finds_type;71" ;
    skos:inScheme <http://id.acdh.oeaw.ac.at/defc/thesaurus/FindsSchema>,
        <http://id.acdh.oeaw.ac.at/defc/thesaurus/FindsSmallFindsType> ;
    skos:prefLabel "Webgewicht"@de,
        "loom weight"@en .

<http://id.acdh.oeaw.ac.at/defc/thesaurus/looting/5.3> a skos:Concept ;
    dc:source "Kipfer, B. A. Encyclopedic Dictionary of Archaeology. Kluwer Academic/Plenum Publishers, New York. P.318." ;
    skos:broader <http://id.acdh.oeaw.ac.at/defc/thesaurus/grave_disturbance/4.084> ;
    skos:definition "Any unscientific and illegal act of pludering archaeological sites, especially graves, for profit." ;
    skos:editorialNote "dc_area_manipulationofgraves;3" ;
    skos:inScheme <http://id.acdh.oeaw.ac.at/defc/thesaurus/AreaManipulationofgraves>,
        <http://id.acdh.oeaw.ac.at/defc/thesaurus/AreaSchema> ;
    skos:prefLabel "Grabraub"@de,
        "looting"@en .

<http://id.acdh.oeaw.ac.at/defc/thesaurus/mace_head/5.44> a skos:Concept ;
    dc:source "Kipfer, B. A. Encyclopedic Dictionary of Archaeology. Kluwer Academic/Plenum Publishers, New York. P.323." ;
    skos:broader <http://id.acdh.oeaw.ac.at/defc/thesaurus/weapon/4.030> ;
    skos:definition "A small club like weapon, usually of stone, crafted to fit snugly in the hand, for pounding. It often had a perforated head and was attached to a shaft of wood (or ivory or hom), often tapering toward the end that was gripped." ;
    skos:editorialNote "dc_finds_small_finds_type;44" ;
    skos:inScheme <http://id.acdh.oeaw.ac.at/defc/thesaurus/FindsSchema>,
        <http://id.acdh.oeaw.ac.at/defc/thesaurus/FindsSmallFindsType> ;
    skos:prefLabel "Keulenkopf"@de,
        "mace head"@en .

<http://id.acdh.oeaw.ac.at/defc/thesaurus/malachite/3.35> a skos:Concept ;
    dc:source "http://dbpedia.org/page/Malachite" ;
    skos:broader <http://id.acdh.oeaw.ac.at/defc/thesaurus/mineral/2.3> ;
    skos:definition "Malachite is a copper carbonate hydroxide mineral, with the formula Cu2CO3(OH)2." ;
    skos:editorialNote "dc_finds_material;35" ;
    skos:inScheme <http://id.acdh.oeaw.ac.at/defc/thesaurus/FindsMaterial>,
        <http://id.acdh.oeaw.ac.at/defc/thesaurus/FindsSchema> ;
    skos:prefLabel "Malachit"@de,
        "malachite"@en .

<http://id.acdh.oeaw.ac.at/defc/thesaurus/male_individuals/6.1> a skos:Concept ;
    dc:source "http://dbpedia.org/page/Male" ;
    skos:broader <http://id.acdh.oeaw.ac.at/defc/thesaurus/sex/5.095> ;
    skos:editorialNote "dc_area_sexes;1" ;
    skos:inScheme <http://id.acdh.oeaw.ac.at/defc/thesaurus/AreaSchema>,
        <http://id.acdh.oeaw.ac.at/defc/thesaurus/AreaSexes> ;
    skos:prefLabel "mänlich"@de,
        "male individuals"@en .

<http://id.acdh.oeaw.ac.at/defc/thesaurus/mallard_duck/6.33> a skos:Concept ;
    dc:source "http://eol.org/pages/1047918/overview" ;
    skos:altLabel "Ente"@de,
        "duck"@en ;
    skos:broader <http://id.acdh.oeaw.ac.at/defc/thesaurus/duck/5.038> ;
    skos:editorialNote "dc_finds_animal_remains_species;33" ;
    skos:inScheme <http://id.acdh.oeaw.ac.at/defc/thesaurus/FindsAnimalRemainsSpecies>,
        <http://id.acdh.oeaw.ac.at/defc/thesaurus/FindsSchema> ;
    skos:prefLabel "Stockente"@de,
        "mallard duck"@en,
        "Anas platyrhynchos"@la .

<http://id.acdh.oeaw.ac.at/defc/thesaurus/manger/5.35> a skos:Concept ;
    dc:source "https://en.oxforddictionaries.com/definition/manger" ;
    skos:altLabel "Krippe"@de ;
    skos:broader <http://id.acdh.oeaw.ac.at/defc/thesaurus/installation/4.078> ;
    skos:definition "A long trough from which horses or cattle feed." ;
    skos:editorialNote "dc_area_specialfeatures;35" ;
    skos:inScheme <http://id.acdh.oeaw.ac.at/defc/thesaurus/AreaSchema>,
        <http://id.acdh.oeaw.ac.at/defc/thesaurus/AreaSpecialfeatures> ;
    skos:prefLabel "manger"@en .

<http://id.acdh.oeaw.ac.at/defc/thesaurus/marble/3.10> a skos:Concept ;
    dc:source "http://dbpedia.org/page/Marble" ;
    skos:broader <http://id.acdh.oeaw.ac.at/defc/thesaurus/stone/2.1> ;
    skos:definition "Marble is a non-foliated metamorphic rock composed of recrystallized carbonate minerals, most commonly calcite or dolomite." ;
    skos:editorialNote "dc_finds_material;10" ;
    skos:inScheme <http://id.acdh.oeaw.ac.at/defc/thesaurus/FindsMaterial>,
        <http://id.acdh.oeaw.ac.at/defc/thesaurus/FindsSchema> ;
    skos:prefLabel "Marmor"@de,
        "marble"@en .

<http://id.acdh.oeaw.ac.at/defc/thesaurus/mat-impressed/5.129> a skos:Concept ;
    dc:source "OREA" ;
    skos:broader <http://id.acdh.oeaw.ac.at/defc/thesaurus/incised/4.168> ;
    skos:definition "Pottery decorated by impressing of mat into the surface." ;
    skos:editorialNote "dc_finds_pottery_decoration;129" ;
    skos:inScheme <http://id.acdh.oeaw.ac.at/defc/thesaurus/FindsPotteryDecoration>,
        <http://id.acdh.oeaw.ac.at/defc/thesaurus/FindsSchema> ;
    skos:prefLabel "Mattenabdrücke"@de,
        "mat-impressed"@en .

<http://id.acdh.oeaw.ac.at/defc/thesaurus/material_culture/4.3> a skos:Concept ;
    dc:source "http://oxfordindex.oup.com/view/10.1093/obo/9780199766567-0085" ;
    skos:broader <http://id.acdh.oeaw.ac.at/defc/thesaurus/dating_method/3.045> ;
    skos:definition "The study of material culture centers upon objects, their properties, and the materials that they are made of, and the ways in which these material facets are central to an understanding of culture and social relations." ;
    skos:editorialNote "dc_period_datingmethod;3" ;
    skos:inScheme <http://id.acdh.oeaw.ac.at/defc/thesaurus/PeriodSchema> ;
    skos:prefLabel "materielle Kultur"@de,
        "material culture"@en .

<http://id.acdh.oeaw.ac.at/defc/thesaurus/matt_brown_on_white/6.199> a skos:Concept ;
    dc:source "OREA" ;
    skos:broader <http://id.acdh.oeaw.ac.at/defc/thesaurus/pattern_painted/5.041> ;
    skos:definition "Pottery decorated with matt brown paint on white ground." ;
    skos:editorialNote "dc_finds_pottery_decoration;199" ;
    skos:inScheme <http://id.acdh.oeaw.ac.at/defc/thesaurus/FindsPotteryDecoration>,
        <http://id.acdh.oeaw.ac.at/defc/thesaurus/FindsSchema> ;
    skos:prefLabel "Matt bemalt, braun auf weiß"@de,
        "matt brown on white"@en .

<http://id.acdh.oeaw.ac.at/defc/thesaurus/matt_painted/6.169> a skos:Concept ;
    dc:source "Kipfer, B. A. Dictionary of Artifacts 2007. Blackwell Publishing, Oxford.p. 191" ;
    skos:altLabel "Matt-painted"@en ;
    skos:broader <http://id.acdh.oeaw.ac.at/defc/thesaurus/pattern_painted/5.041> ;
    skos:definition "Pottery with simple decoration in manganese-based purple-black paint on a pale ground. Matt-painted pottery has been found in the nearer islands to mainland Greece and even as far as Crete and the Anatolian coast." ;
    skos:editorialNote "dc_finds_pottery_decoration;169" ;
    skos:inScheme <http://id.acdh.oeaw.ac.at/defc/thesaurus/FindsPotteryDecoration>,
        <http://id.acdh.oeaw.ac.at/defc/thesaurus/FindsSchema> ;
    skos:prefLabel "Matt bemalt"@de,
        "matt painted"@en .

<http://id.acdh.oeaw.ac.at/defc/thesaurus/mature-senile_(51-70)/6.8> a skos:Concept ;
    skos:broader <http://id.acdh.oeaw.ac.at/defc/thesaurus/age_group/5.097> ;
    skos:editorialNote "dc_area_agegroups;8" ;
    skos:inScheme <http://id.acdh.oeaw.ac.at/defc/thesaurus/AreaAgegroups>,
        <http://id.acdh.oeaw.ac.at/defc/thesaurus/AreaSchema> ;
    skos:prefLabel "mature-senile (51-70)"@en .

<http://id.acdh.oeaw.ac.at/defc/thesaurus/mature_(41-60)/6.7> a skos:Concept ;
    skos:broader <http://id.acdh.oeaw.ac.at/defc/thesaurus/age_group/5.097> ;
    skos:editorialNote "dc_area_agegroups;7" ;
    skos:inScheme <http://id.acdh.oeaw.ac.at/defc/thesaurus/AreaAgegroups>,
        <http://id.acdh.oeaw.ac.at/defc/thesaurus/AreaSchema> ;
    skos:prefLabel "mature (41-60)"@en .

<http://id.acdh.oeaw.ac.at/defc/thesaurus/megaron/5.2> a skos:Concept ;
    dc:source "OREA (M. Brami)" ;
    skos:broader <http://id.acdh.oeaw.ac.at/defc/thesaurus/building_type/4.077> ;
    skos:definition "A three-roomed building with a central axis." ;
    skos:editorialNote "dc_area_constructiontype;2" ;
    skos:inScheme <http://id.acdh.oeaw.ac.at/defc/thesaurus/AreaConstructiontype>,
        <http://id.acdh.oeaw.ac.at/defc/thesaurus/AreaSchema> ;
    skos:prefLabel "megaron"@en .

<http://id.acdh.oeaw.ac.at/defc/thesaurus/metal_detecting_survey/5.20> a skos:Concept ;
    dc:source "http://thesaurus.historicengland.org.uk/thesaurus_term.asp?thes_no=566&term_no=145147" ;
    skos:altLabel "metal detection"@en ;
    skos:broader <http://id.acdh.oeaw.ac.at/defc/thesaurus/geophysical_survey/4.054> ;
    skos:definition "Structured and carefully executed scanning of the ground surface with a metal detecting device in order to recover surface scatters of metal objects and plot them spatially within the study area as part of an archaeological survey or metal detecting rally" ;
    skos:editorialNote "dc_researchevet_researchtype;20" ;
    skos:inScheme <http://id.acdh.oeaw.ac.at/defc/thesaurus/ResearchEventSchema>,
        <http://id.acdh.oeaw.ac.at/defc/thesaurus/ResearchevetResearchtype> ;
    skos:prefLabel "Feldbegehung mit Metalldetektor"@de,
        "metal detecting survey"@en .

<http://id.acdh.oeaw.ac.at/defc/thesaurus/metal_detecting_use/3.7> a skos:Concept ;
    dc:source "http://thesaurus.historicengland.org.uk/thesaurus_term.asp?thes_no=566&term_no=145148" ;
    skos:altLabel "metal detection"@en ;
    skos:broader <http://id.acdh.oeaw.ac.at/defc/thesaurus/intrusive/2.048> ;
    skos:definition "The hobby of using a metal detector to hunt for buried coins or artefacts; alternatively the use of a metal detector to locate metal artefacts on an archaeological excavation that otherwise would go unnoticed." ;
    skos:editorialNote "dc_researchevet_researchtype;7" ;
    skos:inScheme <http://id.acdh.oeaw.ac.at/defc/thesaurus/ResearchEventSchema>,
        <http://id.acdh.oeaw.ac.at/defc/thesaurus/ResearchevetResearchtype> ;
    skos:prefLabel "Metalldetektor Einsatz"@de,
        "metal detecting use"@en .

<http://id.acdh.oeaw.ac.at/defc/thesaurus/metal_production/2.2> a skos:Concept ;
    dc:source "OREA" ;
    skos:broader <http://id.acdh.oeaw.ac.at/defc/thesaurus/production/1.042> ;
    skos:definition "The activity of mining and removing valuable metals from an ore and refining extracted metals into a purer form or production of alloy" ;
    skos:editorialNote "dc_interpretation_productiontype;2" ;
    skos:inScheme <http://id.acdh.oeaw.ac.at/defc/thesaurus/InterpretationProductiontype>,
        <http://id.acdh.oeaw.ac.at/defc/thesaurus/InterpretationSchema> ;
    skos:prefLabel "Metallproduktion"@de,
        "metal production"@en .

<http://id.acdh.oeaw.ac.at/defc/thesaurus/metallurgy/2.21> a skos:Concept ;
    dc:source "https://en.oxforddictionaries.com/definition/metallurgy" ;
    skos:broader <http://id.acdh.oeaw.ac.at/defc/thesaurus/special_analysis/1.057> ;
    skos:definition "The branch of science and technology concerned with the properties of metals and their production and purification." ;
    skos:editorialNote "dc_researchevent_special_analysis/2.21" ;
    skos:inScheme <http://id.acdh.oeaw.ac.at/defc/thesaurus/ResearchEventSchema>,
        <http://id.acdh.oeaw.ac.at/defc/thesaurus/ResearcheventSpecialAnalysis> ;
    skos:prefLabel "Metallurgie"@de,
        "metallurgy"@en .

<http://id.acdh.oeaw.ac.at/defc/thesaurus/micro_end-scraper/4.13> a skos:Concept ;
    dc:source "Inizan, M.-L., M. Reduron-Ballinger, H. Roche, J. Tixier 1999, Technology and Terminology of Knapped Stone. Nanterre: CREP., D. Srejovic (ed) 1997, Arheološki Leksikon." ;
    skos:altLabel "micro end scraper"@en ;
    skos:broader <http://id.acdh.oeaw.ac.at/defc/thesaurus/retouched_tool/3.010> ;
    skos:definition "Every scraper with the length or width less than 25mm. According to the size, it can belong to the category of microliths." ;
    skos:editorialNote "dc_finds_lithics_retouched_tools;13" ;
    skos:inScheme <http://id.acdh.oeaw.ac.at/defc/thesaurus/FindsLithicsRetouchedTools>,
        <http://id.acdh.oeaw.ac.at/defc/thesaurus/FindsSchema> ;
    skos:prefLabel "Mikrokratzer"@de,
        "micro end-scraper"@en .

<http://id.acdh.oeaw.ac.at/defc/thesaurus/microblade/4.4> a skos:Concept ;
    skos:broader <http://id.acdh.oeaw.ac.at/defc/thesaurus/unretouched_tool/3.011> ;
    skos:editorialNote "dc_finds_lithics_unretouched_tools;4" ;
    skos:inScheme <http://id.acdh.oeaw.ac.at/defc/thesaurus/FindsLithicsUnretouchedTools>,
        <http://id.acdh.oeaw.ac.at/defc/thesaurus/FindsSchema> ;
    skos:prefLabel "microblade"@en .

<http://id.acdh.oeaw.ac.at/defc/thesaurus/microlithic_industry/5.3> a skos:Concept ;
    dc:source "Inizan, M.-L., M. Reduron-Ballinger, H. Roche, J. Tixier 1999, Technology and Terminology of Knapped Stone. Nanterre: CREP. p. 143." ;
    skos:broader <http://id.acdh.oeaw.ac.at/defc/thesaurus/lithics_industry/4.024> ;
    skos:definition "Human action applied to raw materials in order to transform them into microliths." ;
    skos:editorialNote "dc_finds_lithics_industry;3" ;
    skos:inScheme <http://id.acdh.oeaw.ac.at/defc/thesaurus/FindsLithicsIndustry>,
        <http://id.acdh.oeaw.ac.at/defc/thesaurus/FindsSchema> ;
    skos:prefLabel "microlithic industry"@en .

<http://id.acdh.oeaw.ac.at/defc/thesaurus/mine_shaft/4.2> a skos:Concept ;
    dc:source "http://thesaurus.historicengland.org.uk/pastscape_term.asp?thes_no=1&term_no=69348" ;
    skos:broader <http://id.acdh.oeaw.ac.at/defc/thesaurus/quarry_type/3.065> ;
    skos:definition "A vertical or inclined excavation giving access to an underground mine." ;
    skos:editorialNote "dc_area_explotationtype;2" ;
    skos:inScheme <http://id.acdh.oeaw.ac.at/defc/thesaurus/AreaExplotationtype>,
        <http://id.acdh.oeaw.ac.at/defc/thesaurus/AreaSchema> ;
    skos:prefLabel "Schlacht"@de,
        "mine shaft"@en .

<http://id.acdh.oeaw.ac.at/defc/thesaurus/mineralogy/2.22> a skos:Concept ;
    dc:source "https://en.oxforddictionaries.com/definition/mineralogy" ;
    skos:broader <http://id.acdh.oeaw.ac.at/defc/thesaurus/special_analysis/1.057> ;
    skos:definition "The scientific study of minerals." ;
    skos:editorialNote "dc_researchevent_special_analysis/2.22" ;
    skos:inScheme <http://id.acdh.oeaw.ac.at/defc/thesaurus/ResearchEventSchema>,
        <http://id.acdh.oeaw.ac.at/defc/thesaurus/ResearcheventSpecialAnalysis> ;
    skos:prefLabel "Mineralogie"@de,
        "mineralogy"@en .

<http://id.acdh.oeaw.ac.at/defc/thesaurus/miniature_strap_handle/6.147> a skos:Concept ;
    dc:source "OREA" ;
    skos:broader <http://id.acdh.oeaw.ac.at/defc/thesaurus/strap_handle/5.78> ;
    skos:definition "A very small strip of clay attached to the vessel body before firing." ;
    skos:editorialNote "dc_finds_pottery_detail;147" ;
    skos:inScheme <http://id.acdh.oeaw.ac.at/defc/thesaurus/FindsPotteryDetail>,
        <http://id.acdh.oeaw.ac.at/defc/thesaurus/FindsSchema> ;
    skos:prefLabel "Miniaturbandhenkel"@de,
        "miniature strap handle"@en .

<http://id.acdh.oeaw.ac.at/defc/thesaurus/molluscs/4.17> a skos:Concept ;
    dc:source "http://eol.org/pages/2195/overview" ;
    skos:altLabel "mollusca"@en ;
    skos:broader <http://id.acdh.oeaw.ac.at/defc/thesaurus/animal_remains_species/3.06> ;
    skos:editorialNote "dc_finds_animal_remains_species;17" ;
    skos:inScheme <http://id.acdh.oeaw.ac.at/defc/thesaurus/FindsAnimalRemainsSpecies>,
        <http://id.acdh.oeaw.ac.at/defc/thesaurus/FindsSchema> ;
    skos:prefLabel "Mollusken"@de,
        "molluscs"@en .

<http://id.acdh.oeaw.ac.at/defc/thesaurus/monochrome_black/6.245> a skos:Concept ;
    dc:source "OREA" ;
    skos:broader <http://id.acdh.oeaw.ac.at/defc/thesaurus/monochrome/5.265> ;
    skos:definition "Pottery painted with black paint on black ground." ;
    skos:editorialNote "dc_finds_pottery_decoration;245" ;
    skos:inScheme <http://id.acdh.oeaw.ac.at/defc/thesaurus/FindsPotteryDecoration>,
        <http://id.acdh.oeaw.ac.at/defc/thesaurus/FindsSchema> ;
    skos:prefLabel "Monochrom schwarz"@de,
        "monochrome black"@en .

<http://id.acdh.oeaw.ac.at/defc/thesaurus/monochrome_brown/6.130> a skos:Concept ;
    dc:source "OREA" ;
    skos:broader <http://id.acdh.oeaw.ac.at/defc/thesaurus/monochrome/5.265> ;
    skos:definition "Pottery painted with brown paint on brown ground." ;
    skos:editorialNote "dc_finds_pottery_decoration;130" ;
    skos:inScheme <http://id.acdh.oeaw.ac.at/defc/thesaurus/FindsPotteryDecoration>,
        <http://id.acdh.oeaw.ac.at/defc/thesaurus/FindsSchema> ;
    skos:prefLabel "Monochrom braun"@de,
        "monochrome brown"@en .

<http://id.acdh.oeaw.ac.at/defc/thesaurus/monochrome_burnished/5.170> a skos:Concept ;
    dc:source "OREA" ;
    skos:broader <http://id.acdh.oeaw.ac.at/defc/thesaurus/burnished/4.297> ;
    skos:definition "Burnished pottery painted with one color." ;
    skos:editorialNote "dc_finds_pottery_decoration;170" ;
    skos:inScheme <http://id.acdh.oeaw.ac.at/defc/thesaurus/FindsPotteryDecoration>,
        <http://id.acdh.oeaw.ac.at/defc/thesaurus/FindsSchema> ;
    skos:prefLabel "Monochrom geglättet"@de,
        "monochrome burnished"@en .

<http://id.acdh.oeaw.ac.at/defc/thesaurus/monochrome_grey/6.294> a skos:Concept ;
    dc:source "OREA" ;
    skos:broader <http://id.acdh.oeaw.ac.at/defc/thesaurus/monochrome/5.265> ;
    skos:definition "Pottery painted with grey paint on grey ground." ;
    skos:editorialNote "dc_finds_pottery_decoration;294" ;
    skos:inScheme <http://id.acdh.oeaw.ac.at/defc/thesaurus/FindsPotteryDecoration>,
        <http://id.acdh.oeaw.ac.at/defc/thesaurus/FindsSchema> ;
    skos:prefLabel "monochrom grau"@de,
        "monochrome grey"@en .

<http://id.acdh.oeaw.ac.at/defc/thesaurus/monochrome_orange/6.200> a skos:Concept ;
    dc:source "OREA" ;
    skos:broader <http://id.acdh.oeaw.ac.at/defc/thesaurus/monochrome/5.265> ;
    skos:definition "Pottery painted with orange paint on orange ground." ;
    skos:editorialNote "dc_finds_pottery_decoration;200" ;
    skos:inScheme <http://id.acdh.oeaw.ac.at/defc/thesaurus/FindsPotteryDecoration>,
        <http://id.acdh.oeaw.ac.at/defc/thesaurus/FindsSchema> ;
    skos:prefLabel "monochrom orange"@de,
        "monochrome orange"@en .

<http://id.acdh.oeaw.ac.at/defc/thesaurus/monochrome_red/6.249> a skos:Concept ;
    dc:source "OREA" ;
    skos:broader <http://id.acdh.oeaw.ac.at/defc/thesaurus/monochrome/5.265> ;
    skos:definition "Pottery painted with red paint on red ground." ;
    skos:editorialNote "dc_finds_pottery_decoration;249" ;
    skos:inScheme <http://id.acdh.oeaw.ac.at/defc/thesaurus/FindsPotteryDecoration>,
        <http://id.acdh.oeaw.ac.at/defc/thesaurus/FindsSchema> ;
    skos:prefLabel "Monochrom rot"@de,
        "monochrome red"@en .

<http://id.acdh.oeaw.ac.at/defc/thesaurus/monochrome_red_(a1)/6.154> a skos:Concept ;
    dc:source "OREA" ;
    skos:broader <http://id.acdh.oeaw.ac.at/defc/thesaurus/monochrome/5.265> ;
    skos:definition "Pottery painted with one color without decoration." ;
    skos:editorialNote "dc_finds_pottery_decoration;154" ;
    skos:inScheme <http://id.acdh.oeaw.ac.at/defc/thesaurus/FindsPotteryDecoration>,
        <http://id.acdh.oeaw.ac.at/defc/thesaurus/FindsSchema> ;
    skos:prefLabel "Monochrom rot  (A1)"@de,
        "monochrome red (a1)"@en .

<http://id.acdh.oeaw.ac.at/defc/thesaurus/monochrome_undecorated_(b1)/6.155> a skos:Concept ;
    dc:source "Kipfer, B. A. Dictionary of Artifacts 2007. Blackwell Publishing, Oxford.p. 329" ;
    skos:broader <http://id.acdh.oeaw.ac.at/defc/thesaurus/monochrome/5.265> ;
    skos:definition "Pottery decorated with glaze-like paint. The pottery has a buff fabric decorated with a dark lustrous slip or glaze. The sauce boat and the askos are the most norable shapes." ;
    skos:editorialNote "dc_finds_pottery_decoration;155" ;
    skos:inScheme <http://id.acdh.oeaw.ac.at/defc/thesaurus/FindsPotteryDecoration>,
        <http://id.acdh.oeaw.ac.at/defc/thesaurus/FindsSchema> ;
    skos:prefLabel "Monochrom undekoriert (B1)"@de,
        "monochrome undecorated (b1)"@en .

<http://id.acdh.oeaw.ac.at/defc/thesaurus/monochrome_urfirnis/6.171> a skos:Concept ;
    dc:source "OREA" ;
    skos:broader <http://id.acdh.oeaw.ac.at/defc/thesaurus/monochrome/5.265> ;
    skos:definition "Pottery painted with white paint on white ground." ;
    skos:editorialNote "dc_finds_pottery_decoration;171" ;
    skos:inScheme <http://id.acdh.oeaw.ac.at/defc/thesaurus/FindsPotteryDecoration>,
        <http://id.acdh.oeaw.ac.at/defc/thesaurus/FindsSchema> ;
    skos:prefLabel "Monochromer Urfirnis"@de,
        "monochrome urfirnis"@en .

<http://id.acdh.oeaw.ac.at/defc/thesaurus/monochrome_white/6.301> a skos:Concept ;
    dc:source "OREA" ;
    skos:broader <http://id.acdh.oeaw.ac.at/defc/thesaurus/monochrome/5.265> ;
    skos:definition "Pottery painted with yellow paint on yellow ground." ;
    skos:editorialNote "dc_finds_pottery_decoration;301" ;
    skos:inScheme <http://id.acdh.oeaw.ac.at/defc/thesaurus/FindsPotteryDecoration>,
        <http://id.acdh.oeaw.ac.at/defc/thesaurus/FindsSchema> ;
    skos:prefLabel "monochrom weiß"@de,
        "monochrome white"@en .

<http://id.acdh.oeaw.ac.at/defc/thesaurus/monochrome_yellow/6.286> a skos:Concept ;
    dc:source "OREA" ;
    skos:broader <http://id.acdh.oeaw.ac.at/defc/thesaurus/monochrome/5.265> ;
    skos:definition "Orange ware made from well purified clay." ;
    skos:editorialNote "dc_finds_pottery_decoration;286" ;
    skos:inScheme <http://id.acdh.oeaw.ac.at/defc/thesaurus/FindsPotteryDecoration>,
        <http://id.acdh.oeaw.ac.at/defc/thesaurus/FindsSchema> ;
    skos:prefLabel "monochrom gelb"@de,
        "monochrome yellow"@en .

<http://id.acdh.oeaw.ac.at/defc/thesaurus/mortar/5.49> a skos:Concept ;
    dc:source "Kipfer, B. A. Dictionary of Artifacts 2007. Blackwell Publishing, Oxford.p.205." ;
    skos:broader <http://id.acdh.oeaw.ac.at/defc/thesaurus/grinding_equipment/4.029> ;
    skos:definition "Part of an ancient device for processing plant foods, usually used with a pestle. It was a stone or wooden receptacle with a cupshaped depression." ;
    skos:editorialNote "dc_finds_small_finds_type;49" ;
    skos:inScheme <http://id.acdh.oeaw.ac.at/defc/thesaurus/FindsSchema>,
        <http://id.acdh.oeaw.ac.at/defc/thesaurus/FindsSmallFindsType> ;
    skos:prefLabel "Mörser"@de,
        "mortar"@en .

<http://id.acdh.oeaw.ac.at/defc/thesaurus/mountain_top/2.6> a skos:Concept ;
    dc:source "https://en.oxforddictionaries.com/definition/mountaintop" ;
    skos:altLabel "summit"@en ;
    skos:broader "topography/1.099" ;
    skos:definition "The area at the top of a mountain."@en ;
    skos:editorialNote "dc_site_topography;6" ;
    skos:inScheme <http://id.acdh.oeaw.ac.at/defc/thesaurus/SiteSchema>,
        "SiteTopography" ;
    skos:prefLabel "Berggipfel"@de,
        "mountain top"@en .

<http://id.acdh.oeaw.ac.at/defc/thesaurus/mouse/5.20> a skos:Concept ;
    dc:source "http://eol.org/pages/8698/overview" ;
    skos:broader <http://id.acdh.oeaw.ac.at/defc/thesaurus/mammal/4.020> ;
    skos:editorialNote "dc_finds_animal_remains_species;20" ;
    skos:inScheme <http://id.acdh.oeaw.ac.at/defc/thesaurus/FindsAnimalRemainsSpecies>,
        <http://id.acdh.oeaw.ac.at/defc/thesaurus/FindsSchema> ;
    skos:prefLabel "Maus"@de,
        "mouse"@en,
        "Muridea"@la .

<http://id.acdh.oeaw.ac.at/defc/thesaurus/mud_brick/6.1> a skos:Concept ;
    dc:source "Kipfer, B. A. Encyclopedic Dictionary of Archaeology. Kluwer Academic/Plenum Publishers, New York. p. 372." ;
    skos:altLabel "adobe"@en ;
    skos:broader <http://id.acdh.oeaw.ac.at/defc/thesaurus/building_material/5.089> ;
    skos:definition "A brick dried in the sun rather than baked, used for construction in dry climates." ;
    skos:editorialNote "dc_area_buildingtechnique;1" ;
    skos:inScheme <http://id.acdh.oeaw.ac.at/defc/thesaurus/AreaBuildingtechnique>,
        <http://id.acdh.oeaw.ac.at/defc/thesaurus/AreaSchema> ;
    skos:prefLabel "Lehmziegel"@de,
        "mud brick"@en .

<http://id.acdh.oeaw.ac.at/defc/thesaurus/mug/4.113> a skos:Concept ;
    dc:source "OREA" ;
    skos:broader <http://id.acdh.oeaw.ac.at/defc/thesaurus/pottery_form/3.016> ;
    skos:definition "A small, narrow, deep, drinking vessel with straight sides." ;
    skos:editorialNote "dc_finds_pottery_form;113" ;
    skos:inScheme <http://id.acdh.oeaw.ac.at/defc/thesaurus/FindsPotteryForm>,
        <http://id.acdh.oeaw.ac.at/defc/thesaurus/FindsSchema> ;
    skos:prefLabel "Becher"@de,
        "mug"@en .

<http://id.acdh.oeaw.ac.at/defc/thesaurus/mushroom_handle/5.75> a skos:Concept ;
    dc:source "OREA" ;
    skos:altLabel "mushroom headed handle"@en ;
    skos:broader <http://id.acdh.oeaw.ac.at/defc/thesaurus/handle/4.031> ;
    skos:definition "A handle with an applied round object on a stem made of clay." ;
    skos:editorialNote "dc_finds_pottery_detail;75" ;
    skos:inScheme <http://id.acdh.oeaw.ac.at/defc/thesaurus/FindsPotteryDetail>,
        <http://id.acdh.oeaw.ac.at/defc/thesaurus/FindsSchema> ;
    skos:prefLabel "Henkel mit pilzförmigem Aufsatz"@de,
        "mushroom handle"@en .

<http://id.acdh.oeaw.ac.at/defc/thesaurus/narrow-mouthed_shallow_bowl/5.109> a skos:Concept ;
    dc:source "OREA" ;
    skos:broader <http://id.acdh.oeaw.ac.at/defc/thesaurus/bowl/4.115> ;
    skos:definition "A low open vessel with narrow mouth and with a rim diameter double than the height." ;
    skos:editorialNote "dc_finds_pottery_form;109" ;
    skos:inScheme <http://id.acdh.oeaw.ac.at/defc/thesaurus/FindsPotteryForm>,
        <http://id.acdh.oeaw.ac.at/defc/thesaurus/FindsSchema> ;
    skos:prefLabel "Engmundige Schale"@de,
        "narrow-mouthed shallow bowl"@en .

<http://id.acdh.oeaw.ac.at/defc/thesaurus/naviform_core/4.10> a skos:Concept ;
    dc:source "OREA" ;
    skos:broader <http://id.acdh.oeaw.ac.at/defc/thesaurus/core/3.12> ;
    skos:definition "A special type of bidirectional core (most common for the area of the Near East)." ;
    skos:editorialNote "dc_finds_lithics_core_shape;10" ;
    skos:inScheme <http://id.acdh.oeaw.ac.at/defc/thesaurus/FindsLithicsCoreShape>,
        <http://id.acdh.oeaw.ac.at/defc/thesaurus/FindsSchema> ;
    skos:prefLabel "naviform core"@en .

<http://id.acdh.oeaw.ac.at/defc/thesaurus/necklace/4.80> a skos:Concept ;
    dc:source "Kipfer, B. A. Dictionary of Artifacts 2007. Blackwell Publishing, Oxford.p.212" ;
    skos:broader <http://id.acdh.oeaw.ac.at/defc/thesaurus/jewellery/3.2> ;
    skos:definition "A chain, band, or cord, often ornamented with beads, pearls, jewels, etc., worn around the neck." ;
    skos:editorialNote "dc_finds_small_finds_type;80" ;
    skos:inScheme <http://id.acdh.oeaw.ac.at/defc/thesaurus/FindsSchema>,
        <http://id.acdh.oeaw.ac.at/defc/thesaurus/FindsSmallFindsType> ;
    skos:prefLabel "Halskette"@de,
        "necklace"@en .

<http://id.acdh.oeaw.ac.at/defc/thesaurus/needle/5.50> a skos:Concept ;
    skos:broader <http://id.acdh.oeaw.ac.at/defc/thesaurus/textile_equipment/4.028> ;
    skos:definition "A very thin pointed piece of metal or bone with a hole or eye for thread at the blunter end, used in sewing." ;
    skos:editorialNote "dc_finds_small_finds_type;50" ;
    skos:inScheme <http://id.acdh.oeaw.ac.at/defc/thesaurus/FindsSchema>,
        <http://id.acdh.oeaw.ac.at/defc/thesaurus/FindsSmallFindsType> ;
    skos:prefLabel "Nadel"@de,
        "needle"@en .

<http://id.acdh.oeaw.ac.at/defc/thesaurus/nemrik_point/6.117> a skos:Concept ;
    dc:source "Peregrine, P. N., Ember, M. (eds.) 2002. Encyclopedia of Prehistory. Vol. 8: Sourth and Southwest Asia. Kluwer Academic/Plenum Pulishers, New York, Boston, Dortrecht, London, Moscow." ;
    skos:broader <http://id.acdh.oeaw.ac.at/defc/thesaurus/projectile_point/5.70> ;
    skos:definition "A diamond-shaped point named after the Nemrik site in today Iraq." ;
    skos:editorialNote "dc_finds_small_finds_type;117" ;
    skos:inScheme <http://id.acdh.oeaw.ac.at/defc/thesaurus/FindsSchema>,
        <http://id.acdh.oeaw.ac.at/defc/thesaurus/FindsSmallFindsType> ;
    skos:prefLabel "nemrik point"@en .

<http://id.acdh.oeaw.ac.at/defc/thesaurus/neonate/6.1> a skos:Concept ;
    skos:broader <http://id.acdh.oeaw.ac.at/defc/thesaurus/age_group/5.097> ;
    skos:editorialNote "dc_area_agegroups;1" ;
    skos:inScheme <http://id.acdh.oeaw.ac.at/defc/thesaurus/AreaAgegroups>,
        <http://id.acdh.oeaw.ac.at/defc/thesaurus/AreaSchema> ;
    skos:prefLabel "neonate"@en .

<http://id.acdh.oeaw.ac.at/defc/thesaurus/net_sinker/5.51> a skos:Concept ;
    dc:source "Kipfer, B. A. Dictionary of Artifacts 2007. Blackwell Publishing, Oxford.p.214" ;
    skos:altLabel "Netzgewicht"@de,
        " sinker"@en,
        "net weight"@en ;
    skos:broader <http://id.acdh.oeaw.ac.at/defc/thesaurus/fishing_object/4.027> ;
    skos:definition "A term applied loosely to any perforated stone or terra cotta object that may have been used to keep a fishing net vertical in the water." ;
    skos:editorialNote "dc_finds_small_finds_type;51" ;
    skos:inScheme <http://id.acdh.oeaw.ac.at/defc/thesaurus/FindsSchema>,
        <http://id.acdh.oeaw.ac.at/defc/thesaurus/FindsSmallFindsType> ;
    skos:prefLabel "Netzsenker"@de,
        "net sinker"@en .

<http://id.acdh.oeaw.ac.at/defc/thesaurus/next_to_cave/5.4> a skos:Concept ;
    skos:broader <http://id.acdh.oeaw.ac.at/defc/thesaurus/grave_location/4.087> ;
    skos:editorialNote "dc_area_topography;4" ;
    skos:inScheme <http://id.acdh.oeaw.ac.at/defc/thesaurus/AreaSchema>,
        <http://id.acdh.oeaw.ac.at/defc/thesaurus/AreaTopography> ;
    skos:prefLabel "next to cave"@en .

<http://id.acdh.oeaw.ac.at/defc/thesaurus/niche/5.28> a skos:Concept ;
    dc:source "M. Brami, PhD after Catalhoyuk Research Project http://www.catalhoyuk.com/database/catal/help_glossary1.asp" ;
    skos:altLabel "Nische"@de ;
    skos:broader <http://id.acdh.oeaw.ac.at/defc/thesaurus/architecture/4.081> ;
    skos:definition "A alcove-like recess in a wall." ;
    skos:editorialNote "dc_area_specialfeatures;28" ;
    skos:inScheme <http://id.acdh.oeaw.ac.at/defc/thesaurus/AreaSchema>,
        <http://id.acdh.oeaw.ac.at/defc/thesaurus/AreaSpecialfeatures> ;
    skos:prefLabel "niche"@en .

<http://id.acdh.oeaw.ac.at/defc/thesaurus/none_recorded/4.4> a skos:Concept ;
    dc:source "OREA" ;
    skos:broader <http://id.acdh.oeaw.ac.at/defc/thesaurus/dating_method/3.045> ;
    skos:definition "The dating method of finds or the site has not been recorded in the documentation." ;
    skos:editorialNote "dc_period_datingmethod;4" ;
    skos:inScheme <http://id.acdh.oeaw.ac.at/defc/thesaurus/PeriodSchema> ;
    skos:prefLabel "none recorded"@en .

<http://id.acdh.oeaw.ac.at/defc/thesaurus/nose_ring/4.127> a skos:Concept ;
    dc:source "https://en.oxforddictionaries.com/definition/nose_ring" ;
    skos:broader <http://id.acdh.oeaw.ac.at/defc/thesaurus/jewellery/3.2> ;
    skos:definition "A ring worn in a person´s nose as a piece of jewellery." ;
    skos:editorialNote "dc_finds_small_finds_type;127" ;
    skos:inScheme <http://id.acdh.oeaw.ac.at/defc/thesaurus/FindsSchema>,
        <http://id.acdh.oeaw.ac.at/defc/thesaurus/FindsSmallFindsType> ;
    skos:prefLabel "Nasenring"@de,
        "nose ring"@en .

<http://id.acdh.oeaw.ac.at/defc/thesaurus/notch/4.14> a skos:Concept ;
    dc:source "Inizan, M.-L., M. Reduron-Ballinger, H. Roche, J. Tixier 1999, Technology and Terminology of Knapped Stone. Nanterre: CREP., D. Srejovic (ed) 1997, Arheološki Leksikon." ;
    skos:altLabel "notched tool"@en ;
    skos:broader <http://id.acdh.oeaw.ac.at/defc/thesaurus/retouched_tool/3.010> ;
    skos:definition "A term describing a tool with the delineation of an edge, indicating a sharp dent, generaly concave, sometimes V-shaped, with a small curvature radius, and created by carious retouch techniques." ;
    skos:editorialNote "dc_finds_lithics_retouched_tools;14" ;
    skos:inScheme <http://id.acdh.oeaw.ac.at/defc/thesaurus/FindsLithicsRetouchedTools>,
        <http://id.acdh.oeaw.ac.at/defc/thesaurus/FindsSchema> ;
    skos:prefLabel "Kerbe"@de,
        "notch"@en .

<http://id.acdh.oeaw.ac.at/defc/thesaurus/oat/5.37> a skos:Concept ;
    dc:source "http://dbpedia.org/page/Oat" ;
    skos:broader <http://id.acdh.oeaw.ac.at/defc/thesaurus/cereal/4.022> ;
    skos:editorialNote "dc_botany_species;37" ;
    skos:inScheme <http://id.acdh.oeaw.ac.at/defc/thesaurus/BotanySpecies>,
        <http://id.acdh.oeaw.ac.at/defc/thesaurus/FindsSchema> ;
    skos:prefLabel "Hafer"@de,
        "oat"@en,
        "Avana"@la .

<http://id.acdh.oeaw.ac.at/defc/thesaurus/obsidian/3.2> a skos:Concept ;
    dc:source "Encyclopaedia Britannica - https://www.britannica.com/science/obsidian" ;
    skos:broader <http://id.acdh.oeaw.ac.at/defc/thesaurus/stone/2.1> ;
    skos:definition "Obsidian, natural glass of volcanic origin that is formed by the rapid cooling of viscous lava. Obsidian is extremely rich in silica, low in water, and has a chemical composition similar to rhyolite." ;
    skos:editorialNote "dc_finds_material;2" ;
    skos:inScheme <http://id.acdh.oeaw.ac.at/defc/thesaurus/FindsMaterial>,
        <http://id.acdh.oeaw.ac.at/defc/thesaurus/FindsSchema> ;
    skos:prefLabel "Obsidian"@de,
        "obsidian"@en .

<http://id.acdh.oeaw.ac.at/defc/thesaurus/ochre/4.8> a skos:Concept ;
    dc:source "https://en.oxforddictionaries.com/definition/ochre" ;
    skos:broader <http://id.acdh.oeaw.ac.at/defc/thesaurus/raw_material/3.066> ;
    skos:definition "An earthy pigment containing ferric oxide, typically with clay, catying from light yellow to brown red.  Extracted from a quarry site." ;
    skos:editorialNote "dc_area_rawmaterial;8" ;
    skos:inScheme <http://id.acdh.oeaw.ac.at/defc/thesaurus/AreaRawmaterial>,
        <http://id.acdh.oeaw.ac.at/defc/thesaurus/AreaSchema> ;
    skos:prefLabel "Ocker"@de,
        "ochre"@en .

<http://id.acdh.oeaw.ac.at/defc/thesaurus/offset_rim/5.163> a skos:Concept ;
    dc:source "http://www.bible.ca/archeology/bible-archeology-pottery-glossary-dictionary-encyclopedia.htm" ;
    skos:broader <http://id.acdh.oeaw.ac.at/defc/thesaurus/rim/4.033> ;
    skos:definition "Offset rims are either in-set or out-set from the vessel wall, resulting in either an inverted or everted rim profile." ;
    skos:editorialNote "dc_finds_pottery_detail;163" ;
    skos:inScheme <http://id.acdh.oeaw.ac.at/defc/thesaurus/FindsPotteryDetail>,
        <http://id.acdh.oeaw.ac.at/defc/thesaurus/FindsSchema> ;
    skos:prefLabel "Abgesetzter Rand"@de,
        "offset rim"@en .

<http://id.acdh.oeaw.ac.at/defc/thesaurus/ogee-pot/4.195> a skos:Concept ;
    dc:source "OREA" ;
    skos:broader <http://id.acdh.oeaw.ac.at/defc/thesaurus/pottery_form/3.016> ;
    skos:editorialNote "dc_finds_pottery_form;195" ;
    skos:inScheme <http://id.acdh.oeaw.ac.at/defc/thesaurus/FindsPotteryForm>,
        <http://id.acdh.oeaw.ac.at/defc/thesaurus/FindsSchema> ;
    skos:prefLabel "ogee-pot"@en .

<http://id.acdh.oeaw.ac.at/defc/thesaurus/olive/4.26> a skos:Concept ;
    dc:source "http://dbpedia.org/page/Olive" ;
    skos:broader <http://id.acdh.oeaw.ac.at/defc/thesaurus/fruit/3.09> ;
    skos:editorialNote "dc_botany_species;26" ;
    skos:inScheme <http://id.acdh.oeaw.ac.at/defc/thesaurus/BotanySpecies>,
        <http://id.acdh.oeaw.ac.at/defc/thesaurus/FindsSchema> ;
    skos:prefLabel "Olive"@de,
        "olive"@en .

<http://id.acdh.oeaw.ac.at/defc/thesaurus/onager/5.39> a skos:Concept ;
    dc:source "http://eol.org/pages/311505/overview" ;
    skos:broader <http://id.acdh.oeaw.ac.at/defc/thesaurus/mammal/4.020> ;
    skos:editorialNote "dc_finds_animal_remains_species;39" ;
    skos:inScheme <http://id.acdh.oeaw.ac.at/defc/thesaurus/FindsAnimalRemainsSpecies>,
        <http://id.acdh.oeaw.ac.at/defc/thesaurus/FindsSchema> ;
    skos:prefLabel "onager"@en .

<http://id.acdh.oeaw.ac.at/defc/thesaurus/one-room/5.3> a skos:Concept ;
    dc:source "OREA" ;
    skos:altLabel "one room"@en ;
    skos:broader <http://id.acdh.oeaw.ac.at/defc/thesaurus/building_type/4.077> ;
    skos:definition "A building with one room." ;
    skos:editorialNote "dc_area_constructiontype;3" ;
    skos:inScheme <http://id.acdh.oeaw.ac.at/defc/thesaurus/AreaConstructiontype>,
        <http://id.acdh.oeaw.ac.at/defc/thesaurus/AreaSchema> ;
    skos:prefLabel "one-room"@en .

<http://id.acdh.oeaw.ac.at/defc/thesaurus/orange_fine_ware/6.259> a skos:Concept ;
    dc:source "OREA" ;
    skos:broader <http://id.acdh.oeaw.ac.at/defc/thesaurus/monochrome/5.265> ;
    skos:editorialNote "dc_finds_pottery_decoration;259" ;
    skos:inScheme <http://id.acdh.oeaw.ac.at/defc/thesaurus/FindsPotteryDecoration>,
        <http://id.acdh.oeaw.ac.at/defc/thesaurus/FindsSchema> ;
    skos:prefLabel "orange fein Ware"@de,
        "orange fine ware"@en .

<http://id.acdh.oeaw.ac.at/defc/thesaurus/ornament/4.124> a skos:Concept ;
    dc:source "https://en.oxforddictionaries.com/definition/ornament" ;
    skos:broader <http://id.acdh.oeaw.ac.at/defc/thesaurus/jewellery/3.2> ;
    skos:definition "A thing used or serving to make something look more attractive but usually having no practical purpose," ;
    skos:editorialNote "dc_finds_small_finds_type;124" ;
    skos:inScheme <http://id.acdh.oeaw.ac.at/defc/thesaurus/FindsSchema>,
        <http://id.acdh.oeaw.ac.at/defc/thesaurus/FindsSmallFindsType> ;
    skos:prefLabel "Ornament"@de,
        "ornament"@en .

<http://id.acdh.oeaw.ac.at/defc/thesaurus/other/4.108> a skos:Concept ;
    skos:broader <http://id.acdh.oeaw.ac.at/defc/thesaurus/jewellery/3.2> ;
    skos:editorialNote "dc_finds_small_finds_type;108" ;
    skos:inScheme <http://id.acdh.oeaw.ac.at/defc/thesaurus/FindsSchema>,
        <http://id.acdh.oeaw.ac.at/defc/thesaurus/FindsSmallFindsType> ;
    skos:prefLabel "other"@en .

<http://id.acdh.oeaw.ac.at/defc/thesaurus/other/4.109> a skos:Concept ;
    skos:broader <http://id.acdh.oeaw.ac.at/defc/thesaurus/tool/3.1> ;
    skos:editorialNote "dc_finds_small_finds_type;109" ;
    skos:inScheme <http://id.acdh.oeaw.ac.at/defc/thesaurus/FindsSchema>,
        <http://id.acdh.oeaw.ac.at/defc/thesaurus/FindsSmallFindsType> ;
    skos:prefLabel "other"@en .

<http://id.acdh.oeaw.ac.at/defc/thesaurus/other/4.99> a skos:Concept ;
    skos:broader <http://id.acdh.oeaw.ac.at/defc/thesaurus/figurine/3.3> ;
    skos:editorialNote "dc_finds_small_finds_type;99" ;
    skos:inScheme <http://id.acdh.oeaw.ac.at/defc/thesaurus/FindsSchema>,
        <http://id.acdh.oeaw.ac.at/defc/thesaurus/FindsSmallFindsType> ;
    skos:prefLabel "other"@en .

<http://id.acdh.oeaw.ac.at/defc/thesaurus/oven/5.11> a skos:Concept ;
    dc:source "M. Brami, PhD after Catalhoyuk Research Project http://www.catalhoyuk.com/database/catal/help_glossary1.asp" ;
    skos:altLabel "Ofen"@de ;
    skos:broader <http://id.acdh.oeaw.ac.at/defc/thesaurus/installation/4.078> ;
    skos:definition "A fire installation with a closed chamber." ;
    skos:editorialNote "dc_area_specialfeatures;11" ;
    skos:inScheme <http://id.acdh.oeaw.ac.at/defc/thesaurus/AreaSchema>,
        <http://id.acdh.oeaw.ac.at/defc/thesaurus/AreaSpecialfeatures> ;
    skos:prefLabel "oven"@en .

<http://id.acdh.oeaw.ac.at/defc/thesaurus/ovoid/5.3> a skos:Concept ;
    dc:source "OREA" ;
    skos:altLabel "oval"@en ;
    skos:broader <http://id.acdh.oeaw.ac.at/defc/thesaurus/building_shape/4.076> ;
    skos:definition "A building with a rounded, slightly enlongated ground plan." ;
    skos:editorialNote "dc_area_constructionshape;3" ;
    skos:inScheme <http://id.acdh.oeaw.ac.at/defc/thesaurus/AreaConstructionshape>,
        <http://id.acdh.oeaw.ac.at/defc/thesaurus/AreaSchema> ;
    skos:prefLabel "ovoid"@en .

<http://id.acdh.oeaw.ac.at/defc/thesaurus/part_of_house/5.5> a skos:Concept ;
    skos:broader <http://id.acdh.oeaw.ac.at/defc/thesaurus/grave_location/4.087> ;
    skos:editorialNote "dc_area_topography;5" ;
    skos:inScheme <http://id.acdh.oeaw.ac.at/defc/thesaurus/AreaSchema>,
        <http://id.acdh.oeaw.ac.at/defc/thesaurus/AreaTopography> ;
    skos:prefLabel "part of house"@en .

<http://id.acdh.oeaw.ac.at/defc/thesaurus/part_of_specialist_report/6.11> a skos:Concept ;
    dc:source "OREA" ;
    skos:broader <http://id.acdh.oeaw.ac.at/defc/thesaurus/age_group/5.097> ;
    skos:definition "The age of human remains has been noted in a specialist report." ;
    skos:editorialNote "dc_area_agegroups;11" ;
    skos:inScheme <http://id.acdh.oeaw.ac.at/defc/thesaurus/AreaAgegroups>,
        <http://id.acdh.oeaw.ac.at/defc/thesaurus/AreaSchema> ;
    skos:prefLabel "part of specialist report"@en .

<http://id.acdh.oeaw.ac.at/defc/thesaurus/part_of_specialist_report/6.4> a skos:Concept ;
    skos:broader <http://id.acdh.oeaw.ac.at/defc/thesaurus/sex/5.095> ;
    skos:editorialNote "dc_area_sexes;4" ;
    skos:inScheme <http://id.acdh.oeaw.ac.at/defc/thesaurus/AreaSchema>,
        <http://id.acdh.oeaw.ac.at/defc/thesaurus/AreaSexes> ;
    skos:prefLabel "part of specialist report"@en .

<http://id.acdh.oeaw.ac.at/defc/thesaurus/partirdge/5.34> a skos:Concept ;
    dc:source "http://dbpedia.org/page/Partridge" ;
    skos:broader <http://id.acdh.oeaw.ac.at/defc/thesaurus/bird/4.36> ;
    skos:editorialNote "dc_finds_animal_remains_species;34" ;
    skos:inScheme <http://id.acdh.oeaw.ac.at/defc/thesaurus/FindsAnimalRemainsSpecies>,
        <http://id.acdh.oeaw.ac.at/defc/thesaurus/FindsSchema> ;
    skos:prefLabel "Rebhuhn"@de,
        "partirdge"@en .

<http://id.acdh.oeaw.ac.at/defc/thesaurus/pattern_burnished/5.131> a skos:Concept ;
    dc:source "OREA" ;
    skos:broader <http://id.acdh.oeaw.ac.at/defc/thesaurus/burnished/4.297> ;
    skos:definition "Pottery decorated by burnished patterns." ;
    skos:editorialNote "dc_finds_pottery_decoration;131" ;
    skos:inScheme <http://id.acdh.oeaw.ac.at/defc/thesaurus/FindsPotteryDecoration>,
        <http://id.acdh.oeaw.ac.at/defc/thesaurus/FindsSchema> ;
    skos:prefLabel "Politurmusterverziert"@de,
        "pattern burnished"@en .

<http://id.acdh.oeaw.ac.at/defc/thesaurus/pattern_jabbed/5.223> a skos:Concept ;
    dc:source "OREA" ;
    skos:broader <http://id.acdh.oeaw.ac.at/defc/thesaurus/incised/4.168> ;
    skos:definition "Pottery decorated by poking the clay with a pointed object." ;
    skos:editorialNote "dc_finds_pottery_decoration;223" ;
    skos:inScheme <http://id.acdh.oeaw.ac.at/defc/thesaurus/FindsPotteryDecoration>,
        <http://id.acdh.oeaw.ac.at/defc/thesaurus/FindsSchema> ;
    skos:prefLabel "Eingedrückter Musterdekor"@de,
        "pattern jabbed"@en .

<http://id.acdh.oeaw.ac.at/defc/thesaurus/patterned_urfirnis/4.173> a skos:Concept ;
    dc:source "OREA" ;
    skos:broader <http://id.acdh.oeaw.ac.at/defc/thesaurus/pottery_surface_treatment/3.019> ;
    skos:definition "Pattern painted decoration with loustrous paint." ;
    skos:editorialNote "dc_finds_pottery_decoration;173" ;
    skos:inScheme <http://id.acdh.oeaw.ac.at/defc/thesaurus/FindsPotteryDecoration>,
        <http://id.acdh.oeaw.ac.at/defc/thesaurus/FindsSchema> ;
    skos:prefLabel "Musterverzierter Urfirnis"@de,
        "patterned urfirnis"@en .

<http://id.acdh.oeaw.ac.at/defc/thesaurus/paved_area/5.13> a skos:Concept ;
    dc:source "https://standards.phorio.com/?t=definition&code=7120921898" ;
    skos:altLabel "paved road"@en,
        "paved way"@en ;
    skos:broader <http://id.acdh.oeaw.ac.at/defc/thesaurus/architecture/4.081> ;
    skos:definition "A distinct piece of land with a continuous surface or a network of surfaces formed artificially, either using man-made materials or constructed out of stable, non-planted natural materials like gravel." ;
    skos:editorialNote "dc_area_specialfeatures;13" ;
    skos:inScheme <http://id.acdh.oeaw.ac.at/defc/thesaurus/AreaSchema>,
        <http://id.acdh.oeaw.ac.at/defc/thesaurus/AreaSpecialfeatures> ;
    skos:prefLabel "paved area"@en .

<http://id.acdh.oeaw.ac.at/defc/thesaurus/pavement/5.2> a skos:Concept ;
    dc:source "http://triggs.djvu.org/century-dictionary.com/djvu2jpgframes.php?volno=05&page=779&query=pavement" ;
    skos:broader <http://id.acdh.oeaw.ac.at/defc/thesaurus/building_technique/4.075> ;
    skos:definition "A floor of surface-covering of flags, stones, tiles, or bricks accurately fitted in masonry with or without a bond material." ;
    skos:editorialNote "dc_area_buildingtechnique;2" ;
    skos:inScheme <http://id.acdh.oeaw.ac.at/defc/thesaurus/AreaBuildingtechnique>,
        <http://id.acdh.oeaw.ac.at/defc/thesaurus/AreaSchema> ;
    skos:prefLabel "Pflasterung"@de,
        "pavement"@en .

<http://id.acdh.oeaw.ac.at/defc/thesaurus/peach/4.15> a skos:Concept ;
    dc:source "http://eol.org/pages/631649/overview" ;
    skos:broader <http://id.acdh.oeaw.ac.at/defc/thesaurus/fruit/3.09> ;
    skos:editorialNote "dc_botany_species;15" ;
    skos:inScheme <http://id.acdh.oeaw.ac.at/defc/thesaurus/BotanySpecies>,
        <http://id.acdh.oeaw.ac.at/defc/thesaurus/FindsSchema> ;
    skos:prefLabel "Pfirsich"@de,
        "peach"@en,
        "Persica vulgaris"@la .

<http://id.acdh.oeaw.ac.at/defc/thesaurus/pear/4.42> a skos:Concept ;
    dc:source "http://eol.org/pages/29920/overview" ;
    skos:broader <http://id.acdh.oeaw.ac.at/defc/thesaurus/fruit/3.09> ;
    skos:editorialNote "dc_botany_species;42" ;
    skos:inScheme <http://id.acdh.oeaw.ac.at/defc/thesaurus/BotanySpecies>,
        <http://id.acdh.oeaw.ac.at/defc/thesaurus/FindsSchema> ;
    skos:prefLabel "Birne"@de,
        "pear"@en,
        "Pyrus"@la .

<http://id.acdh.oeaw.ac.at/defc/thesaurus/pedestal/5.137> a skos:Concept ;
    dc:source "OREA" ;
    skos:broader <http://id.acdh.oeaw.ac.at/defc/thesaurus/foot/4.71> ;
    skos:editorialNote "dc_finds_pottery_detail;137" ;
    skos:inScheme <http://id.acdh.oeaw.ac.at/defc/thesaurus/FindsPotteryDetail>,
        <http://id.acdh.oeaw.ac.at/defc/thesaurus/FindsSchema> ;
    skos:prefLabel "Sockel"@de,
        "pedestal"@en .

<http://id.acdh.oeaw.ac.at/defc/thesaurus/pedestal/5.164> a skos:Concept ;
    dc:source "OREA" ;
    skos:broader <http://id.acdh.oeaw.ac.at/defc/thesaurus/foot/4.71> ;
    skos:editorialNote "dc_finds_pottery_detail;164" ;
    skos:inScheme <http://id.acdh.oeaw.ac.at/defc/thesaurus/FindsPotteryDetail>,
        <http://id.acdh.oeaw.ac.at/defc/thesaurus/FindsSchema> ;
    skos:prefLabel "Sockel"@de,
        "pedestal"@en .

<http://id.acdh.oeaw.ac.at/defc/thesaurus/pedestal_base/5.76> a skos:Concept ;
    dc:source "OREA" ;
    skos:altLabel "Sockel"@de,
        "Pedestal"@en ;
    skos:broader <http://id.acdh.oeaw.ac.at/defc/thesaurus/foot/4.71> ;
    skos:editorialNote "dc_finds_pottery_detail;76" ;
    skos:inScheme <http://id.acdh.oeaw.ac.at/defc/thesaurus/FindsPotteryDetail>,
        <http://id.acdh.oeaw.ac.at/defc/thesaurus/FindsSchema> ;
    skos:prefLabel "Standfuß"@de,
        "pedestal base"@en .

<http://id.acdh.oeaw.ac.at/defc/thesaurus/pendant/4.76> a skos:Concept ;
    dc:source "Kipfer, B. A. Dictionary of Artifacts 2007. Blackwell Publishing, Oxford.p.236" ;
    skos:broader <http://id.acdh.oeaw.ac.at/defc/thesaurus/jewellery/3.2> ;
    skos:definition "An adronment that hangs from a piece of jewelry (necklace or earring)." ;
    skos:editorialNote "dc_finds_small_finds_type;76" ;
    skos:inScheme <http://id.acdh.oeaw.ac.at/defc/thesaurus/FindsSchema>,
        <http://id.acdh.oeaw.ac.at/defc/thesaurus/FindsSmallFindsType> ;
    skos:prefLabel "Anhänger"@de,
        "pendant"@en .

<http://id.acdh.oeaw.ac.at/defc/thesaurus/pestle/5.60> a skos:Concept ;
    dc:source "Kipfer, B. A. Dictionary of Artifacts 2007. Blackwell Publishing, Oxford.p.237" ;
    skos:broader <http://id.acdh.oeaw.ac.at/defc/thesaurus/grinding_equipment/4.029> ;
    skos:definition "Club-shaped (oblong cylindrical or subcylindrical) implement of stone used for pounding, crushing, or grinding substances in a mortar." ;
    skos:editorialNote "dc_finds_small_finds_type;60" ;
    skos:inScheme <http://id.acdh.oeaw.ac.at/defc/thesaurus/FindsSchema>,
        <http://id.acdh.oeaw.ac.at/defc/thesaurus/FindsSmallFindsType> ;
    skos:prefLabel "Stößel"@de,
        "pestle"@en .

<http://id.acdh.oeaw.ac.at/defc/thesaurus/petrological_research/3.25> a skos:Concept ;
    dc:source "https://en.oxforddictionaries.com/definition/petrology" ;
    skos:altLabel "Petrologie"@de,
        "petrology"@en ;
    skos:broader <http://id.acdh.oeaw.ac.at/defc/thesaurus/non-intrusive/2.051> ;
    skos:definition "The study concerned with the origin, structure, and composition of rocks." ;
    skos:editorialNote "dc_researchevet_researchtype;25" ;
    skos:inScheme <http://id.acdh.oeaw.ac.at/defc/thesaurus/ResearchEventSchema>,
        <http://id.acdh.oeaw.ac.at/defc/thesaurus/ResearchevetResearchtype> ;
    skos:prefLabel "petrologische Auswertung"@de,
        "petrological research"@en .

<http://id.acdh.oeaw.ac.at/defc/thesaurus/phallus/6.89> a skos:Concept ;
    dc:source "Kipfer, B. A. Dictionary of Artifacts 2007. Blackwell Publishing, Oxford.p.113" ;
    skos:broader <http://id.acdh.oeaw.ac.at/defc/thesaurus/male_figurine/5.85> ;
    skos:definition "A small carved or sculpted figure of a phallus, usually of clay, stone, wood, or metal." ;
    skos:editorialNote "dc_finds_small_finds_type;89" ;
    skos:inScheme <http://id.acdh.oeaw.ac.at/defc/thesaurus/FindsSchema>,
        <http://id.acdh.oeaw.ac.at/defc/thesaurus/FindsSmallFindsType> ;
    skos:prefLabel "Phallus"@de,
        "phallus"@en .

<http://id.acdh.oeaw.ac.at/defc/thesaurus/pickaxe/4.132> a skos:Concept ;
    dc:source "Kipfer, B. A. Dictionary of Artifacts 2007. Blackwell Publishing, Oxford.p. 240" ;
    skos:altLabel "Pickel"@de,
        "pickax"@en ;
    skos:broader <http://id.acdh.oeaw.ac.at/defc/thesaurus/tool/3.1> ;
    skos:definition "A pick with a point at one end and a cutting blade at the other end." ;
    skos:editorialNote "dc_finds_small_finds_type;132" ;
    skos:inScheme <http://id.acdh.oeaw.ac.at/defc/thesaurus/FindsSchema>,
        <http://id.acdh.oeaw.ac.at/defc/thesaurus/FindsSmallFindsType> ;
    skos:prefLabel "Spitzhacke"@de,
        "pickaxe"@en .

<http://id.acdh.oeaw.ac.at/defc/thesaurus/pig/5.2> a skos:Concept ;
    dc:source "http://eol.org/pages/4445650/overview" ;
    skos:broader <http://id.acdh.oeaw.ac.at/defc/thesaurus/mammal/4.020> ;
    skos:editorialNote "dc_finds_animal_remains_species;2" ;
    skos:inScheme <http://id.acdh.oeaw.ac.at/defc/thesaurus/FindsAnimalRemainsSpecies>,
        <http://id.acdh.oeaw.ac.at/defc/thesaurus/FindsSchema> ;
    skos:prefLabel "Schwein"@de,
        "pig"@en,
        "Sus scrofa domesticus"@la .

<http://id.acdh.oeaw.ac.at/defc/thesaurus/pile_dwelling/5.4> a skos:Concept ;
    dc:source "Kipfer, B. A. Encyclopedic Dictionary of Archaeology. Kluwer Academic/Plenum Publishers, New York. p. 440." ;
    skos:broader <http://id.acdh.oeaw.ac.at/defc/thesaurus/building_type/4.077> ;
    skos:definition "A building with platforms raised on posts above open water or on damp ground at water´s edge." ;
    skos:editorialNote "dc_area_constructiontype;4" ;
    skos:inScheme <http://id.acdh.oeaw.ac.at/defc/thesaurus/AreaConstructiontype>,
        <http://id.acdh.oeaw.ac.at/defc/thesaurus/AreaSchema> ;
    skos:prefLabel "pile dwelling"@en .

<http://id.acdh.oeaw.ac.at/defc/thesaurus/pin/4.128> a skos:Concept ;
    dc:source "Kipfer, B. A. Dictionary of Artifacts 2007. Blackwell Publishing, Oxford.p. 241" ;
    skos:broader <http://id.acdh.oeaw.ac.at/defc/thesaurus/jewellery/3.2> ;
    skos:definition "One of the simplest artifacts, consisting of a narrow metal or bone shaft with a point at one end and usually some sort of decorative head at the other. Ist function was to secure garments (ancestral to the fibula), or, sometimes, the hair." ;
    skos:editorialNote "dc_finds_small_finds_type;128" ;
    skos:inScheme <http://id.acdh.oeaw.ac.at/defc/thesaurus/FindsSchema>,
        <http://id.acdh.oeaw.ac.at/defc/thesaurus/FindsSmallFindsType> ;
    skos:prefLabel "Nadel"@de,
        "pin"@en .

<http://id.acdh.oeaw.ac.at/defc/thesaurus/pine/3.44> a skos:Concept ;
    dc:source "http://eol.org/pages/999491/overview" ;
    skos:broader <http://id.acdh.oeaw.ac.at/defc/thesaurus/botany/2.2> ;
    skos:editorialNote "dc_botany_species;44" ;
    skos:inScheme <http://id.acdh.oeaw.ac.at/defc/thesaurus/BotanySpecies>,
        <http://id.acdh.oeaw.ac.at/defc/thesaurus/FindsSchema> ;
    skos:prefLabel "Kiefer"@de,
        "pine"@en,
        "Pinus pinea"@la .

<http://id.acdh.oeaw.ac.at/defc/thesaurus/pinge/4.1> a skos:Concept ;
    dc:source "https://en.wikipedia.org/wiki/Pinge" ;
    skos:broader <http://id.acdh.oeaw.ac.at/defc/thesaurus/quarry_type/3.065> ;
    skos:definition "A wedge-, ditch- or funnel-shaped depression in the terrain caused by mining activity. This depression or sink-hole is frequently caused by the collapse of old underground mine workings that are close to the Earth's surface." ;
    skos:editorialNote "dc_area_explotationtype;1" ;
    skos:inScheme <http://id.acdh.oeaw.ac.at/defc/thesaurus/AreaExplotationtype>,
        <http://id.acdh.oeaw.ac.at/defc/thesaurus/AreaSchema> ;
    skos:prefLabel "Pinge"@de,
        "pinge"@en .

<http://id.acdh.oeaw.ac.at/defc/thesaurus/pink_ware/6.273> a skos:Concept ;
    dc:source "OREA" ;
    skos:broader <http://id.acdh.oeaw.ac.at/defc/thesaurus/monochrome/5.265> ;
    skos:definition "Ware of pink color." ;
    skos:editorialNote "dc_finds_pottery_decoration;273" ;
    skos:inScheme <http://id.acdh.oeaw.ac.at/defc/thesaurus/FindsPotteryDecoration>,
        <http://id.acdh.oeaw.ac.at/defc/thesaurus/FindsSchema> ;
    skos:prefLabel "Rosa Ware"@de,
        "pink ware"@en .

<http://id.acdh.oeaw.ac.at/defc/thesaurus/pintadera/4.59> a skos:Concept ;
    dc:source "Kipfer, B. A. Dictionary of Artifacts 2007. Blackwell Publishing, Oxford.p.242" ;
    skos:altLabel "Stampel"@de,
        "stamp"@en ;
    skos:broader <http://id.acdh.oeaw.ac.at/defc/thesaurus/tool/3.1> ;
    skos:definition "A small object, usually of terra cotta, consisting of a decorative stamp with a knob at the back for holding. The stamping surface is flat, concave, or convex. It has been suggested that they served to apply pigments to the human skin in repeat patterns as an alternative to tattooing." ;
    skos:editorialNote "dc_finds_small_finds_type;59" ;
    skos:inScheme <http://id.acdh.oeaw.ac.at/defc/thesaurus/FindsSchema>,
        <http://id.acdh.oeaw.ac.at/defc/thesaurus/FindsSmallFindsType> ;
    skos:prefLabel "Pintadera"@de,
        "pintadera"@en .

<http://id.acdh.oeaw.ac.at/defc/thesaurus/piriform_jar/4.152> a skos:Concept ;
    dc:source "OREA" ;
    skos:broader <http://id.acdh.oeaw.ac.at/defc/thesaurus/pottery_form/3.016> ;
    skos:definition "A pear-shaped high and open vessel with a maximal diameter generally at the belly." ;
    skos:editorialNote "dc_finds_pottery_form;152" ;
    skos:inScheme <http://id.acdh.oeaw.ac.at/defc/thesaurus/FindsPotteryForm>,
        <http://id.acdh.oeaw.ac.at/defc/thesaurus/FindsSchema> ;
    skos:prefLabel "Birnenförmiger Topf"@de,
        "piriform jar"@en .

<http://id.acdh.oeaw.ac.at/defc/thesaurus/pistachio/5.28> a skos:Concept ;
    dc:source "http://eol.org/pages/50516/overview" ;
    skos:altLabel "Pistache"@de ;
    skos:broader <http://id.acdh.oeaw.ac.at/defc/thesaurus/nuts/4.31> ;
    skos:editorialNote "dc_botany_species;28" ;
    skos:inScheme <http://id.acdh.oeaw.ac.at/defc/thesaurus/BotanySpecies>,
        <http://id.acdh.oeaw.ac.at/defc/thesaurus/FindsSchema> ;
    skos:prefLabel "Pistazie"@de,
        "pistachio"@en,
        "Pistacia"@la .

<http://id.acdh.oeaw.ac.at/defc/thesaurus/pisé/6.3> a skos:Concept ;
    dc:source "Kipfer, B. A. Encyclopedic Dictionary of Archaeology. Kluwer Academic/Plenum Publishers, New York. p. 441." ;
    skos:broader <http://id.acdh.oeaw.ac.at/defc/thesaurus/building_material/5.089> ;
    skos:definition "A term describing a wall made of mud or clay, not formed into separate bricks but shaped, rammed, or piled up into walls in situ." ;
    skos:editorialNote "dc_area_buildingtechnique;3" ;
    skos:inScheme <http://id.acdh.oeaw.ac.at/defc/thesaurus/AreaBuildingtechnique>,
        <http://id.acdh.oeaw.ac.at/defc/thesaurus/AreaSchema> ;
    skos:prefLabel "Stampflehm"@de,
        "pisé"@en .

<http://id.acdh.oeaw.ac.at/defc/thesaurus/pit-house/5.5> a skos:Concept ;
    dc:source "OREA (M. Brami)" ;
    skos:altLabel "pit house"@en ;
    skos:broader <http://id.acdh.oeaw.ac.at/defc/thesaurus/building_type/4.077> ;
    skos:definition "A semi-subterranean structure with domestic features." ;
    skos:editorialNote "dc_area_constructiontype;5" ;
    skos:inScheme <http://id.acdh.oeaw.ac.at/defc/thesaurus/AreaConstructiontype>,
        <http://id.acdh.oeaw.ac.at/defc/thesaurus/AreaSchema> ;
    skos:prefLabel "pit-house"@en .

<http://id.acdh.oeaw.ac.at/defc/thesaurus/pit/5.4> a skos:Concept ;
    dc:source "http://thesaurus.historicengland.org.uk/thesaurus_term.asp?thes_no=1&term_no=70398" ;
    skos:altLabel "Grube"@de ;
    skos:broader <http://id.acdh.oeaw.ac.at/defc/thesaurus/installation/4.078> ;
    skos:definition "A hole or cavity in the ground, either natural or the result of human activity." ;
    skos:editorialNote "dc_area_specialfeatures;4" ;
    skos:inScheme <http://id.acdh.oeaw.ac.at/defc/thesaurus/AreaSchema>,
        <http://id.acdh.oeaw.ac.at/defc/thesaurus/AreaSpecialfeatures> ;
    skos:prefLabel "pit"@en .

<http://id.acdh.oeaw.ac.at/defc/thesaurus/pit/5.5> a skos:Concept ;
    dc:source "OREA" ;
    skos:broader <http://id.acdh.oeaw.ac.at/defc/thesaurus/occupation_evidence/4.088> ;
    skos:definition "A hole or cavity in the ground, either natural or the result of human activity." ;
    skos:editorialNote "dc_area_evidenceofocupation;5" ;
    skos:inScheme <http://id.acdh.oeaw.ac.at/defc/thesaurus/AreaEvidenceofocupation>,
        <http://id.acdh.oeaw.ac.at/defc/thesaurus/AreaSchema> ;
    skos:prefLabel "Grube"@de,
        "pit"@en .

<http://id.acdh.oeaw.ac.at/defc/thesaurus/pit_grave/5.2> a skos:Concept ;
    skos:broader <http://id.acdh.oeaw.ac.at/defc/thesaurus/grave_type/4.083> ;
    skos:editorialNote "dc_area_gravetype;2" ;
    skos:inScheme <http://id.acdh.oeaw.ac.at/defc/thesaurus/AreaGravetype>,
        <http://id.acdh.oeaw.ac.at/defc/thesaurus/AreaSchema> ;
    skos:prefLabel "Grubengrab"@de,
        "pit grave"@en .

<http://id.acdh.oeaw.ac.at/defc/thesaurus/pithos/4.135> a skos:Concept ;
    dc:source "Kipfer, B. A. Dictionary of Artifacts 2007. Blackwell Publishing, Oxford.p 243" ;
    skos:broader <http://id.acdh.oeaw.ac.at/defc/thesaurus/pottery_form/3.016> ;
    skos:definition "A large storage vessel with thick walls with a narrow neck. On occasion they were also used for jar burial in the Aegean area." ;
    skos:editorialNote "dc_finds_pottery_form;135" ;
    skos:inScheme <http://id.acdh.oeaw.ac.at/defc/thesaurus/FindsPotteryForm>,
        <http://id.acdh.oeaw.ac.at/defc/thesaurus/FindsSchema> ;
    skos:prefLabel "Pithos"@de,
        "pithos"@en .

<http://id.acdh.oeaw.ac.at/defc/thesaurus/pivot_stone/4.135> a skos:Concept ;
    skos:broader <http://id.acdh.oeaw.ac.at/defc/thesaurus/other/3.4> ;
    skos:editorialNote "dc_finds_small_finds_type;135" ;
    skos:inScheme <http://id.acdh.oeaw.ac.at/defc/thesaurus/FindsSchema>,
        <http://id.acdh.oeaw.ac.at/defc/thesaurus/FindsSmallFindsType> ;
    skos:prefLabel "Türangelstein"@de,
        "pivot stone"@en .

<http://id.acdh.oeaw.ac.at/defc/thesaurus/plain/2.7> a skos:Concept ;
    dc:source "https://en.oxforddictionaries.com/definition/plain" ;
    skos:broader "topography/1.099" ;
    skos:definition "A large area of flat land."@en ;
    skos:editorialNote "dc_site_topography;7" ;
    skos:inScheme <http://id.acdh.oeaw.ac.at/defc/thesaurus/SiteSchema>,
        "SiteTopography" ;
    skos:prefLabel "Flachland"@de,
        "plain"@en .

<http://id.acdh.oeaw.ac.at/defc/thesaurus/plaque/4.73> a skos:Concept ;
    dc:source "https://en.oxforddictionaries.com/definition/plaque" ;
    skos:broader <http://id.acdh.oeaw.ac.at/defc/thesaurus/other/3.4> ;
    skos:definition "An ornamental tablet, typically of metal or wood, that is fixed ro a wall or other surface in commemmoration." ;
    skos:editorialNote "dc_finds_small_finds_type;73" ;
    skos:inScheme <http://id.acdh.oeaw.ac.at/defc/thesaurus/FindsSchema>,
        <http://id.acdh.oeaw.ac.at/defc/thesaurus/FindsSmallFindsType> ;
    skos:prefLabel "Platte"@de,
        "plaque"@en .

<http://id.acdh.oeaw.ac.at/defc/thesaurus/plaster_wall/6.4> a skos:Concept ;
    dc:source "Kipfer, B. A. Dictionary of Artifacts 2007. Blackwell Publishing, Oxford.p. 252." ;
    skos:broader <http://id.acdh.oeaw.ac.at/defc/thesaurus/wall/5.090> ;
    skos:definition "A wall covered with a mixture of lime or gypsum, sand and water, which hardens into a smooth solid." ;
    skos:editorialNote "dc_area_buildingtechnique;4" ;
    skos:inScheme <http://id.acdh.oeaw.ac.at/defc/thesaurus/AreaBuildingtechnique>,
        <http://id.acdh.oeaw.ac.at/defc/thesaurus/AreaSchema> ;
    skos:prefLabel "Wandverputz"@de,
        "plaster wall"@en .

<http://id.acdh.oeaw.ac.at/defc/thesaurus/plastered_floor/6.25> a skos:Concept ;
    dc:source "OREA" ;
    skos:broader <http://id.acdh.oeaw.ac.at/defc/thesaurus/floor/5.094> ;
    skos:definition "A layer of plaster on which people tread." ;
    skos:editorialNote "dc_area_specialfeatures;25" ;
    skos:inScheme <http://id.acdh.oeaw.ac.at/defc/thesaurus/AreaSchema>,
        <http://id.acdh.oeaw.ac.at/defc/thesaurus/AreaSpecialfeatures> ;
    skos:prefLabel "plastered floor"@en .

<http://id.acdh.oeaw.ac.at/defc/thesaurus/plastered_threshold/5.9> a skos:Concept ;
    skos:broader <http://id.acdh.oeaw.ac.at/defc/thesaurus/building_technique/4.075> ;
    skos:definition "A strip of plaster forming the bottom of a doorway and crossed in entering a house or room." ;
    skos:editorialNote "dc_area_buildingtechnique;9" ;
    skos:inScheme <http://id.acdh.oeaw.ac.at/defc/thesaurus/AreaBuildingtechnique>,
        <http://id.acdh.oeaw.ac.at/defc/thesaurus/AreaSchema> ;
    skos:prefLabel "Schwelle aus Mörtel"@de,
        "plastered threshold"@en .

<http://id.acdh.oeaw.ac.at/defc/thesaurus/plastic_cordon_decoration/5.225> a skos:Concept ;
    dc:source "Kipfer, B. A. Dictionary of Artifacts 2007. Blackwell Publishing, Oxford.p 83" ;
    skos:broader <http://id.acdh.oeaw.ac.at/defc/thesaurus/plastic_decoration/4.132> ;
    skos:definition "Pottery with a strip of clay added around the outside surface of a pot before firing for decoration or handling. The cordon(s) may be decorated in some way, for example with fingertip or stick impressions." ;
    skos:editorialNote "dc_finds_pottery_decoration;225" ;
    skos:inScheme <http://id.acdh.oeaw.ac.at/defc/thesaurus/FindsPotteryDecoration>,
        <http://id.acdh.oeaw.ac.at/defc/thesaurus/FindsSchema> ;
    skos:prefLabel "Plastischer Banddekor"@de,
        "plastic cordon decoration"@en .

<http://id.acdh.oeaw.ac.at/defc/thesaurus/plate/4.165> a skos:Concept ;
    dc:source "OREA" ;
    skos:altLabel "Teller"@de ;
    skos:broader <http://id.acdh.oeaw.ac.at/defc/thesaurus/pottery_form/3.016> ;
    skos:definition "A very low or even flat vessel." ;
    skos:editorialNote "dc_finds_pottery_form;165" ;
    skos:inScheme <http://id.acdh.oeaw.ac.at/defc/thesaurus/FindsPotteryForm>,
        <http://id.acdh.oeaw.ac.at/defc/thesaurus/FindsSchema> ;
    skos:prefLabel "Platte"@de,
        "plate"@en .

<http://id.acdh.oeaw.ac.at/defc/thesaurus/platform/5.3> a skos:Concept ;
    skos:broader <http://id.acdh.oeaw.ac.at/defc/thesaurus/morturary_feature/4.086> ;
    skos:editorialNote "dc_area_mortuaryfeatures;3" ;
    skos:inScheme <http://id.acdh.oeaw.ac.at/defc/thesaurus/AreaMortuaryfeatures>,
        <http://id.acdh.oeaw.ac.at/defc/thesaurus/AreaSchema> ;
    skos:prefLabel "Plattform"@de,
        "platform"@en .

<http://id.acdh.oeaw.ac.at/defc/thesaurus/pointed_beaker/5.215> a skos:Concept ;
    skos:broader <http://id.acdh.oeaw.ac.at/defc/thesaurus/beaker/4.098> ;
    skos:editorialNote "dc_finds_pottery_form;215" ;
    skos:inScheme <http://id.acdh.oeaw.ac.at/defc/thesaurus/FindsPotteryForm>,
        <http://id.acdh.oeaw.ac.at/defc/thesaurus/FindsSchema> ;
    skos:prefLabel "spitzbodiger Becher"@de,
        "pointed beaker"@en .

<http://id.acdh.oeaw.ac.at/defc/thesaurus/pointillé_decoration/5.227> a skos:Concept ;
    dc:source "Kipfer, B. A. Dictionary of Artifacts 2007. Blackwell Publishing, Oxford.p 247" ;
    skos:broader <http://id.acdh.oeaw.ac.at/defc/thesaurus/plastic_decoration/4.132> ;
    skos:definition "Pottery decoration by marking with dots." ;
    skos:editorialNote "dc_finds_pottery_decoration;227" ;
    skos:inScheme <http://id.acdh.oeaw.ac.at/defc/thesaurus/FindsPotteryDecoration>,
        <http://id.acdh.oeaw.ac.at/defc/thesaurus/FindsSchema> ;
    skos:prefLabel "Pointillé Dekor"@de,
        "pointillé decoration"@en .

<http://id.acdh.oeaw.ac.at/defc/thesaurus/polished/4.228> a skos:Concept ;
    dc:source "OREA" ;
    skos:broader <http://id.acdh.oeaw.ac.at/defc/thesaurus/pottery_surface_treatment/3.019> ;
    skos:definition "Sufficiently dry ceramics in leather-hard stage is polished to compact its surface resulting in evenly smooth pottery." ;
    skos:editorialNote "dc_finds_pottery_decoration;228" ;
    skos:inScheme <http://id.acdh.oeaw.ac.at/defc/thesaurus/FindsPotteryDecoration>,
        <http://id.acdh.oeaw.ac.at/defc/thesaurus/FindsSchema> ;
    skos:prefLabel "Poliert"@de,
        "polished"@en .

<http://id.acdh.oeaw.ac.at/defc/thesaurus/polychrome/6.202> a skos:Concept ;
    dc:source "Kipfer, B. A. Dictionary of Artifacts 2007. Blackwell Publishing, Oxford.p 248" ;
    skos:broader <http://id.acdh.oeaw.ac.at/defc/thesaurus/pattern_painted/5.041> ;
    skos:definition "Pottery that is decorated in more than two colors, but the term is also sometimes applied to pottery with more than one color." ;
    skos:editorialNote "dc_finds_pottery_decoration;202" ;
    skos:inScheme <http://id.acdh.oeaw.ac.at/defc/thesaurus/FindsPotteryDecoration>,
        <http://id.acdh.oeaw.ac.at/defc/thesaurus/FindsSchema> ;
    skos:prefLabel "Polychrom"@de,
        "polychrome"@en .

<http://id.acdh.oeaw.ac.at/defc/thesaurus/polychrome_burnished/5.243> a skos:Concept ;
    dc:source "OREA" ;
    skos:broader <http://id.acdh.oeaw.ac.at/defc/thesaurus/burnished/4.297> ;
    skos:definition "Pottery painted with more than two colors and polished before firing." ;
    skos:editorialNote "dc_finds_pottery_decoration;243" ;
    skos:inScheme <http://id.acdh.oeaw.ac.at/defc/thesaurus/FindsPotteryDecoration>,
        <http://id.acdh.oeaw.ac.at/defc/thesaurus/FindsSchema> ;
    skos:prefLabel "Polychrom geglättet"@de,
        "polychrome burnished"@en .

<http://id.acdh.oeaw.ac.at/defc/thesaurus/poppy/4.16> a skos:Concept ;
    dc:source "http://eol.org/pages/594796/overview" ;
    skos:broader <http://id.acdh.oeaw.ac.at/defc/thesaurus/grain_crop/3.08> ;
    skos:editorialNote "dc_botany_species;16" ;
    skos:inScheme <http://id.acdh.oeaw.ac.at/defc/thesaurus/BotanySpecies>,
        <http://id.acdh.oeaw.ac.at/defc/thesaurus/FindsSchema> ;
    skos:prefLabel "Mohn"@de,
        "poppy"@en,
        "Papaver somniferum"@la .

<http://id.acdh.oeaw.ac.at/defc/thesaurus/porphyry/3.30> a skos:Concept ;
    dc:source "http://dbpedia.org/page/Porphyry_(geology)" ;
    skos:broader <http://id.acdh.oeaw.ac.at/defc/thesaurus/stone/2.1> ;
    skos:definition "Porphyry is a textural term for an igneous rock consisting of large-grained crystals such as feldspar or quartz dispersed in a fine-grained feldspathic matrix or groundmass." ;
    skos:editorialNote "dc_finds_material;30" ;
    skos:inScheme <http://id.acdh.oeaw.ac.at/defc/thesaurus/FindsMaterial>,
        <http://id.acdh.oeaw.ac.at/defc/thesaurus/FindsSchema> ;
    skos:prefLabel "Porphyr"@de,
        "porphyry"@en .

<http://id.acdh.oeaw.ac.at/defc/thesaurus/post_base/5.34> a skos:Concept ;
    dc:source "http://www.dartmouth.edu/~prehistory/aegean/?glossary-term=pier" ;
    skos:altLabel "pier"@en ;
    skos:broader <http://id.acdh.oeaw.ac.at/defc/thesaurus/installation/4.078> ;
    skos:definition "A freestanding, rectangular mass of masonry supporting the superstructure of a building" ;
    skos:editorialNote "dc_area_specialfeatures;34" ;
    skos:inScheme <http://id.acdh.oeaw.ac.at/defc/thesaurus/AreaSchema>,
        <http://id.acdh.oeaw.ac.at/defc/thesaurus/AreaSpecialfeatures> ;
    skos:prefLabel "post base"@en .

<http://id.acdh.oeaw.ac.at/defc/thesaurus/post_hole/5.3> a skos:Concept ;
    dc:source "OREA" ;
    skos:broader <http://id.acdh.oeaw.ac.at/defc/thesaurus/occupation_evidence/4.088> ;
    skos:definition "A hole dug to provide a firm base for an upright post, often with stone packing found in a cave or a rockshelter as evidence of human occupation." ;
    skos:editorialNote "dc_area_evidenceofocupation;3" ;
    skos:inScheme <http://id.acdh.oeaw.ac.at/defc/thesaurus/AreaEvidenceofocupation>,
        <http://id.acdh.oeaw.ac.at/defc/thesaurus/AreaSchema> ;
    skos:prefLabel "Pfostenloch"@de,
        "post hole"@en .

<http://id.acdh.oeaw.ac.at/defc/thesaurus/post_hole/5.5> a skos:Concept ;
    dc:source "http://thesaurus.historicengland.org.uk/thesaurus_term.asp?thes_no=546&term_no=138109" ;
    skos:altLabel "Pfostenloch"@de ;
    skos:broader <http://id.acdh.oeaw.ac.at/defc/thesaurus/installation/4.078> ;
    skos:definition "A hole dug to provide a firm base for an upright post, often with stone packing." ;
    skos:editorialNote "dc_area_specialfeatures;5" ;
    skos:inScheme <http://id.acdh.oeaw.ac.at/defc/thesaurus/AreaSchema>,
        <http://id.acdh.oeaw.ac.at/defc/thesaurus/AreaSpecialfeatures> ;
    skos:prefLabel "post hole"@en .

<http://id.acdh.oeaw.ac.at/defc/thesaurus/pottery_production/2.7> a skos:Concept ;
    dc:source "OREA" ;
    skos:broader <http://id.acdh.oeaw.ac.at/defc/thesaurus/production/1.042> ;
    skos:definition "The activity of making objects of clay and hardened with heat." ;
    skos:editorialNote "dc_interpretation_productiontype;7" ;
    skos:inScheme <http://id.acdh.oeaw.ac.at/defc/thesaurus/InterpretationProductiontype>,
        <http://id.acdh.oeaw.ac.at/defc/thesaurus/InterpretationSchema> ;
    skos:prefLabel "Keramikproduktion"@de,
        "pottery production"@en .

<http://id.acdh.oeaw.ac.at/defc/thesaurus/pottery_tool_production/2.8> a skos:Concept ;
    dc:source "OREA" ;
    skos:broader <http://id.acdh.oeaw.ac.at/defc/thesaurus/production/1.042> ;
    skos:definition "The activity of making physical items of burnt clay that can be afterwards used to achive a certain goal." ;
    skos:editorialNote "dc_interpretation_productiontype;8" ;
    skos:inScheme <http://id.acdh.oeaw.ac.at/defc/thesaurus/InterpretationProductiontype>,
        <http://id.acdh.oeaw.ac.at/defc/thesaurus/InterpretationSchema> ;
    skos:prefLabel "Keramikwerkzeugproduktion"@de,
        "pottery tool production"@en .

<http://id.acdh.oeaw.ac.at/defc/thesaurus/pressure_technique/5.3> a skos:Concept ;
    dc:source "Inizan, M.-L., M. Reduron-Ballinger, H. Roche, J. Tixier 1999, Technology and Terminology of Knapped Stone. Nanterre: CREP. p. 32." ;
    skos:broader <http://id.acdh.oeaw.ac.at/defc/thesaurus/lithics_technology/4.023> ;
    skos:definition "Application of pressure to fracture raw materials. Pressure is applied with the narrow end of a tool made of wood, antler, bone or metal." ;
    skos:editorialNote "dc_finds_lithics_technology;3" ;
    skos:inScheme <http://id.acdh.oeaw.ac.at/defc/thesaurus/FindsLithicsTechnology>,
        <http://id.acdh.oeaw.ac.at/defc/thesaurus/FindsSchema> ;
    skos:prefLabel "pressure technique"@en .

<http://id.acdh.oeaw.ac.at/defc/thesaurus/profile_clearing/3.24> a skos:Concept ;
    skos:broader <http://id.acdh.oeaw.ac.at/defc/thesaurus/intrusive/2.048> ;
    skos:editorialNote "dc_researchevet_researchtype;24" ;
    skos:inScheme <http://id.acdh.oeaw.ac.at/defc/thesaurus/ResearchEventSchema>,
        <http://id.acdh.oeaw.ac.at/defc/thesaurus/ResearchevetResearchtype> ;
    skos:prefLabel "profile clearing"@en .

<http://id.acdh.oeaw.ac.at/defc/thesaurus/projectile_point/4.15> a skos:Concept ;
    dc:source "Inizan, M.-L., M. Reduron-Ballinger, H. Roche, J. Tixier 1999, Technology and Terminology of Knapped Stone. Nanterre: CREP., D. Srejovic (ed) 1997, Arheološki Leksikon." ;
    skos:altLabel "arrowhead"@en,
        "point"@en ;
    skos:broader <http://id.acdh.oeaw.ac.at/defc/thesaurus/retouched_tool/3.010> ;
    skos:definition "A pointed retouched artefact, with or without tang for hafting, used for the purposes of hunting or warfare." ;
    skos:editorialNote "dc_finds_lithics_retouched_tools;15" ;
    skos:inScheme <http://id.acdh.oeaw.ac.at/defc/thesaurus/FindsLithicsRetouchedTools>,
        <http://id.acdh.oeaw.ac.at/defc/thesaurus/FindsSchema> ;
    skos:prefLabel "Projektilspitze"@de,
        "projectile point"@en .

<http://id.acdh.oeaw.ac.at/defc/thesaurus/pronged_wishbone_handle/6.148> a skos:Concept ;
    dc:source "OREA" ;
    skos:broader <http://id.acdh.oeaw.ac.at/defc/thesaurus/wishbone_handle/5.93> ;
    skos:definition "A liminal, horizontal, bird-bone shaped, loop handle with bar application." ;
    skos:editorialNote "dc_finds_pottery_detail;148" ;
    skos:inScheme <http://id.acdh.oeaw.ac.at/defc/thesaurus/FindsPotteryDetail>,
        <http://id.acdh.oeaw.ac.at/defc/thesaurus/FindsSchema> ;
    skos:prefLabel "Gabelhenkel mit Stabaufsatz"@de,
        "pronged wishbone handle"@en .

<http://id.acdh.oeaw.ac.at/defc/thesaurus/punched/5.229> a skos:Concept ;
    dc:source "OREA" ;
    skos:broader <http://id.acdh.oeaw.ac.at/defc/thesaurus/incised/4.168> ;
    skos:definition "Pierced/drilled pottery decoration." ;
    skos:editorialNote "dc_finds_pottery_decoration;229" ;
    skos:inScheme <http://id.acdh.oeaw.ac.at/defc/thesaurus/FindsPotteryDecoration>,
        <http://id.acdh.oeaw.ac.at/defc/thesaurus/FindsSchema> ;
    skos:prefLabel "Lochdekor"@de,
        "punched"@en .

<http://id.acdh.oeaw.ac.at/defc/thesaurus/pyre/5.1> a skos:Concept ;
    skos:broader <http://id.acdh.oeaw.ac.at/defc/thesaurus/morturary_feature/4.086> ;
    skos:editorialNote "dc_area_mortuaryfeatures;1" ;
    skos:inScheme <http://id.acdh.oeaw.ac.at/defc/thesaurus/AreaMortuaryfeatures>,
        <http://id.acdh.oeaw.ac.at/defc/thesaurus/AreaSchema> ;
    skos:prefLabel "Scheiterhaufen"@de,
        "pyre"@en .

<http://id.acdh.oeaw.ac.at/defc/thesaurus/pyxis/4.166> a skos:Concept ;
    dc:source "OREA" ;
    skos:broader <http://id.acdh.oeaw.ac.at/defc/thesaurus/pottery_form/3.016> ;
    skos:definition "A cylindrical box-like vessel with angular shoulders and lid." ;
    skos:editorialNote "dc_finds_pottery_form;166" ;
    skos:inScheme <http://id.acdh.oeaw.ac.at/defc/thesaurus/FindsPotteryForm>,
        <http://id.acdh.oeaw.ac.at/defc/thesaurus/FindsSchema> ;
    skos:prefLabel "Pyxis"@de,
        "pyxis"@en .

<http://id.acdh.oeaw.ac.at/defc/thesaurus/quartz/3.15> a skos:Concept ;
    dc:source "https://www.britannica.com/science/quartz" ;
    skos:broader <http://id.acdh.oeaw.ac.at/defc/thesaurus/stone/2.1> ;
    skos:definition "Widely distributed mineral of many varieties that consists primarily of silica, or silicon dioxide (SiO2)." ;
    skos:editorialNote "dc_finds_material;15" ;
    skos:inScheme <http://id.acdh.oeaw.ac.at/defc/thesaurus/FindsMaterial>,
        <http://id.acdh.oeaw.ac.at/defc/thesaurus/FindsSchema> ;
    skos:prefLabel "quartz"@en .

<http://id.acdh.oeaw.ac.at/defc/thesaurus/quartz/5.6> a skos:Concept ;
    dc:source "https://www.britannica.com/science/quartz" ;
    skos:broader <http://id.acdh.oeaw.ac.at/defc/thesaurus/stone/4.025> ;
    skos:definition "Widely distributed mineral of many varieties that consists primarily of silica, or silicon dioxide (SiO2). Used to produce lithics." ;
    skos:editorialNote "dc_finds_lithics_raw_material;6" ;
    skos:inScheme <http://id.acdh.oeaw.ac.at/defc/thesaurus/FindsLithicsRawMaterial>,
        <http://id.acdh.oeaw.ac.at/defc/thesaurus/FindsSchema> ;
    skos:prefLabel "quartz"@en .

<http://id.acdh.oeaw.ac.at/defc/thesaurus/quartzite/5.8> a skos:Concept ;
    dc:source "https://www.britannica.com/science/quartzite" ;
    skos:broader <http://id.acdh.oeaw.ac.at/defc/thesaurus/stone/4.025> ;
    skos:definition "A sandstone that has been converted into a solid quartz rock. Unlike sandstones, quartzites are free from pores and have a smooth fracture. Used to produce lithics." ;
    skos:editorialNote "dc_finds_lithics_raw_material;8" ;
    skos:inScheme <http://id.acdh.oeaw.ac.at/defc/thesaurus/FindsLithicsRawMaterial>,
        <http://id.acdh.oeaw.ac.at/defc/thesaurus/FindsSchema> ;
    skos:prefLabel "Quarzit"@de,
        "quartzite"@en .

<http://id.acdh.oeaw.ac.at/defc/thesaurus/quarzite/3.17> a skos:Concept ;
    dc:source "https://www.britannica.com/science/quartzite" ;
    skos:broader <http://id.acdh.oeaw.ac.at/defc/thesaurus/stone/2.1> ;
    skos:definition "A sandstone that has been converted into a solid quartz rock. Unlike sandstones, quartzites are free from pores and have a smooth fracture;" ;
    skos:editorialNote "dc_finds_material;17" ;
    skos:inScheme <http://id.acdh.oeaw.ac.at/defc/thesaurus/FindsMaterial>,
        <http://id.acdh.oeaw.ac.at/defc/thesaurus/FindsSchema> ;
    skos:prefLabel "Quarzit"@de,
        "quarzite"@en .

<http://id.acdh.oeaw.ac.at/defc/thesaurus/radiocarbon_dating/4.1> a skos:Concept ;
    dc:source "http://thesaurus.historicengland.org.uk/thesaurus_term.asp?thes_no=560&term_no=142188" ;
    skos:altLabel "C14"@en ;
    skos:broader <http://id.acdh.oeaw.ac.at/defc/thesaurus/dating_method/3.045> ;
    skos:definition "The measurement of the ration of the radioactive Carbon 14 (C-14) isotope and non-radioactive carbon isotopes. Useful for dating organic materials such as wood and bone between 500 and 45000 years old." ;
    skos:editorialNote "dc_period_datingmethod;1" ;
    skos:inScheme <http://id.acdh.oeaw.ac.at/defc/thesaurus/PeriodSchema> ;
    skos:prefLabel "C14-Datierung"@de,
        "radiocarbon dating"@en .

<http://id.acdh.oeaw.ac.at/defc/thesaurus/radiolarite/4.18> a skos:Concept ;
    dc:source "https://en.wikipedia.org/wiki/Radiolarite" ;
    skos:broader <http://id.acdh.oeaw.ac.at/defc/thesaurus/chert/3.12> ;
    skos:definition "Radiolarite is a siliceous, comparatively hard, fine-grained, chert-like, and homogeneous sedimentary rock that is composed predominantly of the microscopic remains of radiolarians used to make stone tools and weapons." ;
    skos:editorialNote "dc_finds_material;18" ;
    skos:inScheme <http://id.acdh.oeaw.ac.at/defc/thesaurus/FindsMaterial>,
        <http://id.acdh.oeaw.ac.at/defc/thesaurus/FindsSchema> ;
    skos:prefLabel "Radiolarit"@de,
        "radiolarite"@en .

<http://id.acdh.oeaw.ac.at/defc/thesaurus/radiolarite/6.9> a skos:Concept ;
    dc:source "https://en.wikipedia.org/wiki/Radiolarite" ;
    skos:broader <http://id.acdh.oeaw.ac.at/defc/thesaurus/chert/5.3> ;
    skos:definition "Radiolarite is a siliceous, comparatively hard, fine-grained, chert-like, and homogeneous sedimentary rock that is composed predominantly of the microscopic remains of radiolarians used to make stone tools and weapons." ;
    skos:editorialNote "dc_finds_lithics_raw_material;9" ;
    skos:inScheme <http://id.acdh.oeaw.ac.at/defc/thesaurus/FindsLithicsRawMaterial>,
        <http://id.acdh.oeaw.ac.at/defc/thesaurus/FindsSchema> ;
    skos:prefLabel "Radiolarit"@de,
        "radiolarite"@en .

<http://id.acdh.oeaw.ac.at/defc/thesaurus/rectangular-apsidal/5.5> a skos:Concept ;
    dc:source "OREA" ;
    skos:broader <http://id.acdh.oeaw.ac.at/defc/thesaurus/building_shape/4.076> ;
    skos:definition "A rectangular building with a semi-circular recess on one sinde." ;
    skos:editorialNote "dc_area_constructionshape;5" ;
    skos:inScheme <http://id.acdh.oeaw.ac.at/defc/thesaurus/AreaConstructionshape>,
        <http://id.acdh.oeaw.ac.at/defc/thesaurus/AreaSchema> ;
    skos:prefLabel "rectangular-apsidal"@en .

<http://id.acdh.oeaw.ac.at/defc/thesaurus/rectangular/5.4> a skos:Concept ;
    dc:source "OREA" ;
    skos:broader <http://id.acdh.oeaw.ac.at/defc/thesaurus/building_shape/4.076> ;
    skos:definition "A building with a rectangular ground plan." ;
    skos:editorialNote "dc_area_constructionshape;4" ;
    skos:inScheme <http://id.acdh.oeaw.ac.at/defc/thesaurus/AreaConstructionshape>,
        <http://id.acdh.oeaw.ac.at/defc/thesaurus/AreaSchema> ;
    skos:prefLabel "rectangular"@en .

<http://id.acdh.oeaw.ac.at/defc/thesaurus/red_burnished/5.248> a skos:Concept ;
    dc:source "OREA" ;
    skos:broader <http://id.acdh.oeaw.ac.at/defc/thesaurus/burnished/4.297> ;
    skos:definition "The red slip was applied onto the vessel and burnished." ;
    skos:editorialNote "dc_finds_pottery_decoration;248" ;
    skos:inScheme <http://id.acdh.oeaw.ac.at/defc/thesaurus/FindsPotteryDecoration>,
        <http://id.acdh.oeaw.ac.at/defc/thesaurus/FindsSchema> ;
    skos:prefLabel "Rot geglättet"@de,
        "red burnished"@en .

<http://id.acdh.oeaw.ac.at/defc/thesaurus/red_burnished_(b1)/5.156> a skos:Concept ;
    dc:source "OREA" ;
    skos:broader <http://id.acdh.oeaw.ac.at/defc/thesaurus/burnished/4.297> ;
    skos:definition "The red slip was applied onto the vessel and burnished." ;
    skos:editorialNote "dc_finds_pottery_decoration;156" ;
    skos:inScheme <http://id.acdh.oeaw.ac.at/defc/thesaurus/FindsPotteryDecoration>,
        <http://id.acdh.oeaw.ac.at/defc/thesaurus/FindsSchema> ;
    skos:prefLabel "Rot geglättet (B1)"@de,
        "red burnished (b1)"@en .

<http://id.acdh.oeaw.ac.at/defc/thesaurus/red_deer/6.13> a skos:Concept ;
    dc:source "http://eol.org/pages/328649/overview" ;
    skos:broader <http://id.acdh.oeaw.ac.at/defc/thesaurus/deer/5.036> ;
    skos:editorialNote "dc_finds_animal_remains_species;13" ;
    skos:inScheme <http://id.acdh.oeaw.ac.at/defc/thesaurus/FindsAnimalRemainsSpecies>,
        <http://id.acdh.oeaw.ac.at/defc/thesaurus/FindsSchema> ;
    skos:prefLabel "Rothirsch"@de,
        "red deer"@en,
        "Cervus elaphus"@la .

<http://id.acdh.oeaw.ac.at/defc/thesaurus/red_fox/5.25> a skos:Concept ;
    dc:source "http://eol.org/pages/328609/overview" ;
    skos:broader <http://id.acdh.oeaw.ac.at/defc/thesaurus/mammal/4.020> ;
    skos:editorialNote "dc_finds_animal_remains_species;25" ;
    skos:inScheme <http://id.acdh.oeaw.ac.at/defc/thesaurus/FindsAnimalRemainsSpecies>,
        <http://id.acdh.oeaw.ac.at/defc/thesaurus/FindsSchema> ;
    skos:prefLabel "roter Fuchs"@de,
        "red fox"@en,
        "Vulpes vulpes"@la .

<http://id.acdh.oeaw.ac.at/defc/thesaurus/red_incrusted/5.203> a skos:Concept ;
    dc:source "OREA" ;
    skos:broader <http://id.acdh.oeaw.ac.at/defc/thesaurus/incised/4.168> ;
    skos:definition "The red slip was impressed into the surface of a ceramic vessel." ;
    skos:editorialNote "dc_finds_pottery_decoration;203" ;
    skos:inScheme <http://id.acdh.oeaw.ac.at/defc/thesaurus/FindsPotteryDecoration>,
        <http://id.acdh.oeaw.ac.at/defc/thesaurus/FindsSchema> ;
    skos:prefLabel "Rot inkrustiert"@de,
        "red incrusted"@en .

<http://id.acdh.oeaw.ac.at/defc/thesaurus/red_on_brown/6.204> a skos:Concept ;
    dc:source "OREA" ;
    skos:broader <http://id.acdh.oeaw.ac.at/defc/thesaurus/pattern_painted/5.041> ;
    skos:definition "Pottery painted with red paint on brown ground." ;
    skos:editorialNote "dc_finds_pottery_decoration;204" ;
    skos:inScheme <http://id.acdh.oeaw.ac.at/defc/thesaurus/FindsPotteryDecoration>,
        <http://id.acdh.oeaw.ac.at/defc/thesaurus/FindsSchema> ;
    skos:prefLabel "Rot auf braun"@de,
        "red on brown"@en .

<http://id.acdh.oeaw.ac.at/defc/thesaurus/red_on_buff/6.230> a skos:Concept ;
    dc:source "OREA" ;
    skos:broader <http://id.acdh.oeaw.ac.at/defc/thesaurus/pattern_painted/5.041> ;
    skos:definition "Pottery painted with red paint on buff ground." ;
    skos:editorialNote "dc_finds_pottery_decoration;230" ;
    skos:inScheme <http://id.acdh.oeaw.ac.at/defc/thesaurus/FindsPotteryDecoration>,
        <http://id.acdh.oeaw.ac.at/defc/thesaurus/FindsSchema> ;
    skos:prefLabel "Rot auf hell"@de,
        "red on buff"@en .

<http://id.acdh.oeaw.ac.at/defc/thesaurus/red_on_red/6.268> a skos:Concept ;
    dc:source "OREA" ;
    skos:broader <http://id.acdh.oeaw.ac.at/defc/thesaurus/pattern_painted/5.041> ;
    skos:definition "Pottery painted with red paint on red ground." ;
    skos:editorialNote "dc_finds_pottery_decoration;268" ;
    skos:inScheme <http://id.acdh.oeaw.ac.at/defc/thesaurus/FindsPotteryDecoration>,
        <http://id.acdh.oeaw.ac.at/defc/thesaurus/FindsSchema> ;
    skos:prefLabel "rot auf rot"@de,
        "red on red"@en .

<http://id.acdh.oeaw.ac.at/defc/thesaurus/red_on_red_(a3γ)/6.158> a skos:Concept ;
    dc:source "OREA" ;
    skos:broader <http://id.acdh.oeaw.ac.at/defc/thesaurus/pattern_painted/5.041> ;
    skos:definition "Pottery painted with red paint on red ground." ;
    skos:editorialNote "dc_finds_pottery_decoration;158" ;
    skos:inScheme <http://id.acdh.oeaw.ac.at/defc/thesaurus/FindsPotteryDecoration>,
        <http://id.acdh.oeaw.ac.at/defc/thesaurus/FindsSchema> ;
    skos:prefLabel "Rot on red (A3c)"@de,
        "red on red (a3γ)"@en .

<http://id.acdh.oeaw.ac.at/defc/thesaurus/red_on_white/6.290> a skos:Concept ;
    dc:source "OREA" ;
    skos:broader <http://id.acdh.oeaw.ac.at/defc/thesaurus/pattern_painted/5.041> ;
    skos:definition "Pottery painted with red paint on white ground." ;
    skos:editorialNote "dc_finds_pottery_decoration;290" ;
    skos:inScheme <http://id.acdh.oeaw.ac.at/defc/thesaurus/FindsPotteryDecoration>,
        <http://id.acdh.oeaw.ac.at/defc/thesaurus/FindsSchema> ;
    skos:prefLabel "Rot auf weiß"@de,
        "red on white"@en .

<http://id.acdh.oeaw.ac.at/defc/thesaurus/red_on_white_(a3ß)/6.157> a skos:Concept ;
    dc:source "OREA" ;
    skos:broader <http://id.acdh.oeaw.ac.at/defc/thesaurus/pattern_painted/5.041> ;
    skos:definition "Pottery painted with red paint on white ground." ;
    skos:editorialNote "dc_finds_pottery_decoration;157" ;
    skos:inScheme <http://id.acdh.oeaw.ac.at/defc/thesaurus/FindsPotteryDecoration>,
        <http://id.acdh.oeaw.ac.at/defc/thesaurus/FindsSchema> ;
    skos:prefLabel "Rot auf weiß (A3b)"@de,
        "red on white (a3ß)"@en .

<http://id.acdh.oeaw.ac.at/defc/thesaurus/red_on_yellow/6.282> a skos:Concept ;
    dc:source "OREA" ;
    skos:broader <http://id.acdh.oeaw.ac.at/defc/thesaurus/pattern_painted/5.041> ;
    skos:definition "Pottery painted with red paint on yellow ground." ;
    skos:editorialNote "dc_finds_pottery_decoration;282" ;
    skos:inScheme <http://id.acdh.oeaw.ac.at/defc/thesaurus/FindsPotteryDecoration>,
        <http://id.acdh.oeaw.ac.at/defc/thesaurus/FindsSchema> ;
    skos:prefLabel "rot auf gelb"@de,
        "red on yellow"@en .

<http://id.acdh.oeaw.ac.at/defc/thesaurus/red_slipped/5.134> a skos:Concept ;
    dc:source "Kipfer, B. A. Dictionary of Artifacts 2007. Blackwell Publishing, Oxford.p 264" ;
    skos:broader <http://id.acdh.oeaw.ac.at/defc/thesaurus/slipped/4.302> ;
    skos:definition "Any pottery to which a slip, a thin layer of fine clay, is applied to pottery before firing by dipping the pot into a thick liquid mixture of clay and water. Slip decorates the fabric, is often chosen to bake to a color such as red and makes the pot more" ;
    skos:editorialNote "dc_finds_pottery_decoration;134" ;
    skos:inScheme <http://id.acdh.oeaw.ac.at/defc/thesaurus/FindsPotteryDecoration>,
        <http://id.acdh.oeaw.ac.at/defc/thesaurus/FindsSchema> ;
    skos:prefLabel "Ware mit rotem Überzug"@de,
        "red slipped"@en .

<http://id.acdh.oeaw.ac.at/defc/thesaurus/red_topped/5.284> a skos:Concept ;
    dc:source "OREA" ;
    skos:altLabel "Red-topped"@de ;
    skos:broader <http://id.acdh.oeaw.ac.at/defc/thesaurus/topped/4.035> ;
    skos:definition "Burnished ware with red oxidized rim and black surface typical for Northern Greece." ;
    skos:editorialNote "dc_finds_pottery_decoration;284" ;
    skos:inScheme <http://id.acdh.oeaw.ac.at/defc/thesaurus/FindsPotteryDecoration>,
        <http://id.acdh.oeaw.ac.at/defc/thesaurus/FindsSchema> ;
    skos:prefLabel "red topped"@de,
        "red topped"@en .

<http://id.acdh.oeaw.ac.at/defc/thesaurus/retouched_blade/4.16> a skos:Concept ;
    dc:source "Inizan, M.-L., M. Reduron-Ballinger, H. Roche, J. Tixier 1999, Technology and Terminology of Knapped Stone. Nanterre: CREP., D. Srejovic (ed) 1997, Arheološki Leksikon." ;
    skos:broader <http://id.acdh.oeaw.ac.at/defc/thesaurus/retouched_tool/3.010> ;
    skos:definition "A blade with retouch on one or both edges." ;
    skos:editorialNote "dc_finds_lithics_retouched_tools;16" ;
    skos:inScheme <http://id.acdh.oeaw.ac.at/defc/thesaurus/FindsLithicsRetouchedTools>,
        <http://id.acdh.oeaw.ac.at/defc/thesaurus/FindsSchema> ;
    skos:prefLabel "retuschierte Klinge"@de,
        "retouched blade"@en .

<http://id.acdh.oeaw.ac.at/defc/thesaurus/retouched_flake/4.17> a skos:Concept ;
    dc:source "Inizan, M.-L., M. Reduron-Ballinger, H. Roche, J. Tixier 1999, Technology and Terminology of Knapped Stone. Nanterre: CREP., D. Srejovic (ed) 1997, Arheološki Leksikon." ;
    skos:broader <http://id.acdh.oeaw.ac.at/defc/thesaurus/retouched_tool/3.010> ;
    skos:definition "A flake with retouches on one or both edges." ;
    skos:editorialNote "dc_finds_lithics_retouched_tools;17" ;
    skos:inScheme <http://id.acdh.oeaw.ac.at/defc/thesaurus/FindsLithicsRetouchedTools>,
        <http://id.acdh.oeaw.ac.at/defc/thesaurus/FindsSchema> ;
    skos:prefLabel "retuschirter Abschlag"@de,
        "retouched flake"@en .

<http://id.acdh.oeaw.ac.at/defc/thesaurus/rhyton/4.186> a skos:Concept ;
    dc:source "OREA" ;
    skos:broader <http://id.acdh.oeaw.ac.at/defc/thesaurus/pottery_form/3.016> ;
    skos:definition "Zoomorphic vessel in a shape of a horn used for drinking and pouring." ;
    skos:editorialNote "dc_finds_pottery_form;186" ;
    skos:inScheme <http://id.acdh.oeaw.ac.at/defc/thesaurus/FindsPotteryForm>,
        <http://id.acdh.oeaw.ac.at/defc/thesaurus/FindsSchema> ;
    skos:prefLabel "Rhyton"@de,
        "rhyton"@en .

<http://id.acdh.oeaw.ac.at/defc/thesaurus/rim-attached_strap_handle/6.151> a skos:Concept ;
    dc:source "OREA" ;
    skos:broader <http://id.acdh.oeaw.ac.at/defc/thesaurus/strap_handle/5.78> ;
    skos:definition "Liminal strip of clay attached to a vessel before firing." ;
    skos:editorialNote "dc_finds_pottery_detail;151" ;
    skos:inScheme <http://id.acdh.oeaw.ac.at/defc/thesaurus/FindsPotteryDetail>,
        <http://id.acdh.oeaw.ac.at/defc/thesaurus/FindsSchema> ;
    skos:prefLabel "Randständiger Bandhenkel"@de,
        "rim-attached strap handle"@en .

<http://id.acdh.oeaw.ac.at/defc/thesaurus/rim_attachment/5.94> a skos:Concept ;
    dc:source "OREA" ;
    skos:broader <http://id.acdh.oeaw.ac.at/defc/thesaurus/attachment/4.034> ;
    skos:definition "An add-on made of clay attached to the upper part of a vessel between the lip or margin and the side wall or neck of a vessel." ;
    skos:editorialNote "dc_finds_pottery_detail;94" ;
    skos:inScheme <http://id.acdh.oeaw.ac.at/defc/thesaurus/FindsPotteryDetail>,
        <http://id.acdh.oeaw.ac.at/defc/thesaurus/FindsSchema> ;
    skos:prefLabel "Randaufsatz"@de,
        "rim attachment"@en .

<http://id.acdh.oeaw.ac.at/defc/thesaurus/ring/4.103> a skos:Concept ;
    dc:source "Kipfer, B. A. Dictionary of Artifacts 2007. Blackwell Publishing, Oxford.p 271" ;
    skos:broader <http://id.acdh.oeaw.ac.at/defc/thesaurus/jewellery/3.2> ;
    skos:definition "A small circular band, typically of precious metal and often set with one or more gemstones, worn on a finger as an ornament or a token of marriage, engagement, or autority." ;
    skos:editorialNote "dc_finds_small_finds_type;103" ;
    skos:inScheme <http://id.acdh.oeaw.ac.at/defc/thesaurus/FindsSchema>,
        <http://id.acdh.oeaw.ac.at/defc/thesaurus/FindsSmallFindsType> ;
    skos:prefLabel "Ring"@de,
        "ring"@en .

<http://id.acdh.oeaw.ac.at/defc/thesaurus/ring_base/5.180> a skos:Concept ;
    dc:source "http://www.bible.ca/archeology/bible-archeology-pottery-glossary-dictionary-encyclopedia.htm" ;
    skos:broader <http://id.acdh.oeaw.ac.at/defc/thesaurus/base/4.032> ;
    skos:definition "A circular clay band encircling the bottom of the vessel and often occurred on wheelmade vessels. This base may also be elevated." ;
    skos:editorialNote "dc_finds_pottery_detail;180" ;
    skos:inScheme <http://id.acdh.oeaw.ac.at/defc/thesaurus/FindsPotteryDetail>,
        <http://id.acdh.oeaw.ac.at/defc/thesaurus/FindsSchema> ;
    skos:prefLabel "Standring"@de,
        "ring base"@en .

<http://id.acdh.oeaw.ac.at/defc/thesaurus/ring_idol/4.137> a skos:Concept ;
    skos:broader <http://id.acdh.oeaw.ac.at/defc/thesaurus/figurine/3.3> ;
    skos:editorialNote "dc_finds_small_finds_type;137" ;
    skos:inScheme <http://id.acdh.oeaw.ac.at/defc/thesaurus/FindsSchema>,
        <http://id.acdh.oeaw.ac.at/defc/thesaurus/FindsSmallFindsType> ;
    skos:prefLabel "Ringidol"@de,
        "ring idol"@en .

<http://id.acdh.oeaw.ac.at/defc/thesaurus/rippled/4.177> a skos:Concept ;
    dc:source "Kipfer, B. A. Dictionary of Artifacts 2007. Blackwell Publishing, Oxford.p 271" ;
    skos:altLabel "ripple burnished"@de ;
    skos:broader <http://id.acdh.oeaw.ac.at/defc/thesaurus/pottery_surface_treatment/3.019> ;
    skos:definition "A technique of pottery burnish in which the whole surface is worked into ripples, in extreme examples it approaches fluting." ;
    skos:editorialNote "dc_finds_pottery_decoration;177" ;
    skos:inScheme <http://id.acdh.oeaw.ac.at/defc/thesaurus/FindsPotteryDecoration>,
        <http://id.acdh.oeaw.ac.at/defc/thesaurus/FindsSchema> ;
    skos:prefLabel "Wellig"@de,
        "rippled"@en .

<http://id.acdh.oeaw.ac.at/defc/thesaurus/rippled_burnished/5.231> a skos:Concept ;
    dc:source "Kipfer, B. A. Dictionary of Artifacts 2007. Blackwell Publishing, Oxford.p 271" ;
    skos:altLabel "rippled"@de ;
    skos:broader <http://id.acdh.oeaw.ac.at/defc/thesaurus/burnished/4.297> ;
    skos:definition "A technique of pottery burnish in which the whole surface is worked into ripples, in extreme examples it approaches fluting." ;
    skos:editorialNote "dc_finds_pottery_decoration;231" ;
    skos:inScheme <http://id.acdh.oeaw.ac.at/defc/thesaurus/FindsPotteryDecoration>,
        <http://id.acdh.oeaw.ac.at/defc/thesaurus/FindsSchema> ;
    skos:prefLabel "Wellig geglättet"@de,
        "rippled burnished"@en .

<http://id.acdh.oeaw.ac.at/defc/thesaurus/river_delta/2.8> a skos:Concept ;
    skos:broader "topography/1.099" ;
    skos:definition "A river mouth in which a river devides into smaller rivers, because of the sediment dropped by the river."@en ;
    skos:editorialNote "dc_site_topography;8" ;
    skos:inScheme <http://id.acdh.oeaw.ac.at/defc/thesaurus/SiteSchema>,
        "SiteTopography" ;
    skos:prefLabel "Flussdelta"@de,
        "river delta"@en .

<http://id.acdh.oeaw.ac.at/defc/thesaurus/rock_crystal/3.16> a skos:Concept ;
    dc:source "https://www.britannica.com/topic/rock-crystal" ;
    skos:broader <http://id.acdh.oeaw.ac.at/defc/thesaurus/mineral/2.3> ;
    skos:definition "Rock crystal, transparent variety of the silica mineral quartz that is valued for its clarity and total lack of colour or flaws. Used for carving and as an ornamental mineral." ;
    skos:editorialNote "dc_finds_material;16" ;
    skos:inScheme <http://id.acdh.oeaw.ac.at/defc/thesaurus/FindsMaterial>,
        <http://id.acdh.oeaw.ac.at/defc/thesaurus/FindsSchema> ;
    skos:prefLabel "Bergkristall"@de,
        "rock crystal"@en .

<http://id.acdh.oeaw.ac.at/defc/thesaurus/rock_crystal/5.7> a skos:Concept ;
    dc:source "https://www.britannica.com/topic/rock-crystal" ;
    skos:broader <http://id.acdh.oeaw.ac.at/defc/thesaurus/mineral/4.026> ;
    skos:definition "Rock crystal, transparent variety of the silica mineral quartz that is valued for its clarity and total lack of colour or flaws. Used for carving (lithics)." ;
    skos:editorialNote "dc_finds_lithics_raw_material;7" ;
    skos:inScheme <http://id.acdh.oeaw.ac.at/defc/thesaurus/FindsLithicsRawMaterial>,
        <http://id.acdh.oeaw.ac.at/defc/thesaurus/FindsSchema> ;
    skos:prefLabel "Bergkristall"@de,
        "rock crystal"@en .

<http://id.acdh.oeaw.ac.at/defc/thesaurus/rock_shelter/3.2> a skos:Concept ;
    dc:source "Kipfer, B. A. Encyclopedic Dictionary of Archaeology. Kluwer Academic/Plenum Publishers, New York. p. 483." ;
    skos:broader <http://id.acdh.oeaw.ac.at/defc/thesaurus/cave_or_rockshelter/2.1> ;
    skos:definition "A natural cave with a roof of overlying rock, which extends beyond the sides of the cave; a cave that is formed by a ledge of overhanging rock. Such a shallow cave or cliff overhang was used by humans as shelter from the elements, especially among hunters" ;
    skos:editorialNote "dc_area_caverockshelterstype;2" ;
    skos:inScheme <http://id.acdh.oeaw.ac.at/defc/thesaurus/AreaCaverockshelterstype>,
        <http://id.acdh.oeaw.ac.at/defc/thesaurus/AreaSchema> ;
    skos:prefLabel "Felsdach"@de,
        "rock shelter"@en .

<http://id.acdh.oeaw.ac.at/defc/thesaurus/roe_deer/6.23> a skos:Concept ;
    dc:source "http://eol.org/pages/308479/overview" ;
    skos:broader <http://id.acdh.oeaw.ac.at/defc/thesaurus/deer/5.036> ;
    skos:editorialNote "dc_finds_animal_remains_species;23" ;
    skos:inScheme <http://id.acdh.oeaw.ac.at/defc/thesaurus/FindsAnimalRemainsSpecies>,
        <http://id.acdh.oeaw.ac.at/defc/thesaurus/FindsSchema> ;
    skos:prefLabel "Reh"@de,
        "roe deer"@en,
        "Capreolus capreolus"@la .

<http://id.acdh.oeaw.ac.at/defc/thesaurus/rolled_rim/5.77> a skos:Concept ;
    dc:source "OREA" ;
    skos:broader <http://id.acdh.oeaw.ac.at/defc/thesaurus/rim/4.033> ;
    skos:definition "Inwards thickened rim with round cross section." ;
    skos:editorialNote "dc_finds_pottery_detail;77" ;
    skos:inScheme <http://id.acdh.oeaw.ac.at/defc/thesaurus/FindsPotteryDetail>,
        <http://id.acdh.oeaw.ac.at/defc/thesaurus/FindsSchema> ;
    skos:prefLabel "eingerollter Rand"@de,
        "rolled rim"@en .

<http://id.acdh.oeaw.ac.at/defc/thesaurus/rounded_base/5.165> a skos:Concept ;
    dc:source "http://www.bible.ca/archeology/bible-archeology-pottery-glossary-dictionary-encyclopedia.htm" ;
    skos:broader <http://id.acdh.oeaw.ac.at/defc/thesaurus/base/4.032> ;
    skos:definition "A curved part of the vessel which provides support with a semicircular cross-section." ;
    skos:editorialNote "dc_finds_pottery_detail;165" ;
    skos:inScheme <http://id.acdh.oeaw.ac.at/defc/thesaurus/FindsPotteryDetail>,
        <http://id.acdh.oeaw.ac.at/defc/thesaurus/FindsSchema> ;
    skos:prefLabel "Runder Boden"@de,
        "rounded base"@en .

<http://id.acdh.oeaw.ac.at/defc/thesaurus/rusticated/5.208> a skos:Concept ;
    dc:source "Kipfer, B. A. Dictionary of Artifacts 2007. Blackwell Publishing, Oxford.p 275" ;
    skos:broader <http://id.acdh.oeaw.ac.at/defc/thesaurus/incised/4.168> ;
    skos:definition "Pottery with roughened surface which may or may not have an applied slip. The roughening may be achieved using fingers, fingernails, twigs, etc., and though it may be pure decoration, in most cases it is probably a device to prevent a greasy pot slipping" ;
    skos:editorialNote "dc_finds_pottery_decoration;208" ;
    skos:inScheme <http://id.acdh.oeaw.ac.at/defc/thesaurus/FindsPotteryDecoration>,
        <http://id.acdh.oeaw.ac.at/defc/thesaurus/FindsSchema> ;
    skos:prefLabel "rustiziert"@de,
        "rusticated"@en .

<http://id.acdh.oeaw.ac.at/defc/thesaurus/rye/5.17> a skos:Concept ;
    dc:source "http://eol.org/pages/1115159/overview" ;
    skos:broader <http://id.acdh.oeaw.ac.at/defc/thesaurus/cereal/4.022> ;
    skos:editorialNote "dc_botany_species;17" ;
    skos:inScheme <http://id.acdh.oeaw.ac.at/defc/thesaurus/BotanySpecies>,
        <http://id.acdh.oeaw.ac.at/defc/thesaurus/FindsSchema> ;
    skos:prefLabel "Roggen"@de,
        "rye"@en,
        "Secale cereale"@la .

<http://id.acdh.oeaw.ac.at/defc/thesaurus/sacral/5.17> a skos:Concept ;
    dc:source "https://en.oxforddictionaries.com/definition/sacral" ;
    skos:broader <http://id.acdh.oeaw.ac.at/defc/thesaurus/building_technique/4.075> ;
    skos:definition "A building related to sacred rites or symbols." ;
    skos:editorialNote "dc_area_buildingtechnique;17" ;
    skos:inScheme <http://id.acdh.oeaw.ac.at/defc/thesaurus/AreaBuildingtechnique>,
        <http://id.acdh.oeaw.ac.at/defc/thesaurus/AreaSchema> ;
    skos:prefLabel "sacral"@en .

<http://id.acdh.oeaw.ac.at/defc/thesaurus/sandstone/3.25> a skos:Concept ;
    dc:source "http://dbpedia.org/page/Sandstone" ;
    skos:broader <http://id.acdh.oeaw.ac.at/defc/thesaurus/stone/2.1> ;
    skos:definition "Sandstone (sometimes known as arenite) is a clastic sedimentary rock composed mainly of sand-sized minerals or rock grains." ;
    skos:editorialNote "dc_finds_material;25" ;
    skos:inScheme <http://id.acdh.oeaw.ac.at/defc/thesaurus/FindsMaterial>,
        <http://id.acdh.oeaw.ac.at/defc/thesaurus/FindsSchema> ;
    skos:prefLabel "Sandstein"@de,
        "sandstone"@en .

<http://id.acdh.oeaw.ac.at/defc/thesaurus/satellite_imaging/4.22> a skos:Concept ;
    dc:source "http://thesaurus.historicengland.org.uk/thesaurus_term.asp?thes_no=566&term_no=145162" ;
    skos:broader <http://id.acdh.oeaw.ac.at/defc/thesaurus/remote_sensing/3.056> ;
    skos:definition "The capture of imagery using an orbiting satellite. The type of imagery is very varied including visible light photography, infrared and multi spectral photography as well as imagery derived from radar and lidar data." ;
    skos:editorialNote "dc_researchevet_researchtype;22" ;
    skos:inScheme <http://id.acdh.oeaw.ac.at/defc/thesaurus/ResearchEventSchema>,
        <http://id.acdh.oeaw.ac.at/defc/thesaurus/ResearchevetResearchtype> ;
    skos:prefLabel "Satellitenbilderauswertung"@de,
        "satellite imaging"@en .

<http://id.acdh.oeaw.ac.at/defc/thesaurus/schist/3.26> a skos:Concept ;
    dc:source "http://dbpedia.org/page/Schist" ;
    skos:broader <http://id.acdh.oeaw.ac.at/defc/thesaurus/stone/2.1> ;
    skos:definition "A medium-grade metamorphic rock with medium to large, flat, sheet-like grains in a preferred orientation (nearby grains are roughly parallel). It is defined by having more than 50% platy and elongated minerals, often finely interleaved with quartz and fel" ;
    skos:editorialNote "dc_finds_material;26" ;
    skos:inScheme <http://id.acdh.oeaw.ac.at/defc/thesaurus/FindsMaterial>,
        <http://id.acdh.oeaw.ac.at/defc/thesaurus/FindsSchema> ;
    skos:prefLabel "Glimmerschiefer"@de,
        "schist"@en .

<http://id.acdh.oeaw.ac.at/defc/thesaurus/scoop/4.136> a skos:Concept ;
    dc:source "OREA" ;
    skos:broader <http://id.acdh.oeaw.ac.at/defc/thesaurus/pottery_form/3.016> ;
    skos:definition "A vessel used for scooping of liquids or solids." ;
    skos:editorialNote "dc_finds_pottery_form;136" ;
    skos:inScheme <http://id.acdh.oeaw.ac.at/defc/thesaurus/FindsPotteryForm>,
        <http://id.acdh.oeaw.ac.at/defc/thesaurus/FindsSchema> ;
    skos:prefLabel "Schöpfgefäß"@de,
        "scoop"@en .

<http://id.acdh.oeaw.ac.at/defc/thesaurus/scored/5.233> a skos:Concept ;
    dc:source "Cline, E. H. The Oxford Handbook of the Bronze Age Aegean. P. 407" ;
    skos:altLabel "wiped"@en,
        "wiped ware"@en ;
    skos:broader <http://id.acdh.oeaw.ac.at/defc/thesaurus/incised/4.168> ;
    skos:definition "The surface of the vessels is decorated with rough vertical, diagonal, or horizontal lines wiped in the moist clay." ;
    skos:editorialNote "dc_finds_pottery_decoration;233" ;
    skos:inScheme <http://id.acdh.oeaw.ac.at/defc/thesaurus/FindsPotteryDecoration>,
        <http://id.acdh.oeaw.ac.at/defc/thesaurus/FindsSchema> ;
    skos:prefLabel "Eingekerbt"@de,
        "scored"@en .

<http://id.acdh.oeaw.ac.at/defc/thesaurus/scraped_(a3ε)/4.159> a skos:Concept ;
    dc:source "http://www.ime.gr/chronos/01/en/nl/mn/mn_potfr.html" ;
    skos:broader <http://id.acdh.oeaw.ac.at/defc/thesaurus/pottery_surface_treatment/3.019> ;
    skos:definition "The whitish surface of the vessel is covered completely with a red colour, from which parallel bands are then scraped off. Typical for Thessaly and central Greece." ;
    skos:editorialNote "dc_finds_pottery_decoration;159" ;
    skos:inScheme <http://id.acdh.oeaw.ac.at/defc/thesaurus/FindsPotteryDecoration>,
        <http://id.acdh.oeaw.ac.at/defc/thesaurus/FindsSchema> ;
    skos:prefLabel "Ausgewischt (A3e)"@de,
        "scraped (a3ε)"@en .

<http://id.acdh.oeaw.ac.at/defc/thesaurus/scraper/4.74> a skos:Concept ;
    dc:source "Kipfer, B. A. Dictionary of Artifacts 2007. Blackwell Publishing, Oxford.p.282" ;
    skos:altLabel "bobbin"@en,
        "weaving bobbin"@en ;
    skos:broader <http://id.acdh.oeaw.ac.at/defc/thesaurus/tool/3.1> ;
    skos:definition "A retouched flake tool with a thick working edge; a flake tool that has been sharpened on one edge and left blunt on other edges to allow grasping, probably used to scrape (dress) animal hides." ;
    skos:editorialNote "dc_finds_small_finds_type;74" ;
    skos:inScheme <http://id.acdh.oeaw.ac.at/defc/thesaurus/FindsSchema>,
        <http://id.acdh.oeaw.ac.at/defc/thesaurus/FindsSmallFindsType> ;
    skos:prefLabel "Schaber"@de,
        "scraper"@en .

<http://id.acdh.oeaw.ac.at/defc/thesaurus/scribble_burnished/5.234> a skos:Concept ;
    dc:source "Vitelli 1993, 152" ;
    skos:broader <http://id.acdh.oeaw.ac.at/defc/thesaurus/burnished/4.297> ;
    skos:definition "MN Urfirnis ware with irregular burnishing lines typical for Southern Greece." ;
    skos:editorialNote "dc_finds_pottery_decoration;234" ;
    skos:inScheme <http://id.acdh.oeaw.ac.at/defc/thesaurus/FindsPotteryDecoration>,
        <http://id.acdh.oeaw.ac.at/defc/thesaurus/FindsSchema> ;
    skos:prefLabel "Geschmiergeglättet"@de,
        "scribble burnished"@en .

<http://id.acdh.oeaw.ac.at/defc/thesaurus/sea_club-rush/3.34> a skos:Concept ;
    dc:source "http://eol.org/pages/30089/overview" ;
    skos:broader <http://id.acdh.oeaw.ac.at/defc/thesaurus/botany/2.2> ;
    skos:editorialNote "dc_botany_species;34" ;
    skos:inScheme <http://id.acdh.oeaw.ac.at/defc/thesaurus/BotanySpecies>,
        <http://id.acdh.oeaw.ac.at/defc/thesaurus/FindsSchema> ;
    skos:prefLabel "Strandbinse"@de,
        "sea club-rush"@en,
        "Schoenoplectus"@la .

<http://id.acdh.oeaw.ac.at/defc/thesaurus/seal/4.62> a skos:Concept ;
    dc:source "Kipfer, B. A. Dictionary of Artifacts 2007. Blackwell Publishing, Oxford.p.284" ;
    skos:broader <http://id.acdh.oeaw.ac.at/defc/thesaurus/tool/3.1> ;
    skos:definition "A device for impressing characteristic marks into a soft surface, such as wet clay or wax, to indicate ownership or authenticity. Seals were made of bone, ivory, stone, or wood and had an intaglio design and were in the form of stamps or cylinder seals." ;
    skos:editorialNote "dc_finds_small_finds_type;62" ;
    skos:inScheme <http://id.acdh.oeaw.ac.at/defc/thesaurus/FindsSchema>,
        <http://id.acdh.oeaw.ac.at/defc/thesaurus/FindsSmallFindsType> ;
    skos:prefLabel "Siegel"@de,
        "seal"@en .

<http://id.acdh.oeaw.ac.at/defc/thesaurus/secondary_deposition/6.3> a skos:Concept ;
    skos:broader <http://id.acdh.oeaw.ac.at/defc/thesaurus/human_remains_type/5.096> ;
    skos:editorialNote "dc_area_typeofhumanremains;3" ;
    skos:inScheme <http://id.acdh.oeaw.ac.at/defc/thesaurus/AreaSchema>,
        <http://id.acdh.oeaw.ac.at/defc/thesaurus/AreaTypeofhumanremains> ;
    skos:prefLabel "secondary deposition"@en .

<http://id.acdh.oeaw.ac.at/defc/thesaurus/seed/4.4> a skos:Concept ;
    dc:source "Kipfer, B. A. Encyclopedic Dictionary of Archaeology. Kluwer Academic/Plenum Publishers, New York. P.502" ;
    skos:broader <http://id.acdh.oeaw.ac.at/defc/thesaurus/dating_material/3.046> ;
    skos:definition "A variety of seeds may be preserved on archaeologcal sites by charring, grain impressions, or as a result of waterlogging. They may be the seeds of weed plants, fruits, pulses, or the grains of cereals." ;
    skos:editorialNote "dc_period_datedby;4" ;
    skos:inScheme <http://id.acdh.oeaw.ac.at/defc/thesaurus/PeriodSchema> ;
    skos:prefLabel "Samen"@de,
        "seed"@en .

<http://id.acdh.oeaw.ac.at/defc/thesaurus/segment/4.18> a skos:Concept ;
    dc:source "Inizan, M.-L., M. Reduron-Ballinger, H. Roche, J. Tixier 1999, Technology and Terminology of Knapped Stone. Nanterre: CREP., D. Srejovic (ed) 1997, Arheološki Leksikon." ;
    skos:altLabel "lunate"@en ;
    skos:broader <http://id.acdh.oeaw.ac.at/defc/thesaurus/retouched_tool/3.010> ;
    skos:definition "A geometric microlith, made on a blade or bladelet and shaped like a half moon; the backing is along a curved arc opposite a straight unretouched edge. It was hafted, possibly as a projectile tip or as part of a cutting tool." ;
    skos:editorialNote "dc_finds_lithics_retouched_tools;18" ;
    skos:inScheme <http://id.acdh.oeaw.ac.at/defc/thesaurus/FindsLithicsRetouchedTools>,
        <http://id.acdh.oeaw.ac.at/defc/thesaurus/FindsSchema> ;
    skos:prefLabel "segment"@en .

<http://id.acdh.oeaw.ac.at/defc/thesaurus/senile_(60-)/6.9> a skos:Concept ;
    skos:broader <http://id.acdh.oeaw.ac.at/defc/thesaurus/age_group/5.097> ;
    skos:editorialNote "dc_area_agegroups;9" ;
    skos:inScheme <http://id.acdh.oeaw.ac.at/defc/thesaurus/AreaAgegroups>,
        <http://id.acdh.oeaw.ac.at/defc/thesaurus/AreaSchema> ;
    skos:prefLabel "senile (60-)"@en .

<http://id.acdh.oeaw.ac.at/defc/thesaurus/separating_wall/5.2> a skos:Concept ;
    skos:broader <http://id.acdh.oeaw.ac.at/defc/thesaurus/morturary_feature/4.086> ;
    skos:editorialNote "dc_area_mortuaryfeatures;2" ;
    skos:inScheme <http://id.acdh.oeaw.ac.at/defc/thesaurus/AreaMortuaryfeatures>,
        <http://id.acdh.oeaw.ac.at/defc/thesaurus/AreaSchema> ;
    skos:prefLabel "trennende Mauer"@de,
        "separating wall"@en .

<http://id.acdh.oeaw.ac.at/defc/thesaurus/serpentine/3.23> a skos:Concept ;
    dc:source "https://en.wikipedia.org/wiki/Serpentine_subgroup" ;
    skos:broader <http://id.acdh.oeaw.ac.at/defc/thesaurus/mineral/2.3> ;
    skos:definition "The serpentine subgroup (part of the kaolinite-serpentine group) are greenish, brownish, or spotted minerals commonly found in serpentinite rocks." ;
    skos:editorialNote "dc_finds_material;23" ;
    skos:inScheme <http://id.acdh.oeaw.ac.at/defc/thesaurus/FindsMaterial>,
        <http://id.acdh.oeaw.ac.at/defc/thesaurus/FindsSchema> ;
    skos:prefLabel "Serpentin"@de,
        "serpentine"@en .

<http://id.acdh.oeaw.ac.at/defc/thesaurus/sex_not_specified/6.3> a skos:Concept ;
    dc:source "OREA" ;
    skos:broader <http://id.acdh.oeaw.ac.at/defc/thesaurus/sex/5.095> ;
    skos:definition "The sex of the found human remains was not determined or could not be specified." ;
    skos:editorialNote "dc_area_sexes;3" ;
    skos:inScheme <http://id.acdh.oeaw.ac.at/defc/thesaurus/AreaSchema>,
        <http://id.acdh.oeaw.ac.at/defc/thesaurus/AreaSexes> ;
    skos:prefLabel "nicht bestimmt"@de,
        "sex not specified"@en .

<http://id.acdh.oeaw.ac.at/defc/thesaurus/shaft_grave/5.5> a skos:Concept ;
    dc:source "Kipfer, B. A. Encyclopedic Dictionary of Archaeology. Kluwer Academic/Plenum Publishers, New York." ;
    skos:altLabel "shaft tomb"@en ;
    skos:broader <http://id.acdh.oeaw.ac.at/defc/thesaurus/grave_type/4.083> ;
    skos:definition "A grave in which the burial chamber was reached by a vertical shaft, the burials themselves placed at the bottom of a deep narrow pit. The tomb was usually rectangular, and the burial chamber was roofed and the shaft above it filled in." ;
    skos:editorialNote "dc_area_gravetype;5" ;
    skos:inScheme <http://id.acdh.oeaw.ac.at/defc/thesaurus/AreaGravetype>,
        <http://id.acdh.oeaw.ac.at/defc/thesaurus/AreaSchema> ;
    skos:prefLabel "Schachtgrab"@de,
        "shaft grave"@en .

<http://id.acdh.oeaw.ac.at/defc/thesaurus/shaft_straightener/4.95> a skos:Concept ;
    dc:source "Kipfer, B. A. Dictionary of Artifacts 2007. Blackwell Publishing, Oxford.p.287" ;
    skos:altLabel "Schaftstrecker"@de ;
    skos:broader <http://id.acdh.oeaw.ac.at/defc/thesaurus/tool/3.1> ;
    skos:definition "An artifact made from a coarse, often volcanic, stone, with a groove used as a rasp to finish spears and arrowshafts." ;
    skos:editorialNote "dc_finds_small_finds_type;95" ;
    skos:inScheme <http://id.acdh.oeaw.ac.at/defc/thesaurus/FindsSchema>,
        <http://id.acdh.oeaw.ac.at/defc/thesaurus/FindsSmallFindsType> ;
    skos:prefLabel "Schaftglätter"@de,
        "shaft straightener"@en .

<http://id.acdh.oeaw.ac.at/defc/thesaurus/shallow_bowl/5.116> a skos:Concept ;
    dc:source "OREA" ;
    skos:broader <http://id.acdh.oeaw.ac.at/defc/thesaurus/bowl/4.115> ;
    skos:definition "A low open vessel with a rim diameter double than the height." ;
    skos:editorialNote "dc_finds_pottery_form;116" ;
    skos:inScheme <http://id.acdh.oeaw.ac.at/defc/thesaurus/FindsPotteryForm>,
        <http://id.acdh.oeaw.ac.at/defc/thesaurus/FindsSchema> ;
    skos:prefLabel "Schale"@de,
        "shallow bowl"@en .

<http://id.acdh.oeaw.ac.at/defc/thesaurus/sheep/5.6> a skos:Concept ;
    dc:source "http://eol.org/pages/311906/overview" ;
    skos:broader <http://id.acdh.oeaw.ac.at/defc/thesaurus/mammal/4.020> ;
    skos:editorialNote "dc_finds_animal_remains_species;6" ;
    skos:inScheme <http://id.acdh.oeaw.ac.at/defc/thesaurus/FindsAnimalRemainsSpecies>,
        <http://id.acdh.oeaw.ac.at/defc/thesaurus/FindsSchema> ;
    skos:prefLabel "Schaf"@de,
        "sheep"@en,
        "Ovis aries"@la .

<http://id.acdh.oeaw.ac.at/defc/thesaurus/sheep/goat/5.5> a skos:Concept ;
    skos:broader <http://id.acdh.oeaw.ac.at/defc/thesaurus/mammal/4.020> ;
    skos:editorialNote "dc_finds_animal_remains_species;5" ;
    skos:inScheme <http://id.acdh.oeaw.ac.at/defc/thesaurus/FindsAnimalRemainsSpecies>,
        <http://id.acdh.oeaw.ac.at/defc/thesaurus/FindsSchema> ;
    skos:prefLabel "Schaf/Ziege"@de,
        "sheep/goat"@en,
        "Ovis/Capra"@la .

<http://id.acdh.oeaw.ac.at/defc/thesaurus/shell_production/2.5> a skos:Concept ;
    skos:broader <http://id.acdh.oeaw.ac.at/defc/thesaurus/production/1.042> ;
    skos:editorialNote "dc_interpretation_productiontype;5" ;
    skos:inScheme <http://id.acdh.oeaw.ac.at/defc/thesaurus/InterpretationProductiontype>,
        <http://id.acdh.oeaw.ac.at/defc/thesaurus/InterpretationSchema> ;
    skos:prefLabel "Muschelverarbeitung"@de,
        "shell production"@en .

<http://id.acdh.oeaw.ac.at/defc/thesaurus/shell_stamped/5.209> a skos:Concept ;
    dc:source "OREA" ;
    skos:altLabel "cardium ware"@en ;
    skos:broader <http://id.acdh.oeaw.ac.at/defc/thesaurus/incised/4.168> ;
    skos:definition "Pottery decorated with imprints of marine mollusc shell (cockle-cerastoderma edule)" ;
    skos:editorialNote "dc_finds_pottery_decoration;209" ;
    skos:inScheme <http://id.acdh.oeaw.ac.at/defc/thesaurus/FindsPotteryDecoration>,
        <http://id.acdh.oeaw.ac.at/defc/thesaurus/FindsSchema> ;
    skos:prefLabel "Mit einer Muschel gestempelt"@de,
        "shell stamped"@en .

<http://id.acdh.oeaw.ac.at/defc/thesaurus/shouldered_bowl/5.156> a skos:Concept ;
    dc:source "Hauptmann - Milojcic 1969" ;
    skos:broader <http://id.acdh.oeaw.ac.at/defc/thesaurus/bowl/4.115> ;
    skos:definition "Bowl with strong carination in its upper part typical for Thessaly." ;
    skos:editorialNote "dc_finds_pottery_form;156" ;
    skos:inScheme <http://id.acdh.oeaw.ac.at/defc/thesaurus/FindsPotteryForm>,
        <http://id.acdh.oeaw.ac.at/defc/thesaurus/FindsSchema> ;
    skos:prefLabel "Schulterschale"@de,
        "shouldered bowl"@en .

<http://id.acdh.oeaw.ac.at/defc/thesaurus/shuttle/5.75> a skos:Concept ;
    dc:source "http://www.dictionary.com/browse/shuttle?s=t" ;
    skos:broader <http://id.acdh.oeaw.ac.at/defc/thesaurus/textile_equipment/4.028> ;
    skos:definition "A device in a loom for passing or shooting the weft thread through the shed from one side of the web to the other, usually consisting of a boat-shaped piece of wood containing a bobbin on which the weft thread is wound." ;
    skos:editorialNote "dc_finds_small_finds_type;75" ;
    skos:inScheme <http://id.acdh.oeaw.ac.at/defc/thesaurus/FindsSchema>,
        <http://id.acdh.oeaw.ac.at/defc/thesaurus/FindsSmallFindsType> ;
    skos:prefLabel "Weberschiffchen"@de,
        "shuttle"@en .

<http://id.acdh.oeaw.ac.at/defc/thesaurus/sickle_blade/4.19> a skos:Concept ;
    dc:source "Inizan, M.-L., M. Reduron-Ballinger, H. Roche, J. Tixier 1999, Technology and Terminology of Knapped Stone. Nanterre: CREP., D. Srejovic (ed) 1997, Arheološki Leksikon." ;
    skos:broader <http://id.acdh.oeaw.ac.at/defc/thesaurus/retouched_tool/3.010> ;
    skos:definition "A blade (rarely flake) with the gloss which occurs on the edge of the artefact, and which is caused by the wear of the blade against the phytoliths in the grasses being reaped. Usually inserted in a bone, antler or wooden handle, as a part of composite to" ;
    skos:editorialNote "dc_finds_lithics_retouched_tools;19" ;
    skos:inScheme <http://id.acdh.oeaw.ac.at/defc/thesaurus/FindsLithicsRetouchedTools>,
        <http://id.acdh.oeaw.ac.at/defc/thesaurus/FindsSchema> ;
    skos:prefLabel "sickle blade"@en .

<http://id.acdh.oeaw.ac.at/defc/thesaurus/sickle_implement/4.107> a skos:Concept ;
    dc:source "Kipfer, B. A. Dictionary of Artifacts 2007. Blackwell Publishing, Oxford.p 290" ;
    skos:altLabel "sickle"@en,
        "sickle element"@en ;
    skos:broader <http://id.acdh.oeaw.ac.at/defc/thesaurus/tool/3.1> ;
    skos:definition "A knife for reaping corn, first used by Neolithic man, made of flint blades mounted in a wooden or bone haft." ;
    skos:editorialNote "dc_finds_small_finds_type;107" ;
    skos:inScheme <http://id.acdh.oeaw.ac.at/defc/thesaurus/FindsSchema>,
        <http://id.acdh.oeaw.ac.at/defc/thesaurus/FindsSmallFindsType> ;
    skos:prefLabel "Sichel"@de,
        "sickle implement"@en .

<http://id.acdh.oeaw.ac.at/defc/thesaurus/side-scraper/4.20> a skos:Concept ;
    dc:source "Inizan, M.-L., M. Reduron-Ballinger, H. Roche, J. Tixier 1999, Technology and Terminology of Knapped Stone. Nanterre: CREP., D. Srejovic (ed) 1997, Arheološki Leksikon." ;
    skos:altLabel "side scraper"@en ;
    skos:broader <http://id.acdh.oeaw.ac.at/defc/thesaurus/retouched_tool/3.010> ;
    skos:definition "A tool with a retouch on one or both lateral edge of a flake." ;
    skos:editorialNote "dc_finds_lithics_retouched_tools;20" ;
    skos:inScheme <http://id.acdh.oeaw.ac.at/defc/thesaurus/FindsLithicsRetouchedTools>,
        <http://id.acdh.oeaw.ac.at/defc/thesaurus/FindsSchema> ;
    skos:prefLabel "Schaber"@de,
        "side-scraper"@en .

<http://id.acdh.oeaw.ac.at/defc/thesaurus/sieve/4.117> a skos:Concept ;
    dc:source "OREA" ;
    skos:broader <http://id.acdh.oeaw.ac.at/defc/thesaurus/pottery_form/3.016> ;
    skos:definition "A container whose walls are completely or partially pierced used for separating liquids and solids." ;
    skos:editorialNote "dc_finds_pottery_form;117" ;
    skos:inScheme <http://id.acdh.oeaw.ac.at/defc/thesaurus/FindsPotteryForm>,
        <http://id.acdh.oeaw.ac.at/defc/thesaurus/FindsSchema> ;
    skos:prefLabel "Sieb"@de,
        "sieve"@en .

<http://id.acdh.oeaw.ac.at/defc/thesaurus/silver/5.9> a skos:Concept ;
    dc:source "https://www.britannica.com/science/silver" ;
    skos:broader <http://id.acdh.oeaw.ac.at/defc/thesaurus/metal/4.7> ;
    skos:definition "Silver (Ag), chemical element, a white, lustrous metal valued for its decorative beauty and electrical conductivity. Extracted from a quarry site." ;
    skos:editorialNote "dc_area_rawmaterial;9" ;
    skos:inScheme <http://id.acdh.oeaw.ac.at/defc/thesaurus/AreaRawmaterial>,
        <http://id.acdh.oeaw.ac.at/defc/thesaurus/AreaSchema> ;
    skos:prefLabel "Silber"@de,
        "silver"@en .

<http://id.acdh.oeaw.ac.at/defc/thesaurus/single_jabbed/5.235> a skos:Concept ;
    dc:source "Tomkins 2007" ;
    skos:broader <http://id.acdh.oeaw.ac.at/defc/thesaurus/incised/4.168> ;
    skos:definition "Ware decorated with single engraved lines." ;
    skos:editorialNote "dc_finds_pottery_decoration;235" ;
    skos:inScheme <http://id.acdh.oeaw.ac.at/defc/thesaurus/FindsPotteryDecoration>,
        <http://id.acdh.oeaw.ac.at/defc/thesaurus/FindsSchema> ;
    skos:prefLabel "Einzeln eingedrückter Musterdekor"@de,
        "single jabbed"@en .

<http://id.acdh.oeaw.ac.at/defc/thesaurus/skull/5.1> a skos:Concept ;
    dc:source "https://en.oxforddictionaries.com/definition/skull" ;
    skos:broader <http://id.acdh.oeaw.ac.at/defc/thesaurus/bone/4.021> ;
    skos:definition "A bone framework enclosing the brain of a vertebrate; the skeleton of a person's or animal's head." ;
    skos:editorialNote "dc_animal_remains_part;1" ;
    skos:inScheme <http://id.acdh.oeaw.ac.at/defc/thesaurus/AnimalRemainsPart>,
        <http://id.acdh.oeaw.ac.at/defc/thesaurus/FindsSchema> ;
    skos:prefLabel "skull"@en,
        "cranium"@la .

<http://id.acdh.oeaw.ac.at/defc/thesaurus/skyphos/4.157> a skos:Concept ;
    dc:source "OREA" ;
    skos:broader <http://id.acdh.oeaw.ac.at/defc/thesaurus/pottery_form/3.016> ;
    skos:definition "A two-handled deep drinking cup." ;
    skos:editorialNote "dc_finds_pottery_form;157" ;
    skos:inScheme <http://id.acdh.oeaw.ac.at/defc/thesaurus/FindsPotteryForm>,
        <http://id.acdh.oeaw.ac.at/defc/thesaurus/FindsSchema> ;
    skos:prefLabel "Skyphos"@de,
        "skyphos"@en .

<http://id.acdh.oeaw.ac.at/defc/thesaurus/slingstone/5.53> a skos:Concept ;
    dc:source "http://dbpedia.org/page/Sling_(weapon)" ;
    skos:altLabel "sling bullet"@en ;
    skos:broader <http://id.acdh.oeaw.ac.at/defc/thesaurus/weapon/4.030> ;
    skos:definition "A stone used as a blunt projectile with a sling." ;
    skos:editorialNote "dc_finds_small_finds_type;53" ;
    skos:inScheme <http://id.acdh.oeaw.ac.at/defc/thesaurus/FindsSchema>,
        <http://id.acdh.oeaw.ac.at/defc/thesaurus/FindsSmallFindsType> ;
    skos:prefLabel "Schleudergeschoss"@de,
        "slingstone"@en .

<http://id.acdh.oeaw.ac.at/defc/thesaurus/small_foot/5.167> a skos:Concept ;
    dc:source "OREA" ;
    skos:broader <http://id.acdh.oeaw.ac.at/defc/thesaurus/foot/4.71> ;
    skos:definition "A small supporting lower part of the vessel, normally attached to the base or vessel bottom after the vessel has got its form." ;
    skos:editorialNote "dc_finds_pottery_detail;167" ;
    skos:inScheme <http://id.acdh.oeaw.ac.at/defc/thesaurus/FindsPotteryDetail>,
        <http://id.acdh.oeaw.ac.at/defc/thesaurus/FindsSchema> ;
    skos:prefLabel "Kleiner Fuß"@de,
        "small foot"@en .

<http://id.acdh.oeaw.ac.at/defc/thesaurus/small_ring_handle/6.102> a skos:Concept ;
    dc:source "OREA" ;
    skos:broader <http://id.acdh.oeaw.ac.at/defc/thesaurus/ring_handle/5.100> ;
    skos:definition "A handle with a very small round loop." ;
    skos:editorialNote "dc_finds_pottery_detail;102" ;
    skos:inScheme <http://id.acdh.oeaw.ac.at/defc/thesaurus/FindsPotteryDetail>,
        <http://id.acdh.oeaw.ac.at/defc/thesaurus/FindsSchema> ;
    skos:prefLabel "kleiner Ringhenkel"@de,
        "small ring handle"@en .

<http://id.acdh.oeaw.ac.at/defc/thesaurus/smeared/4.260> a skos:Concept ;
    dc:source "OREA" ;
    skos:altLabel "smooth ware"@de ;
    skos:broader <http://id.acdh.oeaw.ac.at/defc/thesaurus/pottery_surface_treatment/3.019> ;
    skos:definition "Middle Helladic smeared ware." ;
    skos:editorialNote "dc_finds_pottery_decoration;260" ;
    skos:inScheme <http://id.acdh.oeaw.ac.at/defc/thesaurus/FindsPotteryDecoration>,
        <http://id.acdh.oeaw.ac.at/defc/thesaurus/FindsSchema> ;
    skos:prefLabel "Geschmiert"@de,
        "smeared"@en .

<http://id.acdh.oeaw.ac.at/defc/thesaurus/smoothed/4.261> a skos:Concept ;
    dc:source "Horvat, M. 1999, Keramika. Tehnologija keramike, tipologija lonöenine, keramiöni arhiv. Filozofska fakulteta, Ljubljana. P. 25" ;
    skos:broader <http://id.acdh.oeaw.ac.at/defc/thesaurus/pottery_surface_treatment/3.019> ;
    skos:definition "Vessel that has been smoothed when still wet before drying and firing. The surface is wiped without additional use of water. Traces of wiping direction can be often observed." ;
    skos:editorialNote "dc_finds_pottery_decoration;261" ;
    skos:inScheme <http://id.acdh.oeaw.ac.at/defc/thesaurus/FindsPotteryDecoration>,
        <http://id.acdh.oeaw.ac.at/defc/thesaurus/FindsSchema> ;
    skos:prefLabel "Glatt gestrichen"@de,
        "smoothed"@en .

<http://id.acdh.oeaw.ac.at/defc/thesaurus/soil_analysis%3A_particle_size_analysis%2F3.23> a skos:Concept ;
    dc:source "http://thesaurus.historicengland.org.uk/thesaurus_term.asp?thes_no=56&term_no=142179" ;
    skos:altLabel "particle size analysis"@en ;
    skos:broader <http://id.acdh.oeaw.ac.at/defc/thesaurus/soil_analysis/2.063> ;
    skos:definition "The analysis of the distribution and proportion of sand, silt and clay in a deposit." ;
    skos:editorialNote "dc_researchevent_special_analysis;23" ;
    skos:inScheme <http://id.acdh.oeaw.ac.at/defc/thesaurus/ResearchEventSchema>,
        <http://id.acdh.oeaw.ac.at/defc/thesaurus/ResearcheventSpecialAnalysis> ;
    skos:prefLabel "Korngrößenanalyse"@de,
        "soil analysis: particle size analysis"@en .

<http://id.acdh.oeaw.ac.at/defc/thesaurus/soil_analysis%3A_soil_chemistry%2F3.24> a skos:Concept ;
    dc:source "http://oxfordindex.oup.com/view/1.193/oi/authority.21183151659?rskey=A9d7Zt&result=&q=soil%2chemistry" ;
    skos:altLabel "soil chemistry"@en ;
    skos:broader <http://id.acdh.oeaw.ac.at/defc/thesaurus/soil_analysis/2.063> ;
    skos:definition "The study of the chemical composition and properties of soils and archaeological deposits in order to determine the nature and extent of activities within the area examined." ;
    skos:editorialNote "dc_researchevent_special_analysis;24" ;
    skos:inScheme <http://id.acdh.oeaw.ac.at/defc/thesaurus/ResearchEventSchema>,
        <http://id.acdh.oeaw.ac.at/defc/thesaurus/ResearcheventSpecialAnalysis> ;
    skos:prefLabel "Bodenchemie"@de,
        "soil analysis: soil chemistry"@en .

<http://id.acdh.oeaw.ac.at/defc/thesaurus/soil_analysis%3A_soil_micromorphology%2F3.25> a skos:Concept ;
    dc:source "http://www.britac.ac.uk/pubs/proc/files/77p39.pdf" ;
    skos:altLabel " micromorphology"@en,
        "soil micromorphology"@en ;
    skos:broader <http://id.acdh.oeaw.ac.at/defc/thesaurus/soil_analysis/2.063> ;
    skos:definition "Soil micromorphology consits of the integrated use of various microscopic techniques for studying the arrangement and the nature othat form sediments and soils to provide information which can discriminate the sedimentary signatures diagnostic of human-re" ;
    skos:editorialNote "dc_researchevent_special_analysis;25" ;
    skos:inScheme <http://id.acdh.oeaw.ac.at/defc/thesaurus/ResearchEventSchema>,
        <http://id.acdh.oeaw.ac.at/defc/thesaurus/ResearcheventSpecialAnalysis> ;
    skos:prefLabel "Mikromorphologie"@de,
        "soil analysis: soil micromorphology"@en .

<http://id.acdh.oeaw.ac.at/defc/thesaurus/soil_analysis%3A_soil_phosphorus_analysis%2F3.26> a skos:Concept ;
    dc:source "http://thesaurus.historicengland.org.uk/thesaurus_term.asp?thes_no=56&term_no=142197" ;
    skos:altLabel "soil phosphorus analysis"@en ;
    skos:broader <http://id.acdh.oeaw.ac.at/defc/thesaurus/soil_analysis/2.063> ;
    skos:definition "The analysis of the amount of phosphorus (P) present in a soil." ;
    skos:editorialNote "dc_researchevent_special_analysis;26" ;
    skos:inScheme <http://id.acdh.oeaw.ac.at/defc/thesaurus/ResearchEventSchema>,
        <http://id.acdh.oeaw.ac.at/defc/thesaurus/ResearcheventSpecialAnalysis> ;
    skos:prefLabel "Phosphoranalyse"@de,
        "soil analysis: soil phosphorus analysis"@en .

<http://id.acdh.oeaw.ac.at/defc/thesaurus/spatula/4.55> a skos:Concept ;
    dc:source "Kipfer, B. A. Dictionary of Artifacts 2007. Blackwell Publishing, Oxford.p.297" ;
    skos:broader <http://id.acdh.oeaw.ac.at/defc/thesaurus/tool/3.1> ;
    skos:definition "A tool, usually of bone, lime, wood, ebony, turtleshell, etc., consisting of a broad but thin blade. It served many general purposes – spreading, mixing, scooping, lifting – including burnishing pottery, workworking pelts, spooning flour, etc." ;
    skos:editorialNote "dc_finds_small_finds_type;55" ;
    skos:inScheme <http://id.acdh.oeaw.ac.at/defc/thesaurus/FindsSchema>,
        <http://id.acdh.oeaw.ac.at/defc/thesaurus/FindsSmallFindsType> ;
    skos:prefLabel "Spatula"@de,
        "spatula"@en .

<http://id.acdh.oeaw.ac.at/defc/thesaurus/spear/5.113> a skos:Concept ;
    dc:source "Kipfer, B. A. Dictionary of Artifacts 2007. Blackwell Publishing, Oxford.p 298" ;
    skos:altLabel "Lanze"@de ;
    skos:broader <http://id.acdh.oeaw.ac.at/defc/thesaurus/weapon/4.030> ;
    skos:definition "A pole weapon with a sharp point, either thrown or thrust at an enemy or prey." ;
    skos:editorialNote "dc_finds_small_finds_type;113" ;
    skos:inScheme <http://id.acdh.oeaw.ac.at/defc/thesaurus/FindsSchema>,
        <http://id.acdh.oeaw.ac.at/defc/thesaurus/FindsSmallFindsType> ;
    skos:prefLabel "Speer"@de,
        "spear"@en .

<http://id.acdh.oeaw.ac.at/defc/thesaurus/spindle_whorl/5.56> a skos:Concept ;
    dc:source "Kipfer, B. A. Dictionary of Artifacts 2007. Blackwell Publishing, Oxford.p.299" ;
    skos:broader <http://id.acdh.oeaw.ac.at/defc/thesaurus/textile_equipment/4.028> ;
    skos:definition "A circular object with a central perforation intended to act as a fly wheel on a spindle, giving momentum to its rotation – an artifact providing evidence of the spinning of thread. It maintained the momentum of the spindle rotated by the spinner while he" ;
    skos:editorialNote "dc_finds_small_finds_type;56" ;
    skos:inScheme <http://id.acdh.oeaw.ac.at/defc/thesaurus/FindsSchema>,
        <http://id.acdh.oeaw.ac.at/defc/thesaurus/FindsSmallFindsType> ;
    skos:prefLabel "Spinnwirtel"@de,
        "spindle whorl"@en .

<http://id.acdh.oeaw.ac.at/defc/thesaurus/splinter/4.21> a skos:Concept ;
    dc:source "Inizan, M.-L., M. Reduron-Ballinger, H. Roche, J. Tixier 1999, Technology and Terminology of Knapped Stone. Nanterre: CREP., D. Srejovic (ed) 1997, Arheološki Leksikon." ;
    skos:altLabel "Non-flake"@en ;
    skos:broader <http://id.acdh.oeaw.ac.at/defc/thesaurus/retouched_tool/3.010> ;
    skos:definition "A type of chipped stone artifact manufactured by the bipolar percussion technique, used for spliting a wood on two pieces. synonym: piece esquillee." ;
    skos:editorialNote "dc_finds_lithics_retouched_tools;21" ;
    skos:inScheme <http://id.acdh.oeaw.ac.at/defc/thesaurus/FindsLithicsRetouchedTools>,
        <http://id.acdh.oeaw.ac.at/defc/thesaurus/FindsSchema> ;
    skos:prefLabel "Trümmer"@de,
        "splinter"@en .

<http://id.acdh.oeaw.ac.at/defc/thesaurus/spondylus_shell/4.4> a skos:Concept ;
    dc:source "http://dbpedia.org/page/Spondylus" ;
    skos:broader <http://id.acdh.oeaw.ac.at/defc/thesaurus/shell/3.6> ;
    skos:definition "Spondylus is a genus of bivalve molluscs, the only genus in the family Spondylidae." ;
    skos:editorialNote "dc_finds_material;4" ;
    skos:inScheme <http://id.acdh.oeaw.ac.at/defc/thesaurus/FindsMaterial>,
        <http://id.acdh.oeaw.ac.at/defc/thesaurus/FindsSchema> ;
    skos:prefLabel "Stachelaustern"@de,
        "spondylus shell"@en .

<http://id.acdh.oeaw.ac.at/defc/thesaurus/spongy/4.244> a skos:Concept ;
    dc:source "Biers, W. R. 1969. Excavations at Phlius, 1924 the prehistoric deposits. Hesperia: The journal of the American School of Classical Studies at Athens. Vol. 38, No.4. pp. 443-458. P. 446" ;
    skos:altLabel "spongy ware"@de ;
    skos:broader <http://id.acdh.oeaw.ac.at/defc/thesaurus/pottery_surface_treatment/3.019> ;
    skos:definition "The fabric of a spongy vessel is quite coarse and contains many inclusions of limestone and plant matter which exploded or burnt out upon firing, leaving the surface pitted." ;
    skos:editorialNote "dc_finds_pottery_decoration;244" ;
    skos:inScheme <http://id.acdh.oeaw.ac.at/defc/thesaurus/FindsPotteryDecoration>,
        <http://id.acdh.oeaw.ac.at/defc/thesaurus/FindsSchema> ;
    skos:prefLabel "Spongy"@de,
        "spongy"@en .

<http://id.acdh.oeaw.ac.at/defc/thesaurus/spoon/4.48> a skos:Concept ;
    dc:source "Kipfer, B. A. Dictionary of Artifacts 2007. Blackwell Publishing, Oxford.p.300." ;
    skos:broader <http://id.acdh.oeaw.ac.at/defc/thesaurus/tool/3.1> ;
    skos:definition "An implement consisting of a small, shallow oval or round bowl on a long handle, used for eating, stirring, and serving food." ;
    skos:editorialNote "dc_finds_small_finds_type;48" ;
    skos:inScheme <http://id.acdh.oeaw.ac.at/defc/thesaurus/FindsSchema>,
        <http://id.acdh.oeaw.ac.at/defc/thesaurus/FindsSmallFindsType> ;
    skos:prefLabel "Löffel"@de,
        "spoon"@en .

<http://id.acdh.oeaw.ac.at/defc/thesaurus/square/5.30> a skos:Concept ;
    dc:source "https://standards.phorio.com/?t=definition&code=5935638133" ;
    skos:altLabel "plaza"@en ;
    skos:broader <http://id.acdh.oeaw.ac.at/defc/thesaurus/place/4.082> ;
    skos:definition "An open paved area within a street system, traditionally used for open markets or large gatherings of people." ;
    skos:editorialNote "dc_area_specialfeatures;30" ;
    skos:inScheme <http://id.acdh.oeaw.ac.at/defc/thesaurus/AreaSchema>,
        <http://id.acdh.oeaw.ac.at/defc/thesaurus/AreaSpecialfeatures> ;
    skos:prefLabel "square"@en .

<http://id.acdh.oeaw.ac.at/defc/thesaurus/stairway/5.17> a skos:Concept ;
    dc:source "OREA" ;
    skos:broader <http://id.acdh.oeaw.ac.at/defc/thesaurus/architecture/4.081> ;
    skos:definition "A set of steps or stairs leading to an upper storey." ;
    skos:editorialNote "dc_area_specialfeatures;17" ;
    skos:inScheme <http://id.acdh.oeaw.ac.at/defc/thesaurus/AreaSchema>,
        <http://id.acdh.oeaw.ac.at/defc/thesaurus/AreaSpecialfeatures> ;
    skos:prefLabel "stairway"@en .

<http://id.acdh.oeaw.ac.at/defc/thesaurus/stand/4.169> a skos:Concept ;
    dc:source "http://www.bible.ca/archeology/bible-archeology-pottery-glossary-dictionary-encyclopedia.htm" ;
    skos:broader <http://id.acdh.oeaw.ac.at/defc/thesaurus/pottery_form/3.016> ;
    skos:definition "A ceramic collar placed under a round or pointed bottom vessel in order to support or stabilize the vessel." ;
    skos:editorialNote "dc_finds_pottery_form;169" ;
    skos:inScheme <http://id.acdh.oeaw.ac.at/defc/thesaurus/FindsPotteryForm>,
        <http://id.acdh.oeaw.ac.at/defc/thesaurus/FindsSchema> ;
    skos:prefLabel "Ständer"@de,
        "stand"@en .

<http://id.acdh.oeaw.ac.at/defc/thesaurus/stele/5.31> a skos:Concept ;
    dc:source "Kipfer, B. A. Encyclopedic Dictionary of Archaeology. Kluwer Academic/Plenum Publishers, New York." ;
    skos:altLabel "Stele"@de ;
    skos:broader <http://id.acdh.oeaw.ac.at/defc/thesaurus/ritual/4.079> ;
    skos:definition "An upright, freestanding monumne, often inscribed and used for funerary or commemorative purposes." ;
    skos:editorialNote "dc_area_specialfeatures;31" ;
    skos:inScheme <http://id.acdh.oeaw.ac.at/defc/thesaurus/AreaSchema>,
        <http://id.acdh.oeaw.ac.at/defc/thesaurus/AreaSpecialfeatures> ;
    skos:prefLabel "stele"@en .

<http://id.acdh.oeaw.ac.at/defc/thesaurus/stone/6.11> a skos:Concept ;
    dc:source "https://en.oxforddictionaries.com/definition/stone" ;
    skos:broader <http://id.acdh.oeaw.ac.at/defc/thesaurus/building_material/5.089> ;
    skos:definition "Hard solid non-metallic mineral matter of which rock is made, especailly as a building material." ;
    skos:editorialNote "dc_area_buildingtechnique;11" ;
    skos:inScheme <http://id.acdh.oeaw.ac.at/defc/thesaurus/AreaBuildingtechnique>,
        <http://id.acdh.oeaw.ac.at/defc/thesaurus/AreaSchema> ;
    skos:prefLabel "Stein"@de,
        "stone"@en .

<http://id.acdh.oeaw.ac.at/defc/thesaurus/stone_figurine/4.82> a skos:Concept ;
    dc:source "Kipfer, B. A. Dictionary of Artifacts 2007. Blackwell Publishing, Oxford.p.113" ;
    skos:broader <http://id.acdh.oeaw.ac.at/defc/thesaurus/figurine/3.3> ;
    skos:definition "A small carved figure of a human or animal of stone." ;
    skos:editorialNote "dc_finds_small_finds_type;82" ;
    skos:inScheme <http://id.acdh.oeaw.ac.at/defc/thesaurus/FindsSchema>,
        <http://id.acdh.oeaw.ac.at/defc/thesaurus/FindsSmallFindsType> ;
    skos:prefLabel "Steinfigur"@de,
        "stone figurine"@en .

<http://id.acdh.oeaw.ac.at/defc/thesaurus/stone_lining/5.12> a skos:Concept ;
    skos:broader <http://id.acdh.oeaw.ac.at/defc/thesaurus/building_technique/4.075> ;
    skos:editorialNote "dc_area_buildingtechnique;12" ;
    skos:inScheme <http://id.acdh.oeaw.ac.at/defc/thesaurus/AreaBuildingtechnique>,
        <http://id.acdh.oeaw.ac.at/defc/thesaurus/AreaSchema> ;
    skos:prefLabel "stone lining"@en .

<http://id.acdh.oeaw.ac.at/defc/thesaurus/stone_platform/6.19> a skos:Concept ;
    dc:source "M. Brami, PhD after Catalhoyuk Research Project http://www.catalhoyuk.com/database/catal/help_glossary1.asp" ;
    skos:broader <http://id.acdh.oeaw.ac.at/defc/thesaurus/platform/5.093> ;
    skos:definition "A raised flat stone surface with a ridge." ;
    skos:editorialNote "dc_area_specialfeatures;19" ;
    skos:inScheme <http://id.acdh.oeaw.ac.at/defc/thesaurus/AreaSchema>,
        <http://id.acdh.oeaw.ac.at/defc/thesaurus/AreaSpecialfeatures> ;
    skos:prefLabel "stone platform"@en .

<http://id.acdh.oeaw.ac.at/defc/thesaurus/stone_row_structure/5.38> a skos:Concept ;
    skos:broader <http://id.acdh.oeaw.ac.at/defc/thesaurus/architecture/4.081> ;
    skos:editorialNote "dc_area_specialfeatures;38" ;
    skos:inScheme <http://id.acdh.oeaw.ac.at/defc/thesaurus/AreaSchema>,
        <http://id.acdh.oeaw.ac.at/defc/thesaurus/AreaSpecialfeatures> ;
    skos:prefLabel "Steinreihenstruktur"@de,
        "stone row structure"@en .

<http://id.acdh.oeaw.ac.at/defc/thesaurus/stone_setting/5.4> a skos:Concept ;
    dc:source "OREA" ;
    skos:broader <http://id.acdh.oeaw.ac.at/defc/thesaurus/occupation_evidence/4.088> ;
    skos:definition "An arrangement of one or more standing stones inside or in the vicinity of a cave or a rockshelter as a sign of human occupation." ;
    skos:editorialNote "dc_area_evidenceofocupation;4" ;
    skos:inScheme <http://id.acdh.oeaw.ac.at/defc/thesaurus/AreaEvidenceofocupation>,
        <http://id.acdh.oeaw.ac.at/defc/thesaurus/AreaSchema> ;
    skos:prefLabel "Steinsetzung"@de,
        "stone setting"@en .

<http://id.acdh.oeaw.ac.at/defc/thesaurus/stone_setting/5.6> a skos:Concept ;
    dc:source "http://thesaurus.historicengland.org.uk/thesaurus_term.asp?thes_no=1&term_no=70194" ;
    skos:altLabel "Steinsetzung"@de ;
    skos:broader <http://id.acdh.oeaw.ac.at/defc/thesaurus/ritual/4.079> ;
    skos:definition "An arrangement of one or more standing stones." ;
    skos:editorialNote "dc_area_specialfeatures;6" ;
    skos:inScheme <http://id.acdh.oeaw.ac.at/defc/thesaurus/AreaSchema>,
        <http://id.acdh.oeaw.ac.at/defc/thesaurus/AreaSpecialfeatures> ;
    skos:prefLabel "stone setting"@en .

<http://id.acdh.oeaw.ac.at/defc/thesaurus/stone_socket/5.5> a skos:Concept ;
    skos:broader <http://id.acdh.oeaw.ac.at/defc/thesaurus/building_technique/4.075> ;
    skos:editorialNote "dc_area_buildingtechnique;5" ;
    skos:inScheme <http://id.acdh.oeaw.ac.at/defc/thesaurus/AreaBuildingtechnique>,
        <http://id.acdh.oeaw.ac.at/defc/thesaurus/AreaSchema> ;
    skos:prefLabel "Steinsockel"@de,
        "stone socket"@en .

<http://id.acdh.oeaw.ac.at/defc/thesaurus/stone_tool_production/2.4> a skos:Concept ;
    dc:source "OREA" ;
    skos:broader <http://id.acdh.oeaw.ac.at/defc/thesaurus/production/1.042> ;
    skos:definition "The activity of making physical items of stone that can be afterwards used to achive a certain goal." ;
    skos:editorialNote "dc_interpretation_productiontype;4" ;
    skos:inScheme <http://id.acdh.oeaw.ac.at/defc/thesaurus/InterpretationProductiontype>,
        <http://id.acdh.oeaw.ac.at/defc/thesaurus/InterpretationSchema> ;
    skos:prefLabel "Steinwerkzeugherstellung"@de,
        "stone tool production"@en .

<http://id.acdh.oeaw.ac.at/defc/thesaurus/storage_building/5.7> a skos:Concept ;
    dc:source "OREA" ;
    skos:altLabel "Lagerhaus"@de ;
    skos:broader <http://id.acdh.oeaw.ac.at/defc/thesaurus/storage/4.080> ;
    skos:definition "A building used for storing food and other goods." ;
    skos:editorialNote "dc_area_specialfeatures;7" ;
    skos:inScheme <http://id.acdh.oeaw.ac.at/defc/thesaurus/AreaSchema>,
        <http://id.acdh.oeaw.ac.at/defc/thesaurus/AreaSpecialfeatures> ;
    skos:prefLabel "storage building"@en .

<http://id.acdh.oeaw.ac.at/defc/thesaurus/storage_facilities/5.2> a skos:Concept ;
    dc:source "OREA" ;
    skos:broader <http://id.acdh.oeaw.ac.at/defc/thesaurus/occupation_evidence/4.088> ;
    skos:definition "A place, amenity, or piece of equipment provided to store food and other goods inside of a cave or a rockshelter as evidence of human occupation." ;
    skos:editorialNote "dc_area_evidenceofocupation;2" ;
    skos:inScheme <http://id.acdh.oeaw.ac.at/defc/thesaurus/AreaEvidenceofocupation>,
        <http://id.acdh.oeaw.ac.at/defc/thesaurus/AreaSchema> ;
    skos:prefLabel "Lagerungseinrichtungen"@de,
        "storage facilities"@en .

<http://id.acdh.oeaw.ac.at/defc/thesaurus/storage_pit/5.8> a skos:Concept ;
    dc:source "http://thesaurus.historicengland.org.uk/pastscape_term.asp?thes_no=1&term_no=68668" ;
    skos:altLabel "Vorratsgrube"@de ;
    skos:broader <http://id.acdh.oeaw.ac.at/defc/thesaurus/storage/4.080> ;
    skos:definition "A pit dug in the ground used to store foodstuffs." ;
    skos:editorialNote "dc_area_specialfeatures;8" ;
    skos:inScheme <http://id.acdh.oeaw.ac.at/defc/thesaurus/AreaSchema>,
        <http://id.acdh.oeaw.ac.at/defc/thesaurus/AreaSpecialfeatures> ;
    skos:prefLabel "storage pit"@en .

<http://id.acdh.oeaw.ac.at/defc/thesaurus/storage_systems/2.6> a skos:Concept ;
    skos:broader <http://id.acdh.oeaw.ac.at/defc/thesaurus/subsistence/1.043> ;
    skos:editorialNote "dc_interpretation_subsistencetype;6" ;
    skos:inScheme <http://id.acdh.oeaw.ac.at/defc/thesaurus/InterpretationSchema>,
        <http://id.acdh.oeaw.ac.at/defc/thesaurus/InterpretationSubsistencetype> ;
    skos:prefLabel "storage systems"@en .

<http://id.acdh.oeaw.ac.at/defc/thesaurus/storage_vessel/5.9> a skos:Concept ;
    dc:source "OREA" ;
    skos:altLabel "Vorratsgefäß"@de ;
    skos:broader <http://id.acdh.oeaw.ac.at/defc/thesaurus/storage/4.080> ;
    skos:definition "A container used for storing food and liquids such as storage jar, pithos, amphore etc." ;
    skos:editorialNote "dc_area_specialfeatures;9" ;
    skos:inScheme <http://id.acdh.oeaw.ac.at/defc/thesaurus/AreaSchema>,
        <http://id.acdh.oeaw.ac.at/defc/thesaurus/AreaSpecialfeatures> ;
    skos:prefLabel "storage vessel"@en .

<http://id.acdh.oeaw.ac.at/defc/thesaurus/strap_handle_with_knob/6.91> a skos:Concept ;
    dc:source "Kipfer, B. A. Dictionary of Artifacts 2007. Blackwell Publishing, Oxford.p 305" ;
    skos:broader <http://id.acdh.oeaw.ac.at/defc/thesaurus/strap_handle/5.78> ;
    skos:definition "A handle made from a strip of clay with round application, attached to the body of the pot at two points before firing." ;
    skos:editorialNote "dc_finds_pottery_detail;91" ;
    skos:inScheme <http://id.acdh.oeaw.ac.at/defc/thesaurus/FindsPotteryDetail>,
        <http://id.acdh.oeaw.ac.at/defc/thesaurus/FindsSchema> ;
    skos:prefLabel "Bandhenkel mit Knubbe"@de,
        "strap handle with knob"@en .

<http://id.acdh.oeaw.ac.at/defc/thesaurus/strap_handle_with_round_hole/6.149> a skos:Concept ;
    dc:source "Kipfer, B. A. Dictionary of Artifacts 2007. Blackwell Publishing, Oxford.p 305" ;
    skos:broader <http://id.acdh.oeaw.ac.at/defc/thesaurus/strap_handle/5.78> ;
    skos:definition "A handle made from a strip of clay with a round loop and attached to the body of the pot at two points before firing." ;
    skos:editorialNote "dc_finds_pottery_detail;149" ;
    skos:inScheme <http://id.acdh.oeaw.ac.at/defc/thesaurus/FindsPotteryDetail>,
        <http://id.acdh.oeaw.ac.at/defc/thesaurus/FindsSchema> ;
    skos:prefLabel "Bandhenkel mit rundem Loch"@de,
        "strap handle with round hole"@en .

<http://id.acdh.oeaw.ac.at/defc/thesaurus/straw/6.8> a skos:Concept ;
    dc:source "OREA" ;
    skos:altLabel "hay"@en ;
    skos:broader <http://id.acdh.oeaw.ac.at/defc/thesaurus/building_material/5.089> ;
    skos:definition "Sried stalks of grain used as building material." ;
    skos:editorialNote "dc_area_buildingtechnique;8" ;
    skos:inScheme <http://id.acdh.oeaw.ac.at/defc/thesaurus/AreaBuildingtechnique>,
        <http://id.acdh.oeaw.ac.at/defc/thesaurus/AreaSchema> ;
    skos:prefLabel "Stroh"@de,
        "straw"@en .

<http://id.acdh.oeaw.ac.at/defc/thesaurus/stringhole_lug/6.79> a skos:Concept ;
    dc:source "Kipfer, B. A. Dictionary of Artifacts 2007. Blackwell Publishing, Oxford.p 184" ;
    skos:altLabel "preforated lug"@en ;
    skos:broader <http://id.acdh.oeaw.ac.at/defc/thesaurus/lug/5.040> ;
    skos:definition "An ear-shaped protuberance added to the wall of a pot to assist in hodling it. After attachment it was perforated. The hole was designed to take a cord or thong only and it was not a true handle." ;
    skos:editorialNote "dc_finds_pottery_detail;79" ;
    skos:inScheme <http://id.acdh.oeaw.ac.at/defc/thesaurus/FindsPotteryDetail>,
        <http://id.acdh.oeaw.ac.at/defc/thesaurus/FindsSchema> ;
    skos:prefLabel "Schnuröse"@de,
        "stringhole lug"@en .

<http://id.acdh.oeaw.ac.at/defc/thesaurus/stroke-and_pattern_burnished/5.178> a skos:Concept ;
    dc:source "Kipfer, B. A. Dictionary of Artifacts 2007. Blackwell Publishing, Oxford.p 50" ;
    skos:altLabel "Pattern-burnished"@de,
        "stroke-burnished"@de ;
    skos:broader <http://id.acdh.oeaw.ac.at/defc/thesaurus/burnished/4.297> ;
    skos:definition "Pottery decorated with network patterns. In stroke burnish, the surface is completey polished, but the marks of the burnished, a pebble or bone slip, remain distinct." ;
    skos:editorialNote "dc_finds_pottery_decoration;178" ;
    skos:inScheme <http://id.acdh.oeaw.ac.at/defc/thesaurus/FindsPotteryDecoration>,
        <http://id.acdh.oeaw.ac.at/defc/thesaurus/FindsSchema> ;
    skos:prefLabel "Strich- und mustergeglättet"@de,
        "stroke-and pattern burnished"@en .

<http://id.acdh.oeaw.ac.at/defc/thesaurus/subadult/6.14> a skos:Concept ;
    skos:broader <http://id.acdh.oeaw.ac.at/defc/thesaurus/age_group/5.097> ;
    skos:editorialNote "dc_area_agegroups;14" ;
    skos:inScheme <http://id.acdh.oeaw.ac.at/defc/thesaurus/AreaAgegroups>,
        <http://id.acdh.oeaw.ac.at/defc/thesaurus/AreaSchema> ;
    skos:prefLabel "subadult"@en .

<http://id.acdh.oeaw.ac.at/defc/thesaurus/surface/4.3> a skos:Concept ;
    dc:source "OREA" ;
    skos:altLabel "Tagebau"@de ;
    skos:broader <http://id.acdh.oeaw.ac.at/defc/thesaurus/quarry_type/3.065> ;
    skos:definition "Tool marks recognized on a rock surface as the evidence for mining activities." ;
    skos:editorialNote "dc_area_explotationtype;3" ;
    skos:inScheme <http://id.acdh.oeaw.ac.at/defc/thesaurus/AreaExplotationtype>,
        <http://id.acdh.oeaw.ac.at/defc/thesaurus/AreaSchema> ;
    skos:prefLabel "oberflächennaher Abbau"@de,
        "surface"@en .

<http://id.acdh.oeaw.ac.at/defc/thesaurus/t-pillar/6.18> a skos:Concept ;
    dc:source "OREA (M. Brami)" ;
    skos:broader <http://id.acdh.oeaw.ac.at/defc/thesaurus/pillar/5.091> ;
    skos:definition "A megalithic pillar cut in a T-shape, typical of the Southeast Anatolian PPNA." ;
    skos:editorialNote "dc_area_buildingtechnique;18" ;
    skos:inScheme <http://id.acdh.oeaw.ac.at/defc/thesaurus/AreaBuildingtechnique>,
        <http://id.acdh.oeaw.ac.at/defc/thesaurus/AreaSchema> ;
    skos:prefLabel "T-Pfeiler"@de,
        "t-pillar"@en .

<http://id.acdh.oeaw.ac.at/defc/thesaurus/tab_handle/5.169> a skos:Concept ;
    dc:source "OREA" ;
    skos:altLabel "hammer rims"@en ;
    skos:broader <http://id.acdh.oeaw.ac.at/defc/thesaurus/handle/4.031> ;
    skos:definition "Flat handle." ;
    skos:editorialNote "dc_finds_pottery_detail;169" ;
    skos:inScheme <http://id.acdh.oeaw.ac.at/defc/thesaurus/FindsPotteryDetail>,
        <http://id.acdh.oeaw.ac.at/defc/thesaurus/FindsSchema> ;
    skos:prefLabel "Grifflappen"@de,
        "tab handle"@en .

<http://id.acdh.oeaw.ac.at/defc/thesaurus/table/4.61> a skos:Concept ;
    dc:source "OREA" ;
    skos:broader <http://id.acdh.oeaw.ac.at/defc/thesaurus/figurine/3.3> ;
    skos:definition "A figurine shaped in form of a table." ;
    skos:editorialNote "dc_finds_small_finds_type;61" ;
    skos:inScheme <http://id.acdh.oeaw.ac.at/defc/thesaurus/FindsSchema>,
        <http://id.acdh.oeaw.ac.at/defc/thesaurus/FindsSmallFindsType> ;
    skos:prefLabel "Tisch"@de,
        "table"@en .

<http://id.acdh.oeaw.ac.at/defc/thesaurus/tablet/4.11> a skos:Concept ;
    skos:broader <http://id.acdh.oeaw.ac.at/defc/thesaurus/core_preparation/3.013> ;
    skos:editorialNote "dc_finds_lithics_core_shape;11" ;
    skos:inScheme <http://id.acdh.oeaw.ac.at/defc/thesaurus/FindsLithicsCoreShape>,
        <http://id.acdh.oeaw.ac.at/defc/thesaurus/FindsSchema> ;
    skos:prefLabel "tablet"@en .

<http://id.acdh.oeaw.ac.at/defc/thesaurus/tally_stick/4.100> a skos:Concept ;
    dc:source "http://dbpedia.org/page/Tally_stick" ;
    skos:broader <http://id.acdh.oeaw.ac.at/defc/thesaurus/tool/3.1> ;
    skos:definition "A tally (or tally stick) was an ancient memory aid device used to record and document numbers, quantities, or even messages." ;
    skos:editorialNote "dc_finds_small_finds_type;100" ;
    skos:inScheme <http://id.acdh.oeaw.ac.at/defc/thesaurus/FindsSchema>,
        <http://id.acdh.oeaw.ac.at/defc/thesaurus/FindsSmallFindsType> ;
    skos:prefLabel "Kerbholz"@de,
        "tally stick"@en .

<http://id.acdh.oeaw.ac.at/defc/thesaurus/tank/5.12> a skos:Concept ;
    dc:source "OREA" ;
    skos:altLabel "Wasserbecken"@de ;
    skos:broader <http://id.acdh.oeaw.ac.at/defc/thesaurus/storage/4.080> ;
    skos:definition "A  container for storing liquid." ;
    skos:editorialNote "dc_area_specialfeatures;12" ;
    skos:inScheme <http://id.acdh.oeaw.ac.at/defc/thesaurus/AreaSchema>,
        <http://id.acdh.oeaw.ac.at/defc/thesaurus/AreaSpecialfeatures> ;
    skos:prefLabel "tank"@en .

<http://id.acdh.oeaw.ac.at/defc/thesaurus/tapered-up_rim/5.157> a skos:Concept ;
    dc:source "OREA" ;
    skos:broader <http://id.acdh.oeaw.ac.at/defc/thesaurus/rim/4.033> ;
    skos:definition "The upper portion of the vessel closest to its orifice that has been thinned." ;
    skos:editorialNote "dc_finds_pottery_detail;157" ;
    skos:inScheme <http://id.acdh.oeaw.ac.at/defc/thesaurus/FindsPotteryDetail>,
        <http://id.acdh.oeaw.ac.at/defc/thesaurus/FindsSchema> ;
    skos:prefLabel "Verjüngender Rand"@de,
        "tapered-up rim"@en .

<http://id.acdh.oeaw.ac.at/defc/thesaurus/tell/4.2> a skos:Concept ;
    dc:source "OREA (M. Brami)" ;
    skos:altLabel "Tepe"@de,
        "tel"@en,
        "tepe"@en ;
    skos:broader <http://id.acdh.oeaw.ac.at/defc/thesaurus/settlment_type/3.068> ;
    skos:definition "An artificial mound made of a build-up of settlement debris." ;
    skos:editorialNote "dc_area_settlementtype;2" ;
    skos:inScheme <http://id.acdh.oeaw.ac.at/defc/thesaurus/AreaSchema>,
        <http://id.acdh.oeaw.ac.at/defc/thesaurus/AreaSettlementtype> ;
    skos:prefLabel "Tell"@de,
        "tell"@en .

<http://id.acdh.oeaw.ac.at/defc/thesaurus/terrace_wall/5.14> a skos:Concept ;
    dc:source "OREA" ;
    skos:altLabel "Terrassenmauer"@de ;
    skos:broader <http://id.acdh.oeaw.ac.at/defc/thesaurus/architecture/4.081> ;
    skos:definition "A wall supporting the slope or shielding from erosion." ;
    skos:editorialNote "dc_area_specialfeatures;14" ;
    skos:inScheme <http://id.acdh.oeaw.ac.at/defc/thesaurus/AreaSchema>,
        <http://id.acdh.oeaw.ac.at/defc/thesaurus/AreaSpecialfeatures> ;
    skos:prefLabel "terrace wall"@en .

<http://id.acdh.oeaw.ac.at/defc/thesaurus/terrazzo_floor/6.15> a skos:Concept ;
    dc:source "https://en.oxforddictionaries.com/definition/terrazzo" ;
    skos:broader <http://id.acdh.oeaw.ac.at/defc/thesaurus/floor/5.092> ;
    skos:definition "Floor consisting of chips of marble or granite set in concrete and polished to give a smooth surface involving a complex firing procedure." ;
    skos:editorialNote "dc_area_buildingtechnique;15" ;
    skos:inScheme <http://id.acdh.oeaw.ac.at/defc/thesaurus/AreaBuildingtechnique>,
        <http://id.acdh.oeaw.ac.at/defc/thesaurus/AreaSchema> ;
    skos:prefLabel "Terazzo Boden"@de,
        "terrazzo floor"@en .

<http://id.acdh.oeaw.ac.at/defc/thesaurus/test_pit/4.8> a skos:Concept ;
    dc:source "http://thesaurus.historicengland.org.uk/thesaurus_term.asp?thes_no=566&term_no=145172" ;
    skos:broader <http://id.acdh.oeaw.ac.at/defc/thesaurus/evaluation/3.050> ;
    skos:definition "Systematically positioned hole, or holes, utilised in all studies that aim to sample the nature of the topsoil and subsurface deposits." ;
    skos:editorialNote "dc_researchevet_researchtype;8" ;
    skos:inScheme <http://id.acdh.oeaw.ac.at/defc/thesaurus/ResearchEventSchema>,
        <http://id.acdh.oeaw.ac.at/defc/thesaurus/ResearchevetResearchtype> ;
    skos:prefLabel "Sondage"@de,
        "test pit"@en .

<http://id.acdh.oeaw.ac.at/defc/thesaurus/textile_production/2.1> a skos:Concept ;
    dc:source "OREA" ;
    skos:broader <http://id.acdh.oeaw.ac.at/defc/thesaurus/production/1.042> ;
    skos:definition "The activity of making cloth or wover fabric." ;
    skos:editorialNote "dc_interpretation_productiontype;1" ;
    skos:inScheme <http://id.acdh.oeaw.ac.at/defc/thesaurus/InterpretationProductiontype>,
        <http://id.acdh.oeaw.ac.at/defc/thesaurus/InterpretationSchema> ;
    skos:prefLabel "Textilproduktion"@de,
        "textile production"@en .

<http://id.acdh.oeaw.ac.at/defc/thesaurus/thermal_structure/5.27> a skos:Concept ;
    dc:source "OREA" ;
    skos:broader <http://id.acdh.oeaw.ac.at/defc/thesaurus/architecture/4.081> ;
    skos:definition "A construction used for heating." ;
    skos:editorialNote "dc_area_specialfeatures;27" ;
    skos:inScheme <http://id.acdh.oeaw.ac.at/defc/thesaurus/AreaSchema>,
        <http://id.acdh.oeaw.ac.at/defc/thesaurus/AreaSpecialfeatures> ;
    skos:prefLabel "thermal structure"@en .

<http://id.acdh.oeaw.ac.at/defc/thesaurus/thickened_rim/5.166> a skos:Concept ;
    dc:source "OREA" ;
    skos:broader <http://id.acdh.oeaw.ac.at/defc/thesaurus/rim/4.033> ;
    skos:definition "The upper portion of the vessel closest to its orifice that has been thickened." ;
    skos:editorialNote "dc_finds_pottery_detail;166" ;
    skos:inScheme <http://id.acdh.oeaw.ac.at/defc/thesaurus/FindsPotteryDetail>,
        <http://id.acdh.oeaw.ac.at/defc/thesaurus/FindsSchema> ;
    skos:prefLabel "Verdickter Rand"@de,
        "thickened rim"@en .

<http://id.acdh.oeaw.ac.at/defc/thesaurus/thin_plate/4.104> a skos:Concept ;
    dc:source "OREA" ;
    skos:broader <http://id.acdh.oeaw.ac.at/defc/thesaurus/figurine/3.3> ;
    skos:definition "Decorated small ceramic plates of an unknown function." ;
    skos:editorialNote "dc_finds_small_finds_type;104" ;
    skos:inScheme <http://id.acdh.oeaw.ac.at/defc/thesaurus/FindsSchema>,
        <http://id.acdh.oeaw.ac.at/defc/thesaurus/FindsSmallFindsType> ;
    skos:prefLabel "Plättchen"@de,
        "thin plate"@en .

<http://id.acdh.oeaw.ac.at/defc/thesaurus/timber-frame_construction/5.7> a skos:Concept ;
    dc:source "Kipfer, B. A. Encyclopedic Dictionary of Archaeology. Kluwer Academic/Plenum Publishers, New York. p. 226." ;
    skos:altLabel "half-timbered"@en,
        "timber frame"@en,
        "timber framing"@en ;
    skos:broader <http://id.acdh.oeaw.ac.at/defc/thesaurus/building_technique/4.075> ;
    skos:definition "Constructed of wood framing with spaces filled with masonry, or by stone, rubble, or mud brick." ;
    skos:editorialNote "dc_area_buildingtechnique;7" ;
    skos:inScheme <http://id.acdh.oeaw.ac.at/defc/thesaurus/AreaBuildingtechnique>,
        <http://id.acdh.oeaw.ac.at/defc/thesaurus/AreaSchema> ;
    skos:prefLabel "Holzskelett"@de,
        "timber-frame construction"@en .

<http://id.acdh.oeaw.ac.at/defc/thesaurus/timber/6.10> a skos:Concept ;
    dc:source "https://en.oxforddictionaries.com/definition/timber" ;
    skos:broader <http://id.acdh.oeaw.ac.at/defc/thesaurus/building_material/5.089> ;
    skos:definition "Wood prepared for use in building and carpentry." ;
    skos:editorialNote "dc_area_buildingtechnique;10" ;
    skos:inScheme <http://id.acdh.oeaw.ac.at/defc/thesaurus/AreaBuildingtechnique>,
        <http://id.acdh.oeaw.ac.at/defc/thesaurus/AreaSchema> ;
    skos:prefLabel "timber"@en .

<http://id.acdh.oeaw.ac.at/defc/thesaurus/tip/4.101> a skos:Concept ;
    dc:source "Kipfer, B. A. Dictionary of Artifacts 2007. Blackwell Publishing, Oxford.p 319" ;
    skos:altLabel "shaft"@en ;
    skos:broader <http://id.acdh.oeaw.ac.at/defc/thesaurus/tool/3.1> ;
    skos:definition "Top and bottom of a point or blade." ;
    skos:editorialNote "dc_finds_small_finds_type;101" ;
    skos:inScheme <http://id.acdh.oeaw.ac.at/defc/thesaurus/FindsSchema>,
        <http://id.acdh.oeaw.ac.at/defc/thesaurus/FindsSmallFindsType> ;
    skos:prefLabel "Spitze"@de,
        "tip"@en .

<http://id.acdh.oeaw.ac.at/defc/thesaurus/token/4.105> a skos:Concept ;
    dc:source "Kipfer, B. A. Dictionary of Artifacts 2007. Blackwell Publishing, Oxford.p 319" ;
    skos:broader <http://id.acdh.oeaw.ac.at/defc/thesaurus/other/3.4> ;
    skos:definition "Small artifacts, generally of clay, made into cones, shperes, disks, or cylinders, tetrahedrons with usually plain surface. Such objects were used on Early Neolithic sites in western Asia as counters to keep records of goods." ;
    skos:editorialNote "dc_finds_small_finds_type;105" ;
    skos:inScheme <http://id.acdh.oeaw.ac.at/defc/thesaurus/FindsSchema>,
        <http://id.acdh.oeaw.ac.at/defc/thesaurus/FindsSmallFindsType> ;
    skos:prefLabel "Zeichen"@de,
        "token"@en .

<http://id.acdh.oeaw.ac.at/defc/thesaurus/tooth/3.28> a skos:Concept ;
    dc:source "http://dbpedia.org/page/Tooth" ;
    skos:broader <http://id.acdh.oeaw.ac.at/defc/thesaurus/organic/2.4> ;
    skos:definition "A tooth (plural teeth) is a small, calcified, whitish structure found in the jaws (or mouths) of many vertebrates and used to break down food." ;
    skos:editorialNote "dc_finds_material;28" ;
    skos:inScheme <http://id.acdh.oeaw.ac.at/defc/thesaurus/FindsMaterial>,
        <http://id.acdh.oeaw.ac.at/defc/thesaurus/FindsSchema> ;
    skos:prefLabel "Zahn"@de,
        "tooth"@en .

<http://id.acdh.oeaw.ac.at/defc/thesaurus/tortoise/5.29> a skos:Concept ;
    dc:source "http://eol.org/pages/8132/overview" ;
    skos:broader <http://id.acdh.oeaw.ac.at/defc/thesaurus/reptile/4.35> ;
    skos:editorialNote "dc_finds_animal_remains_species;29" ;
    skos:inScheme <http://id.acdh.oeaw.ac.at/defc/thesaurus/FindsAnimalRemainsSpecies>,
        <http://id.acdh.oeaw.ac.at/defc/thesaurus/FindsSchema> ;
    skos:prefLabel "Schildkröte"@de,
        "tortoise"@en .

<http://id.acdh.oeaw.ac.at/defc/thesaurus/trapeze/4.22> a skos:Concept ;
    dc:source "Inizan, M.-L., M. Reduron-Ballinger, H. Roche, J. Tixier 1999, Technology and Terminology of Knapped Stone. Nanterre: CREP., D. Srejovic (ed) 1997, Arheološki Leksikon." ;
    skos:broader <http://id.acdh.oeaw.ac.at/defc/thesaurus/retouched_tool/3.010> ;
    skos:definition "A geometric microlith whose outline has four sides - two lateral nearly parallel sides with the longer one being the cutting edge and the shorter opposite edge backed or not-backed. Also called transverse arrowhead." ;
    skos:editorialNote "dc_finds_lithics_retouched_tools;22" ;
    skos:inScheme <http://id.acdh.oeaw.ac.at/defc/thesaurus/FindsLithicsRetouchedTools>,
        <http://id.acdh.oeaw.ac.at/defc/thesaurus/FindsSchema> ;
    skos:prefLabel "Trapez"@de,
        "trapeze"@en .

<http://id.acdh.oeaw.ac.at/defc/thesaurus/trial_trench/4.9> a skos:Concept ;
    dc:source "http://thesaurus.historicengland.org.uk/thesaurus_term.asp?thes_no=566&term_no=145175" ;
    skos:broader <http://id.acdh.oeaw.ac.at/defc/thesaurus/evaluation/3.050> ;
    skos:definition "Archaeologically excavated trench, either hand or machine dug, as part of a sampling programme to evaluate the presence/absence, nature, preservation, age and extent of any buried archaeological features." ;
    skos:editorialNote "dc_researchevet_researchtype;9" ;
    skos:inScheme <http://id.acdh.oeaw.ac.at/defc/thesaurus/ResearchEventSchema>,
        <http://id.acdh.oeaw.ac.at/defc/thesaurus/ResearchevetResearchtype> ;
    skos:prefLabel "Suchschnitt"@de,
        "trial trench"@en .

<http://id.acdh.oeaw.ac.at/defc/thesaurus/triangular_ring_handle/6.101> a skos:Concept ;
    dc:source "OREA" ;
    skos:broader <http://id.acdh.oeaw.ac.at/defc/thesaurus/ring_handle/5.100> ;
    skos:definition "Pyramid-shaped handle with a round loop." ;
    skos:editorialNote "dc_finds_pottery_detail;101" ;
    skos:inScheme <http://id.acdh.oeaw.ac.at/defc/thesaurus/FindsPotteryDetail>,
        <http://id.acdh.oeaw.ac.at/defc/thesaurus/FindsSchema> ;
    skos:prefLabel "dreieckiger Ringhenkel"@de,
        "triangular ring handle"@en .

<http://id.acdh.oeaw.ac.at/defc/thesaurus/tripod/4.137> a skos:Concept ;
    dc:source "OREA" ;
    skos:broader <http://id.acdh.oeaw.ac.at/defc/thesaurus/pottery_form/3.016> ;
    skos:definition "A vessel standing on three legs." ;
    skos:editorialNote "dc_finds_pottery_form;137" ;
    skos:inScheme <http://id.acdh.oeaw.ac.at/defc/thesaurus/FindsPotteryForm>,
        <http://id.acdh.oeaw.ac.at/defc/thesaurus/FindsSchema> ;
    skos:prefLabel "Dreifuß"@de,
        "tripod"@en .

<http://id.acdh.oeaw.ac.at/defc/thesaurus/truncation/4.23> a skos:Concept ;
    dc:source "Inizan, M.-L., M. Reduron-Ballinger, H. Roche, J. Tixier 1999, Technology and Terminology of Knapped Stone. Nanterre: CREP., D. Srejovic (ed) 1997, Arheološki Leksikon." ;
    skos:broader <http://id.acdh.oeaw.ac.at/defc/thesaurus/retouched_tool/3.010> ;
    skos:definition "A blade with a steep retouch made on a broken end." ;
    skos:editorialNote "dc_finds_lithics_retouched_tools;23" ;
    skos:inScheme <http://id.acdh.oeaw.ac.at/defc/thesaurus/FindsLithicsRetouchedTools>,
        <http://id.acdh.oeaw.ac.at/defc/thesaurus/FindsSchema> ;
    skos:prefLabel "Endretusche"@de,
        "truncation"@en .

<http://id.acdh.oeaw.ac.at/defc/thesaurus/tsangli_house/5.6> a skos:Concept ;
    dc:source "OREA (M. Brami)" ;
    skos:broader <http://id.acdh.oeaw.ac.at/defc/thesaurus/building_type/4.077> ;
    skos:definition "A type of building with internal buttresses projecting from the walls. Named after the eponymous site of Tsangli in Thessaly." ;
    skos:editorialNote "dc_area_constructiontype;6" ;
    skos:inScheme <http://id.acdh.oeaw.ac.at/defc/thesaurus/AreaConstructiontype>,
        <http://id.acdh.oeaw.ac.at/defc/thesaurus/AreaSchema> ;
    skos:prefLabel "tsangli house"@en .

<http://id.acdh.oeaw.ac.at/defc/thesaurus/tubular_lug/6.80> a skos:Concept ;
    dc:source "OREA" ;
    skos:altLabel "Griffplatte"@de,
        "tubular handle"@en ;
    skos:broader <http://id.acdh.oeaw.ac.at/defc/thesaurus/lug/5.040> ;
    skos:definition "Tunnel shaped not preforated protuberance added to the wall of a pot to assist in hodling it." ;
    skos:editorialNote "dc_finds_pottery_detail;80" ;
    skos:inScheme <http://id.acdh.oeaw.ac.at/defc/thesaurus/FindsPotteryDetail>,
        <http://id.acdh.oeaw.ac.at/defc/thesaurus/FindsSchema> ;
    skos:prefLabel "Röhrenöse"@de,
        "tubular lug"@en .

<http://id.acdh.oeaw.ac.at/defc/thesaurus/tulip-shaped_beaker/5.118> a skos:Concept ;
    dc:source "OREA" ;
    skos:broader <http://id.acdh.oeaw.ac.at/defc/thesaurus/beaker/4.098> ;
    skos:definition "A handled cup in a form of a bell." ;
    skos:editorialNote "dc_finds_pottery_form;118" ;
    skos:inScheme <http://id.acdh.oeaw.ac.at/defc/thesaurus/FindsPotteryForm>,
        <http://id.acdh.oeaw.ac.at/defc/thesaurus/FindsSchema> ;
    skos:prefLabel "Tulpenförmger Becher"@de,
        "tulip-shaped beaker"@en .

<http://id.acdh.oeaw.ac.at/defc/thesaurus/tumulus/5.6> a skos:Concept ;
    dc:source "Kipfer, B. A. Encyclopedic Dictionary of Archaeology. Kluwer Academic/Plenum Publishers, New York. P.578" ;
    skos:broader <http://id.acdh.oeaw.ac.at/defc/thesaurus/grave_type/4.083> ;
    skos:definition "A mound of earth or stones built over a burial - most often a large, circular tomb." ;
    skos:editorialNote "dc_area_gravetype;6" ;
    skos:inScheme <http://id.acdh.oeaw.ac.at/defc/thesaurus/AreaGravetype>,
        <http://id.acdh.oeaw.ac.at/defc/thesaurus/AreaSchema> ;
    skos:prefLabel "Grabhügel"@de,
        "tumulus"@en .

<http://id.acdh.oeaw.ac.at/defc/thesaurus/tuna/5.18> a skos:Concept ;
    dc:source "http://eol.org/pages/25172/overview" ;
    skos:broader <http://id.acdh.oeaw.ac.at/defc/thesaurus/fish/4.16> ;
    skos:editorialNote "dc_finds_animal_remains_species;18" ;
    skos:inScheme <http://id.acdh.oeaw.ac.at/defc/thesaurus/FindsAnimalRemainsSpecies>,
        <http://id.acdh.oeaw.ac.at/defc/thesaurus/FindsSchema> ;
    skos:prefLabel "Thunfisch"@de,
        "tuna"@en,
        "Thunnus"@la .

<http://id.acdh.oeaw.ac.at/defc/thesaurus/tusk/5.12> a skos:Concept ;
    dc:source "https://en.oxforddictionaries.com/definition/tusk" ;
    skos:broader <http://id.acdh.oeaw.ac.at/defc/thesaurus/tooth/4.11> ;
    skos:definition "A long pointed tooth, especially one which protrudes from the closed mouth, as in the elephant, walrus, or wild boar." ;
    skos:editorialNote "dc_animal_remains_part;12" ;
    skos:inScheme <http://id.acdh.oeaw.ac.at/defc/thesaurus/AnimalRemainsPart>,
        <http://id.acdh.oeaw.ac.at/defc/thesaurus/FindsSchema> ;
    skos:prefLabel "Stoßzahn"@de,
        "tusk"@en .

<http://id.acdh.oeaw.ac.at/defc/thesaurus/unburnished/4.135> a skos:Concept ;
    dc:source "OREA" ;
    skos:broader <http://id.acdh.oeaw.ac.at/defc/thesaurus/pottery_surface_treatment/3.019> ;
    skos:definition "A vessle that was not polished with a dull surface." ;
    skos:editorialNote "dc_finds_pottery_decoration;135" ;
    skos:inScheme <http://id.acdh.oeaw.ac.at/defc/thesaurus/FindsPotteryDecoration>,
        <http://id.acdh.oeaw.ac.at/defc/thesaurus/FindsSchema> ;
    skos:prefLabel "Ungeglättet"@de,
        "unburnished"@en .

<http://id.acdh.oeaw.ac.at/defc/thesaurus/undefined/2.5> a skos:Concept ;
    skos:broader <http://id.acdh.oeaw.ac.at/defc/thesaurus/area_type/1.064> ;
    skos:definition "An area where archaeological evidence has been found. However, the finds were not diagnostic or the amount was too small to interpret the type of the area (settlement, grave, etc.)" ;
    skos:editorialNote "dc_area_type;5" ;
    skos:inScheme <http://id.acdh.oeaw.ac.at/defc/thesaurus/AreaSchema>,
        <http://id.acdh.oeaw.ac.at/defc/thesaurus/AreaType> ;
    skos:prefLabel "undefined"@en .

<http://id.acdh.oeaw.ac.at/defc/thesaurus/underwater_evaluation/4.10> a skos:Concept ;
    dc:source "http://thesaurus.historicengland.org.uk/thesaurus_term.asp?thes_no=566&term_no=163243" ;
    skos:broader <http://id.acdh.oeaw.ac.at/defc/thesaurus/evaluation/3.050> ;
    skos:definition "A limited programme of intrusive fieldwork which determines the presence or absence of archaeological features, structures, deposits, artefacts or ecofacts within a specified underwater area." ;
    skos:editorialNote "dc_researchevet_researchtype;10" ;
    skos:inScheme <http://id.acdh.oeaw.ac.at/defc/thesaurus/ResearchEventSchema>,
        <http://id.acdh.oeaw.ac.at/defc/thesaurus/ResearchevetResearchtype> ;
    skos:prefLabel "Testgrabung Unterwasser"@de,
        "underwater evaluation"@en .

<http://id.acdh.oeaw.ac.at/defc/thesaurus/underwater_survey/4.23> a skos:Concept ;
    dc:source "http://thesaurus.historicengland.org.uk/thesaurus_term.asp?thes_no=566&term_no=163245" ;
    skos:broader <http://id.acdh.oeaw.ac.at/defc/thesaurus/field_survey/3.052> ;
    skos:definition "The non-intrusive processes by which information is collected about the location, distribution and organisation of past human activities that are now submerged by water. The approaches can be either extensive or intensive depending on the objectives." ;
    skos:editorialNote "dc_researchevet_researchtype;23" ;
    skos:inScheme <http://id.acdh.oeaw.ac.at/defc/thesaurus/ResearchEventSchema>,
        <http://id.acdh.oeaw.ac.at/defc/thesaurus/ResearchevetResearchtype> ;
    skos:prefLabel "Unterwassersurvey"@de,
        "underwater survey"@en .

<http://id.acdh.oeaw.ac.at/defc/thesaurus/unidirectional_core/4.12> a skos:Concept ;
    dc:source "OREA" ;
    skos:broader <http://id.acdh.oeaw.ac.at/defc/thesaurus/core/3.12> ;
    skos:definition "A core with the main detachment from the one single platform" ;
    skos:editorialNote "dc_finds_lithics_core_shape;12" ;
    skos:inScheme <http://id.acdh.oeaw.ac.at/defc/thesaurus/FindsLithicsCoreShape>,
        <http://id.acdh.oeaw.ac.at/defc/thesaurus/FindsSchema> ;
    skos:prefLabel "unidirektionaler Kern"@de,
        "unidirectional core"@en .

<http://id.acdh.oeaw.ac.at/defc/thesaurus/unknown/4.110> a skos:Concept ;
    skos:broader <http://id.acdh.oeaw.ac.at/defc/thesaurus/jewellery/3.2> ;
    skos:editorialNote "dc_finds_small_finds_type;110" ;
    skos:inScheme <http://id.acdh.oeaw.ac.at/defc/thesaurus/FindsSchema>,
        <http://id.acdh.oeaw.ac.at/defc/thesaurus/FindsSmallFindsType> ;
    skos:prefLabel "unknown"@en .

<http://id.acdh.oeaw.ac.at/defc/thesaurus/unknown/4.111> a skos:Concept ;
    skos:broader <http://id.acdh.oeaw.ac.at/defc/thesaurus/tool/3.1> ;
    skos:editorialNote "dc_finds_small_finds_type;111" ;
    skos:inScheme <http://id.acdh.oeaw.ac.at/defc/thesaurus/FindsSchema>,
        <http://id.acdh.oeaw.ac.at/defc/thesaurus/FindsSmallFindsType> ;
    skos:prefLabel "unknown"@en .

<http://id.acdh.oeaw.ac.at/defc/thesaurus/unknown/4.9> a skos:Concept ;
    skos:broader <http://id.acdh.oeaw.ac.at/defc/thesaurus/animal_remains_part/3.07> ;
    skos:editorialNote "dc_animal_remains_part;9" ;
    skos:inScheme <http://id.acdh.oeaw.ac.at/defc/thesaurus/AnimalRemainsPart>,
        <http://id.acdh.oeaw.ac.at/defc/thesaurus/FindsSchema> ;
    skos:prefLabel "unknown"@en .

<http://id.acdh.oeaw.ac.at/defc/thesaurus/unknown/4.98> a skos:Concept ;
    skos:broader <http://id.acdh.oeaw.ac.at/defc/thesaurus/figurine/3.3> ;
    skos:editorialNote "dc_finds_small_finds_type;98" ;
    skos:inScheme <http://id.acdh.oeaw.ac.at/defc/thesaurus/FindsSchema>,
        <http://id.acdh.oeaw.ac.at/defc/thesaurus/FindsSmallFindsType> ;
    skos:prefLabel "unknown"@en .

<http://id.acdh.oeaw.ac.at/defc/thesaurus/v-shaped_spout/5.126> a skos:Concept ;
    dc:source "OREA" ;
    skos:broader <http://id.acdh.oeaw.ac.at/defc/thesaurus/spout/4.88> ;
    skos:definition "A V-shaped tube or lip projecting from a vessel, through which liquid can be poured." ;
    skos:editorialNote "dc_finds_pottery_detail;126" ;
    skos:inScheme <http://id.acdh.oeaw.ac.at/defc/thesaurus/FindsPotteryDetail>,
        <http://id.acdh.oeaw.ac.at/defc/thesaurus/FindsSchema> ;
    skos:prefLabel "V-förmiger Ausguss"@de,
        "v-shaped spout"@en .

<http://id.acdh.oeaw.ac.at/defc/thesaurus/valley_bottom/2.5> a skos:Concept ;
    dc:source "http://www.collinsdictionary.com/dictionary/english/valley" ;
    skos:broader "topography/1.099" ;
    skos:definition "A long depression in the land surface, usually containing a river, formed by erosion or by movements in the earth's crust."@en ;
    skos:editorialNote "dc_site_topography;5" ;
    skos:inScheme <http://id.acdh.oeaw.ac.at/defc/thesaurus/SiteSchema>,
        "SiteTopography" ;
    skos:prefLabel "Talsohle"@de,
        "valley bottom"@en .

<http://id.acdh.oeaw.ac.at/defc/thesaurus/vessel/4.94> a skos:Concept ;
    dc:source "Kipfer, B. A. Dictionary of Artifacts 2007. Blackwell Publishing, Oxford.p.333" ;
    skos:broader <http://id.acdh.oeaw.ac.at/defc/thesaurus/other/3.4> ;
    skos:definition "An object used as a container (especially for liquids) typically of clay." ;
    skos:editorialNote "dc_finds_small_finds_type;94" ;
    skos:inScheme <http://id.acdh.oeaw.ac.at/defc/thesaurus/FindsSchema>,
        <http://id.acdh.oeaw.ac.at/defc/thesaurus/FindsSmallFindsType> ;
    skos:prefLabel "Gefäß"@de,
        "vessel"@en .

<http://id.acdh.oeaw.ac.at/defc/thesaurus/vessel/5.3> a skos:Concept ;
    skos:broader <http://id.acdh.oeaw.ac.at/defc/thesaurus/grave_type/4.083> ;
    skos:editorialNote "dc_area_gravetype;3" ;
    skos:inScheme <http://id.acdh.oeaw.ac.at/defc/thesaurus/AreaGravetype>,
        <http://id.acdh.oeaw.ac.at/defc/thesaurus/AreaSchema> ;
    skos:prefLabel "Gefäß"@de,
        "vessel"@en .

<http://id.acdh.oeaw.ac.at/defc/thesaurus/wall/5.18> a skos:Concept ;
    dc:source "http://thesaurus.historicengland.org.uk/thesaurus_term.asp?thes_no=546&term_no=138407" ;
    skos:altLabel "Mauer"@de ;
    skos:broader <http://id.acdh.oeaw.ac.at/defc/thesaurus/architecture/4.081> ;
    skos:definition "An enclosing structure composed of bricks, stones, wood or similar materials, laid in courses." ;
    skos:editorialNote "dc_area_specialfeatures;18" ;
    skos:inScheme <http://id.acdh.oeaw.ac.at/defc/thesaurus/AreaSchema>,
        <http://id.acdh.oeaw.ac.at/defc/thesaurus/AreaSpecialfeatures> ;
    skos:prefLabel "wall"@en .

<http://id.acdh.oeaw.ac.at/defc/thesaurus/wall_painting/5.37> a skos:Concept ;
    skos:broader <http://id.acdh.oeaw.ac.at/defc/thesaurus/architecture/4.081> ;
    skos:editorialNote "dc_area_specialfeatures;37" ;
    skos:inScheme <http://id.acdh.oeaw.ac.at/defc/thesaurus/AreaSchema>,
        <http://id.acdh.oeaw.ac.at/defc/thesaurus/AreaSpecialfeatures> ;
    skos:prefLabel "wall painting"@en .

<http://id.acdh.oeaw.ac.at/defc/thesaurus/waste_pit/5.20> a skos:Concept ;
    dc:source "OREA" ;
    skos:altLabel "Abfallgrube"@de ;
    skos:broader <http://id.acdh.oeaw.ac.at/defc/thesaurus/installation/4.078> ;
    skos:definition "A hole dug into the ground used for rubbish disposal." ;
    skos:editorialNote "dc_area_specialfeatures;20" ;
    skos:inScheme <http://id.acdh.oeaw.ac.at/defc/thesaurus/AreaSchema>,
        <http://id.acdh.oeaw.ac.at/defc/thesaurus/AreaSpecialfeatures> ;
    skos:prefLabel "waste pit"@en .

<http://id.acdh.oeaw.ac.at/defc/thesaurus/water_vole/5.19> a skos:Concept ;
    dc:source "http://dbpedia.org/page/Water_vole" ;
    skos:broader <http://id.acdh.oeaw.ac.at/defc/thesaurus/mammal/4.020> ;
    skos:editorialNote "dc_finds_animal_remains_species;19" ;
    skos:inScheme <http://id.acdh.oeaw.ac.at/defc/thesaurus/FindsAnimalRemainsSpecies>,
        <http://id.acdh.oeaw.ac.at/defc/thesaurus/FindsSchema> ;
    skos:prefLabel "Schermaus"@de,
        "water vole"@en .

<http://id.acdh.oeaw.ac.at/defc/thesaurus/wattle_and_daub/6.6> a skos:Concept ;
    dc:source "Kipfer, B. A. Encyclopedic Dictionary of Archaeology. Kluwer Academic/Plenum Publishers, New York. p. 598." ;
    skos:altLabel "wattle"@en,
        "wattle-and-daub"@en ;
    skos:broader <http://id.acdh.oeaw.ac.at/defc/thesaurus/building_material/5.089> ;
    skos:definition "A building techniques in which walls were made by plastering mud (daub, possibly with sand and plant fibers) over a lattice of branches and sticks (wattle). Interwoven twigs or thin split timbers were used." ;
    skos:editorialNote "dc_area_buildingtechnique;6" ;
    skos:inScheme <http://id.acdh.oeaw.ac.at/defc/thesaurus/AreaBuildingtechnique>,
        <http://id.acdh.oeaw.ac.at/defc/thesaurus/AreaSchema> ;
    skos:prefLabel "wattle and daub"@en .

<http://id.acdh.oeaw.ac.at/defc/thesaurus/wedge-shaped_core/4.13> a skos:Concept ;
    dc:source "OREA" ;
    skos:broader <http://id.acdh.oeaw.ac.at/defc/thesaurus/core/3.12> ;
    skos:definition "An unidirectional blade core with crested back, usually determined by a frontal reduction. (*when the reduction is all around the platform, the core is conical, while the systematic, regular blade detachment finally leads to bullet core shape). " ;
    skos:editorialNote "dc_finds_lithics_core_shape;13" ;
    skos:inScheme <http://id.acdh.oeaw.ac.at/defc/thesaurus/FindsLithicsCoreShape>,
        <http://id.acdh.oeaw.ac.at/defc/thesaurus/FindsSchema> ;
    skos:prefLabel "wedge-shaped core"@en .

<http://id.acdh.oeaw.ac.at/defc/thesaurus/weight/4.112> a skos:Concept ;
    dc:source "Kipfer, B. A. Dictionary of Artifacts 2007. Blackwell Publishing, Oxford.p 337" ;
    skos:broader <http://id.acdh.oeaw.ac.at/defc/thesaurus/tool/3.1> ;
    skos:definition "Stone, clay, or metal object of standard weight used in measurement on balances or scales of some kind; an object used to weigh something down or to measure the weight of another object." ;
    skos:editorialNote "dc_finds_small_finds_type;112" ;
    skos:inScheme <http://id.acdh.oeaw.ac.at/defc/thesaurus/FindsSchema>,
        <http://id.acdh.oeaw.ac.at/defc/thesaurus/FindsSmallFindsType> ;
    skos:prefLabel "Gewicht"@de,
        "weight"@en .

<http://id.acdh.oeaw.ac.at/defc/thesaurus/well/5.10> a skos:Concept ;
    dc:source "http://thesaurus.historicengland.org.uk/thesaurus_term.asp?thes_no=1&term_no=70202" ;
    skos:altLabel "Brunnen"@de ;
    skos:broader <http://id.acdh.oeaw.ac.at/defc/thesaurus/installation/4.078> ;
    skos:definition "A shaft or pit dug in the ground over a supplyof spring-water." ;
    skos:editorialNote "dc_area_specialfeatures;10" ;
    skos:inScheme <http://id.acdh.oeaw.ac.at/defc/thesaurus/AreaSchema>,
        <http://id.acdh.oeaw.ac.at/defc/thesaurus/AreaSpecialfeatures> ;
    skos:prefLabel "well"@en .

<http://id.acdh.oeaw.ac.at/defc/thesaurus/white/6.275> a skos:Concept ;
    dc:source "OREA" ;
    skos:broader <http://id.acdh.oeaw.ac.at/defc/thesaurus/monochrome/5.265> ;
    skos:definition "White painted pottery decoration." ;
    skos:editorialNote "dc_finds_pottery_decoration;275" ;
    skos:inScheme <http://id.acdh.oeaw.ac.at/defc/thesaurus/FindsPotteryDecoration>,
        <http://id.acdh.oeaw.ac.at/defc/thesaurus/FindsSchema> ;
    skos:prefLabel "Weiß"@de,
        "white"@en .

<http://id.acdh.oeaw.ac.at/defc/thesaurus/white_on_black/6.181> a skos:Concept ;
    dc:source "OREA" ;
    skos:broader <http://id.acdh.oeaw.ac.at/defc/thesaurus/pattern_painted/5.041> ;
    skos:definition "Pottery painted with white paint on black ground." ;
    skos:editorialNote "dc_finds_pottery_decoration;181" ;
    skos:inScheme <http://id.acdh.oeaw.ac.at/defc/thesaurus/FindsPotteryDecoration>,
        <http://id.acdh.oeaw.ac.at/defc/thesaurus/FindsSchema> ;
    skos:prefLabel "Weiß auf schwarz"@de,
        "white on black"@en .

<http://id.acdh.oeaw.ac.at/defc/thesaurus/white_on_red/6.137> a skos:Concept ;
    dc:source "OREA" ;
    skos:broader <http://id.acdh.oeaw.ac.at/defc/thesaurus/pattern_painted/5.041> ;
    skos:definition "Pottery painted with white paint on red ground." ;
    skos:editorialNote "dc_finds_pottery_decoration;137" ;
    skos:inScheme <http://id.acdh.oeaw.ac.at/defc/thesaurus/FindsPotteryDecoration>,
        <http://id.acdh.oeaw.ac.at/defc/thesaurus/FindsSchema> ;
    skos:prefLabel "Weiß auf rot"@de,
        "white on red"@en .

<http://id.acdh.oeaw.ac.at/defc/thesaurus/white_on_red_(a3α)/6.160> a skos:Concept ;
    dc:source "OREA" ;
    skos:broader <http://id.acdh.oeaw.ac.at/defc/thesaurus/pattern_painted/5.041> ;
    skos:definition "Pottery painted with white paint on red ground." ;
    skos:editorialNote "dc_finds_pottery_decoration;160" ;
    skos:inScheme <http://id.acdh.oeaw.ac.at/defc/thesaurus/FindsPotteryDecoration>,
        <http://id.acdh.oeaw.ac.at/defc/thesaurus/FindsSchema> ;
    skos:prefLabel "Weiß auf rot (A3a)"@de,
        "white on red (a3α)"@en .

<http://id.acdh.oeaw.ac.at/defc/thesaurus/white_on_red_(β3α1)/6.161> a skos:Concept ;
    dc:source "OREA" ;
    skos:broader <http://id.acdh.oeaw.ac.at/defc/thesaurus/pattern_painted/5.041> ;
    skos:definition "Pottery painted with white paint on red ground." ;
    skos:editorialNote "dc_finds_pottery_decoration;161" ;
    skos:inScheme <http://id.acdh.oeaw.ac.at/defc/thesaurus/FindsPotteryDecoration>,
        <http://id.acdh.oeaw.ac.at/defc/thesaurus/FindsSchema> ;
    skos:prefLabel "Weiß auf rot (B3a1)"@de,
        "white on red (β3α1)"@en .

<http://id.acdh.oeaw.ac.at/defc/thesaurus/white_topped/5.285> a skos:Concept ;
    dc:source "OREA" ;
    skos:broader <http://id.acdh.oeaw.ac.at/defc/thesaurus/topped/4.035> ;
    skos:definition "Ware with white crusted rim typical for Thessaly." ;
    skos:editorialNote "dc_finds_pottery_decoration;285" ;
    skos:inScheme <http://id.acdh.oeaw.ac.at/defc/thesaurus/FindsPotteryDecoration>,
        <http://id.acdh.oeaw.ac.at/defc/thesaurus/FindsSchema> ;
    skos:prefLabel "white topped"@de,
        "white topped"@en .

<http://id.acdh.oeaw.ac.at/defc/thesaurus/wild_barley/5.18> a skos:Concept ;
    dc:source "http://eol.org/pages/1114455/overview" ;
    skos:broader <http://id.acdh.oeaw.ac.at/defc/thesaurus/cereal/4.022> ;
    skos:editorialNote "dc_botany_species;18" ;
    skos:inScheme <http://id.acdh.oeaw.ac.at/defc/thesaurus/BotanySpecies>,
        <http://id.acdh.oeaw.ac.at/defc/thesaurus/FindsSchema> ;
    skos:prefLabel "Wilde Gerste"@de,
        "wild barley"@en,
        "Hordeum vulgare subsp. spontaneum"@la .

<http://id.acdh.oeaw.ac.at/defc/thesaurus/wild_bitter_vetch/6.19> a skos:Concept ;
    dc:source "http://eol.org/pages/703201/overview" ;
    skos:broader <http://id.acdh.oeaw.ac.at/defc/thesaurus/vetch/5.33> ;
    skos:editorialNote "dc_botany_species;19" ;
    skos:inScheme <http://id.acdh.oeaw.ac.at/defc/thesaurus/BotanySpecies>,
        <http://id.acdh.oeaw.ac.at/defc/thesaurus/FindsSchema> ;
    skos:prefLabel "Wilde Linsen-Wicke"@de,
        "wild bitter vetch"@en,
        "Vicia ervilia"@la .

<http://id.acdh.oeaw.ac.at/defc/thesaurus/wild_board/5.1> a skos:Concept ;
    dc:source "http://eol.org/pages/328663/overview" ;
    skos:broader <http://id.acdh.oeaw.ac.at/defc/thesaurus/mammal/4.020> ;
    skos:editorialNote "dc_finds_animal_remains_species;1" ;
    skos:inScheme <http://id.acdh.oeaw.ac.at/defc/thesaurus/FindsAnimalRemainsSpecies>,
        <http://id.acdh.oeaw.ac.at/defc/thesaurus/FindsSchema> ;
    skos:prefLabel "Wildschwein"@de,
        "wild board"@en,
        "Sus scrofa"@la .

<http://id.acdh.oeaw.ac.at/defc/thesaurus/wild_cattle/5.38> a skos:Concept ;
    skos:broader <http://id.acdh.oeaw.ac.at/defc/thesaurus/mammal/4.020> ;
    skos:editorialNote "dc_finds_animal_remains_species;38" ;
    skos:inScheme <http://id.acdh.oeaw.ac.at/defc/thesaurus/FindsAnimalRemainsSpecies>,
        <http://id.acdh.oeaw.ac.at/defc/thesaurus/FindsSchema> ;
    skos:prefLabel "Wildrind"@de,
        "wild cattle"@en .

<http://id.acdh.oeaw.ac.at/defc/thesaurus/wild_chickpea/6.20> a skos:Concept ;
    dc:source "http://eol.org/pages/643350/overview" ;
    skos:broader <http://id.acdh.oeaw.ac.at/defc/thesaurus/pea/5.14> ;
    skos:editorialNote "dc_botany_species;20" ;
    skos:inScheme <http://id.acdh.oeaw.ac.at/defc/thesaurus/BotanySpecies>,
        <http://id.acdh.oeaw.ac.at/defc/thesaurus/FindsSchema> ;
    skos:prefLabel "Wilde Kirchererbse"@de,
        "wild chickpea"@en,
        "Cicer reticulatum"@la .

<http://id.acdh.oeaw.ac.at/defc/thesaurus/wild_einkorn/6.21> a skos:Concept ;
    dc:source "http://eol.org/data_objects/32398343" ;
    skos:broader <http://id.acdh.oeaw.ac.at/defc/thesaurus/wheat/5.39> ;
    skos:editorialNote "dc_botany_species;21" ;
    skos:inScheme <http://id.acdh.oeaw.ac.at/defc/thesaurus/BotanySpecies>,
        <http://id.acdh.oeaw.ac.at/defc/thesaurus/FindsSchema> ;
    skos:prefLabel "Wilder Einkorn"@de,
        "wild einkorn"@en,
        "Triticum monococcum subsp. baeoticum"@la .

<http://id.acdh.oeaw.ac.at/defc/thesaurus/wild_emmer/6.22> a skos:Concept ;
    dc:source "http://eol.org/pages/5835380/overview" ;
    skos:broader <http://id.acdh.oeaw.ac.at/defc/thesaurus/wheat/5.39> ;
    skos:editorialNote "dc_botany_species;22" ;
    skos:inScheme <http://id.acdh.oeaw.ac.at/defc/thesaurus/BotanySpecies>,
        <http://id.acdh.oeaw.ac.at/defc/thesaurus/FindsSchema> ;
    skos:prefLabel "Wilder Emmer"@de,
        "wild emmer"@en,
        "Triticum turgidum subsp. dicoccoides"@la .

<http://id.acdh.oeaw.ac.at/defc/thesaurus/wild_flax/4.23> a skos:Concept ;
    dc:source "http://eol.org/pages/581539/overview" ;
    skos:broader <http://id.acdh.oeaw.ac.at/defc/thesaurus/grain_crop/3.08> ;
    skos:editorialNote "dc_botany_species;23" ;
    skos:inScheme <http://id.acdh.oeaw.ac.at/defc/thesaurus/BotanySpecies>,
        <http://id.acdh.oeaw.ac.at/defc/thesaurus/FindsSchema> ;
    skos:prefLabel "Wilder Flachs"@de,
        "wild flax"@en,
        "Linum bienne"@la .

<http://id.acdh.oeaw.ac.at/defc/thesaurus/wild_goat/5.9> a skos:Concept ;
    dc:source "http://eol.org/pages/2870013/overview" ;
    skos:broader <http://id.acdh.oeaw.ac.at/defc/thesaurus/mammal/4.020> ;
    skos:editorialNote "dc_finds_animal_remains_species;9" ;
    skos:inScheme <http://id.acdh.oeaw.ac.at/defc/thesaurus/FindsAnimalRemainsSpecies>,
        <http://id.acdh.oeaw.ac.at/defc/thesaurus/FindsSchema> ;
    skos:prefLabel "Wildziege"@de,
        "wild goat"@en,
        "Capra aegagrus"@la .

<http://id.acdh.oeaw.ac.at/defc/thesaurus/wild_lentil/5.24> a skos:Concept ;
    dc:source "http://eol.org/pages/1230180/overview" ;
    skos:broader <http://id.acdh.oeaw.ac.at/defc/thesaurus/pulse/4.32> ;
    skos:editorialNote "dc_botany_species;24" ;
    skos:inScheme <http://id.acdh.oeaw.ac.at/defc/thesaurus/BotanySpecies>,
        <http://id.acdh.oeaw.ac.at/defc/thesaurus/FindsSchema> ;
    skos:prefLabel "Wilde Linse"@de,
        "wild lentil"@en,
        "Lens orientalis"@la .

<http://id.acdh.oeaw.ac.at/defc/thesaurus/wild_pea/6.25> a skos:Concept ;
    dc:source "http://eol.org/pages/1230334/overview" ;
    skos:broader <http://id.acdh.oeaw.ac.at/defc/thesaurus/pea/5.14> ;
    skos:editorialNote "dc_botany_species;25" ;
    skos:inScheme <http://id.acdh.oeaw.ac.at/defc/thesaurus/BotanySpecies>,
        <http://id.acdh.oeaw.ac.at/defc/thesaurus/FindsSchema> ;
    skos:prefLabel "Wilde Erbse"@de,
        "wild pea"@en,
        "Pisum humile"@la .

<http://id.acdh.oeaw.ac.at/defc/thesaurus/wild_plum/4.45> a skos:Concept ;
    dc:source "http://eol.org/pages/301085/overview" ;
    skos:broader <http://id.acdh.oeaw.ac.at/defc/thesaurus/fruit/3.09> ;
    skos:editorialNote "dc_botany_species;45" ;
    skos:inScheme <http://id.acdh.oeaw.ac.at/defc/thesaurus/BotanySpecies>,
        <http://id.acdh.oeaw.ac.at/defc/thesaurus/FindsSchema> ;
    skos:prefLabel "Wilde Pflaume"@de,
        "wild plum"@en,
        "Prunus americana"@la .

<http://id.acdh.oeaw.ac.at/defc/thesaurus/wild_sheep/5.7> a skos:Concept ;
    dc:source "http://eol.org/pages/4447671/overview" ;
    skos:broader <http://id.acdh.oeaw.ac.at/defc/thesaurus/mammal/4.020> ;
    skos:editorialNote "dc_finds_animal_remains_species;7" ;
    skos:inScheme <http://id.acdh.oeaw.ac.at/defc/thesaurus/FindsAnimalRemainsSpecies>,
        <http://id.acdh.oeaw.ac.at/defc/thesaurus/FindsSchema> ;
    skos:prefLabel "Wildschaf"@de,
        "wild sheep"@en,
        "Ovis orientalis"@la .

<http://id.acdh.oeaw.ac.at/defc/thesaurus/wildcat/5.24> a skos:Concept ;
    dc:source "http://eol.org/pages/328605/overview" ;
    skos:altLabel "wild cat"@en ;
    skos:broader <http://id.acdh.oeaw.ac.at/defc/thesaurus/mammal/4.020> ;
    skos:editorialNote "dc_finds_animal_remains_species;24" ;
    skos:inScheme <http://id.acdh.oeaw.ac.at/defc/thesaurus/FindsAnimalRemainsSpecies>,
        <http://id.acdh.oeaw.ac.at/defc/thesaurus/FindsSchema> ;
    skos:prefLabel "Wildkatze"@de,
        "wildcat"@en,
        "Felis silvestris"@la .

<http://id.acdh.oeaw.ac.at/defc/thesaurus/winged_strap_handle/6.154> a skos:Concept ;
    dc:source "OREA" ;
    skos:broader <http://id.acdh.oeaw.ac.at/defc/thesaurus/strap_handle/5.78> ;
    skos:definition "Strap handle with winged side." ;
    skos:editorialNote "dc_finds_pottery_detail;154" ;
    skos:inScheme <http://id.acdh.oeaw.ac.at/defc/thesaurus/FindsPotteryDetail>,
        <http://id.acdh.oeaw.ac.at/defc/thesaurus/FindsSchema> ;
    skos:prefLabel "“geflügelte” Bandhenkel"@de,
        "winged strap handle"@en .

<http://id.acdh.oeaw.ac.at/defc/thesaurus/wiped/4.237> a skos:Concept ;
    dc:source "OREA" ;
    skos:broader <http://id.acdh.oeaw.ac.at/defc/thesaurus/pottery_surface_treatment/3.019> ;
    skos:definition "Wiped surface." ;
    skos:editorialNote "dc_finds_pottery_decoration;237" ;
    skos:inScheme <http://id.acdh.oeaw.ac.at/defc/thesaurus/FindsPotteryDecoration>,
        <http://id.acdh.oeaw.ac.at/defc/thesaurus/FindsSchema> ;
    skos:prefLabel "Ausgewischt"@de,
        "wiped"@en .

<http://id.acdh.oeaw.ac.at/defc/thesaurus/wire/4.118> a skos:Concept ;
    dc:source "Kipfer, B. A. Dictionary of Artifacts 2007. Blackwell Publishing, Oxford.p 341" ;
    skos:broader <http://id.acdh.oeaw.ac.at/defc/thesaurus/other/3.4> ;
    skos:definition "Metal drawn out into a thin flexible thread or rod." ;
    skos:editorialNote "dc_finds_small_finds_type;118" ;
    skos:inScheme <http://id.acdh.oeaw.ac.at/defc/thesaurus/FindsSchema>,
        <http://id.acdh.oeaw.ac.at/defc/thesaurus/FindsSmallFindsType> ;
    skos:prefLabel "Draht"@de,
        "wire"@en .

<http://id.acdh.oeaw.ac.at/defc/thesaurus/wolf/5.26> a skos:Concept ;
    dc:source "http://eol.org/pages/328607/overview" ;
    skos:broader <http://id.acdh.oeaw.ac.at/defc/thesaurus/mammal/4.020> ;
    skos:editorialNote "dc_finds_animal_remains_species;26" ;
    skos:inScheme <http://id.acdh.oeaw.ac.at/defc/thesaurus/FindsAnimalRemainsSpecies>,
        <http://id.acdh.oeaw.ac.at/defc/thesaurus/FindsSchema> ;
    skos:prefLabel "Wolf"@de,
        "wolf"@en,
        "Canis lupus"@la .

<http://id.acdh.oeaw.ac.at/defc/thesaurus/wood/3.32> a skos:Concept ;
    dc:source "http://dbpedia.org/page/Wood" ;
    skos:broader <http://id.acdh.oeaw.ac.at/defc/thesaurus/organic/2.4> ;
    skos:definition "Wood is a porous and fibrous structural tissue found in the stems and roots of trees and other woody plants. It is an organic material, a natural composite of cellulose fibers (which are strong in tension) embedded in a matrix of lignin which resists comp" ;
    skos:editorialNote "dc_finds_material;32" ;
    skos:inScheme <http://id.acdh.oeaw.ac.at/defc/thesaurus/FindsMaterial>,
        <http://id.acdh.oeaw.ac.at/defc/thesaurus/FindsSchema> ;
    skos:prefLabel "Holz"@de,
        "wood"@en .

<http://id.acdh.oeaw.ac.at/defc/thesaurus/wooden_floor/6.19> a skos:Concept ;
    dc:source "https://en.oxforddictionaries.com/definition/floor" ;
    skos:broader <http://id.acdh.oeaw.ac.at/defc/thesaurus/floor/5.092> ;
    skos:definition "The lower surface of a room, on which one may walk, made of wood." ;
    skos:editorialNote "dc_area_buildingtechnique;19" ;
    skos:inScheme <http://id.acdh.oeaw.ac.at/defc/thesaurus/AreaBuildingtechnique>,
        <http://id.acdh.oeaw.ac.at/defc/thesaurus/AreaSchema> ;
    skos:prefLabel "Holzboden"@de,
        "wooden floor"@en .

<http://id.acdh.oeaw.ac.at/defc/thesaurus/y_blade/4.5> a skos:Concept ;
    skos:broader <http://id.acdh.oeaw.ac.at/defc/thesaurus/unretouched_tool/3.011> ;
    skos:editorialNote "dc_finds_lithics_unretouched_tools;5" ;
    skos:inScheme <http://id.acdh.oeaw.ac.at/defc/thesaurus/FindsLithicsUnretouchedTools>,
        <http://id.acdh.oeaw.ac.at/defc/thesaurus/FindsSchema> ;
    skos:prefLabel "Y Klinge"@de,
        "y blade"@en .

<http://id.acdh.oeaw.ac.at/defc/thesaurus/zoomorphic_figurine/4.83> a skos:Concept ;
    dc:source "Kipfer, B. A. Dictionary of Artifacts 2007. Blackwell Publishing, Oxford.p.113" ;
    skos:broader <http://id.acdh.oeaw.ac.at/defc/thesaurus/figurine/3.3> ;
    skos:definition "A small carved or sculpted figure of an animal, usually of clay, stone, wood, or metal." ;
    skos:editorialNote "dc_finds_small_finds_type;83" ;
    skos:inScheme <http://id.acdh.oeaw.ac.at/defc/thesaurus/FindsSchema>,
        <http://id.acdh.oeaw.ac.at/defc/thesaurus/FindsSmallFindsType> ;
    skos:prefLabel "Zoomorphe Figur"@de,
        "zoomorphic figurine"@en .

<http://id.acdh.oeaw.ac.at/defc/thesaurus/zoomorphic_handle_attachment/5.81> a skos:Concept ;
    dc:source "OREA" ;
    skos:altLabel "Tierkopfgriff"@de ;
    skos:broader <http://id.acdh.oeaw.ac.at/defc/thesaurus/attachment/4.034> ;
    skos:definition "A handhold in a shape of an animal." ;
    skos:editorialNote "dc_finds_pottery_detail;81" ;
    skos:inScheme <http://id.acdh.oeaw.ac.at/defc/thesaurus/FindsPotteryDetail>,
        <http://id.acdh.oeaw.ac.at/defc/thesaurus/FindsSchema> ;
    skos:prefLabel "Zoomorpher Griffaufsatz"@de,
        "zoomorphic handle attachment"@en .

<http://id.acdh.oeaw.ac.at/defc/thesaurus/zoomorphic_vessel/4.100> a skos:Concept ;
    dc:source "OREA" ;
    skos:broader <http://id.acdh.oeaw.ac.at/defc/thesaurus/pottery_form/3.016> ;
    skos:definition "Animal shaped vessel." ;
    skos:editorialNote "dc_finds_pottery_form;100" ;
    skos:inScheme <http://id.acdh.oeaw.ac.at/defc/thesaurus/FindsPotteryForm>,
        <http://id.acdh.oeaw.ac.at/defc/thesaurus/FindsSchema> ;
    skos:prefLabel "Zoomorphes Gefäß"@de,
        "zoomorphic vessel"@en .

<http://id.acdh.oeaw.ac.at/defc/thesaurus/çayönü_tool/4.3> a skos:Concept ;
    dc:source "Inizan, M.-L., M. Reduron-Ballinger, H. Roche, J. Tixier 1999, Technology and Terminology of Knapped Stone. Nanterre: CREP., D. Srejovic (ed) 1997, Arheološki Leksikon." ;
    skos:broader <http://id.acdh.oeaw.ac.at/defc/thesaurus/retouched_tool/3.010> ;
    skos:definition "A particular type of retouched blade appearing in the region of the Upper Mesopotamia during the Pre-Pottery Neolithic, named after the site of Çayönü. Function unknown due to the dull edges and special type fo the retouch." ;
    skos:editorialNote "dc_finds_lithics_retouched_tools;3" ;
    skos:inScheme <http://id.acdh.oeaw.ac.at/defc/thesaurus/FindsLithicsRetouchedTools>,
        <http://id.acdh.oeaw.ac.at/defc/thesaurus/FindsSchema> ;
    skos:prefLabel "Çayönü Werkzeug"@de,
        "çayönü tool"@en .

<isotopes:_carbon_(C)/3.15> a skos:Concept ;
    dc:source "http://www.sfu.museum/forensics/eng/pg_media-media_pg/isotopes/" ;
    skos:altLabel "Kohlenstoffanalyse"@de,
        "carbon analysis"@en ;
    skos:broader <http://id.acdh.oeaw.ac.at/defc/thesaurus/stable_isotope_analysis/2.061> ;
    skos:definition "Comparison of different proportions of natural occuring carbon isotope to determine the kind of environment and individual came from and their likely diet." ;
    skos:editorialNote "dc_researchevent_special_analysis;15" ;
    skos:inScheme <http://id.acdh.oeaw.ac.at/defc/thesaurus/ResearchEventSchema>,
        <http://id.acdh.oeaw.ac.at/defc/thesaurus/ResearcheventSpecialAnalysis> ;
    skos:prefLabel "Kohlenstoff (C)"@de,
        "isotopes: carbon (C)"@en .

<isotopes:_lead_(Pb)/3.16> a skos:Concept ;
    dc:source "http://oxalid.arch.ox.ac.uk/" ;
    skos:altLabel "Bleianalyse"@de,
        "lead analysis"@en ;
    skos:broader <http://id.acdh.oeaw.ac.at/defc/thesaurus/stable_isotope_analysis/2.061> ;
    skos:definition "Comparison of different proportions of natural occuring lead isotope to determine the geographical origin of ancient metals and other materials, for which minerals containing lead were used in their manufacture, for example: pigments, glass, glaze and pai" ;
    skos:editorialNote "dc_researchevent_special_analysis;16" ;
    skos:inScheme <http://id.acdh.oeaw.ac.at/defc/thesaurus/ResearchEventSchema>,
        <http://id.acdh.oeaw.ac.at/defc/thesaurus/ResearcheventSpecialAnalysis> ;
    skos:prefLabel "Blei (Pb)"@de,
        "isotopes: lead (Pb)"@en .

<isotopes:_nitrogen_(N)/3.17> a skos:Concept ;
    dc:source "http://www.sfu.museum/forensics/eng/pg_media-media_pg/isotopes/" ;
    skos:altLabel "Stickstoffanalyse"@de,
        "nitrogen analysis"@en ;
    skos:broader <http://id.acdh.oeaw.ac.at/defc/thesaurus/stable_isotope_analysis/2.061> ;
    skos:definition "Comparison of different proportions of natural occuring nitrogen isotope to determine what level of the food chain an organism was on and whether they were herbivore, a carnivore or an omnivore." ;
    skos:editorialNote "dc_researchevent_special_analysis;17" ;
    skos:inScheme <http://id.acdh.oeaw.ac.at/defc/thesaurus/ResearchEventSchema>,
        <http://id.acdh.oeaw.ac.at/defc/thesaurus/ResearcheventSpecialAnalysis> ;
    skos:prefLabel "Stickstoff (N)"@de,
        "isotopes: nitrogen (N)"@en .

<isotopes:_oxygen_(O)/3.18> a skos:Concept ;
    dc:source "http://www.sfu.museum/forensics/eng/pg_media-media_pg/isotopes/" ;
    skos:altLabel "Sauerstoffanalyse"@de,
        "oxygen analysis"@en ;
    skos:broader <http://id.acdh.oeaw.ac.at/defc/thesaurus/stable_isotope_analysis/2.061> ;
    skos:definition "Comparison of different proportions of natural occuring oxygen isotope to determine of an individual moved to different geographic areas during their lifetime or if two or more people are from the same area." ;
    skos:editorialNote "dc_researchevent_special_analysis;18" ;
    skos:inScheme <http://id.acdh.oeaw.ac.at/defc/thesaurus/ResearchEventSchema>,
        <http://id.acdh.oeaw.ac.at/defc/thesaurus/ResearcheventSpecialAnalysis> ;
    skos:prefLabel "Sauerstoff (O)"@de,
        "isotopes: oxygen (O)"@en .

<isotopes:_strontium_(Sr)/3.19> a skos:Concept ;
    dc:source "http://www.sfu.museum/forensics/eng/pg_media-media_pg/isotopes/" ;
    skos:altLabel "Strontiumanalyse"@de,
        "strontium analysis"@en ;
    skos:broader <http://id.acdh.oeaw.ac.at/defc/thesaurus/stable_isotope_analysis/2.061> ;
    skos:definition "Comparison of different proportions of natural occuring strontium isotope to determine where a person came from or to distinguish individuals whose remains are comingeld but who come from different places." ;
    skos:editorialNote "dc_researchevent_special_analysis;19" ;
    skos:inScheme <http://id.acdh.oeaw.ac.at/defc/thesaurus/ResearchEventSchema>,
        <http://id.acdh.oeaw.ac.at/defc/thesaurus/ResearcheventSpecialAnalysis> ;
    skos:prefLabel "Strontium (Sr)"@de,
        "isotopes: strontium (Sr)"@en .

<lithics:_raw_material_sourcing/3.20> a skos:Concept ;
    dc:source "OREA" ;
    skos:altLabel " sourcing"@en,
        "lithics sourcing"@en ;
    skos:broader <http://id.acdh.oeaw.ac.at/defc/thesaurus/lithics_analysis/2.062> ;
    skos:definition "An analysis to find out where the raw material of the object was obtained." ;
    skos:editorialNote "dc_researchevent_special_analysis;20" ;
    skos:inScheme <http://id.acdh.oeaw.ac.at/defc/thesaurus/ResearchEventSchema>,
        <http://id.acdh.oeaw.ac.at/defc/thesaurus/ResearcheventSpecialAnalysis> ;
    skos:prefLabel "Herkunftanalyse"@de,
        "lithics: raw material sourcing"@en .

<http://id.acdh.oeaw.ac.at/defc/thesaurus/AreaCaverockshelterstype> a skos:ConceptScheme ;
    rdfs:comment "A concept schema related to the particular Area properties." .

<http://id.acdh.oeaw.ac.at/defc/thesaurus/AreaEvidenceofgraveshumanremains> a skos:ConceptScheme ;
    rdfs:comment "A concept schema related to the particular Area properties." .

<http://id.acdh.oeaw.ac.at/defc/thesaurus/AreaSettlementtype> a skos:ConceptScheme ;
    rdfs:comment "A concept schema related to the particular Area properties." .

<http://id.acdh.oeaw.ac.at/defc/thesaurus/FindsAnimalRemainsCompletness> a skos:ConceptScheme ;
    rdfs:comment "A concept schema related to the particular Finds properties." .

<http://id.acdh.oeaw.ac.at/defc/thesaurus/cave/3.1> a skos:Concept ;
    dc:source "http://thesaurus.historicengland.org.uk/pastscape_term.asp?thes_no=1&term_no=70384" ;
    skos:broader <http://id.acdh.oeaw.ac.at/defc/thesaurus/cave_or_rockshelter/2.1> ;
    skos:definition "A subterranean feature entered from a hillside, cliff face, etc. A cave may have been used for occupation, storage, burial, refuse, or as a hide-away." ;
    skos:editorialNote "dc_area_caverockshelterstype;1" ;
    skos:inScheme <http://id.acdh.oeaw.ac.at/defc/thesaurus/AreaCaverockshelterstype>,
        <http://id.acdh.oeaw.ac.at/defc/thesaurus/AreaSchema> ;
    skos:narrower <http://id.acdh.oeaw.ac.at/defc/thesaurus/occupation_evidence/4.088> ;
    skos:prefLabel "Höhle"@de,
        "cave"@en .

<http://id.acdh.oeaw.ac.at/defc/thesaurus/cemetery_or_grave/2.2> a skos:Concept ;
    dc:source "OREA" ;
    skos:broader <http://id.acdh.oeaw.ac.at/defc/thesaurus/area_type/1.064> ;
    skos:definition "An archaeological site consisting of a grave or a complete cemetery." ;
    skos:editorialNote "dc_area_type;2" ;
    skos:inScheme <http://id.acdh.oeaw.ac.at/defc/thesaurus/AreaSchema>,
        <http://id.acdh.oeaw.ac.at/defc/thesaurus/AreaType> ;
    skos:narrower <http://id.acdh.oeaw.ac.at/defc/thesaurus/grave/3.071> ;
    skos:prefLabel "cemetery or grave"@en .

<http://id.acdh.oeaw.ac.at/defc/thesaurus/chert/5.5> a skos:Concept ;
    dc:source "Encyclopaedia Britannica - https://www.britannica.com/science/chert#ref272901" ;
    skos:altLabel "Gestein"@de ;
    skos:broader <http://id.acdh.oeaw.ac.at/defc/thesaurus/stone/4.072> ;
    skos:definition "Chert is a very fine-grained quarz and a silica mineral. Several varieties are included under the general term: jasper, chalcedony, agate, flint, porcelanite, and novaculite. It was dug at the quarry site and probably used for tools and weapon." ;
    skos:editorialNote "dc_area_rawmaterial;5" ;
    skos:inScheme <http://id.acdh.oeaw.ac.at/defc/thesaurus/AreaRawmaterial>,
        <http://id.acdh.oeaw.ac.at/defc/thesaurus/AreaSchema> ;
    skos:narrower <http://id.acdh.oeaw.ac.at/defc/thesaurus/flint/6.4> ;
    skos:prefLabel "Kieselschiefer"@de,
        "chert"@en .

<http://id.acdh.oeaw.ac.at/defc/thesaurus/duck/5.038> a skos:Concept ;
    skos:broader <http://id.acdh.oeaw.ac.at/defc/thesaurus/bird/4.36> ;
    skos:inScheme <http://id.acdh.oeaw.ac.at/defc/thesaurus/FindsSchema> ;
    skos:narrower <http://id.acdh.oeaw.ac.at/defc/thesaurus/mallard_duck/6.33> ;
    skos:prefLabel "duck"@en .

<http://id.acdh.oeaw.ac.at/defc/thesaurus/fish/4.16> a skos:Concept ;
    dc:source "http://dbpedia.org/page/Fish" ;
    skos:broader <http://id.acdh.oeaw.ac.at/defc/thesaurus/animal_remains_species/3.06> ;
    skos:editorialNote "dc_finds_animal_remains_species;16" ;
    skos:inScheme <http://id.acdh.oeaw.ac.at/defc/thesaurus/FindsAnimalRemainsSpecies>,
        <http://id.acdh.oeaw.ac.at/defc/thesaurus/FindsSchema> ;
    skos:narrower <http://id.acdh.oeaw.ac.at/defc/thesaurus/tuna/5.18> ;
    skos:prefLabel "Fisch"@de,
        "fish"@en .

<http://id.acdh.oeaw.ac.at/defc/thesaurus/jug/4.110> a skos:Concept ;
    dc:source "OREA" ;
    skos:broader <http://id.acdh.oeaw.ac.at/defc/thesaurus/pottery_form/3.016> ;
    skos:definition "A closed vessel designed for pouring, usually with a pouring lip/spout. It may have one handle or none—typically, one." ;
    skos:editorialNote "dc_finds_pottery_form;110" ;
    skos:inScheme <http://id.acdh.oeaw.ac.at/defc/thesaurus/FindsPotteryForm>,
        <http://id.acdh.oeaw.ac.at/defc/thesaurus/FindsSchema> ;
    skos:narrower <http://id.acdh.oeaw.ac.at/defc/thesaurus/beak_spouted_jug/5.216> ;
    skos:prefLabel "Krug"@de,
        "jug"@en .

<http://id.acdh.oeaw.ac.at/defc/thesaurus/lithics_analysis/2.062> a skos:Concept ;
    skos:broader <http://id.acdh.oeaw.ac.at/defc/thesaurus/special_analysis/1.057> ;
    skos:editorialNote "dc_not_in_database/2.062" ;
    skos:inScheme <http://id.acdh.oeaw.ac.at/defc/thesaurus/NotInDatabase>,
        <http://id.acdh.oeaw.ac.at/defc/thesaurus/ResearchEventSchema> ;
    skos:narrower <lithics:_raw_material_sourcing/3.20> ;
    skos:prefLabel "Steinanalyse"@de,
        "lithics analysis"@en .

<http://id.acdh.oeaw.ac.at/defc/thesaurus/male_figurine/5.85> a skos:Concept ;
    dc:source "Kipfer, B. A. Dictionary of Artifacts 2007. Blackwell Publishing, Oxford.p.113" ;
    skos:broader <http://id.acdh.oeaw.ac.at/defc/thesaurus/anthropomorphic_figurine/4.84> ;
    skos:definition "A small carved or sculpted figure of a male human, usually of clay, stone, wood, or metal." ;
    skos:editorialNote "dc_finds_small_finds_type;85" ;
    skos:inScheme <http://id.acdh.oeaw.ac.at/defc/thesaurus/FindsSchema>,
        <http://id.acdh.oeaw.ac.at/defc/thesaurus/FindsSmallFindsType> ;
    skos:narrower <http://id.acdh.oeaw.ac.at/defc/thesaurus/phallus/6.89> ;
    skos:prefLabel "Männliche Figur"@de,
        "male figurine"@en .

<http://id.acdh.oeaw.ac.at/defc/thesaurus/mineral/4.026> a skos:Concept ;
    dc:source "OREA" ;
    skos:broader <http://id.acdh.oeaw.ac.at/defc/thesaurus/lithic_material/3.015> ;
    skos:definition "A mineral used to produce lithics." ;
    skos:editorialNote "dc_not_in_database;026" ;
    skos:inScheme <http://id.acdh.oeaw.ac.at/defc/thesaurus/FindsSchema>,
        <http://id.acdh.oeaw.ac.at/defc/thesaurus/NotInDatabase> ;
    skos:narrower <http://id.acdh.oeaw.ac.at/defc/thesaurus/rock_crystal/5.7> ;
    skos:prefLabel "mineral"@en .

<http://id.acdh.oeaw.ac.at/defc/thesaurus/none_recorded/5.4> a skos:Concept ;
    dc:source "OREA" ;
    skos:broader <http://id.acdh.oeaw.ac.at/defc/thesaurus/grave_disturbance/4.084>,
        <http://id.acdh.oeaw.ac.at/defc/thesaurus/grave_type/4.083> ;
    skos:definition "The type of grave has not been recorded.",
        "There has been no disturbance or removal of the grave prior to the research conducted at the site." ;
    skos:editorialNote "dc_area_gravetype;4",
        "dc_area_manipulationofgraves;4" ;
    skos:inScheme <http://id.acdh.oeaw.ac.at/defc/thesaurus/AreaGravetype>,
        <http://id.acdh.oeaw.ac.at/defc/thesaurus/AreaManipulationofgraves>,
        <http://id.acdh.oeaw.ac.at/defc/thesaurus/AreaSchema> ;
    skos:prefLabel "nicht bestimmt"@de,
        "none recorded"@en .

<http://id.acdh.oeaw.ac.at/defc/thesaurus/obsidian/5.1> a skos:Concept ;
    dc:source "Encyclopaedia Britannica - https://www.britannica.com/science/obsidian" ;
    skos:broader <http://id.acdh.oeaw.ac.at/defc/thesaurus/stone/4.025>,
        <http://id.acdh.oeaw.ac.at/defc/thesaurus/stone/4.072> ;
    skos:definition "Obsidian, natural glass of volcanic origin (formed by the rapid cooling of viscous lava) that has been extracted at a quarry site.",
        "Obsidian, natural glass of volcanic origin that is formed by the rapid cooling of viscous lava. Obsidian is extremely rich in silica, low in water, and has a chemical composition similar to rhyolite. Used to produce lithics." ;
    skos:editorialNote "dc_area_rawmaterial;1",
        "dc_finds_lithics_raw_material;1" ;
    skos:inScheme <http://id.acdh.oeaw.ac.at/defc/thesaurus/AreaRawmaterial>,
        <http://id.acdh.oeaw.ac.at/defc/thesaurus/AreaSchema>,
        <http://id.acdh.oeaw.ac.at/defc/thesaurus/FindsLithicsRawMaterial>,
        <http://id.acdh.oeaw.ac.at/defc/thesaurus/FindsSchema> ;
    skos:prefLabel "Obsidian"@de,
        "obsidian"@en .

<http://id.acdh.oeaw.ac.at/defc/thesaurus/pillar/5.091> a skos:Concept ;
    skos:broader <http://id.acdh.oeaw.ac.at/defc/thesaurus/building_technique/4.075> ;
    skos:editorialNote "dc_not_in_database;091" ;
    skos:inScheme <http://id.acdh.oeaw.ac.at/defc/thesaurus/AreaSchema>,
        <http://id.acdh.oeaw.ac.at/defc/thesaurus/NotInDatabase> ;
    skos:narrower <http://id.acdh.oeaw.ac.at/defc/thesaurus/t-pillar/6.18> ;
    skos:prefLabel "pillar"@en .

<http://id.acdh.oeaw.ac.at/defc/thesaurus/pronged_handle/5.130> a skos:Concept ;
    dc:source "OREA" ;
    skos:broader <http://id.acdh.oeaw.ac.at/defc/thesaurus/handle/4.031> ;
    skos:definition "A handle with bar application." ;
    skos:editorialNote "dc_finds_pottery_detail;130" ;
    skos:inScheme <http://id.acdh.oeaw.ac.at/defc/thesaurus/FindsPotteryDetail>,
        <http://id.acdh.oeaw.ac.at/defc/thesaurus/FindsSchema> ;
    skos:narrower <http://id.acdh.oeaw.ac.at/defc/thesaurus/elongated_prong_handle_with_knob/6.183> ;
    skos:prefLabel "Henkel mit Stabaufsatz"@de,
        "pronged handle"@en .

<http://id.acdh.oeaw.ac.at/defc/thesaurus/reptile/4.35> a skos:Concept ;
    dc:source "http://eol.org/pages/10567249/overview" ;
    skos:broader <http://id.acdh.oeaw.ac.at/defc/thesaurus/animal_remains_species/3.06> ;
    skos:editorialNote "dc_finds_animal_remains_species;35" ;
    skos:inScheme <http://id.acdh.oeaw.ac.at/defc/thesaurus/FindsAnimalRemainsSpecies>,
        <http://id.acdh.oeaw.ac.at/defc/thesaurus/FindsSchema> ;
    skos:narrower <http://id.acdh.oeaw.ac.at/defc/thesaurus/tortoise/5.29> ;
    skos:prefLabel "Reptil"@de,
        "reptile"@en .

<http://id.acdh.oeaw.ac.at/defc/thesaurus/research_type/1.047> a skos:Concept ;
    dc:source "OREA" ;
    skos:definition "A type of research conducted during archaeological investigation." ;
    skos:editorialNote "dc_not_in_database;047" ;
    skos:inScheme <http://id.acdh.oeaw.ac.at/defc/thesaurus/ResearchEventSchema>,
        "NotInDatabase" ;
    skos:narrower <http://id.acdh.oeaw.ac.at/defc/thesaurus/intrusive/2.048>,
        <http://id.acdh.oeaw.ac.at/defc/thesaurus/non-intrusive/2.051> ;
    skos:prefLabel "Forschungsart"@de,
        "research type"@en .

<http://id.acdh.oeaw.ac.at/defc/thesaurus/round_bar_handle/5.109> a skos:Concept ;
    dc:source "OREA" ;
    skos:broader <http://id.acdh.oeaw.ac.at/defc/thesaurus/handle/4.031> ;
    skos:definition "Flattened handle with a round cross section." ;
    skos:editorialNote "dc_finds_pottery_detail;109" ;
    skos:inScheme <http://id.acdh.oeaw.ac.at/defc/thesaurus/FindsPotteryDetail>,
        <http://id.acdh.oeaw.ac.at/defc/thesaurus/FindsSchema> ;
    skos:narrower <http://id.acdh.oeaw.ac.at/defc/thesaurus/bar_handle_with_knob/6.67> ;
    skos:prefLabel "Stabhenkel"@de,
        "round bar handle"@en .

<http://id.acdh.oeaw.ac.at/defc/thesaurus/slipped/4.302> a skos:Concept ;
    dc:source "OREA" ;
    skos:altLabel "slip ware"@de ;
    skos:broader <http://id.acdh.oeaw.ac.at/defc/thesaurus/pottery_surface_treatment/3.019> ;
    skos:definition "Surface treatment of applying the slip (or coat) as a suspension of clay in water. It can be applied once or several times to the surface of the vessel with a brush, naked hand or a piece of cloth by dipping or pouring. It is applied to change the surface" ;
    skos:editorialNote "dc_finds_pottery_decoration;302" ;
    skos:inScheme <http://id.acdh.oeaw.ac.at/defc/thesaurus/FindsPotteryDecoration>,
        <http://id.acdh.oeaw.ac.at/defc/thesaurus/FindsSchema> ;
    skos:narrower <http://id.acdh.oeaw.ac.at/defc/thesaurus/red_slipped/5.134> ;
    skos:prefLabel "Ware mit Überzug"@de,
        "slipped"@en .

<http://id.acdh.oeaw.ac.at/defc/thesaurus/tab_handle/5.96> a skos:Concept ;
    dc:source "OREA" ;
    skos:altLabel "hammer rims"@en ;
    skos:broader <http://id.acdh.oeaw.ac.at/defc/thesaurus/handle/4.031> ;
    skos:definition "Flat handle." ;
    skos:editorialNote "dc_finds_pottery_detail;96" ;
    skos:inScheme <http://id.acdh.oeaw.ac.at/defc/thesaurus/FindsPotteryDetail>,
        <http://id.acdh.oeaw.ac.at/defc/thesaurus/FindsSchema> ;
    skos:narrower <http://id.acdh.oeaw.ac.at/defc/thesaurus/double_tab_handle/6.97> ;
    skos:prefLabel "Grifflappen"@de,
        "tab handle"@en .

<http://id.acdh.oeaw.ac.at/defc/thesaurus/tooth/4.11> a skos:Concept ;
    dc:source "https://en.oxforddictionaries.com/definition/tooth" ;
    skos:broader <http://id.acdh.oeaw.ac.at/defc/thesaurus/animal_remains_part/3.07> ;
    skos:definition "Each of a set of hard, bony enamel-coated structures in the jaws of most vertebrates, used for biting and chewing." ;
    skos:editorialNote "dc_animal_remains_part;11" ;
    skos:inScheme <http://id.acdh.oeaw.ac.at/defc/thesaurus/AnimalRemainsPart>,
        <http://id.acdh.oeaw.ac.at/defc/thesaurus/FindsSchema> ;
    skos:narrower <http://id.acdh.oeaw.ac.at/defc/thesaurus/tusk/5.12> ;
    skos:prefLabel "Zahn"@de,
        "tooth"@en .

<http://id.acdh.oeaw.ac.at/defc/thesaurus/wall/5.090> a skos:Concept ;
    dc:source "OREA" ;
    skos:broader <http://id.acdh.oeaw.ac.at/defc/thesaurus/building_technique/4.075> ;
    skos:definition "A wall structure inside of a building." ;
    skos:editorialNote "dc_not_in_database;090" ;
    skos:inScheme <http://id.acdh.oeaw.ac.at/defc/thesaurus/AreaSchema>,
        <http://id.acdh.oeaw.ac.at/defc/thesaurus/NotInDatabase> ;
    skos:narrower <http://id.acdh.oeaw.ac.at/defc/thesaurus/plaster_wall/6.4> ;
    skos:prefLabel "wall"@en .

<http://id.acdh.oeaw.ac.at/defc/thesaurus/AreaExplotationtype> a skos:ConceptScheme ;
    rdfs:comment "A concept schema related to the particular Area properties." .

<http://id.acdh.oeaw.ac.at/defc/thesaurus/AreaMortuaryfeatures> a skos:ConceptScheme ;
    rdfs:comment "A concept schema related to the particular Area properties." .

<http://id.acdh.oeaw.ac.at/defc/thesaurus/AreaTypeofhumanremains> a skos:ConceptScheme ;
    rdfs:comment "A concept schema related to the particular Area properties." .

<http://id.acdh.oeaw.ac.at/defc/thesaurus/FindsLithicsIndustry> a skos:ConceptScheme ;
    rdfs:comment "A concept schema related to the particular Finds properties." .

<http://id.acdh.oeaw.ac.at/defc/thesaurus/FindsLithicsTechnology> a skos:ConceptScheme ;
    rdfs:comment "A concept schema related to the particular Finds properties." .

<http://id.acdh.oeaw.ac.at/defc/thesaurus/archeobotany/2.058> a skos:Concept ;
    skos:broader <http://id.acdh.oeaw.ac.at/defc/thesaurus/special_analysis/1.057> ;
    skos:editorialNote "dc_not_in_database/2.058" ;
    skos:inScheme <http://id.acdh.oeaw.ac.at/defc/thesaurus/NotInDatabase>,
        <http://id.acdh.oeaw.ac.at/defc/thesaurus/ResearchEventSchema> ;
    skos:narrower <archaeobotany:_macro-botany/3.2>,
        <archaeobotany:_pollen/3.3> ;
    skos:prefLabel "archeobotany"@en .

<http://id.acdh.oeaw.ac.at/defc/thesaurus/beaker/4.098> a skos:Concept ;
    skos:broader <http://id.acdh.oeaw.ac.at/defc/thesaurus/pottery_form/3.016> ;
    skos:editorialNote "dc_not_in_database;098" ;
    skos:inScheme <http://id.acdh.oeaw.ac.at/defc/thesaurus/FindsSchema>,
        <http://id.acdh.oeaw.ac.at/defc/thesaurus/NotInDatabase> ;
    skos:narrower <http://id.acdh.oeaw.ac.at/defc/thesaurus/pointed_beaker/5.215>,
        <http://id.acdh.oeaw.ac.at/defc/thesaurus/tulip-shaped_beaker/5.118> ;
    skos:prefLabel "Becher"@de,
        "beaker"@en .

<http://id.acdh.oeaw.ac.at/defc/thesaurus/carinated_bowl/5.104> a skos:Concept ;
    dc:source "OREA" ;
    skos:broader <http://id.acdh.oeaw.ac.at/defc/thesaurus/bowl/4.115> ;
    skos:definition "A low, open vessel with bent walls." ;
    skos:editorialNote "dc_finds_pottery_form;104" ;
    skos:inScheme <http://id.acdh.oeaw.ac.at/defc/thesaurus/FindsPotteryForm>,
        <http://id.acdh.oeaw.ac.at/defc/thesaurus/FindsSchema> ;
    skos:narrower <http://id.acdh.oeaw.ac.at/defc/thesaurus/carinated_bowl_with_inverted_rim/6.105>,
        <http://id.acdh.oeaw.ac.at/defc/thesaurus/carinated_incurved_bowl/6.174> ;
    skos:prefLabel "Knickwandschale"@de,
        "carinated bowl"@en .

<http://id.acdh.oeaw.ac.at/defc/thesaurus/cave_or_rockshelter/2.1> a skos:Concept ;
    dc:source "OREA" ;
    skos:broader <http://id.acdh.oeaw.ac.at/defc/thesaurus/area_type/1.064> ;
    skos:definition "A cave or a rockshelter used by early humans." ;
    skos:editorialNote "dc_area_type;1" ;
    skos:inScheme <http://id.acdh.oeaw.ac.at/defc/thesaurus/AreaSchema>,
        <http://id.acdh.oeaw.ac.at/defc/thesaurus/AreaType> ;
    skos:narrower <http://id.acdh.oeaw.ac.at/defc/thesaurus/cave/3.1>,
        <http://id.acdh.oeaw.ac.at/defc/thesaurus/rock_shelter/3.2> ;
    skos:prefLabel "cave or rockshelter"@en .

<http://id.acdh.oeaw.ac.at/defc/thesaurus/ceramic_analysis/2.059> a skos:Concept ;
    skos:broader <http://id.acdh.oeaw.ac.at/defc/thesaurus/special_analysis/1.057> ;
    skos:editorialNote "dc_not_in_database/2.059" ;
    skos:inScheme <http://id.acdh.oeaw.ac.at/defc/thesaurus/NotInDatabase>,
        <http://id.acdh.oeaw.ac.at/defc/thesaurus/ResearchEventSchema> ;
    skos:narrower <ceramics:_sourcing/3.4>,
        <ceramics:_thin_section_analysis/3.5> ;
    skos:prefLabel "ceramic analysis"@en .

<http://id.acdh.oeaw.ac.at/defc/thesaurus/chert/3.12> a skos:Concept ;
    dc:source "Encyclopaedia Britannica - https://www.britannica.com/science/chert#ref272901" ;
    skos:altLabel "Gestein"@de ;
    skos:broader <http://id.acdh.oeaw.ac.at/defc/thesaurus/stone/2.1> ;
    skos:definition "Chert is a very fine-grained quarz and a silica mineral. Several varieties are included under the general term: jasper, chalcedony, agate, flint, porcelanite, and novaculite. In Neolithic it was used for tools and weapon." ;
    skos:editorialNote "dc_finds_material;12" ;
    skos:inScheme <http://id.acdh.oeaw.ac.at/defc/thesaurus/FindsMaterial>,
        <http://id.acdh.oeaw.ac.at/defc/thesaurus/FindsSchema> ;
    skos:narrower <http://id.acdh.oeaw.ac.at/defc/thesaurus/flint/4.11>,
        <http://id.acdh.oeaw.ac.at/defc/thesaurus/radiolarite/4.18> ;
    skos:prefLabel "Kieselschiefer"@de,
        "chert"@en .

<http://id.acdh.oeaw.ac.at/defc/thesaurus/chert/5.3> a skos:Concept ;
    dc:source "Encyclopaedia Britannica - https://www.britannica.com/science/chert#ref272901" ;
    skos:altLabel "Gestein"@de ;
    skos:broader <http://id.acdh.oeaw.ac.at/defc/thesaurus/stone/4.025> ;
    skos:definition "Chert is a very fine-grained quarz and a silica mineral. Several varieties are included under the general term: jasper, chalcedony, agate, flint, porcelanite, and novaculite. In Neolithic it was used for tools and weapon." ;
    skos:editorialNote "dc_finds_lithics_raw_material;3" ;
    skos:inScheme <http://id.acdh.oeaw.ac.at/defc/thesaurus/FindsLithicsRawMaterial>,
        <http://id.acdh.oeaw.ac.at/defc/thesaurus/FindsSchema> ;
    skos:narrower <http://id.acdh.oeaw.ac.at/defc/thesaurus/flint/6.2>,
        <http://id.acdh.oeaw.ac.at/defc/thesaurus/radiolarite/6.9> ;
    skos:prefLabel "Kieselschiefer"@de,
        "chert"@en .

<http://id.acdh.oeaw.ac.at/defc/thesaurus/completness_of_animal_remains/3.05> a skos:Concept ;
    skos:broader <http://id.acdh.oeaw.ac.at/defc/thesaurus/animal_remains/2.1> ;
    skos:inScheme <http://id.acdh.oeaw.ac.at/defc/thesaurus/FindsSchema> ;
    skos:narrower <http://id.acdh.oeaw.ac.at/defc/thesaurus/complete/4.1>,
        <http://id.acdh.oeaw.ac.at/defc/thesaurus/incomplete/4.2> ;
    skos:prefLabel "completness of animal remains"@en .

<http://id.acdh.oeaw.ac.at/defc/thesaurus/extremity/5.4> a skos:Concept ;
    dc:source "http://dbpedia.org/page/Limb_(anatomy)" ;
    skos:altLabel "Extrimität"@de ;
    skos:broader <http://id.acdh.oeaw.ac.at/defc/thesaurus/bone/4.021> ;
    skos:definition "A jointed, or prehensile, appendage of the human or other animal body." ;
    skos:editorialNote "dc_animal_remains_part;4" ;
    skos:inScheme <http://id.acdh.oeaw.ac.at/defc/thesaurus/AnimalRemainsPart>,
        <http://id.acdh.oeaw.ac.at/defc/thesaurus/FindsSchema> ;
    skos:narrower <http://id.acdh.oeaw.ac.at/defc/thesaurus/forelimb/6.3>,
        <http://id.acdh.oeaw.ac.at/defc/thesaurus/hindlimb/6.2> ;
    skos:prefLabel "Gliedmaß"@de,
        "extremity"@en .

<http://id.acdh.oeaw.ac.at/defc/thesaurus/floor/5.094> a skos:Concept ;
    dc:source "OREA" ;
    skos:broader <http://id.acdh.oeaw.ac.at/defc/thesaurus/architecture/4.081> ;
    skos:definition "Walking surface in an open space." ;
    skos:editorialNote "dc_not_in_database;094" ;
    skos:inScheme <http://id.acdh.oeaw.ac.at/defc/thesaurus/AreaSchema>,
        <http://id.acdh.oeaw.ac.at/defc/thesaurus/NotInDatabase> ;
    skos:narrower <http://id.acdh.oeaw.ac.at/defc/thesaurus/clay_floor/6.22>,
        <http://id.acdh.oeaw.ac.at/defc/thesaurus/plastered_floor/6.25> ;
    skos:prefLabel "floor"@en .

<http://id.acdh.oeaw.ac.at/defc/thesaurus/goose/5.037> a skos:Concept ;
    skos:broader <http://id.acdh.oeaw.ac.at/defc/thesaurus/bird/4.36> ;
    skos:inScheme <http://id.acdh.oeaw.ac.at/defc/thesaurus/FindsSchema> ;
    skos:narrower <http://id.acdh.oeaw.ac.at/defc/thesaurus/bean_goose/6.32>,
        <http://id.acdh.oeaw.ac.at/defc/thesaurus/graylag_goose/6.31> ;
    skos:prefLabel "goose"@en .

<http://id.acdh.oeaw.ac.at/defc/thesaurus/heritage_assessment/3.055> a skos:Concept ;
    skos:broader <http://id.acdh.oeaw.ac.at/defc/thesaurus/non-intrusive/2.051> ;
    skos:editorialNote "dc_not_in_database;055" ;
    skos:inScheme <http://id.acdh.oeaw.ac.at/defc/thesaurus/NotInDatabase>,
        <http://id.acdh.oeaw.ac.at/defc/thesaurus/ResearchEventSchema> ;
    skos:narrower <http://id.acdh.oeaw.ac.at/defc/thesaurus/aerial_photograph_interpretation/4.12>,
        <http://id.acdh.oeaw.ac.at/defc/thesaurus/antiquarian_observation/4.13> ;
    skos:prefLabel "heritage assessment"@en .

<http://id.acdh.oeaw.ac.at/defc/thesaurus/lithic_material/3.015> a skos:Concept ;
    dc:source "OREA" ;
    skos:broader <http://id.acdh.oeaw.ac.at/defc/thesaurus/lithics/2.3> ;
    skos:definition "Material from which lithic object was made of." ;
    skos:editorialNote "dc_not_in_database;015" ;
    skos:inScheme <http://id.acdh.oeaw.ac.at/defc/thesaurus/FindsSchema>,
        <http://id.acdh.oeaw.ac.at/defc/thesaurus/NotInDatabase> ;
    skos:narrower <http://id.acdh.oeaw.ac.at/defc/thesaurus/mineral/4.026>,
        <http://id.acdh.oeaw.ac.at/defc/thesaurus/stone/4.025> ;
    skos:prefLabel "Rohmaterial"@de,
        "lithic material"@en .

<http://id.acdh.oeaw.ac.at/defc/thesaurus/lithic_production/3.014> a skos:Concept ;
    skos:broader <http://id.acdh.oeaw.ac.at/defc/thesaurus/lithics/2.3> ;
    skos:editorialNote "dc_not_in_database;014" ;
    skos:inScheme <http://id.acdh.oeaw.ac.at/defc/thesaurus/FindsSchema>,
        <http://id.acdh.oeaw.ac.at/defc/thesaurus/NotInDatabase> ;
    skos:narrower <http://id.acdh.oeaw.ac.at/defc/thesaurus/lithics_industry/4.024>,
        <http://id.acdh.oeaw.ac.at/defc/thesaurus/lithics_technology/4.023> ;
    skos:prefLabel "lithic production"@en .

<http://id.acdh.oeaw.ac.at/defc/thesaurus/metal/2.9> a skos:Concept ;
    dc:source "https://en.oxforddictionaries.com/definition/metal" ;
    skos:broader <http://id.acdh.oeaw.ac.at/defc/thesaurus/finds_material/1.01> ;
    skos:definition "A solid material which is typically hard, shiny, malleable, fusible, and ductile, with good thermal conductivity (e.g. iron, gold, silver, steel)." ;
    skos:editorialNote "dc_finds_material;9" ;
    skos:inScheme <http://id.acdh.oeaw.ac.at/defc/thesaurus/FindsMaterial>,
        <http://id.acdh.oeaw.ac.at/defc/thesaurus/FindsSchema> ;
    skos:narrower <http://id.acdh.oeaw.ac.at/defc/thesaurus/copper/3.31>,
        <http://id.acdh.oeaw.ac.at/defc/thesaurus/gold/3.34> ;
    skos:prefLabel "Metall"@de,
        "metal"@en .

<http://id.acdh.oeaw.ac.at/defc/thesaurus/millet/5.039> a skos:Concept ;
    skos:broader <http://id.acdh.oeaw.ac.at/defc/thesaurus/cereal/4.022> ;
    skos:editorialNote "dc_not_in_database;039" ;
    skos:inScheme <http://id.acdh.oeaw.ac.at/defc/thesaurus/FindsSchema>,
        <http://id.acdh.oeaw.ac.at/defc/thesaurus/NotInDatabase> ;
    skos:narrower <http://id.acdh.oeaw.ac.at/defc/thesaurus/broomcorn_millet/6.4>,
        <http://id.acdh.oeaw.ac.at/defc/thesaurus/foxtail_millet/6.10> ;
    skos:prefLabel "millet"@en .

<http://id.acdh.oeaw.ac.at/defc/thesaurus/painted/4.239> a skos:Concept ;
    dc:source "OREA" ;
    skos:broader <http://id.acdh.oeaw.ac.at/defc/thesaurus/pottery_decoration/3.018> ;
    skos:definition "Paint applied to pottery." ;
    skos:editorialNote "dc_finds_pottery_decoration;239" ;
    skos:inScheme <http://id.acdh.oeaw.ac.at/defc/thesaurus/FindsPotteryDecoration>,
        <http://id.acdh.oeaw.ac.at/defc/thesaurus/FindsSchema> ;
    skos:narrower <http://id.acdh.oeaw.ac.at/defc/thesaurus/monochrome/5.265>,
        <http://id.acdh.oeaw.ac.at/defc/thesaurus/pattern_painted/5.041> ;
    skos:prefLabel "Bemalt"@de,
        "painted"@en .

<http://id.acdh.oeaw.ac.at/defc/thesaurus/place/4.082> a skos:Concept ;
    dc:source "OREA" ;
    skos:broader <http://id.acdh.oeaw.ac.at/defc/thesaurus/special_feature/3.070> ;
    skos:definition "A defined empty spave surrounded by one or several buildings (courtyard, square)." ;
    skos:editorialNote "dc_not_in_database;082" ;
    skos:inScheme <http://id.acdh.oeaw.ac.at/defc/thesaurus/AreaSchema>,
        <http://id.acdh.oeaw.ac.at/defc/thesaurus/NotInDatabase> ;
    skos:narrower <http://id.acdh.oeaw.ac.at/defc/thesaurus/courtyard/5.23>,
        <http://id.acdh.oeaw.ac.at/defc/thesaurus/square/5.30> ;
    skos:prefLabel "place"@en .

<http://id.acdh.oeaw.ac.at/defc/thesaurus/platform/5.093> a skos:Concept ;
    dc:source "OREA" ;
    skos:broader <http://id.acdh.oeaw.ac.at/defc/thesaurus/installation/4.078> ;
    skos:definition "A raised surface." ;
    skos:editorialNote "dc_not_in_database;093" ;
    skos:inScheme <http://id.acdh.oeaw.ac.at/defc/thesaurus/AreaSchema>,
        <http://id.acdh.oeaw.ac.at/defc/thesaurus/NotInDatabase> ;
    skos:narrower <http://id.acdh.oeaw.ac.at/defc/thesaurus/clay_platform/6.26>,
        <http://id.acdh.oeaw.ac.at/defc/thesaurus/stone_platform/6.19> ;
    skos:prefLabel "platform"@en .

<http://id.acdh.oeaw.ac.at/defc/thesaurus/projectile_point/5.70> a skos:Concept ;
    dc:source "Inizan, M.-L., M. Reduron-Ballinger, H. Roche, J. Tixier 1999, Technology and Terminology of Knapped Stone. Nanterre: CREP., D. Srejovic (ed) 1997, Arheološki Leksikon." ;
    skos:altLabel "Pfeilspitze"@de,
        "arrowhead"@en,
        "point"@en ;
    skos:broader <http://id.acdh.oeaw.ac.at/defc/thesaurus/weapon/4.030> ;
    skos:definition "A pointed retouched artefact, with or without tang for hafting, used for the purposes of hunting or warfare." ;
    skos:editorialNote "dc_finds_small_finds_type;70" ;
    skos:inScheme <http://id.acdh.oeaw.ac.at/defc/thesaurus/FindsSchema>,
        <http://id.acdh.oeaw.ac.at/defc/thesaurus/FindsSmallFindsType> ;
    skos:narrower <http://id.acdh.oeaw.ac.at/defc/thesaurus/byblos_point/6.116>,
        <http://id.acdh.oeaw.ac.at/defc/thesaurus/nemrik_point/6.117> ;
    skos:prefLabel "Projektilspitze"@de,
        "projectile point"@en .

<http://id.acdh.oeaw.ac.at/defc/thesaurus/quarry/2.3> a skos:Concept ;
    dc:source "http://thesaurus.historicengland.org.uk/thesaurus_term.asp?thes_no=1&term_no=69068" ;
    skos:altLabel "mining"@en,
        "mining site"@en ;
    skos:broader <http://id.acdh.oeaw.ac.at/defc/thesaurus/area_type/1.064> ;
    skos:definition "An excavation form which stone for building and other functions, is obtained by cutting, blasting, etc." ;
    skos:editorialNote "dc_area_type;3" ;
    skos:inScheme <http://id.acdh.oeaw.ac.at/defc/thesaurus/AreaSchema>,
        <http://id.acdh.oeaw.ac.at/defc/thesaurus/AreaType> ;
    skos:narrower <http://id.acdh.oeaw.ac.at/defc/thesaurus/quarry_type/3.065>,
        <http://id.acdh.oeaw.ac.at/defc/thesaurus/raw_material/3.066> ;
    skos:prefLabel "Steinbruch"@de,
        "quarry"@en .

<http://id.acdh.oeaw.ac.at/defc/thesaurus/remote_sensing/3.056> a skos:Concept ;
    skos:broader <http://id.acdh.oeaw.ac.at/defc/thesaurus/non-intrusive/2.051> ;
    skos:editorialNote "dc_not_in_database;056" ;
    skos:inScheme <http://id.acdh.oeaw.ac.at/defc/thesaurus/NotInDatabase>,
        <http://id.acdh.oeaw.ac.at/defc/thesaurus/ResearchEventSchema> ;
    skos:narrower <http://id.acdh.oeaw.ac.at/defc/thesaurus/airborne_laser_scanning_(ALS)/4.21>,
        <http://id.acdh.oeaw.ac.at/defc/thesaurus/satellite_imaging/4.22> ;
    skos:prefLabel "Fernerkundung"@de,
        "remote sensing"@en .

<http://id.acdh.oeaw.ac.at/defc/thesaurus/ring_handle/5.100> a skos:Concept ;
    dc:source "OREA" ;
    skos:broader <http://id.acdh.oeaw.ac.at/defc/thesaurus/handle/4.031> ;
    skos:definition "A handle with a round loop." ;
    skos:editorialNote "dc_finds_pottery_detail;100" ;
    skos:inScheme <http://id.acdh.oeaw.ac.at/defc/thesaurus/FindsPotteryDetail>,
        <http://id.acdh.oeaw.ac.at/defc/thesaurus/FindsSchema> ;
    skos:narrower <http://id.acdh.oeaw.ac.at/defc/thesaurus/small_ring_handle/6.102>,
        <http://id.acdh.oeaw.ac.at/defc/thesaurus/triangular_ring_handle/6.101> ;
    skos:prefLabel "Ringhenkel"@de,
        "ring handle"@en .

<http://id.acdh.oeaw.ac.at/defc/thesaurus/settlement_structure/3.067> a skos:Concept ;
    dc:source "OREA" ;
    skos:broader <http://id.acdh.oeaw.ac.at/defc/thesaurus/settlement/2.4> ;
    skos:definition "Organization and structure of the settlement – type of enclosure and the layout of houses." ;
    skos:editorialNote "dc_not_in_database;067" ;
    skos:inScheme <http://id.acdh.oeaw.ac.at/defc/thesaurus/AreaSchema>,
        <http://id.acdh.oeaw.ac.at/defc/thesaurus/NotInDatabase> ;
    skos:narrower <http://id.acdh.oeaw.ac.at/defc/thesaurus/house_layout/4.074>,
        <http://id.acdh.oeaw.ac.at/defc/thesaurus/settlement_enclosure/4.073> ;
    skos:prefLabel "Siedlungsstruktur"@de,
        "settlement structure"@en .

<http://id.acdh.oeaw.ac.at/defc/thesaurus/settlment_type/3.068> a skos:Concept ;
    dc:source "OREA" ;
    skos:broader <http://id.acdh.oeaw.ac.at/defc/thesaurus/settlement/2.4> ;
    skos:definition "A type of a settlement: tell or flat site." ;
    skos:editorialNote "dc_not_in_database;068" ;
    skos:inScheme <http://id.acdh.oeaw.ac.at/defc/thesaurus/AreaSchema>,
        <http://id.acdh.oeaw.ac.at/defc/thesaurus/NotInDatabase> ;
    skos:narrower <http://id.acdh.oeaw.ac.at/defc/thesaurus/flat_site/4.1>,
        <http://id.acdh.oeaw.ac.at/defc/thesaurus/tell/4.2> ;
    skos:prefLabel "Siedlungstyp"@de,
        "settlment type"@en .

<http://id.acdh.oeaw.ac.at/defc/thesaurus/shell/3.6> a skos:Concept ;
    dc:source "https://en.oxforddictionaries.com/definition/shell" ;
    skos:broader <http://id.acdh.oeaw.ac.at/defc/thesaurus/organic/2.4> ;
    skos:definition "The hard protective outer case of a mollusc or crustacean." ;
    skos:editorialNote "dc_finds_material;6" ;
    skos:inScheme <http://id.acdh.oeaw.ac.at/defc/thesaurus/FindsMaterial>,
        <http://id.acdh.oeaw.ac.at/defc/thesaurus/FindsSchema> ;
    skos:narrower <http://id.acdh.oeaw.ac.at/defc/thesaurus/cardium_shell/4.36>,
        <http://id.acdh.oeaw.ac.at/defc/thesaurus/spondylus_shell/4.4> ;
    skos:prefLabel "Schale"@de,
        "shell"@en .

<http://id.acdh.oeaw.ac.at/defc/thesaurus/spout/4.88> a skos:Concept ;
    dc:source "OREA" ;
    skos:broader <http://id.acdh.oeaw.ac.at/defc/thesaurus/pottery_detail/3.017> ;
    skos:definition "A tube or lip projecting from a vessel, through which liquid can be poured." ;
    skos:editorialNote "dc_finds_pottery_detail;88" ;
    skos:inScheme <http://id.acdh.oeaw.ac.at/defc/thesaurus/FindsPotteryDetail>,
        <http://id.acdh.oeaw.ac.at/defc/thesaurus/FindsSchema> ;
    skos:narrower <http://id.acdh.oeaw.ac.at/defc/thesaurus/bridge_spout/5.138>,
        <http://id.acdh.oeaw.ac.at/defc/thesaurus/v-shaped_spout/5.126> ;
    skos:prefLabel "Ausguss"@de,
        "spout"@en .

<http://id.acdh.oeaw.ac.at/defc/thesaurus/topped/4.035> a skos:Concept ;
    skos:broader <http://id.acdh.oeaw.ac.at/defc/thesaurus/pottery_surface_treatment/3.019> ;
    skos:editorialNote "dc_not_in_database;035" ;
    skos:inScheme <http://id.acdh.oeaw.ac.at/defc/thesaurus/FindsSchema>,
        <http://id.acdh.oeaw.ac.at/defc/thesaurus/NotInDatabase> ;
    skos:narrower <http://id.acdh.oeaw.ac.at/defc/thesaurus/red_topped/5.284>,
        <http://id.acdh.oeaw.ac.at/defc/thesaurus/white_topped/5.285> ;
    skos:prefLabel "topped"@en .

<http://id.acdh.oeaw.ac.at/defc/thesaurus/vetch/5.33> a skos:Concept ;
    dc:source "http://eol.org/pages/13463/overview" ;
    skos:broader <http://id.acdh.oeaw.ac.at/defc/thesaurus/pulse/4.32> ;
    skos:editorialNote "dc_botany_species;33" ;
    skos:inScheme <http://id.acdh.oeaw.ac.at/defc/thesaurus/BotanySpecies>,
        <http://id.acdh.oeaw.ac.at/defc/thesaurus/FindsSchema> ;
    skos:narrower <http://id.acdh.oeaw.ac.at/defc/thesaurus/bitter_vetch/6.3>,
        <http://id.acdh.oeaw.ac.at/defc/thesaurus/wild_bitter_vetch/6.19> ;
    skos:prefLabel "Wicke"@de,
        "vetch"@en,
        "Vicia"@la .

<http://id.acdh.oeaw.ac.at/defc/thesaurus/AreaManipulationofgraves> a skos:ConceptScheme ;
    rdfs:comment "A concept schema related to the particular Area properties." .

<http://id.acdh.oeaw.ac.at/defc/thesaurus/AreaSexes> a skos:ConceptScheme ;
    rdfs:comment "A concept schema related to the particular Area properties." .

<http://id.acdh.oeaw.ac.at/defc/thesaurus/SmallFindsCategory> a skos:ConceptScheme ;
    rdfs:comment "A concept schema related to the particular Finds properties." .

<http://id.acdh.oeaw.ac.at/defc/thesaurus/animal_remains/2.1> a skos:Concept ;
    dc:source "https://en.wikipedia.org/wiki/Zooarchaeology" ;
    skos:altLabel "faunal remains"@en ;
    skos:broader <http://id.acdh.oeaw.ac.at/defc/thesaurus/finds_type/1.02> ;
    skos:definition "The items left behind when an animal dies such as bones, shells, hair, chitin, scales, hides, proteins and DNA." ;
    skos:editorialNote "dc_finds_type;1" ;
    skos:inScheme <http://id.acdh.oeaw.ac.at/defc/thesaurus/FindsSchema>,
        <http://id.acdh.oeaw.ac.at/defc/thesaurus/FindsType> ;
    skos:narrower <http://id.acdh.oeaw.ac.at/defc/thesaurus/animal_remains_part/3.07>,
        <http://id.acdh.oeaw.ac.at/defc/thesaurus/animal_remains_species/3.06>,
        <http://id.acdh.oeaw.ac.at/defc/thesaurus/completness_of_animal_remains/3.05> ;
    skos:prefLabel "Tierüberreste"@de,
        "animal remains"@en .

<http://id.acdh.oeaw.ac.at/defc/thesaurus/building/3.069> a skos:Concept ;
    dc:source "OREA" ;
    skos:broader <http://id.acdh.oeaw.ac.at/defc/thesaurus/settlement/2.4> ;
    skos:definition "Describing everything in connection to a building found on a site (settlement or undifined site) such as building technique, type and shape." ;
    skos:editorialNote "dc_not_in_database;069" ;
    skos:inScheme <http://id.acdh.oeaw.ac.at/defc/thesaurus/AreaSchema>,
        <http://id.acdh.oeaw.ac.at/defc/thesaurus/NotInDatabase> ;
    skos:narrower <http://id.acdh.oeaw.ac.at/defc/thesaurus/building_shape/4.076>,
        <http://id.acdh.oeaw.ac.at/defc/thesaurus/building_technique/4.075>,
        <http://id.acdh.oeaw.ac.at/defc/thesaurus/building_type/4.077> ;
    skos:prefLabel "building"@en .

<http://id.acdh.oeaw.ac.at/defc/thesaurus/dating_method/3.045> a skos:Concept ;
    skos:editorialNote "dc_not_in_database;045" ;
    skos:inScheme <http://id.acdh.oeaw.ac.at/defc/thesaurus/PeriodSchema> ;
    skos:narrower <http://id.acdh.oeaw.ac.at/defc/thesaurus/dendrochronology/4.2>,
        <http://id.acdh.oeaw.ac.at/defc/thesaurus/material_culture/4.3>,
        <http://id.acdh.oeaw.ac.at/defc/thesaurus/none_recorded/4.4>,
        <http://id.acdh.oeaw.ac.at/defc/thesaurus/radiocarbon_dating/4.1> ;
    skos:prefLabel "Datierungsmethode"@de,
        "dating method"@en .

<http://id.acdh.oeaw.ac.at/defc/thesaurus/deer/5.036> a skos:Concept ;
    skos:broader <http://id.acdh.oeaw.ac.at/defc/thesaurus/mammal/4.020> ;
    skos:inScheme <http://id.acdh.oeaw.ac.at/defc/thesaurus/FindsSchema> ;
    skos:narrower <http://id.acdh.oeaw.ac.at/defc/thesaurus/fallow_deer/6.14>,
        <http://id.acdh.oeaw.ac.at/defc/thesaurus/red_deer/6.13>,
        <http://id.acdh.oeaw.ac.at/defc/thesaurus/roe_deer/6.23> ;
    skos:prefLabel "deer"@en .

<http://id.acdh.oeaw.ac.at/defc/thesaurus/evaluation/3.050> a skos:Concept ;
    skos:broader <http://id.acdh.oeaw.ac.at/defc/thesaurus/intrusive/2.048> ;
    skos:editorialNote "dc_not_in_database;050" ;
    skos:inScheme <http://id.acdh.oeaw.ac.at/defc/thesaurus/NotInDatabase>,
        <http://id.acdh.oeaw.ac.at/defc/thesaurus/ResearchEventSchema> ;
    skos:narrower <http://id.acdh.oeaw.ac.at/defc/thesaurus/test_pit/4.8>,
        <http://id.acdh.oeaw.ac.at/defc/thesaurus/trial_trench/4.9>,
        <http://id.acdh.oeaw.ac.at/defc/thesaurus/underwater_evaluation/4.10> ;
    skos:prefLabel "Evaluierung"@de,
        "evaluation"@en .

<http://id.acdh.oeaw.ac.at/defc/thesaurus/field_walking_survey/4.053> a skos:Concept ;
    skos:broader <http://id.acdh.oeaw.ac.at/defc/thesaurus/field_survey/3.052> ;
    skos:editorialNote "dc_not_in_database;053" ;
    skos:inScheme <http://id.acdh.oeaw.ac.at/defc/thesaurus/NotInDatabase>,
        <http://id.acdh.oeaw.ac.at/defc/thesaurus/ResearchEventSchema> ;
    skos:narrower <http://id.acdh.oeaw.ac.at/defc/thesaurus/field_walking_survey%3A_non-systematic%2F5.15>,
        <http://id.acdh.oeaw.ac.at/defc/thesaurus/field_walking_survey%3A_systematic%2F5.16>,
        <http://id.acdh.oeaw.ac.at/defc/thesaurus/field_walking_survey%3A_undetermined%2F5.11> ;
    skos:prefLabel "Feldbegehung"@de,
        "Feldbegehung: nicht bestimmt"@de,
        "systematisch Feldbegehung"@de,
        "unsystematisch Feldbegehung"@de,
        "field walking survey"@en .

<http://id.acdh.oeaw.ac.at/defc/thesaurus/fishing_object/4.027> a skos:Concept ;
    dc:source "OREA" ;
    skos:broader <http://id.acdh.oeaw.ac.at/defc/thesaurus/tool/3.1> ;
    skos:definition "An object used for fishing." ;
    skos:editorialNote "dc_not_in_database;027" ;
    skos:inScheme <http://id.acdh.oeaw.ac.at/defc/thesaurus/FindsSchema>,
        <http://id.acdh.oeaw.ac.at/defc/thesaurus/NotInDatabase> ;
    skos:narrower <http://id.acdh.oeaw.ac.at/defc/thesaurus/anchor/5.93>,
        <http://id.acdh.oeaw.ac.at/defc/thesaurus/fish_hook/5.45>,
        <http://id.acdh.oeaw.ac.at/defc/thesaurus/net_sinker/5.51> ;
    skos:prefLabel "fishing object"@en .

<http://id.acdh.oeaw.ac.at/defc/thesaurus/floor/5.092> a skos:Concept ;
    dc:source "OREA" ;
    skos:broader <http://id.acdh.oeaw.ac.at/defc/thesaurus/building_technique/4.075> ;
    skos:definition "A floor construction inside of a building." ;
    skos:editorialNote "dc_not_in_database;092" ;
    skos:inScheme <http://id.acdh.oeaw.ac.at/defc/thesaurus/AreaSchema>,
        <http://id.acdh.oeaw.ac.at/defc/thesaurus/NotInDatabase> ;
    skos:narrower <http://id.acdh.oeaw.ac.at/defc/thesaurus/limestone_floor/6.20>,
        <http://id.acdh.oeaw.ac.at/defc/thesaurus/terrazzo_floor/6.15>,
        <http://id.acdh.oeaw.ac.at/defc/thesaurus/wooden_floor/6.19> ;
    skos:prefLabel "floor"@en .

<http://id.acdh.oeaw.ac.at/defc/thesaurus/geophysical_survey/4.054> a skos:Concept ;
    skos:broader <http://id.acdh.oeaw.ac.at/defc/thesaurus/field_survey/3.052> ;
    skos:editorialNote "dc_not_in_database;054" ;
    skos:inScheme <http://id.acdh.oeaw.ac.at/defc/thesaurus/NotInDatabase>,
        <http://id.acdh.oeaw.ac.at/defc/thesaurus/ResearchEventSchema> ;
    skos:narrower <http://id.acdh.oeaw.ac.at/defc/thesaurus/geophysical_survey%3A_magnetic%2F5.17>,
        <http://id.acdh.oeaw.ac.at/defc/thesaurus/geophysical_survey%3A_radar%2F5.18>,
        <http://id.acdh.oeaw.ac.at/defc/thesaurus/metal_detecting_survey/5.20> ;
    skos:prefLabel "Bodenradarmessung"@de,
        "Feldbegehung mit Metalldetektor"@de,
        "geomagnetische Messung"@de,
        "geophysicalischer Survey"@de,
        "geophysical survey"@en .

<http://id.acdh.oeaw.ac.at/defc/thesaurus/grinding_equipment/4.029> a skos:Concept ;
    dc:source "OREA" ;
    skos:broader <http://id.acdh.oeaw.ac.at/defc/thesaurus/tool/3.1> ;
    skos:definition "Tools used for grinding." ;
    skos:editorialNote "dc_not_in_database;029" ;
    skos:inScheme <http://id.acdh.oeaw.ac.at/defc/thesaurus/FindsSchema>,
        <http://id.acdh.oeaw.ac.at/defc/thesaurus/NotInDatabase> ;
    skos:narrower <http://id.acdh.oeaw.ac.at/defc/thesaurus/grindstone/5.58>,
        <http://id.acdh.oeaw.ac.at/defc/thesaurus/mortar/5.49>,
        <http://id.acdh.oeaw.ac.at/defc/thesaurus/pestle/5.60> ;
    skos:prefLabel "grinding equipment"@en .

<http://id.acdh.oeaw.ac.at/defc/thesaurus/house_layout/4.074> a skos:Concept ;
    dc:source "OREA" ;
    skos:broader <http://id.acdh.oeaw.ac.at/defc/thesaurus/settlement_structure/3.067> ;
    skos:definition "A system according to which houses in a settlement are arranged." ;
    skos:editorialNote "dc_not_in_database;074" ;
    skos:inScheme <http://id.acdh.oeaw.ac.at/defc/thesaurus/AreaSchema>,
        <http://id.acdh.oeaw.ac.at/defc/thesaurus/NotInDatabase> ;
    skos:narrower <http://id.acdh.oeaw.ac.at/defc/thesaurus/houses_agglutinated/5.5>,
        <http://id.acdh.oeaw.ac.at/defc/thesaurus/houses_free-standing/5.4>,
        <http://id.acdh.oeaw.ac.at/defc/thesaurus/houses_radial/5.6> ;
    skos:prefLabel "house layout"@en .

<http://id.acdh.oeaw.ac.at/defc/thesaurus/human_remains_type/5.096> a skos:Concept ;
    skos:broader <http://id.acdh.oeaw.ac.at/defc/thesaurus/human_remains/4.085> ;
    skos:editorialNote "dc_not_in_database;096" ;
    skos:inScheme <http://id.acdh.oeaw.ac.at/defc/thesaurus/AreaSchema>,
        <http://id.acdh.oeaw.ac.at/defc/thesaurus/NotInDatabase> ;
    skos:narrower <http://id.acdh.oeaw.ac.at/defc/thesaurus/cremation/6.1>,
        <http://id.acdh.oeaw.ac.at/defc/thesaurus/inhumation/6.2>,
        <http://id.acdh.oeaw.ac.at/defc/thesaurus/secondary_deposition/6.3> ;
    skos:prefLabel "Art der menschlichen Überreste"@de,
        "human remains type"@en .

<http://id.acdh.oeaw.ac.at/defc/thesaurus/lithics_industry/4.024> a skos:Concept ;
    skos:broader <http://id.acdh.oeaw.ac.at/defc/thesaurus/lithic_production/3.014> ;
    skos:editorialNote "dc_not_in_database;024" ;
    skos:inScheme <http://id.acdh.oeaw.ac.at/defc/thesaurus/FindsSchema>,
        <http://id.acdh.oeaw.ac.at/defc/thesaurus/NotInDatabase> ;
    skos:narrower <http://id.acdh.oeaw.ac.at/defc/thesaurus/blade_industry/5.1>,
        <http://id.acdh.oeaw.ac.at/defc/thesaurus/flake_industry/5.2>,
        <http://id.acdh.oeaw.ac.at/defc/thesaurus/microlithic_industry/5.3> ;
    skos:prefLabel "Industrie"@de,
        "lithics industry"@en .

<http://id.acdh.oeaw.ac.at/defc/thesaurus/lithics_technology/4.023> a skos:Concept ;
    skos:broader <http://id.acdh.oeaw.ac.at/defc/thesaurus/lithic_production/3.014> ;
    skos:editorialNote "dc_not_in_database;023" ;
    skos:inScheme <http://id.acdh.oeaw.ac.at/defc/thesaurus/FindsSchema>,
        <http://id.acdh.oeaw.ac.at/defc/thesaurus/NotInDatabase> ;
    skos:narrower <http://id.acdh.oeaw.ac.at/defc/thesaurus/direct_percussion/5.1>,
        <http://id.acdh.oeaw.ac.at/defc/thesaurus/indirect_percussion/5.2>,
        <http://id.acdh.oeaw.ac.at/defc/thesaurus/pressure_technique/5.3> ;
    skos:prefLabel "Technologie"@de,
        "lithics technology"@en .

<http://id.acdh.oeaw.ac.at/defc/thesaurus/metal/4.7> a skos:Concept ;
    dc:source "https://en.oxforddictionaries.com/definition/metal" ;
    skos:broader <http://id.acdh.oeaw.ac.at/defc/thesaurus/raw_material/3.066> ;
    skos:definition "A solid material which is typically hard, shiny, malleable, fusible, and ductile, with good thermal conductivity (e.g. iron, gold, silver, steel) extracted from a quarry site." ;
    skos:editorialNote "dc_area_rawmaterial;7" ;
    skos:inScheme <http://id.acdh.oeaw.ac.at/defc/thesaurus/AreaRawmaterial>,
        <http://id.acdh.oeaw.ac.at/defc/thesaurus/AreaSchema> ;
    skos:narrower <http://id.acdh.oeaw.ac.at/defc/thesaurus/copper/5.2>,
        <http://id.acdh.oeaw.ac.at/defc/thesaurus/lead/5.10>,
        <http://id.acdh.oeaw.ac.at/defc/thesaurus/silver/5.9> ;
    skos:prefLabel "Metall"@de,
        "metal"@en .

<http://id.acdh.oeaw.ac.at/defc/thesaurus/morturary_feature/4.086> a skos:Concept ;
    skos:broader <http://id.acdh.oeaw.ac.at/defc/thesaurus/grave/3.071> ;
    skos:editorialNote "dc_not_in_database;086" ;
    skos:inScheme <http://id.acdh.oeaw.ac.at/defc/thesaurus/AreaSchema>,
        <http://id.acdh.oeaw.ac.at/defc/thesaurus/NotInDatabase> ;
    skos:narrower <http://id.acdh.oeaw.ac.at/defc/thesaurus/platform/5.3>,
        <http://id.acdh.oeaw.ac.at/defc/thesaurus/pyre/5.1>,
        <http://id.acdh.oeaw.ac.at/defc/thesaurus/separating_wall/5.2> ;
    skos:prefLabel "Befunde"@de,
        "morturary feature"@en .

<http://id.acdh.oeaw.ac.at/defc/thesaurus/nuts/4.31> a skos:Concept ;
    dc:source "http://dbpedia.org/page/Nut_(fruit)" ;
    skos:broader <http://id.acdh.oeaw.ac.at/defc/thesaurus/fruit/3.09> ;
    skos:editorialNote "dc_botany_species;31" ;
    skos:inScheme <http://id.acdh.oeaw.ac.at/defc/thesaurus/BotanySpecies>,
        <http://id.acdh.oeaw.ac.at/defc/thesaurus/FindsSchema> ;
    skos:narrower <http://id.acdh.oeaw.ac.at/defc/thesaurus/acorn/5.35>,
        <http://id.acdh.oeaw.ac.at/defc/thesaurus/almond/5.30>,
        <http://id.acdh.oeaw.ac.at/defc/thesaurus/pistachio/5.28> ;
    skos:prefLabel "Nuß"@de,
        "nuts"@en .

<http://id.acdh.oeaw.ac.at/defc/thesaurus/pottery_decoration/3.018> a skos:Concept ;
    skos:broader <http://id.acdh.oeaw.ac.at/defc/thesaurus/pottery/2.4> ;
    skos:editorialNote "dc_not_in_database;018" ;
    skos:inScheme <http://id.acdh.oeaw.ac.at/defc/thesaurus/FindsSchema>,
        <http://id.acdh.oeaw.ac.at/defc/thesaurus/NotInDatabase> ;
    skos:narrower <http://id.acdh.oeaw.ac.at/defc/thesaurus/incised/4.168>,
        <http://id.acdh.oeaw.ac.at/defc/thesaurus/painted/4.239>,
        <http://id.acdh.oeaw.ac.at/defc/thesaurus/plastic_decoration/4.132> ;
    skos:prefLabel "Keramikdekor"@de,
        "pottery decoration"@en .

<http://id.acdh.oeaw.ac.at/defc/thesaurus/quarry_type/3.065> a skos:Concept ;
    dc:source "OREA" ;
    skos:broader <http://id.acdh.oeaw.ac.at/defc/thesaurus/quarry/2.3> ;
    skos:definition "A type of evidence pointing to the existence of a quarry" ;
    skos:editorialNote "dc_not_in_database;065" ;
    skos:inScheme <http://id.acdh.oeaw.ac.at/defc/thesaurus/AreaSchema>,
        <http://id.acdh.oeaw.ac.at/defc/thesaurus/NotInDatabase> ;
    skos:narrower <http://id.acdh.oeaw.ac.at/defc/thesaurus/mine_shaft/4.2>,
        <http://id.acdh.oeaw.ac.at/defc/thesaurus/pinge/4.1>,
        <http://id.acdh.oeaw.ac.at/defc/thesaurus/surface/4.3> ;
    skos:prefLabel "Abbauart"@de,
        "quarry type"@en .

<http://id.acdh.oeaw.ac.at/defc/thesaurus/stone/4.072> a skos:Concept ;
    dc:source "OREA" ;
    skos:altLabel "rock"@en ;
    skos:broader <http://id.acdh.oeaw.ac.at/defc/thesaurus/raw_material/3.066> ;
    skos:definition "Stone that has been extraced from a querry site." ;
    skos:editorialNote "dc_not_in_database;072" ;
    skos:inScheme <http://id.acdh.oeaw.ac.at/defc/thesaurus/AreaSchema>,
        <http://id.acdh.oeaw.ac.at/defc/thesaurus/NotInDatabase> ;
    skos:narrower <http://id.acdh.oeaw.ac.at/defc/thesaurus/chert/5.5>,
        <http://id.acdh.oeaw.ac.at/defc/thesaurus/limestone/5.3>,
        <http://id.acdh.oeaw.ac.at/defc/thesaurus/obsidian/5.1> ;
    skos:prefLabel "Stein"@de,
        "stone"@en .

<http://id.acdh.oeaw.ac.at/defc/thesaurus/wishbone_handle/5.93> a skos:Concept ;
    dc:source "OREA" ;
    skos:altLabel "Wishbonehenkel"@de ;
    skos:broader <http://id.acdh.oeaw.ac.at/defc/thesaurus/handle/4.031> ;
    skos:definition "A liminal horizontal loop handle with a bird-bone shape." ;
    skos:editorialNote "dc_finds_pottery_detail;93" ;
    skos:inScheme <http://id.acdh.oeaw.ac.at/defc/thesaurus/FindsPotteryDetail>,
        <http://id.acdh.oeaw.ac.at/defc/thesaurus/FindsSchema> ;
    skos:narrower <http://id.acdh.oeaw.ac.at/defc/thesaurus/double-horned_wishbone_handle/6.156>,
        <http://id.acdh.oeaw.ac.at/defc/thesaurus/knobbed_wishbone_handle/6.144>,
        <http://id.acdh.oeaw.ac.at/defc/thesaurus/pronged_wishbone_handle/6.148> ;
    skos:prefLabel "Gabelhenkel"@de,
        "wishbone handle"@en .

<http://id.acdh.oeaw.ac.at/defc/thesaurus/AreaConstructionshape> a skos:ConceptScheme ;
    rdfs:comment "A concept schema related to the particular Area properties." .

<http://id.acdh.oeaw.ac.at/defc/thesaurus/AreaTopography> a skos:ConceptScheme ;
    rdfs:comment "A concept schema related to the particular Area properties." .

<http://id.acdh.oeaw.ac.at/defc/thesaurus/AreaType> a skos:ConceptScheme ;
    rdfs:comment "A concept schema related to the particular Area properties." .

<http://id.acdh.oeaw.ac.at/defc/thesaurus/FindsLithicsUnretouchedTools> a skos:ConceptScheme ;
    rdfs:comment "A concept schema related to the particular Finds properties." .

<http://id.acdh.oeaw.ac.at/defc/thesaurus/FindsType> a skos:ConceptScheme ;
    rdfs:comment "A concept schema related to the particular Finds properties." .

<http://id.acdh.oeaw.ac.at/defc/thesaurus/anthropomorphic_figurine/4.84> a skos:Concept ;
    dc:source "Kipfer, B. A. Dictionary of Artifacts 2007. Blackwell Publishing, Oxford.p.113" ;
    skos:broader <http://id.acdh.oeaw.ac.at/defc/thesaurus/figurine/3.3> ;
    skos:definition "A small carved or sculpted figure of a human, usually of clay, stone, wood, or metal." ;
    skos:editorialNote "dc_finds_small_finds_type;84" ;
    skos:inScheme <http://id.acdh.oeaw.ac.at/defc/thesaurus/FindsSchema>,
        <http://id.acdh.oeaw.ac.at/defc/thesaurus/FindsSmallFindsType> ;
    skos:narrower <http://id.acdh.oeaw.ac.at/defc/thesaurus/acrolith/5.92>,
        <http://id.acdh.oeaw.ac.at/defc/thesaurus/female_figurine/5.86>,
        <http://id.acdh.oeaw.ac.at/defc/thesaurus/kiliya_figurine/5.136>,
        <http://id.acdh.oeaw.ac.at/defc/thesaurus/male_figurine/5.85> ;
    skos:prefLabel "Anthropomorphe Figur"@de,
        "anthropomorphic figurine"@en .

<http://id.acdh.oeaw.ac.at/defc/thesaurus/area_type/1.064> a skos:Concept ;
    dc:source "OREA" ;
    skos:definition "A type of an archaeological site: settlement, cave or rockshelter, grave and cemetery, quarry, undefined." ;
    skos:editorialNote "dc_not_in_database;064" ;
    skos:inScheme <http://id.acdh.oeaw.ac.at/defc/thesaurus/AreaSchema>,
        <http://id.acdh.oeaw.ac.at/defc/thesaurus/NotInDatabase> ;
    skos:narrower <http://id.acdh.oeaw.ac.at/defc/thesaurus/cave_or_rockshelter/2.1>,
        <http://id.acdh.oeaw.ac.at/defc/thesaurus/cemetery_or_grave/2.2>,
        <http://id.acdh.oeaw.ac.at/defc/thesaurus/quarry/2.3>,
        <http://id.acdh.oeaw.ac.at/defc/thesaurus/settlement/2.4>,
        <http://id.acdh.oeaw.ac.at/defc/thesaurus/undefined/2.5> ;
    skos:prefLabel "Grabungsareal Kategorie"@de,
        "area type"@en .

<http://id.acdh.oeaw.ac.at/defc/thesaurus/attachment/4.034> a skos:Concept ;
    skos:broader <http://id.acdh.oeaw.ac.at/defc/thesaurus/pottery_detail/3.017> ;
    skos:editorialNote "dc_not_in_database;034" ;
    skos:inScheme <http://id.acdh.oeaw.ac.at/defc/thesaurus/FindsSchema>,
        <http://id.acdh.oeaw.ac.at/defc/thesaurus/NotInDatabase> ;
    skos:narrower <http://id.acdh.oeaw.ac.at/defc/thesaurus/knob-row/5.99>,
        <http://id.acdh.oeaw.ac.at/defc/thesaurus/knob/5.74>,
        <http://id.acdh.oeaw.ac.at/defc/thesaurus/rim_attachment/5.94>,
        <http://id.acdh.oeaw.ac.at/defc/thesaurus/zoomorphic_handle_attachment/5.81> ;
    skos:prefLabel "attachment"@en .

<http://id.acdh.oeaw.ac.at/defc/thesaurus/base/4.032> a skos:Concept ;
    skos:broader <http://id.acdh.oeaw.ac.at/defc/thesaurus/pottery_detail/3.017> ;
    skos:editorialNote "dc_not_in_database;032" ;
    skos:inScheme <http://id.acdh.oeaw.ac.at/defc/thesaurus/FindsSchema>,
        <http://id.acdh.oeaw.ac.at/defc/thesaurus/NotInDatabase> ;
    skos:narrower <http://id.acdh.oeaw.ac.at/defc/thesaurus/concave_flat_base/5.139>,
        <http://id.acdh.oeaw.ac.at/defc/thesaurus/flat_base/5.86>,
        <http://id.acdh.oeaw.ac.at/defc/thesaurus/ring_base/5.180>,
        <http://id.acdh.oeaw.ac.at/defc/thesaurus/rounded_base/5.165> ;
    skos:prefLabel "base"@en .

<http://id.acdh.oeaw.ac.at/defc/thesaurus/core/3.12> a skos:Concept ;
    skos:broader <http://id.acdh.oeaw.ac.at/defc/thesaurus/lithics/2.3> ;
    skos:inScheme <http://id.acdh.oeaw.ac.at/defc/thesaurus/FindsSchema> ;
    skos:narrower <http://id.acdh.oeaw.ac.at/defc/thesaurus/flake_core/4.9>,
        <http://id.acdh.oeaw.ac.at/defc/thesaurus/naviform_core/4.10>,
        <http://id.acdh.oeaw.ac.at/defc/thesaurus/unidirectional_core/4.12>,
        <http://id.acdh.oeaw.ac.at/defc/thesaurus/wedge-shaped_core/4.13> ;
    skos:prefLabel "core"@en .

<http://id.acdh.oeaw.ac.at/defc/thesaurus/core_preparation/3.013> a skos:Concept ;
    skos:broader <http://id.acdh.oeaw.ac.at/defc/thesaurus/lithics/2.3> ;
    skos:inScheme <http://id.acdh.oeaw.ac.at/defc/thesaurus/FindsSchema> ;
    skos:narrower <http://id.acdh.oeaw.ac.at/defc/thesaurus/cortical_blade/4.6>,
        <http://id.acdh.oeaw.ac.at/defc/thesaurus/crested_blade/4.7>,
        <http://id.acdh.oeaw.ac.at/defc/thesaurus/crested_flake/4.8>,
        <http://id.acdh.oeaw.ac.at/defc/thesaurus/tablet/4.11> ;
    skos:prefLabel "core preparation"@en .

<http://id.acdh.oeaw.ac.at/defc/thesaurus/dating_material/3.046> a skos:Concept ;
    dc:source "OREA" ;
    skos:definition "Material used for dating procedures (using radiocarbon dating)." ;
    skos:editorialNote "dc_not_in_database;046" ;
    skos:inScheme <http://id.acdh.oeaw.ac.at/defc/thesaurus/PeriodSchema> ;
    skos:narrower <http://id.acdh.oeaw.ac.at/defc/thesaurus/bone/4.2>,
        <http://id.acdh.oeaw.ac.at/defc/thesaurus/ceramics/4.5>,
        <http://id.acdh.oeaw.ac.at/defc/thesaurus/charcoal/4.1>,
        <http://id.acdh.oeaw.ac.at/defc/thesaurus/grain/4.3>,
        <http://id.acdh.oeaw.ac.at/defc/thesaurus/seed/4.4> ;
    skos:prefLabel "Datierbaresmaterial"@de,
        "dating material"@en .

<http://id.acdh.oeaw.ac.at/defc/thesaurus/excavation/3.049> a skos:Concept ;
    skos:broader <http://id.acdh.oeaw.ac.at/defc/thesaurus/intrusive/2.048> ;
    skos:editorialNote "dc_not_in_database;049" ;
    skos:inScheme <http://id.acdh.oeaw.ac.at/defc/thesaurus/NotInDatabase>,
        <http://id.acdh.oeaw.ac.at/defc/thesaurus/ResearchEventSchema> ;
    skos:narrower <excavation:_rescue/4.2>,
        <excavation:_research/4.3>,
        <excavation:_underwater/4.4>,
        <excavation:_undetermined/4.5> ;
    skos:prefLabel "Ausgrabung"@de,
        "excavation"@en .

<http://id.acdh.oeaw.ac.at/defc/thesaurus/finds_type/1.02> a skos:Concept ;
    dc:source "DARIAH backbone thesaurus v 1.2 - http://83.212.168.219/DariahCrete/en/bbt_intro_en" ;
    skos:definition "This term classifies material things that result from human endeavor, have aesthetic, cultural, historical, scientific, or other utilirarian value, and are by design or through collecting portable functional entities (animal remains, botany, small finds and lithics)." ;
    skos:editorialNote "dc_not_in_database;02" ;
    skos:inScheme <http://id.acdh.oeaw.ac.at/defc/thesaurus/FindsSchema>,
        <http://id.acdh.oeaw.ac.at/defc/thesaurus/NotInDatabase> ;
    skos:narrower <http://id.acdh.oeaw.ac.at/defc/thesaurus/animal_remains/2.1>,
        <http://id.acdh.oeaw.ac.at/defc/thesaurus/botany/2.2>,
        <http://id.acdh.oeaw.ac.at/defc/thesaurus/lithics/2.3>,
        <http://id.acdh.oeaw.ac.at/defc/thesaurus/pottery/2.4>,
        <http://id.acdh.oeaw.ac.at/defc/thesaurus/small_finds/2.5> ;
    skos:prefLabel "Fundtypus"@de,
        "finds type"@en .

<http://id.acdh.oeaw.ac.at/defc/thesaurus/grave_disturbance/4.084> a skos:Concept ;
    skos:broader <http://id.acdh.oeaw.ac.at/defc/thesaurus/grave/3.071> ;
    skos:editorialNote "dc_not_in_database;084" ;
    skos:inScheme <http://id.acdh.oeaw.ac.at/defc/thesaurus/AreaSchema>,
        <http://id.acdh.oeaw.ac.at/defc/thesaurus/NotInDatabase> ;
    skos:narrower <http://id.acdh.oeaw.ac.at/defc/thesaurus/consecutive_burials/5.1>,
        <http://id.acdh.oeaw.ac.at/defc/thesaurus/construction_of_settlement/5.2>,
        <http://id.acdh.oeaw.ac.at/defc/thesaurus/looting/5.3>,
        <http://id.acdh.oeaw.ac.at/defc/thesaurus/none_recorded/5.4> ;
    skos:prefLabel "Grabmanupulation"@de,
        "grave disturbance"@en .

<http://id.acdh.oeaw.ac.at/defc/thesaurus/lug/5.040> a skos:Concept ;
    skos:broader <http://id.acdh.oeaw.ac.at/defc/thesaurus/handle/4.031> ;
    skos:editorialNote "dc_not_in_database;040" ;
    skos:inScheme <http://id.acdh.oeaw.ac.at/defc/thesaurus/FindsSchema>,
        <http://id.acdh.oeaw.ac.at/defc/thesaurus/NotInDatabase> ;
    skos:narrower <http://id.acdh.oeaw.ac.at/defc/thesaurus/elephant_lug/6.68>,
        <http://id.acdh.oeaw.ac.at/defc/thesaurus/ledge_lug/6.70>,
        <http://id.acdh.oeaw.ac.at/defc/thesaurus/stringhole_lug/6.79>,
        <http://id.acdh.oeaw.ac.at/defc/thesaurus/tubular_lug/6.80> ;
    skos:prefLabel "lug"@en .

<http://id.acdh.oeaw.ac.at/defc/thesaurus/pea/5.14> a skos:Concept ;
    dc:source "http://eol.org/pages/703192/overview" ;
    skos:broader <http://id.acdh.oeaw.ac.at/defc/thesaurus/pulse/4.32> ;
    skos:editorialNote "dc_botany_species;14" ;
    skos:inScheme <http://id.acdh.oeaw.ac.at/defc/thesaurus/BotanySpecies>,
        <http://id.acdh.oeaw.ac.at/defc/thesaurus/FindsSchema> ;
    skos:narrower <http://id.acdh.oeaw.ac.at/defc/thesaurus/chickpea/6.5>,
        <http://id.acdh.oeaw.ac.at/defc/thesaurus/grass_pea/6.11>,
        <http://id.acdh.oeaw.ac.at/defc/thesaurus/wild_chickpea/6.20>,
        <http://id.acdh.oeaw.ac.at/defc/thesaurus/wild_pea/6.25> ;
    skos:prefLabel "Erbse"@de,
        "pea"@en,
        "Pisum sativum"@la .

<http://id.acdh.oeaw.ac.at/defc/thesaurus/pottery/2.4> a skos:Concept ;
    skos:broader <http://id.acdh.oeaw.ac.at/defc/thesaurus/finds_type/1.02> ;
    skos:editorialNote "dc_finds_type;4" ;
    skos:inScheme <http://id.acdh.oeaw.ac.at/defc/thesaurus/FindsSchema>,
        <http://id.acdh.oeaw.ac.at/defc/thesaurus/FindsType> ;
    skos:narrower <http://id.acdh.oeaw.ac.at/defc/thesaurus/pottery_decoration/3.018>,
        <http://id.acdh.oeaw.ac.at/defc/thesaurus/pottery_detail/3.017>,
        <http://id.acdh.oeaw.ac.at/defc/thesaurus/pottery_form/3.016>,
        <http://id.acdh.oeaw.ac.at/defc/thesaurus/pottery_surface_treatment/3.019> ;
    skos:prefLabel "Keramik"@de,
        "pottery"@en .

<http://id.acdh.oeaw.ac.at/defc/thesaurus/raw_material/3.066> a skos:Concept ;
    dc:source "OREA" ;
    skos:broader <http://id.acdh.oeaw.ac.at/defc/thesaurus/quarry/2.3> ;
    skos:definition "Raw material that has been exploited at a quarry site." ;
    skos:editorialNote "dc_not_in_database;066" ;
    skos:inScheme <http://id.acdh.oeaw.ac.at/defc/thesaurus/AreaSchema>,
        <http://id.acdh.oeaw.ac.at/defc/thesaurus/NotInDatabase> ;
    skos:narrower <http://id.acdh.oeaw.ac.at/defc/thesaurus/clay/4.6>,
        <http://id.acdh.oeaw.ac.at/defc/thesaurus/metal/4.7>,
        <http://id.acdh.oeaw.ac.at/defc/thesaurus/ochre/4.8>,
        <http://id.acdh.oeaw.ac.at/defc/thesaurus/stone/4.072> ;
    skos:prefLabel "raw material"@en .

<http://id.acdh.oeaw.ac.at/defc/thesaurus/ritual/4.079> a skos:Concept ;
    dc:source "OREA" ;
    skos:broader <http://id.acdh.oeaw.ac.at/defc/thesaurus/special_feature/3.070> ;
    skos:definition "An archaeological feature found in the open space that has a ritual meaning or was used to carry out a ritual." ;
    skos:editorialNote "dc_not_in_database;079" ;
    skos:inScheme <http://id.acdh.oeaw.ac.at/defc/thesaurus/AreaSchema>,
        <http://id.acdh.oeaw.ac.at/defc/thesaurus/NotInDatabase> ;
    skos:narrower <http://id.acdh.oeaw.ac.at/defc/thesaurus/altar/5.33>,
        <http://id.acdh.oeaw.ac.at/defc/thesaurus/bothros/5.21>,
        <http://id.acdh.oeaw.ac.at/defc/thesaurus/stele/5.31>,
        <http://id.acdh.oeaw.ac.at/defc/thesaurus/stone_setting/5.6> ;
    skos:prefLabel "ritual"@en .

<http://id.acdh.oeaw.ac.at/defc/thesaurus/settlement/2.4> a skos:Concept ;
    dc:source "http://thesaurus.historicengland.org.uk/thesaurus_term.asp?thes_no=1&term_no=68977" ;
    skos:broader <http://id.acdh.oeaw.ac.at/defc/thesaurus/area_type/1.064> ;
    skos:definition "A small concentration of dwellings." ;
    skos:editorialNote "dc_area_type;4" ;
    skos:inScheme <http://id.acdh.oeaw.ac.at/defc/thesaurus/AreaSchema>,
        <http://id.acdh.oeaw.ac.at/defc/thesaurus/AreaType> ;
    skos:narrower <http://id.acdh.oeaw.ac.at/defc/thesaurus/building/3.069>,
        <http://id.acdh.oeaw.ac.at/defc/thesaurus/settlement_structure/3.067>,
        <http://id.acdh.oeaw.ac.at/defc/thesaurus/settlment_type/3.068>,
        <http://id.acdh.oeaw.ac.at/defc/thesaurus/special_feature/3.070> ;
    skos:prefLabel "Siedlung"@de,
        "settlement"@en .

<http://id.acdh.oeaw.ac.at/defc/thesaurus/settlement_enclosure/4.073> a skos:Concept ;
    dc:source "OREA" ;
    skos:broader <http://id.acdh.oeaw.ac.at/defc/thesaurus/settlement_structure/3.067> ;
    skos:definition "A structure enclosing a settlement." ;
    skos:editorialNote "dc_not_in_database;073" ;
    skos:inScheme <http://id.acdh.oeaw.ac.at/defc/thesaurus/AreaSchema>,
        <http://id.acdh.oeaw.ac.at/defc/thesaurus/NotInDatabase> ;
    skos:narrower <http://id.acdh.oeaw.ac.at/defc/thesaurus/enclosure_ditch/5.1>,
        <http://id.acdh.oeaw.ac.at/defc/thesaurus/enclosure_rampart/5.2>,
        <http://id.acdh.oeaw.ac.at/defc/thesaurus/enclosure_undetermined/5.7>,
        <http://id.acdh.oeaw.ac.at/defc/thesaurus/enclosure_wall/5.3> ;
    skos:prefLabel "settlement enclosure"@en .

<http://id.acdh.oeaw.ac.at/defc/thesaurus/sex/5.095> a skos:Concept ;
    skos:broader <http://id.acdh.oeaw.ac.at/defc/thesaurus/human_remains/4.085> ;
    skos:editorialNote "dc_not_in_database;095" ;
    skos:inScheme <http://id.acdh.oeaw.ac.at/defc/thesaurus/AreaSchema>,
        <http://id.acdh.oeaw.ac.at/defc/thesaurus/NotInDatabase> ;
    skos:narrower <http://id.acdh.oeaw.ac.at/defc/thesaurus/female_individuals/6.2>,
        <http://id.acdh.oeaw.ac.at/defc/thesaurus/male_individuals/6.1>,
        <http://id.acdh.oeaw.ac.at/defc/thesaurus/part_of_specialist_report/6.4>,
        <http://id.acdh.oeaw.ac.at/defc/thesaurus/sex_not_specified/6.3> ;
    skos:prefLabel "Geschlecht"@de,
        "sex"@en .

<http://id.acdh.oeaw.ac.at/defc/thesaurus/small_finds/2.5> a skos:Concept ;
    dc:source "OREA" ;
    skos:broader <http://id.acdh.oeaw.ac.at/defc/thesaurus/finds_type/1.02> ;
    skos:definition "Artifacts that can be picked up and transported, as opposed to features excluding pottery, stone tools and organic finds." ;
    skos:editorialNote "dc_finds_type;5" ;
    skos:inScheme <http://id.acdh.oeaw.ac.at/defc/thesaurus/FindsSchema>,
        <http://id.acdh.oeaw.ac.at/defc/thesaurus/FindsType> ;
    skos:narrower <http://id.acdh.oeaw.ac.at/defc/thesaurus/figurine/3.3>,
        <http://id.acdh.oeaw.ac.at/defc/thesaurus/jewellery/3.2>,
        <http://id.acdh.oeaw.ac.at/defc/thesaurus/other/3.4>,
        <http://id.acdh.oeaw.ac.at/defc/thesaurus/tool/3.1> ;
    skos:prefLabel "Kleinfund"@de,
        "small finds"@en .

<http://id.acdh.oeaw.ac.at/defc/thesaurus/soil_analysis/2.063> a skos:Concept ;
    skos:broader <http://id.acdh.oeaw.ac.at/defc/thesaurus/special_analysis/1.057> ;
    skos:editorialNote "dc_not_in_database/2.063" ;
    skos:inScheme <http://id.acdh.oeaw.ac.at/defc/thesaurus/NotInDatabase>,
        <http://id.acdh.oeaw.ac.at/defc/thesaurus/ResearchEventSchema> ;
    skos:narrower <http://id.acdh.oeaw.ac.at/defc/thesaurus/soil_analysis%3A_particle_size_analysis%2F3.23>,
        <http://id.acdh.oeaw.ac.at/defc/thesaurus/soil_analysis%3A_soil_chemistry%2F3.24>,
        <http://id.acdh.oeaw.ac.at/defc/thesaurus/soil_analysis%3A_soil_micromorphology%2F3.25>,
        <http://id.acdh.oeaw.ac.at/defc/thesaurus/soil_analysis%3A_soil_phosphorus_analysis%2F3.26> ;
    skos:prefLabel "Bodenanalyse"@de,
        "soil analysis"@en .

<http://id.acdh.oeaw.ac.at/defc/thesaurus/storage/4.080> a skos:Concept ;
    dc:source "OREA" ;
    skos:broader <http://id.acdh.oeaw.ac.at/defc/thesaurus/special_feature/3.070> ;
    skos:definition "An archaeological feature found in the open space that was used for storage." ;
    skos:editorialNote "dc_not_in_database;080" ;
    skos:inScheme <http://id.acdh.oeaw.ac.at/defc/thesaurus/AreaSchema>,
        <http://id.acdh.oeaw.ac.at/defc/thesaurus/NotInDatabase> ;
    skos:narrower <http://id.acdh.oeaw.ac.at/defc/thesaurus/storage_building/5.7>,
        <http://id.acdh.oeaw.ac.at/defc/thesaurus/storage_pit/5.8>,
        <http://id.acdh.oeaw.ac.at/defc/thesaurus/storage_vessel/5.9>,
        <http://id.acdh.oeaw.ac.at/defc/thesaurus/tank/5.12> ;
    skos:prefLabel "storage"@en .

<http://id.acdh.oeaw.ac.at/defc/thesaurus/textile_equipment/4.028> a skos:Concept ;
    dc:source "OREA" ;
    skos:broader <http://id.acdh.oeaw.ac.at/defc/thesaurus/tool/3.1> ;
    skos:definition "Equipment used in production of textile materials." ;
    skos:editorialNote "dc_not_in_database;028" ;
    skos:inScheme <http://id.acdh.oeaw.ac.at/defc/thesaurus/FindsSchema>,
        <http://id.acdh.oeaw.ac.at/defc/thesaurus/NotInDatabase> ;
    skos:narrower <http://id.acdh.oeaw.ac.at/defc/thesaurus/loom_weight/5.71>,
        <http://id.acdh.oeaw.ac.at/defc/thesaurus/needle/5.50>,
        <http://id.acdh.oeaw.ac.at/defc/thesaurus/shuttle/5.75>,
        <http://id.acdh.oeaw.ac.at/defc/thesaurus/spindle_whorl/5.56> ;
    skos:prefLabel "textile equipment"@en .

<http://id.acdh.oeaw.ac.at/defc/thesaurus/wheat/5.39> a skos:Concept ;
    dc:source "http://eol.org/pages/1115240/overview" ;
    skos:broader <http://id.acdh.oeaw.ac.at/defc/thesaurus/cereal/4.022> ;
    skos:editorialNote "dc_botany_species;39" ;
    skos:inScheme <http://id.acdh.oeaw.ac.at/defc/thesaurus/BotanySpecies>,
        <http://id.acdh.oeaw.ac.at/defc/thesaurus/FindsSchema> ;
    skos:narrower <http://id.acdh.oeaw.ac.at/defc/thesaurus/einkorn_wheat/6.6>,
        <http://id.acdh.oeaw.ac.at/defc/thesaurus/emmer_wheat/6.7>,
        <http://id.acdh.oeaw.ac.at/defc/thesaurus/wild_einkorn/6.21>,
        <http://id.acdh.oeaw.ac.at/defc/thesaurus/wild_emmer/6.22> ;
    skos:prefLabel "Weizen"@de,
        "wheat"@en,
        "Tritcum aestivum"@la .

<http://id.acdh.oeaw.ac.at/defc/thesaurus/AreaConstructiontype> a skos:ConceptScheme ;
    rdfs:comment "A concept schema related to the particular Area properties." .

<http://id.acdh.oeaw.ac.at/defc/thesaurus/InterpretationSubsistencetype> a skos:ConceptScheme ;
    rdfs:comment "A concept schema related to the particular Interpretation properties." .

<http://id.acdh.oeaw.ac.at/defc/thesaurus/animal_remains_part/3.07> a skos:Concept ;
    skos:broader <http://id.acdh.oeaw.ac.at/defc/thesaurus/animal_remains/2.1> ;
    skos:inScheme <http://id.acdh.oeaw.ac.at/defc/thesaurus/FindsSchema> ;
    skos:narrower <http://id.acdh.oeaw.ac.at/defc/thesaurus/bone/4.021>,
        <http://id.acdh.oeaw.ac.at/defc/thesaurus/claw/4.10>,
        <http://id.acdh.oeaw.ac.at/defc/thesaurus/horn/4.7>,
        <http://id.acdh.oeaw.ac.at/defc/thesaurus/tooth/4.11>,
        <http://id.acdh.oeaw.ac.at/defc/thesaurus/unknown/4.9> ;
    skos:prefLabel "animal remains part"@en .

<http://id.acdh.oeaw.ac.at/defc/thesaurus/animal_remains_species/3.06> a skos:Concept ;
    skos:broader <http://id.acdh.oeaw.ac.at/defc/thesaurus/animal_remains/2.1> ;
    skos:inScheme <http://id.acdh.oeaw.ac.at/defc/thesaurus/FindsSchema> ;
    skos:narrower <http://id.acdh.oeaw.ac.at/defc/thesaurus/bird/4.36>,
        <http://id.acdh.oeaw.ac.at/defc/thesaurus/fish/4.16>,
        <http://id.acdh.oeaw.ac.at/defc/thesaurus/mammal/4.020>,
        <http://id.acdh.oeaw.ac.at/defc/thesaurus/molluscs/4.17>,
        <http://id.acdh.oeaw.ac.at/defc/thesaurus/reptile/4.35> ;
    skos:prefLabel "animal remains species"@en .

<http://id.acdh.oeaw.ac.at/defc/thesaurus/bird/4.36> a skos:Concept ;
    dc:source "http://eol.org/pages/695/overview" ;
    skos:broader <http://id.acdh.oeaw.ac.at/defc/thesaurus/animal_remains_species/3.06> ;
    skos:editorialNote "dc_finds_animal_remains_species;36" ;
    skos:inScheme <http://id.acdh.oeaw.ac.at/defc/thesaurus/FindsAnimalRemainsSpecies>,
        <http://id.acdh.oeaw.ac.at/defc/thesaurus/FindsSchema> ;
    skos:narrower <http://id.acdh.oeaw.ac.at/defc/thesaurus/chicken/5.40>,
        <http://id.acdh.oeaw.ac.at/defc/thesaurus/duck/5.038>,
        <http://id.acdh.oeaw.ac.at/defc/thesaurus/goose/5.037>,
        <http://id.acdh.oeaw.ac.at/defc/thesaurus/great_bustard/5.30>,
        <http://id.acdh.oeaw.ac.at/defc/thesaurus/partirdge/5.34> ;
    skos:prefLabel "Vogel"@de,
        "bird"@en,
        "Aves"@la .

<http://id.acdh.oeaw.ac.at/defc/thesaurus/bone/4.021> a skos:Concept ;
    skos:broader <http://id.acdh.oeaw.ac.at/defc/thesaurus/animal_remains_part/3.07> ;
    skos:inScheme <http://id.acdh.oeaw.ac.at/defc/thesaurus/FindsSchema> ;
    skos:narrower <http://id.acdh.oeaw.ac.at/defc/thesaurus/antler/5.8>,
        <http://id.acdh.oeaw.ac.at/defc/thesaurus/body/5.5>,
        <http://id.acdh.oeaw.ac.at/defc/thesaurus/extremity/5.4>,
        <http://id.acdh.oeaw.ac.at/defc/thesaurus/jaw/5.6>,
        <http://id.acdh.oeaw.ac.at/defc/thesaurus/skull/5.1> ;
    skos:prefLabel "bone"@en .

<http://id.acdh.oeaw.ac.at/defc/thesaurus/building_shape/4.076> a skos:Concept ;
    dc:source "OREA" ;
    skos:broader <http://id.acdh.oeaw.ac.at/defc/thesaurus/building/3.069> ;
    skos:definition "Ground plan shape of a building (apsidal, circular, ovoid, rectangular…)" ;
    skos:editorialNote "dc_not_in_database;076" ;
    skos:inScheme <http://id.acdh.oeaw.ac.at/defc/thesaurus/AreaSchema>,
        <http://id.acdh.oeaw.ac.at/defc/thesaurus/NotInDatabase> ;
    skos:narrower <http://id.acdh.oeaw.ac.at/defc/thesaurus/apsidal/5.1>,
        <http://id.acdh.oeaw.ac.at/defc/thesaurus/circular/5.2>,
        <http://id.acdh.oeaw.ac.at/defc/thesaurus/ovoid/5.3>,
        <http://id.acdh.oeaw.ac.at/defc/thesaurus/rectangular-apsidal/5.5>,
        <http://id.acdh.oeaw.ac.at/defc/thesaurus/rectangular/5.4> ;
    skos:prefLabel "Grundriss"@de,
        "building shape"@en .

<http://id.acdh.oeaw.ac.at/defc/thesaurus/core/3.012> a skos:Concept ;
    skos:broader <http://id.acdh.oeaw.ac.at/defc/thesaurus/lithics/2.3> ;
    skos:editorialNote "dc_not_in_database;012" ;
    skos:inScheme <http://id.acdh.oeaw.ac.at/defc/thesaurus/FindsSchema>,
        <http://id.acdh.oeaw.ac.at/defc/thesaurus/NotInDatabase> ;
    skos:narrower <http://id.acdh.oeaw.ac.at/defc/thesaurus/bidirectional_core/4.1>,
        <http://id.acdh.oeaw.ac.at/defc/thesaurus/blade_core/4.2>,
        <http://id.acdh.oeaw.ac.at/defc/thesaurus/bullet_core/4.3>,
        <http://id.acdh.oeaw.ac.at/defc/thesaurus/conical_core/4.4>,
        <http://id.acdh.oeaw.ac.at/defc/thesaurus/core_fragment/4.5> ;
    skos:prefLabel "Kerne"@de,
        "core"@en .

<http://id.acdh.oeaw.ac.at/defc/thesaurus/field_survey/3.052> a skos:Concept ;
    skos:altLabel "Prospektion"@de,
        " prospection"@en,
        "survey"@en ;
    skos:broader <http://id.acdh.oeaw.ac.at/defc/thesaurus/non-intrusive/2.051> ;
    skos:editorialNote "dc_not_in_database;052" ;
    skos:inScheme <http://id.acdh.oeaw.ac.at/defc/thesaurus/NotInDatabase>,
        <http://id.acdh.oeaw.ac.at/defc/thesaurus/ResearchEventSchema> ;
    skos:narrower <http://id.acdh.oeaw.ac.at/defc/thesaurus/architectural_survey/4.14>,
        <http://id.acdh.oeaw.ac.at/defc/thesaurus/field_walking_survey/4.053>,
        <http://id.acdh.oeaw.ac.at/defc/thesaurus/geophysical_survey/4.054>,
        <http://id.acdh.oeaw.ac.at/defc/thesaurus/laser_scanning_survey/4.19>,
        <http://id.acdh.oeaw.ac.at/defc/thesaurus/underwater_survey/4.23> ;
    skos:prefLabel "Geländeprospektion"@de,
        "field survey"@en .

<http://id.acdh.oeaw.ac.at/defc/thesaurus/finds_material/1.01> a skos:Concept ;
    dc:source "OREA" ;
    skos:definition "A material from which an archaeological artefact (small finds, lithics) were made of." ;
    skos:editorialNote "dc_not_in_database;01" ;
    skos:inScheme <http://id.acdh.oeaw.ac.at/defc/thesaurus/FindsSchema>,
        <http://id.acdh.oeaw.ac.at/defc/thesaurus/NotInDatabase> ;
    skos:narrower <http://id.acdh.oeaw.ac.at/defc/thesaurus/clay/2.19>,
        <http://id.acdh.oeaw.ac.at/defc/thesaurus/fabric/2.3>,
        <http://id.acdh.oeaw.ac.at/defc/thesaurus/metal/2.9>,
        <http://id.acdh.oeaw.ac.at/defc/thesaurus/mineral/2.3>,
        <http://id.acdh.oeaw.ac.at/defc/thesaurus/organic/2.4>,
        <http://id.acdh.oeaw.ac.at/defc/thesaurus/stone/2.1> ;
    skos:prefLabel "Fundmaterial"@de,
        "finds material"@en .

<http://id.acdh.oeaw.ac.at/defc/thesaurus/foot/4.71> a skos:Concept ;
    dc:source "OREA" ;
    skos:altLabel "Fuß"@de,
        "Leg"@en ;
    skos:broader <http://id.acdh.oeaw.ac.at/defc/thesaurus/pottery_detail/3.017> ;
    skos:definition "Supporting lower part of the vessel such as a tripod, normally attached to the base or vessel bottom after the vessel has got its form." ;
    skos:editorialNote "dc_finds_pottery_detail;71" ;
    skos:inScheme <http://id.acdh.oeaw.ac.at/defc/thesaurus/FindsPotteryDetail>,
        <http://id.acdh.oeaw.ac.at/defc/thesaurus/FindsSchema> ;
    skos:narrower <http://id.acdh.oeaw.ac.at/defc/thesaurus/fenestrated_pedestal/5.160>,
        <http://id.acdh.oeaw.ac.at/defc/thesaurus/pedestal/5.137>,
        <http://id.acdh.oeaw.ac.at/defc/thesaurus/pedestal/5.164>,
        <http://id.acdh.oeaw.ac.at/defc/thesaurus/pedestal_base/5.76>,
        <http://id.acdh.oeaw.ac.at/defc/thesaurus/small_foot/5.167> ;
    skos:prefLabel "Bein"@de,
        "foot"@en .

<http://id.acdh.oeaw.ac.at/defc/thesaurus/grain_crop/3.08> a skos:Concept ;
    skos:broader <http://id.acdh.oeaw.ac.at/defc/thesaurus/botany/2.2> ;
    skos:editorialNote "dc_not_in_database;08" ;
    skos:inScheme <http://id.acdh.oeaw.ac.at/defc/thesaurus/FindsSchema>,
        <http://id.acdh.oeaw.ac.at/defc/thesaurus/NotInDatabase> ;
    skos:narrower <http://id.acdh.oeaw.ac.at/defc/thesaurus/cereal/4.022>,
        <http://id.acdh.oeaw.ac.at/defc/thesaurus/flax/4.9>,
        <http://id.acdh.oeaw.ac.at/defc/thesaurus/poppy/4.16>,
        <http://id.acdh.oeaw.ac.at/defc/thesaurus/pulse/4.32>,
        <http://id.acdh.oeaw.ac.at/defc/thesaurus/wild_flax/4.23> ;
    skos:prefLabel "Getreidesorte"@de,
        "grain crop"@en .

<http://id.acdh.oeaw.ac.at/defc/thesaurus/grave/3.071> a skos:Concept ;
    skos:broader <http://id.acdh.oeaw.ac.at/defc/thesaurus/cemetery_or_grave/2.2> ;
    skos:editorialNote "dc_not_in_database;071" ;
    skos:inScheme <http://id.acdh.oeaw.ac.at/defc/thesaurus/AreaSchema>,
        <http://id.acdh.oeaw.ac.at/defc/thesaurus/NotInDatabase> ;
    skos:narrower <http://id.acdh.oeaw.ac.at/defc/thesaurus/grave_disturbance/4.084>,
        <http://id.acdh.oeaw.ac.at/defc/thesaurus/grave_location/4.087>,
        <http://id.acdh.oeaw.ac.at/defc/thesaurus/grave_type/4.083>,
        <http://id.acdh.oeaw.ac.at/defc/thesaurus/human_remains/4.085>,
        <http://id.acdh.oeaw.ac.at/defc/thesaurus/morturary_feature/4.086> ;
    skos:prefLabel "Grab"@de,
        "grave"@en .

<http://id.acdh.oeaw.ac.at/defc/thesaurus/grave_location/4.087> a skos:Concept ;
    skos:broader <http://id.acdh.oeaw.ac.at/defc/thesaurus/grave/3.071> ;
    skos:editorialNote "dc_not_in_database;087" ;
    skos:inScheme <http://id.acdh.oeaw.ac.at/defc/thesaurus/AreaSchema>,
        <http://id.acdh.oeaw.ac.at/defc/thesaurus/NotInDatabase> ;
    skos:narrower <http://id.acdh.oeaw.ac.at/defc/thesaurus/extramural/5.2>,
        <http://id.acdh.oeaw.ac.at/defc/thesaurus/in_cave/5.3>,
        <http://id.acdh.oeaw.ac.at/defc/thesaurus/intramural/5.1>,
        <http://id.acdh.oeaw.ac.at/defc/thesaurus/next_to_cave/5.4>,
        <http://id.acdh.oeaw.ac.at/defc/thesaurus/part_of_house/5.5> ;
    skos:prefLabel "grave location"@en .

<http://id.acdh.oeaw.ac.at/defc/thesaurus/human_remains/4.085> a skos:Concept ;
    skos:broader <http://id.acdh.oeaw.ac.at/defc/thesaurus/grave/3.071> ;
    skos:editorialNote "dc_not_in_database;085" ;
    skos:inScheme <http://id.acdh.oeaw.ac.at/defc/thesaurus/AreaSchema>,
        <http://id.acdh.oeaw.ac.at/defc/thesaurus/NotInDatabase> ;
    skos:narrower <http://id.acdh.oeaw.ac.at/defc/thesaurus/age_group/5.097>,
        <http://id.acdh.oeaw.ac.at/defc/thesaurus/human_remains_absence/5.1>,
        <http://id.acdh.oeaw.ac.at/defc/thesaurus/human_remains_presence/5.2>,
        <http://id.acdh.oeaw.ac.at/defc/thesaurus/human_remains_type/5.096>,
        <http://id.acdh.oeaw.ac.at/defc/thesaurus/sex/5.095> ;
    skos:prefLabel "menschliche Überreste"@de,
        "human remains"@en .

<http://id.acdh.oeaw.ac.at/defc/thesaurus/jar/4.145> a skos:Concept ;
    dc:source "OREA" ;
    skos:broader <http://id.acdh.oeaw.ac.at/defc/thesaurus/pottery_form/3.016> ;
    skos:definition "An open vessel whose height can be equal or greater than their maximum diameter. They can occur in various sizes with various with or without necks." ;
    skos:editorialNote "dc_finds_pottery_form;145" ;
    skos:inScheme <http://id.acdh.oeaw.ac.at/defc/thesaurus/FindsPotteryForm>,
        <http://id.acdh.oeaw.ac.at/defc/thesaurus/FindsSchema> ;
    skos:narrower <http://id.acdh.oeaw.ac.at/defc/thesaurus/carinated_jar/5.175>,
        <http://id.acdh.oeaw.ac.at/defc/thesaurus/collared_jar/5.127>,
        <http://id.acdh.oeaw.ac.at/defc/thesaurus/funnel-necked_jar/5.180>,
        <http://id.acdh.oeaw.ac.at/defc/thesaurus/globular_jar/5.106>,
        <http://id.acdh.oeaw.ac.at/defc/thesaurus/hole-mouthed_jar/5.131> ;
    skos:prefLabel "Topf"@de,
        "jar"@en .

<http://id.acdh.oeaw.ac.at/defc/thesaurus/mineral/2.3> a skos:Concept ;
    dc:source "OREA" ;
    skos:broader <http://id.acdh.oeaw.ac.at/defc/thesaurus/finds_material/1.01> ;
    skos:definition "Different kinds of minerals used to produce small finds and lithics." ;
    skos:editorialNote "dc_not_in_database;3" ;
    skos:inScheme <http://id.acdh.oeaw.ac.at/defc/thesaurus/FindsSchema>,
        <http://id.acdh.oeaw.ac.at/defc/thesaurus/NotInDatabase> ;
    skos:narrower <http://id.acdh.oeaw.ac.at/defc/thesaurus/calcite/3.37>,
        <http://id.acdh.oeaw.ac.at/defc/thesaurus/chlorite/3.21>,
        <http://id.acdh.oeaw.ac.at/defc/thesaurus/malachite/3.35>,
        <http://id.acdh.oeaw.ac.at/defc/thesaurus/rock_crystal/3.16>,
        <http://id.acdh.oeaw.ac.at/defc/thesaurus/serpentine/3.23> ;
    skos:prefLabel "Mineral"@de,
        "mineral"@en .

<http://id.acdh.oeaw.ac.at/defc/thesaurus/non-intrusive/2.051> a skos:Concept ;
    skos:broader <http://id.acdh.oeaw.ac.at/defc/thesaurus/research_type/1.047> ;
    skos:editorialNote "dc_not_in_database/2.051" ;
    skos:inScheme <http://id.acdh.oeaw.ac.at/defc/thesaurus/NotInDatabase>,
        <http://id.acdh.oeaw.ac.at/defc/thesaurus/ResearchEventSchema> ;
    skos:narrower <http://id.acdh.oeaw.ac.at/defc/thesaurus/field_survey/3.052>,
        <http://id.acdh.oeaw.ac.at/defc/thesaurus/geological_research/3.26>,
        <http://id.acdh.oeaw.ac.at/defc/thesaurus/heritage_assessment/3.055>,
        <http://id.acdh.oeaw.ac.at/defc/thesaurus/petrological_research/3.25>,
        <http://id.acdh.oeaw.ac.at/defc/thesaurus/remote_sensing/3.056> ;
    skos:prefLabel "Nicht-intrusiv"@de,
        "non-intrusive"@en .

<http://id.acdh.oeaw.ac.at/defc/thesaurus/pulse/4.32> a skos:Concept ;
    skos:altLabel "Legume"@en ;
    skos:broader <http://id.acdh.oeaw.ac.at/defc/thesaurus/grain_crop/3.08> ;
    skos:editorialNote "dc_botany_species;32" ;
    skos:inScheme <http://id.acdh.oeaw.ac.at/defc/thesaurus/BotanySpecies>,
        <http://id.acdh.oeaw.ac.at/defc/thesaurus/FindsSchema> ;
    skos:narrower <http://id.acdh.oeaw.ac.at/defc/thesaurus/fava_bean/5.8>,
        <http://id.acdh.oeaw.ac.at/defc/thesaurus/lentil/5.13>,
        <http://id.acdh.oeaw.ac.at/defc/thesaurus/pea/5.14>,
        <http://id.acdh.oeaw.ac.at/defc/thesaurus/vetch/5.33>,
        <http://id.acdh.oeaw.ac.at/defc/thesaurus/wild_lentil/5.24> ;
    skos:prefLabel "Hülsenfrucht"@de,
        "pulse"@en .

<http://id.acdh.oeaw.ac.at/defc/thesaurus/special_feature/3.070> a skos:Concept ;
    dc:source "OREA" ;
    skos:broader <http://id.acdh.oeaw.ac.at/defc/thesaurus/settlement/2.4> ;
    skos:definition "Special archaeological features (architecture and installation) that has been found outside of a building." ;
    skos:editorialNote "dc_not_in_database;070" ;
    skos:inScheme <http://id.acdh.oeaw.ac.at/defc/thesaurus/AreaSchema>,
        <http://id.acdh.oeaw.ac.at/defc/thesaurus/NotInDatabase> ;
    skos:narrower <http://id.acdh.oeaw.ac.at/defc/thesaurus/architecture/4.081>,
        <http://id.acdh.oeaw.ac.at/defc/thesaurus/installation/4.078>,
        <http://id.acdh.oeaw.ac.at/defc/thesaurus/place/4.082>,
        <http://id.acdh.oeaw.ac.at/defc/thesaurus/ritual/4.079>,
        <http://id.acdh.oeaw.ac.at/defc/thesaurus/storage/4.080> ;
    skos:prefLabel "spezielle Befunde"@de,
        "special feature"@en .

<http://id.acdh.oeaw.ac.at/defc/thesaurus/stable_isotope_analysis/2.061> a skos:Concept ;
    skos:broader <http://id.acdh.oeaw.ac.at/defc/thesaurus/special_analysis/1.057> ;
    skos:editorialNote "dc_not_in_database/2.061" ;
    skos:inScheme <http://id.acdh.oeaw.ac.at/defc/thesaurus/NotInDatabase>,
        <http://id.acdh.oeaw.ac.at/defc/thesaurus/ResearchEventSchema> ;
    skos:narrower <isotopes:_carbon_(C)/3.15>,
        <isotopes:_lead_(Pb)/3.16>,
        <isotopes:_nitrogen_(N)/3.17>,
        <isotopes:_oxygen_(O)/3.18>,
        <isotopes:_strontium_(Sr)/3.19> ;
    skos:prefLabel "Isotopanalyse"@de,
        "stable isotope analysis"@en .

<http://id.acdh.oeaw.ac.at/defc/thesaurus/subsistence/1.043> a skos:Concept ;
    skos:editorialNote "dc_not_in_database;043" ;
    skos:inScheme <http://id.acdh.oeaw.ac.at/defc/thesaurus/InterpretationSchema>,
        <http://id.acdh.oeaw.ac.at/defc/thesaurus/NotInDatabase> ;
    skos:narrower <http://id.acdh.oeaw.ac.at/defc/thesaurus/animal_husbandry/2.3>,
        <http://id.acdh.oeaw.ac.at/defc/thesaurus/farming/2.2>,
        <http://id.acdh.oeaw.ac.at/defc/thesaurus/fishing/2.1>,
        <http://id.acdh.oeaw.ac.at/defc/thesaurus/gathering/2.5>,
        <http://id.acdh.oeaw.ac.at/defc/thesaurus/hunting/2.4>,
        <http://id.acdh.oeaw.ac.at/defc/thesaurus/storage_systems/2.6> ;
    skos:prefLabel "subsistence"@en .

<http://id.acdh.oeaw.ac.at/defc/thesaurus/unretouched_tool/3.011> a skos:Concept ;
    skos:broader <http://id.acdh.oeaw.ac.at/defc/thesaurus/lithics/2.3> ;
    skos:editorialNote "dc_not_in_database;011" ;
    skos:inScheme <http://id.acdh.oeaw.ac.at/defc/thesaurus/FindsSchema>,
        <http://id.acdh.oeaw.ac.at/defc/thesaurus/NotInDatabase> ;
    skos:narrower <http://id.acdh.oeaw.ac.at/defc/thesaurus/blade/4.1>,
        <http://id.acdh.oeaw.ac.at/defc/thesaurus/bladelet/4.2>,
        <http://id.acdh.oeaw.ac.at/defc/thesaurus/flake/4.3>,
        <http://id.acdh.oeaw.ac.at/defc/thesaurus/microblade/4.4>,
        <http://id.acdh.oeaw.ac.at/defc/thesaurus/y_blade/4.5> ;
    skos:prefLabel "unretouched tool"@en .

<http://id.acdh.oeaw.ac.at/defc/thesaurus/weapon/4.030> a skos:Concept ;
    skos:broader <http://id.acdh.oeaw.ac.at/defc/thesaurus/tool/3.1> ;
    skos:editorialNote "dc_not_in_database;030" ;
    skos:inScheme <http://id.acdh.oeaw.ac.at/defc/thesaurus/FindsSchema>,
        <http://id.acdh.oeaw.ac.at/defc/thesaurus/NotInDatabase> ;
    skos:narrower <http://id.acdh.oeaw.ac.at/defc/thesaurus/dagger/5.72>,
        <http://id.acdh.oeaw.ac.at/defc/thesaurus/mace_head/5.44>,
        <http://id.acdh.oeaw.ac.at/defc/thesaurus/projectile_point/5.70>,
        <http://id.acdh.oeaw.ac.at/defc/thesaurus/slingstone/5.53>,
        <http://id.acdh.oeaw.ac.at/defc/thesaurus/spear/5.113> ;
    skos:prefLabel "Waffe"@de,
        "weapon"@en .

<http://id.acdh.oeaw.ac.at/defc/thesaurus/AreaEvidenceofocupation> a skos:ConceptScheme ;
    rdfs:comment "A concept schema related to the particular Area properties." .

<http://id.acdh.oeaw.ac.at/defc/thesaurus/AreaSettlementstructure> a skos:ConceptScheme ;
    rdfs:comment "A concept schema related to the particular Area properties." .

<http://id.acdh.oeaw.ac.at/defc/thesaurus/building_type/4.077> a skos:Concept ;
    dc:source "OREA" ;
    skos:broader <http://id.acdh.oeaw.ac.at/defc/thesaurus/building/3.069> ;
    skos:definition "A type of a building based on a certain building technique, space arangement, architectural, functional and cultural distinction." ;
    skos:editorialNote "dc_not_in_database;077" ;
    skos:inScheme <http://id.acdh.oeaw.ac.at/defc/thesaurus/AreaSchema>,
        <http://id.acdh.oeaw.ac.at/defc/thesaurus/NotInDatabase> ;
    skos:narrower <http://id.acdh.oeaw.ac.at/defc/thesaurus/longhouse/5.1>,
        <http://id.acdh.oeaw.ac.at/defc/thesaurus/megaron/5.2>,
        <http://id.acdh.oeaw.ac.at/defc/thesaurus/one-room/5.3>,
        <http://id.acdh.oeaw.ac.at/defc/thesaurus/pile_dwelling/5.4>,
        <http://id.acdh.oeaw.ac.at/defc/thesaurus/pit-house/5.5>,
        <http://id.acdh.oeaw.ac.at/defc/thesaurus/tsangli_house/5.6> ;
    skos:prefLabel "Bautyp"@de,
        "building type"@en .

<http://id.acdh.oeaw.ac.at/defc/thesaurus/cereal/4.022> a skos:Concept ;
    skos:broader <http://id.acdh.oeaw.ac.at/defc/thesaurus/grain_crop/3.08> ;
    skos:editorialNote "dc_not_in_database;022" ;
    skos:inScheme <http://id.acdh.oeaw.ac.at/defc/thesaurus/FindsSchema>,
        <http://id.acdh.oeaw.ac.at/defc/thesaurus/NotInDatabase> ;
    skos:narrower <http://id.acdh.oeaw.ac.at/defc/thesaurus/barley/5.2>,
        <http://id.acdh.oeaw.ac.at/defc/thesaurus/millet/5.039>,
        <http://id.acdh.oeaw.ac.at/defc/thesaurus/oat/5.37>,
        <http://id.acdh.oeaw.ac.at/defc/thesaurus/rye/5.17>,
        <http://id.acdh.oeaw.ac.at/defc/thesaurus/wheat/5.39>,
        <http://id.acdh.oeaw.ac.at/defc/thesaurus/wild_barley/5.18> ;
    skos:prefLabel "Getreide"@de,
        "cereal"@en .

<http://id.acdh.oeaw.ac.at/defc/thesaurus/intrusive/2.048> a skos:Concept ;
    skos:broader <http://id.acdh.oeaw.ac.at/defc/thesaurus/research_type/1.047> ;
    skos:editorialNote "dc_not_in_database/2.048" ;
    skos:inScheme <http://id.acdh.oeaw.ac.at/defc/thesaurus/NotInDatabase>,
        <http://id.acdh.oeaw.ac.at/defc/thesaurus/ResearchEventSchema> ;
    skos:narrower <http://id.acdh.oeaw.ac.at/defc/thesaurus/borehole_survey/3.1>,
        <http://id.acdh.oeaw.ac.at/defc/thesaurus/evaluation/3.050>,
        <http://id.acdh.oeaw.ac.at/defc/thesaurus/excavation/3.049>,
        <http://id.acdh.oeaw.ac.at/defc/thesaurus/field_observation_(monitoring)/3.6>,
        <http://id.acdh.oeaw.ac.at/defc/thesaurus/metal_detecting_use/3.7>,
        <http://id.acdh.oeaw.ac.at/defc/thesaurus/profile_clearing/3.24> ;
    skos:prefLabel "Intrusiv"@de,
        "intrusive"@en .

<http://id.acdh.oeaw.ac.at/defc/thesaurus/organic/2.4> a skos:Concept ;
    dc:source "OREA" ;
    skos:altLabel "organisch"@de ;
    skos:broader <http://id.acdh.oeaw.ac.at/defc/thesaurus/finds_material/1.01> ;
    skos:definition "Organic material that was used to create objects." ;
    skos:editorialNote "dc_not_in_database;4" ;
    skos:inScheme <http://id.acdh.oeaw.ac.at/defc/thesaurus/FindsSchema>,
        <http://id.acdh.oeaw.ac.at/defc/thesaurus/NotInDatabase> ;
    skos:narrower <http://id.acdh.oeaw.ac.at/defc/thesaurus/antler/3.7>,
        <http://id.acdh.oeaw.ac.at/defc/thesaurus/bone/3.5>,
        <http://id.acdh.oeaw.ac.at/defc/thesaurus/horn/3.8>,
        <http://id.acdh.oeaw.ac.at/defc/thesaurus/shell/3.6>,
        <http://id.acdh.oeaw.ac.at/defc/thesaurus/tooth/3.28>,
        <http://id.acdh.oeaw.ac.at/defc/thesaurus/wood/3.32> ;
    skos:prefLabel "Organisches Material"@de,
        "organic"@en .

<http://id.acdh.oeaw.ac.at/defc/thesaurus/plastic_decoration/4.132> a skos:Concept ;
    dc:source "OREA" ;
    skos:broader <http://id.acdh.oeaw.ac.at/defc/thesaurus/pottery_decoration/3.018> ;
    skos:definition "Pottery with applied material on its surface such as clay or bead." ;
    skos:editorialNote "dc_finds_pottery_decoration;132" ;
    skos:inScheme <http://id.acdh.oeaw.ac.at/defc/thesaurus/FindsPotteryDecoration>,
        <http://id.acdh.oeaw.ac.at/defc/thesaurus/FindsSchema> ;
    skos:narrower <http://id.acdh.oeaw.ac.at/defc/thesaurus/applied_disc/5.211>,
        <http://id.acdh.oeaw.ac.at/defc/thesaurus/barbotine/5.240>,
        <http://id.acdh.oeaw.ac.at/defc/thesaurus/bead_inlay/5.118>,
        <http://id.acdh.oeaw.ac.at/defc/thesaurus/granulata_ware/5.216>,
        <http://id.acdh.oeaw.ac.at/defc/thesaurus/plastic_cordon_decoration/5.225>,
        <http://id.acdh.oeaw.ac.at/defc/thesaurus/pointillé_decoration/5.227> ;
    skos:prefLabel "Plastischer Dekor"@de,
        "plastic decoration"@en .

<http://id.acdh.oeaw.ac.at/defc/thesaurus/pottery_detail/3.017> a skos:Concept ;
    skos:broader <http://id.acdh.oeaw.ac.at/defc/thesaurus/pottery/2.4> ;
    skos:editorialNote "dc_not_in_database;017" ;
    skos:inScheme <http://id.acdh.oeaw.ac.at/defc/thesaurus/FindsSchema>,
        <http://id.acdh.oeaw.ac.at/defc/thesaurus/NotInDatabase> ;
    skos:narrower <http://id.acdh.oeaw.ac.at/defc/thesaurus/attachment/4.034>,
        <http://id.acdh.oeaw.ac.at/defc/thesaurus/base/4.032>,
        <http://id.acdh.oeaw.ac.at/defc/thesaurus/foot/4.71>,
        <http://id.acdh.oeaw.ac.at/defc/thesaurus/handle/4.031>,
        <http://id.acdh.oeaw.ac.at/defc/thesaurus/rim/4.033>,
        <http://id.acdh.oeaw.ac.at/defc/thesaurus/spout/4.88> ;
    skos:prefLabel "Keramikdetail"@de,
        "pottery detail"@en .

<http://id.acdh.oeaw.ac.at/defc/thesaurus/stone/4.025> a skos:Concept ;
    dc:source "OREA" ;
    skos:broader <http://id.acdh.oeaw.ac.at/defc/thesaurus/lithic_material/3.015> ;
    skos:definition "Different kinds of stone used to produce lithics." ;
    skos:editorialNote "dc_not_in_database;025" ;
    skos:inScheme <http://id.acdh.oeaw.ac.at/defc/thesaurus/FindsSchema>,
        <http://id.acdh.oeaw.ac.at/defc/thesaurus/NotInDatabase> ;
    skos:narrower <http://id.acdh.oeaw.ac.at/defc/thesaurus/chalcedony/5.4>,
        <http://id.acdh.oeaw.ac.at/defc/thesaurus/chert/5.3>,
        <http://id.acdh.oeaw.ac.at/defc/thesaurus/jasper/5.5>,
        <http://id.acdh.oeaw.ac.at/defc/thesaurus/obsidian/5.1>,
        <http://id.acdh.oeaw.ac.at/defc/thesaurus/quartz/5.6>,
        <http://id.acdh.oeaw.ac.at/defc/thesaurus/quartzite/5.8> ;
    skos:prefLabel "Stein"@de,
        "stone"@en,
        "rock"@la .

<http://id.acdh.oeaw.ac.at/defc/thesaurus/AreaGravetype> a skos:ConceptScheme ;
    rdfs:comment "A concept schema related to the particular Area properties." .

<http://id.acdh.oeaw.ac.at/defc/thesaurus/botany/2.2> a skos:Concept ;
    dc:source "OREA" ;
    skos:altLabel "plant remains"@en ;
    skos:broader <http://id.acdh.oeaw.ac.at/defc/thesaurus/finds_type/1.02> ;
    skos:definition "Remains of plants cultivated or used by man in ancient times and plants of ancient environment, which have survived in archaeological contexts." ;
    skos:editorialNote "dc_finds_type;2" ;
    skos:inScheme <http://id.acdh.oeaw.ac.at/defc/thesaurus/FindsSchema>,
        <http://id.acdh.oeaw.ac.at/defc/thesaurus/FindsType> ;
    skos:narrower <http://id.acdh.oeaw.ac.at/defc/thesaurus/black_nightshade/3.38>,
        <http://id.acdh.oeaw.ac.at/defc/thesaurus/buckthorn/3.43>,
        <http://id.acdh.oeaw.ac.at/defc/thesaurus/fruit/3.09>,
        <http://id.acdh.oeaw.ac.at/defc/thesaurus/grain_crop/3.08>,
        <http://id.acdh.oeaw.ac.at/defc/thesaurus/hemp/3.12>,
        <http://id.acdh.oeaw.ac.at/defc/thesaurus/pine/3.44>,
        <http://id.acdh.oeaw.ac.at/defc/thesaurus/sea_club-rush/3.34> ;
    skos:prefLabel "Botanische Rückstände"@de,
        "botany"@en .

<http://id.acdh.oeaw.ac.at/defc/thesaurus/building_material/5.089> a skos:Concept ;
    dc:source "OREA" ;
    skos:broader <http://id.acdh.oeaw.ac.at/defc/thesaurus/building_technique/4.075> ;
    skos:definition "A certain type of building technique distinctive on the material that has been used." ;
    skos:editorialNote "dc_not_in_database;089" ;
    skos:inScheme <http://id.acdh.oeaw.ac.at/defc/thesaurus/AreaSchema>,
        <http://id.acdh.oeaw.ac.at/defc/thesaurus/NotInDatabase> ;
    skos:narrower <http://id.acdh.oeaw.ac.at/defc/thesaurus/concrete/6.16>,
        <http://id.acdh.oeaw.ac.at/defc/thesaurus/mud_brick/6.1>,
        <http://id.acdh.oeaw.ac.at/defc/thesaurus/pisé/6.3>,
        <http://id.acdh.oeaw.ac.at/defc/thesaurus/stone/6.11>,
        <http://id.acdh.oeaw.ac.at/defc/thesaurus/straw/6.8>,
        <http://id.acdh.oeaw.ac.at/defc/thesaurus/timber/6.10>,
        <http://id.acdh.oeaw.ac.at/defc/thesaurus/wattle_and_daub/6.6> ;
    skos:prefLabel "building material"@en .

<http://id.acdh.oeaw.ac.at/defc/thesaurus/dating/2.060> a skos:Concept ;
    skos:broader <http://id.acdh.oeaw.ac.at/defc/thesaurus/special_analysis/1.057> ;
    skos:editorialNote "dc_not_in_database/2.060" ;
    skos:inScheme <http://id.acdh.oeaw.ac.at/defc/thesaurus/NotInDatabase>,
        <http://id.acdh.oeaw.ac.at/defc/thesaurus/ResearchEventSchema> ;
    skos:narrower <dating:_archaeomagnetism/3.6>,
        <dating:_dendrochronology/3.7>,
        <dating:_lead_isotope_dating/3.8>,
        <dating:_luminescence_dating/3.9>,
        <dating:_mitochondrial_dna/3.10>,
        <dating:_oxygen_isotope_analysis/3.11>,
        <dating:_radiocarbon_dating/3.12> ;
    skos:prefLabel "Datierung"@de,
        "dating"@en .

<http://id.acdh.oeaw.ac.at/defc/thesaurus/lithics/2.3> a skos:Concept ;
    skos:altLabel "Steingerät"@de,
        "Stone tool"@en ;
    skos:broader <http://id.acdh.oeaw.ac.at/defc/thesaurus/finds_type/1.02> ;
    skos:editorialNote "dc_finds_type;3" ;
    skos:inScheme <http://id.acdh.oeaw.ac.at/defc/thesaurus/FindsSchema>,
        <http://id.acdh.oeaw.ac.at/defc/thesaurus/FindsType> ;
    skos:narrower <http://id.acdh.oeaw.ac.at/defc/thesaurus/core/3.012>,
        <http://id.acdh.oeaw.ac.at/defc/thesaurus/core/3.12>,
        <http://id.acdh.oeaw.ac.at/defc/thesaurus/core_preparation/3.013>,
        <http://id.acdh.oeaw.ac.at/defc/thesaurus/lithic_material/3.015>,
        <http://id.acdh.oeaw.ac.at/defc/thesaurus/lithic_production/3.014>,
        <http://id.acdh.oeaw.ac.at/defc/thesaurus/retouched_tool/3.010>,
        <http://id.acdh.oeaw.ac.at/defc/thesaurus/unretouched_tool/3.011> ;
    skos:prefLabel "Steinwerkzeug"@de,
        "lithics"@en .

<http://id.acdh.oeaw.ac.at/defc/thesaurus/occupation_evidence/4.088> a skos:Concept ;
    skos:broader <http://id.acdh.oeaw.ac.at/defc/thesaurus/cave/3.1> ;
    skos:editorialNote "dc_not_in_database;088" ;
    skos:inScheme <http://id.acdh.oeaw.ac.at/defc/thesaurus/AreaSchema>,
        <http://id.acdh.oeaw.ac.at/defc/thesaurus/NotInDatabase> ;
    skos:narrower <http://id.acdh.oeaw.ac.at/defc/thesaurus/clay_structure/5.6>,
        <http://id.acdh.oeaw.ac.at/defc/thesaurus/fireplace/5.1>,
        <http://id.acdh.oeaw.ac.at/defc/thesaurus/hearth/5.7>,
        <http://id.acdh.oeaw.ac.at/defc/thesaurus/pit/5.5>,
        <http://id.acdh.oeaw.ac.at/defc/thesaurus/post_hole/5.3>,
        <http://id.acdh.oeaw.ac.at/defc/thesaurus/stone_setting/5.4>,
        <http://id.acdh.oeaw.ac.at/defc/thesaurus/storage_facilities/5.2> ;
    skos:prefLabel "Nachweis von menschlichen Tätigkeiten"@de,
        "occupation evidence"@en .

<http://id.acdh.oeaw.ac.at/defc/thesaurus/FindsLithicsRawMaterial> a skos:ConceptScheme ;
    rdfs:comment "A concept schema related to the particular Finds properties." .

<http://id.acdh.oeaw.ac.at/defc/thesaurus/InterpretationProductiontype> a skos:ConceptScheme ;
    rdfs:comment "A concept schema related to the particular Interpretation properties." .

<http://id.acdh.oeaw.ac.at/defc/thesaurus/grave_type/4.083> a skos:Concept ;
    skos:broader <http://id.acdh.oeaw.ac.at/defc/thesaurus/grave/3.071> ;
    skos:editorialNote "dc_not_in_database;083" ;
    skos:inScheme <http://id.acdh.oeaw.ac.at/defc/thesaurus/AreaSchema>,
        <http://id.acdh.oeaw.ac.at/defc/thesaurus/NotInDatabase> ;
    skos:narrower <http://id.acdh.oeaw.ac.at/defc/thesaurus/cairn/5.8>,
        <http://id.acdh.oeaw.ac.at/defc/thesaurus/chamber_grave/5.7>,
        <http://id.acdh.oeaw.ac.at/defc/thesaurus/cist_grave/5.1>,
        <http://id.acdh.oeaw.ac.at/defc/thesaurus/none_recorded/5.4>,
        <http://id.acdh.oeaw.ac.at/defc/thesaurus/pit_grave/5.2>,
        <http://id.acdh.oeaw.ac.at/defc/thesaurus/shaft_grave/5.5>,
        <http://id.acdh.oeaw.ac.at/defc/thesaurus/tumulus/5.6>,
        <http://id.acdh.oeaw.ac.at/defc/thesaurus/vessel/5.3> ;
    skos:prefLabel "Grabtyp"@de,
        "grave type"@en .

<http://id.acdh.oeaw.ac.at/defc/thesaurus/production/1.042> a skos:Concept ;
    skos:editorialNote "dc_not_in_database;042" ;
    skos:inScheme <http://id.acdh.oeaw.ac.at/defc/thesaurus/InterpretationSchema>,
        <http://id.acdh.oeaw.ac.at/defc/thesaurus/NotInDatabase> ;
    skos:narrower <http://id.acdh.oeaw.ac.at/defc/thesaurus/bone_tool_production/2.6>,
        <http://id.acdh.oeaw.ac.at/defc/thesaurus/chipped_stone_tool_production/2.3>,
        <http://id.acdh.oeaw.ac.at/defc/thesaurus/jewellery_production/2.9>,
        <http://id.acdh.oeaw.ac.at/defc/thesaurus/metal_production/2.2>,
        <http://id.acdh.oeaw.ac.at/defc/thesaurus/pottery_production/2.7>,
        <http://id.acdh.oeaw.ac.at/defc/thesaurus/pottery_tool_production/2.8>,
        <http://id.acdh.oeaw.ac.at/defc/thesaurus/shell_production/2.5>,
        <http://id.acdh.oeaw.ac.at/defc/thesaurus/stone_tool_production/2.4>,
        <http://id.acdh.oeaw.ac.at/defc/thesaurus/textile_production/2.1> ;
    skos:prefLabel "production"@en .

<http://id.acdh.oeaw.ac.at/defc/thesaurus/strap_handle/5.78> a skos:Concept ;
    dc:source "Kipfer, B. A. Dictionary of Artifacts 2007. Blackwell Publishing, Oxford.p 305" ;
    skos:broader <http://id.acdh.oeaw.ac.at/defc/thesaurus/handle/4.031> ;
    skos:definition "A handle made from a strip of clay and attached to the body of the pot at two points before firing." ;
    skos:editorialNote "dc_finds_pottery_detail;78" ;
    skos:inScheme <http://id.acdh.oeaw.ac.at/defc/thesaurus/FindsPotteryDetail>,
        <http://id.acdh.oeaw.ac.at/defc/thesaurus/FindsSchema> ;
    skos:narrower <http://id.acdh.oeaw.ac.at/defc/thesaurus/high_strap_handle/6.119>,
        <http://id.acdh.oeaw.ac.at/defc/thesaurus/high_strap_handle_with_knob/6.90>,
        <http://id.acdh.oeaw.ac.at/defc/thesaurus/horned_strap_handle/6.92>,
        <http://id.acdh.oeaw.ac.at/defc/thesaurus/miniature_strap_handle/6.147>,
        <http://id.acdh.oeaw.ac.at/defc/thesaurus/rim-attached_strap_handle/6.151>,
        <http://id.acdh.oeaw.ac.at/defc/thesaurus/strap_handle_with_knob/6.91>,
        <http://id.acdh.oeaw.ac.at/defc/thesaurus/strap_handle_with_round_hole/6.149>,
        <http://id.acdh.oeaw.ac.at/defc/thesaurus/winged_strap_handle/6.154> ;
    skos:prefLabel "Bandhenkel"@de,
        "strap handle"@en .

<http://id.acdh.oeaw.ac.at/defc/thesaurus/AreaRawmaterial> a skos:ConceptScheme ;
    rdfs:comment "A concept schema related to the particular Area properties." .

<http://id.acdh.oeaw.ac.at/defc/thesaurus/SiteSchema> a skos:ConceptScheme ;
    rdfs:comment "A concept schema related to class Site in database." .

<http://id.acdh.oeaw.ac.at/defc/thesaurus/figurine/3.3> a skos:Concept ;
    dc:source "http://dbpedia.org/page/Figurine" ;
    skos:altLabel "kleine Statue"@de,
        "stattuete"@en,
        "terracotta"@en ;
    skos:broader <http://id.acdh.oeaw.ac.at/defc/thesaurus/small_finds/2.5> ;
    skos:definition "A figurine or statuette is a small statue that represents a human, deity or animal, or in practice a pair or small group of them." ;
    skos:editorialNote "dc_small_finds_category;3" ;
    skos:inScheme <http://id.acdh.oeaw.ac.at/defc/thesaurus/FindsSchema>,
        <http://id.acdh.oeaw.ac.at/defc/thesaurus/SmallFindsCategory> ;
    skos:narrower <http://id.acdh.oeaw.ac.at/defc/thesaurus/anthropomorphic_figurine/4.84>,
        <http://id.acdh.oeaw.ac.at/defc/thesaurus/house_model/4.88>,
        <http://id.acdh.oeaw.ac.at/defc/thesaurus/other/4.99>,
        <http://id.acdh.oeaw.ac.at/defc/thesaurus/ring_idol/4.137>,
        <http://id.acdh.oeaw.ac.at/defc/thesaurus/stone_figurine/4.82>,
        <http://id.acdh.oeaw.ac.at/defc/thesaurus/table/4.61>,
        <http://id.acdh.oeaw.ac.at/defc/thesaurus/thin_plate/4.104>,
        <http://id.acdh.oeaw.ac.at/defc/thesaurus/unknown/4.98>,
        <http://id.acdh.oeaw.ac.at/defc/thesaurus/zoomorphic_figurine/4.83> ;
    skos:prefLabel "Statuette"@de,
        "figurine"@en .

<http://id.acdh.oeaw.ac.at/defc/thesaurus/rim/4.033> a skos:Concept ;
    skos:broader <http://id.acdh.oeaw.ac.at/defc/thesaurus/pottery_detail/3.017> ;
    skos:inScheme <http://id.acdh.oeaw.ac.at/defc/thesaurus/FindsSchema> ;
    skos:narrower <http://id.acdh.oeaw.ac.at/defc/thesaurus/curved_tapered-up_rim/5.140>,
        <http://id.acdh.oeaw.ac.at/defc/thesaurus/everted_rim/5.173>,
        <http://id.acdh.oeaw.ac.at/defc/thesaurus/flaring_rim/5.69>,
        <http://id.acdh.oeaw.ac.at/defc/thesaurus/flat-topped_rim/5.158>,
        <http://id.acdh.oeaw.ac.at/defc/thesaurus/inside_bevelled_and_decorated_rim/5.73>,
        <http://id.acdh.oeaw.ac.at/defc/thesaurus/offset_rim/5.163>,
        <http://id.acdh.oeaw.ac.at/defc/thesaurus/rolled_rim/5.77>,
        <http://id.acdh.oeaw.ac.at/defc/thesaurus/tapered-up_rim/5.157>,
        <http://id.acdh.oeaw.ac.at/defc/thesaurus/thickened_rim/5.166> ;
    skos:prefLabel "rim"@en .

<http://id.acdh.oeaw.ac.at/defc/thesaurus/PeriodSchema> a skos:ConceptScheme ;
    rdfs:comment "A concept schema related to the class Area (and Research Event) in the database." .

<http://id.acdh.oeaw.ac.at/defc/thesaurus/fruit/3.09> a skos:Concept ;
    skos:broader <http://id.acdh.oeaw.ac.at/defc/thesaurus/botany/2.2> ;
    skos:inScheme <http://id.acdh.oeaw.ac.at/defc/thesaurus/FindsSchema> ;
    skos:narrower <http://id.acdh.oeaw.ac.at/defc/thesaurus/apple/4.41>,
        <http://id.acdh.oeaw.ac.at/defc/thesaurus/apricot/4.1>,
        <http://id.acdh.oeaw.ac.at/defc/thesaurus/blackberry/4.36>,
        <http://id.acdh.oeaw.ac.at/defc/thesaurus/fig/4.27>,
        <http://id.acdh.oeaw.ac.at/defc/thesaurus/grape/4.29>,
        <http://id.acdh.oeaw.ac.at/defc/thesaurus/nuts/4.31>,
        <http://id.acdh.oeaw.ac.at/defc/thesaurus/olive/4.26>,
        <http://id.acdh.oeaw.ac.at/defc/thesaurus/peach/4.15>,
        <http://id.acdh.oeaw.ac.at/defc/thesaurus/pear/4.42>,
        <http://id.acdh.oeaw.ac.at/defc/thesaurus/wild_plum/4.45> ;
    skos:prefLabel "fruit"@en .

<http://id.acdh.oeaw.ac.at/defc/thesaurus/other/3.4> a skos:Concept ;
    skos:broader <http://id.acdh.oeaw.ac.at/defc/thesaurus/small_finds/2.5> ;
    skos:definition "A small find that is not a figurine, tool nor jewlry" ;
    skos:editorialNote "dc_small_finds_category;4" ;
    skos:inScheme <http://id.acdh.oeaw.ac.at/defc/thesaurus/FindsSchema>,
        <http://id.acdh.oeaw.ac.at/defc/thesaurus/SmallFindsCategory> ;
    skos:narrower <http://id.acdh.oeaw.ac.at/defc/thesaurus/belt_hook/4.54>,
        <http://id.acdh.oeaw.ac.at/defc/thesaurus/button/4.102>,
        <http://id.acdh.oeaw.ac.at/defc/thesaurus/dross/4.129>,
        <http://id.acdh.oeaw.ac.at/defc/thesaurus/dugout/4.115>,
        <http://id.acdh.oeaw.ac.at/defc/thesaurus/inscription/4.114>,
        <http://id.acdh.oeaw.ac.at/defc/thesaurus/pivot_stone/4.135>,
        <http://id.acdh.oeaw.ac.at/defc/thesaurus/plaque/4.73>,
        <http://id.acdh.oeaw.ac.at/defc/thesaurus/token/4.105>,
        <http://id.acdh.oeaw.ac.at/defc/thesaurus/vessel/4.94>,
        <http://id.acdh.oeaw.ac.at/defc/thesaurus/wire/4.118> ;
    skos:prefLabel "other"@en .

<http://id.acdh.oeaw.ac.at/defc/thesaurus/special_analysis/1.057> a skos:Concept ;
    dc:source "OREA" ;
    skos:definition "A type of special analysis conducted during an archaeological investigation." ;
    skos:editorialNote "dc_not_in_database;057" ;
    skos:inScheme <http://id.acdh.oeaw.ac.at/defc/thesaurus/ResearchEventSchema>,
        "NotInDatabase" ;
    skos:narrower <http://id.acdh.oeaw.ac.at/defc/thesaurus/DNA_analysis/2.13>,
        <http://id.acdh.oeaw.ac.at/defc/thesaurus/animal_remains_report/2.1>,
        <http://id.acdh.oeaw.ac.at/defc/thesaurus/archeobotany/2.058>,
        <http://id.acdh.oeaw.ac.at/defc/thesaurus/ceramic_analysis/2.059>,
        <http://id.acdh.oeaw.ac.at/defc/thesaurus/dating/2.060>,
        <http://id.acdh.oeaw.ac.at/defc/thesaurus/human_remains_report/2.14>,
        <http://id.acdh.oeaw.ac.at/defc/thesaurus/lithics_analysis/2.062>,
        <http://id.acdh.oeaw.ac.at/defc/thesaurus/metallurgy/2.21>,
        <http://id.acdh.oeaw.ac.at/defc/thesaurus/mineralogy/2.22>,
        <http://id.acdh.oeaw.ac.at/defc/thesaurus/soil_analysis/2.063>,
        <http://id.acdh.oeaw.ac.at/defc/thesaurus/stable_isotope_analysis/2.061> ;
    skos:prefLabel "special analysis"@en .

<http://id.acdh.oeaw.ac.at/defc/thesaurus/AnimalRemainsPart> a skos:ConceptScheme ;
    rdfs:comment "A concept schema related to the particular Finds properties." .

<http://id.acdh.oeaw.ac.at/defc/thesaurus/architecture/4.081> a skos:Concept ;
    skos:broader <http://id.acdh.oeaw.ac.at/defc/thesaurus/special_feature/3.070> ;
    skos:editorialNote "dc_not_in_database;081" ;
    skos:inScheme <http://id.acdh.oeaw.ac.at/defc/thesaurus/AreaSchema>,
        <http://id.acdh.oeaw.ac.at/defc/thesaurus/NotInDatabase> ;
    skos:narrower <http://id.acdh.oeaw.ac.at/defc/thesaurus/buttress/5.32>,
        <http://id.acdh.oeaw.ac.at/defc/thesaurus/clay_structure/5.16>,
        <http://id.acdh.oeaw.ac.at/defc/thesaurus/floor/5.094>,
        <http://id.acdh.oeaw.ac.at/defc/thesaurus/niche/5.28>,
        <http://id.acdh.oeaw.ac.at/defc/thesaurus/paved_area/5.13>,
        <http://id.acdh.oeaw.ac.at/defc/thesaurus/stairway/5.17>,
        <http://id.acdh.oeaw.ac.at/defc/thesaurus/stone_row_structure/5.38>,
        <http://id.acdh.oeaw.ac.at/defc/thesaurus/terrace_wall/5.14>,
        <http://id.acdh.oeaw.ac.at/defc/thesaurus/thermal_structure/5.27>,
        <http://id.acdh.oeaw.ac.at/defc/thesaurus/wall/5.18>,
        <http://id.acdh.oeaw.ac.at/defc/thesaurus/wall_painting/5.37> ;
    skos:prefLabel "architecture"@en .

<http://id.acdh.oeaw.ac.at/defc/thesaurus/building_technique/4.075> a skos:Concept ;
    skos:broader <http://id.acdh.oeaw.ac.at/defc/thesaurus/building/3.069> ;
    skos:definition "A building technique in which a building has been build (mud brick, wattle and daub...). Also distinctive architectural elements such as pillars and floor." ;
    skos:editorialNote "dc_not_in_database;075" ;
    skos:inScheme <http://id.acdh.oeaw.ac.at/defc/thesaurus/AreaSchema>,
        <http://id.acdh.oeaw.ac.at/defc/thesaurus/NotInDatabase> ;
    skos:narrower <http://id.acdh.oeaw.ac.at/defc/thesaurus/building_material/5.089>,
        <http://id.acdh.oeaw.ac.at/defc/thesaurus/floor/5.092>,
        <http://id.acdh.oeaw.ac.at/defc/thesaurus/foundation_trench/5.13>,
        <http://id.acdh.oeaw.ac.at/defc/thesaurus/pavement/5.2>,
        <http://id.acdh.oeaw.ac.at/defc/thesaurus/pillar/5.091>,
        <http://id.acdh.oeaw.ac.at/defc/thesaurus/plastered_threshold/5.9>,
        <http://id.acdh.oeaw.ac.at/defc/thesaurus/sacral/5.17>,
        <http://id.acdh.oeaw.ac.at/defc/thesaurus/stone_lining/5.12>,
        <http://id.acdh.oeaw.ac.at/defc/thesaurus/stone_socket/5.5>,
        <http://id.acdh.oeaw.ac.at/defc/thesaurus/timber-frame_construction/5.7>,
        <http://id.acdh.oeaw.ac.at/defc/thesaurus/wall/5.090> ;
    skos:prefLabel "Bautechnik"@de,
        "building technique"@en .

<http://id.acdh.oeaw.ac.at/defc/thesaurus/AreaAgegroups> a skos:ConceptScheme ;
    rdfs:comment "A concept schema related to the particular Area properties." .

<http://id.acdh.oeaw.ac.at/defc/thesaurus/FindsLithicsCoreShape> a skos:ConceptScheme ;
    rdfs:comment "A concept schema related to the particular Finds properties." .

<http://id.acdh.oeaw.ac.at/defc/thesaurus/bowl/4.115> a skos:Concept ;
    dc:source "OREA" ;
    skos:broader <http://id.acdh.oeaw.ac.at/defc/thesaurus/pottery_form/3.016> ;
    skos:definition "A container whose height can measure from 1/3 to equal the amount of ist maximum diameter." ;
    skos:editorialNote "dc_finds_pottery_form;115" ;
    skos:inScheme <http://id.acdh.oeaw.ac.at/defc/thesaurus/FindsPotteryForm>,
        <http://id.acdh.oeaw.ac.at/defc/thesaurus/FindsSchema> ;
    skos:narrower <http://id.acdh.oeaw.ac.at/defc/thesaurus/carinated_bowl/5.104>,
        <http://id.acdh.oeaw.ac.at/defc/thesaurus/collared_bowl/5.146>,
        <http://id.acdh.oeaw.ac.at/defc/thesaurus/deep_bowl/5.178>,
        <http://id.acdh.oeaw.ac.at/defc/thesaurus/dimini_bowl/5.129>,
        <http://id.acdh.oeaw.ac.at/defc/thesaurus/dome-shaped_shallow_bowl/5.108>,
        <http://id.acdh.oeaw.ac.at/defc/thesaurus/flat_based_oval_bowl/5.193>,
        <http://id.acdh.oeaw.ac.at/defc/thesaurus/gouged_bowl/5.149>,
        <http://id.acdh.oeaw.ac.at/defc/thesaurus/husking_bowl/5.190>,
        <http://id.acdh.oeaw.ac.at/defc/thesaurus/husking_bowl/5.196>,
        <http://id.acdh.oeaw.ac.at/defc/thesaurus/narrow-mouthed_shallow_bowl/5.109>,
        <http://id.acdh.oeaw.ac.at/defc/thesaurus/shallow_bowl/5.116>,
        <http://id.acdh.oeaw.ac.at/defc/thesaurus/shouldered_bowl/5.156> ;
    skos:prefLabel "Schüssel"@de,
        "bowl"@en .

<http://id.acdh.oeaw.ac.at/defc/thesaurus/age_group/5.097> a skos:Concept ;
    skos:broader <http://id.acdh.oeaw.ac.at/defc/thesaurus/human_remains/4.085> ;
    skos:definition "Age group of human remains." ;
    skos:editorialNote "dc_not_in_database;097" ;
    skos:inScheme <http://id.acdh.oeaw.ac.at/defc/thesaurus/AreaSchema>,
        <http://id.acdh.oeaw.ac.at/defc/thesaurus/NotInDatabase> ;
    skos:narrower <http://id.acdh.oeaw.ac.at/defc/thesaurus/adult-mature_(19-45)/6.6>,
        <http://id.acdh.oeaw.ac.at/defc/thesaurus/adult/6.15>,
        <http://id.acdh.oeaw.ac.at/defc/thesaurus/adult_(19-40)/6.5>,
        <http://id.acdh.oeaw.ac.at/defc/thesaurus/age_not_specified/6.10>,
        <http://id.acdh.oeaw.ac.at/defc/thesaurus/infans_i_(0-6)/6.2>,
        <http://id.acdh.oeaw.ac.at/defc/thesaurus/infans_ii_(7-12)/6.3>,
        <http://id.acdh.oeaw.ac.at/defc/thesaurus/juvenile_(13-18)/6.4>,
        <http://id.acdh.oeaw.ac.at/defc/thesaurus/mature-senile_(51-70)/6.8>,
        <http://id.acdh.oeaw.ac.at/defc/thesaurus/mature_(41-60)/6.7>,
        <http://id.acdh.oeaw.ac.at/defc/thesaurus/neonate/6.1>,
        <http://id.acdh.oeaw.ac.at/defc/thesaurus/part_of_specialist_report/6.11>,
        <http://id.acdh.oeaw.ac.at/defc/thesaurus/senile_(60-)/6.9>,
        <http://id.acdh.oeaw.ac.at/defc/thesaurus/subadult/6.14> ;
    skos:prefLabel "Altersgruppe"@de,
        "age group"@en .

<http://id.acdh.oeaw.ac.at/defc/thesaurus/monochrome/5.265> a skos:Concept ;
    dc:source "OREA" ;
    skos:broader <http://id.acdh.oeaw.ac.at/defc/thesaurus/painted/4.239> ;
    skos:definition "Pottery painted with one or maximally two colors." ;
    skos:editorialNote "dc_finds_pottery_decoration;265" ;
    skos:inScheme <http://id.acdh.oeaw.ac.at/defc/thesaurus/FindsPotteryDecoration>,
        <http://id.acdh.oeaw.ac.at/defc/thesaurus/FindsSchema> ;
    skos:narrower <http://id.acdh.oeaw.ac.at/defc/thesaurus/monochrome_black/6.245>,
        <http://id.acdh.oeaw.ac.at/defc/thesaurus/monochrome_brown/6.130>,
        <http://id.acdh.oeaw.ac.at/defc/thesaurus/monochrome_grey/6.294>,
        <http://id.acdh.oeaw.ac.at/defc/thesaurus/monochrome_orange/6.200>,
        <http://id.acdh.oeaw.ac.at/defc/thesaurus/monochrome_red/6.249>,
        <http://id.acdh.oeaw.ac.at/defc/thesaurus/monochrome_red_(a1)/6.154>,
        <http://id.acdh.oeaw.ac.at/defc/thesaurus/monochrome_undecorated_(b1)/6.155>,
        <http://id.acdh.oeaw.ac.at/defc/thesaurus/monochrome_urfirnis/6.171>,
        <http://id.acdh.oeaw.ac.at/defc/thesaurus/monochrome_white/6.301>,
        <http://id.acdh.oeaw.ac.at/defc/thesaurus/monochrome_yellow/6.286>,
        <http://id.acdh.oeaw.ac.at/defc/thesaurus/orange_fine_ware/6.259>,
        <http://id.acdh.oeaw.ac.at/defc/thesaurus/pink_ware/6.273>,
        <http://id.acdh.oeaw.ac.at/defc/thesaurus/white/6.275> ;
    skos:prefLabel "Monochrom"@de,
        "monochrome"@en .

<http://id.acdh.oeaw.ac.at/defc/thesaurus/handle/4.031> a skos:Concept ;
    skos:broader <http://id.acdh.oeaw.ac.at/defc/thesaurus/pottery_detail/3.017> ;
    skos:editorialNote "dc_not_in_database;031" ;
    skos:inScheme <http://id.acdh.oeaw.ac.at/defc/thesaurus/FindsSchema>,
        <http://id.acdh.oeaw.ac.at/defc/thesaurus/NotInDatabase> ;
    skos:narrower <http://id.acdh.oeaw.ac.at/defc/thesaurus/crescent-shaped_handle/5.171>,
        <http://id.acdh.oeaw.ac.at/defc/thesaurus/ear_handle/5.118>,
        <http://id.acdh.oeaw.ac.at/defc/thesaurus/elongated_handle/5.170>,
        <http://id.acdh.oeaw.ac.at/defc/thesaurus/handle_with_knob/5.182>,
        <http://id.acdh.oeaw.ac.at/defc/thesaurus/horned_handle/5.72>,
        <http://id.acdh.oeaw.ac.at/defc/thesaurus/knobbed_handle/5.120>,
        <http://id.acdh.oeaw.ac.at/defc/thesaurus/lug/5.040>,
        <http://id.acdh.oeaw.ac.at/defc/thesaurus/mushroom_handle/5.75>,
        <http://id.acdh.oeaw.ac.at/defc/thesaurus/pronged_handle/5.130>,
        <http://id.acdh.oeaw.ac.at/defc/thesaurus/ring_handle/5.100>,
        <http://id.acdh.oeaw.ac.at/defc/thesaurus/round_bar_handle/5.109>,
        <http://id.acdh.oeaw.ac.at/defc/thesaurus/strap_handle/5.78>,
        <http://id.acdh.oeaw.ac.at/defc/thesaurus/tab_handle/5.169>,
        <http://id.acdh.oeaw.ac.at/defc/thesaurus/tab_handle/5.96>,
        <http://id.acdh.oeaw.ac.at/defc/thesaurus/wishbone_handle/5.93> ;
    skos:prefLabel "Henkel"@de,
        "handle"@en .

<http://id.acdh.oeaw.ac.at/defc/thesaurus/installation/4.078> a skos:Concept ;
    dc:source "OREA" ;
    skos:broader <http://id.acdh.oeaw.ac.at/defc/thesaurus/special_feature/3.070> ;
    skos:definition "An installed mostly communal facilities such as pits, kilns etc. that were found in space between residential buildings." ;
    skos:editorialNote "dc_not_in_database;078" ;
    skos:inScheme <http://id.acdh.oeaw.ac.at/defc/thesaurus/AreaSchema>,
        <http://id.acdh.oeaw.ac.at/defc/thesaurus/NotInDatabase> ;
    skos:narrower <http://id.acdh.oeaw.ac.at/defc/thesaurus/basin/5.29>,
        <http://id.acdh.oeaw.ac.at/defc/thesaurus/bench/5.1>,
        <http://id.acdh.oeaw.ac.at/defc/thesaurus/channel/5.2>,
        <http://id.acdh.oeaw.ac.at/defc/thesaurus/fireplace/5.15>,
        <http://id.acdh.oeaw.ac.at/defc/thesaurus/hearth/5.3>,
        <http://id.acdh.oeaw.ac.at/defc/thesaurus/hole/5.24>,
        <http://id.acdh.oeaw.ac.at/defc/thesaurus/kiln/5.36>,
        <http://id.acdh.oeaw.ac.at/defc/thesaurus/manger/5.35>,
        <http://id.acdh.oeaw.ac.at/defc/thesaurus/oven/5.11>,
        <http://id.acdh.oeaw.ac.at/defc/thesaurus/pit/5.4>,
        <http://id.acdh.oeaw.ac.at/defc/thesaurus/platform/5.093>,
        <http://id.acdh.oeaw.ac.at/defc/thesaurus/post_base/5.34>,
        <http://id.acdh.oeaw.ac.at/defc/thesaurus/post_hole/5.5>,
        <http://id.acdh.oeaw.ac.at/defc/thesaurus/waste_pit/5.20>,
        <http://id.acdh.oeaw.ac.at/defc/thesaurus/well/5.10> ;
    skos:prefLabel "installation"@en .

<http://id.acdh.oeaw.ac.at/defc/thesaurus/jewellery/3.2> a skos:Concept ;
    dc:source "http://dbpedia.org/page/Jewellery" ;
    skos:altLabel "jewelry"@en ;
    skos:broader <http://id.acdh.oeaw.ac.at/defc/thesaurus/small_finds/2.5> ;
    skos:definition "Jewellery or jewelry consists of small decorative items worn for personal adornment, such as brooches, rings, necklaces, earrings, and bracelets. Jewellery may be attached to the body or the clothes, and the term is restricted to durable ornaments, exclud" ;
    skos:editorialNote "dc_small_finds_category;2" ;
    skos:inScheme <http://id.acdh.oeaw.ac.at/defc/thesaurus/FindsSchema>,
        <http://id.acdh.oeaw.ac.at/defc/thesaurus/SmallFindsCategory> ;
    skos:narrower <http://id.acdh.oeaw.ac.at/defc/thesaurus/appliqué/4.126>,
        <http://id.acdh.oeaw.ac.at/defc/thesaurus/bead/4.78>,
        <http://id.acdh.oeaw.ac.at/defc/thesaurus/bracelet/4.77>,
        <http://id.acdh.oeaw.ac.at/defc/thesaurus/ear_plug/4.79>,
        <http://id.acdh.oeaw.ac.at/defc/thesaurus/earring/4.81>,
        <http://id.acdh.oeaw.ac.at/defc/thesaurus/inlay/4.125>,
        <http://id.acdh.oeaw.ac.at/defc/thesaurus/labret/4.106>,
        <http://id.acdh.oeaw.ac.at/defc/thesaurus/necklace/4.80>,
        <http://id.acdh.oeaw.ac.at/defc/thesaurus/nose_ring/4.127>,
        <http://id.acdh.oeaw.ac.at/defc/thesaurus/ornament/4.124>,
        <http://id.acdh.oeaw.ac.at/defc/thesaurus/other/4.108>,
        <http://id.acdh.oeaw.ac.at/defc/thesaurus/pendant/4.76>,
        <http://id.acdh.oeaw.ac.at/defc/thesaurus/pin/4.128>,
        <http://id.acdh.oeaw.ac.at/defc/thesaurus/ring/4.103>,
        <http://id.acdh.oeaw.ac.at/defc/thesaurus/unknown/4.110> ;
    skos:prefLabel "Schmuck"@de,
        "jewellery"@en .

<http://id.acdh.oeaw.ac.at/defc/thesaurus/stone/2.1> a skos:Concept ;
    dc:source "OREA" ;
    skos:altLabel "rock"@en ;
    skos:broader <http://id.acdh.oeaw.ac.at/defc/thesaurus/finds_material/1.01> ;
    skos:definition "Different kinds of stone used to produce small finds and lithics." ;
    skos:editorialNote "dc_finds_material;1" ;
    skos:inScheme <http://id.acdh.oeaw.ac.at/defc/thesaurus/FindsMaterial>,
        <http://id.acdh.oeaw.ac.at/defc/thesaurus/FindsSchema> ;
    skos:narrower <http://id.acdh.oeaw.ac.at/defc/thesaurus/agate/3.27>,
        <http://id.acdh.oeaw.ac.at/defc/thesaurus/andesit/3.29>,
        <http://id.acdh.oeaw.ac.at/defc/thesaurus/basalt/3.20>,
        <http://id.acdh.oeaw.ac.at/defc/thesaurus/chalcedony/3.13>,
        <http://id.acdh.oeaw.ac.at/defc/thesaurus/chert/3.12>,
        <http://id.acdh.oeaw.ac.at/defc/thesaurus/granite/3.24>,
        <http://id.acdh.oeaw.ac.at/defc/thesaurus/green_stone/3.33>,
        <http://id.acdh.oeaw.ac.at/defc/thesaurus/jasper/3.14>,
        <http://id.acdh.oeaw.ac.at/defc/thesaurus/limestone/3.22>,
        <http://id.acdh.oeaw.ac.at/defc/thesaurus/marble/3.10>,
        <http://id.acdh.oeaw.ac.at/defc/thesaurus/obsidian/3.2>,
        <http://id.acdh.oeaw.ac.at/defc/thesaurus/porphyry/3.30>,
        <http://id.acdh.oeaw.ac.at/defc/thesaurus/quartz/3.15>,
        <http://id.acdh.oeaw.ac.at/defc/thesaurus/quarzite/3.17>,
        <http://id.acdh.oeaw.ac.at/defc/thesaurus/sandstone/3.25>,
        <http://id.acdh.oeaw.ac.at/defc/thesaurus/schist/3.26> ;
    skos:prefLabel "Stein"@de,
        "stone"@en .

<http://id.acdh.oeaw.ac.at/defc/thesaurus/InterpretationSchema> a skos:ConceptScheme ;
    rdfs:comment "A concept schema related to the class Interpretation in the database" .

<http://id.acdh.oeaw.ac.at/defc/thesaurus/burnished/4.297> a skos:Concept ;
    dc:source "OREA" ;
    skos:broader <http://id.acdh.oeaw.ac.at/defc/thesaurus/pottery_surface_treatment/3.019> ;
    skos:definition "Surface treatment of rubbing and smooting the surface of a vessel when it is leather-hard (before firing) with a hard tool made out of wood, stone or bone in order to obtain a bright, even, compact, and non-porous surface." ;
    skos:editorialNote "dc_finds_pottery_decoration;297" ;
    skos:inScheme <http://id.acdh.oeaw.ac.at/defc/thesaurus/FindsPotteryDecoration>,
        <http://id.acdh.oeaw.ac.at/defc/thesaurus/FindsSchema> ;
    skos:narrower <http://id.acdh.oeaw.ac.at/defc/thesaurus/black/red_burnished_arapi/5.307>,
        <http://id.acdh.oeaw.ac.at/defc/thesaurus/black_burnished/5.271>,
        <http://id.acdh.oeaw.ac.at/defc/thesaurus/black_burnished_with_channeled_decoration_(γ1α3)/5.142>,
        <http://id.acdh.oeaw.ac.at/defc/thesaurus/black_burnished_with_white_paint_(γ1α1)/5.143>,
        <http://id.acdh.oeaw.ac.at/defc/thesaurus/black_burnished_“larisa”_(γ1α)/5.141>,
        <http://id.acdh.oeaw.ac.at/defc/thesaurus/black_pattern_burnished_(γ1α2)/5.146>,
        <http://id.acdh.oeaw.ac.at/defc/thesaurus/brown_burnished/5.120>,
        <http://id.acdh.oeaw.ac.at/defc/thesaurus/dark_faced_burished_ware_(dfbw)/5.247>,
        <http://id.acdh.oeaw.ac.at/defc/thesaurus/grey_burnished/5.289>,
        <http://id.acdh.oeaw.ac.at/defc/thesaurus/monochrome_burnished/5.170>,
        <http://id.acdh.oeaw.ac.at/defc/thesaurus/pattern_burnished/5.131>,
        <http://id.acdh.oeaw.ac.at/defc/thesaurus/polychrome_burnished/5.243>,
        <http://id.acdh.oeaw.ac.at/defc/thesaurus/red_burnished/5.248>,
        <http://id.acdh.oeaw.ac.at/defc/thesaurus/red_burnished_(b1)/5.156>,
        <http://id.acdh.oeaw.ac.at/defc/thesaurus/rippled_burnished/5.231>,
        <http://id.acdh.oeaw.ac.at/defc/thesaurus/scribble_burnished/5.234>,
        <http://id.acdh.oeaw.ac.at/defc/thesaurus/stroke-and_pattern_burnished/5.178> ;
    skos:prefLabel "Geglättet"@de,
        "burnished"@en .

<http://id.acdh.oeaw.ac.at/defc/thesaurus/pottery_surface_treatment/3.019> a skos:Concept ;
    skos:broader <http://id.acdh.oeaw.ac.at/defc/thesaurus/pottery/2.4> ;
    skos:editorialNote "dc_not_in_database;019" ;
    skos:inScheme <http://id.acdh.oeaw.ac.at/defc/thesaurus/FindsSchema>,
        <http://id.acdh.oeaw.ac.at/defc/thesaurus/NotInDatabase> ;
    skos:narrower <http://id.acdh.oeaw.ac.at/defc/thesaurus/black_slipped/4.258>,
        <http://id.acdh.oeaw.ac.at/defc/thesaurus/black_topped/4.242>,
        <http://id.acdh.oeaw.ac.at/defc/thesaurus/brushed/4.213>,
        <http://id.acdh.oeaw.ac.at/defc/thesaurus/burnished/4.297>,
        <http://id.acdh.oeaw.ac.at/defc/thesaurus/coarse/4.252>,
        <http://id.acdh.oeaw.ac.at/defc/thesaurus/gray_lustre/4.195>,
        <http://id.acdh.oeaw.ac.at/defc/thesaurus/patterned_urfirnis/4.173>,
        <http://id.acdh.oeaw.ac.at/defc/thesaurus/polished/4.228>,
        <http://id.acdh.oeaw.ac.at/defc/thesaurus/rippled/4.177>,
        <http://id.acdh.oeaw.ac.at/defc/thesaurus/scraped_(a3ε)/4.159>,
        <http://id.acdh.oeaw.ac.at/defc/thesaurus/slipped/4.302>,
        <http://id.acdh.oeaw.ac.at/defc/thesaurus/smeared/4.260>,
        <http://id.acdh.oeaw.ac.at/defc/thesaurus/smoothed/4.261>,
        <http://id.acdh.oeaw.ac.at/defc/thesaurus/spongy/4.244>,
        <http://id.acdh.oeaw.ac.at/defc/thesaurus/topped/4.035>,
        <http://id.acdh.oeaw.ac.at/defc/thesaurus/unburnished/4.135>,
        <http://id.acdh.oeaw.ac.at/defc/thesaurus/wiped/4.237> ;
    skos:prefLabel "Oberflächenbehandlung"@de,
        "pottery surface treatment"@en .

<http://id.acdh.oeaw.ac.at/defc/thesaurus/AreaBuildingtechnique> a skos:ConceptScheme ;
    rdfs:comment "A concept schema related to the particular Area properties." .

<http://id.acdh.oeaw.ac.at/defc/thesaurus/incised/4.168> a skos:Concept ;
    dc:source "OREA" ;
    skos:broader <http://id.acdh.oeaw.ac.at/defc/thesaurus/pottery_decoration/3.018> ;
    skos:definition "Pottery decorated by cuts into the surface." ;
    skos:editorialNote "dc_finds_pottery_decoration;168" ;
    skos:inScheme <http://id.acdh.oeaw.ac.at/defc/thesaurus/FindsPotteryDecoration>,
        <http://id.acdh.oeaw.ac.at/defc/thesaurus/FindsSchema> ;
    skos:narrower <http://id.acdh.oeaw.ac.at/defc/thesaurus/coarse_urfirnis/5.164>,
        <http://id.acdh.oeaw.ac.at/defc/thesaurus/excised-with-graphite/5.192>,
        <http://id.acdh.oeaw.ac.at/defc/thesaurus/excised/5.191>,
        <http://id.acdh.oeaw.ac.at/defc/thesaurus/figure_relief_decoration/5.133>,
        <http://id.acdh.oeaw.ac.at/defc/thesaurus/grooved/5.123>,
        <http://id.acdh.oeaw.ac.at/defc/thesaurus/grooved_with_graphite/5.197>,
        <http://id.acdh.oeaw.ac.at/defc/thesaurus/impresso/5.126>,
        <http://id.acdh.oeaw.ac.at/defc/thesaurus/impresso_(a2)/5.151>,
        <http://id.acdh.oeaw.ac.at/defc/thesaurus/incised-pointillé_decoration/5.127>,
        <http://id.acdh.oeaw.ac.at/defc/thesaurus/incised_(b2)/5.152>,
        <http://id.acdh.oeaw.ac.at/defc/thesaurus/incised_(γ2)/5.153>,
        <http://id.acdh.oeaw.ac.at/defc/thesaurus/incrusted/5.122>,
        <http://id.acdh.oeaw.ac.at/defc/thesaurus/mat-impressed/5.129>,
        <http://id.acdh.oeaw.ac.at/defc/thesaurus/pattern_jabbed/5.223>,
        <http://id.acdh.oeaw.ac.at/defc/thesaurus/punched/5.229>,
        <http://id.acdh.oeaw.ac.at/defc/thesaurus/red_incrusted/5.203>,
        <http://id.acdh.oeaw.ac.at/defc/thesaurus/rusticated/5.208>,
        <http://id.acdh.oeaw.ac.at/defc/thesaurus/scored/5.233>,
        <http://id.acdh.oeaw.ac.at/defc/thesaurus/shell_stamped/5.209>,
        <http://id.acdh.oeaw.ac.at/defc/thesaurus/single_jabbed/5.235> ;
    skos:prefLabel "Ritzverziert"@de,
        "incised"@en .

<http://id.acdh.oeaw.ac.at/defc/thesaurus/FindsLithicsRetouchedTools> a skos:ConceptScheme ;
    rdfs:comment "A concept schema related to the particular Finds properties." .

<http://id.acdh.oeaw.ac.at/defc/thesaurus/retouched_tool/3.010> a skos:Concept ;
    skos:broader <http://id.acdh.oeaw.ac.at/defc/thesaurus/lithics/2.3> ;
    skos:editorialNote "dc_not_in_database;010" ;
    skos:inScheme <http://id.acdh.oeaw.ac.at/defc/thesaurus/FindsSchema>,
        <http://id.acdh.oeaw.ac.at/defc/thesaurus/NotInDatabase> ;
    skos:narrower <http://id.acdh.oeaw.ac.at/defc/thesaurus/backed_bladelet/4.1>,
        <http://id.acdh.oeaw.ac.at/defc/thesaurus/burin/4.2>,
        <http://id.acdh.oeaw.ac.at/defc/thesaurus/cicrular_scraper/4.4>,
        <http://id.acdh.oeaw.ac.at/defc/thesaurus/denticulate/4.5>,
        <http://id.acdh.oeaw.ac.at/defc/thesaurus/double-baked_blade/4.7>,
        <http://id.acdh.oeaw.ac.at/defc/thesaurus/double_truncation/4.6>,
        <http://id.acdh.oeaw.ac.at/defc/thesaurus/drill/4.8>,
        <http://id.acdh.oeaw.ac.at/defc/thesaurus/end-scraper_on_blade/4.9>,
        <http://id.acdh.oeaw.ac.at/defc/thesaurus/end-scraper_on_flake/4.10>,
        <http://id.acdh.oeaw.ac.at/defc/thesaurus/high_scraper/4.11>,
        <http://id.acdh.oeaw.ac.at/defc/thesaurus/knife/4.12>,
        <http://id.acdh.oeaw.ac.at/defc/thesaurus/micro_end-scraper/4.13>,
        <http://id.acdh.oeaw.ac.at/defc/thesaurus/notch/4.14>,
        <http://id.acdh.oeaw.ac.at/defc/thesaurus/projectile_point/4.15>,
        <http://id.acdh.oeaw.ac.at/defc/thesaurus/retouched_blade/4.16>,
        <http://id.acdh.oeaw.ac.at/defc/thesaurus/retouched_flake/4.17>,
        <http://id.acdh.oeaw.ac.at/defc/thesaurus/segment/4.18>,
        <http://id.acdh.oeaw.ac.at/defc/thesaurus/sickle_blade/4.19>,
        <http://id.acdh.oeaw.ac.at/defc/thesaurus/side-scraper/4.20>,
        <http://id.acdh.oeaw.ac.at/defc/thesaurus/splinter/4.21>,
        <http://id.acdh.oeaw.ac.at/defc/thesaurus/trapeze/4.22>,
        <http://id.acdh.oeaw.ac.at/defc/thesaurus/truncation/4.23>,
        <http://id.acdh.oeaw.ac.at/defc/thesaurus/çayönü_tool/4.3> ;
    skos:prefLabel "retouched tool"@en .

<http://id.acdh.oeaw.ac.at/defc/thesaurus/ResearcheventSpecialAnalysis> a skos:ConceptScheme ;
    rdfs:comment "A concept schema related to the particular properties of Research Event in the database.",
        "A concept scheme related to the particular Research Event properties" .

<http://id.acdh.oeaw.ac.at/defc/thesaurus/ResearchevetResearchtype> a skos:ConceptScheme ;
    rdfs:comment "A concept schema related to the particular properties of Research Event in the database.",
        "A concept schema related to the particular properties of Research Event." .

<http://id.acdh.oeaw.ac.at/defc/thesaurus/mammal/4.020> a skos:Concept ;
    skos:broader <http://id.acdh.oeaw.ac.at/defc/thesaurus/animal_remains_species/3.06> ;
    skos:editorialNote "dc_not_in_database;020" ;
    skos:inScheme <http://id.acdh.oeaw.ac.at/defc/thesaurus/FindsSchema>,
        <http://id.acdh.oeaw.ac.at/defc/thesaurus/NotInDatabase> ;
    skos:narrower <http://id.acdh.oeaw.ac.at/defc/thesaurus/aurochs/5.4>,
        <http://id.acdh.oeaw.ac.at/defc/thesaurus/beaver/5.28>,
        <http://id.acdh.oeaw.ac.at/defc/thesaurus/brown_bear/5.22>,
        <http://id.acdh.oeaw.ac.at/defc/thesaurus/cattle/5.3>,
        <http://id.acdh.oeaw.ac.at/defc/thesaurus/chamois/5.40>,
        <http://id.acdh.oeaw.ac.at/defc/thesaurus/deer/5.036>,
        <http://id.acdh.oeaw.ac.at/defc/thesaurus/dog/5.10>,
        <http://id.acdh.oeaw.ac.at/defc/thesaurus/donkey/5.21>,
        <http://id.acdh.oeaw.ac.at/defc/thesaurus/game/5.15>,
        <http://id.acdh.oeaw.ac.at/defc/thesaurus/gazelle/5.37>,
        <http://id.acdh.oeaw.ac.at/defc/thesaurus/goat/5.8>,
        <http://id.acdh.oeaw.ac.at/defc/thesaurus/hare/5.12>,
        <http://id.acdh.oeaw.ac.at/defc/thesaurus/hare/5.27>,
        <http://id.acdh.oeaw.ac.at/defc/thesaurus/horse/5.11>,
        <http://id.acdh.oeaw.ac.at/defc/thesaurus/mouse/5.20>,
        <http://id.acdh.oeaw.ac.at/defc/thesaurus/onager/5.39>,
        <http://id.acdh.oeaw.ac.at/defc/thesaurus/pig/5.2>,
        <http://id.acdh.oeaw.ac.at/defc/thesaurus/red_fox/5.25>,
        <http://id.acdh.oeaw.ac.at/defc/thesaurus/sheep/5.6>,
        <http://id.acdh.oeaw.ac.at/defc/thesaurus/sheep/goat/5.5>,
        <http://id.acdh.oeaw.ac.at/defc/thesaurus/water_vole/5.19>,
        <http://id.acdh.oeaw.ac.at/defc/thesaurus/wild_board/5.1>,
        <http://id.acdh.oeaw.ac.at/defc/thesaurus/wild_cattle/5.38>,
        <http://id.acdh.oeaw.ac.at/defc/thesaurus/wild_goat/5.9>,
        <http://id.acdh.oeaw.ac.at/defc/thesaurus/wild_sheep/5.7>,
        <http://id.acdh.oeaw.ac.at/defc/thesaurus/wildcat/5.24>,
        <http://id.acdh.oeaw.ac.at/defc/thesaurus/wolf/5.26> ;
    skos:prefLabel "mammal"@en .

<http://id.acdh.oeaw.ac.at/defc/thesaurus/pottery_form/3.016> a skos:Concept ;
    skos:broader <http://id.acdh.oeaw.ac.at/defc/thesaurus/pottery/2.4> ;
    skos:inScheme <http://id.acdh.oeaw.ac.at/defc/thesaurus/FindsSchema> ;
    skos:narrower <http://id.acdh.oeaw.ac.at/defc/thesaurus/amphora/4.119>,
        <http://id.acdh.oeaw.ac.at/defc/thesaurus/anthropomorphic_vessel/4.99>,
        <http://id.acdh.oeaw.ac.at/defc/thesaurus/askos/4.101>,
        <http://id.acdh.oeaw.ac.at/defc/thesaurus/baking_pan/4.103>,
        <http://id.acdh.oeaw.ac.at/defc/thesaurus/basin/4.122>,
        <http://id.acdh.oeaw.ac.at/defc/thesaurus/beaker/4.098>,
        <http://id.acdh.oeaw.ac.at/defc/thesaurus/bowl/4.115>,
        <http://id.acdh.oeaw.ac.at/defc/thesaurus/chalice/4.185>,
        <http://id.acdh.oeaw.ac.at/defc/thesaurus/cheese_pot/4.126>,
        <http://id.acdh.oeaw.ac.at/defc/thesaurus/cup/4.107>,
        <http://id.acdh.oeaw.ac.at/defc/thesaurus/fikirtepe_box/4.111>,
        <http://id.acdh.oeaw.ac.at/defc/thesaurus/fruitstand/4.130>,
        <http://id.acdh.oeaw.ac.at/defc/thesaurus/goblet/4.201>,
        <http://id.acdh.oeaw.ac.at/defc/thesaurus/jar/4.145>,
        <http://id.acdh.oeaw.ac.at/defc/thesaurus/jug/4.110>,
        <http://id.acdh.oeaw.ac.at/defc/thesaurus/ladle/4.133>,
        <http://id.acdh.oeaw.ac.at/defc/thesaurus/lamp/4.134>,
        <http://id.acdh.oeaw.ac.at/defc/thesaurus/lid/4.112>,
        <http://id.acdh.oeaw.ac.at/defc/thesaurus/mug/4.113>,
        <http://id.acdh.oeaw.ac.at/defc/thesaurus/ogee-pot/4.195>,
        <http://id.acdh.oeaw.ac.at/defc/thesaurus/piriform_jar/4.152>,
        <http://id.acdh.oeaw.ac.at/defc/thesaurus/pithos/4.135>,
        <http://id.acdh.oeaw.ac.at/defc/thesaurus/plate/4.165>,
        <http://id.acdh.oeaw.ac.at/defc/thesaurus/pyxis/4.166>,
        <http://id.acdh.oeaw.ac.at/defc/thesaurus/rhyton/4.186>,
        <http://id.acdh.oeaw.ac.at/defc/thesaurus/scoop/4.136>,
        <http://id.acdh.oeaw.ac.at/defc/thesaurus/sieve/4.117>,
        <http://id.acdh.oeaw.ac.at/defc/thesaurus/skyphos/4.157>,
        <http://id.acdh.oeaw.ac.at/defc/thesaurus/stand/4.169>,
        <http://id.acdh.oeaw.ac.at/defc/thesaurus/tripod/4.137>,
        <http://id.acdh.oeaw.ac.at/defc/thesaurus/zoomorphic_vessel/4.100> ;
    skos:prefLabel "pottery form"@en .

<http://id.acdh.oeaw.ac.at/defc/thesaurus/pattern_painted/5.041> a skos:Concept ;
    skos:broader <http://id.acdh.oeaw.ac.at/defc/thesaurus/painted/4.239> ;
    skos:editorialNote "dc_not_in_database;041" ;
    skos:inScheme <http://id.acdh.oeaw.ac.at/defc/thesaurus/FindsSchema>,
        <http://id.acdh.oeaw.ac.at/defc/thesaurus/NotInDatabase> ;
    skos:narrower <http://id.acdh.oeaw.ac.at/defc/thesaurus/black_and_red_on_cream_(polychrome)_(β3β)/6.138>,
        <http://id.acdh.oeaw.ac.at/defc/thesaurus/black_and_red_on_white_(polychrome)_(β3γ)/6.139>,
        <http://id.acdh.oeaw.ac.at/defc/thesaurus/black_and_white_on_red_(polychrome)_(β3β)/6.140>,
        <http://id.acdh.oeaw.ac.at/defc/thesaurus/black_on_grey/6.287>,
        <http://id.acdh.oeaw.ac.at/defc/thesaurus/black_on_red/6.163>,
        <http://id.acdh.oeaw.ac.at/defc/thesaurus/black_on_red_(β3α2b)/6.144>,
        <http://id.acdh.oeaw.ac.at/defc/thesaurus/black_on_white/6.279>,
        <http://id.acdh.oeaw.ac.at/defc/thesaurus/black_on_white_(b3α3)/6.145>,
        <http://id.acdh.oeaw.ac.at/defc/thesaurus/brown_on_buff/6.185>,
        <http://id.acdh.oeaw.ac.at/defc/thesaurus/brown_on_buff_(matt_painted)_(b3ε)/6.147>,
        <http://id.acdh.oeaw.ac.at/defc/thesaurus/brown_on_cream/6.262>,
        <http://id.acdh.oeaw.ac.at/defc/thesaurus/brown_on_cream_(b3α2a)/6.148>,
        <http://id.acdh.oeaw.ac.at/defc/thesaurus/brown_on_red/6.186>,
        <http://id.acdh.oeaw.ac.at/defc/thesaurus/brown_on_yellow/6.283>,
        <http://id.acdh.oeaw.ac.at/defc/thesaurus/graphite_painted/6.194>,
        <http://id.acdh.oeaw.ac.at/defc/thesaurus/grey_on_grey/6.277>,
        <http://id.acdh.oeaw.ac.at/defc/thesaurus/grey_on_grey_(γ1β)/6.150>,
        <http://id.acdh.oeaw.ac.at/defc/thesaurus/grey_ware/6.246>,
        <http://id.acdh.oeaw.ac.at/defc/thesaurus/halaf_painted/6.125>,
        <http://id.acdh.oeaw.ac.at/defc/thesaurus/matt_brown_on_white/6.199>,
        <http://id.acdh.oeaw.ac.at/defc/thesaurus/matt_painted/6.169>,
        <http://id.acdh.oeaw.ac.at/defc/thesaurus/polychrome/6.202>,
        <http://id.acdh.oeaw.ac.at/defc/thesaurus/red_on_brown/6.204>,
        <http://id.acdh.oeaw.ac.at/defc/thesaurus/red_on_buff/6.230>,
        <http://id.acdh.oeaw.ac.at/defc/thesaurus/red_on_red/6.268>,
        <http://id.acdh.oeaw.ac.at/defc/thesaurus/red_on_red_(a3γ)/6.158>,
        <http://id.acdh.oeaw.ac.at/defc/thesaurus/red_on_white/6.290>,
        <http://id.acdh.oeaw.ac.at/defc/thesaurus/red_on_white_(a3ß)/6.157>,
        <http://id.acdh.oeaw.ac.at/defc/thesaurus/red_on_yellow/6.282>,
        <http://id.acdh.oeaw.ac.at/defc/thesaurus/white_on_black/6.181>,
        <http://id.acdh.oeaw.ac.at/defc/thesaurus/white_on_red/6.137>,
        <http://id.acdh.oeaw.ac.at/defc/thesaurus/white_on_red_(a3α)/6.160>,
        <http://id.acdh.oeaw.ac.at/defc/thesaurus/white_on_red_(β3α1)/6.161> ;
    skos:prefLabel "Musterbemalt"@de,
        "pattern painted"@en .

<http://id.acdh.oeaw.ac.at/defc/thesaurus/FindsMaterial> a skos:ConceptScheme ;
    rdfs:comment "A concept schema related to the particular Finds properties." .

<http://id.acdh.oeaw.ac.at/defc/thesaurus/AreaSpecialfeatures> a skos:ConceptScheme ;
    rdfs:comment "A concept schema related to the particular Area properties." .

<http://id.acdh.oeaw.ac.at/defc/thesaurus/tool/3.1> a skos:Concept ;
    dc:source "https://en.oxforddictionaries.com/definition/tool" ;
    skos:broader <http://id.acdh.oeaw.ac.at/defc/thesaurus/small_finds/2.5> ;
    skos:definition "A device or implement, especially one held in the hand, used to carry out a particular function." ;
    skos:editorialNote "dc_small_finds_category;1" ;
    skos:inScheme <http://id.acdh.oeaw.ac.at/defc/thesaurus/FindsSchema>,
        <http://id.acdh.oeaw.ac.at/defc/thesaurus/SmallFindsCategory> ;
    skos:narrower <http://id.acdh.oeaw.ac.at/defc/thesaurus/adze/4.66>,
        <http://id.acdh.oeaw.ac.at/defc/thesaurus/awl/4.87>,
        <http://id.acdh.oeaw.ac.at/defc/thesaurus/axe/4.57>,
        <http://id.acdh.oeaw.ac.at/defc/thesaurus/ball/4.120>,
        <http://id.acdh.oeaw.ac.at/defc/thesaurus/blade/4.68>,
        <http://id.acdh.oeaw.ac.at/defc/thesaurus/burnisher/4.65>,
        <http://id.acdh.oeaw.ac.at/defc/thesaurus/chipped_disk/4.134>,
        <http://id.acdh.oeaw.ac.at/defc/thesaurus/chisel/4.69>,
        <http://id.acdh.oeaw.ac.at/defc/thesaurus/coil/4.133>,
        <http://id.acdh.oeaw.ac.at/defc/thesaurus/cone/4.119>,
        <http://id.acdh.oeaw.ac.at/defc/thesaurus/crucible/4.67>,
        <http://id.acdh.oeaw.ac.at/defc/thesaurus/disc/4.63>,
        <http://id.acdh.oeaw.ac.at/defc/thesaurus/drill/4.121>,
        <http://id.acdh.oeaw.ac.at/defc/thesaurus/fire_dog/4.90>,
        <http://id.acdh.oeaw.ac.at/defc/thesaurus/fishing_object/4.027>,
        <http://id.acdh.oeaw.ac.at/defc/thesaurus/grinding_equipment/4.029>,
        <http://id.acdh.oeaw.ac.at/defc/thesaurus/grinding_stone/4.52>,
        <http://id.acdh.oeaw.ac.at/defc/thesaurus/haft/4.123>,
        <http://id.acdh.oeaw.ac.at/defc/thesaurus/hammer/4.46>,
        <http://id.acdh.oeaw.ac.at/defc/thesaurus/hoe/4.131>,
        <http://id.acdh.oeaw.ac.at/defc/thesaurus/knife/4.122>,
        <http://id.acdh.oeaw.ac.at/defc/thesaurus/knob/4.130>,
        <http://id.acdh.oeaw.ac.at/defc/thesaurus/other/4.109>,
        <http://id.acdh.oeaw.ac.at/defc/thesaurus/pickaxe/4.132>,
        <http://id.acdh.oeaw.ac.at/defc/thesaurus/pintadera/4.59>,
        <http://id.acdh.oeaw.ac.at/defc/thesaurus/scraper/4.74>,
        <http://id.acdh.oeaw.ac.at/defc/thesaurus/seal/4.62>,
        <http://id.acdh.oeaw.ac.at/defc/thesaurus/shaft_straightener/4.95>,
        <http://id.acdh.oeaw.ac.at/defc/thesaurus/sickle_implement/4.107>,
        <http://id.acdh.oeaw.ac.at/defc/thesaurus/spatula/4.55>,
        <http://id.acdh.oeaw.ac.at/defc/thesaurus/spoon/4.48>,
        <http://id.acdh.oeaw.ac.at/defc/thesaurus/tally_stick/4.100>,
        <http://id.acdh.oeaw.ac.at/defc/thesaurus/textile_equipment/4.028>,
        <http://id.acdh.oeaw.ac.at/defc/thesaurus/tip/4.101>,
        <http://id.acdh.oeaw.ac.at/defc/thesaurus/unknown/4.111>,
        <http://id.acdh.oeaw.ac.at/defc/thesaurus/weapon/4.030>,
        <http://id.acdh.oeaw.ac.at/defc/thesaurus/weight/4.112> ;
    skos:prefLabel "Werkzeug"@de,
        "tool"@en .

<http://id.acdh.oeaw.ac.at/defc/thesaurus/FindsAnimalRemainsSpecies> a skos:ConceptScheme ;
    rdfs:comment "A concept schema related to the particular Finds properties." .

<http://id.acdh.oeaw.ac.at/defc/thesaurus/BotanySpecies> a skos:ConceptScheme ;
    rdfs:comment "A concept schema related to the particular Finds properties." .

<http://id.acdh.oeaw.ac.at/defc/thesaurus/FindsPotteryForm> a skos:ConceptScheme ;
    rdfs:comment "A concept schema related to the particular Finds properties." .

<http://id.acdh.oeaw.ac.at/defc/thesaurus/FindsPotteryDetail> a skos:ConceptScheme ;
    rdfs:comment "A concept schema related to the particular Finds properties." .

<http://id.acdh.oeaw.ac.at/defc/thesaurus/ResearchEventSchema> a skos:ConceptScheme ;
    rdfs:comment "A concept schema related to the Research Event class in the database." .

<http://id.acdh.oeaw.ac.at/defc/thesaurus/NotInDatabase> a skos:ConceptScheme ;
    rdfs:comment "A concept schema for terms that are not present in the database, but are essential for hierarchy of terms related to the period (Area class)",
        "A concept schema related to the particular Area properties.",
        "A concept schema related to the particular Finds properties.",
        "A concept schema related to the particular Interpretation properties.",
        "A concept schema related to the particular Site properties.",
        "A concept schema related to the particular properties of Research Event in the database.",
        "A concept schema related to the particular properties of Research Event.",
        "A concept scheme related to the particular Research Event properties" .

<http://id.acdh.oeaw.ac.at/defc/thesaurus/FindsSmallFindsType> a skos:ConceptScheme ;
    rdfs:comment "A concept schema related to the particular Finds properties." .

<http://id.acdh.oeaw.ac.at/defc/thesaurus/FindsPotteryDecoration> a skos:ConceptScheme ;
    rdfs:comment "A concept schema related to the particular Finds properties." .

<http://id.acdh.oeaw.ac.at/defc/thesaurus/AreaSchema> a skos:ConceptScheme ;
    rdfs:comment "A concept schema related to class Area in database." .

<http://id.acdh.oeaw.ac.at/defc/thesaurus/FindsSchema> a skos:ConceptScheme ;
    rdfs:comment "A concept schema related to class Finds in database." .

